# baseURI: https://w3id.org/con-tax/components/aat-furn
# prefix: aat-furn

@prefix : <https://w3id.org/con-tax/components/aat-furn#> .
@prefix aat: <http://vocab.getty.edu/aat/> .
@prefix aat-furn: <https://w3id.org/con-tax/components/aat-furn#> .
@prefix cc: <http://creativecommons.org/ns#> .
@prefix contax: <https://w3id.org/con-tax#> .
@prefix dbr: <http://dbpedia.org/resource/> .
@prefix dct: <http://purl.org/dc/terms/> .
@prefix dcterms: <http://purl.org/dc/terms/> .
@prefix gvp: <http://vocab.getty.edu/ontology#> .
@prefix iso-thes: <http://purl.org/iso25964/skos-thes#> .
@prefix owl: <http://www.w3.org/2002/07/owl#> .
@prefix rdf: <http://www.w3.org/1999/02/22-rdf-syntax-ns#> .
@prefix rdfs: <http://www.w3.org/2000/01/rdf-schema#> .
@prefix schema: <http://schema.org/> .
@prefix skos: <http://www.w3.org/2004/02/skos/core#> .
@prefix vann: <http://purl.org/vocab/vann/> .
@prefix vcard: <http://www.w3.org/2006/vcard/ns#> .
@prefix voaf: <http://purl.org/vocommons/voaf#> .
@prefix wd: <http://www.wikidata.org/entity/> .
@prefix xl: <http://www.w3.org/2008/05/skos-xl#> .
@prefix xsd: <http://www.w3.org/2001/XMLSchema#> .

contax:ConstructionComponent
  rdf:type owl:Class ;
.
<https://w3id.org/con-tax/components/aat-furn>
  rdf:type voaf:Vocabulary ;
  rdf:type owl:Ontology ;
  cc:license <https://opendatacommons.org/licenses/by/1-0/> ;
  dcterms:creator [
      rdf:type vcard:Individual ;
      vcard:family-name "Bonduel" ;
      vcard:fn "Mathias Bonduel" ;
      vcard:given-name "Mathias" ;
      vcard:hasOrganizationName [
          rdf:type vcard:Organization ;
          owl:sameAs dbr:Katholieke_Universiteit_Leuven ;
          vcard:hasURL <https://www.kuleuven.be> ;
          vcard:organization-name "KU Leuven" ;
        ] ;
      vcard:hasURL <https://orcid.org/0000-0002-3313-924X> ;
      vcard:hasURL <https://www.kuleuven.be/wieiswie/nl/person/00110827> ;
      vcard:hasURL <https://www.researchgate.net/profile/Mathias_Bonduel> ;
    ] ;
  dcterms:description """A taxonomy of furniture construction components derived from the Getty Art & Architecture Thesaurus (Getty AAT: https://www.getty.edu/research/tools/vocabularies/aat/about.html), v2020-07-29.

Note: Contains information from the J. Paul Getty Trust, Getty Research Institute, the Art & Architecture Thesaurus, which is made available under the ODC Attribution License."""@en ;
  dcterms:issued "2020-11-29"^^xsd:date ;
  dcterms:title "AAT-FURN taxonomy"@en ;
  vann:preferredNamespacePrefix "aat-furn" ;
  vann:preferredNamespaceUri "https://w3id.org/con-tax/components/aat-furn#" ;
  rdfs:comment "- Version 0.0.1: initial version"@en ;
  owl:versionInfo "0.0.1" ;
.
<https://w3id.org/con-tax/components/aat-furn#300003784>
  rdf:type owl:Class ;
  rdfs:comment "Schermen in oosters-orthodoxe kerken die het heiligdom van het schip scheiden, waar meestal drie deuren in zitten en die sinds de veertiende of vijftiende eeuw bedekt zijn met iconen."@nl ;
  rdfs:comment "Screens in Eastern Orthodox and Catholic churches that separate the sanctuary from the nave, usually pierced by three doors and, since the 14th or 15th century, covered with icons. The function of the iconostasis is modeled on the Temple in Jerusalem, where people other than the priests were separated from the holiest area."@en ;
  rdfs:isDefinedBy <https://w3id.org/con-tax/components/aat-furn> ;
  rdfs:label "iconostase"@nl ;
  rdfs:label "iconostasen"@nl ;
  rdfs:label "iconostases"@en ;
  rdfs:seeAlso <http://vocab.getty.edu/aat/300003784> ;
  rdfs:seeAlso wd:Q193073 ;
  rdfs:subClassOf <https://w3id.org/con-tax/components/aat-furn#300037737> ;
.
<https://w3id.org/con-tax/components/aat-furn#300008734>
  rdf:type owl:Class ;
  rdfs:comment "Generally used either for the lines forming boundaries between land and sea or specifically for the lines reached by the highest storm waves or the high-water marks of median tides; for strips of land bordering any large bodies of water, use \"shores (landforms).\""@en ;
  rdfs:comment "Wordt meestal gebruikt voor de lijnen die de grens vormen tussen de zee en het vasteland, maar soms ook specifiek voor het niveau dat de hoogste stormgolven bereiken of de hoogwaterstanden van het gemiddeld getij; gebruik `oevers (aardoppervlakten)' voor stroken land die aan grote watermassa's grenzen."@nl ;
  rdfs:isDefinedBy <https://w3id.org/con-tax/components/aat-furn> ;
  rdfs:label "coastlines"@en-us ;
  rdfs:label "kustlijn"@nl ;
  rdfs:label "kustlijnen"@nl ;
  rdfs:seeAlso <http://vocab.getty.edu/aat/300008734> ;
  rdfs:subClassOf <https://w3id.org/con-tax/components/aat-furn#300039009> ;
.
<https://w3id.org/con-tax/components/aat-furn#300022862>
  rdf:type owl:Class ;
  rdfs:comment "Stands of various designs for supporting one or more pipes."@en ;
  rdfs:isDefinedBy <https://w3id.org/con-tax/components/aat-furn> ;
  rdfs:label "pipe stands"@en ;
  rdfs:seeAlso <http://vocab.getty.edu/aat/300022862> ;
  rdfs:subClassOf <https://w3id.org/con-tax/components/aat-furn#300039767> ;
.
<https://w3id.org/con-tax/components/aat-furn#300037680>
  rdf:type owl:Class ;
  rdfs:comment "Movable or fixed objects or equipment, which may be either functional or ornamental, particularly objects for sitting, reclining, or storage, such as chairs, beds, tables, cabinets, etc.,  in a dwelling, business, or public space."@en ;
  rdfs:isDefinedBy <https://w3id.org/con-tax/components/aat-furn> ;
  rdfs:label "furniture"@en ;
  rdfs:label "meubilair"@nl ;
  rdfs:seeAlso <http://vocab.getty.edu/aat/300037680> ;
  rdfs:seeAlso wd:Q14745 ;
  rdfs:subClassOf contax:ConstructionComponent ;
  contax:containsGuideTerm <https://w3id.org/con-tax/components/aat-furn#300040026> ;
  contax:containsGuideTerm <https://w3id.org/con-tax/components/aat-furn#300040132> ;
  contax:containsGuideTerm <https://w3id.org/con-tax/components/aat-furn#300048628> ;
  contax:containsGuideTerm <https://w3id.org/con-tax/components/aat-furn#300136953> ;
.
<https://w3id.org/con-tax/components/aat-furn#300037709>
  rdf:type owl:Class ;
  rdfs:comment "Kleine, vrijstaande spiegels,  meestal in een rechtopstaande omlijsting waarbinnen de spiegel kan worden versteld. Ze zijn bedoeld voor gebruik op de toilettafel en hebben soms een doosachtig onderstuk met kleine laatjes."@nl ;
  rdfs:comment "Small freestanding mirrors, usually supported on a standing frame within which the glass can be adjusted, designed to be used on a dressing table. Dressing glasses are sometimes made with a boxlike base fitted with small drawers."@en ;
  rdfs:isDefinedBy <https://w3id.org/con-tax/components/aat-furn> ;
  rdfs:label "dressing glasses"@en ;
  rdfs:label "toiletspiegel"@nl ;
  rdfs:label "toiletspiegels"@nl ;
  rdfs:seeAlso <http://vocab.getty.edu/aat/300037709> ;
  rdfs:subClassOf <https://w3id.org/con-tax/components/aat-furn#300039767> ;
.
<https://w3id.org/con-tax/components/aat-furn#300037737>
  rdf:type owl:Class ;
  rdfs:comment "Refers to furniture or built-in features in the form of an upright partition that can be used to embellish, partition, shelter, and provide privacy. Screens are often highly decorated."@en ;
  rdfs:comment "Verwijst naar meubilair in de vorm van een staande scheidingswand die kan worden gebruikt om een ruimte te verfraaien, af te scheiden of af te schermen, of om privacy te waarborgen. Schermen zijn vaak rijk gedecoreerd."@nl ;
  rdfs:isDefinedBy <https://w3id.org/con-tax/components/aat-furn> ;
  rdfs:label "scherm (meubilair)"@nl ;
  rdfs:label "scherm"@nl ;
  rdfs:label "schermen (meubilair)"@nl ;
  rdfs:label "schermen"@nl ;
  rdfs:label "screens (furniture)"@en ;
  rdfs:seeAlso <http://vocab.getty.edu/aat/300037737> ;
  rdfs:subClassOf <https://w3id.org/con-tax/components/aat-furn#300037680> ;
  contax:containsGuideTerm <https://w3id.org/con-tax/components/aat-furn#300265151> ;
.
<https://w3id.org/con-tax/components/aat-furn#300037741>
  rdf:type owl:Class ;
  rdfs:comment "Kleine schermen die worden gebruikt om brandende kaarsen mee te beschermen. Ze werden gemaakt in de 18e eeuw."@nl ;
  rdfs:comment "Small 18th-century screens used to protect lighted candles."@en ;
  rdfs:isDefinedBy <https://w3id.org/con-tax/components/aat-furn> ;
  rdfs:label "candle screens"@en ;
  rdfs:label "kaarsenscherm"@nl ;
  rdfs:label "kaarsenschermen"@nl ;
  rdfs:seeAlso <http://vocab.getty.edu/aat/300037741> ;
  rdfs:subClassOf <https://w3id.org/con-tax/components/aat-furn#300037737> ;
.
<https://w3id.org/con-tax/components/aat-furn#300037744>
  rdf:type owl:Class ;
  rdfs:comment "Firescreens with a shelf or slide attached, to be used for writing before the fire."@en ;
  rdfs:comment "Vuurschermen waaraan een plank of schuif is bevestigd om op te schrijven bij het haardvuur."@nl ;
  rdfs:isDefinedBy <https://w3id.org/con-tax/components/aat-furn> ;
  rdfs:label "écran à secrétaire"@nl ;
  rdfs:label "écrans à secrétaire"@en ;
  rdfs:label "écrans à secrétaire"@nl ;
  rdfs:seeAlso <http://vocab.getty.edu/aat/300037744> ;
  rdfs:subClassOf <https://w3id.org/con-tax/components/aat-furn#300172148> ;
.
<https://w3id.org/con-tax/components/aat-furn#300037745>
  rdf:type owl:Class ;
  rdfs:comment "Schermen die worden gebruikt om het gezicht of de benen tegen het vuur te beschermen. Vaak met gedecoreerd paneel of panelen."@nl ;
  rdfs:comment "Screens used to shelter the face or legs from the full heat of a fire in a fireplace. May include a decorated panel or panels, often set into a decorative wooden furniture structure that can be moved for the convenience of the sitter. For nonflammable metal screens placed directly in front of fireplace openings to prevent logs and sparks from escaping, use \"fire screens (equipment).\""@en ;
  rdfs:isDefinedBy <https://w3id.org/con-tax/components/aat-furn> ;
  rdfs:label "fire screens (furniture)"@en ;
  rdfs:label "haardschermen"@nl ;
  rdfs:label "vuurscherm (meubilair)"@nl ;
  rdfs:label "vuurscherm"@nl ;
  rdfs:label "vuurschermen (meubilair)"@nl ;
  rdfs:label "vuurschermen"@nl ;
  rdfs:seeAlso <http://vocab.getty.edu/aat/300037745> ;
  rdfs:subClassOf <https://w3id.org/con-tax/components/aat-furn#300037737> ;
.
<https://w3id.org/con-tax/components/aat-furn#300037747>
  rdf:type owl:Class ;
  rdfs:comment "Fire screens with a panel set between two standards or a frame, on four legs; distinguished from \"pole screens\" which have a tripod base and shaft which supports the fire screen."@en ;
  rdfs:comment "Vuurscherm met een schuifpaneel dat tussen twee houders op vier poten staat. Te onderscheiden van 'pole screens', waarbij het scherm wordt ondersteund door een drievoetige sokkel met schacht."@nl ;
  rdfs:isDefinedBy <https://w3id.org/con-tax/components/aat-furn> ;
  rdfs:label "cheval fire screen"@nl ;
  rdfs:label "cheval fire screens"@en ;
  rdfs:label "cheval fire screens"@nl ;
  rdfs:seeAlso <http://vocab.getty.edu/aat/300037747> ;
  rdfs:subClassOf <https://w3id.org/con-tax/components/aat-furn#300037745> ;
.
<https://w3id.org/con-tax/components/aat-furn#300037748>
  rdf:type owl:Class ;
  rdfs:comment "Fire screens of various designs, characterized by being adjustable or extendable to cover alternatively a smaller or largerspace as necessary."@en ;
  rdfs:isDefinedBy <https://w3id.org/con-tax/components/aat-furn> ;
  rdfs:label "extension fire screen"@nl ;
  rdfs:label "extension fire screens"@en ;
  rdfs:label "extension fire screens"@nl ;
  rdfs:seeAlso <http://vocab.getty.edu/aat/300037748> ;
  rdfs:subClassOf <https://w3id.org/con-tax/components/aat-furn#300037745> ;
.
<https://w3id.org/con-tax/components/aat-furn#300037749>
  rdf:type owl:Class ;
  rdfs:comment "Fire screens designed with two hinged leaves."@en ;
  rdfs:comment "Vuurschermen die met twee scharnierende bladen zijn ontworpen."@nl ;
  rdfs:isDefinedBy <https://w3id.org/con-tax/components/aat-furn> ;
  rdfs:label "folding fire screens"@en ;
  rdfs:label "vouwbaar haardscherm"@nl ;
  rdfs:label "vouwbare haardschermen"@nl ;
  rdfs:seeAlso <http://vocab.getty.edu/aat/300037749> ;
  rdfs:subClassOf <https://w3id.org/con-tax/components/aat-furn#300037745> ;
  rdfs:subClassOf <https://w3id.org/con-tax/components/aat-furn#300265156> ;
.
<https://w3id.org/con-tax/components/aat-furn#300037752>
  rdf:type owl:Class ;
  rdfs:comment "Firescreens with a tripod base and an upright shaft which supports the framed panel; distinguished from \"cheval fire screens\" which are supported on four legs."@en ;
  rdfs:comment "Vuurschermen met een drievoetige sokkel en een rechtopstaande schacht die het omlijste paneel ondersteunen. Te onderscheiden  van 'cheval fire screens' die door vier poten worden ondersteund."@nl ;
  rdfs:isDefinedBy <https://w3id.org/con-tax/components/aat-furn> ;
  rdfs:label "pole screen"@nl ;
  rdfs:label "pole screens"@en ;
  rdfs:label "pole screens"@nl ;
  rdfs:seeAlso <http://vocab.getty.edu/aat/300037752> ;
  rdfs:subClassOf <https://w3id.org/con-tax/components/aat-furn#300037745> ;
.
<https://w3id.org/con-tax/components/aat-furn#300037758>
  rdf:type owl:Class ;
  rdfs:comment "Fire screens supported upon a stand and designed so that the panels may be moved or extended by means of sliding the panels on a pole (a pole screen) or in a frame (a cheval screen)."@en ;
  rdfs:comment "Historische term voor vuurschermen uit de 18e eeuw die op een houder steunen en door schuifpanelen kunnen worden verlengd."@nl ;
  rdfs:isDefinedBy <https://w3id.org/con-tax/components/aat-furn> ;
  rdfs:label "sliding fire screen"@nl ;
  rdfs:label "sliding fire screens (furniture)"@en ;
  rdfs:label "sliding fire screens"@nl ;
  rdfs:seeAlso <http://vocab.getty.edu/aat/300037758> ;
  rdfs:subClassOf <https://w3id.org/con-tax/components/aat-furn#300037745> ;
.
<https://w3id.org/con-tax/components/aat-furn#300037769>
  rdf:type owl:Class ;
  rdfs:comment "General term for any furniture intended for seating."@en ;
  rdfs:isDefinedBy <https://w3id.org/con-tax/components/aat-furn> ;
  rdfs:label "seating furniture"@en ;
  rdfs:label "zitmeubel"@nl ;
  rdfs:label "zitmeubels"@nl ;
  rdfs:seeAlso <http://vocab.getty.edu/aat/300037769> ;
  rdfs:seeAlso wd:Q2731419 ;
  rdfs:subClassOf <https://w3id.org/con-tax/components/aat-furn#300037680> ;
  contax:containsGuideTerm <https://w3id.org/con-tax/components/aat-furn#300435629> ;
.
<https://w3id.org/con-tax/components/aat-furn#300037771>
  rdf:type owl:Class ;
  rdfs:comment "Seating furniture produced for use by one person. "@en ;
  rdfs:isDefinedBy <https://w3id.org/con-tax/components/aat-furn> ;
  rdfs:label "eenpersoonszitmeubels"@nl ;
  rdfs:label "single seating furniture"@en ;
  rdfs:seeAlso <http://vocab.getty.edu/aat/300037771> ;
  rdfs:subClassOf <https://w3id.org/con-tax/components/aat-furn#300037769> ;
.
<https://w3id.org/con-tax/components/aat-furn#300037772>
  rdf:type owl:Class ;
  rdfs:comment "Seats for one person with a back or a back and arms. Distinct from \"stools\" which have no back."@en ;
  rdfs:comment "Zitplaats voor één persoon met een rugleuning of een rug- en armleuning. Ze verschillen van 'krukken' die geen rug hebben."@nl ;
  rdfs:isDefinedBy <https://w3id.org/con-tax/components/aat-furn> ;
  rdfs:label "chairs (furniture forms)"@en ;
  rdfs:label "stoel"@nl ;
  rdfs:label "stoelen"@nl ;
  rdfs:seeAlso <http://vocab.getty.edu/aat/300037772> ;
  rdfs:seeAlso wd:Q15026 ;
  rdfs:subClassOf <https://w3id.org/con-tax/components/aat-furn#300037771> ;
  contax:containsGuideTerm <https://w3id.org/con-tax/components/aat-furn#300037775> ;
  contax:containsGuideTerm <https://w3id.org/con-tax/components/aat-furn#300038131> ;
  contax:containsGuideTerm <https://w3id.org/con-tax/components/aat-furn#300038257> ;
  contax:containsGuideTerm <https://w3id.org/con-tax/components/aat-furn#300137711> ;
.
<https://w3id.org/con-tax/components/aat-furn#300037775>
  rdf:type gvp:GuideTerm ;
  rdfs:isDefinedBy <https://w3id.org/con-tax/components/aat-furn> ;
  rdfs:label "<chairs by form>"@en ;
  rdfs:label "<stoel naar vorm>"@nl ;
  rdfs:label "<stoelen naar vorm>"@nl ;
  rdfs:label "stoel naar vorm"@nl ;
  rdfs:label "stoelen naar vorm"@nl ;
  rdfs:seeAlso <http://vocab.getty.edu/aat/300037775> ;
  contax:containsConcept <https://w3id.org/con-tax/components/aat-furn#300037776> ;
  contax:containsConcept <https://w3id.org/con-tax/components/aat-furn#300037784> ;
  contax:containsConcept <https://w3id.org/con-tax/components/aat-furn#300037789> ;
  contax:containsConcept <https://w3id.org/con-tax/components/aat-furn#300037798> ;
  contax:containsConcept <https://w3id.org/con-tax/components/aat-furn#300037800> ;
  contax:containsConcept <https://w3id.org/con-tax/components/aat-furn#300037819> ;
  contax:containsConcept <https://w3id.org/con-tax/components/aat-furn#300037824> ;
  contax:containsConcept <https://w3id.org/con-tax/components/aat-furn#300037825> ;
  contax:containsConcept <https://w3id.org/con-tax/components/aat-furn#300037830> ;
  contax:containsConcept <https://w3id.org/con-tax/components/aat-furn#300037833> ;
  contax:containsConcept <https://w3id.org/con-tax/components/aat-furn#300037834> ;
  contax:containsConcept <https://w3id.org/con-tax/components/aat-furn#300037838> ;
  contax:containsConcept <https://w3id.org/con-tax/components/aat-furn#300037861> ;
  contax:containsConcept <https://w3id.org/con-tax/components/aat-furn#300037865> ;
  contax:containsConcept <https://w3id.org/con-tax/components/aat-furn#300037867> ;
  contax:containsConcept <https://w3id.org/con-tax/components/aat-furn#300037874> ;
  contax:containsConcept <https://w3id.org/con-tax/components/aat-furn#300037896> ;
  contax:containsConcept <https://w3id.org/con-tax/components/aat-furn#300037904> ;
  contax:containsConcept <https://w3id.org/con-tax/components/aat-furn#300038088> ;
  contax:containsConcept <https://w3id.org/con-tax/components/aat-furn#300038126> ;
  contax:containsConcept <https://w3id.org/con-tax/components/aat-furn#300038128> ;
  contax:containsConcept <https://w3id.org/con-tax/components/aat-furn#300038148> ;
  contax:containsConcept <https://w3id.org/con-tax/components/aat-furn#300038151> ;
  contax:containsConcept <https://w3id.org/con-tax/components/aat-furn#300038220> ;
  contax:containsConcept <https://w3id.org/con-tax/components/aat-furn#300038225> ;
  contax:containsConcept <https://w3id.org/con-tax/components/aat-furn#300077250> ;
  contax:containsConcept <https://w3id.org/con-tax/components/aat-furn#300077252> ;
  contax:containsConcept <https://w3id.org/con-tax/components/aat-furn#300121145> ;
  contax:containsConcept <https://w3id.org/con-tax/components/aat-furn#300121151> ;
  contax:containsConcept <https://w3id.org/con-tax/components/aat-furn#300121196> ;
  contax:containsConcept <https://w3id.org/con-tax/components/aat-furn#300133763> ;
  contax:containsConcept <https://w3id.org/con-tax/components/aat-furn#300133811> ;
  contax:containsConcept <https://w3id.org/con-tax/components/aat-furn#300138142> ;
  contax:containsConcept <https://w3id.org/con-tax/components/aat-furn#300140010> ;
  contax:containsConcept <https://w3id.org/con-tax/components/aat-furn#300144135> ;
  contax:containsConcept <https://w3id.org/con-tax/components/aat-furn#300164655> ;
  contax:containsConcept <https://w3id.org/con-tax/components/aat-furn#300165324> ;
  contax:containsConcept <https://w3id.org/con-tax/components/aat-furn#300165855> ;
  contax:containsConcept <https://w3id.org/con-tax/components/aat-furn#300167589> ;
  contax:containsConcept <https://w3id.org/con-tax/components/aat-furn#300170152> ;
  contax:containsConcept <https://w3id.org/con-tax/components/aat-furn#300170221> ;
  contax:containsConcept <https://w3id.org/con-tax/components/aat-furn#300170227> ;
  contax:containsConcept <https://w3id.org/con-tax/components/aat-furn#300170233> ;
  contax:containsConcept <https://w3id.org/con-tax/components/aat-furn#300170239> ;
  contax:containsConcept <https://w3id.org/con-tax/components/aat-furn#300170242> ;
  contax:containsConcept <https://w3id.org/con-tax/components/aat-furn#300170245> ;
  contax:containsConcept <https://w3id.org/con-tax/components/aat-furn#300170256> ;
  contax:containsConcept <https://w3id.org/con-tax/components/aat-furn#300170262> ;
  contax:containsConcept <https://w3id.org/con-tax/components/aat-furn#300170271> ;
  contax:containsConcept <https://w3id.org/con-tax/components/aat-furn#300170285> ;
  contax:containsConcept <https://w3id.org/con-tax/components/aat-furn#300170291> ;
  contax:containsConcept <https://w3id.org/con-tax/components/aat-furn#300170297> ;
  contax:containsConcept <https://w3id.org/con-tax/components/aat-furn#300170301> ;
  contax:containsConcept <https://w3id.org/con-tax/components/aat-furn#300170305> ;
  contax:containsConcept <https://w3id.org/con-tax/components/aat-furn#300171674> ;
  contax:containsConcept <https://w3id.org/con-tax/components/aat-furn#300265223> ;
  contax:containsConcept <https://w3id.org/con-tax/components/aat-furn#300266583> ;
  contax:containsConcept <https://w3id.org/con-tax/components/aat-furn#300312264> ;
  contax:containsGuideTerm <https://w3id.org/con-tax/components/aat-furn#300037920> ;
.
<https://w3id.org/con-tax/components/aat-furn#300037776>
  rdf:type owl:Class ;
  rdfs:comment "Term applied to a wide variety of chairs with arms, to distinguish them from side chairs which have no arms."@en ;
  rdfs:comment "Term die wordt gebruikt voor een groot assortiment stoelen met armleuningen om ze te onderscheiden van 'stoelen zonder armleuningen' die geen armleuningen hebben."@nl ;
  rdfs:isDefinedBy <https://w3id.org/con-tax/components/aat-furn> ;
  rdfs:label "armchairs"@en ;
  rdfs:label "leunstoel"@nl ;
  rdfs:label "leunstoelen"@nl ;
  rdfs:seeAlso <http://vocab.getty.edu/aat/300037776> ;
  rdfs:seeAlso wd:Q25503439 ;
  rdfs:subClassOf <https://w3id.org/con-tax/components/aat-furn#300037772> ;
.
<https://w3id.org/con-tax/components/aat-furn#300037784>
  rdf:type owl:Class ;
  rdfs:comment "Armchairs with adjustable backs and loose cushions, of a type first produced by William Morris, Philip Webb, and the firm Morris, Marshall, Faulkner and Co. about 1866 in England."@en ;
  rdfs:comment "Leunstoelen met verstelbare rugleuningen en losse kussens. Dit type is als eerst gemaakt in 1866 in Engeland door William Morris, Philip Webb en de firma Morris, Marshall, Faulkner and Co."@nl ;
  rdfs:isDefinedBy <https://w3id.org/con-tax/components/aat-furn> ;
  rdfs:label "Morris chairs"@en ;
  rdfs:label "Morrisstoel"@nl ;
  rdfs:label "Morrisstoelen"@nl ;
  rdfs:seeAlso <http://vocab.getty.edu/aat/300037784> ;
  rdfs:seeAlso wd:Q12062043 ;
  rdfs:subClassOf <https://w3id.org/con-tax/components/aat-furn#300037772> ;
  rdfs:subClassOf <https://w3id.org/con-tax/components/aat-furn#300037776> ;
.
<https://w3id.org/con-tax/components/aat-furn#300037789>
  rdf:type owl:Class ;
  rdfs:comment "Chairs in the form of a four-legged stool to which a back has been added. The term first appeared in the 16th century and was sometimes used in the 17th and 18th centuries for a chair without arms."@en ;
  rdfs:comment "Stoelen in de vorm van een krukje met vier poten waar een rugleuning aan is gezet. De term werd voor het eerst gebruikt in de 16e eeuw en in de 17e en 18e eeuw werd er ook wel een stoel zonder armleuningen mee aangeduid."@nl ;
  rdfs:isDefinedBy <https://w3id.org/con-tax/components/aat-furn> ;
  rdfs:label "backstools"@en ;
  rdfs:label "schamel"@nl ;
  rdfs:label "schamels"@nl ;
  rdfs:label "schemel"@nl ;
  rdfs:label "schemels"@nl ;
  rdfs:seeAlso <http://vocab.getty.edu/aat/300037789> ;
  rdfs:seeAlso wd:Q21550379 ;
  rdfs:subClassOf <https://w3id.org/con-tax/components/aat-furn#300037772> ;
.
<https://w3id.org/con-tax/components/aat-furn#300037798>
  rdf:type owl:Class ;
  rdfs:comment "Chairs with a solid, rounded wood back, the cruder type being made by cutting away parts of a barrel. For easy chairs having a semicircular back, use \"circular easy chairs.\""@en ;
  rdfs:comment "Stoelen met een stevige, ronde houten rug, waarbij de grovere soort werd gemaakt door het wegsnijden van delen van een vat. Voor luie stoelen met een halfronde rug gebruik 'ronde luie stoelen'."@nl ;
  rdfs:isDefinedBy <https://w3id.org/con-tax/components/aat-furn> ;
  rdfs:label "barrel chairs (rounded wood-backed chairs)"@en ;
  rdfs:label "tonstoel"@nl ;
  rdfs:label "tonstoelen (stoelen naar vorm)"@nl ;
  rdfs:label "tonstoelen"@nl ;
  rdfs:seeAlso <http://vocab.getty.edu/aat/300037798> ;
  rdfs:subClassOf <https://w3id.org/con-tax/components/aat-furn#300037772> ;
.
<https://w3id.org/con-tax/components/aat-furn#300037800>
  rdf:type owl:Class ;
  rdfs:comment "Grote, zachte stoelen zonder frame die op een zak met bonen lijken en meestal bestaan uit een zak van een soort stofachtig plastic dat met stukjes plastic wordt gevuld. Ze vormen zich gemakkelijk naar de omtrek van de zittende persoon."@nl ;
  rdfs:comment "Large, soft frameless chairs resembling a beanbag; typically a clothlike plastic shell filled with plastic chips, that molds itself readily to the contour of the occupant."@en ;
  rdfs:isDefinedBy <https://w3id.org/con-tax/components/aat-furn> ;
  rdfs:label "beanbag chairs"@en ;
  rdfs:label "zitzak"@nl ;
  rdfs:label "zitzakken"@nl ;
  rdfs:seeAlso <http://vocab.getty.edu/aat/300037800> ;
  rdfs:subClassOf <https://w3id.org/con-tax/components/aat-furn#300037772> ;
.
<https://w3id.org/con-tax/components/aat-furn#300037801>
  rdf:type owl:Class ;
  rdfs:comment "Gestoffeerde leunstoelen die verschillen van andere leunstoelen omdat ze tussen de armleuning en de zitting zijn gestoffeerd."@nl ;
  rdfs:comment "Upholstered armchairs, differing from other armchairs in being upholstered between the arms and seats."@en ;
  rdfs:isDefinedBy <https://w3id.org/con-tax/components/aat-furn> ;
  rdfs:label "bergère (stoel)"@nl ;
  rdfs:label "bergère"@nl ;
  rdfs:label "bergères (armchairs)"@en ;
  rdfs:label "bergères (stoelen)"@nl ;
  rdfs:label "bergères"@nl ;
  rdfs:seeAlso <http://vocab.getty.edu/aat/300037801> ;
  rdfs:subClassOf <https://w3id.org/con-tax/components/aat-furn#300037776> ;
.
<https://w3id.org/con-tax/components/aat-furn#300037809>
  rdf:type owl:Class ;
  rdfs:comment "Grote, diepe leunstoelen met zijleuningen en oren."@nl ;
  rdfs:comment "Large, deep armchairs with sides and wings."@en ;
  rdfs:isDefinedBy <https://w3id.org/con-tax/components/aat-furn> ;
  rdfs:label "bergère en confessional"@nl ;
  rdfs:label "bergères en confessional"@en ;
  rdfs:label "bergères en confessional"@nl ;
  rdfs:seeAlso <http://vocab.getty.edu/aat/300037809> ;
  rdfs:subClassOf <https://w3id.org/con-tax/components/aat-furn#300037838> ;
.
<https://w3id.org/con-tax/components/aat-furn#300037813>
  rdf:type owl:Class ;
  rdfs:comment "Bergères met een vlakke rugleuning. Te onderscheiden van bergères met een holle rugleuning die 'bergères en cabriolet' worden genoemd."@nl ;
  rdfs:comment "Bergères with flat backs; distinct from bergères with concave backs, which are called \"bergères en cabriolet.\""@en ;
  rdfs:isDefinedBy <https://w3id.org/con-tax/components/aat-furn> ;
  rdfs:label "bergère à la reine"@nl ;
  rdfs:label "bergères à la reine"@en ;
  rdfs:label "bergères à la reine"@nl ;
  rdfs:seeAlso <http://vocab.getty.edu/aat/300037813> ;
  rdfs:subClassOf <https://w3id.org/con-tax/components/aat-furn#300133822> ;
.
<https://w3id.org/con-tax/components/aat-furn#300037814>
  rdf:type owl:Class ;
  rdfs:comment "Bergères met een holle rugleuning. Ze verschillen van bergères met een vlakke rugleuning die 'bergères à la reine' worden genoemd."@nl ;
  rdfs:comment "Bergères with concave backs; distinct from bergères with flat backs, which are called \"bergères à la reine.\""@en ;
  rdfs:isDefinedBy <https://w3id.org/con-tax/components/aat-furn> ;
  rdfs:label "bergère en cabriolet"@nl ;
  rdfs:label "bergères en cabriolet"@en ;
  rdfs:label "bergères en cabriolet"@nl ;
  rdfs:seeAlso <http://vocab.getty.edu/aat/300037814> ;
  rdfs:subClassOf <https://w3id.org/con-tax/components/aat-furn#300174701> ;
.
<https://w3id.org/con-tax/components/aat-furn#300037815>
  rdf:type owl:Class ;
  rdfs:comment "Stoelen met een U-vorm waarvan de bovenste rand van de rugleuning met een lichte boog naar de armleuningen afloopt. Ze kenden hun grootste populariteit tijdens de periode van Louis XV."@nl ;
  rdfs:comment "U-shaped armchairs, the upper rail of the back gently sloping down to the arms. Most popular during the Louis XV period."@en ;
  rdfs:isDefinedBy <https://w3id.org/con-tax/components/aat-furn> ;
  rdfs:label "bergère en gondole"@nl ;
  rdfs:label "bergères en gondole"@en ;
  rdfs:label "bergères en gondole"@nl ;
  rdfs:seeAlso <http://vocab.getty.edu/aat/300037815> ;
  rdfs:subClassOf <https://w3id.org/con-tax/components/aat-furn#300037861> ;
.
<https://w3id.org/con-tax/components/aat-furn#300037819>
  rdf:type owl:Class ;
  rdfs:comment "Chairs with a stuffed oval or cartouche-shaped back; of a type popular in the late 18th century."@en ;
  rdfs:comment "Stoelen met een opgevulde ovale of cartouchevormige rug. Dit type kwam veel voor aan het eind van de 18e eeuw."@nl ;
  rdfs:isDefinedBy <https://w3id.org/con-tax/components/aat-furn> ;
  rdfs:label "cabriole chairs"@en ;
  rdfs:label "cabriolestoel"@nl ;
  rdfs:label "cabriolestoelen"@nl ;
  rdfs:seeAlso <http://vocab.getty.edu/aat/300037819> ;
  rdfs:subClassOf <https://w3id.org/con-tax/components/aat-furn#300037772> ;
.
<https://w3id.org/con-tax/components/aat-furn#300037824>
  rdf:type owl:Class ;
  rdfs:comment "Kleine, lage leunstoelen of schemels die vaak zijn gestoffeerd en een brede voorkant, een zeer smalle achterkant en een trapezoïde zitting hebben."@nl ;
  rdfs:comment "Small, low armchairs, or backstools, often upholstered, which have a wide front, a very narrow back, and a trapezoidal seat."@en ;
  rdfs:isDefinedBy <https://w3id.org/con-tax/components/aat-furn> ;
  rdfs:label "caquetoire"@nl ;
  rdfs:label "caquetoires"@en ;
  rdfs:label "caquetoires"@nl ;
  rdfs:label "praatstoel"@nl ;
  rdfs:label "praatstoelen"@nl ;
  rdfs:seeAlso <http://vocab.getty.edu/aat/300037824> ;
  rdfs:seeAlso wd:Q2937736 ;
  rdfs:subClassOf <https://w3id.org/con-tax/components/aat-furn#300037772> ;
  rdfs:subClassOf <https://w3id.org/con-tax/components/aat-furn#300037789> ;
.
<https://w3id.org/con-tax/components/aat-furn#300037825>
  rdf:type owl:Class ;
  rdfs:comment "Heavily upholstered chairs having solid sides and low backs."@en ;
  rdfs:comment "Zwaar gestoffeerde stoelen die zijn uitgerust met massieve zijkanten en lage rugleuningen."@nl ;
  rdfs:isDefinedBy <https://w3id.org/con-tax/components/aat-furn> ;
  rdfs:label "club chairs"@en ;
  rdfs:label "clubstoel"@nl ;
  rdfs:label "clubstoelen"@nl ;
  rdfs:seeAlso <http://vocab.getty.edu/aat/300037825> ;
  rdfs:seeAlso wd:Q458771 ;
  rdfs:subClassOf <https://w3id.org/con-tax/components/aat-furn#300037772> ;
.
<https://w3id.org/con-tax/components/aat-furn#300037830>
  rdf:type owl:Class ;
  rdfs:comment "Franse leunstoelen waarvan de rugleuning in het midden naar beneden buigt zodat het haar kan worden verzorgd."@nl ;
  rdfs:comment "French armchairs with the crest rail curving downward in the center to enable the hair to be dressed."@en ;
  rdfs:isDefinedBy <https://w3id.org/con-tax/components/aat-furn> ;
  rdfs:label "coiffeuse (stoel)"@nl ;
  rdfs:label "coiffeuse"@nl ;
  rdfs:label "coiffeuses (chairs)"@en ;
  rdfs:label "coiffeuses (stoelen)"@nl ;
  rdfs:label "coiffeuses"@nl ;
  rdfs:seeAlso <http://vocab.getty.edu/aat/300037830> ;
  rdfs:subClassOf <https://w3id.org/con-tax/components/aat-furn#300037772> ;
.
<https://w3id.org/con-tax/components/aat-furn#300037833>
  rdf:type owl:Class ;
  rdfs:comment "Heavily upholstered low armchairs, generally with fringe hiding the legs and woodwork; of a type first made in France in the 1840s."@en ;
  rdfs:comment "Zwaar gestoffeerde, lage leunstoelen waarbij een franje meestal de poten en het houtwerk verbergt. Dit type werd geïntroduceerd in Frankrijk  in de jaren veertig van de 19e eeuw."@nl ;
  rdfs:isDefinedBy <https://w3id.org/con-tax/components/aat-furn> ;
  rdfs:label "crapaud"@nl ;
  rdfs:label "crapauds"@en ;
  rdfs:label "crapauds"@nl ;
  rdfs:seeAlso <http://vocab.getty.edu/aat/300037833> ;
  rdfs:seeAlso wd:Q287792 ;
  rdfs:subClassOf <https://w3id.org/con-tax/components/aat-furn#300037772> ;
.
<https://w3id.org/con-tax/components/aat-furn#300037834>
  rdf:type owl:Class ;
  rdfs:comment "Benaming die door verzamelaars wordt gebruikt voor rechthoekige stoelen met een lage rugleuning en vaak zonder armleuning. Ze hebben gedraaide poten en dwarsbalken. Dit type is bedekt met leer of marokijn en stamt uit een periode van ver voor Cromwell, maar werd zeer populair in Engeland in het midden van de 16e eeuw."@nl ;
  rdfs:comment "Collector's term for square low-back chairs, often without arms, having turned legs and stretchers; this type, covered in leather or turkey work, long antedated the period of Cromwell but became widely popular in England in the mid-1600s."@en ;
  rdfs:isDefinedBy <https://w3id.org/con-tax/components/aat-furn> ;
  rdfs:label "Cromwellian chairs"@en ;
  rdfs:label "Cromwellstoel"@nl ;
  rdfs:label "Cromwellstoelen"@nl ;
  rdfs:seeAlso <http://vocab.getty.edu/aat/300037834> ;
  rdfs:subClassOf <https://w3id.org/con-tax/components/aat-furn#300037772> ;
.
<https://w3id.org/con-tax/components/aat-furn#300037837>
  rdf:type owl:Class ;
  rdfs:comment "Chairs usually with arms and having full-length leg rests, designed for lounging outdoors. Use \"chaises longues\" for similar forms used indoors."@en ;
  rdfs:comment "Stoelen met meestal armleuningen en met steun over de volle lengte van de benen. Ontworpen om buiten te relaxen. Gebruik \"chaises longues\" voor soortgelijke vormen voor gebruik binnenshuis."@nl ;
  rdfs:isDefinedBy <https://w3id.org/con-tax/components/aat-furn> ;
  rdfs:label "deck chairs"@en ;
  rdfs:label "dekstoel (buitenmeubel)"@nl ;
  rdfs:label "dekstoel"@nl ;
  rdfs:label "dekstoelen (buitenmeubels)"@nl ;
  rdfs:label "dekstoelen"@nl ;
  rdfs:seeAlso <http://vocab.getty.edu/aat/300037837> ;
  rdfs:seeAlso wd:Q1824203 ;
  rdfs:subClassOf <https://w3id.org/con-tax/components/aat-furn#300037772> ;
  rdfs:subClassOf <https://w3id.org/con-tax/components/aat-furn#300165810> ;
.
<https://w3id.org/con-tax/components/aat-furn#300037838>
  rdf:type owl:Class ;
  rdfs:comment "Armchairs with an upholstered frame and projecting wings for protection against drafts."@en ;
  rdfs:comment "Leunstoelen met een gestoffeerd frame en uitstekende oren voor bescherming tegen tocht."@nl ;
  rdfs:isDefinedBy <https://w3id.org/con-tax/components/aat-furn> ;
  rdfs:label "easy chairs"@en ;
  rdfs:label "luie stoel"@nl ;
  rdfs:label "luie stoelen"@nl ;
  rdfs:seeAlso <http://vocab.getty.edu/aat/300037838> ;
  rdfs:seeAlso wd:Q1847455 ;
  rdfs:subClassOf <https://w3id.org/con-tax/components/aat-furn#300037772> ;
.
<https://w3id.org/con-tax/components/aat-furn#300037850>
  rdf:type owl:Class ;
  rdfs:comment "Easy chairs having a semicircular back forming a single upholstered piece with the wings and arms. For chairs with a solid, rounded wooden back or those made from cutting away parts of a barrel, use \"barrel chairs.\""@en ;
  rdfs:comment "Term uit de 18e eeuw voor luie stoelen met een halfronde rugleuning die een gestoffeerd geheel vormt met de oren en armleuningen. Gebruik 'tonstoelen' voor stoelen met een stevige, ronde rugleuning van hout of stoelen die uit een ton zijn gemaakt."@nl ;
  rdfs:isDefinedBy <https://w3id.org/con-tax/components/aat-furn> ;
  rdfs:label "circular easy chairs"@en ;
  rdfs:label "ronde luie stoel"@nl ;
  rdfs:label "ronde luie stoelen"@nl ;
  rdfs:seeAlso <http://vocab.getty.edu/aat/300037850> ;
  rdfs:subClassOf <https://w3id.org/con-tax/components/aat-furn#300037838> ;
.
<https://w3id.org/con-tax/components/aat-furn#300037854>
  rdf:type owl:Class ;
  rdfs:comment "Easy chairs having a straight back, as distinguished from those with circular backs."@en ;
  rdfs:comment "Historische term die aan het eind van de 18e en het begin van de 19e eeuw werd gebruikt om onderscheid te maken tussen luie stoelen met een rechte en met een ronde rugleuning."@nl ;
  rdfs:isDefinedBy <https://w3id.org/con-tax/components/aat-furn> ;
  rdfs:label "square easy chair"@nl ;
  rdfs:label "square easy chairs"@en ;
  rdfs:label "square easy chairs"@nl ;
  rdfs:seeAlso <http://vocab.getty.edu/aat/300037854> ;
  rdfs:subClassOf <https://w3id.org/con-tax/components/aat-furn#300037838> ;
.
<https://w3id.org/con-tax/components/aat-furn#300037856>
  rdf:type owl:Class ;
  rdfs:comment "Franse stoelen met open armleuningen."@nl ;
  rdfs:comment "French chairs with open arms."@en ;
  rdfs:isDefinedBy <https://w3id.org/con-tax/components/aat-furn> ;
  rdfs:label "fauteuil"@nl ;
  rdfs:label "fauteuils (elbow chairs)"@en ;
  rdfs:label "fauteuils"@nl ;
  rdfs:seeAlso <http://vocab.getty.edu/aat/300037856> ;
  rdfs:seeAlso wd:Q981009 ;
  rdfs:subClassOf <https://w3id.org/con-tax/components/aat-furn#300165321> ;
.
<https://w3id.org/con-tax/components/aat-furn#300037861>
  rdf:type owl:Class ;
  rdfs:comment "Chairs whose backs gently curve forward and downward to form the arms; so called because of their resemblance to 18th-century gondolas."@en ;
  rdfs:comment "Stoelen waarvan de rugleuning een lichte boog naar voren en naar beneden maakt om zo de armleuningen te vormen. Ze worden zo genoemd omdat ze op gondels uit de 18e eeuw lijken."@nl ;
  rdfs:isDefinedBy <https://w3id.org/con-tax/components/aat-furn> ;
  rdfs:label "chaise en gondole"@nl ;
  rdfs:label "chaises en gondole"@nl ;
  rdfs:label "gondola chairs"@en ;
  rdfs:seeAlso <http://vocab.getty.edu/aat/300037861> ;
  rdfs:subClassOf <https://w3id.org/con-tax/components/aat-furn#300037772> ;
.
<https://w3id.org/con-tax/components/aat-furn#300037865>
  rdf:type owl:Class ;
  rdfs:comment "Armchairs that are stuffed or have a loose cushion to support the back, and wooden legs and a slide-out frame in the front upon which to rest the feet. In many versions, the slide may extend to full length so that the occupant may recline. Popular in the late-18th- and early-19th-centuries, the name refers to the chairs having been common in hunting lodges."@en ;
  rdfs:comment "Historische benaming voor leunstoelen uit het eind van de 18e en begin van de 19e eeuw die helemaal zijn opgevuld, behalve de poten, die van hout zijn gemaakt."@nl ;
  rdfs:isDefinedBy <https://w3id.org/con-tax/components/aat-furn> ;
  rdfs:label "hunting chair"@nl ;
  rdfs:label "hunting chairs"@en ;
  rdfs:label "hunting chairs"@nl ;
  rdfs:seeAlso <http://vocab.getty.edu/aat/300037865> ;
  rdfs:subClassOf <https://w3id.org/con-tax/components/aat-furn#300037772> ;
  rdfs:subClassOf <https://w3id.org/con-tax/components/aat-furn#300037776> ;
.
<https://w3id.org/con-tax/components/aat-furn#300037867>
  rdf:type owl:Class ;
  rdfs:comment "Ancient Greek chairs having a deep top rail curving forward from the back and sabre legs; usually undecorated. Imitated during various classical revivals, especially in the 19th century."@en ;
  rdfs:comment "Klassieke Griekse stoelen met een diepe bovenrand die vanuit de rugleuning in een gebogen lijn naar voren gaat, en sabelpoten. Ze zijn meestal onversierd en werden veel geïmiteerd tijdens diverse klassieke oplevingen, met name in de 19e eeuw."@nl ;
  rdfs:isDefinedBy <https://w3id.org/con-tax/components/aat-furn> ;
  rdfs:label "klismoi"@en ;
  rdfs:label "klismos-stoel"@nl ;
  rdfs:label "klismos-stoelen"@nl ;
  rdfs:seeAlso <http://vocab.getty.edu/aat/300037867> ;
  rdfs:seeAlso wd:Q1386950 ;
  rdfs:subClassOf <https://w3id.org/con-tax/components/aat-furn#300037772> ;
.
<https://w3id.org/con-tax/components/aat-furn#300037874>
  rdf:type owl:Class ;
  rdfs:comment "Historische benaming voor Amerikaanse stoelen met open armleuningen uit de 19e eeuw met een gestoffeerde zitting en rugleuning. De zittingen zijn meestal laag en ondiep en de rugleuningen zijn hoog en hebben vaak een slingerende rand."@nl ;
  rdfs:comment "Open-arm chairs with upholstered seats and backs, popular in the 18th and 19th centuries in North America. Seats are generally low and shallow, and the backs are high and often have serpentine cresting."@en ;
  rdfs:isDefinedBy <https://w3id.org/con-tax/components/aat-furn> ;
  rdfs:label "lolling chair"@nl ;
  rdfs:label "lolling chairs"@en ;
  rdfs:label "lolling chairs"@nl ;
  rdfs:seeAlso <http://vocab.getty.edu/aat/300037874> ;
  rdfs:subClassOf <https://w3id.org/con-tax/components/aat-furn#300037772> ;
  rdfs:subClassOf <https://w3id.org/con-tax/components/aat-furn#300037776> ;
.
<https://w3id.org/con-tax/components/aat-furn#300037892>
  rdf:type owl:Class ;
  rdfs:comment "Refers to 16th-century Italian wooden side chairs having a solid carved back and small, usually octagonal, seat supported on carved end boards in the front and back, instead of legs."@en ;
  rdfs:comment "Term die buiten Italië wordt gebruikt voor de houten, Italiaanse 'stoelen zonder armleuningen' uit de 16e eeuw die bestaan uit een stevige, bewerkte rugleuning en een kleine, meestal achthoekige zitting die niet door poten wordt ondersteund maar door bewerkte eindplanken aan de voor- en achterkant."@nl ;
  rdfs:isDefinedBy <https://w3id.org/con-tax/components/aat-furn> ;
  rdfs:label "schabel"@nl ;
  rdfs:label "schabellen"@nl ;
  rdfs:label "sgabelli"@nl ;
  rdfs:label "sgabello"@nl ;
  rdfs:label "sgabellos (chairs)"@en ;
  rdfs:seeAlso <http://vocab.getty.edu/aat/300037892> ;
  rdfs:subClassOf <https://w3id.org/con-tax/components/aat-furn#300140010> ;
.
<https://w3id.org/con-tax/components/aat-furn#300037896>
  rdf:type owl:Class ;
  rdfs:comment "Benaming die meestal betrekking heeft op een groot assortiment stoelen zonder armleuningen om ze te onderscheiden van leunstoelen."@nl ;
  rdfs:comment "Term generally applied to a wide range of chairs without arms to distinguish them from armchairs."@en ;
  rdfs:isDefinedBy <https://w3id.org/con-tax/components/aat-furn> ;
  rdfs:label "side chairs"@en ;
  rdfs:label "stoelen zonder armleuning"@nl ;
  rdfs:label "stoelen zonder armleuningen"@nl ;
  rdfs:seeAlso <http://vocab.getty.edu/aat/300037896> ;
  rdfs:subClassOf <https://w3id.org/con-tax/components/aat-furn#300037772> ;
.
<https://w3id.org/con-tax/components/aat-furn#300037899>
  rdf:type owl:Class ;
  rdfs:comment "Chairs made from looped and twisted iron wire, usually having circular oak seats. Chairs of this type were patented in the early 1900s. A number of manufacturers made such wire chairs; the name derives from their use in public restaurants and cafes."@en ;
  rdfs:comment "Stoelen die zijn gemaakt van gedraaid ijzerdraad,  meestal met een ronde eikenhouten zitting. In het begin van de 19e eeuw werd dit type gepatenteerd. Er waren een aantal fabrikanten die zulke draadstoelen maakten. De naam is afkomstig van het gebruik in openbare restaurants en cafés."@nl ;
  rdfs:isDefinedBy <https://w3id.org/con-tax/components/aat-furn> ;
  rdfs:label "ice-cream parlor chairs"@en ;
  rdfs:label "ijssalonstoel"@nl ;
  rdfs:label "ijssalonstoelen"@nl ;
  rdfs:seeAlso <http://vocab.getty.edu/aat/300037899> ;
  rdfs:subClassOf <https://w3id.org/con-tax/components/aat-furn#300037772> ;
.
<https://w3id.org/con-tax/components/aat-furn#300037904>
  rdf:type owl:Class ;
  rdfs:comment "Chairs with X-shaped frames; often designed to fold."@en ;
  rdfs:comment "Stoelen met een X-vormig frame, die vaak opvouwbaar zijn. Afgeleid van de Romeinse curulis (ceremoniele vouwstoel), Tijdens de renaissance werd  het stoeltype gemeengoed."@nl ;
  rdfs:isDefinedBy <https://w3id.org/con-tax/components/aat-furn> ;
  rdfs:label "X-chairs"@en ;
  rdfs:label "curulische zetel"@nl ;
  rdfs:label "curulische zetels"@nl ;
  rdfs:seeAlso <http://vocab.getty.edu/aat/300037904> ;
  rdfs:subClassOf <https://w3id.org/con-tax/components/aat-furn#300037772> ;
.
<https://w3id.org/con-tax/components/aat-furn#300037909>
  rdf:type owl:Class ;
  rdfs:comment "Benaming van verzamelaars voor de  X-framestoelen in Italiaanse renaissancestijl met alleen aan de voor- en achterkant dwarsverbindingen. De naam is afgeleid van de dichter Dante uit de 14e eeuw, hoewel het maar de vraag is of zulke stoelen daadwerkelijk door hem werden gebruikt."@nl ;
  rdfs:comment "Collector's term for Italian Renaissance X-chairs with crossing assemblies only in the front and back. Their name is derived from association with the 14th-century poet Dante, although it is questionable that such chairs were actually used by him."@en ;
  rdfs:isDefinedBy <https://w3id.org/con-tax/components/aat-furn> ;
  rdfs:label "Dante chairs"@en ;
  rdfs:label "Dante stoel"@nl ;
  rdfs:label "Dante stoelen"@nl ;
  rdfs:label "dagobertstoel"@nl ;
  rdfs:label "dagobertstoelen"@nl ;
  rdfs:seeAlso <http://vocab.getty.edu/aat/300037909> ;
  rdfs:subClassOf <https://w3id.org/con-tax/components/aat-furn#300037904> ;
.
<https://w3id.org/con-tax/components/aat-furn#300037913>
  rdf:type owl:Class ;
  rdfs:comment "Benaming die door verzamelaars wordt gebruikt voor Engelse vouwstoelen uit het begin van de 17e eeuw, waarvan de poten elkaar van voor naar achter kruisen en de armleuningen aan de rugleuning en en de voorste regel van de zitting vastzitten. Ze zijn waarschijnlijk gebaseerd op een stoel die werd gebruikt door de laatste abt van Glastonbury in de kathedraal van Wells."@nl ;
  rdfs:comment "Early 17th-century English folding chairs having legs crossed front to back and having arms connected to the back and to the front seat rail; design supposedly based on a chair used by the last Abbot of Glastonbury at Wells Cathedral and term derived from collectors' use."@en ;
  rdfs:isDefinedBy <https://w3id.org/con-tax/components/aat-furn> ;
  rdfs:label "Glastonbury chairs"@en ;
  rdfs:label "Glastonburystoel"@nl ;
  rdfs:label "Glastonburystoelen"@nl ;
  rdfs:seeAlso <http://vocab.getty.edu/aat/300037913> ;
  rdfs:subClassOf <https://w3id.org/con-tax/components/aat-furn#300244770> ;
.
<https://w3id.org/con-tax/components/aat-furn#300037918>
  rdf:type owl:Class ;
  rdfs:comment "Benaming die verzamelaars gebruiken voor stoelen in Italiaanse renaissancestijl  met talrijke dwarsverbindingen die onderling verbonden zijn aan de zijkanten. Ze zijn vernoemd naar de hervormende monnik uit de 15e eeuw, hoewel het maar de vraag is of zulke stoelen daadwerkelijk door hem werden gebruikt."@nl ;
  rdfs:comment "Collector's term for Italian Renaissance chairs with numerous crosspieces linked up along the sides. Named for the 15th-century reforming monk, although it is questionable that such chairs were actually used by him."@en ;
  rdfs:isDefinedBy <https://w3id.org/con-tax/components/aat-furn> ;
  rdfs:label "Savonarola chairs"@en ;
  rdfs:label "Savonarolastoel"@nl ;
  rdfs:label "Savonarolastoelen"@nl ;
  rdfs:seeAlso <http://vocab.getty.edu/aat/300037918> ;
  rdfs:subClassOf <https://w3id.org/con-tax/components/aat-furn#300037904> ;
.
<https://w3id.org/con-tax/components/aat-furn#300037920>
  rdf:type gvp:GuideTerm ;
  rdfs:isDefinedBy <https://w3id.org/con-tax/components/aat-furn> ;
  rdfs:label "<chairs by form: back form>"@en ;
  rdfs:label "<stoel naar vorm: vorm van de rug>"@nl ;
  rdfs:label "<stoelen naar vorm: vorm van de rug>"@nl ;
  rdfs:label "stoel naar vorm: vorm van de rug"@nl ;
  rdfs:label "stoelen naar vorm: vorm van de rug"@nl ;
  rdfs:seeAlso <http://vocab.getty.edu/aat/300037920> ;
  contax:containsConcept <https://w3id.org/con-tax/components/aat-furn#300037925> ;
  contax:containsConcept <https://w3id.org/con-tax/components/aat-furn#300037927> ;
  contax:containsConcept <https://w3id.org/con-tax/components/aat-furn#300037969> ;
  contax:containsConcept <https://w3id.org/con-tax/components/aat-furn#300037976> ;
  contax:containsConcept <https://w3id.org/con-tax/components/aat-furn#300037977> ;
  contax:containsConcept <https://w3id.org/con-tax/components/aat-furn#300037989> ;
  contax:containsConcept <https://w3id.org/con-tax/components/aat-furn#300037998> ;
  contax:containsConcept <https://w3id.org/con-tax/components/aat-furn#300038003> ;
  contax:containsConcept <https://w3id.org/con-tax/components/aat-furn#300038017> ;
  contax:containsConcept <https://w3id.org/con-tax/components/aat-furn#300038082> ;
  contax:containsConcept <https://w3id.org/con-tax/components/aat-furn#300038085> ;
  contax:containsConcept <https://w3id.org/con-tax/components/aat-furn#300038092> ;
  contax:containsConcept <https://w3id.org/con-tax/components/aat-furn#300038107> ;
  contax:containsConcept <https://w3id.org/con-tax/components/aat-furn#300038111> ;
  contax:containsConcept <https://w3id.org/con-tax/components/aat-furn#300038117> ;
  contax:containsConcept <https://w3id.org/con-tax/components/aat-furn#300038122> ;
  contax:containsConcept <https://w3id.org/con-tax/components/aat-furn#300133822> ;
  contax:containsConcept <https://w3id.org/con-tax/components/aat-furn#300133839> ;
  contax:containsConcept <https://w3id.org/con-tax/components/aat-furn#300139997> ;
  contax:containsConcept <https://w3id.org/con-tax/components/aat-furn#300146616> ;
  contax:containsConcept <https://w3id.org/con-tax/components/aat-furn#300165496> ;
  contax:containsConcept <https://w3id.org/con-tax/components/aat-furn#300174701> ;
.
<https://w3id.org/con-tax/components/aat-furn#300037925>
  rdf:type owl:Class ;
  rdfs:comment "Chairs with open backs and usually horizontal splats with the top rail and uprights rounded to give an overall balloon shape to the back."@en ;
  rdfs:comment "Stoelen met een open rugleuning en meestal een horizontaal middenblad waarbij de bovenregel en stijlen zijn gebogen, zodat de rugleuning de vorm van een ballon krijgt."@nl ;
  rdfs:isDefinedBy <https://w3id.org/con-tax/components/aat-furn> ;
  rdfs:label "ballonrugstoel"@nl ;
  rdfs:label "ballonrugstoelen"@nl ;
  rdfs:label "balloon-back chairs"@en ;
  rdfs:seeAlso <http://vocab.getty.edu/aat/300037925> ;
  rdfs:subClassOf <https://w3id.org/con-tax/components/aat-furn#300037772> ;
.
<https://w3id.org/con-tax/components/aat-furn#300037927>
  rdf:type owl:Class ;
  rdfs:comment "Use with reference to chairs with backs consisting of a series of vertical banisters between the seat and top rail; of a type first made in the 18th century."@en ;
  rdfs:comment "Wordt gebruikt om te verwijzen naar stoelen waarvan de rugleuning bestaat uit een reeks verticale spijlen tussen de zitting en bovenregel. Ze werden voor het eerst gemaakt in de 18e eeuw."@nl ;
  rdfs:isDefinedBy <https://w3id.org/con-tax/components/aat-furn> ;
  rdfs:label "banister-back chair"@nl ;
  rdfs:label "banister-back chairs"@en ;
  rdfs:label "banister-back chairs"@nl ;
  rdfs:seeAlso <http://vocab.getty.edu/aat/300037927> ;
  rdfs:subClassOf <https://w3id.org/con-tax/components/aat-furn#300037772> ;
.
<https://w3id.org/con-tax/components/aat-furn#300037933>
  rdf:type owl:Class ;
  rdfs:comment "18th-century American turned baluster-back chairs whose crest rail has cutouts of these shapes; the period name for these chairs is not known."@en ;
  rdfs:comment "Gedraaide, Amerikaanse '@baluster-back chairs' uit de 18e eeuw met uitgesneden harten en kronen in de bovenregel. De historische benaming voor deze stoelen is niet bekend."@nl ;
  rdfs:isDefinedBy <https://w3id.org/con-tax/components/aat-furn> ;
  rdfs:label "hearts and crown chair"@nl ;
  rdfs:label "hearts and crown chairs"@en ;
  rdfs:label "hearts and crown chairs"@nl ;
  rdfs:seeAlso <http://vocab.getty.edu/aat/300037933> ;
  rdfs:subClassOf <https://w3id.org/con-tax/components/aat-furn#300037927> ;
.
<https://w3id.org/con-tax/components/aat-furn#300037946>
  rdf:type owl:Class ;
  rdfs:comment "Gestoffeerde stoelen met een iets holle rugleuning, zodat die bij de omtrek van het menselijke lichaam past. Ze verschillen van de zogenoemde 'chaises à la reine', die een vlakke rugleuning hebben."@nl ;
  rdfs:comment "Upholstered chairs with slightly concave backs to fit the contours of the human body; distinct from those with flat backs called \"chaises à la reine.\""@en ;
  rdfs:isDefinedBy <https://w3id.org/con-tax/components/aat-furn> ;
  rdfs:label "chaise en cabriolet"@nl ;
  rdfs:label "chaises en cabriolet (concave-back chairs)"@en ;
  rdfs:label "chaises en cabriolet"@nl ;
  rdfs:seeAlso <http://vocab.getty.edu/aat/300037946> ;
  rdfs:subClassOf <https://w3id.org/con-tax/components/aat-furn#300174701> ;
.
<https://w3id.org/con-tax/components/aat-furn#300037948>
  rdf:type owl:Class ;
  rdfs:comment "Fauteuils met een holle rugleuning die verschillen van 'fauteuils à la reine', die  een vlakke rugleuning hebben."@nl ;
  rdfs:comment "Fauteuils with concave backs; distinct from \"fauteuils à la reine,\" which have flat backs."@en ;
  rdfs:isDefinedBy <https://w3id.org/con-tax/components/aat-furn> ;
  rdfs:label "fauteuil a cabriolet"@nl ;
  rdfs:label "fauteuils a cabriolet"@nl ;
  rdfs:label "fauteuils en cabriolet"@en ;
  rdfs:seeAlso <http://vocab.getty.edu/aat/300037948> ;
  rdfs:subClassOf <https://w3id.org/con-tax/components/aat-furn#300037856> ;
  rdfs:subClassOf <https://w3id.org/con-tax/components/aat-furn#300174701> ;
.
<https://w3id.org/con-tax/components/aat-furn#300037953>
  rdf:type owl:Class ;
  rdfs:comment "Gestoffeerde stoelen met een vlakke rug. Te onderscheiden van de zogenoemde 'chaises en cabriolet', die een holle rugleuning hebben."@nl ;
  rdfs:comment "Upholstered chairs with flat backs; distinct from those with concave backs called \"chaises en cabriolet.\""@en ;
  rdfs:isDefinedBy <https://w3id.org/con-tax/components/aat-furn> ;
  rdfs:label "chaise à la reine"@nl ;
  rdfs:label "chaises à la reine"@en ;
  rdfs:label "chaises à la reine"@nl ;
  rdfs:seeAlso <http://vocab.getty.edu/aat/300037953> ;
  rdfs:subClassOf <https://w3id.org/con-tax/components/aat-furn#300133822> ;
.
<https://w3id.org/con-tax/components/aat-furn#300037954>
  rdf:type owl:Class ;
  rdfs:comment "Fauteuils met een vlakke rugleuning. Te onderscheiden van 'fauteuils en cabriolet' met een holle rugleuning."@nl ;
  rdfs:comment "Fauteuils with flat backs; distinct from \"fauteuils en cabriolet,\" which have concave backs."@en ;
  rdfs:isDefinedBy <https://w3id.org/con-tax/components/aat-furn> ;
  rdfs:label "fauteuil à la reine"@nl ;
  rdfs:label "fauteuils à la reine"@en ;
  rdfs:label "fauteuils à la reine"@nl ;
  rdfs:seeAlso <http://vocab.getty.edu/aat/300037954> ;
  rdfs:subClassOf <https://w3id.org/con-tax/components/aat-furn#300037856> ;
  rdfs:subClassOf <https://w3id.org/con-tax/components/aat-furn#300133822> ;
.
<https://w3id.org/con-tax/components/aat-furn#300037956>
  rdf:type owl:Class ;
  rdfs:comment "Benaming die door Chippendale en anderen wordt gebruikt voor fret-backstoelen met Chinees sierwerk."@nl ;
  rdfs:comment "Term used by Chippendale and others for fret-back chairs incorporating Chinese frets."@en ;
  rdfs:isDefinedBy <https://w3id.org/con-tax/components/aat-furn> ;
  rdfs:label "Chinese chairs"@en ;
  rdfs:label "Chinese stoel"@nl ;
  rdfs:label "Chinese stoelen"@nl ;
  rdfs:seeAlso <http://vocab.getty.edu/aat/300037956> ;
  rdfs:subClassOf <https://w3id.org/con-tax/components/aat-furn#300146616> ;
.
<https://w3id.org/con-tax/components/aat-furn#300037969>
  rdf:type owl:Class ;
  rdfs:comment "Amerikaanse stoelen uit het eind van de 18e eeuw waarvan de rugleuning hartvormig is. Ze waren vooral populair in New England."@nl ;
  rdfs:comment "Late 18th-century American chairs, with heart-shaped backs; especially popular in New England."@en ;
  rdfs:isDefinedBy <https://w3id.org/con-tax/components/aat-furn> ;
  rdfs:label "heart-back chairs"@en ;
  rdfs:label "heart-back stoel"@nl ;
  rdfs:label "heart-back stoelen"@nl ;
  rdfs:seeAlso <http://vocab.getty.edu/aat/300037969> ;
  rdfs:subClassOf <https://w3id.org/con-tax/components/aat-furn#300037772> ;
.
<https://w3id.org/con-tax/components/aat-furn#300037976>
  rdf:type owl:Class ;
  rdfs:comment "Chairs with backs consisting of two crescent shapes, one inverted above the other."@en ;
  rdfs:comment "Wordt gebruikt voor stoelen waarvan de rugleuning bestaat uit twee halvemaanvormen, waarvan er één omgekeerd boven de ander is geplaatst."@nl ;
  rdfs:isDefinedBy <https://w3id.org/con-tax/components/aat-furn> ;
  rdfs:label "lunette-back chairs"@en ;
  rdfs:label "lunette-backstoel"@nl ;
  rdfs:label "lunette-backstoelen"@nl ;
  rdfs:seeAlso <http://vocab.getty.edu/aat/300037976> ;
  rdfs:seeAlso wd:Q21550753 ;
  rdfs:subClassOf <https://w3id.org/con-tax/components/aat-furn#300037772> ;
.
<https://w3id.org/con-tax/components/aat-furn#300037977>
  rdf:type owl:Class ;
  rdfs:comment "Chairs whose backs are oval shaped."@en ;
  rdfs:isDefinedBy <https://w3id.org/con-tax/components/aat-furn> ;
  rdfs:label "oval-back chairs"@en ;
  rdfs:label "oval-backstoel"@nl ;
  rdfs:label "oval-backstoelen"@nl ;
  rdfs:seeAlso <http://vocab.getty.edu/aat/300037977> ;
  rdfs:subClassOf <https://w3id.org/con-tax/components/aat-furn#300037772> ;
.
<https://w3id.org/con-tax/components/aat-furn#300037989>
  rdf:type owl:Class ;
  rdfs:comment "Chairs featuring an ornamental design pressed into its back. This effect is created by the use of a sharp steel die stamp mounted on a roller, passed over the chair with great pressure, resulting in a perfect impression of a design that was literally pressed into the wood, giving the illusion of hand carving. Press-back chairs were popular in the late 19th-early 20th century."@en ;
  rdfs:isDefinedBy <https://w3id.org/con-tax/components/aat-furn> ;
  rdfs:label "press-back chairs"@en ;
  rdfs:label "press-backstoel"@nl ;
  rdfs:label "press-backstoelen"@nl ;
  rdfs:seeAlso <http://vocab.getty.edu/aat/300037989> ;
  rdfs:subClassOf <https://w3id.org/con-tax/components/aat-furn#300037772> ;
.
<https://w3id.org/con-tax/components/aat-furn#300037998>
  rdf:type owl:Class ;
  rdfs:comment "Chair designs made fashionable in the 1780s by George Hepplewhite. The rail and stile form the shape of a shield."@en ;
  rdfs:comment "Stoelontwerpen die rond 1780 populair werden gemaakt door George Hepplewhite. De bovenregel en stijl hebben samen de vorm van een schild."@nl ;
  rdfs:isDefinedBy <https://w3id.org/con-tax/components/aat-furn> ;
  rdfs:label "shield-back chairs"@en ;
  rdfs:label "shield-backstoel"@nl ;
  rdfs:label "shield-backstoelen"@nl ;
  rdfs:seeAlso <http://vocab.getty.edu/aat/300037998> ;
  rdfs:subClassOf <https://w3id.org/con-tax/components/aat-furn#300037772> ;
.
<https://w3id.org/con-tax/components/aat-furn#300038000>
  rdf:type owl:Class ;
  rdfs:comment "Chairs or sofas of the Hepplewhite period whose back is comprised of carved or shaped veritcal bars curved to fit the shield of a shield-back chair."@en ;
  rdfs:isDefinedBy <https://w3id.org/con-tax/components/aat-furn> ;
  rdfs:label "bar-back chairs"@en ;
  rdfs:label "bar-backstoel"@nl ;
  rdfs:label "bar-backstoelen"@nl ;
  rdfs:seeAlso <http://vocab.getty.edu/aat/300038000> ;
  rdfs:subClassOf <https://w3id.org/con-tax/components/aat-furn#300037998> ;
.
<https://w3id.org/con-tax/components/aat-furn#300038003>
  rdf:type owl:Class ;
  rdfs:comment "Chairs with horizontal slats across the back."@en ;
  rdfs:comment "Stoelen met horizontale spijlen in de rugleuning."@nl ;
  rdfs:isDefinedBy <https://w3id.org/con-tax/components/aat-furn> ;
  rdfs:label "slat-back chairs"@en ;
  rdfs:label "slat-backstoel"@nl ;
  rdfs:label "slat-backstoelen"@nl ;
  rdfs:seeAlso <http://vocab.getty.edu/aat/300038003> ;
  rdfs:subClassOf <https://w3id.org/con-tax/components/aat-furn#300037772> ;
.
<https://w3id.org/con-tax/components/aat-furn#300038011>
  rdf:type owl:Class ;
  rdfs:comment "Amerikaanse stoelen uit het einde van de 18e eeuw met ineengestrengelde, opengewerkte spijlen. Ze worden meestal geassocieerd met meubelmakers uit Philadelphia."@nl ;
  rdfs:comment "Late 18th-century American chairs with pierced and intertwined slats and generally associated with Philadelphia cabinetmakers."@en ;
  rdfs:isDefinedBy <https://w3id.org/con-tax/components/aat-furn> ;
  rdfs:label "pretzel-back chairs"@en ;
  rdfs:label "pretzel-backstoel"@nl ;
  rdfs:label "pretzel-backstoelen"@nl ;
  rdfs:seeAlso <http://vocab.getty.edu/aat/300038011> ;
  rdfs:subClassOf <https://w3id.org/con-tax/components/aat-furn#300038003> ;
.
<https://w3id.org/con-tax/components/aat-furn#300038017>
  rdf:type owl:Class ;
  rdfs:comment "Chairs whose backs are comprised of framed cylindrical bars or \"spindles.\""@en ;
  rdfs:isDefinedBy <https://w3id.org/con-tax/components/aat-furn> ;
  rdfs:label "spindle-back chairs"@en ;
  rdfs:label "spindle-backstoel"@nl ;
  rdfs:label "spindle-backstoelen"@nl ;
  rdfs:seeAlso <http://vocab.getty.edu/aat/300038017> ;
  rdfs:subClassOf <https://w3id.org/con-tax/components/aat-furn#300037772> ;
.
<https://w3id.org/con-tax/components/aat-furn#300038020>
  rdf:type owl:Class ;
  rdfs:comment "Armchairs designed to be the largest pieces of furniture in a sitting room, particularly common in 17th-century Britain and America. They are made of wood, usually with conspicuous carvings and occasionally with upholstered seats. They may resemble a throne."@en ;
  rdfs:comment "Historische term die wordt gebruikt voor grote Amerikaanse leunstoelen uit de 17e eeuw."@nl ;
  rdfs:isDefinedBy <https://w3id.org/con-tax/components/aat-furn> ;
  rdfs:label "great chair"@nl ;
  rdfs:label "great chairs"@en ;
  rdfs:label "great chairs"@nl ;
  rdfs:seeAlso <http://vocab.getty.edu/aat/300038020> ;
  rdfs:subClassOf <https://w3id.org/con-tax/components/aat-furn#300037776> ;
.
<https://w3id.org/con-tax/components/aat-furn#300038026>
  rdf:type owl:Class ;
  rdfs:comment "17th-century American turned great chairs styled after one that belonged to Elder William Brewster of Plymouth Colony. Such chairs have boldly turned posts and decorative spindles, but unlike Carver chairs they have spindles below the seat as well as in the back and below the arms."@en ;
  rdfs:comment "Benaming die door verzamelaars wordt gebruikt voor Amerikaanse gedraaide leunstoelen uit de 17e eeuw die zijn gevormd naar een stoel van senator William Brewster van de kolonie van Plymouth. Zulke stoelen hebben sterk gedraaide poten en decoratieve spijlen. In tegenstelling tot Carverstoelen hebben ze naast spijlen onder de zitting ook spijlen in de rug- en onder de armleuning."@nl ;
  rdfs:isDefinedBy <https://w3id.org/con-tax/components/aat-furn> ;
  rdfs:label "Brewster chairs"@en ;
  rdfs:label "Brewsterstoel"@nl ;
  rdfs:label "Brewsterstoelen"@nl ;
  rdfs:seeAlso <http://vocab.getty.edu/aat/300038026> ;
  rdfs:seeAlso wd:Q4962745 ;
  rdfs:subClassOf <https://w3id.org/con-tax/components/aat-furn#300038020> ;
.
<https://w3id.org/con-tax/components/aat-furn#300038027>
  rdf:type owl:Class ;
  rdfs:comment "17th-century American turned great chairs styled after one that belonged to John Carver, Governor of Massachusetts Bay Colony. Such chairs have boldly turned posts and decorative spindles, but unlike Brewster chairs they have spindles only in the back and below the arms, and not below the seat."@en ;
  rdfs:comment "Benaming die door verzamelaars wordt gebruikt voor Amerikaanse gedraaide leunstoelen uit de 17e eeuw die zijn gevormd naar een stoel van John Carver die gouverneur was van de kolonie van Massachusetts Bay.  Zulke stoelen hebben sterk gedraaide poten en decoratieve spijlen. In tegenstelling tot Brewsterstoelen zitten de spijlen alleen aan de achterkant en onder de armleuningen en niet onder de zitting."@nl ;
  rdfs:isDefinedBy <https://w3id.org/con-tax/components/aat-furn> ;
  rdfs:label "Carver chairs"@en ;
  rdfs:label "Carverstoel"@nl ;
  rdfs:label "Carverstoelen"@nl ;
  rdfs:seeAlso <http://vocab.getty.edu/aat/300038027> ;
  rdfs:subClassOf <https://w3id.org/con-tax/components/aat-furn#300038020> ;
.
<https://w3id.org/con-tax/components/aat-furn#300038082>
  rdf:type owl:Class ;
  rdfs:comment "Early 18th-century chairs with or without arms, having a vase-shaped splat in the back which was curved to give comfortable support to the back."@en ;
  rdfs:comment "Stoelen uit het begin van de 18e eeuw, met of zonder armleuningen, met een vaasvormig middenblad in de rugleuning, die is gebogen om als aangenaam steuntje in de rug te dienen."@nl ;
  rdfs:isDefinedBy <https://w3id.org/con-tax/components/aat-furn> ;
  rdfs:label "bended-back chairs"@en ;
  rdfs:label "geronde-rug stoel"@nl ;
  rdfs:label "geronde-rug stoelen"@nl ;
  rdfs:seeAlso <http://vocab.getty.edu/aat/300038082> ;
  rdfs:subClassOf <https://w3id.org/con-tax/components/aat-furn#300037772> ;
.
<https://w3id.org/con-tax/components/aat-furn#300038085>
  rdf:type owl:Class ;
  rdfs:comment "Chairs with a single back splat which resembles the outline of a fiddle."@en ;
  rdfs:comment "Stoelen waarvan de rugleuning bestaat uit een enkel middenblad in de vorm van een viool."@nl ;
  rdfs:isDefinedBy <https://w3id.org/con-tax/components/aat-furn> ;
  rdfs:label "fiddle-back chairs"@en ;
  rdfs:label "fiddle-back stoel"@nl ;
  rdfs:label "fiddle-back stoelen"@nl ;
  rdfs:seeAlso <http://vocab.getty.edu/aat/300038085> ;
  rdfs:subClassOf <https://w3id.org/con-tax/components/aat-furn#300037772> ;
.
<https://w3id.org/con-tax/components/aat-furn#300038088>
  rdf:type owl:Class ;
  rdfs:comment "Chairs that incorporate latticework adapted from Chinese sources in the back or arms. Coined by Thomas Chippendale."@en ;
  rdfs:isDefinedBy <https://w3id.org/con-tax/components/aat-furn> ;
  rdfs:label "India chair"@nl ;
  rdfs:label "India chairs"@en ;
  rdfs:label "India chairs"@nl ;
  rdfs:seeAlso <http://vocab.getty.edu/aat/300038088> ;
  rdfs:subClassOf <https://w3id.org/con-tax/components/aat-furn#300037772> ;
.
<https://w3id.org/con-tax/components/aat-furn#300038092>
  rdf:type owl:Class ;
  rdfs:comment "Chairs with interwoven splats in the form of interlaced ribbons, such as those popularized by Chippendale and appearing in mid-18th century England and America."@en ;
  rdfs:comment "Stoelen met verstrengelde spijlen in de vorm van gevlochten linten, die bekendheid kregen door Chippendale en vanaf het midden van de 18e eeuw voorkwamen in Engeland en Amerika."@nl ;
  rdfs:isDefinedBy <https://w3id.org/con-tax/components/aat-furn> ;
  rdfs:label "ribbon-back chairs"@en ;
  rdfs:label "ribbon-backstoel"@nl ;
  rdfs:label "ribbon-backstoelen"@nl ;
  rdfs:seeAlso <http://vocab.getty.edu/aat/300038092> ;
  rdfs:subClassOf <https://w3id.org/con-tax/components/aat-furn#300037772> ;
.
<https://w3id.org/con-tax/components/aat-furn#300038100>
  rdf:type owl:Class ;
  rdfs:comment "Chairs whose splats are pierced to form a cypher with the initials of their owners."@en ;
  rdfs:comment "Stoelen waarbij de rugleuning is opengewerkt in de vorm van een monogram van de initialen van de eigenaar."@nl ;
  rdfs:isDefinedBy <https://w3id.org/con-tax/components/aat-furn> ;
  rdfs:label "cypher-back chairs"@en ;
  rdfs:label "cypher-backstoel"@nl ;
  rdfs:label "cypher-backstoelen"@nl ;
  rdfs:seeAlso <http://vocab.getty.edu/aat/300038100> ;
  rdfs:subClassOf <https://w3id.org/con-tax/components/aat-furn#300133839> ;
.
<https://w3id.org/con-tax/components/aat-furn#300038107>
  rdf:type owl:Class ;
  rdfs:comment "Deze naam wordt soms gebruikt voor stoelen uit het begin van de 18e eeuw waarvan de rugleuning een lichte, dubbele kromming heeft die is ontworpen om zich naar de rug van de zittende persoon te voegen. De naam wordt ook gebruikt voor een stoel uit het midden van de 19e eeuw met een ronde, getailleerde rugleuning en korte poten."@nl ;
  rdfs:comment "The name sometimes given to early 18th-century chairs in which the back has a gentle double curve designed to fit the back of the sitter. Also a mid-19th century chair with a rounded, waisted back and short legs."@en ;
  rdfs:isDefinedBy <https://w3id.org/con-tax/components/aat-furn> ;
  rdfs:label "spoon-back chairs"@en ;
  rdfs:label "spoon-backstoel"@nl ;
  rdfs:label "spoon-backstoelen"@nl ;
  rdfs:seeAlso <http://vocab.getty.edu/aat/300038107> ;
  rdfs:subClassOf <https://w3id.org/con-tax/components/aat-furn#300037772> ;
.
<https://w3id.org/con-tax/components/aat-furn#300038108>
  rdf:type owl:Class ;
  rdfs:comment "Hedendaagse benaming voor stoelen die in het midden van de 18e eeuw werden gemaakt, met een getailleerde, opengewerkte rugleuning in de vorm van een korenschoof."@nl ;
  rdfs:comment "Modern term for chair backs, made in the mid-18th century, with a waisted, pierced splat, which resembles the shape of a wheatsheaf."@en ;
  rdfs:isDefinedBy <https://w3id.org/con-tax/components/aat-furn> ;
  rdfs:label "sheaf-back chairs"@en ;
  rdfs:label "sheaf-backstoel"@nl ;
  rdfs:label "sheaf-backstoelen"@nl ;
  rdfs:seeAlso <http://vocab.getty.edu/aat/300038108> ;
  rdfs:subClassOf <https://w3id.org/con-tax/components/aat-furn#300133839> ;
.
<https://w3id.org/con-tax/components/aat-furn#300038111>
  rdf:type owl:Class ;
  rdfs:comment "Use with reference to chairs with a square back such as those popularized by Sheraton and appearing from the late 18th century."@en ;
  rdfs:comment "Wordt gebruikt voor stoelen met een vierkante rugleuning die vanaf het einde van de 18e eeuw voorkomen en door Sheraton bekendheid kregen."@nl ;
  rdfs:isDefinedBy <https://w3id.org/con-tax/components/aat-furn> ;
  rdfs:label "square-back chairs"@en ;
  rdfs:label "square-backstoel"@nl ;
  rdfs:label "square-backstoelen"@nl ;
  rdfs:seeAlso <http://vocab.getty.edu/aat/300038111> ;
  rdfs:subClassOf <https://w3id.org/con-tax/components/aat-furn#300037772> ;
.
<https://w3id.org/con-tax/components/aat-furn#300038112>
  rdf:type owl:Class ;
  rdfs:comment "Chairs having a back formed by slender members crossing over each other in a netlike pattern."@en ;
  rdfs:comment "Stoelen met een rugleuning die uit smalle delen bestaat die elkaar kruisen zodat ze een netachtig patroon vormen."@nl ;
  rdfs:isDefinedBy <https://w3id.org/con-tax/components/aat-furn> ;
  rdfs:label "lattice-back chairs"@en ;
  rdfs:label "lattice-backstoel"@nl ;
  rdfs:label "lattice-backstoelen"@nl ;
  rdfs:seeAlso <http://vocab.getty.edu/aat/300038112> ;
  rdfs:subClassOf <https://w3id.org/con-tax/components/aat-furn#300038111> ;
.
<https://w3id.org/con-tax/components/aat-furn#300038117>
  rdf:type owl:Class ;
  rdfs:comment "16th- and 17th-century joined chairs having a solid paneled back and a plank seat; generally made of oak and often carved."@en ;
  rdfs:comment "Stoelen van schrijnwerk, uit de 16e en 17e eeuw, met een zitting van planken en een rugleuning uit  massieve panelen. Ze zijn meestal van eikenhout gemaakt en zijn vaak met houtsnijwerk versierd."@nl ;
  rdfs:isDefinedBy <https://w3id.org/con-tax/components/aat-furn> ;
  rdfs:label "wainscot chair"@nl ;
  rdfs:label "wainscot chairs"@en ;
  rdfs:label "wainscot chairs"@nl ;
  rdfs:seeAlso <http://vocab.getty.edu/aat/300038117> ;
  rdfs:seeAlso wd:Q7960183 ;
  rdfs:subClassOf <https://w3id.org/con-tax/components/aat-furn#300037772> ;
.
<https://w3id.org/con-tax/components/aat-furn#300038122>
  rdf:type owl:Class ;
  rdfs:comment "Engelse stoelen uit het eind van de 18e eeuw die een ronde of ellipsvormige rugleuning hebben met straalsgewijs uitlopende spijlen of staven, die op de spaken van een wiel lijken."@nl ;
  rdfs:comment "Late 18th-century English chairs having round or oval backs with radiating spindles or bars resembling the spokes of a wheel."@en ;
  rdfs:isDefinedBy <https://w3id.org/con-tax/components/aat-furn> ;
  rdfs:label "wheel-back chairs"@en ;
  rdfs:label "wheel-backstoel"@nl ;
  rdfs:label "wheel-backstoelen"@nl ;
  rdfs:seeAlso <http://vocab.getty.edu/aat/300038122> ;
  rdfs:subClassOf <https://w3id.org/con-tax/components/aat-furn#300037772> ;
.
<https://w3id.org/con-tax/components/aat-furn#300038126>
  rdf:type owl:Class ;
  rdfs:comment "Benaming die meestal betrekking heeft op verschillende soorten stoelen met een zitting en rugleuning die zijn gevormd uit één stuk canvas, leer of iets dergelijks en die losjes rond het frame hangen."@nl ;
  rdfs:comment "Term generally applied to any of several varieties of chairs having a seat and back formed from a single sheet of canvas, leather, or the like, and hanging loosely on a frame."@en ;
  rdfs:isDefinedBy <https://w3id.org/con-tax/components/aat-furn> ;
  rdfs:label "sling chair"@nl ;
  rdfs:label "sling chairs"@en ;
  rdfs:label "sling chairs"@nl ;
  rdfs:seeAlso <http://vocab.getty.edu/aat/300038126> ;
  rdfs:subClassOf <https://w3id.org/con-tax/components/aat-furn#300037772> ;
.
<https://w3id.org/con-tax/components/aat-furn#300038128>
  rdf:type owl:Class ;
  rdfs:comment "Chairs constructed of a molded shell mounted on a single support on a flared base."@en ;
  rdfs:comment "Stoelen die bestaan uit een gevormd geraamte dat bovenop een steun met een wijd uitlopende voet staat."@nl ;
  rdfs:isDefinedBy <https://w3id.org/con-tax/components/aat-furn> ;
  rdfs:label "pedestal chairs"@en ;
  rdfs:label "piedestalstoel"@nl ;
  rdfs:label "piëdestalstoelen"@nl ;
  rdfs:seeAlso <http://vocab.getty.edu/aat/300038128> ;
  rdfs:subClassOf <https://w3id.org/con-tax/components/aat-furn#300037772> ;
.
<https://w3id.org/con-tax/components/aat-furn#300038131>
  rdf:type gvp:GuideTerm ;
  rdfs:isDefinedBy <https://w3id.org/con-tax/components/aat-furn> ;
  rdfs:label "<chairs by function>"@en ;
  rdfs:label "<stoel naar functie>"@nl ;
  rdfs:label "<stoelen naar functie>"@nl ;
  rdfs:label "stoel naar functie"@nl ;
  rdfs:label "stoelen naar functie"@nl ;
  rdfs:seeAlso <http://vocab.getty.edu/aat/300038131> ;
  contax:containsConcept <https://w3id.org/con-tax/components/aat-furn#300038132> ;
  contax:containsConcept <https://w3id.org/con-tax/components/aat-furn#300038144> ;
  contax:containsConcept <https://w3id.org/con-tax/components/aat-furn#300038155> ;
  contax:containsConcept <https://w3id.org/con-tax/components/aat-furn#300038164> ;
  contax:containsConcept <https://w3id.org/con-tax/components/aat-furn#300038165> ;
  contax:containsConcept <https://w3id.org/con-tax/components/aat-furn#300038180> ;
  contax:containsConcept <https://w3id.org/con-tax/components/aat-furn#300038191> ;
  contax:containsConcept <https://w3id.org/con-tax/components/aat-furn#300038205> ;
  contax:containsConcept <https://w3id.org/con-tax/components/aat-furn#300038208> ;
  contax:containsConcept <https://w3id.org/con-tax/components/aat-furn#300038217> ;
  contax:containsConcept <https://w3id.org/con-tax/components/aat-furn#300038224> ;
  contax:containsConcept <https://w3id.org/con-tax/components/aat-furn#300038227> ;
  contax:containsConcept <https://w3id.org/con-tax/components/aat-furn#300038228> ;
  contax:containsConcept <https://w3id.org/con-tax/components/aat-furn#300038229> ;
  contax:containsConcept <https://w3id.org/con-tax/components/aat-furn#300038232> ;
  contax:containsConcept <https://w3id.org/con-tax/components/aat-furn#300038252> ;
  contax:containsConcept <https://w3id.org/con-tax/components/aat-furn#300038283> ;
  contax:containsConcept <https://w3id.org/con-tax/components/aat-furn#300133851> ;
  contax:containsConcept <https://w3id.org/con-tax/components/aat-furn#300133860> ;
  contax:containsConcept <https://w3id.org/con-tax/components/aat-furn#300141151> ;
  contax:containsConcept <https://w3id.org/con-tax/components/aat-furn#300164567> ;
  contax:containsConcept <https://w3id.org/con-tax/components/aat-furn#300164591> ;
  contax:containsConcept <https://w3id.org/con-tax/components/aat-furn#300164594> ;
  contax:containsConcept <https://w3id.org/con-tax/components/aat-furn#300164657> ;
  contax:containsConcept <https://w3id.org/con-tax/components/aat-furn#300171016> ;
  contax:containsConcept <https://w3id.org/con-tax/components/aat-furn#300172137> ;
  contax:containsConcept <https://w3id.org/con-tax/components/aat-furn#300246035> ;
  contax:containsConcept <https://w3id.org/con-tax/components/aat-furn#300251230> ;
  contax:containsConcept <https://w3id.org/con-tax/components/aat-furn#300391486> ;
.
<https://w3id.org/con-tax/components/aat-furn#300038132>
  rdf:type owl:Class ;
  rdfs:comment "Chairs used to seat the clients of a barber, specifically chairs fixed to the floor and incorporating a mechanical means of adjusting height, rotation, or angle of recline."@en ;
  rdfs:isDefinedBy <https://w3id.org/con-tax/components/aat-furn> ;
  rdfs:label "barbers' chairs"@en ;
  rdfs:label "kappersstoel"@nl ;
  rdfs:label "kappersstoelen"@nl ;
  rdfs:seeAlso <http://vocab.getty.edu/aat/300038132> ;
  rdfs:seeAlso wd:Q2947719 ;
  rdfs:subClassOf <https://w3id.org/con-tax/components/aat-furn#300037772> ;
  rdfs:subClassOf <https://w3id.org/con-tax/components/aat-furn#300040036> ;
.
<https://w3id.org/con-tax/components/aat-furn#300038134>
  rdf:type owl:Class ;
  rdfs:comment "Een soort uitgebreide rolstoelen die soms van glas zijn voorzien. Ze werden vooral gemaakt in het midden van de 19e eeuw en bij kuuroorden en badplaatsen gebruikt."@nl ;
  rdfs:comment "Type of elaborate wheelchairs, sometimes glassed, especially those made in England in the mid-19th century and used at spas and seaside resorts."@en ;
  rdfs:isDefinedBy <https://w3id.org/con-tax/components/aat-furn> ;
  rdfs:label "bath chair"@nl ;
  rdfs:label "bath chairs"@en ;
  rdfs:label "bath chairs"@nl ;
  rdfs:seeAlso <http://vocab.getty.edu/aat/300038134> ;
  rdfs:seeAlso wd:Q4868971 ;
  rdfs:subClassOf <https://w3id.org/con-tax/components/aat-furn#300038243> ;
.
<https://w3id.org/con-tax/components/aat-furn#300038140>
  rdf:type owl:Class ;
  rdfs:comment "Richly or splendidly decorated chairs used on ceremonial occasions by a monarch or other person of high rank. Generally less grandiose than \"thrones.\""@en ;
  rdfs:comment "Stoelen met een hoge rugleuning en uitgebreide versieringen. Ze zijn speciaal voor uiterlijk vertoon gemaakt."@nl ;
  rdfs:isDefinedBy <https://w3id.org/con-tax/components/aat-furn> ;
  rdfs:label "state chairs"@en ;
  rdfs:label "statiestoel"@nl ;
  rdfs:label "statiestoelen"@nl ;
  rdfs:seeAlso <http://vocab.getty.edu/aat/300038140> ;
  rdfs:subClassOf <https://w3id.org/con-tax/components/aat-furn#300133851> ;
.
<https://w3id.org/con-tax/components/aat-furn#300038141>
  rdf:type owl:Class ;
  rdfs:comment "Ceremonial chairs or seats occupied by a monarch, prelate, or other high dignitary, especially on state or other special occasions; usually placed upon a dais and covered with a canopy."@en ;
  rdfs:comment "Te gebruiken voor ceremoniële stoelen of zetels voor monarchen, prelaten of andere hoogwaardigheidsbekleders, vooral gebruikt bij staatsiegelegenheden en andere speciale gebeurtenissen; gewoonlijk geplaatst op een podium en voorzien van een baldakijn."@nl ;
  rdfs:isDefinedBy <https://w3id.org/con-tax/components/aat-furn> ;
  rdfs:label "thrones"@en ;
  rdfs:label "tronen"@nl ;
  rdfs:label "troon"@nl ;
  rdfs:seeAlso <http://vocab.getty.edu/aat/300038141> ;
  rdfs:subClassOf <https://w3id.org/con-tax/components/aat-furn#300133851> ;
.
<https://w3id.org/con-tax/components/aat-furn#300038144>
  rdf:type owl:Class ;
  rdfs:comment "Chairs with backs which may be lowered and seats that are hinged to unfold or that can otherwise be extended to form beds."@en ;
  rdfs:comment "Stoelen waarvan de rugleuning omlaag kan en de zitting kan worden uitgeklapt door middel van scharnieren, of anderszins kan worden verlengd om een bed te vormen."@nl ;
  rdfs:isDefinedBy <https://w3id.org/con-tax/components/aat-furn> ;
  rdfs:label "bed chair"@nl ;
  rdfs:label "bed chairs"@en ;
  rdfs:label "bed chairs"@nl ;
  rdfs:seeAlso <http://vocab.getty.edu/aat/300038144> ;
  rdfs:subClassOf <https://w3id.org/con-tax/components/aat-furn#300037772> ;
  rdfs:subClassOf <https://w3id.org/con-tax/components/aat-furn#300038697> ;
.
<https://w3id.org/con-tax/components/aat-furn#300038148>
  rdf:type owl:Class ;
  rdfs:comment "Armchairs with large backs which are hinged so that they can be swung forward to rest on the arms, converting the piece into a table. Chairs of this type were made from the Middle Ages to the late 17th century in Europe and until the late 19th century in America."@en ;
  rdfs:comment "Stoelen met grote rugleuning, die scharnierde zodat ze naar voren kunnen worden gezwaaid om op de armen te rusten, waardoorn het meubel in een tabel veranderd wordt. Stoelen van dit type werden in Europa van de middeleeuwen tot de late 17e eeuw gemaakt en in Amerika tot in de late 19e eeuw."@nl ;
  rdfs:isDefinedBy <https://w3id.org/con-tax/components/aat-furn> ;
  rdfs:label "chair-table"@nl ;
  rdfs:label "chair-tables"@en ;
  rdfs:label "chair-tables"@nl ;
  rdfs:seeAlso <http://vocab.getty.edu/aat/300038148> ;
  rdfs:subClassOf <https://w3id.org/con-tax/components/aat-furn#300037772> ;
  rdfs:subClassOf <https://w3id.org/con-tax/components/aat-furn#300039548> ;
.
<https://w3id.org/con-tax/components/aat-furn#300038151>
  rdf:type owl:Class ;
  rdfs:comment "Chairs, often upholstered, having a full-length leg rest and usually arms, designed for one person to recline on. For similar chairs used outdoors, use \"deck chairs.\""@en ;
  rdfs:comment "Stoelen die vaak zijn gestoffeerd, een volledige beensteun  en meestal armleuningen hebben en zijn ontworpen om in te luieren. Gebruik 'ligstoelen' voor soortgelijke stoelen die buiten worden gebruikt."@nl ;
  rdfs:isDefinedBy <https://w3id.org/con-tax/components/aat-furn> ;
  rdfs:label "chaise longue"@nl ;
  rdfs:label "chaises longues"@en ;
  rdfs:label "chaises longues"@nl ;
  rdfs:seeAlso <http://vocab.getty.edu/aat/300038151> ;
  rdfs:subClassOf <https://w3id.org/con-tax/components/aat-furn#300037680> ;
  rdfs:subClassOf <https://w3id.org/con-tax/components/aat-furn#300037772> ;
.
<https://w3id.org/con-tax/components/aat-furn#300038153>
  rdf:type owl:Class ;
  rdfs:comment "Duchesses chairs made in two or three parts, each of which can be used separately as a seat."@en ;
  rdfs:comment "Duchesses die worden gemaakt in twee of drie delen waarvan elk stuk apart kan worden gebruikt als zitplaats."@nl ;
  rdfs:isDefinedBy <https://w3id.org/con-tax/components/aat-furn> ;
  rdfs:label "duchesse brisée"@nl ;
  rdfs:label "duchesses brisées"@en ;
  rdfs:label "duchesses brisées"@nl ;
  rdfs:seeAlso <http://vocab.getty.edu/aat/300038153> ;
  rdfs:subClassOf <https://w3id.org/con-tax/components/aat-furn#300165523> ;
.
<https://w3id.org/con-tax/components/aat-furn#300038155>
  rdf:type owl:Class ;
  rdfs:comment "Benaming die meestal wordt gebruikt voor verschillende soorten stoelen die met een po zijn uitgerust. Gebruik 'bidets' voor box stools met po."@nl ;
  rdfs:comment "Term generally applied to a variety of chairs fitted with a chamber pot. Use \"bidets (box stools)\" for box stools with a chamber pot."@en ;
  rdfs:isDefinedBy <https://w3id.org/con-tax/components/aat-furn> ;
  rdfs:label "commode chairs"@en ;
  rdfs:label "commodestoel"@nl ;
  rdfs:label "commodestoelen"@nl ;
  rdfs:label "kamergemak"@nl ;
  rdfs:label "kamergemakken"@nl ;
  rdfs:label "poepdozen"@nl ;
  rdfs:label "stilletje"@nl ;
  rdfs:label "stilletjes"@nl ;
  rdfs:seeAlso <http://vocab.getty.edu/aat/300038155> ;
  rdfs:subClassOf <https://w3id.org/con-tax/components/aat-furn#300037772> ;
.
<https://w3id.org/con-tax/components/aat-furn#300038164>
  rdf:type owl:Class ;
  rdfs:comment "Chairs designed to be used in dentists' offices that allow the patient to be positioned in various ways for dental work. These are usually accessorized with various appliances. Modern dental chairs are equipped with pneumatics for raising or lowering the chair itself."@en ;
  rdfs:isDefinedBy <https://w3id.org/con-tax/components/aat-furn> ;
  rdfs:label "dental chairs"@en ;
  rdfs:label "tandartsstoel"@nl ;
  rdfs:label "tandartsstoelen"@nl ;
  rdfs:seeAlso <http://vocab.getty.edu/aat/300038164> ;
  rdfs:subClassOf <https://w3id.org/con-tax/components/aat-furn#300037772> ;
  rdfs:subClassOf <https://w3id.org/con-tax/components/aat-furn#300040036> ;
.
<https://w3id.org/con-tax/components/aat-furn#300038165>
  rdf:type owl:Class ;
  rdfs:comment "Chairs of various form designed to be used in tandem with case furniture for readers or writers."@en ;
  rdfs:isDefinedBy <https://w3id.org/con-tax/components/aat-furn> ;
  rdfs:label "bureaustoel"@nl ;
  rdfs:label "bureaustoelen"@nl ;
  rdfs:label "desk chairs"@en ;
  rdfs:seeAlso <http://vocab.getty.edu/aat/300038165> ;
  rdfs:subClassOf <https://w3id.org/con-tax/components/aat-furn#300037772> ;
.
<https://w3id.org/con-tax/components/aat-furn#300038180>
  rdf:type owl:Class ;
  rdfs:comment "Devices which allow the motions of horse exercise to be simulated indoors, consisting of springs encased in a concertinalike leather envelope, framed in mahogany."@en ;
  rdfs:comment "Toestellen die binnenshuis staan en de bewegingen bij het paardrijden kunnen imiteren. Het toestel bestaat uit veren die in een leren omhulsel als een harmonica in elkaar schuiven. Het geraamte bestaat uit mahoniehout."@nl ;
  rdfs:isDefinedBy <https://w3id.org/con-tax/components/aat-furn> ;
  rdfs:label "chamber horse"@nl ;
  rdfs:label "chamber horses"@en ;
  rdfs:label "chamber horses"@nl ;
  rdfs:seeAlso <http://vocab.getty.edu/aat/300038180> ;
  rdfs:seeAlso wd:Q21550460 ;
  rdfs:subClassOf <https://w3id.org/con-tax/components/aat-furn#300037772> ;
.
<https://w3id.org/con-tax/components/aat-furn#300038184>
  rdf:type owl:Class ;
  rdfs:comment "Children's chairs with long legs, a feeding tray, and a footrest."@en ;
  rdfs:comment "Stoelen voor kinderen met lange poten, een etensblad en een voetensteun."@nl ;
  rdfs:isDefinedBy <https://w3id.org/con-tax/components/aat-furn> ;
  rdfs:label "highchairs (children's chairs)"@en ;
  rdfs:label "kinderstoel"@nl ;
  rdfs:label "kinderstoelen"@nl ;
  rdfs:seeAlso <http://vocab.getty.edu/aat/300038184> ;
  rdfs:seeAlso wd:Q1622390 ;
  rdfs:subClassOf <https://w3id.org/con-tax/components/aat-furn#300246035> ;
.
<https://w3id.org/con-tax/components/aat-furn#300038191>
  rdf:type owl:Class ;
  rdfs:comment "Benaming die van toepassing is op verschillende soorten stoelen uit het midden van de 19e eeuw die speciaal zijn ontworpen voor zieken en invaliden. Ze hebben vaak een palmechanisme voor het omhoog- of omlaagbrengen van de armleuningen, de rugleuning of het voetensteuntje, of grote wielen voor een gemakkelijke voortbeweging. Gebruik 'touring chairs' voor stoelen uit het eind van de 19e en het begin van de 20e eeuw die voornamelijk voor gebruik door toeristen op promenades waren bedoeld."@nl ;
  rdfs:comment "Term applied to a variety of mid-19th-century chairs designed especially for those who are sick or disabled and which often have ratchet mechanisms for raising and lowering the arms, back, or footrest or with large wheels for ease of motion. Use \"touring chairs\" for late 19th- and early 20th-century chairs intended primarily for tourists' use on boardwalks."@en ;
  rdfs:isDefinedBy <https://w3id.org/con-tax/components/aat-furn> ;
  rdfs:label "invalidenstoel"@nl ;
  rdfs:label "invalidenstoelen"@nl ;
  rdfs:label "invalids' chairs"@en ;
  rdfs:seeAlso <http://vocab.getty.edu/aat/300038191> ;
  rdfs:subClassOf <https://w3id.org/con-tax/components/aat-furn#300037772> ;
  rdfs:subClassOf <https://w3id.org/con-tax/components/aat-furn#300040036> ;
.
<https://w3id.org/con-tax/components/aat-furn#300038193>
  rdf:type owl:Class ;
  rdfs:comment "Wheel chairs, sometimes propelled and steered by turning winches on the arms, and having a foot rest designed to elevate the legs. Developed by John Joseph Merlin in the 18th century."@en ;
  rdfs:isDefinedBy <https://w3id.org/con-tax/components/aat-furn> ;
  rdfs:label "gouty chair"@nl ;
  rdfs:label "gouty chairs"@en ;
  rdfs:label "gouty chairs"@nl ;
  rdfs:seeAlso <http://vocab.getty.edu/aat/300038193> ;
  rdfs:subClassOf <https://w3id.org/con-tax/components/aat-furn#300038191> ;
.
<https://w3id.org/con-tax/components/aat-furn#300038205>
  rdf:type owl:Class ;
  rdfs:comment "Spaans-renaissancistische leunstoel met een rechthoekige, opgehangen zitting van leer en een leren of fluwelen rugleuning. Meestal zit er een brede dwarsbalk aan de voorkant die vaak is versierd met houtsnijwerk. Soms zijn ze voorzien van scharnieren zodat ze opklapbaar en makkelijk vervoerbaar zijn."@nl ;
  rdfs:comment "Spanish Renaissance type of armchair with a rectangular leather hung seat and with a leather or velvet back; generally having a broad front stretcher, which is often carved. Sometimes hinged to allow for folding and easy transportation."@en ;
  rdfs:isDefinedBy <https://w3id.org/con-tax/components/aat-furn> ;
  rdfs:label "frailero"@nl ;
  rdfs:label "fraileros"@en ;
  rdfs:label "fraileros"@nl ;
  rdfs:seeAlso <http://vocab.getty.edu/aat/300038205> ;
  rdfs:seeAlso wd:Q39737934 ;
  rdfs:subClassOf <https://w3id.org/con-tax/components/aat-furn#300037772> ;
.
<https://w3id.org/con-tax/components/aat-furn#300038208>
  rdf:type owl:Class ;
  rdfs:comment "Benaming die meestal van toepassing is op verschillende soorten stoelen met een verstelbare rugleuning en soms ook een verstelbare of roterende zitting die tijdens het spelen op een muziekinstrument wordt gebruikt. Gebruik 'muziekkruk' voor soortgelijke stoelen met roterende of verstelbare zitting zonder rugleuning die zijn bedoeld voor gebruik tijdens het spelen van de piano of andere muziekinstrumenten."@nl ;
  rdfs:comment "Term generally applied to a variety of chairs with adjustable back heights and sometimes adjustable or revolving seats intended for use while playing a musical instrument. Use \"music stools\" for similar seating with a revolving or adjustable seat but no back and intended for use while playing the piano or other musical instruments."@en ;
  rdfs:isDefinedBy <https://w3id.org/con-tax/components/aat-furn> ;
  rdfs:label "music chairs"@en ;
  rdfs:label "muziekstoel"@nl ;
  rdfs:label "muziekstoelen"@nl ;
  rdfs:seeAlso <http://vocab.getty.edu/aat/300038208> ;
  rdfs:subClassOf <https://w3id.org/con-tax/components/aat-furn#300037772> ;
.
<https://w3id.org/con-tax/components/aat-furn#300038217>
  rdf:type owl:Class ;
  rdfs:comment "Comfortable chairs for reading, particularly 18th-century armchairs with padded, leather-covered, saddle-shaped seats and an adjustable platform to hold a book projecting from the back; designed so that the occupant may either sit on it in a normal way or straddle the seat facing the back. For adjustable reading platforms that are not attached to chairs, use \"reading desks.\" For backward-facing chairs intended for viewing card games, use \"voyeuses.\""@en ;
  rdfs:comment "Luie stoelen om in te lezen. Soms wordt deze term gebruikt ter aanduiding van Engelse leunstoelen uit de 18e eeuw die een zadelvormige, leren zitting hebben met opvulling en een verstelbare verhoging die aan de rugleuning vastzit als boekenstandaard. Ze zijn zo ontworpen dat de zittende persoon op de normale manier plaats kan nemen of schrijlings met het gezicht naar de rugleuning gekeerd."@nl ;
  rdfs:isDefinedBy <https://w3id.org/con-tax/components/aat-furn> ;
  rdfs:label "leesstoel"@nl ;
  rdfs:label "leesstoelen"@nl ;
  rdfs:label "reading chairs"@en ;
  rdfs:seeAlso <http://vocab.getty.edu/aat/300038217> ;
  rdfs:subClassOf <https://w3id.org/con-tax/components/aat-furn#300037772> ;
  rdfs:subClassOf <https://w3id.org/con-tax/components/aat-furn#300037776> ;
.
<https://w3id.org/con-tax/components/aat-furn#300038220>
  rdf:type owl:Class ;
  rdfs:comment "Draagbare stoelen die op twee lange palen steunen en meestal uitvoerig zijn gestoffeerd en gedecoreerd. Gebruik 'brancards' voor het vervoer van één persoon die meestal bestaan uit canvas of soortgelijk materiaal dat over een draagstel wordt gespannen of gelegd om zo zieken, gewonden of doden te vervoeren. Gebruik 'draagkoetsen' voor meer uitgebreid vervoer dat doosvormig is, vaak door gordijnen wordt omsloten en door mensen of dieren op palen wordt gedragen."@nl ;
  rdfs:comment "Portable chairs borne on two long poles; generally with elaborate upholstery and decoration. For conveyances for one person consisting generally of canvas or similar material stretched or laid across a frame for transporting the sick, wounded, or dead use \"stretchers (conveyances).\" For more elaborate conveyances boxlike in form and often enclosed by curtains and carried on poles by people or animals use \"litters.\""@en ;
  rdfs:isDefinedBy <https://w3id.org/con-tax/components/aat-furn> ;
  rdfs:label "draagstoel"@nl ;
  rdfs:label "draagstoelen"@nl ;
  rdfs:label "sedan chairs"@en ;
  rdfs:seeAlso <http://vocab.getty.edu/aat/300038220> ;
  rdfs:seeAlso wd:Q476850 ;
  rdfs:subClassOf <https://w3id.org/con-tax/components/aat-furn#300037772> ;
.
<https://w3id.org/con-tax/components/aat-furn#300038224>
  rdf:type owl:Class ;
  rdfs:comment "Gestoffeerde leunstoelen met een rugleuning met oren die door middel van een palmechanisme in elke gewenste stand kan worden ingesteld. Ze kwamen voor het eerst voor ten tijde van de Restauratie."@nl ;
  rdfs:comment "Upholstered armchairs with a winged back which by means of a ratchet can be adjusted to any desired angle; first made in the Restoration period."@en ;
  rdfs:isDefinedBy <https://w3id.org/con-tax/components/aat-furn> ;
  rdfs:label "slaapstoel"@nl ;
  rdfs:label "slaapstoelen"@nl ;
  rdfs:label "sleeping chairs"@en ;
  rdfs:seeAlso <http://vocab.getty.edu/aat/300038224> ;
  rdfs:subClassOf <https://w3id.org/con-tax/components/aat-furn#300037772> ;
  rdfs:subClassOf <https://w3id.org/con-tax/components/aat-furn#300037776> ;
.
<https://w3id.org/con-tax/components/aat-furn#300038225>
  rdf:type owl:Class ;
  rdfs:comment "High-backed, low-seated chairs without arms and often upholstered; intended for bedroom use."@en ;
  rdfs:comment "Stoelen met een hoge rugleuning en een lage zitting, zonder armleuningen. Ze zijn vaak gestoffeerd en zijn bedoeld voor gebruik in de slaapkamer."@nl ;
  rdfs:isDefinedBy <https://w3id.org/con-tax/components/aat-furn> ;
  rdfs:label "slipper chair"@nl ;
  rdfs:label "slipper chairs"@en ;
  rdfs:label "slipper chairs"@nl ;
  rdfs:seeAlso <http://vocab.getty.edu/aat/300038225> ;
  rdfs:subClassOf <https://w3id.org/con-tax/components/aat-furn#300037772> ;
  rdfs:subClassOf <https://w3id.org/con-tax/components/aat-furn#300141151> ;
.
<https://w3id.org/con-tax/components/aat-furn#300038227>
  rdf:type owl:Class ;
  rdfs:comment "Chairs convertible into a stepladder."@en ;
  rdfs:comment "Stoelen die in een trapje kunnen worden veranderd."@nl ;
  rdfs:isDefinedBy <https://w3id.org/con-tax/components/aat-furn> ;
  rdfs:label "step chairs"@en ;
  rdfs:label "trapstoel"@nl ;
  rdfs:label "trapstoelen"@nl ;
  rdfs:seeAlso <http://vocab.getty.edu/aat/300038227> ;
  rdfs:subClassOf <https://w3id.org/con-tax/components/aat-furn#300037772> ;
.
<https://w3id.org/con-tax/components/aat-furn#300038228>
  rdf:type owl:Class ;
  rdfs:comment "Late 19th- and early 20th-century chairs intended primarily for tourists' use on boardwalks. Use \"invalids' chairs\" for chairs with ratchet mechanisms for raising or lowering arms, back, or footrest or with large wheels and designed especially for those who are sick or disabled."@en ;
  rdfs:comment "Stoelen uit het einde van de 19e en het begin van de 20e eeuw, die voornamelijk waren bedoeld voor gebruik door toeristen op de promenades. Gebruik 'invalidenstoelen' voor stoelen met een palmechanisme voor het omhoog- of omlaagbrengen van de armleuningen, rug, voetensteuntje of met grote wielen, die speciaal voor zieken of invaliden zijn ontworpen."@nl ;
  rdfs:isDefinedBy <https://w3id.org/con-tax/components/aat-furn> ;
  rdfs:label "touring chair"@nl ;
  rdfs:label "touring chairs"@en ;
  rdfs:label "touring chairs"@nl ;
  rdfs:seeAlso <http://vocab.getty.edu/aat/300038228> ;
  rdfs:subClassOf <https://w3id.org/con-tax/components/aat-furn#300037772> ;
.
<https://w3id.org/con-tax/components/aat-furn#300038229>
  rdf:type owl:Class ;
  rdfs:comment "Draaiende stoelen die meestal een rugleuning met veren hebben en in een kantoor worden gebruikt."@nl ;
  rdfs:comment "Revolving chairs, usually with a spring back, made for office use."@en ;
  rdfs:isDefinedBy <https://w3id.org/con-tax/components/aat-furn> ;
  rdfs:label "kantoorstoel"@nl ;
  rdfs:label "kantoorstoelen (stoelen naar functie)"@nl ;
  rdfs:label "kantoorstoelen"@nl ;
  rdfs:label "typewriter chairs"@en ;
  rdfs:seeAlso <http://vocab.getty.edu/aat/300038229> ;
  rdfs:subClassOf <https://w3id.org/con-tax/components/aat-furn#300037772> ;
.
<https://w3id.org/con-tax/components/aat-furn#300038232>
  rdf:type owl:Class ;
  rdfs:comment "Chairs having a rather low seat and a padded top rail, designed to allow male spectators of card games to astride while resting their arms or elbows on the top rail. The term is derived from the French verb \"voir,\" \"to see.\" First made in France about 1740 and later in England. For a lower-seated variant of this chair designed for women, use \"voyeuse á genoux.\" "@en ;
  rdfs:comment "Franse benaming uit de 18e eeuw voor stoelen met een lage zitting en een opgevuld bovenstuk aan de achterkant waarop een zittend persoon de ellebogen kan neerleggen als er schrijlings op de stoel wordt gezeten. Dit type werd voor het eerst gemaakt in Frankrijk rond 1740, en later ook in Engeland."@nl ;
  rdfs:isDefinedBy <https://w3id.org/con-tax/components/aat-furn> ;
  rdfs:label "kijkstoel"@nl ;
  rdfs:label "kijkstoelen"@nl ;
  rdfs:label "voyeuse"@nl ;
  rdfs:label "voyeuses"@en ;
  rdfs:label "voyeuses"@nl ;
  rdfs:seeAlso <http://vocab.getty.edu/aat/300038232> ;
  rdfs:seeAlso wd:Q21551087 ;
  rdfs:subClassOf <https://w3id.org/con-tax/components/aat-furn#300037772> ;
.
<https://w3id.org/con-tax/components/aat-furn#300038242>
  rdf:type owl:Class ;
  rdfs:comment "Chairs having a very low seat and a padded top rail, designed for female spectators of card games, who could kneel while resting their arms on the padded top rail. Males would sit astride a \"voyeuse\" with a somewhat higher seat, but it was considered inelegant for women to sit astride. For chairs having a very similar design but intended for prayer, use \"prie-dieu chairs.\" Prie-dieu chairs may be made of humble materials, such as a wooden frame with a rattan seat-kneeler, or they may be upholstered; they may include a shelf for prayer books. If they are part of a set, it is usually a bedroom set. Voyeuses à genoux are always upholstered, and are generally part of a larger set along with voyeuses intended for males."@en ;
  rdfs:comment "Een bepaald soort voyeuse die speciaal voor vrouwen was gemaakt om op te knielen, aangezien schrijlings zitten voor hen niet elegant werd gevonden."@nl ;
  rdfs:isDefinedBy <https://w3id.org/con-tax/components/aat-furn> ;
  rdfs:label "voyeuse à genoux"@nl ;
  rdfs:label "voyeuses à genoux"@en ;
  rdfs:label "voyeuses à genoux"@nl ;
  rdfs:seeAlso <http://vocab.getty.edu/aat/300038242> ;
  rdfs:subClassOf <https://w3id.org/con-tax/components/aat-furn#300038232> ;
  rdfs:subClassOf <https://w3id.org/con-tax/components/aat-furn#300137869> ;
  rdfs:subClassOf <https://w3id.org/con-tax/components/aat-furn#300141151> ;
.
<https://w3id.org/con-tax/components/aat-furn#300038243>
  rdf:type owl:Class ;
  rdfs:comment "Chairs mounted on wheels that may either be pushed or propelled by the occupant by means of hand rims attached to the two large side wheels."@en ;
  rdfs:comment "Stoelen met wielen die kunnen worden geduwd of door de zittende persoon kunnen worden voortbewogen door middel van handvelgen die aan de twee grote zijwielen zitten."@nl ;
  rdfs:isDefinedBy <https://w3id.org/con-tax/components/aat-furn> ;
  rdfs:label "rolstoel"@nl ;
  rdfs:label "rolstoelen"@nl ;
  rdfs:label "wheelchairs"@en ;
  rdfs:seeAlso <http://vocab.getty.edu/aat/300038243> ;
  rdfs:seeAlso wd:Q191931 ;
  rdfs:subClassOf <https://w3id.org/con-tax/components/aat-furn#300038191> ;
.
<https://w3id.org/con-tax/components/aat-furn#300038249>
  rdf:type owl:Class ;
  rdfs:comment "Chairs used for wheeling the elderly and the infirm through large gardens."@en ;
  rdfs:comment "Stoelen die werden gebruikt om bejaarden en zieken door grote tuinen te rijden."@nl ;
  rdfs:isDefinedBy <https://w3id.org/con-tax/components/aat-furn> ;
  rdfs:label "garden machines"@en ;
  rdfs:label "ziekenstoel"@nl ;
  rdfs:label "ziekenstoelen"@nl ;
  rdfs:seeAlso <http://vocab.getty.edu/aat/300038249> ;
  rdfs:subClassOf <https://w3id.org/con-tax/components/aat-furn#300038191> ;
.
<https://w3id.org/con-tax/components/aat-furn#300038252>
  rdf:type owl:Class ;
  rdfs:comment "Chairs having one flat arm wide enough to use as a writing surface, or with a small table surface attached to one arm."@en ;
  rdfs:comment "Leunstoelen met een platte armleuning die breed genoeg is om als schrijfblad te gebruiken."@nl ;
  rdfs:isDefinedBy <https://w3id.org/con-tax/components/aat-furn> ;
  rdfs:label "schrijfarmstoel"@nl ;
  rdfs:label "schrijfarmstoelen"@nl ;
  rdfs:label "tablet-arm chairs"@en ;
  rdfs:seeAlso <http://vocab.getty.edu/aat/300038252> ;
  rdfs:subClassOf <https://w3id.org/con-tax/components/aat-furn#300037772> ;
.
<https://w3id.org/con-tax/components/aat-furn#300038257>
  rdf:type gvp:GuideTerm ;
  rdfs:isDefinedBy <https://w3id.org/con-tax/components/aat-furn> ;
  rdfs:label "<chairs by design>"@en ;
  rdfs:label "<stoel naar ontwerp>"@nl ;
  rdfs:label "<stoelen naar ontwerp>"@nl ;
  rdfs:label "stoel naar ontwerp"@nl ;
  rdfs:label "stoelen naar ontwerp"@nl ;
  rdfs:seeAlso <http://vocab.getty.edu/aat/300038257> ;
  contax:containsConcept <https://w3id.org/con-tax/components/aat-furn#300038272> ;
  contax:containsConcept <https://w3id.org/con-tax/components/aat-furn#300038273> ;
  contax:containsConcept <https://w3id.org/con-tax/components/aat-furn#300038303> ;
  contax:containsConcept <https://w3id.org/con-tax/components/aat-furn#300038305> ;
  contax:containsConcept <https://w3id.org/con-tax/components/aat-furn#300244770> ;
.
<https://w3id.org/con-tax/components/aat-furn#300038272>
  rdf:type owl:Class ;
  rdfs:comment "Easy chairs with a back and footrest adjustable up or down to comfort the user."@en ;
  rdfs:comment "Luie stoelen die een verstelbare rugleuning en voetensteuntje hebben om de gebruiker comfort te bieden."@nl ;
  rdfs:isDefinedBy <https://w3id.org/con-tax/components/aat-furn> ;
  rdfs:label "ligstoel"@nl ;
  rdfs:label "ligstoelen"@nl ;
  rdfs:label "reclining chairs"@en ;
  rdfs:seeAlso <http://vocab.getty.edu/aat/300038272> ;
  rdfs:seeAlso wd:Q3067542 ;
  rdfs:subClassOf <https://w3id.org/con-tax/components/aat-furn#300037772> ;
.
<https://w3id.org/con-tax/components/aat-furn#300038273>
  rdf:type owl:Class ;
  rdfs:comment "Chairs having legs mounted on curved supports, usually bands of wood or metal, which allow the chair to be rocked back and forth."@en ;
  rdfs:isDefinedBy <https://w3id.org/con-tax/components/aat-furn> ;
  rdfs:label "berceuses"@nl ;
  rdfs:label "rocking chairs"@en ;
  rdfs:label "schommelstoel"@nl ;
  rdfs:label "schommelstoelen"@nl ;
  rdfs:seeAlso <http://vocab.getty.edu/aat/300038273> ;
  rdfs:seeAlso wd:Q14963 ;
  rdfs:subClassOf <https://w3id.org/con-tax/components/aat-furn#300037772> ;
.
<https://w3id.org/con-tax/components/aat-furn#300038280>
  rdf:type owl:Class ;
  rdfs:comment "19th-century American rocking chairs derived from Windsor chairs and having wooden seats that curve upwards to meet the spindles of the noticeably high, curved back with a scrolled top rail; usually grained or painted with fine ornamental detail."@en ;
  rdfs:comment "Amerikaanse schommelstoelen uit de 19e eeuw die afgeleid zijn van Windsorstoelen. Ze hebben een houten zitting die omhoog buigt naar de spijlen van de opmerkelijk hoge gewelfde rugleuning met omgekrulde bovenregel. Ze zijn meestal gedetailleerd beschilderd of bewerkt."@nl ;
  rdfs:isDefinedBy <https://w3id.org/con-tax/components/aat-furn> ;
  rdfs:label "Boston rockers"@en ;
  rdfs:label "Boston schommelstoel"@nl ;
  rdfs:label "Boston schommelstoelen"@nl ;
  rdfs:seeAlso <http://vocab.getty.edu/aat/300038280> ;
  rdfs:subClassOf <https://w3id.org/con-tax/components/aat-furn#300038273> ;
.
<https://w3id.org/con-tax/components/aat-furn#300038282>
  rdf:type owl:Class ;
  rdfs:comment "Popular term for mid-19th-century American rocking chairs with a high, upholstered back and seat and open arms with upholstered pads on the elbows."@en ;
  rdfs:comment "Veel gebruikte benaming voor Amerikaanse schommelstoelen uit het midden van de 19e eeuw met een hoge, gestoffeerde rugleuning en zitting en open armleuningen met beklede, opgevulde armen."@nl ;
  rdfs:isDefinedBy <https://w3id.org/con-tax/components/aat-furn> ;
  rdfs:label "Lincoln rockers"@en ;
  rdfs:label "Lincoln schommelstoel"@nl ;
  rdfs:label "Lincoln schommelstoelen"@nl ;
  rdfs:seeAlso <http://vocab.getty.edu/aat/300038282> ;
  rdfs:subClassOf <https://w3id.org/con-tax/components/aat-furn#300038273> ;
.
<https://w3id.org/con-tax/components/aat-furn#300038283>
  rdf:type owl:Class ;
  rdfs:comment "Low-seated chairs, with the seats between 13 and 15 inches high, without arms."@en ;
  rdfs:comment "Stoelen met een lage zitting, die ongeveer tussen de 32,5 en 37,5 cm hoog is, zonder armleuningen."@nl ;
  rdfs:isDefinedBy <https://w3id.org/con-tax/components/aat-furn> ;
  rdfs:label "nursing chairs"@en ;
  rdfs:label "zorg (stoelen naar functie)"@nl ;
  rdfs:label "zorg"@nl ;
  rdfs:label "zorgstoel"@nl ;
  rdfs:label "zorgstoelen"@nl ;
  rdfs:seeAlso <http://vocab.getty.edu/aat/300038283> ;
  rdfs:subClassOf <https://w3id.org/con-tax/components/aat-furn#300037772> ;
  rdfs:subClassOf <https://w3id.org/con-tax/components/aat-furn#300141151> ;
.
<https://w3id.org/con-tax/components/aat-furn#300038284>
  rdf:type owl:Class ;
  rdfs:comment "Rocking chairs which move upon a stationary base instead of rocking on curved bends."@en ;
  rdfs:comment "Schommelstoelen die op een vaste basis bewegen in plaats van op gebogen balken te schommelen."@nl ;
  rdfs:isDefinedBy <https://w3id.org/con-tax/components/aat-furn> ;
  rdfs:label "platform rocker"@nl ;
  rdfs:label "platform rockers"@en ;
  rdfs:label "platform rockers"@nl ;
  rdfs:seeAlso <http://vocab.getty.edu/aat/300038284> ;
  rdfs:subClassOf <https://w3id.org/con-tax/components/aat-furn#300038273> ;
.
<https://w3id.org/con-tax/components/aat-furn#300038303>
  rdf:type owl:Class ;
  rdfs:comment "Chairs that may be stacked on top of each other, usually for space-saving purposes."@en ;
  rdfs:isDefinedBy <https://w3id.org/con-tax/components/aat-furn> ;
  rdfs:label "stacking chairs"@en ;
  rdfs:label "stapelstoel"@nl ;
  rdfs:label "stapelstoelen"@nl ;
  rdfs:seeAlso <http://vocab.getty.edu/aat/300038303> ;
  rdfs:subClassOf <https://w3id.org/con-tax/components/aat-furn#300037772> ;
.
<https://w3id.org/con-tax/components/aat-furn#300038305>
  rdf:type owl:Class ;
  rdfs:comment "Chairs with a revolving seat on a fixed frame."@en ;
  rdfs:comment "Stoelen met een draaiende zitting die aan een vast frame is bevestigd."@nl ;
  rdfs:isDefinedBy <https://w3id.org/con-tax/components/aat-furn> ;
  rdfs:label "draaistoel"@nl ;
  rdfs:label "draaistoelen"@nl ;
  rdfs:label "swivel chairs"@en ;
  rdfs:seeAlso <http://vocab.getty.edu/aat/300038305> ;
  rdfs:seeAlso wd:Q3954162 ;
  rdfs:subClassOf <https://w3id.org/con-tax/components/aat-furn#300037772> ;
.
<https://w3id.org/con-tax/components/aat-furn#300038379>
  rdf:type owl:Class ;
  rdfs:comment "Chairs designed for and used at a dining table, intended for use while eating meals."@en ;
  rdfs:isDefinedBy <https://w3id.org/con-tax/components/aat-furn> ;
  rdfs:label "dining chairs"@en ;
  rdfs:label "eetkamerstoel"@nl ;
  rdfs:label "eetkamerstoelen"@nl ;
  rdfs:seeAlso <http://vocab.getty.edu/aat/300038379> ;
  rdfs:subClassOf <https://w3id.org/con-tax/components/aat-furn#300037772> ;
.
<https://w3id.org/con-tax/components/aat-furn#300038382>
  rdf:type owl:Class ;
  rdfs:comment "Chairs with elaborately carved or painted backs, frequently bearing emblems and coats of arms, and having solid wood seats often with hinged lids to reveal a storage compartment. Intended for use in halls and corridors."@en ;
  rdfs:comment "Stoelen met een uitvoerig met houtsnijwerk versierde of beschilderde rugleuning, meestal met een embleem en wapenschild. De massieve houten zitting heeft vaak een klep waaronder een opbergruimte zit. Ze zijn bedoeld voor gebruik in hallen en gangen."@nl ;
  rdfs:isDefinedBy <https://w3id.org/con-tax/components/aat-furn> ;
  rdfs:label "hall chairs"@en ;
  rdfs:label "halstoel"@nl ;
  rdfs:label "halstoelen"@nl ;
  rdfs:seeAlso <http://vocab.getty.edu/aat/300038382> ;
  rdfs:subClassOf <https://w3id.org/con-tax/components/aat-furn#300037772> ;
.
<https://w3id.org/con-tax/components/aat-furn#300038383>
  rdf:type owl:Class ;
  rdfs:comment "Chairs designed for use with kitchen tables."@en ;
  rdfs:isDefinedBy <https://w3id.org/con-tax/components/aat-furn> ;
  rdfs:label "keukenstoel"@nl ;
  rdfs:label "keukenstoelen"@nl ;
  rdfs:label "kitchen chairs"@en ;
  rdfs:seeAlso <http://vocab.getty.edu/aat/300038383> ;
  rdfs:subClassOf <https://w3id.org/con-tax/components/aat-furn#300037772> ;
.
<https://w3id.org/con-tax/components/aat-furn#300038386>
  rdf:type owl:Class ;
  rdfs:comment "Benaming die vanaf het midden van de 18e eeuw wordt gebruikt voor speciaal ontworpen '@side chairs' met uitvoerige ornamentatie. Ze waren bedoeld voor gebruik in eetkamers."@nl ;
  rdfs:comment "Contemporary term used from the mid-18th century for specially designed side chairs, often with elaborate ornamentation, intended for use in dining rooms."@en ;
  rdfs:isDefinedBy <https://w3id.org/con-tax/components/aat-furn> ;
  rdfs:label "parlor chairs"@en-us ;
  rdfs:label "salonstoel"@nl ;
  rdfs:label "salonstoelen"@nl ;
  rdfs:seeAlso <http://vocab.getty.edu/aat/300038386> ;
  rdfs:subClassOf <https://w3id.org/con-tax/components/aat-furn#300037896> ;
  rdfs:subClassOf <https://w3id.org/con-tax/components/aat-furn#300038379> ;
.
<https://w3id.org/con-tax/components/aat-furn#300038418>
  rdf:type owl:Class ;
  rdfs:comment "A seat for one person, often without a back. They were the most common type of seat furniture until the 19th century. Distinct from \"benches\" in that they seat only one person; usually distinguished from \"chairs\" in that they have no back; however, tall seating pieces at a bar or counter are called stools though they sometimes have backs. Generally made in two types; one supported on four straight legs and the other with legs arranged crosswise."@en ;
  rdfs:comment "Het meest algemene soort zitmeubel tot de 19e eeuw. Ze verschillen van 'banken' omdat er maar één persoon op past en worden meestal onderscheiden van 'stoelen' omdat ze geen rugleuning hebben. De hoge zitmeubels bij een bar of toonbank worden echter ook krukken genoemd, hoewel ze soms een rugleuning hebben. Ze worden meestal in twee typen uitgevoerd; het ene type heeft vier rechte poten en bij het andere type kruisen de poten elkaar."@nl ;
  rdfs:isDefinedBy <https://w3id.org/con-tax/components/aat-furn> ;
  rdfs:label "kruk"@nl ;
  rdfs:label "krukken"@nl ;
  rdfs:label "stools (seating furniture)"@en ;
  rdfs:seeAlso <http://vocab.getty.edu/aat/300038418> ;
  rdfs:seeAlso wd:Q33163 ;
  rdfs:subClassOf <https://w3id.org/con-tax/components/aat-furn#300037771> ;
  contax:containsGuideTerm <https://w3id.org/con-tax/components/aat-furn#300038421> ;
  contax:containsGuideTerm <https://w3id.org/con-tax/components/aat-furn#300165536> ;
  contax:containsGuideTerm <https://w3id.org/con-tax/components/aat-furn#300165537> ;
  contax:containsGuideTerm <https://w3id.org/con-tax/components/aat-furn#300165539> ;
.
<https://w3id.org/con-tax/components/aat-furn#300038421>
  rdf:type gvp:GuideTerm ;
  rdfs:isDefinedBy <https://w3id.org/con-tax/components/aat-furn> ;
  rdfs:label "<krukken naar vorm>"@nl ;
  rdfs:label "<stools by form>"@en ;
  rdfs:label "krukken naar vorm"@nl ;
  rdfs:seeAlso <http://vocab.getty.edu/aat/300038421> ;
  contax:containsConcept <https://w3id.org/con-tax/components/aat-furn#300038424> ;
  contax:containsConcept <https://w3id.org/con-tax/components/aat-furn#300038426> ;
  contax:containsConcept <https://w3id.org/con-tax/components/aat-furn#300038428> ;
  contax:containsConcept <https://w3id.org/con-tax/components/aat-furn#300038435> ;
  contax:containsConcept <https://w3id.org/con-tax/components/aat-furn#300038450> ;
  contax:containsConcept <https://w3id.org/con-tax/components/aat-furn#300038452> ;
  contax:containsConcept <https://w3id.org/con-tax/components/aat-furn#300038459> ;
  contax:containsConcept <https://w3id.org/con-tax/components/aat-furn#300038467> ;
  contax:containsConcept <https://w3id.org/con-tax/components/aat-furn#300038489> ;
  contax:containsConcept <https://w3id.org/con-tax/components/aat-furn#300133874> ;
  contax:containsConcept <https://w3id.org/con-tax/components/aat-furn#300170149> ;
  contax:containsConcept <https://w3id.org/con-tax/components/aat-furn#300170829> ;
.
<https://w3id.org/con-tax/components/aat-furn#300038422>
  rdf:type owl:Class ;
  rdfs:comment "High stools that are usually one of a row of such stools standing in front of a bar, often taking the form of a rounded seat fixed on a central post."@en ;
  rdfs:comment "Hoge krukken die meestal deel uitmaken van een reeks dezelfde krukken die voor een bar staan. Ze bestaan vaak uit een ronde zitting die op een centrale staander is bevestigd."@nl ;
  rdfs:isDefinedBy <https://w3id.org/con-tax/components/aat-furn> ;
  rdfs:label "barkruk"@nl ;
  rdfs:label "barkrukken"@nl ;
  rdfs:label "barstools"@en ;
  rdfs:seeAlso <http://vocab.getty.edu/aat/300038422> ;
  rdfs:seeAlso wd:Q376339 ;
  rdfs:subClassOf <https://w3id.org/con-tax/components/aat-furn#300038418> ;
.
<https://w3id.org/con-tax/components/aat-furn#300038424>
  rdf:type owl:Class ;
  rdfs:comment "Krukken waarbij de zitting met scharnieren aan de rand vastzit in de vorm van een kleine kist met deksel."@nl ;
  rdfs:comment "Stools with the seat board hinged to the seat-rail in the form of a small lidded chest."@en ;
  rdfs:isDefinedBy <https://w3id.org/con-tax/components/aat-furn> ;
  rdfs:label "box stool"@nl ;
  rdfs:label "box stools"@en ;
  rdfs:label "box stools"@nl ;
  rdfs:seeAlso <http://vocab.getty.edu/aat/300038424> ;
  rdfs:subClassOf <https://w3id.org/con-tax/components/aat-furn#300038418> ;
.
<https://w3id.org/con-tax/components/aat-furn#300038426>
  rdf:type owl:Class ;
  rdfs:comment "Kleine krukken die in kerken in Schotland werden gebruikt voordat de kerkbankjes werden geïntroduceerd."@nl ;
  rdfs:comment "Low stools used in churches in Scotland before pews were introduced."@en ;
  rdfs:isDefinedBy <https://w3id.org/con-tax/components/aat-furn> ;
  rdfs:label "cutty stools"@en ;
  rdfs:label "zondaarsbankje"@nl ;
  rdfs:label "zondaarsbankjes"@nl ;
  rdfs:seeAlso <http://vocab.getty.edu/aat/300038426> ;
  rdfs:seeAlso wd:Q5196966 ;
  rdfs:subClassOf <https://w3id.org/con-tax/components/aat-furn#300038418> ;
.
<https://w3id.org/con-tax/components/aat-furn#300038428>
  rdf:type owl:Class ;
  rdfs:comment "Ancient Greek stools without a back and having four turned legs, sometimes connected by stretchers."@en ;
  rdfs:comment "Oud-Griekse krukken zonder rugleunig met vier gedraaide poten die soms onderling zijn verbonden met dwarsbalken."@nl ;
  rdfs:isDefinedBy <https://w3id.org/con-tax/components/aat-furn> ;
  rdfs:label "diphroi"@en ;
  rdfs:label "diphroi"@nl ;
  rdfs:label "diphros"@nl ;
  rdfs:seeAlso <http://vocab.getty.edu/aat/300038428> ;
  rdfs:subClassOf <https://w3id.org/con-tax/components/aat-furn#300038418> ;
.
<https://w3id.org/con-tax/components/aat-furn#300038429>
  rdf:type owl:Class ;
  rdfs:comment "Krukken die als zitje voor een toilettafel zijn ontworpen. Ze werden in de 18e eeuw geïntroduceerd."@nl ;
  rdfs:comment "Stools designed as seats at dressing tables; introduced in the 18th century."@en ;
  rdfs:isDefinedBy <https://w3id.org/con-tax/components/aat-furn> ;
  rdfs:label "dressing stools"@en ;
  rdfs:label "toilettafelkruk"@nl ;
  rdfs:label "toilettafelkrukken"@nl ;
  rdfs:seeAlso <http://vocab.getty.edu/aat/300038429> ;
  rdfs:subClassOf <https://w3id.org/con-tax/components/aat-furn#300038418> ;
.
<https://w3id.org/con-tax/components/aat-furn#300038431>
  rdf:type owl:Class ;
  rdfs:comment "Long stools located near or extending from a fireplace fender. Popular in the 18th century."@en ;
  rdfs:isDefinedBy <https://w3id.org/con-tax/components/aat-furn> ;
  rdfs:label "fender stool"@nl ;
  rdfs:label "fender stools"@en ;
  rdfs:label "fender stools"@nl ;
  rdfs:seeAlso <http://vocab.getty.edu/aat/300038431> ;
  rdfs:subClassOf <https://w3id.org/con-tax/components/aat-furn#300038418> ;
.
<https://w3id.org/con-tax/components/aat-furn#300038435>
  rdf:type owl:Class ;
  rdfs:comment "Kleine, lage krukken die worden gebruikt om de voeten te ondersteunen."@nl ;
  rdfs:comment "Small, low stools, to support one's feet."@en ;
  rdfs:isDefinedBy <https://w3id.org/con-tax/components/aat-furn> ;
  rdfs:label "footstools (stools)"@en ;
  rdfs:label "voetenbankje"@nl ;
  rdfs:label "voetenbankjes"@nl ;
  rdfs:seeAlso <http://vocab.getty.edu/aat/300038435> ;
  rdfs:seeAlso wd:Q14973416 ;
  rdfs:subClassOf <https://w3id.org/con-tax/components/aat-furn#300038418> ;
.
<https://w3id.org/con-tax/components/aat-furn#300038438>
  rdf:type owl:Class ;
  rdfs:comment "Footstools with a padded top which may be adjusted to support a gouty foot at the least uncomfortable angle. Made mainly in 18th-century England."@en ;
  rdfs:comment "Voetenbankjes met een opgevuld bovenstuk dat verstelbaar is en als ondersteuning voor een jichtige voet kan dienen zodat deze zo comfortabel mogelijk ligt. Ze werden voornamelijk gemaakt in Engeland in de 18e eeuw."@nl ;
  rdfs:isDefinedBy <https://w3id.org/con-tax/components/aat-furn> ;
  rdfs:label "gout stools"@en ;
  rdfs:label "goutstool"@nl ;
  rdfs:label "goutstools"@nl ;
  rdfs:seeAlso <http://vocab.getty.edu/aat/300038438> ;
  rdfs:subClassOf <https://w3id.org/con-tax/components/aat-furn#300038435> ;
.
<https://w3id.org/con-tax/components/aat-furn#300038440>
  rdf:type owl:Class ;
  rdfs:comment "Grote opgevulde kussens die als zitplaats of beensteun dienst doen."@nl ;
  rdfs:comment "Large stuffed cushions that serve as seats or leg rests."@en ;
  rdfs:isDefinedBy <https://w3id.org/con-tax/components/aat-furn> ;
  rdfs:label "hassocks"@en ;
  rdfs:label "voetenkussen"@nl ;
  rdfs:label "voetenkussens"@nl ;
  rdfs:seeAlso <http://vocab.getty.edu/aat/300038440> ;
  rdfs:seeAlso wd:Q3545350 ;
  rdfs:subClassOf <https://w3id.org/con-tax/components/aat-furn#300038435> ;
.
<https://w3id.org/con-tax/components/aat-furn#300038442>
  rdf:type owl:Class ;
  rdfs:comment "Footstools with thickly padded upholstered tops."@en ;
  rdfs:comment "Te gebruiken voor voetenbankjes met een dik gestoffeerde, gevulde bovenzijde."@nl ;
  rdfs:isDefinedBy <https://w3id.org/con-tax/components/aat-furn> ;
  rdfs:label "ottomaans voetenbankje"@nl ;
  rdfs:label "ottomaanse voetenbankjes"@nl ;
  rdfs:label "ottoman footstools"@en ;
  rdfs:seeAlso <http://vocab.getty.edu/aat/300038442> ;
  rdfs:seeAlso wd:Q1286741 ;
  rdfs:subClassOf <https://w3id.org/con-tax/components/aat-furn#300038435> ;
.
<https://w3id.org/con-tax/components/aat-furn#300038449>
  rdf:type owl:Class ;
  rdfs:comment "Lage krukken die meestal drie poten hebben met een zware, ronde bovenkant op poten met ronde onderkanten."@nl ;
  rdfs:comment "Low, usually three-legged stools with heavy circular tops set on round-bottomed bases."@en ;
  rdfs:isDefinedBy <https://w3id.org/con-tax/components/aat-furn> ;
  rdfs:label "melkkruk"@nl ;
  rdfs:label "melkkrukken"@nl ;
  rdfs:label "milking stools"@en ;
  rdfs:seeAlso <http://vocab.getty.edu/aat/300038449> ;
  rdfs:subClassOf <https://w3id.org/con-tax/components/aat-furn#300038418> ;
.
<https://w3id.org/con-tax/components/aat-furn#300038450>
  rdf:type owl:Class ;
  rdfs:comment "Krukken die meestal een draaibare of verstelbare zitting hebben. Ze worden bij het pianospelen of het spelen van andere instrumenten gebruikt. Geef de voorkeur aan 'muziekstoelen' voor gelijksoortig zitmeubilair met verstelbare rugleuning en eventueel met verstelbare of draaibare zitting."@nl ;
  rdfs:comment "Stools generally having a revolving or adjustable seat and intended for use while playing the piano or other musical instrument. Prefer \"music chairs\" for similar forms of seating having an adjustable back and sometimes an adjustable or revolving seat."@en ;
  rdfs:isDefinedBy <https://w3id.org/con-tax/components/aat-furn> ;
  rdfs:label "music stools"@en ;
  rdfs:label "muziekkruk"@nl ;
  rdfs:label "muziekkrukken"@nl ;
  rdfs:seeAlso <http://vocab.getty.edu/aat/300038450> ;
  rdfs:subClassOf <https://w3id.org/con-tax/components/aat-furn#300038418> ;
.
<https://w3id.org/con-tax/components/aat-furn#300038452>
  rdf:type owl:Class ;
  rdfs:comment "Stools or low seats with brightly colored cushions, generally used by women."@en ;
  rdfs:isDefinedBy <https://w3id.org/con-tax/components/aat-furn> ;
  rdfs:label "placet"@nl ;
  rdfs:label "placets"@en ;
  rdfs:label "placets"@nl ;
  rdfs:seeAlso <http://vocab.getty.edu/aat/300038452> ;
  rdfs:subClassOf <https://w3id.org/con-tax/components/aat-furn#300038418> ;
.
<https://w3id.org/con-tax/components/aat-furn#300038454>
  rdf:type owl:Class ;
  rdfs:comment "Low, bench-like seats or kneelers used for prayer or meditation. Known in many cultures, including in Christianity and indigenous African cultures. For specifically Western Christian prayer furniture, 'prie-dieu (benches)' and 'prie-dieu chairs' are sometimes called 'prayer stools.'"@en ;
  rdfs:isDefinedBy <https://w3id.org/con-tax/components/aat-furn> ;
  rdfs:label "bidkruk"@nl ;
  rdfs:label "bidkrukken"@nl ;
  rdfs:label "prayer stools (stools, general)"@en ;
  rdfs:seeAlso <http://vocab.getty.edu/aat/300038454> ;
  rdfs:subClassOf <https://w3id.org/con-tax/components/aat-furn#300038418> ;
.
<https://w3id.org/con-tax/components/aat-furn#300038457>
  rdf:type owl:Class ;
  rdfs:comment "Krukken met een of twee treden die vaak onder de zitting zijn opgeklapt."@nl ;
  rdfs:comment "Stools with one or two steps that often fold away beneath the seat."@en ;
  rdfs:isDefinedBy <https://w3id.org/con-tax/components/aat-furn> ;
  rdfs:label "keukentrap"@nl ;
  rdfs:label "keukentrappen"@nl ;
  rdfs:label "step stools"@en ;
  rdfs:seeAlso <http://vocab.getty.edu/aat/300038457> ;
  rdfs:subClassOf <https://w3id.org/con-tax/components/aat-furn#300038418> ;
  rdfs:subClassOf <https://w3id.org/con-tax/components/aat-furn#300165788> ;
.
<https://w3id.org/con-tax/components/aat-furn#300038459>
  rdf:type owl:Class ;
  rdfs:comment "Refers to low seats or stools, without back or arms, often used for a child or as a footstool. It was originally in the shape of a drum, thus the name (from the diminutive of the French \"tambour,\" for drum). In the 18th century the term was applied to any low stool with fixed upright legs, as distinct from \"pliants,\" which had folding crossed legs. 18th-century tabourets were rectangular, not drum-shaped, with upholstered seats. For similar seats supported on six or more legs, use \"banquettes (benches).\""@en ;
  rdfs:comment "Stoeltje zonder leuning. Gebruik 'banquettes' voor soortgelijke stoelen met zes of meer poten."@nl ;
  rdfs:isDefinedBy <https://w3id.org/con-tax/components/aat-furn> ;
  rdfs:label "taboeret"@nl ;
  rdfs:label "taboeretten"@nl ;
  rdfs:label "tabourets (low stools)"@en ;
  rdfs:seeAlso <http://vocab.getty.edu/aat/300038459> ;
  rdfs:seeAlso wd:Q4733163 ;
  rdfs:subClassOf <https://w3id.org/con-tax/components/aat-furn#300038418> ;
.
<https://w3id.org/con-tax/components/aat-furn#300038461>
  rdf:type owl:Class ;
  rdfs:comment "Taboeretten uit de 18e eeuw die vaak overdadig zijn versierd met houtsnijwerk en soms aan drie kanten worden omsloten door een rugleuning,  zodat ze op het uiteinde van een miniatuur '@duchesse brisée' lijken."@nl ;
  rdfs:comment "Tabourets stools from the 18th-century, often lavishly carved and sometimes surrounded by a back on three sides so that they resembled the end of a miniature duchesse brisée."@en ;
  rdfs:isDefinedBy <https://w3id.org/con-tax/components/aat-furn> ;
  rdfs:label "tabouret en chancelière"@nl ;
  rdfs:label "tabourets en chancelière"@en ;
  rdfs:label "tabourets en chancelière"@nl ;
  rdfs:seeAlso <http://vocab.getty.edu/aat/300038461> ;
  rdfs:subClassOf <https://w3id.org/con-tax/components/aat-furn#300038459> ;
.
<https://w3id.org/con-tax/components/aat-furn#300038467>
  rdf:type owl:Class ;
  rdfs:comment "Applies to a variety of small stools, such as footstools, generally having splayed legs."@en ;
  rdfs:comment "Wordt gebruikt voor verschillende soorten kleine krukken, zoals  voetenbankjes, die meestal wijd uitlopende poten hebben."@nl ;
  rdfs:isDefinedBy <https://w3id.org/con-tax/components/aat-furn> ;
  rdfs:label "cricket stool"@nl ;
  rdfs:label "cricket stools"@en ;
  rdfs:label "cricket stools"@nl ;
  rdfs:seeAlso <http://vocab.getty.edu/aat/300038467> ;
  rdfs:seeAlso wd:Q21550512 ;
  rdfs:subClassOf <https://w3id.org/con-tax/components/aat-furn#300038418> ;
.
<https://w3id.org/con-tax/components/aat-furn#300038478>
  rdf:type owl:Class ;
  rdfs:comment "Franse krukken met gekruiste, inklapbare poten. Ze verschillen van 'taboeretten', die vaste, verticale poten hebben en in woonhuizen worden gebruikt. Gebruik 'bisschopskrukken' voor vouwstoelen met een kerkelijke oorsprong en gebruik ‘faldistoria’ voor vouwstoelen die door bisschoppen of andere prelaten in het koor van een kerk worden gebruikt."@nl ;
  rdfs:comment "French stools with folding crossed legs; distinct from \"tabourets\" which have fixed upright legs, and used in domestic environments. For folding stools with ecclesiastical origins generally, use \"faldstools.\" For folding chairs used by bishops or other prelates in the chancel of a church, use \"faldistories.\""@en ;
  rdfs:isDefinedBy <https://w3id.org/con-tax/components/aat-furn> ;
  rdfs:label "pliants (folding stools)"@en ;
  rdfs:label "pliants"@nl ;
  rdfs:seeAlso <http://vocab.getty.edu/aat/300038478> ;
  rdfs:subClassOf <https://w3id.org/con-tax/components/aat-furn#300244761> ;
.
<https://w3id.org/con-tax/components/aat-furn#300038482>
  rdf:type owl:Class ;
  rdfs:comment "Kleine opvouwbare krukken met een afneembare zitting van canvas of leer."@nl ;
  rdfs:comment "Small, folding stools with a detachable seat of canvas or leather."@en ;
  rdfs:isDefinedBy <https://w3id.org/con-tax/components/aat-furn> ;
  rdfs:label "campstools"@en ;
  rdfs:label "kampeerkruk"@nl ;
  rdfs:label "kampeerkrukken"@nl ;
  rdfs:seeAlso <http://vocab.getty.edu/aat/300038482> ;
  rdfs:seeAlso wd:Q2738685 ;
  rdfs:seeAlso wd:Q29347378 ;
  rdfs:subClassOf <https://w3id.org/con-tax/components/aat-furn#300244761> ;
.
<https://w3id.org/con-tax/components/aat-furn#300038483>
  rdf:type owl:Class ;
  rdfs:comment "Stools designed to placed or stacked on top of one another."@en ;
  rdfs:isDefinedBy <https://w3id.org/con-tax/components/aat-furn> ;
  rdfs:label "stacking stools"@en ;
  rdfs:label "stapelkruk"@nl ;
  rdfs:label "stapelkrukken"@nl ;
  rdfs:seeAlso <http://vocab.getty.edu/aat/300038483> ;
  rdfs:subClassOf <https://w3id.org/con-tax/components/aat-furn#300038418> ;
.
<https://w3id.org/con-tax/components/aat-furn#300038489>
  rdf:type owl:Class ;
  rdfs:comment "Early backless seating forms of stout mortise and tenon construction and with turned legs joined by stretchers."@en ;
  rdfs:comment "Een oude vorm van zitmeubilair, zonder rugleuning, met een stevige  pen-en-gatconstructie en gedraaide poten die met dwarsbalken zijn verbonden."@nl ;
  rdfs:isDefinedBy <https://w3id.org/con-tax/components/aat-furn> ;
  rdfs:label "joint stool"@nl ;
  rdfs:label "joint stools"@en ;
  rdfs:label "joint stools"@nl ;
  rdfs:seeAlso <http://vocab.getty.edu/aat/300038489> ;
  rdfs:subClassOf <https://w3id.org/con-tax/components/aat-furn#300038418> ;
.
<https://w3id.org/con-tax/components/aat-furn#300038493>
  rdf:type owl:Class ;
  rdfs:comment "Seating furniture produced for use by multiple persons. "@en ;
  rdfs:isDefinedBy <https://w3id.org/con-tax/components/aat-furn> ;
  rdfs:label "meubilair met meerdere zitplaatsen"@nl ;
  rdfs:label "multiple-seating furniture"@en ;
  rdfs:seeAlso <http://vocab.getty.edu/aat/300038493> ;
  rdfs:subClassOf <https://w3id.org/con-tax/components/aat-furn#300037769> ;
.
<https://w3id.org/con-tax/components/aat-furn#300038494>
  rdf:type owl:Class ;
  rdfs:comment "Long seats for two or more people, with or without a back, usually of wood, but also of stone, metal, or another material. A bench is distinguished from a stool by its greater length."@en ;
  rdfs:comment "Zitplaatsen voor twee of meer personen, meestal zonder rugleuning."@nl ;
  rdfs:isDefinedBy <https://w3id.org/con-tax/components/aat-furn> ;
  rdfs:label "bank (meubilair)"@nl ;
  rdfs:label "bank"@nl ;
  rdfs:label "banken (meubilair)"@nl ;
  rdfs:label "banken"@nl ;
  rdfs:label "benches (furniture)"@en ;
  rdfs:label "zitbank (meubilair)"@nl ;
  rdfs:label "zitbank"@nl ;
  rdfs:label "zitbanken (meubilair)"@nl ;
  rdfs:label "zitbanken"@nl ;
  rdfs:seeAlso <http://vocab.getty.edu/aat/300038494> ;
  rdfs:seeAlso wd:Q204776 ;
  rdfs:subClassOf <https://w3id.org/con-tax/components/aat-furn#300038493> ;
  contax:containsGuideTerm <https://w3id.org/con-tax/components/aat-furn#300165544> ;
  contax:containsGuideTerm <https://w3id.org/con-tax/components/aat-furn#300165548> ;
.
<https://w3id.org/con-tax/components/aat-furn#300038498>
  rdf:type owl:Class ;
  rdfs:comment "Kleine bankjes die meestal een gestoffeerde zitting hebben. Ze lijken op een verlengde taboeret met zes of meer poten."@nl ;
  rdfs:comment "Small benches usually with upholstered seats; in form they resemble a tabouret lengthened and supported on six or more legs."@en ;
  rdfs:isDefinedBy <https://w3id.org/con-tax/components/aat-furn> ;
  rdfs:label "banquettes (benches)"@en ;
  rdfs:label "muurbank (bank)"@nl ;
  rdfs:label "muurbank"@nl ;
  rdfs:label "muurbanken (banken)"@nl ;
  rdfs:label "muurbanken"@nl ;
  rdfs:seeAlso <http://vocab.getty.edu/aat/300038498> ;
  rdfs:seeAlso wd:Q590095 ;
  rdfs:subClassOf <https://w3id.org/con-tax/components/aat-furn#300038494> ;
.
<https://w3id.org/con-tax/components/aat-furn#300038502>
  rdf:type owl:Class ;
  rdfs:comment "Early American furniture for holding buckets. The furniture developed in Pennsylvania German communities in the 18th century, spread throughout the eastern United States and beyond by the 19th century. Early forms comprised a bench-like piece for holding buckets, but soon the form added shelves or cupboards with closed doors for holding water or milk buckets, cleaning supplies, or other kitchen or bathing supplies. May also be used for reproductions of this furniture form."@en ;
  rdfs:comment "Wandkasten met een onderste gedeelte dat met deuren wordt afgesloten waarachter melkemmers worden geplaatst, een open plank voor wateremmers en een bovengedeelte met ondiepe laden. Dit type werd gemaakt door de Duitsers in Pennsylvania."@nl ;
  rdfs:isDefinedBy <https://w3id.org/con-tax/components/aat-furn> ;
  rdfs:label "water bench"@nl ;
  rdfs:label "water benches"@en ;
  rdfs:label "water benches"@nl ;
  rdfs:seeAlso <http://vocab.getty.edu/aat/300038502> ;
  rdfs:subClassOf <https://w3id.org/con-tax/components/aat-furn#300039183> ;
.
<https://w3id.org/con-tax/components/aat-furn#300038507>
  rdf:type owl:Class ;
  rdfs:comment "Italiaanse, houten bankjes met een ruimte onder de zitting die vaak de vorm van een 'cassone' met een rechtopstaande rugleuning heeft."@nl ;
  rdfs:comment "Italian wood benches with a chest under the seat, in the form of a large cassone with back and arms added to form a settee or sofa with storage below. Loose cushions were used for comfort. The form was popular in Florence. "@en ;
  rdfs:isDefinedBy <https://w3id.org/con-tax/components/aat-furn> ;
  rdfs:label "cassapanca"@nl ;
  rdfs:label "cassapanca' s"@nl ;
  rdfs:label "cassapanche"@en ;
  rdfs:seeAlso <http://vocab.getty.edu/aat/300038507> ;
  rdfs:subClassOf <https://w3id.org/con-tax/components/aat-furn#300038494> ;
.
<https://w3id.org/con-tax/components/aat-furn#300038509>
  rdf:type owl:Class ;
  rdfs:comment "Benches that were historically seats for the deacons in early protestant church services; the style is now commonly seen in homes. The forms vary, but they are typically long enough for two or three sitters, with a wooden seat, often with a wooden back; the seat may comprise a hinged cover that opens to reveal storage. "@en ;
  rdfs:isDefinedBy <https://w3id.org/con-tax/components/aat-furn> ;
  rdfs:label "deacons' benches"@en ;
  rdfs:label "dekaanbank"@nl ;
  rdfs:label "dekaanbanken"@nl ;
  rdfs:seeAlso <http://vocab.getty.edu/aat/300038509> ;
  rdfs:subClassOf <https://w3id.org/con-tax/components/aat-furn#300038494> ;
.
<https://w3id.org/con-tax/components/aat-furn#300038514>
  rdf:type owl:Class ;
  rdfs:comment "Lange banken zonder rugleuning."@nl ;
  rdfs:comment "Long benches without a back."@en ;
  rdfs:isDefinedBy <https://w3id.org/con-tax/components/aat-furn> ;
  rdfs:label "forms (benches)"@en ;
  rdfs:label "schoolbank"@nl ;
  rdfs:label "schoolbanken"@nl ;
  rdfs:seeAlso <http://vocab.getty.edu/aat/300038514> ;
  rdfs:subClassOf <https://w3id.org/con-tax/components/aat-furn#300038494> ;
.
<https://w3id.org/con-tax/components/aat-furn#300038521>
  rdf:type owl:Class ;
  rdfs:comment "Bankachtige stoelen, vaak op een vaste plaats, die achterkanten hebben en toegankelijk zijn vanaf de gangpaden, voor het gebruik van een kerkgemeente."@nl ;
  rdfs:comment "Benchlike seats for the use of a church congregation. They are often fixed in place in rows, have backs and often walls, and are accessible by aisles."@en ;
  rdfs:isDefinedBy <https://w3id.org/con-tax/components/aat-furn> ;
  rdfs:label "kerkbank"@nl ;
  rdfs:label "kerkbanken"@nl ;
  rdfs:label "pews"@en ;
  rdfs:seeAlso <http://vocab.getty.edu/aat/300038521> ;
  rdfs:seeAlso wd:Q848162 ;
  rdfs:subClassOf <https://w3id.org/con-tax/components/aat-furn#300038494> ;
.
<https://w3id.org/con-tax/components/aat-furn#300038523>
  rdf:type owl:Class ;
  rdfs:comment "Banken die bij het pianospelen worden gebruikt. Ze hebben meestal een scharnierende zitting waaronder een bergruimte zit voor bladmuziek, boeken en ander soortgelijk materiaal. Ze worden vaak bijpassend bij een piano gemaakt en verkocht."@nl ;
  rdfs:comment "Benches intended for use at a piano, generally made with a hinged seat that opens to reveal a storage area for sheet music, books, and other such items; often made en suite with the piano with which it is sold."@en ;
  rdfs:isDefinedBy <https://w3id.org/con-tax/components/aat-furn> ;
  rdfs:label "piano benches"@en ;
  rdfs:label "pianobank"@nl ;
  rdfs:label "pianobanken"@nl ;
  rdfs:seeAlso <http://vocab.getty.edu/aat/300038523> ;
  rdfs:subClassOf <https://w3id.org/con-tax/components/aat-furn#300038494> ;
.
<https://w3id.org/con-tax/components/aat-furn#300038524>
  rdf:type owl:Class ;
  rdfs:comment "Benches used at picnics, used in conjuction with picnic tables, and typically fused to the table itself to create one piece of furniture. Commonly seen in parks and campgrounds."@en ;
  rdfs:isDefinedBy <https://w3id.org/con-tax/components/aat-furn> ;
  rdfs:label "picknickbank"@nl ;
  rdfs:label "picknickbanken"@nl ;
  rdfs:label "picnic benches"@en ;
  rdfs:seeAlso <http://vocab.getty.edu/aat/300038524> ;
  rdfs:subClassOf <https://w3id.org/con-tax/components/aat-furn#300038494> ;
  rdfs:subClassOf <https://w3id.org/con-tax/components/aat-furn#300165810> ;
.
<https://w3id.org/con-tax/components/aat-furn#300038532>
  rdf:type owl:Class ;
  rdfs:comment "Lange banken die in twee basistypen bestaan: een bank met armleuningen en een lage rug, en een bank met armleuningen, oren en een meestal massieve, hoge rugleuning. Gebruik 'box settles' voor een zittekist met een scharnierende zitting."@nl ;
  rdfs:comment "Long seats of two basic types: a low-back bench with arms and a bench with a high, usually solid, back and with arms and wings. For settles with hinged seats use \"box settles.\""@en ;
  rdfs:isDefinedBy <https://w3id.org/con-tax/components/aat-furn> ;
  rdfs:label "settles"@en ;
  rdfs:label "zittekist"@nl ;
  rdfs:label "zittekisten"@nl ;
  rdfs:seeAlso <http://vocab.getty.edu/aat/300038532> ;
  rdfs:subClassOf <https://w3id.org/con-tax/components/aat-furn#300038494> ;
  rdfs:subClassOf <https://w3id.org/con-tax/components/aat-furn#300164316> ;
.
<https://w3id.org/con-tax/components/aat-furn#300038534>
  rdf:type owl:Class ;
  rdfs:comment "Settles with a box seat with a hinged lid which allows access to a storage space beneath."@en ;
  rdfs:comment "Zittekisten waarbij onder de zitting een bergruimte zit die door middel van een scharnierende klep toegankelijk is."@nl ;
  rdfs:isDefinedBy <https://w3id.org/con-tax/components/aat-furn> ;
  rdfs:label "box settle"@nl ;
  rdfs:label "box settles"@en ;
  rdfs:label "box settles"@nl ;
  rdfs:seeAlso <http://vocab.getty.edu/aat/300038534> ;
  rdfs:subClassOf <https://w3id.org/con-tax/components/aat-furn#300038532> ;
.
<https://w3id.org/con-tax/components/aat-furn#300038552>
  rdf:type owl:Class ;
  rdfs:comment "Freestanding or built-in benches intended for use in the embrasure of a window."@en ;
  rdfs:comment "Wordt gebruikt voor vrijstaande of ingebouwde stoelen bij de vensteropening. Historische term."@nl ;
  rdfs:isDefinedBy <https://w3id.org/con-tax/components/aat-furn> ;
  rdfs:label "vensterbank (bank)"@nl ;
  rdfs:label "vensterbank"@nl ;
  rdfs:label "vensterbanken (banken)"@nl ;
  rdfs:label "vensterbanken"@nl ;
  rdfs:label "window seats"@en ;
  rdfs:seeAlso <http://vocab.getty.edu/aat/300038552> ;
  rdfs:subClassOf <https://w3id.org/con-tax/components/aat-furn#300038494> ;
  rdfs:subClassOf <https://w3id.org/con-tax/components/aat-furn#300040157> ;
.
<https://w3id.org/con-tax/components/aat-furn#300038555>
  rdf:type owl:Class ;
  rdfs:comment "Banquettes made to stand in the embrasure of a window."@en ;
  rdfs:comment "Muurbanken die bij een vensteropening staan."@nl ;
  rdfs:isDefinedBy <https://w3id.org/con-tax/components/aat-furn> ;
  rdfs:label "banquette de croisée"@nl ;
  rdfs:label "banquettes de croisée"@en ;
  rdfs:label "banquettes de croisée"@nl ;
  rdfs:seeAlso <http://vocab.getty.edu/aat/300038555> ;
  rdfs:subClassOf <https://w3id.org/con-tax/components/aat-furn#300038552> ;
.
<https://w3id.org/con-tax/components/aat-furn#300038583>
  rdf:type owl:Class ;
  rdfs:comment "Lange zitmeubels die aan een kant een ruggensteun hebben. Ze worden voornamelijk gebruikt als rustmeubel in plaats van zitmeubel. Ze verschillen van 'sofa's' die een rug met twee zijleuningen hebben en voornamelijk worden gebruikt om op te zitten in plaats van te liggen.."@nl ;
  rdfs:comment "Long seating forms with a back support and one end; primarily used for reclining rather than sitting. Distinct from \"sofas\" which have a back and two ends and are primarily used for sitting rather than reclining."@en ;
  rdfs:isDefinedBy <https://w3id.org/con-tax/components/aat-furn> ;
  rdfs:label "couches (reclining furniture)"@en ;
  rdfs:label "ligbank"@nl ;
  rdfs:label "ligbanken"@nl ;
  rdfs:seeAlso <http://vocab.getty.edu/aat/300038583> ;
  rdfs:subClassOf <https://w3id.org/con-tax/components/aat-furn#300037680> ;
.
<https://w3id.org/con-tax/components/aat-furn#300038586>
  rdf:type owl:Class ;
  rdfs:comment "Extended chairs, generally without arms, used for lounging with one backed end usually made to tilt; often supported on a stretcher frame with six or eight legs. Also, long, wide, sofalike seats, often with two low ends that somewhat resemble headboards or footboards, that can be used for sitting or sleeping. Daybeds are typically designed for one person to recline on and were historically sometimes used for the formal reception of visitors. They are generally placed against the wall or in a niche."@en ;
  rdfs:comment "Verlengde ruststoelen, meestal zonder armleuningen en met een rugleuning die tot horizontale positie versteld kan worden. Ze worden gebruikt om in te luieren en staan vaak op een stretcherframe met zes of acht poten. Wordt ook gebruikt voor lange, brede, sofa-achtige zitmeubels, vaak met twee lage uiteinden die enigszins doen denken aan het hoofd- of voeteneinde van een bed, welke kunnen worden gebruikt om op te zitten of slapen. Zitslaapbanken zijn meestal bedoeld voor één persoon om op te liggen, en zijn in de loop der geschiedenis ook wel gebruikt bij de formele ontvangst van gasten. Doorgaans staan ze tegen de muur of in een nis."@nl ;
  rdfs:isDefinedBy <https://w3id.org/con-tax/components/aat-furn> ;
  rdfs:label "daybeds"@en ;
  rdfs:label "slaapbanken"@nl ;
  rdfs:label "zitslaapbank"@nl ;
  rdfs:label "zitslaapbanken"@nl ;
  rdfs:seeAlso <http://vocab.getty.edu/aat/300038586> ;
  rdfs:seeAlso wd:Q5243076 ;
  rdfs:subClassOf <https://w3id.org/con-tax/components/aat-furn#300037680> ;
.
<https://w3id.org/con-tax/components/aat-furn#300038592>
  rdf:type owl:Class ;
  rdfs:comment "Benaming die tijdens de periode van de Griekse heropleving werd gebruikt voor een rustbank met gekrulde uiteinden die aan Griekse en Romeinse meubelontwerpen doen denken."@nl ;
  rdfs:comment "Term used during the Greek Revival era to describe the form of couch produced with scrolled ends reminiscent of Greek and Roman furniture designs."@en ;
  rdfs:isDefinedBy <https://w3id.org/con-tax/components/aat-furn> ;
  rdfs:label "Grecian couches"@en ;
  rdfs:label "Griekse rustbank"@nl ;
  rdfs:label "Griekse rustbanken"@nl ;
  rdfs:seeAlso <http://vocab.getty.edu/aat/300038592> ;
  rdfs:subClassOf <https://w3id.org/con-tax/components/aat-furn#300038583> ;
.
<https://w3id.org/con-tax/components/aat-furn#300038595>
  rdf:type owl:Class ;
  rdfs:comment "Refers to long seats with a back and usually arms; large enough for two or more persons. The terms sofa and settee are virtually interchangeable in 20th-century usage but there is a distinction between the two; a settee is less fully upholstered than a sofa and can even be unupholstered."@en ;
  rdfs:comment "Verwijst naar lange zitmeubelen die van een rugleuning en meestal van armleuningen zijn voorzien. Ze zijn groot genoeg voor twee of meer personen. Tussen de termen 'rustbank' en 'sofa' wordt tegenwoordig vrijwel geen onderscheid gemaakt, maar er is wel degelijk een verschil: een rustbank is minder volledig bekleed dan een sofa, en soms ontbreekt de bekleding zelfs geheel."@nl ;
  rdfs:isDefinedBy <https://w3id.org/con-tax/components/aat-furn> ;
  rdfs:label "rustbank"@nl ;
  rdfs:label "rustbanken"@nl ;
  rdfs:label "settees (multiple-seating furniture)"@en ;
  rdfs:seeAlso <http://vocab.getty.edu/aat/300038595> ;
  rdfs:subClassOf <https://w3id.org/con-tax/components/aat-furn#300038493> ;
.
<https://w3id.org/con-tax/components/aat-furn#300038599>
  rdf:type owl:Class ;
  rdfs:comment "Rustbanken die uit drie verbonden leunstoelen bestaan."@nl ;
  rdfs:comment "Settees formed of three linked armchairs."@en ;
  rdfs:isDefinedBy <https://w3id.org/con-tax/components/aat-furn> ;
  rdfs:label "indiscret"@nl ;
  rdfs:label "indiscrets"@en ;
  rdfs:label "indiscrets"@nl ;
  rdfs:seeAlso <http://vocab.getty.edu/aat/300038599> ;
  rdfs:subClassOf <https://w3id.org/con-tax/components/aat-furn#300038595> ;
.
<https://w3id.org/con-tax/components/aat-furn#300038601>
  rdf:type owl:Class ;
  rdfs:comment "Benaming uit de 19e en 20e eeuw die werd gebruikt voor kleine, beklede sofa's of '@settees' waarop twee mensen konden zitten."@nl ;
  rdfs:comment "Term used, from the 19th century on, for a small upholstered sofa or settee designed to seat two people."@en ;
  rdfs:isDefinedBy <https://w3id.org/con-tax/components/aat-furn> ;
  rdfs:label "causeuse"@nl ;
  rdfs:label "causeuses"@nl ;
  rdfs:label "cosy-corner"@nl ;
  rdfs:label "cosy-corners"@nl ;
  rdfs:label "love seats"@en ;
  rdfs:label "tweezitsbank"@nl ;
  rdfs:label "tweezitsbanken"@nl ;
  rdfs:seeAlso <http://vocab.getty.edu/aat/300038601> ;
  rdfs:seeAlso wd:Q10552078 ;
  rdfs:subClassOf <https://w3id.org/con-tax/components/aat-furn#300038595> ;
.
<https://w3id.org/con-tax/components/aat-furn#300038607>
  rdf:type owl:Class ;
  rdfs:comment "Backless upholstered seats, usually round, and large enough for several people."@en ;
  rdfs:comment "Beklede zitmeubelen zonder rugleuning die groot genoeg zijn voor meerdere personen en meestal een ronde vorm hebben."@nl ;
  rdfs:isDefinedBy <https://w3id.org/con-tax/components/aat-furn> ;
  rdfs:label "poef"@nl ;
  rdfs:label "poefen"@nl ;
  rdfs:label "pouffes"@en ;
  rdfs:seeAlso <http://vocab.getty.edu/aat/300038607> ;
  rdfs:seeAlso wd:Q3545350 ;
  rdfs:subClassOf <https://w3id.org/con-tax/components/aat-furn#300038493> ;
.
<https://w3id.org/con-tax/components/aat-furn#300038611>
  rdf:type owl:Class ;
  rdfs:comment "Kleine bankjes met twee of drie gecombineerde stoelrugleuningen. Ze hebben armleuningen, een rug en poten die lijken op die van de stoelen met open rug uit de betreffende periode."@nl ;
  rdfs:comment "Small sofas formed of two or three combined chair backs, with arms, backs, and legs similar to those of the open-back chairs of the particular period."@en ;
  rdfs:isDefinedBy <https://w3id.org/con-tax/components/aat-furn> ;
  rdfs:label "chair-back settee"@nl ;
  rdfs:label "chair-back settees"@en ;
  rdfs:label "chair-back settees"@nl ;
  rdfs:seeAlso <http://vocab.getty.edu/aat/300038611> ;
  rdfs:subClassOf <https://w3id.org/con-tax/components/aat-furn#300038595> ;
.
<https://w3id.org/con-tax/components/aat-furn#300038618>
  rdf:type owl:Class ;
  rdfs:comment "Settees consisting of a solid wooden seat into which separate members for the back and legs are round-tenoned, or pushed into drilled holes. This is in contrast to standard chairs, where the back legs and the uprights of the back are of one continuous piece. "@en ;
  rdfs:isDefinedBy <https://w3id.org/con-tax/components/aat-furn> ;
  rdfs:label "Windsor settees"@en ;
  rdfs:label "Windsor settees"@nl ;
  rdfs:seeAlso <http://vocab.getty.edu/aat/300038618> ;
  rdfs:subClassOf <https://w3id.org/con-tax/components/aat-furn#300038595> ;
.
<https://w3id.org/con-tax/components/aat-furn#300038634>
  rdf:type owl:Class ;
  rdfs:comment "Lange, beklede zitbanken met een rugleuning en twee armleuningen; worden hoofdzakelijk gebruikt om op te zitten en niet om op te liggen. Te onderscheiden van 'rustbanken (sofa's)', die een ruggensteun aan één kant hebben en die voornamelijk worden gebruikt om op te liggen en niet om op te zitten. Tussen de termen 'bank' en 'sofa' wordt tegenwoordig vrijwel geen onderscheid gemaakt, maar er is wel degelijk een verschil: een sofa is meestal volledig bekleed."@nl ;
  rdfs:comment "Long, upholstered seating objects with a back and two ends, and primarily used for sitting rather than reclining. Distinct from \"couches (reclining furniture)\" which have a back support and one end and are primarily used for reclining rather than sitting. The term \"sofa\" was first used in France at the end of the 17th century as an alternative for canapé. The terms sofa and settee are virtually interchangeable in 20th-century usage but there is a distinction between the two; a sofa is generally completely upholstered."@en ;
  rdfs:isDefinedBy <https://w3id.org/con-tax/components/aat-furn> ;
  rdfs:label "sofa"@nl ;
  rdfs:label "sofa's"@nl ;
  rdfs:label "sofas"@en ;
  rdfs:seeAlso <http://vocab.getty.edu/aat/300038634> ;
  rdfs:seeAlso wd:Q131514 ;
  rdfs:subClassOf <https://w3id.org/con-tax/components/aat-furn#300038493> ;
.
<https://w3id.org/con-tax/components/aat-furn#300038636>
  rdf:type owl:Class ;
  rdfs:comment "Types of sofas or settees that were developed in France in the 18th century and picked up by Thomas Chippendale and other furniture makers in Europe and North America. They are distinguished by having a rather delicate and curvilinear style, carved and polished exposed sections of the wood frame, with stuffed backs and seats, arms that may or may not be stuffed, and elegantly carved exposed legs. "@en ;
  rdfs:comment "Verwijst naar een Frans type zitbank met armsteunen."@nl ;
  rdfs:isDefinedBy <https://w3id.org/con-tax/components/aat-furn> ;
  rdfs:label "canape"@nl ;
  rdfs:label "canapés (elegant sofas)"@en ;
  rdfs:label "canapés"@nl ;
  rdfs:seeAlso <http://vocab.getty.edu/aat/300038636> ;
  rdfs:subClassOf <https://w3id.org/con-tax/components/aat-furn#300038634> ;
.
<https://w3id.org/con-tax/components/aat-furn#300038638>
  rdf:type owl:Class ;
  rdfs:comment "Frans soort ovale of ronde sofa met een beklede, pilaarachtige rugleuning in het middden van de zitting. Ze zijn bedoeld om in het midden van de kamer te staan."@nl ;
  rdfs:comment "Sofas that are oval or round in form, with an upholstered pillar-like back located in the center of the seating area. Intended to stand in the center of the room, with seating around all sides of the sofa. The form developed in France."@en ;
  rdfs:isDefinedBy <https://w3id.org/con-tax/components/aat-furn> ;
  rdfs:label "borne"@nl ;
  rdfs:label "borne's"@nl ;
  rdfs:label "bornes"@en ;
  rdfs:seeAlso <http://vocab.getty.edu/aat/300038638> ;
  rdfs:subClassOf <https://w3id.org/con-tax/components/aat-furn#300038634> ;
.
<https://w3id.org/con-tax/components/aat-furn#300038639>
  rdf:type owl:Class ;
  rdfs:comment "Historische term voor sofa's met een steile rugleuning die uit het einde van de 18e en begin van de 19e eeuw stammen."@nl ;
  rdfs:comment "Late 18th- and early 19th-century sofas having a high-pitch back."@en ;
  rdfs:isDefinedBy <https://w3id.org/con-tax/components/aat-furn> ;
  rdfs:label "cabriole sofa"@nl ;
  rdfs:label "cabriole sofa's"@nl ;
  rdfs:label "cabriole sofas"@en ;
  rdfs:seeAlso <http://vocab.getty.edu/aat/300038639> ;
  rdfs:subClassOf <https://w3id.org/con-tax/components/aat-furn#300038634> ;
.
<https://w3id.org/con-tax/components/aat-furn#300038644>
  rdf:type owl:Class ;
  rdfs:comment "Straight-fronted sofas with small triangular seats (sometimes detachable) set outside the arms at either end. For S-shaped sofas with ends curving inward so two people could sit face to face, use \"canapés à confident.\""@en ;
  rdfs:comment "Wordt gebruikt voor sofa's met een rechte voorkant en kleine, driehoekige zitplaatsen die aan de buitenkant van de armleuningen zitten en soms afneembaar zijn. Gebruik 'canapés à confident' voor sofa's met een S-vorm waarvan de zijleuningen naar binnen buigen zodat twee mensen met het gezicht naar elkaar toe kunnen zitten."@nl ;
  rdfs:isDefinedBy <https://w3id.org/con-tax/components/aat-furn> ;
  rdfs:label "confidantes"@en ;
  rdfs:label "confidente"@nl ;
  rdfs:label "confidentes"@nl ;
  rdfs:seeAlso <http://vocab.getty.edu/aat/300038644> ;
  rdfs:seeAlso wd:Q2992489 ;
  rdfs:subClassOf <https://w3id.org/con-tax/components/aat-furn#300038634> ;
.
<https://w3id.org/con-tax/components/aat-furn#300038659>
  rdf:type owl:Class ;
  rdfs:comment "Engelse benaming uit het eind van de 18de-eeuw voor lange, lage zitbanken met bekleding. De term 'ottomane' werd voor het eerst gebruikt in 'La Petite Maison' van Bastide, in 1753-1754. De Franse benaming is specifieker en verwijst meestal naar ottomanes op basis van ovale vormen, waarbij het ene uiteinde hoger is dan het andere."@nl ;
  rdfs:comment "Late 18th-century English name for long, low, upholstered sofas. The term 'ottoman' first appeared in Le Bastide's \"La Petite Maison\" of 1753-1754. The French term is more precise, usually referring more specifically to ottomans built on an oval plan with one end higher than the other."@en ;
  rdfs:isDefinedBy <https://w3id.org/con-tax/components/aat-furn> ;
  rdfs:label "ottomane"@nl ;
  rdfs:label "ottomanes"@nl ;
  rdfs:label "ottomans (sofas)"@en ;
  rdfs:seeAlso <http://vocab.getty.edu/aat/300038659> ;
  rdfs:subClassOf <https://w3id.org/con-tax/components/aat-furn#300038493> ;
.
<https://w3id.org/con-tax/components/aat-furn#300038669>
  rdf:type owl:Class ;
  rdfs:comment "Furniture made up of modular units capable of use separately or in various combinations."@en ;
  rdfs:comment "Meubilair dat uit losse standaard-eenheden bestaat die afzonderlijk of in verschillende combinaties kunnen worden gebruikt."@nl ;
  rdfs:isDefinedBy <https://w3id.org/con-tax/components/aat-furn> ;
  rdfs:label "sectional furniture"@en ;
  rdfs:label "sectional furniture"@nl ;
  rdfs:seeAlso <http://vocab.getty.edu/aat/300038669> ;
  rdfs:subClassOf <https://w3id.org/con-tax/components/aat-furn#300040039> ;
.
<https://w3id.org/con-tax/components/aat-furn#300038670>
  rdf:type owl:Class ;
  rdfs:comment "Sofa's die in bedden kunnen worden veranderd."@nl ;
  rdfs:comment "Sofas that can be converted into beds."@en ;
  rdfs:isDefinedBy <https://w3id.org/con-tax/components/aat-furn> ;
  rdfs:label "sofa beds"@en ;
  rdfs:label "sofabed"@nl ;
  rdfs:label "sofabedden"@nl ;
  rdfs:seeAlso <http://vocab.getty.edu/aat/300038670> ;
  rdfs:seeAlso wd:Q19953097 ;
  rdfs:subClassOf <https://w3id.org/con-tax/components/aat-furn#300038634> ;
  rdfs:subClassOf <https://w3id.org/con-tax/components/aat-furn#300038697> ;
  rdfs:subClassOf <https://w3id.org/con-tax/components/aat-furn#300038801> ;
.
<https://w3id.org/con-tax/components/aat-furn#300038671>
  rdf:type owl:Class ;
  rdfs:comment "Grote, beklede sofa's die vaak in een bed kunnen worden veranderd."@nl ;
  rdfs:comment "Large upholstered sofas, often convertible into beds."@en ;
  rdfs:isDefinedBy <https://w3id.org/con-tax/components/aat-furn> ;
  rdfs:label "davenport (sofa)"@nl ;
  rdfs:label "davenport"@nl ;
  rdfs:label "davenports (sofabedden)"@nl ;
  rdfs:label "davenports (sofas)"@en ;
  rdfs:label "davenports"@nl ;
  rdfs:seeAlso <http://vocab.getty.edu/aat/300038671> ;
  rdfs:subClassOf <https://w3id.org/con-tax/components/aat-furn#300038670> ;
.
<https://w3id.org/con-tax/components/aat-furn#300038689>
  rdf:type owl:Class ;
  rdfs:comment "Dik opgevulde, beklede sofa's waarvan het houtwerk niet zichtbaar is."@nl ;
  rdfs:comment "Sofas with heavily overstuffed ends and backs that have no exposed wood and together form a continuous line that typically terminates in spiral-curved arm rest. One end may be adjustable or removable. The legs may be exposed or not; if exposed, they are typically the only exposed wood on the piece. Chesterfields are often upholstered in leather, but may also be covered in various textile fabrics."@en ;
  rdfs:isDefinedBy <https://w3id.org/con-tax/components/aat-furn> ;
  rdfs:label "chesterfield (sofa's)"@nl ;
  rdfs:label "chesterfield"@nl ;
  rdfs:label "chesterfields (overstuffed sofas)"@en ;
  rdfs:label "chesterfields (sofa's)"@nl ;
  rdfs:label "chesterfields"@nl ;
  rdfs:seeAlso <http://vocab.getty.edu/aat/300038689> ;
  rdfs:subClassOf <https://w3id.org/con-tax/components/aat-furn#300038634> ;
.
<https://w3id.org/con-tax/components/aat-furn#300038694>
  rdf:type owl:Class ;
  rdfs:comment "Eenvoudige, beklede '@settees', meestal met spijlen in de rugleuning. Ze worden binnenshuis of in een wagen gebruikt."@nl ;
  rdfs:comment "Plain, unupholstered settees, usually with slat backs, for use either indoors or in a wagon."@en ;
  rdfs:isDefinedBy <https://w3id.org/con-tax/components/aat-furn> ;
  rdfs:label "wagenbank"@nl ;
  rdfs:label "wagenbanken"@nl ;
  rdfs:label "wagon seats"@en ;
  rdfs:seeAlso <http://vocab.getty.edu/aat/300038694> ;
  rdfs:subClassOf <https://w3id.org/con-tax/components/aat-furn#300038493> ;
.
<https://w3id.org/con-tax/components/aat-furn#300038696>
  rdf:type gvp:GuideTerm ;
  rdfs:isDefinedBy <https://w3id.org/con-tax/components/aat-furn> ;
  rdfs:label "<ligmeubels>"@nl ;
  rdfs:label "<sleeping and reclining furniture>"@en ;
  rdfs:label "ligmeubels"@nl ;
  rdfs:seeAlso <http://vocab.getty.edu/aat/300038696> ;
  contax:containsConcept <https://w3id.org/con-tax/components/aat-furn#300038151> ;
  contax:containsConcept <https://w3id.org/con-tax/components/aat-furn#300038583> ;
  contax:containsConcept <https://w3id.org/con-tax/components/aat-furn#300038586> ;
  contax:containsConcept <https://w3id.org/con-tax/components/aat-furn#300038697> ;
  contax:containsConcept <https://w3id.org/con-tax/components/aat-furn#300134616> ;
  contax:containsConcept <https://w3id.org/con-tax/components/aat-furn#300137869> ;
  contax:containsConcept <https://w3id.org/con-tax/components/aat-furn#300375158> ;
  contax:containsGuideTerm <https://w3id.org/con-tax/components/aat-furn#300435632> ;
.
<https://w3id.org/con-tax/components/aat-furn#300038697>
  rdf:type owl:Class ;
  rdfs:comment "Generally, the sleeping places of humans and animals. Specifically, permanent pieces of furniture comprised of a bedstead, which is the wooden or metal support, and the bedding, including the mattress and cover."@en ;
  rdfs:comment "In algemene zin, de slaapplaats van mensen en dieren. In specifieke zin, permanente meubelstukken die bestaan uit een ledikant, het uit hout of metaal vervaardigde dragende gedeelte, en het beddengoed, met inbegrip van matras en dekens."@nl ;
  rdfs:isDefinedBy <https://w3id.org/con-tax/components/aat-furn> ;
  rdfs:label "bed"@nl ;
  rdfs:label "bedden (meubilair)"@nl ;
  rdfs:label "bedden"@nl ;
  rdfs:label "beds (furniture)"@en ;
  rdfs:seeAlso <http://vocab.getty.edu/aat/300038697> ;
  rdfs:seeAlso wd:Q42177 ;
  rdfs:subClassOf <https://w3id.org/con-tax/components/aat-furn#300037680> ;
  contax:containsGuideTerm <https://w3id.org/con-tax/components/aat-furn#300038776> ;
.
<https://w3id.org/con-tax/components/aat-furn#300038700>
  rdf:type owl:Class ;
  rdfs:comment "Bedden die, behalve aan de kant van de gordijnopening, aan elke zijde door panelen werden omsloten. Ze stonden meestal tegen de wand maar werden soms ook in de wand ingebouwd of in de lambrisering geïntegreerd."@nl ;
  rdfs:comment "Beds enclosed with paneling on all sides but one, where there was a curtain over the opening; usually stood against the wall and, in some cases, were built into the wall or incorporated into the scheme of paneling."@en ;
  rdfs:isDefinedBy <https://w3id.org/con-tax/components/aat-furn> ;
  rdfs:label "bedstede"@nl ;
  rdfs:label "bedsteden"@nl ;
  rdfs:label "bedstee"@nl ;
  rdfs:label "box beds"@en ;
  rdfs:seeAlso <http://vocab.getty.edu/aat/300038700> ;
  rdfs:seeAlso wd:Q2378930 ;
  rdfs:subClassOf <https://w3id.org/con-tax/components/aat-furn#300038697> ;
.
<https://w3id.org/con-tax/components/aat-furn#300038704>
  rdf:type owl:Class ;
  rdfs:comment "Bedden die worden gebruikt voor twee mensen waarbij de ene slaapplaats bovenop de ander is gestapeld."@nl ;
  rdfs:comment "Beds for two people with one sleeping place above the other in the manner of tiered bunks."@en ;
  rdfs:isDefinedBy <https://w3id.org/con-tax/components/aat-furn> ;
  rdfs:label "bunk beds"@en ;
  rdfs:label "stapelbed"@nl ;
  rdfs:label "stapelbedden"@nl ;
  rdfs:seeAlso <http://vocab.getty.edu/aat/300038704> ;
  rdfs:seeAlso wd:Q594918 ;
  rdfs:subClassOf <https://w3id.org/con-tax/components/aat-furn#300038697> ;
.
<https://w3id.org/con-tax/components/aat-furn#300038710>
  rdf:type owl:Class ;
  rdfs:comment "Bedden met overkappingen die alleen het hoofdeinde van het bed bedekken."@nl ;
  rdfs:comment "Beds with testers which only cover the head half of the bed."@en ;
  rdfs:isDefinedBy <https://w3id.org/con-tax/components/aat-furn> ;
  rdfs:label "half-tester bed"@nl ;
  rdfs:label "half-tester beds"@en ;
  rdfs:label "half-tester beds"@nl ;
  rdfs:seeAlso <http://vocab.getty.edu/aat/300038710> ;
  rdfs:seeAlso wd:Q26879928 ;
  rdfs:subClassOf <https://w3id.org/con-tax/components/aat-furn#300038697> ;
.
<https://w3id.org/con-tax/components/aat-furn#300038715>
  rdf:type owl:Class ;
  rdfs:comment "Bedden met een baldakijn dat aan de wand achter het hoofd of aan het plafond is bevestigd en niet door posten of zuilen wordt ondersteund."@nl ;
  rdfs:comment "Beds with a canopy, often suspended from an ornate horizontal frame, attached to the wall behind the head or to the ceiling and not supported on posts or columns. The term refers particularly to beds dating from the 17th century and later. For beds having simpler unsupported curtains, spanning a space shorter than the length bed, use \"lits d'ange.\""@en ;
  rdfs:isDefinedBy <https://w3id.org/con-tax/components/aat-furn> ;
  rdfs:label "lit à la duchesse"@nl ;
  rdfs:label "lits à la duchesse"@en ;
  rdfs:label "lits à la duchesse"@nl ;
  rdfs:seeAlso <http://vocab.getty.edu/aat/300038715> ;
  rdfs:subClassOf <https://w3id.org/con-tax/components/aat-furn#300142742> ;
.
<https://w3id.org/con-tax/components/aat-furn#300038716>
  rdf:type owl:Class ;
  rdfs:comment "Bedden met een zwevend baldakijn dat korter is dan het bed zelf; een lit d'ange is niet voorzien van stijlen."@nl ;
  rdfs:comment "Beds with an unsupported canopy, typically shorter than the bed; there are no posts on a lit d'ange, although sometimes the term is used incorrectly to refer to types of canopy beds with posts. For grander beds with a frame supporting the canopy, use \"lits à la duchesse.\""@en ;
  rdfs:isDefinedBy <https://w3id.org/con-tax/components/aat-furn> ;
  rdfs:label "lit d'ange"@nl ;
  rdfs:label "lits d'ange"@en ;
  rdfs:label "lits d'ange"@nl ;
  rdfs:seeAlso <http://vocab.getty.edu/aat/300038716> ;
  rdfs:subClassOf <https://w3id.org/con-tax/components/aat-furn#300142742> ;
.
<https://w3id.org/con-tax/components/aat-furn#300038719>
  rdf:type owl:Class ;
  rdfs:comment "Bedden met een frame uit drie delen, uitgerust met springveren die het hoofd, voeteneind of midden van het bed op gewenste hoogte kunnen brengen."@nl ;
  rdfs:comment "Beds with frames in three sections equipped with mechanical spring parts that permit raising the head, foot, or middle as required."@en ;
  rdfs:isDefinedBy <https://w3id.org/con-tax/components/aat-furn> ;
  rdfs:label "hospital beds"@en ;
  rdfs:label "ziekenhuisbed"@nl ;
  rdfs:label "ziekenhuisbedden"@nl ;
  rdfs:seeAlso <http://vocab.getty.edu/aat/300038719> ;
  rdfs:seeAlso wd:Q142259 ;
  rdfs:subClassOf <https://w3id.org/con-tax/components/aat-furn#300038697> ;
.
<https://w3id.org/con-tax/components/aat-furn#300038721>
  rdf:type owl:Class ;
  rdfs:comment "Benaming die werd gebruikt voor Franse bedden uit het begin van de 19e eeuw die op klassieke modellen waren gebaseerd."@nl ;
  rdfs:comment "Early 19th-century French beds having styles based on Classical models."@en ;
  rdfs:isDefinedBy <https://w3id.org/con-tax/components/aat-furn> ;
  rdfs:label "lit à l'antique"@nl ;
  rdfs:label "lits à l'antique"@en ;
  rdfs:label "lits à l'antique"@nl ;
  rdfs:seeAlso <http://vocab.getty.edu/aat/300038721> ;
  rdfs:subClassOf <https://w3id.org/con-tax/components/aat-furn#300038697> ;
.
<https://w3id.org/con-tax/components/aat-furn#300038723>
  rdf:type owl:Class ;
  rdfs:comment "Bedden die voor gebruik van bedienden waren. Deze benaming wordt vaak aangetroffen op 16e- en 17e-eeuwse inventarislijsten."@nl ;
  rdfs:comment "Beds for servants' use; term frequently found in 16th- and 17th-century inventories."@en ;
  rdfs:isDefinedBy <https://w3id.org/con-tax/components/aat-furn> ;
  rdfs:label "livery bed"@nl ;
  rdfs:label "livery beds"@en ;
  rdfs:label "livery beds"@nl ;
  rdfs:seeAlso <http://vocab.getty.edu/aat/300038723> ;
  rdfs:subClassOf <https://w3id.org/con-tax/components/aat-furn#300038697> ;
.
<https://w3id.org/con-tax/components/aat-furn#300038725>
  rdf:type owl:Class ;
  rdfs:comment "Bedden die vanaf ongeveer 1930 in Scandinavië werden gebouwd. Ze bestaan uit een eenvoudige, ondiepe kist waar een matras in ligt op een iets verzonken frame."@nl ;
  rdfs:comment "Beds, originating in Scandinavia in the 1930s, consisting of a simple shallow box for holding a mattress situated on a slightly recessed frame."@en ;
  rdfs:isDefinedBy <https://w3id.org/con-tax/components/aat-furn> ;
  rdfs:label "Zweeds bed"@nl ;
  rdfs:label "Zweedse bedden"@nl ;
  rdfs:label "platform beds"@en ;
  rdfs:seeAlso <http://vocab.getty.edu/aat/300038725> ;
  rdfs:subClassOf <https://w3id.org/con-tax/components/aat-furn#300038697> ;
.
<https://w3id.org/con-tax/components/aat-furn#300038732>
  rdf:type owl:Class ;
  rdfs:comment "Bedden met twee of vier posten die een hoogte van ongeveer 1.80 cm hebben en meestal een overkapping ondersteunen."@nl ;
  rdfs:comment "Beds with two or four posts approximately six feet in height which often, but not always, support a tester."@en ;
  rdfs:isDefinedBy <https://w3id.org/con-tax/components/aat-furn> ;
  rdfs:label "high-post bed"@nl ;
  rdfs:label "high-post beds"@en ;
  rdfs:label "high-post beds"@nl ;
  rdfs:seeAlso <http://vocab.getty.edu/aat/300038732> ;
  rdfs:subClassOf <https://w3id.org/con-tax/components/aat-furn#300038697> ;
.
<https://w3id.org/con-tax/components/aat-furn#300038737>
  rdf:type owl:Class ;
  rdfs:comment "Bedden met een dakachtig onderdeel dat boven het bed door posten wordt ondersteund. Gebruik 'half-tester beds' voor bedden met een overkapping die alleen het hoofdeinde van het bed overdekt. Gebruik 'hemelbedden' wanneer het dakachtige onderdeel aan het plafond wordt gehangen in plaats van door posten te worden ondersteund."@nl ;
  rdfs:comment "Beds with a rooflike component supported above the bed by the bed posts. For beds with testers that only cover the head half of the bed, use \"half-tester beds.\" Use \"canopy beds\" when the rooflike component is suspended from the ceiling or the wall, as opposed to being supported on posts."@en ;
  rdfs:isDefinedBy <https://w3id.org/con-tax/components/aat-furn> ;
  rdfs:label "baldakijnbed"@nl ;
  rdfs:label "baldakijnbedden"@nl ;
  rdfs:label "tester beds"@en ;
  rdfs:seeAlso <http://vocab.getty.edu/aat/300038737> ;
  rdfs:subClassOf <https://w3id.org/con-tax/components/aat-furn#300038732> ;
.
<https://w3id.org/con-tax/components/aat-furn#300038744>
  rdf:type owl:Class ;
  rdfs:comment "Canopy beds having an upper portion in the shape of a dome over the bed, from which the curtains are suspended."@en ;
  rdfs:isDefinedBy <https://w3id.org/con-tax/components/aat-furn> ;
  rdfs:label "dome bed"@nl ;
  rdfs:label "dome beds"@en ;
  rdfs:label "dome beds"@nl ;
  rdfs:seeAlso <http://vocab.getty.edu/aat/300038744> ;
  rdfs:subClassOf <https://w3id.org/con-tax/components/aat-furn#300142742> ;
.
<https://w3id.org/con-tax/components/aat-furn#300038745>
  rdf:type owl:Class ;
  rdfs:comment "High-post beds with arched, or in the Federal period often serpentine, as opposed to straight canopies and whose posts are generally less than six feet in height."@en ;
  rdfs:comment "Wordt gebruikt voor '@high-post beds' met een gewelfde in plaats van een rechte hemel. In de Federale periode werd ook vaak een hemel met slingers gebruikt. De posten zijn meestal minder dan 1.80 cm hoog."@nl ;
  rdfs:isDefinedBy <https://w3id.org/con-tax/components/aat-furn> ;
  rdfs:label "field beds"@en ;
  rdfs:label "veldbed"@nl ;
  rdfs:label "veldbedden"@nl ;
  rdfs:seeAlso <http://vocab.getty.edu/aat/300038745> ;
  rdfs:subClassOf <https://w3id.org/con-tax/components/aat-furn#300038737> ;
.
<https://w3id.org/con-tax/components/aat-furn#300038753>
  rdf:type owl:Class ;
  rdfs:comment "Bedden met zes- of achthoekige posten, waarvan men meestal aanneemt dat ze vóór de Amerikaanse Onafhankelijkheidsoorlog werden gemaakt."@nl ;
  rdfs:comment "Beds with hexagonal or octagonal posts, usually thought to have been made prior to the American Revolution."@en ;
  rdfs:isDefinedBy <https://w3id.org/con-tax/components/aat-furn> ;
  rdfs:label "pencil-post bed"@nl ;
  rdfs:label "pencil-post beds"@en ;
  rdfs:label "pencil-post beds"@nl ;
  rdfs:seeAlso <http://vocab.getty.edu/aat/300038753> ;
  rdfs:subClassOf <https://w3id.org/con-tax/components/aat-furn#300038732> ;
.
<https://w3id.org/con-tax/components/aat-furn#300038754>
  rdf:type owl:Class ;
  rdfs:comment "Bedden met twee of vier posten met een hoogte van ongeveer 1,20 cm."@nl ;
  rdfs:comment "Beds with two or four posts approximately four feet in height."@en ;
  rdfs:isDefinedBy <https://w3id.org/con-tax/components/aat-furn> ;
  rdfs:label "low-post bed"@nl ;
  rdfs:label "low-post beds"@en ;
  rdfs:label "low-post beds"@nl ;
  rdfs:seeAlso <http://vocab.getty.edu/aat/300038754> ;
  rdfs:subClassOf <https://w3id.org/con-tax/components/aat-furn#300038697> ;
.
<https://w3id.org/con-tax/components/aat-furn#300038756>
  rdf:type owl:Class ;
  rdfs:comment "Settles convertible into beds."@en ;
  rdfs:comment "Zittekisten die in bedden kunnen worden veranderd."@nl ;
  rdfs:isDefinedBy <https://w3id.org/con-tax/components/aat-furn> ;
  rdfs:label "settle bed"@nl ;
  rdfs:label "settle beds"@en ;
  rdfs:label "settle beds"@nl ;
  rdfs:seeAlso <http://vocab.getty.edu/aat/300038756> ;
  rdfs:subClassOf <https://w3id.org/con-tax/components/aat-furn#300038532> ;
  rdfs:subClassOf <https://w3id.org/con-tax/components/aat-furn#300038697> ;
.
<https://w3id.org/con-tax/components/aat-furn#300038758>
  rdf:type owl:Class ;
  rdfs:comment "Beds with two ends of equal height intended to stand lengthwise along the wall. For beds with a simple wooden framework, which supports the bed hangings so as to form a plain, rectangular box, use \"French beds.\""@en ;
  rdfs:comment "Te gebruiken voor bedden met twee uiteinden op dezelfde hoogte die in de lengte tegen de muur dienen te staan. Gebruik 'Franse bedden' voor bedden met een eenvoudig houten raamwerk waaraan de bedbehangsels zijn opgehangen zodat ze een vlakke, rechthoekige 'doos' vormen."@nl ;
  rdfs:isDefinedBy <https://w3id.org/con-tax/components/aat-furn> ;
  rdfs:label "sledebed"@nl ;
  rdfs:label "sledebedden"@nl ;
  rdfs:label "sleigh beds"@en ;
  rdfs:seeAlso <http://vocab.getty.edu/aat/300038758> ;
  rdfs:subClassOf <https://w3id.org/con-tax/components/aat-furn#300038697> ;
.
<https://w3id.org/con-tax/components/aat-furn#300038770>
  rdf:type owl:Class ;
  rdfs:comment "Bedden met een gestoffeerde achterkant en uiteindes die op gelijke hoogte zitten."@nl ;
  rdfs:comment "Beds with ends of equal height and an upholstered back."@en ;
  rdfs:isDefinedBy <https://w3id.org/con-tax/components/aat-furn> ;
  rdfs:label "lit à la turque"@nl ;
  rdfs:label "lits à la turque (sleigh beds)"@en ;
  rdfs:label "lits à la turque"@nl ;
  rdfs:seeAlso <http://vocab.getty.edu/aat/300038770> ;
  rdfs:subClassOf <https://w3id.org/con-tax/components/aat-furn#300038758> ;
.
<https://w3id.org/con-tax/components/aat-furn#300038771>
  rdf:type owl:Class ;
  rdfs:comment "Grand, lavishly upholstered beds intended for princes and noblemen."@en ;
  rdfs:comment "Grote, weelderig beklede bedden die voor vorsten en edellieden zijn bestemd."@nl ;
  rdfs:isDefinedBy <https://w3id.org/con-tax/components/aat-furn> ;
  rdfs:label "staatsbed"@nl ;
  rdfs:label "staatsbedden"@nl ;
  rdfs:label "state beds"@en ;
  rdfs:seeAlso <http://vocab.getty.edu/aat/300038771> ;
  rdfs:subClassOf <https://w3id.org/con-tax/components/aat-furn#300038697> ;
.
<https://w3id.org/con-tax/components/aat-furn#300038775>
  rdf:type owl:Class ;
  rdfs:comment "Bedden die een met vloeistof gevuld matras van rubber of plastic hebben in een onbuigzaam, vaak verwarmd, waterbestendig frame. Het oppervlak vormt zich naar elke positie van het lichaam van de slapende persoon."@nl ;
  rdfs:comment "Beds having a liquid-filled rubber or plastic mattress in a rigid, often heated, waterproof frame and providing a surface that conforms to the sleeper's body in any position."@en ;
  rdfs:isDefinedBy <https://w3id.org/con-tax/components/aat-furn> ;
  rdfs:label "water beds"@en ;
  rdfs:label "waterbed"@nl ;
  rdfs:label "waterbedden"@nl ;
  rdfs:seeAlso <http://vocab.getty.edu/aat/300038775> ;
  rdfs:subClassOf <https://w3id.org/con-tax/components/aat-furn#300038697> ;
.
<https://w3id.org/con-tax/components/aat-furn#300038776>
  rdf:type gvp:GuideTerm ;
  rdf:type skos:OrderedCollection ;
  rdfs:isDefinedBy <https://w3id.org/con-tax/components/aat-furn> ;
  rdfs:label "<bedden naar afmeting>"@nl ;
  rdfs:label "<beds by size>"@en ;
  rdfs:label "bedden naar afmeting"@nl ;
  rdfs:seeAlso <http://vocab.getty.edu/aat/300038776> ;
  contax:containsConcept <https://w3id.org/con-tax/components/aat-furn#300038777> ;
  contax:containsConcept <https://w3id.org/con-tax/components/aat-furn#300038781> ;
  contax:containsConcept <https://w3id.org/con-tax/components/aat-furn#300038782> ;
  contax:containsConcept <https://w3id.org/con-tax/components/aat-furn#300038786> ;
.
<https://w3id.org/con-tax/components/aat-furn#300038777>
  rdf:type owl:Class ;
  rdfs:comment "Bedden die 135 cm breed zijn en voor twee volwassenen zijn bestemd."@nl ;
  rdfs:comment "Beds which are 54 inches wide; large enough to accommodate two adults."@en ;
  rdfs:isDefinedBy <https://w3id.org/con-tax/components/aat-furn> ;
  rdfs:label "double beds"@en ;
  rdfs:label "tweepersoonsbed"@nl ;
  rdfs:label "tweepersoonsbedden"@nl ;
  rdfs:seeAlso <http://vocab.getty.edu/aat/300038777> ;
  rdfs:subClassOf <https://w3id.org/con-tax/components/aat-furn#300038697> ;
.
<https://w3id.org/con-tax/components/aat-furn#300038781>
  rdf:type owl:Class ;
  rdfs:comment "Benaming die meestal betrekking heeft op bedden die tussen de 190 en 195 cm breed en tussen de 200 en 210 cm lang zijn."@nl ;
  rdfs:comment "Term generally applied to beds measuring between 76 and 78 inches wide and between 80 and 84 inches long."@en ;
  rdfs:isDefinedBy <https://w3id.org/con-tax/components/aat-furn> ;
  rdfs:label "king-size bed"@nl ;
  rdfs:label "king-size bedden"@nl ;
  rdfs:label "king-size beds"@en ;
  rdfs:seeAlso <http://vocab.getty.edu/aat/300038781> ;
  rdfs:subClassOf <https://w3id.org/con-tax/components/aat-furn#300038697> ;
.
<https://w3id.org/con-tax/components/aat-furn#300038782>
  rdf:type owl:Class ;
  rdfs:comment "Term generally applied to beds larger than double beds but smaller than king-size beds."@en ;
  rdfs:comment "Term over het algemeen van toepassing op bedden die groter zijn dan tweepersoonbedden, maar kleiner dan de king-size bedden."@nl ;
  rdfs:isDefinedBy <https://w3id.org/con-tax/components/aat-furn> ;
  rdfs:label "queen-size beds"@en ;
  rdfs:label "queensize bed"@nl ;
  rdfs:label "queensize bedden"@nl ;
  rdfs:seeAlso <http://vocab.getty.edu/aat/300038782> ;
  rdfs:subClassOf <https://w3id.org/con-tax/components/aat-furn#300038697> ;
.
<https://w3id.org/con-tax/components/aat-furn#300038785>
  rdf:type owl:Class ;
  rdfs:comment "Bedden die bestaan uit een metalen frame, springveren, matrassen en een plank aan het hoofdeinde,  maar niet aan het voeteneinde. Dit type werd omstreeks 1945 in Amerika gemaakt."@nl ;
  rdfs:comment "Beds consisting of metal frames, box springs, mattresses, and headboards, but lacking footboards; of a type made in America about 1945."@en ;
  rdfs:isDefinedBy <https://w3id.org/con-tax/components/aat-furn> ;
  rdfs:label "hollywood beds"@en ;
  rdfs:label "hollywoodbed"@nl ;
  rdfs:label "hollywoodbedden"@nl ;
  rdfs:seeAlso <http://vocab.getty.edu/aat/300038785> ;
  rdfs:subClassOf <https://w3id.org/con-tax/components/aat-furn#300038697> ;
.
<https://w3id.org/con-tax/components/aat-furn#300038786>
  rdf:type owl:Class ;
  rdfs:comment "Beds for one person, especially a matching pair in a bedroom."@en ;
  rdfs:comment "Eénpersoonsbedden, vooral een bij elkaar passend paar in een slaapkamer."@nl ;
  rdfs:isDefinedBy <https://w3id.org/con-tax/components/aat-furn> ;
  rdfs:label "lits jumeaux"@nl ;
  rdfs:label "twin beds"@en ;
  rdfs:seeAlso <http://vocab.getty.edu/aat/300038786> ;
  rdfs:seeAlso wd:Q10950518 ;
  rdfs:subClassOf <https://w3id.org/con-tax/components/aat-furn#300038697> ;
.
<https://w3id.org/con-tax/components/aat-furn#300038788>
  rdf:type owl:Class ;
  rdfs:comment "Benaming die door Thomas Sheraton werd gebruikt voor een elegant ontwerp van twee lits jumeaux met een gemeenschappelijk baldakijn,  waarbij een doorgang tussen de bedden zorgt dat de bedienden gemakkelijk toegang hebben."@nl ;
  rdfs:comment "Term used by Thomas Sheraton for a fanciful design which incorporates two twin beds sharing a common tester and having a passageway between the beds to allow easy access for servants."@en ;
  rdfs:isDefinedBy <https://w3id.org/con-tax/components/aat-furn> ;
  rdfs:label "summer beds"@en ;
  rdfs:label "zomerbed"@nl ;
  rdfs:label "zomerbedden"@nl ;
  rdfs:seeAlso <http://vocab.getty.edu/aat/300038788> ;
  rdfs:subClassOf <https://w3id.org/con-tax/components/aat-furn#300038737> ;
.
<https://w3id.org/con-tax/components/aat-furn#300038791>
  rdf:type owl:Class ;
  rdfs:comment "Beds, generally of the 19th-century, which when folded closed, looked to be an exact representation of another piece of furniture, such as a bureau, a dresser, or a cabinet. "@en ;
  rdfs:isDefinedBy <https://w3id.org/con-tax/components/aat-furn> ;
  rdfs:label "folding beds"@en ;
  rdfs:label "opklapbed"@nl ;
  rdfs:label "opklapbedden"@nl ;
  rdfs:seeAlso <http://vocab.getty.edu/aat/300038791> ;
  rdfs:subClassOf <https://w3id.org/con-tax/components/aat-furn#300038697> ;
.
<https://w3id.org/con-tax/components/aat-furn#300038799>
  rdf:type owl:Class ;
  rdfs:comment "Lichte bedden die vaak opklapbaar zijn en vooral bij kamperen of voor kinderen worden gebruikt. Ze zijn meestal gemaakt van canvas dat over een frame wordt gespannen."@nl ;
  rdfs:comment "Light beds, often collapsible and typically used for camping or by a child; generally made of canvas stretched on a frame."@en ;
  rdfs:isDefinedBy <https://w3id.org/con-tax/components/aat-furn> ;
  rdfs:label "cots (beds)"@en ;
  rdfs:label "stretcher"@nl ;
  rdfs:label "stretchers"@nl ;
  rdfs:seeAlso <http://vocab.getty.edu/aat/300038799> ;
  rdfs:subClassOf <https://w3id.org/con-tax/components/aat-furn#300038697> ;
  rdfs:subClassOf <https://w3id.org/con-tax/components/aat-furn#300040045> ;
.
<https://w3id.org/con-tax/components/aat-furn#300038801>
  rdf:type owl:Class ;
  rdfs:comment "Beds converted from sofas, settees, and other forms of seating furniture usually by folding out a concealed mattress and springs."@en ;
  rdfs:comment "Wordt gebruikt voor bedden die worden gevormd van sofa's, canapés en andere soorten zitmeubilair, meestal door een verborgen matras en bedbodem uit te klappen."@nl ;
  rdfs:isDefinedBy <https://w3id.org/con-tax/components/aat-furn> ;
  rdfs:label "hideaway beds"@en ;
  rdfs:label "opklapbaar bed"@nl ;
  rdfs:label "opklapbare bedden"@nl ;
  rdfs:seeAlso <http://vocab.getty.edu/aat/300038801> ;
  rdfs:subClassOf <https://w3id.org/con-tax/components/aat-furn#300038697> ;
.
<https://w3id.org/con-tax/components/aat-furn#300038803>
  rdf:type owl:Class ;
  rdfs:comment "Any of various kinds of concealed or disguised beds first designed in the 18th century. Such beds were among the many ingenious forms of late 19th-century patent furniture."@en ;
  rdfs:comment "Verschillende soorten bedden die onherkenbaar worden gemaakt of die verborgen zijn. Ze werden in de 18e eeuw voor het eerst ontworpen. Zulke bedden bevonden zich onder de vele vindingrijke vormen van gepatenteerd meubilair uit het eind van de 19e eeuw."@nl ;
  rdfs:isDefinedBy <https://w3id.org/con-tax/components/aat-furn> ;
  rdfs:label "deception beds"@en ;
  rdfs:label "verborgen bed"@nl ;
  rdfs:label "verborgen bedden"@nl ;
  rdfs:seeAlso <http://vocab.getty.edu/aat/300038803> ;
  rdfs:subClassOf <https://w3id.org/con-tax/components/aat-furn#300038791> ;
.
<https://w3id.org/con-tax/components/aat-furn#300038804>
  rdf:type owl:Class ;
  rdfs:comment "Deception beds concealed in a carcase that outwardly resembles a bureau."@en ;
  rdfs:comment "Verborgen bedden die in een frame zijn verborgen dat van buitenaf op een bureau lijkt."@nl ;
  rdfs:isDefinedBy <https://w3id.org/con-tax/components/aat-furn> ;
  rdfs:label "bureau beds"@en ;
  rdfs:label "bureaubed"@nl ;
  rdfs:label "bureaubedden"@nl ;
  rdfs:seeAlso <http://vocab.getty.edu/aat/300038804> ;
  rdfs:subClassOf <https://w3id.org/con-tax/components/aat-furn#300038803> ;
.
<https://w3id.org/con-tax/components/aat-furn#300038806>
  rdf:type owl:Class ;
  rdfs:comment "Deception beds which look like an upright piano but unfold to form a bed."@en ;
  rdfs:comment "Verborgen bedden die op een piano lijken maar tot bed kunnen worden uitgeklapt."@nl ;
  rdfs:isDefinedBy <https://w3id.org/con-tax/components/aat-furn> ;
  rdfs:label "piano beds"@en ;
  rdfs:label "pianobed"@nl ;
  rdfs:label "pianobedden"@nl ;
  rdfs:seeAlso <http://vocab.getty.edu/aat/300038806> ;
  rdfs:subClassOf <https://w3id.org/con-tax/components/aat-furn#300038803> ;
  rdfs:subClassOf <https://w3id.org/con-tax/components/aat-furn#300040038> ;
.
<https://w3id.org/con-tax/components/aat-furn#300038807>
  rdf:type owl:Class ;
  rdfs:comment "Folding beds built into a cabinet which outwardly resembles a press or chest."@en ;
  rdfs:comment "Opklapbedden die in een kabinet zijn ingebouwd dat van buitenaf op een muurkast of gewone kast lijkt."@nl ;
  rdfs:isDefinedBy <https://w3id.org/con-tax/components/aat-furn> ;
  rdfs:label "kastbed (verborgen bed)"@nl ;
  rdfs:label "kastbed"@nl ;
  rdfs:label "kastbedden (verborgen bedden)"@nl ;
  rdfs:label "kastbedden"@nl ;
  rdfs:label "press beds (deception beds)"@en ;
  rdfs:seeAlso <http://vocab.getty.edu/aat/300038807> ;
  rdfs:subClassOf <https://w3id.org/con-tax/components/aat-furn#300038803> ;
  rdfs:subClassOf <https://w3id.org/con-tax/components/aat-furn#300039252> ;
.
<https://w3id.org/con-tax/components/aat-furn#300038817>
  rdf:type owl:Class ;
  rdfs:comment "Lage ledikanten die speciaal zijn ontworpen om onder een ander bed te kunnen worden geschoven als ze niet in gebruik zijn."@nl ;
  rdfs:comment "Low bedsteads specifically designed so that they can be moved under another bed when not in use."@en ;
  rdfs:isDefinedBy <https://w3id.org/con-tax/components/aat-furn> ;
  rdfs:label "onderschuifbed"@nl ;
  rdfs:label "onderschuifbedden"@nl ;
  rdfs:label "trundle beds"@en ;
  rdfs:seeAlso <http://vocab.getty.edu/aat/300038817> ;
  rdfs:subClassOf <https://w3id.org/con-tax/components/aat-furn#300038697> ;
.
<https://w3id.org/con-tax/components/aat-furn#300038822>
  rdf:type owl:Class ;
  rdfs:comment "Bedden die in een kast kunnen worden opgeklapt of gedraaid. Ze zijn genoemd naar de Amerikaanse uitvinder, William L. Murphy."@nl ;
  rdfs:comment "Beds constructed so that they can be folded or swung into a closet; named after William L. Murphy, American inventor."@en ;
  rdfs:isDefinedBy <https://w3id.org/con-tax/components/aat-furn> ;
  rdfs:label "Murphy beds"@en ;
  rdfs:label "Murphybed"@nl ;
  rdfs:label "Murphybedden"@nl ;
  rdfs:seeAlso <http://vocab.getty.edu/aat/300038822> ;
  rdfs:subClassOf <https://w3id.org/con-tax/components/aat-furn#300038791> ;
.
<https://w3id.org/con-tax/components/aat-furn#300038829>
  rdf:type owl:Class ;
  rdfs:comment "Wooden beds with spool-shaped turnings in the spindles and usually in the rails and posts of the headboard and footboard."@en ;
  rdfs:isDefinedBy <https://w3id.org/con-tax/components/aat-furn> ;
  rdfs:label "spijlenbed"@nl ;
  rdfs:label "spijlenbedden"@nl ;
  rdfs:label "spool beds"@en ;
  rdfs:seeAlso <http://vocab.getty.edu/aat/300038829> ;
  rdfs:subClassOf <https://w3id.org/con-tax/components/aat-furn#300038697> ;
.
<https://w3id.org/con-tax/components/aat-furn#300038847>
  rdf:type owl:Class ;
  rdfs:comment "Kleine bedjes voor kinderen die meestal op schommelbalken staan."@nl ;
  rdfs:comment "Small beds for infants, usually on bends."@en ;
  rdfs:isDefinedBy <https://w3id.org/con-tax/components/aat-furn> ;
  rdfs:label "cradles (children's beds)"@en ;
  rdfs:label "wieg"@nl ;
  rdfs:label "wiegen"@nl ;
  rdfs:seeAlso <http://vocab.getty.edu/aat/300038847> ;
  rdfs:subClassOf <https://w3id.org/con-tax/components/aat-furn#300165757> ;
.
<https://w3id.org/con-tax/components/aat-furn#300038850>
  rdf:type owl:Class ;
  rdfs:comment "Infants' beds, especially those with a hood over one end."@en ;
  rdfs:comment "Wordt gebruikt voor kinderbedjes, met name de bedjes die een kap over één kant hebben."@nl ;
  rdfs:isDefinedBy <https://w3id.org/con-tax/components/aat-furn> ;
  rdfs:label "bassinets (children's beds)"@en ;
  rdfs:label "mandewieg"@nl ;
  rdfs:label "mandewiegen"@nl ;
  rdfs:seeAlso <http://vocab.getty.edu/aat/300038850> ;
  rdfs:seeAlso wd:Q412770 ;
  rdfs:subClassOf <https://w3id.org/con-tax/components/aat-furn#300165757> ;
.
<https://w3id.org/con-tax/components/aat-furn#300038852>
  rdf:type owl:Class ;
  rdfs:comment "Kleine bedjes met een hoge rand en meestal met spijlen aan de zijkant voor kinderen."@nl ;
  rdfs:comment "Small bedsteads with a high enclosure and usually slatted sides for a child."@en ;
  rdfs:isDefinedBy <https://w3id.org/con-tax/components/aat-furn> ;
  rdfs:label "cribs (children's beds)"@en ;
  rdfs:label "ledikant"@nl ;
  rdfs:label "ledikanten"@nl ;
  rdfs:seeAlso <http://vocab.getty.edu/aat/300038852> ;
  rdfs:subClassOf <https://w3id.org/con-tax/components/aat-furn#300165757> ;
.
<https://w3id.org/con-tax/components/aat-furn#300038859>
  rdf:type owl:Class ;
  rdfs:comment "Cribs, typically consisting of a cot or bassinet suspended from a upright member, designed to allow to swing back and forth as to rock a baby to sleep. "@en ;
  rdfs:isDefinedBy <https://w3id.org/con-tax/components/aat-furn> ;
  rdfs:label "schommelbedje"@nl ;
  rdfs:label "schommelbedjes"@nl ;
  rdfs:label "swinging cribs"@en ;
  rdfs:seeAlso <http://vocab.getty.edu/aat/300038859> ;
  rdfs:subClassOf <https://w3id.org/con-tax/components/aat-furn#300038852> ;
.
<https://w3id.org/con-tax/components/aat-furn#300038860>
  rdf:type owl:Class ;
  rdfs:comment "Furniture that encloses a space and is generally boxlike in structure; intended for storage or display."@en ;
  rdfs:comment "Meubilair dat een ruimte omsluit en meestal ongeveer de constructie van een kist of doos heeft en dient voor opslag of vertoning van voorwerpen."@nl ;
  rdfs:isDefinedBy <https://w3id.org/con-tax/components/aat-furn> ;
  rdfs:label "bergmeubel"@nl ;
  rdfs:label "bergmeubels"@nl ;
  rdfs:label "case furniture"@en ;
  rdfs:label "kast"@nl ;
  rdfs:label "kasten"@nl ;
  rdfs:label "kastmeubilair"@nl ;
  rdfs:seeAlso <http://vocab.getty.edu/aat/300038860> ;
  rdfs:subClassOf <https://w3id.org/con-tax/components/aat-furn#300037680> ;
.
<https://w3id.org/con-tax/components/aat-furn#300038866>
  rdf:type owl:Class ;
  rdfs:comment "Case furniture of the 18th century, often in the \"Chinese style,\" which incorporate bookshelves behind glassed-in or trelliswork doors over chests of drawers.The design is epitomized in plate XXI of Ince and Mayhew's \"Universal System of Household Furniture\" (1762)."@en ;
  rdfs:isDefinedBy <https://w3id.org/con-tax/components/aat-furn> ;
  rdfs:label "gentleman's vergaarplaats"@nl ;
  rdfs:label "gentleman's vergaarplaatsen"@nl ;
  rdfs:label "gentlemen's repositories"@en ;
  rdfs:seeAlso <http://vocab.getty.edu/aat/300038866> ;
  rdfs:subClassOf <https://w3id.org/con-tax/components/aat-furn#300143716> ;
.
<https://w3id.org/con-tax/components/aat-furn#300038867>
  rdf:type owl:Class ;
  rdfs:comment "Book furniture comprising bookcase units surmounting a cupboard support. These are of various design, but often with a center double-doored unit with two wings with single doors. The doors are often glassed or have a screen to allow viewing the contents within."@en ;
  rdfs:isDefinedBy <https://w3id.org/con-tax/components/aat-furn> ;
  rdfs:label "bibliotheekboekenkast"@nl ;
  rdfs:label "bibliotheekboekenkasten"@nl ;
  rdfs:label "library bookcases"@en ;
  rdfs:seeAlso <http://vocab.getty.edu/aat/300038867> ;
  rdfs:subClassOf <https://w3id.org/con-tax/components/aat-furn#300143716> ;
.
<https://w3id.org/con-tax/components/aat-furn#300038870>
  rdf:type owl:Class ;
  rdfs:comment "Writing desks surmounted by a bookcase, particularly where the desk and bookcase are separate units."@en ;
  rdfs:isDefinedBy <https://w3id.org/con-tax/components/aat-furn> ;
  rdfs:label "secretaire-boekenkast"@nl ;
  rdfs:label "secretaire-boekenkasten"@nl ;
  rdfs:label "secretary-bookcases (bookcases)"@en ;
  rdfs:seeAlso <http://vocab.getty.edu/aat/300038870> ;
  rdfs:subClassOf <https://w3id.org/con-tax/components/aat-furn#300143716> ;
.
<https://w3id.org/con-tax/components/aat-furn#300038888>
  rdf:type owl:Class ;
  rdfs:comment "Bergmeubilair dat uit een aantal planken, kleine laadjes of vakjes bestaat waar één of meer deuren voor zitten. Ze zijn bestemd als opslagruimte en soms voor het vertonen van kleine voorwerpen. Er bestaan ook soortgelijke, vaste of ingebouwde kasten die vaak voor bepaalde doeleinden worden ontworpen zoals in een keuken of badkamer."@nl ;
  rdfs:comment "Case furniture consisting of a set of shelves, small drawers, or pigeonholes, fronted by one or more doors, and intended for the storage and sometimes the display of small objects. Also, similar built-in or fitted cases often designed for specific purposes, as in a kitchen or bathroom."@en ;
  rdfs:isDefinedBy <https://w3id.org/con-tax/components/aat-furn> ;
  rdfs:label "cabinets (case furniture)"@en ;
  rdfs:label "kabinet (kastmeubilair)"@nl ;
  rdfs:label "kabinet"@nl ;
  rdfs:label "kabinetten (kastmeubilair)"@nl ;
  rdfs:label "kabinetten"@nl ;
  rdfs:seeAlso <http://vocab.getty.edu/aat/300038888> ;
  rdfs:subClassOf <https://w3id.org/con-tax/components/aat-furn#300038860> ;
  rdfs:subClassOf <https://w3id.org/con-tax/components/aat-furn#300040157> ;
  contax:containsGuideTerm <https://w3id.org/con-tax/components/aat-furn#300038890> ;
  contax:containsGuideTerm <https://w3id.org/con-tax/components/aat-furn#300038907> ;
.
<https://w3id.org/con-tax/components/aat-furn#300038890>
  rdf:type gvp:GuideTerm ;
  rdfs:isDefinedBy <https://w3id.org/con-tax/components/aat-furn> ;
  rdfs:label "<cabinets by form>"@en ;
  rdfs:label "<kabinetten naar vorm>"@nl ;
  rdfs:label "kabinetten naar vorm"@nl ;
  rdfs:seeAlso <http://vocab.getty.edu/aat/300038890> ;
  contax:containsConcept <https://w3id.org/con-tax/components/aat-furn#300038892> ;
  contax:containsConcept <https://w3id.org/con-tax/components/aat-furn#300038896> ;
  contax:containsConcept <https://w3id.org/con-tax/components/aat-furn#300038949> ;
  contax:containsConcept <https://w3id.org/con-tax/components/aat-furn#300038976> ;
  contax:containsConcept <https://w3id.org/con-tax/components/aat-furn#300172167> ;
  contax:containsConcept <https://w3id.org/con-tax/components/aat-furn#300176753> ;
.
<https://w3id.org/con-tax/components/aat-furn#300038892>
  rdf:type owl:Class ;
  rdfs:comment "Case furniture consisting of a set of small drawers intended for the storage or display of objects."@en ;
  rdfs:isDefinedBy <https://w3id.org/con-tax/components/aat-furn> ;
  rdfs:label "cabinets of drawers"@en ;
  rdfs:label "ladenkabinet"@nl ;
  rdfs:label "ladenkabinetten"@nl ;
  rdfs:seeAlso <http://vocab.getty.edu/aat/300038892> ;
  rdfs:subClassOf <https://w3id.org/con-tax/components/aat-furn#300038888> ;
.
<https://w3id.org/con-tax/components/aat-furn#300038896>
  rdf:type owl:Class ;
  rdfs:comment "Bureau-cabinets typical of fine furniture originating in the 17th century that feature cabinets of drawers or pigeon holes, fronted by one or more doors, and supported on a stand from which it may be detached."@en ;
  rdfs:isDefinedBy <https://w3id.org/con-tax/components/aat-furn> ;
  rdfs:label "cabinets on stands"@en ;
  rdfs:label "kabinet op voet"@nl ;
  rdfs:label "kabinetten op voet"@nl ;
  rdfs:seeAlso <http://vocab.getty.edu/aat/300038896> ;
  rdfs:subClassOf <https://w3id.org/con-tax/components/aat-furn#300038888> ;
.
<https://w3id.org/con-tax/components/aat-furn#300038898>
  rdf:type owl:Class ;
  rdfs:comment "Spaanse uitklapbare schrijfkabinetten in de vorm van een rechthoekige kist die op een decoratieve pie de puente of schraag steunt. De binnenkant is vaak uitbundig versierd en bevat meestal een rij laden, soms aangevuld met vakjes en een klein kastje. De naam dateert uit het einde van de 19de eeuw en verwijst foutief naar de plaats waar dit type kast zou zijn gemaakt, namelijk het dorp Vargas in de provincie Toledo."@nl ;
  rdfs:comment "Spanish fall-front writing cabinets, taking the form of a rectangular chest supported on a decorative pie de puente or trestle stand. The interior is often elaborately decorated and generally contains tiers of drawers which may be supplemented with pigeonholes and a small cupboard. The name is a late 19th-century name that erroneously suggests that this type of writing cabinet was made in the Toledan village of Vargas."@en ;
  rdfs:isDefinedBy <https://w3id.org/con-tax/components/aat-furn> ;
  rdfs:label "vargueño's"@nl ;
  rdfs:label "vargueños"@en ;
  rdfs:seeAlso <http://vocab.getty.edu/aat/300038898> ;
  rdfs:subClassOf <https://w3id.org/con-tax/components/aat-furn#300039521> ;
.
<https://w3id.org/con-tax/components/aat-furn#300038907>
  rdf:type gvp:GuideTerm ;
  rdfs:isDefinedBy <https://w3id.org/con-tax/components/aat-furn> ;
  rdfs:label "<cabinets by function>"@en ;
  rdfs:label "<kabinetten naar functie>"@nl ;
  rdfs:label "kabinetten naar functie"@nl ;
  rdfs:seeAlso <http://vocab.getty.edu/aat/300038907> ;
  contax:containsConcept <https://w3id.org/con-tax/components/aat-furn#300038908> ;
  contax:containsConcept <https://w3id.org/con-tax/components/aat-furn#300038916> ;
  contax:containsConcept <https://w3id.org/con-tax/components/aat-furn#300038919> ;
  contax:containsConcept <https://w3id.org/con-tax/components/aat-furn#300038924> ;
  contax:containsConcept <https://w3id.org/con-tax/components/aat-furn#300038936> ;
  contax:containsConcept <https://w3id.org/con-tax/components/aat-furn#300038937> ;
  contax:containsConcept <https://w3id.org/con-tax/components/aat-furn#300038939> ;
  contax:containsConcept <https://w3id.org/con-tax/components/aat-furn#300038940> ;
  contax:containsConcept <https://w3id.org/con-tax/components/aat-furn#300038950> ;
  contax:containsConcept <https://w3id.org/con-tax/components/aat-furn#300038960> ;
  contax:containsConcept <https://w3id.org/con-tax/components/aat-furn#300079633> ;
  contax:containsConcept <https://w3id.org/con-tax/components/aat-furn#300162353> ;
  contax:containsConcept <https://w3id.org/con-tax/components/aat-furn#300164516> ;
  contax:containsConcept <https://w3id.org/con-tax/components/aat-furn#300164614> ;
  contax:containsConcept <https://w3id.org/con-tax/components/aat-furn#300170867> ;
  contax:containsConcept <https://w3id.org/con-tax/components/aat-furn#300170870> ;
  contax:containsConcept <https://w3id.org/con-tax/components/aat-furn#300174275> ;
  contax:containsConcept <https://w3id.org/con-tax/components/aat-furn#300250532> ;
  contax:containsConcept <https://w3id.org/con-tax/components/aat-furn#300263125> ;
  contax:containsConcept <https://w3id.org/con-tax/components/aat-furn#300375159> ;
  contax:containsConcept <https://w3id.org/con-tax/components/aat-furn#300375160> ;
  contax:containsConcept <https://w3id.org/con-tax/components/aat-furn#300391454> ;
.
<https://w3id.org/con-tax/components/aat-furn#300038908>
  rdf:type owl:Class ;
  rdfs:comment "Hoge, smalle en diepe kabinetten om de uitvoerig versierde hoeden uit de 18e eeuw in Normandië en Bretagne in te zetten."@nl ;
  rdfs:comment "Tall, narrow, and deep cabinets intended to accommodate the elaborate bonnets peculiar to Normandy and Brittany in the 18th century."@en ;
  rdfs:isDefinedBy <https://w3id.org/con-tax/components/aat-furn> ;
  rdfs:label "bonnetière"@nl ;
  rdfs:label "bonnetières"@en ;
  rdfs:label "bonnetières"@nl ;
  rdfs:seeAlso <http://vocab.getty.edu/aat/300038908> ;
  rdfs:seeAlso wd:Q21550410 ;
  rdfs:subClassOf <https://w3id.org/con-tax/components/aat-furn#300038888> ;
.
<https://w3id.org/con-tax/components/aat-furn#300038916>
  rdf:type owl:Class ;
  rdfs:comment "Meubelstukken met vakken of laden waarin zich kastjes bevinden die als afzonderlijk stuk meubilair kunnen dienen of bovenop het bureaublad worden gezet."@nl ;
  rdfs:comment "Pieces of furniture fitted with pigeonholes or compartments to hold boxes made either as independent pieces of furniture or as pieces to be placed on top of a bureau plat."@en ;
  rdfs:isDefinedBy <https://w3id.org/con-tax/components/aat-furn> ;
  rdfs:label "cartonnier"@nl ;
  rdfs:label "cartonniers"@en ;
  rdfs:label "cartonniers"@nl ;
  rdfs:seeAlso <http://vocab.getty.edu/aat/300038916> ;
  rdfs:subClassOf <https://w3id.org/con-tax/components/aat-furn#300038888> ;
.
<https://w3id.org/con-tax/components/aat-furn#300038919>
  rdf:type owl:Class ;
  rdfs:comment "Cabinets, often with glass fronts and sides, used to hold and display china."@en ;
  rdfs:comment "Wordt gebruikt voor kabinetten met een glazen voorkant om porselein in op te bergen en te vertonen."@nl ;
  rdfs:isDefinedBy <https://w3id.org/con-tax/components/aat-furn> ;
  rdfs:label "china cabinets"@en ;
  rdfs:label "porseleinkast"@nl ;
  rdfs:label "porseleinkasten"@nl ;
  rdfs:seeAlso <http://vocab.getty.edu/aat/300038919> ;
  rdfs:subClassOf <https://w3id.org/con-tax/components/aat-furn#300038888> ;
.
<https://w3id.org/con-tax/components/aat-furn#300038924>
  rdf:type owl:Class ;
  rdfs:comment "18th-century French cabinets with small drawers designed to house a collection of shells; fashionable between 1730 and 1750."@en ;
  rdfs:comment "Franse kabinetten uit de 18e eeuw met kleine laadjes waarin een schelpencollectie wordt opgeborgen. Ze waren in de mode tussen 1730 en 1750."@nl ;
  rdfs:isDefinedBy <https://w3id.org/con-tax/components/aat-furn> ;
  rdfs:label "coquillier"@nl ;
  rdfs:label "coquilliers"@en ;
  rdfs:label "coquilliers"@nl ;
  rdfs:seeAlso <http://vocab.getty.edu/aat/300038924> ;
  rdfs:subClassOf <https://w3id.org/con-tax/components/aat-furn#300038888> ;
.
<https://w3id.org/con-tax/components/aat-furn#300038936>
  rdf:type owl:Class ;
  rdfs:comment "Cabinets with drawers sized to hold documents; often, but not always, made of metal."@en ;
  rdfs:comment "Kabinetten met laden voor documenten. Ze zijn vaak, maar niet altijd, van metaal gemaakt."@nl ;
  rdfs:isDefinedBy <https://w3id.org/con-tax/components/aat-furn> ;
  rdfs:label "filing cabinets"@en ;
  rdfs:label "opbergkast"@nl ;
  rdfs:label "opbergkasten"@nl ;
  rdfs:seeAlso <http://vocab.getty.edu/aat/300038936> ;
  rdfs:seeAlso wd:Q17053456 ;
  rdfs:subClassOf <https://w3id.org/con-tax/components/aat-furn#300038888> ;
.
<https://w3id.org/con-tax/components/aat-furn#300038937>
  rdf:type owl:Class ;
  rdfs:comment "Cabinets specially designed to hold handguns, long guns and other types of small arms; often with glass-fronted doors."@en ;
  rdfs:comment "Kabinetten die speciaal zijn ontworpen voor pistolen, geweren en andere soorten handwapens. De deuren zijn vaak van glas."@nl ;
  rdfs:isDefinedBy <https://w3id.org/con-tax/components/aat-furn> ;
  rdfs:label "geweerkast"@nl ;
  rdfs:label "geweerkasten"@nl ;
  rdfs:label "gun cabinets"@en ;
  rdfs:seeAlso <http://vocab.getty.edu/aat/300038937> ;
  rdfs:subClassOf <https://w3id.org/con-tax/components/aat-furn#300038888> ;
.
<https://w3id.org/con-tax/components/aat-furn#300038939>
  rdf:type owl:Class ;
  rdfs:comment "Algemene benaming voor grote keukenkabinetten die tijdens het begin van de 20e eeuw in massa werden geproduceerd met een geëmailleerd werkblad, opslagruimte en een bloemzeef."@nl ;
  rdfs:comment "Popular term for tall kitchen cabinets mass-produced during the early 20th century; usually oak, with such features as an enameled work surface, storage bins, and a flour sifter."@en ;
  rdfs:isDefinedBy <https://w3id.org/con-tax/components/aat-furn> ;
  rdfs:label "Hoosier cabinets"@en ;
  rdfs:label "Hoosierkast"@nl ;
  rdfs:label "Hoosierkasten"@nl ;
  rdfs:seeAlso <http://vocab.getty.edu/aat/300038939> ;
  rdfs:seeAlso wd:Q3692562 ;
  rdfs:subClassOf <https://w3id.org/con-tax/components/aat-furn#300038888> ;
.
<https://w3id.org/con-tax/components/aat-furn#300038940>
  rdf:type owl:Class ;
  rdfs:comment "Franse 17e- en 18e-eeuwse kabinetten met voetstuk waarin juwelen worden opgeborgen. Ze zijn vaak met veel inlegwerk versierd."@nl ;
  rdfs:comment "French 17th- and 18th-century cabinets on stands used to store jewels; often heavily adorned with inlay."@en ;
  rdfs:isDefinedBy <https://w3id.org/con-tax/components/aat-furn> ;
  rdfs:label "jewel cabinets"@en ;
  rdfs:label "juweelkast"@nl ;
  rdfs:label "juweelkasten"@nl ;
  rdfs:seeAlso <http://vocab.getty.edu/aat/300038940> ;
  rdfs:subClassOf <https://w3id.org/con-tax/components/aat-furn#300038888> ;
  rdfs:subClassOf <https://w3id.org/con-tax/components/aat-furn#300038896> ;
.
<https://w3id.org/con-tax/components/aat-furn#300038949>
  rdf:type owl:Class ;
  rdfs:comment "Cabinets intended to stand against a pier."@en ;
  rdfs:comment "Kabinetten die zijn bestemd om tegen een penant te staan."@nl ;
  rdfs:isDefinedBy <https://w3id.org/con-tax/components/aat-furn> ;
  rdfs:label "meuble d'entre deux"@nl ;
  rdfs:label "meubles d'entre deux"@en ;
  rdfs:label "meubles d'entre deux"@nl ;
  rdfs:seeAlso <http://vocab.getty.edu/aat/300038949> ;
  rdfs:subClassOf <https://w3id.org/con-tax/components/aat-furn#300038888> ;
.
<https://w3id.org/con-tax/components/aat-furn#300038950>
  rdf:type owl:Class ;
  rdfs:comment "Cabinets of various form, but usually single or double-doored narrow vertically oriented cases intended to store sheet music."@en ;
  rdfs:isDefinedBy <https://w3id.org/con-tax/components/aat-furn> ;
  rdfs:label "music cabinets"@en ;
  rdfs:label "muziekkast"@nl ;
  rdfs:label "muziekkasten"@nl ;
  rdfs:seeAlso <http://vocab.getty.edu/aat/300038950> ;
  rdfs:subClassOf <https://w3id.org/con-tax/components/aat-furn#300038888> ;
.
<https://w3id.org/con-tax/components/aat-furn#300038952>
  rdf:type owl:Class ;
  rdfs:comment "Keukenkasten waarin voedsel wordt bewaard, met ventilatieopeningen aan de voorkant die meestal uit geperforeerd tin en soms metaalgaas of stof bestaat."@nl ;
  rdfs:comment "Kitchen cabinets in which food is stored, having a ventilated front, generally of pierced tin or sometimes of screening or cloth."@en ;
  rdfs:isDefinedBy <https://w3id.org/con-tax/components/aat-furn> ;
  rdfs:label "kitchen safe"@nl ;
  rdfs:label "kitchen safes"@en ;
  rdfs:label "kitchen safes"@nl ;
  rdfs:seeAlso <http://vocab.getty.edu/aat/300038952> ;
  rdfs:subClassOf <https://w3id.org/con-tax/components/aat-furn#300249925> ;
.
<https://w3id.org/con-tax/components/aat-furn#300038960>
  rdf:type owl:Class ;
  rdfs:comment "Cabinets intended to hold household or cleaning supplies made of any material, but especially used in reference to such cabinets made of enameled steel."@en ;
  rdfs:comment "Wordt gebruikt voor kasten waarin huishoudelijke of schoonmaakmiddelen worden opgeslagen, met name wanneer ze van geëmailleerd staal zijn gemaakt."@nl ;
  rdfs:isDefinedBy <https://w3id.org/con-tax/components/aat-furn> ;
  rdfs:label "installatiekast"@nl ;
  rdfs:label "installatiekasten"@nl ;
  rdfs:label "utility cabinets"@en ;
  rdfs:seeAlso <http://vocab.getty.edu/aat/300038960> ;
  rdfs:subClassOf <https://w3id.org/con-tax/components/aat-furn#300038888> ;
  rdfs:subClassOf <https://w3id.org/con-tax/components/aat-furn#300040163> ;
.
<https://w3id.org/con-tax/components/aat-furn#300038976>
  rdf:type owl:Class ;
  rdfs:comment "Cabinets designed to fit into a corner of a room, usually by being triangular."@en ;
  rdfs:comment "Kabinetten die zijn ontworpen zodat ze in een hoek van een kamer kunnen staan, meestal in de vorm van een driehoek."@nl ;
  rdfs:isDefinedBy <https://w3id.org/con-tax/components/aat-furn> ;
  rdfs:label "corner cabinets"@en ;
  rdfs:label "hoekkabinet"@nl ;
  rdfs:label "hoekkabinetten"@nl ;
  rdfs:seeAlso <http://vocab.getty.edu/aat/300038976> ;
  rdfs:subClassOf <https://w3id.org/con-tax/components/aat-furn#300038888> ;
.
<https://w3id.org/con-tax/components/aat-furn#300038978>
  rdf:type owl:Class ;
  rdfs:comment "Small chests or cabinets designed to store bottles of wine or liquor, often set on legs, and usually with locks and fitted with side handles. For metal-lined tubs or stands for cooling wine bottles, use \"wine coolers (containers).\" For sideboards with a place at one end to hold bottles of wine, use \"cellaret sideboards.\""@en ;
  rdfs:comment "Wordt gebruikt voor kleine kisten of kasten, meestal met slot en handvatten aan de zijkant, waar flessen wijn of sterke drank in worden bewaard. Gebruik 'wijnkoelers' voor met metaal gevoerde vaten of standaarden waarin wijnflessen worden gekoeld. Gebruik 'celleret sideboards' voor buffetten die aan één kant ruimte hebben voor wijnflessen."@nl ;
  rdfs:isDefinedBy <https://w3id.org/con-tax/components/aat-furn> ;
  rdfs:label "cellarets (liquor chests)"@en ;
  rdfs:label "celleret"@nl ;
  rdfs:label "cellerets"@nl ;
  rdfs:seeAlso <http://vocab.getty.edu/aat/300038978> ;
  rdfs:subClassOf <https://w3id.org/con-tax/components/aat-furn#300038992> ;
.
<https://w3id.org/con-tax/components/aat-furn#300038992>
  rdf:type owl:Class ;
  rdfs:comment "Grote kisten met scharnierende deksels die worden gebruikt om textiel, kleding en andere artikelen in op te bergen."@nl ;
  rdfs:comment "Large boxes with hinged lids intended for the storage of textiles, clothing, and other articles."@en ;
  rdfs:isDefinedBy <https://w3id.org/con-tax/components/aat-furn> ;
  rdfs:label "chests (case furniture)"@en ;
  rdfs:label "kist"@nl ;
  rdfs:label "kisten"@nl ;
  rdfs:seeAlso <http://vocab.getty.edu/aat/300038992> ;
  rdfs:seeAlso wd:Q366134 ;
  rdfs:subClassOf <https://w3id.org/con-tax/components/aat-furn#300038860> ;
.
<https://w3id.org/con-tax/components/aat-furn#300038995>
  rdf:type owl:Class ;
  rdfs:comment "Chests for the safe-keeping of valuables usually made of wood and sheathed in iron, of a type made in the ancient and Medieval periods."@en ;
  rdfs:comment "Kasten die worden gebruikt voor het veilig opbergen van kostbaarheden. Ze zijn meestal van hout met een ijzeren buitenkant. Dit soort werd in de oudheid en in de Middeleeuwen gemaakt."@nl ;
  rdfs:isDefinedBy <https://w3id.org/con-tax/components/aat-furn> ;
  rdfs:label "arca"@nl ;
  rdfs:label "arcae"@en ;
  rdfs:label "arcae"@nl ;
  rdfs:seeAlso <http://vocab.getty.edu/aat/300038995> ;
  rdfs:seeAlso wd:Q867621 ;
  rdfs:subClassOf <https://w3id.org/con-tax/components/aat-furn#300038992> ;
.
<https://w3id.org/con-tax/components/aat-furn#300038998>
  rdf:type owl:Class ;
  rdfs:comment "Chests with one or two tiers of drawers below a deep storage space; precursor to chests of drawers. Use \"chests of drawers\" for case furniture having two or more drawers but lacking a deep storage space."@en ;
  rdfs:comment "Kisten die één of twee rijen met laden hebben onder een diepe opbergruimte. Ze waren de voorlopers van de ladenkast. Gebruik 'ladenkasten' voor bergmeubilair dat  twee of meer laden heeft, zonder een diepe opbergruimte."@nl ;
  rdfs:isDefinedBy <https://w3id.org/con-tax/components/aat-furn> ;
  rdfs:label "chests with drawers"@en ;
  rdfs:label "ladenkist"@nl ;
  rdfs:label "ladenkisten"@nl ;
  rdfs:seeAlso <http://vocab.getty.edu/aat/300038998> ;
  rdfs:subClassOf <https://w3id.org/con-tax/components/aat-furn#300038992> ;
.
<https://w3id.org/con-tax/components/aat-furn#300039006>
  rdf:type owl:Class ;
  rdfs:comment "Kleine doosjes voor het bewaren van juwelen, waardevolle zaken of kleine voorwerpen; meestal van hout of metaal en vaak versierd."@nl ;
  rdfs:comment "Small chests or boxes for holding objects of value such as money, letters, and jewels; usually of wood or metal and highly ornamented and often hinged."@en ;
  rdfs:isDefinedBy <https://w3id.org/con-tax/components/aat-furn> ;
  rdfs:label "bijouteriekistje"@nl ;
  rdfs:label "bijouteriekistjes"@nl ;
  rdfs:label "caskets (personal gear)"@en ;
  rdfs:label "juwelenkistje"@nl ;
  rdfs:label "juwelenkistjes"@nl ;
  rdfs:seeAlso <http://vocab.getty.edu/aat/300039006> ;
  rdfs:subClassOf <https://w3id.org/con-tax/components/aat-furn#300038992> ;
.
<https://w3id.org/con-tax/components/aat-furn#300039007>
  rdf:type owl:Class ;
  rdfs:comment "Refers to chests, particularly to Italian chests produced from the 14th through the 16th centuries, primarily in Florence, Siena and the Veneto. They were often richly carved or decorated with pastiglia decoration and painted panels. They were typically commissioned in pairs when a house was renovated for a newly married couple, and were generally purchased by the groom."@en ;
  rdfs:comment "Verwijst naar kisten, met name Italiaanse kisten die vanaf de 14de tot en met de 16de eeuw werden vervaardigd, hoofdzakelijk in Florence, Siena en de Veneto. Vaak waren ze voorzien van rijk beeldsnijwerk of rijke decoraties met pastiglia en geschilderde panelen. Meestal liet men ze per paar vervaardigen wanneer een huis werd ingericht voor een jong echtpaar, en werden ze door de bruidegom gekocht."@nl ;
  rdfs:isDefinedBy <https://w3id.org/con-tax/components/aat-furn> ;
  rdfs:label "cassone"@nl ;
  rdfs:label "cassoni"@en ;
  rdfs:label "cassoni"@nl ;
  rdfs:seeAlso <http://vocab.getty.edu/aat/300039007> ;
  rdfs:seeAlso wd:Q945313 ;
  rdfs:subClassOf <https://w3id.org/con-tax/components/aat-furn#300038992> ;
  rdfs:subClassOf <https://w3id.org/con-tax/components/aat-furn#300039125> ;
.
<https://w3id.org/con-tax/components/aat-furn#300039009>
  rdf:type owl:Class ;
  rdfs:comment "Case furniture characterized by having drawers, typically three to five in number. A chest of drawers is generally supported on feet, but sometimes rests directly on the floor. Use \"commodes (chests of drawers)\" for similar case pieces generally supported on short legs. Use \"chests with drawers\" for chests with one or more tiers of drawers below a deep storage space."@en ;
  rdfs:comment "Verwijst naar een type kastmeubel met meestal drie à vijf laden. Een ladekast staat doorgaans op poten, maar kan ook rechtstreeks op de vloer staan. Gebruik 'commodes (ladekasten)' voor soortgelijke kasten die meestal op korte poten staan. Gebruik 'ladekisten' voor kisten met één of meer rijen laden onder een diepe opslagruimte."@nl ;
  rdfs:isDefinedBy <https://w3id.org/con-tax/components/aat-furn> ;
  rdfs:label "chests of drawers"@en ;
  rdfs:label "ladekasten"@nl ;
  rdfs:label "ladenkast"@nl ;
  rdfs:seeAlso <http://vocab.getty.edu/aat/300039009> ;
  rdfs:seeAlso wd:Q14169227 ;
  rdfs:subClassOf <https://w3id.org/con-tax/components/aat-furn#300038860> ;
.
<https://w3id.org/con-tax/components/aat-furn#300039021>
  rdf:type owl:Class ;
  rdfs:comment "Chests of drawers having a folding top which, when open, serves as a writing board; of a type made in 18th-century England."@en ;
  rdfs:comment "Ladenkasten met een opklapbaar deksel dat kan worden geopend om als schrijfblad te gebruiken. Dit type werd in de 18e eeuw in Engeland gemaakt."@nl ;
  rdfs:isDefinedBy <https://w3id.org/con-tax/components/aat-furn> ;
  rdfs:label "bachelors' chest"@nl ;
  rdfs:label "bachelors' chests"@en ;
  rdfs:label "bachelors' chests"@nl ;
  rdfs:seeAlso <http://vocab.getty.edu/aat/300039021> ;
  rdfs:subClassOf <https://w3id.org/con-tax/components/aat-furn#300039009> ;
.
<https://w3id.org/con-tax/components/aat-furn#300039027>
  rdf:type owl:Class ;
  rdfs:comment "Twee-delige ladekasten, de een gestapeld bovenop de andere."@nl ;
  rdfs:comment "Two-part chests of drawers, one stacked on top of the other."@en ;
  rdfs:isDefinedBy <https://w3id.org/con-tax/components/aat-furn> ;
  rdfs:label "chest on chest"@nl ;
  rdfs:label "chests-on-chests"@en ;
  rdfs:label "chests-on-chests"@nl ;
  rdfs:seeAlso <http://vocab.getty.edu/aat/300039027> ;
  rdfs:subClassOf <https://w3id.org/con-tax/components/aat-furn#300039009> ;
.
<https://w3id.org/con-tax/components/aat-furn#300039039>
  rdf:type owl:Class ;
  rdfs:comment "Chests of drawers which sit on a framed stand."@en ;
  rdfs:comment "Ladenkasten die op een dragend geraamte staan."@nl ;
  rdfs:isDefinedBy <https://w3id.org/con-tax/components/aat-furn> ;
  rdfs:label "chest on frame"@nl ;
  rdfs:label "chests on frames"@en ;
  rdfs:label "chests on frames"@nl ;
  rdfs:seeAlso <http://vocab.getty.edu/aat/300039039> ;
  rdfs:seeAlso wd:Q21706015 ;
  rdfs:subClassOf <https://w3id.org/con-tax/components/aat-furn#300039009> ;
.
<https://w3id.org/con-tax/components/aat-furn#300039042>
  rdf:type owl:Class ;
  rdfs:comment "18th-century French term for a piece of furniture for the storage of stuffs (chiffons) and small articles of clothing. It is usually, but not necessarily, a small, low chest of drawers, narrower than the normal commode. For small cupboards with a top forming a sideboard, use \"chiffoniers (sideboards).\""@en ;
  rdfs:comment "Franse benaming uit de 18e eeuw voor een meubelstuk waarin rommeltjes en kleine kledingstukken worden opgeborgen. Het is meestal, maar niet altijd, een kleine, lage ladenkast, smaller dan de normale commode. Gebruik 'chiffonnières (zijtafels)' voor kleine kasten waarvan de bovenkant een dressoir vormt."@nl ;
  rdfs:isDefinedBy <https://w3id.org/con-tax/components/aat-furn> ;
  rdfs:label "chiffonnière (ladenkast)"@nl ;
  rdfs:label "chiffonnière"@nl ;
  rdfs:label "chiffonnières (ladenkasten)"@nl ;
  rdfs:label "chiffonnières (low chests of drawers)"@en ;
  rdfs:label "chiffonnières"@nl ;
  rdfs:seeAlso <http://vocab.getty.edu/aat/300039042> ;
  rdfs:subClassOf <https://w3id.org/con-tax/components/aat-furn#300039009> ;
.
<https://w3id.org/con-tax/components/aat-furn#300039044>
  rdf:type owl:Class ;
  rdfs:comment "Commodes die naast een rij laden een openkast-systeem of een wandkast hebben."@nl ;
  rdfs:comment "Commodes incorporating a tier of drawers flanked by open shelves or cupboards."@en ;
  rdfs:isDefinedBy <https://w3id.org/con-tax/components/aat-furn> ;
  rdfs:label "commode à encoignures"@nl ;
  rdfs:label "commodes à encoignures"@en ;
  rdfs:label "commodes à encoignures"@nl ;
  rdfs:seeAlso <http://vocab.getty.edu/aat/300039044> ;
  rdfs:subClassOf <https://w3id.org/con-tax/components/aat-furn#300077277> ;
.
<https://w3id.org/con-tax/components/aat-furn#300039046>
  rdf:type owl:Class ;
  rdfs:comment "Benaming die in de 18e eeuw werd gebruikt voor commodes die op hoge poten stonden, met twee rijen laden boven elkaar. De benaming werd later gebruikt voor commodes met drie of vier rijen laden boven elkaar."@nl ;
  rdfs:comment "Term used in the 18th century for commodes with two tiers of drawers set on high legs; term later used for commodes with three or four tiers of drawers."@en ;
  rdfs:isDefinedBy <https://w3id.org/con-tax/components/aat-furn> ;
  rdfs:label "commode à la régence"@nl ;
  rdfs:label "commodes à la régence"@en ;
  rdfs:label "commodes à la régence"@nl ;
  rdfs:seeAlso <http://vocab.getty.edu/aat/300039046> ;
  rdfs:subClassOf <https://w3id.org/con-tax/components/aat-furn#300077277> ;
.
<https://w3id.org/con-tax/components/aat-furn#300039047>
  rdf:type owl:Class ;
  rdfs:comment "Commodes met twee wandkastdeuren aan de voorkant in plaats van laden. Binnenin de kast kunnen laden of openkast-systemen zitten."@nl ;
  rdfs:comment "Commodes with two cupboard doors instead of the more usual drawer front. Inside there may be drawers or open shelves."@en ;
  rdfs:isDefinedBy <https://w3id.org/con-tax/components/aat-furn> ;
  rdfs:label "commode à vantaux"@nl ;
  rdfs:label "commodes à vantaux"@en ;
  rdfs:label "commodes à vantaux"@nl ;
  rdfs:seeAlso <http://vocab.getty.edu/aat/300039047> ;
  rdfs:subClassOf <https://w3id.org/con-tax/components/aat-furn#300077277> ;
.
<https://w3id.org/con-tax/components/aat-furn#300039050>
  rdf:type owl:Class ;
  rdfs:comment "Commodes met een enkele la op hoge poten die waarschijnlijk zijn bestemd om onder een spiegel te staan."@nl ;
  rdfs:comment "Commodes which consist of a single drawer set on tall legs presumably intended to stand beneath a mirror."@en ;
  rdfs:isDefinedBy <https://w3id.org/con-tax/components/aat-furn> ;
  rdfs:label "commode en console"@nl ;
  rdfs:label "commodes en console"@en ;
  rdfs:label "commodes en console"@nl ;
  rdfs:seeAlso <http://vocab.getty.edu/aat/300039050> ;
  rdfs:subClassOf <https://w3id.org/con-tax/components/aat-furn#300077277> ;
.
<https://w3id.org/con-tax/components/aat-furn#300039055>
  rdf:type owl:Class ;
  rdfs:comment "Kleine, smalle ladenkasten of kabinetten die zijn bestemd om onder een spiegel te staan."@nl ;
  rdfs:comment "Small and narrow chests of drawers or cabinets intended to stand beneath a mirror."@en ;
  rdfs:isDefinedBy <https://w3id.org/con-tax/components/aat-furn> ;
  rdfs:label "demi-commode"@nl ;
  rdfs:label "demi-commodes"@en ;
  rdfs:label "demi-commodes"@nl ;
  rdfs:seeAlso <http://vocab.getty.edu/aat/300039055> ;
  rdfs:subClassOf <https://w3id.org/con-tax/components/aat-furn#300077277> ;
.
<https://w3id.org/con-tax/components/aat-furn#300039072>
  rdf:type owl:Class ;
  rdfs:comment "Hoge kasten die meestal zeven of meer laden hebben en door een kroonlijst in twee secties zijn verdeeld. De onderste kast lijkt op een vergrote toilettafel en de bovenste lijkt op een ladenkast. Gebruik 'tallboys' voor soortgelijke Engelse meubelstukken."@nl ;
  rdfs:comment "Tall case pieces generally having seven or more drawers, and divided by a cornice into two sections, consisting of a lower case resembling an enlarged dressing table and an upper case resembling a chest of drawers. For equivalent English pieces, use \"tallboys (furniture).\""@en ;
  rdfs:isDefinedBy <https://w3id.org/con-tax/components/aat-furn> ;
  rdfs:label "high chests of drawers"@en ;
  rdfs:label "hoge ladenkast"@nl ;
  rdfs:label "hoge ladenkasten"@nl ;
  rdfs:seeAlso <http://vocab.getty.edu/aat/300039072> ;
  rdfs:subClassOf <https://w3id.org/con-tax/components/aat-furn#300039009> ;
.
<https://w3id.org/con-tax/components/aat-furn#300039119>
  rdf:type owl:Class ;
  rdfs:comment "Kleine kisten voor het opbergen van kostbaarheden. Ze kunnen ook als zitplaats of tafel dienen."@nl ;
  rdfs:comment "Small chests for the storage of valuables which may also serve as seats or tables."@en ;
  rdfs:isDefinedBy <https://w3id.org/con-tax/components/aat-furn> ;
  rdfs:label "coffers (furniture)"@en ;
  rdfs:label "koffer (meubilair)"@nl ;
  rdfs:label "koffer"@nl ;
  rdfs:label "koffers (meubilair)"@nl ;
  rdfs:label "koffers"@nl ;
  rdfs:seeAlso <http://vocab.getty.edu/aat/300039119> ;
  rdfs:seeAlso wd:Q640104 ;
  rdfs:subClassOf <https://w3id.org/con-tax/components/aat-furn#300038992> ;
.
<https://w3id.org/con-tax/components/aat-furn#300039121>
  rdf:type owl:Class ;
  rdfs:comment "19th-century term for heavy iron-bound coffers used for the storage of valuables; generally of German make and rarely dating from before the 17th century."@en ;
  rdfs:comment "Benaming uit de 19e eeuw voor met veel ijzer beslagen koffers waarin kostbaarheden werden opgeborgen. Ze zijn meestal van Duitse makelij en dateren over het algemeen van na  de 17e eeuw."@nl ;
  rdfs:isDefinedBy <https://w3id.org/con-tax/components/aat-furn> ;
  rdfs:label "armada chests"@en ;
  rdfs:label "armadakist"@nl ;
  rdfs:label "armadakisten"@nl ;
  rdfs:seeAlso <http://vocab.getty.edu/aat/300039121> ;
  rdfs:subClassOf <https://w3id.org/con-tax/components/aat-furn#300039119> ;
.
<https://w3id.org/con-tax/components/aat-furn#300039122>
  rdf:type owl:Class ;
  rdfs:comment "Medieval French term for portable coffers or chests used for personal luggage, covered in leather and studded with nails and usually having a rounded top. Eventually they took the form of a chest mounted on feet, used for storing goods. The current French form is a decorative high chest or cabinet with an arched or curved top."@en ;
  rdfs:comment "Middeleeuwse Franse benaming voor draagbare koffers of kisten die voor persoonlijke bagage worden gebruikt. Ze zijn met leer bedekt en met spijkers beslagen en hebben meestal een afgeronde bovenkant. Uiteindelijk namen ze de vorm aan van een kist op poten die werd gebruikt om goederen in op te slaan. De huidige Franse vorm bestaat uit een decoratieve hoge kist of kast met een gewelfde ofgebogen bovenkant."@nl ;
  rdfs:isDefinedBy <https://w3id.org/con-tax/components/aat-furn> ;
  rdfs:label "bahut"@nl ;
  rdfs:label "bahuts"@en ;
  rdfs:label "bahuts"@nl ;
  rdfs:seeAlso <http://vocab.getty.edu/aat/300039122> ;
  rdfs:seeAlso wd:Q4842939 ;
  rdfs:subClassOf <https://w3id.org/con-tax/components/aat-furn#300039119> ;
.
<https://w3id.org/con-tax/components/aat-furn#300039124>
  rdf:type owl:Class ;
  rdfs:comment "Houten kisten die vaak met leer werden bedekt en verguld of met ijzer beslagen. Ze werden gebruikt als reiskoffer om paperassen, kostbaarheden en kleding in op te bergen. Dit type werd aan het eind van de Middeleeuwen gemaakt."@nl ;
  rdfs:comment "Wood boxes, often covered in leather and tooled in gilt or bound with iron, which were used as traveling trunks to store papers, valuables, and clothes; of a type made in the late Medieval period."@en ;
  rdfs:isDefinedBy <https://w3id.org/con-tax/components/aat-furn> ;
  rdfs:label "trussing coffer"@nl ;
  rdfs:label "trussing coffers"@en ;
  rdfs:label "trussing coffers"@nl ;
  rdfs:seeAlso <http://vocab.getty.edu/aat/300039124> ;
  rdfs:subClassOf <https://w3id.org/con-tax/components/aat-furn#300039119> ;
.
<https://w3id.org/con-tax/components/aat-furn#300039125>
  rdf:type owl:Class ;
  rdfs:comment "Chests made to commemorate or anticipate a wedding; usually incorporating names and dates in their decoration."@en ;
  rdfs:comment "Kisten die voor een bruiloft zijn gemaakt of ter nagedachtenis hiervan. Meestal werden er  namen en data in de decoraties verwerkt."@nl ;
  rdfs:isDefinedBy <https://w3id.org/con-tax/components/aat-furn> ;
  rdfs:label "bruidskist"@nl ;
  rdfs:label "bruidskisten"@nl ;
  rdfs:label "dower chests"@en ;
  rdfs:label "huwelijkskist"@nl ;
  rdfs:label "huwelijkskisten"@nl ;
  rdfs:seeAlso <http://vocab.getty.edu/aat/300039125> ;
  rdfs:subClassOf <https://w3id.org/con-tax/components/aat-furn#300038992> ;
.
<https://w3id.org/con-tax/components/aat-furn#300039136>
  rdf:type owl:Class ;
  rdfs:comment "Benaming die wordt gebruikt voor kisten met een voetstuk dat twee of meer laden bevat."@nl ;
  rdfs:comment "Term used for chests having a base containing two or more drawers."@en ;
  rdfs:isDefinedBy <https://w3id.org/con-tax/components/aat-furn> ;
  rdfs:label "mule chest"@nl ;
  rdfs:label "mule chests"@en ;
  rdfs:label "mule chests"@nl ;
  rdfs:seeAlso <http://vocab.getty.edu/aat/300039136> ;
  rdfs:subClassOf <https://w3id.org/con-tax/components/aat-furn#300038992> ;
.
<https://w3id.org/con-tax/components/aat-furn#300039137>
  rdf:type owl:Class ;
  rdfs:comment "Seaman's chests, generally used to store personal property."@en ;
  rdfs:isDefinedBy <https://w3id.org/con-tax/components/aat-furn> ;
  rdfs:label "sea chests"@en ;
  rdfs:label "zeekist"@nl ;
  rdfs:label "zeekisten"@nl ;
  rdfs:seeAlso <http://vocab.getty.edu/aat/300039137> ;
  rdfs:seeAlso wd:Q1523365 ;
  rdfs:subClassOf <https://w3id.org/con-tax/components/aat-furn#300038992> ;
.
<https://w3id.org/con-tax/components/aat-furn#300039139>
  rdf:type owl:Class ;
  rdfs:comment "Miniature chests consisting of innumerable small drawers for holding spices; intended to be placed on a table or chest of drawers."@en ;
  rdfs:comment "Miniatuurkisten met ontelbaar veel kleine laadjes voor kruiden. Ze worden op een tafel of een ladenkast gezet."@nl ;
  rdfs:isDefinedBy <https://w3id.org/con-tax/components/aat-furn> ;
  rdfs:label "specerijkist"@nl ;
  rdfs:label "specerijkisten"@nl ;
  rdfs:label "spice chests"@en ;
  rdfs:seeAlso <http://vocab.getty.edu/aat/300039139> ;
  rdfs:subClassOf <https://w3id.org/con-tax/components/aat-furn#300038992> ;
.
<https://w3id.org/con-tax/components/aat-furn#300039142>
  rdf:type owl:Class ;
  rdfs:comment "Gespecialiseerde meubelstukken die vooral voorkomen in het zuiden van de Verenigde Staten. Ze hebben meestal een scharnierende deksel bovenop een grote, verdeelde opslagkamer voor bruine en witte suiker."@nl ;
  rdfs:comment "Specialized furniture form most popular in the American South; generally having a hinged lid on top covering a large divided storage chamber for brown and white sugar."@en ;
  rdfs:isDefinedBy <https://w3id.org/con-tax/components/aat-furn> ;
  rdfs:label "sugar chests"@en ;
  rdfs:label "suikerkist"@nl ;
  rdfs:label "suikerkisten"@nl ;
  rdfs:seeAlso <http://vocab.getty.edu/aat/300039142> ;
  rdfs:subClassOf <https://w3id.org/con-tax/components/aat-furn#300038992> ;
.
<https://w3id.org/con-tax/components/aat-furn#300039143>
  rdf:type owl:Class ;
  rdfs:comment "Square wooden cases usually fixed with sheet lead or tin and used for exporting tea."@en ;
  rdfs:comment "Vierkante, houten kisten die meestal worden verstevigd met bladlood of -tin en worden gebruikt om thee in te vervoeren."@nl ;
  rdfs:isDefinedBy <https://w3id.org/con-tax/components/aat-furn> ;
  rdfs:label "tea chests"@en ;
  rdfs:label "theekist"@nl ;
  rdfs:label "theekisten"@nl ;
  rdfs:seeAlso <http://vocab.getty.edu/aat/300039143> ;
  rdfs:seeAlso wd:Q7691116 ;
  rdfs:subClassOf <https://w3id.org/con-tax/components/aat-furn#300038992> ;
.
<https://w3id.org/con-tax/components/aat-furn#300039169>
  rdf:type owl:Class ;
  rdfs:comment "Chests richly decorated with marquetry patterns of arches and fantastic architecture, reminiscent of Henry VIII's (vanished) palace of Nonsuch; the appellation means unequalled. Probably made in North Germany, or by 16th-century German craftsmen who settled in London."@en ;
  rdfs:comment "Kisten die rijkelijk zijn versierd met inlegwerk van gewelven  en fantasie-architectuur ter nagedachtenis van het (verdwenen) paleis Nonsuch van Hendrik VIII. De naam van het paleis betekent 'ongeëvenaard'. Ze zijn waarschijnlijk in Noord-Duitsland gemaakt, of in London door 16e-eeuwse Duitse handwerkslieden die zich daar hadden gevestigd."@nl ;
  rdfs:isDefinedBy <https://w3id.org/con-tax/components/aat-furn> ;
  rdfs:label "Nonsuch chests"@en ;
  rdfs:label "Nonsuch kist"@nl ;
  rdfs:label "Nonsuch kisten"@nl ;
  rdfs:seeAlso <http://vocab.getty.edu/aat/300039169> ;
  rdfs:subClassOf <https://w3id.org/con-tax/components/aat-furn#300038992> ;
.
<https://w3id.org/con-tax/components/aat-furn#300039183>
  rdf:type owl:Class ;
  rdfs:comment "Benaming die oorspronkelijk werd gebruikt voor planken of openplank-systemen waarop - met name zilveren - kopjes konden worden geplaatst of vertoond. De benaming werd in de Middeleeuwen vaak onderling verwisseld met buffetten en keukenkasten. In het begin van de 15e eeuw werden deuren toegevoegd.Tegenwoordig is het een algemene benaming voor alle vergaarplaatsen die met deuren worden afgesloten en soms zijn ingebouwd."@nl ;
  rdfs:comment "General term for a closet or a cabinet enclosed by doors, often placed in a corner of a room or a recess in the wall, with shelves for keeping cups, dishes, provisions, books, or valuables. Originally boards or open structures of shelves on which cups, especially silver, might be placed for storage or display. Beginning in the 15th century, doors were added."@en ;
  rdfs:isDefinedBy <https://w3id.org/con-tax/components/aat-furn> ;
  rdfs:label "cupboards (case furniture)"@en ;
  rdfs:label "wandkast"@nl ;
  rdfs:label "wandkasten"@nl ;
  rdfs:seeAlso <http://vocab.getty.edu/aat/300039183> ;
  rdfs:seeAlso wd:Q5662058 ;
  rdfs:subClassOf <https://w3id.org/con-tax/components/aat-furn#300038860> ;
  rdfs:subClassOf <https://w3id.org/con-tax/components/aat-furn#300040157> ;
.
<https://w3id.org/con-tax/components/aat-furn#300039198>
  rdf:type owl:Class ;
  rdfs:comment "Italiaanse wandkasten die oorspronkelijk bestonden uit cassoni met een deur in plaats van een deksel maar die zich later (16e eeuw) tot een tweedelig meubel ontwikkelden dat op de Engelse perskast lijkt. Ze hebben meestal veel architectonische decoratie, inclusief pilaren met een monumentale deklijst. Ze worden vaak voor sacristieën gebruikt."@nl ;
  rdfs:comment "Italian cupboards that were originally cassoni with doors instead of a lid, but from the 16th century developed into two-tiered pieces similar to English press cupboards. Generally having massive architectural decoration, including pilasters supporting a monumental cornice; frequently made for sacristies."@en ;
  rdfs:isDefinedBy <https://w3id.org/con-tax/components/aat-furn> ;
  rdfs:label "armadio"@nl ;
  rdfs:label "armadio's"@nl ;
  rdfs:label "armadios"@en ;
  rdfs:seeAlso <http://vocab.getty.edu/aat/300039198> ;
  rdfs:subClassOf <https://w3id.org/con-tax/components/aat-furn#300039007> ;
  rdfs:subClassOf <https://w3id.org/con-tax/components/aat-furn#300039183> ;
.
<https://w3id.org/con-tax/components/aat-furn#300039206>
  rdf:type owl:Class ;
  rdfs:comment "Grote, maar tamelijk lage wandkasten met bovenin een opbergkast en onderin een openkast-systeem of planken. Dit type werd in de 16e en 17e eeuw in Engeland en in de 17e eeuw in Amerika gemaakt. Te onderscheiden van 'perskasten' die een dichte boven- en onderkant hebben."@nl ;
  rdfs:comment "Large but fairly low cupboards with an enclosed storage cabinet above and an open shelf or shelves below, or having two or three shelves and no enclosed cabinet. It is a type made in 16th- and 17th-century England and 17th-century America. Distinct from \"press cupboards,\" which have both the upper and lower sections enclosed."@en ;
  rdfs:isDefinedBy <https://w3id.org/con-tax/components/aat-furn> ;
  rdfs:label "court cupboard"@nl ;
  rdfs:label "court cupboards"@en ;
  rdfs:label "court cupboards"@nl ;
  rdfs:seeAlso <http://vocab.getty.edu/aat/300039206> ;
  rdfs:seeAlso wd:Q847462 ;
  rdfs:subClassOf <https://w3id.org/con-tax/components/aat-furn#300039183> ;
.
<https://w3id.org/con-tax/components/aat-furn#300039218>
  rdf:type owl:Class ;
  rdfs:comment "Benaming die in het midden van de 16e eeuw in Engeland in gebruik kwam voor vrijstaande kasten waarin voedsel en drinken wordt opgeslagen. Ze hebben de vorm van een twee kasten op elkaar, waarvan de deuren van spijlen of perforatie zijn voorzien voor de ventilatie. Gebruik 'spinden' om naar soortgelijke vormen te verwijzen die voor, na of tijdens de middeleeuwen zijn gemaakt."@nl ;
  rdfs:comment "Freestanding cupboards, particulary with reference to cupboards in use in the mid-16th century in England for freestanding cupboards used for the storage of food and drink, generally in the form of a two-tier cupboard with pierced or spindle doors for ventilation. Use \"aumbries\" with reference to similar forms made before, after, or during the Medieval period."@en ;
  rdfs:isDefinedBy <https://w3id.org/con-tax/components/aat-furn> ;
  rdfs:label "livery cupboards"@en ;
  rdfs:label "provisiekast"@nl ;
  rdfs:label "provisiekasten"@nl ;
  rdfs:seeAlso <http://vocab.getty.edu/aat/300039218> ;
  rdfs:subClassOf <https://w3id.org/con-tax/components/aat-furn#300249925> ;
.
<https://w3id.org/con-tax/components/aat-furn#300039221>
  rdf:type owl:Class ;
  rdfs:comment "Middeleeuwse benaming voor in de muur uitgespaarde wandkasten of opbergruimten die door deuren zijn afgesloten. Ze dienden als vergaarplaats voor levensmiddelen die als aalmoezen werden weggegeven. De benaming bleef voornamelijk in gebruik voor aumbries die in de muur waren uitgespaard of aan de muur hingen nabij het altaar in een kerk waarin gewijde voorwerpen werden bewaard. Gebruik 'wandkasten' voor soortgelijke, met deuren afgesloten kasten van na de 17e eeuw."@nl ;
  rdfs:comment "Places for keeping victuals; variously applied to a store-closet, pantry, or cupboard in a pantry. The term was first used in the Medieval period for enclosed cupboards or storage niches enclosed by doors; often a receptacle for provisions to be given away as alms. The term remained in use chiefly for the aumbries enclosed in or hung on a wall near the altar in churches in which sacramental vessels were kept. When referring to such forms enclosed by doors from the 17th century on, use \"cupboards.\""@en ;
  rdfs:isDefinedBy <https://w3id.org/con-tax/components/aat-furn> ;
  rdfs:label "aumbries"@en ;
  rdfs:label "spinde"@nl ;
  rdfs:label "spinden"@nl ;
  rdfs:seeAlso <http://vocab.getty.edu/aat/300039221> ;
  rdfs:seeAlso wd:Q4821857 ;
  rdfs:subClassOf <https://w3id.org/con-tax/components/aat-furn#300249925> ;
.
<https://w3id.org/con-tax/components/aat-furn#300039235>
  rdf:type owl:Class ;
  rdfs:comment "Grote, maar tamelijk lage wandkasten met een afgesloten opbergruimte in het boven- en ondergedeelte. Dit type werd gemaakt in de 16e en 17e eeuw in Engeland en in de 17e eeuw in Amerika. Te onderscheiden van '@court cupboards', waarbij het bovengedeelte een afgesloten opbergkast en het ondergedeelte een of meerdere open planken heeft."@nl ;
  rdfs:comment "Large, but fairly low, cupboards with both the upper and lower sections containing enclosed storage space; of a type made in 16th- and 17th-century England and 17th-century America. Distinct from \"court cupboards\" which have an enclosed storage cabinet above and an open shelf or shelves below."@en ;
  rdfs:isDefinedBy <https://w3id.org/con-tax/components/aat-furn> ;
  rdfs:label "press cupboard"@nl ;
  rdfs:label "press cupboards"@en ;
  rdfs:label "press cupboards"@nl ;
  rdfs:seeAlso <http://vocab.getty.edu/aat/300039235> ;
  rdfs:subClassOf <https://w3id.org/con-tax/components/aat-furn#300039252> ;
.
<https://w3id.org/con-tax/components/aat-furn#300039236>
  rdf:type owl:Class ;
  rdfs:comment "Cupboards that are constructed in three levels, the lower two levels closed by doors and the upper level opened for display."@en ;
  rdfs:comment "Wandkasten uit Wales die uit drie delen bestaan; de onderste twee delen zijn door twee deuren gesloten en het bovenste gedeelte is open gelaten om voorwerpen te vertonen."@nl ;
  rdfs:isDefinedBy <https://w3id.org/con-tax/components/aat-furn> ;
  rdfs:label "tridarns"@en ;
  rdfs:label "tridarns"@nl ;
  rdfs:seeAlso <http://vocab.getty.edu/aat/300039236> ;
  rdfs:subClassOf <https://w3id.org/con-tax/components/aat-furn#300039252> ;
.
<https://w3id.org/con-tax/components/aat-furn#300039237>
  rdf:type owl:Class ;
  rdfs:comment "Large upright pieces of furniture fitted with hooks, pegs, or rods, used for hanging clothes, generally with two large doors and perhaps a drawer or drawers below. Although there may be a shelf in a wardrobe, the term is typically distinct from \"clothes presses,\" in which clothes are stored exclusively on shelves rather than hanging."@en ;
  rdfs:comment "Wordt gebruikt voor grote, rechtopstaande meubelstukken, met name de meubels met haakjes, knijpers of roedes om kleren aan op te hangen. Ze hebben meestal twee grote deuren en kunnen één of meerdere laden aan de onderkant hebben."@nl ;
  rdfs:isDefinedBy <https://w3id.org/con-tax/components/aat-furn> ;
  rdfs:label "kledingkast"@nl ;
  rdfs:label "kledingkasten"@nl ;
  rdfs:label "kleerkast"@nl ;
  rdfs:label "kleerkasten"@nl ;
  rdfs:label "wardrobes (case furniture)"@en ;
  rdfs:seeAlso <http://vocab.getty.edu/aat/300039237> ;
  rdfs:subClassOf <https://w3id.org/con-tax/components/aat-furn#300038860> ;
.
<https://w3id.org/con-tax/components/aat-furn#300039240>
  rdf:type owl:Class ;
  rdfs:comment "Originally large closets or chests for storing arms, implements, or tools. Today refers to French-styled wardrobes for the storage of clothing or linens, with large doors opening to shelves, sometimes with drawers on the bottom of the piece, and short legs."@en ;
  rdfs:comment "Wordt gebruikt om te verwijzen naar kleerkasten in Franse stijl waarin kleding of linnengoed wordt opgeborgen."@nl ;
  rdfs:isDefinedBy <https://w3id.org/con-tax/components/aat-furn> ;
  rdfs:label "armoire"@nl ;
  rdfs:label "armoires"@en ;
  rdfs:label "armoires"@nl ;
  rdfs:seeAlso <http://vocab.getty.edu/aat/300039240> ;
  rdfs:subClassOf <https://w3id.org/con-tax/components/aat-furn#300039237> ;
.
<https://w3id.org/con-tax/components/aat-furn#300039243>
  rdf:type owl:Class ;
  rdfs:comment "Franse bergmeubels die bestaan uit twee wandkasten  boven op elkaar, elk met twee deuren waarbij de voorkant en de zijdes van de bovenste kast iets zijn verzonken. Ze hebben meestal een architectonisch raamwerk met pilasters die door een timpaan worden bekroond."@nl ;
  rdfs:comment "French case furniture consisting of two cupboards, set one above the other, each with two doors, the front and sides of the upper cupboard being recessed. They generally have an architectural framework with pilasters and a crowning pediment."@en ;
  rdfs:isDefinedBy <https://w3id.org/con-tax/components/aat-furn> ;
  rdfs:label "amoire à deux corps"@nl ;
  rdfs:label "amoires à deux corps"@nl ;
  rdfs:label "armoires à deux corps"@en ;
  rdfs:seeAlso <http://vocab.getty.edu/aat/300039243> ;
  rdfs:subClassOf <https://w3id.org/con-tax/components/aat-furn#300039240> ;
.
<https://w3id.org/con-tax/components/aat-furn#300039249>
  rdf:type owl:Class ;
  rdfs:comment "Wardrobes that are a typically American variations on the 17th-century Netherlandish kast or large cupboard; made by Dutch settlers in the Hudson and Delaware valleys about 1675-1750 and more widely into the 19th century. Generally have two raised paneled doors, and a heavy overhanging cornice with a drawer or drawers below; sometimes decoratively painted with grisaille panels and fruit."@en ;
  rdfs:comment "Wordt gebruikt voor de Amerikaanse versie van de 17e-eeuwse Nederlandse kast of grote wandkast, die rond 1675-1750 door Nederlandse immigranten in het laagland van de Hudson en Delaware werden gemaakt en vanaf  de 19e eeuw ook elders. Ze hebben meestal twee   deuren met opgelegde panelen en een zware, overhangende kroonlijst met één of meerdere laden eronder. Soms zijn ze decoratief beschilderd met grisaillepanelen en fruit."@nl ;
  rdfs:isDefinedBy <https://w3id.org/con-tax/components/aat-furn> ;
  rdfs:label "kas (meubilair)"@nl ;
  rdfs:label "kas"@nl ;
  rdfs:label "kassen (meubilair)"@nl ;
  rdfs:label "kassen (wardrobes)"@en ;
  rdfs:label "kassen"@nl ;
  rdfs:seeAlso <http://vocab.getty.edu/aat/300039249> ;
  rdfs:subClassOf <https://w3id.org/con-tax/components/aat-furn#300039237> ;
.
<https://w3id.org/con-tax/components/aat-furn#300039252>
  rdf:type owl:Class ;
  rdfs:comment "Benaming uit de middeleeuwen die meestal van toepassing is op grote wandkasten met deuren en planken om linnengoed, kleding en keukengerei in op te bergen. Gebruik 'clothes presses' voor presses met schuivende planken en dichte deuren."@nl ;
  rdfs:comment "Term of Medieval origin generally applied to tall cupboards with doors and shelves for storing linens, clothing, and kitchen utensils. For presses with sliding shelves behind closed doors, use \"clothes presses.\""@en ;
  rdfs:isDefinedBy <https://w3id.org/con-tax/components/aat-furn> ;
  rdfs:label "press (cupboard)"@nl ;
  rdfs:label "press"@nl ;
  rdfs:label "presses (cupboards)"@en ;
  rdfs:label "presses (cupboards)"@nl ;
  rdfs:label "presses"@nl ;
  rdfs:seeAlso <http://vocab.getty.edu/aat/300039252> ;
  rdfs:subClassOf <https://w3id.org/con-tax/components/aat-furn#300039183> ;
.
<https://w3id.org/con-tax/components/aat-furn#300039253>
  rdf:type owl:Class ;
  rdfs:comment "18e-eeuwse benaming voor grote wandkasten met schuivende planken achter dichte deuren, waarin kleding wordt opgeborgen. Gebruik 'kleerkasten' voor grote kasten met haken, knijpers of roedes om kleren aan te hangen."@nl ;
  rdfs:comment "Eighteenth-century term for large chests or cupboards used to store clothes, often having sliding shelves behind closed doors. For large upright case pieces fitted with hooks, pegs, or rods to hang clothes, use \"wardrobes (case furniture).\""@en ;
  rdfs:isDefinedBy <https://w3id.org/con-tax/components/aat-furn> ;
  rdfs:label "clothes presse"@nl ;
  rdfs:label "clothes presses"@en ;
  rdfs:label "clothes presses"@nl ;
  rdfs:seeAlso <http://vocab.getty.edu/aat/300039253> ;
  rdfs:subClassOf <https://w3id.org/con-tax/components/aat-furn#300039252> ;
.
<https://w3id.org/con-tax/components/aat-furn#300039264>
  rdf:type owl:Class ;
  rdfs:comment "German wardrobes for the storage of clothes and linens; generally with two paneled doors and sometimes having one side with drawers and shelves and the other side an open space for hanging clothes."@en ;
  rdfs:comment "Wordt gebruikt voor een kleerkast, oorspronkelijk van een Duits type, waarin kleding en linnengoed wordt opgeborgen. Ze hebben meestal twee deuren met panelen en soms aan één kant laden en planken en aan de andere kant een open ruimte om kleren op te hangen."@nl ;
  rdfs:isDefinedBy <https://w3id.org/con-tax/components/aat-furn> ;
  rdfs:label "schrank"@nl ;
  rdfs:label "schranks"@en ;
  rdfs:label "schranks"@nl ;
  rdfs:seeAlso <http://vocab.getty.edu/aat/300039264> ;
  rdfs:subClassOf <https://w3id.org/con-tax/components/aat-furn#300039237> ;
.
<https://w3id.org/con-tax/components/aat-furn#300039285>
  rdf:type owl:Class ;
  rdfs:comment "Freestanding, built-in, or hanging cupboards made to fit the shape of a room's corner."@en ;
  rdfs:comment "Vrijstaande, hangende of ingebouwde kasten, die zo gemaakt zijn dat ze precies in een hoek van een kamer passen."@nl ;
  rdfs:isDefinedBy <https://w3id.org/con-tax/components/aat-furn> ;
  rdfs:label "corner cupboards"@en ;
  rdfs:label "hoekkast"@nl ;
  rdfs:label "hoekkasten"@nl ;
  rdfs:seeAlso <http://vocab.getty.edu/aat/300039285> ;
  rdfs:subClassOf <https://w3id.org/con-tax/components/aat-furn#300039183> ;
  rdfs:subClassOf <https://w3id.org/con-tax/components/aat-furn#300040157> ;
.
<https://w3id.org/con-tax/components/aat-furn#300039298>
  rdf:type owl:Class ;
  rdfs:comment "Relatief kleine kasten gemaakt om te worden opgehangen aan een muur in plaats van op de vloer te staan, soms boven een groter kastmeubel gehangen."@nl ;
  rdfs:comment "Relatively small cupboards constructed to be hung on a wall rather than standing on the floor, sometimes placed above a larger piece of case furnture."@en ;
  rdfs:isDefinedBy <https://w3id.org/con-tax/components/aat-furn> ;
  rdfs:label "hangende kast"@nl ;
  rdfs:label "hangende kasten"@nl ;
  rdfs:label "hanging cupboards"@en ;
  rdfs:seeAlso <http://vocab.getty.edu/aat/300039298> ;
  rdfs:subClassOf <https://w3id.org/con-tax/components/aat-furn#300039183> ;
.
<https://w3id.org/con-tax/components/aat-furn#300039300>
  rdf:type owl:Class ;
  rdfs:comment "Open-tiered shelves for displaying small objects; often with a mirrored back and sometimes having drawers or a cabinet below."@en ;
  rdfs:comment "Openkast-systeem met planken boven elkaar, waarop kleine voorwerpen worden vertoond. Ze hebben vaak een spiegel aan de achterkant en soms laden of een kastje aan de onderkant."@nl ;
  rdfs:isDefinedBy <https://w3id.org/con-tax/components/aat-furn> ;
  rdfs:label "etagère (opslag en tentoonstellingsmeubilair)"@nl ;
  rdfs:label "etagère"@nl ;
  rdfs:label "étagères (opslag en tentoonstellingsmeubilair)"@nl ;
  rdfs:label "étagères (shelves)"@en ;
  rdfs:label "étagères"@nl ;
  rdfs:seeAlso <http://vocab.getty.edu/aat/300039300> ;
  rdfs:seeAlso wd:Q1370886 ;
  rdfs:subClassOf <https://w3id.org/con-tax/components/aat-furn#300037680> ;
.
<https://w3id.org/con-tax/components/aat-furn#300039305>
  rdf:type owl:Class ;
  rdfs:comment "Chests of drawers having seven drawers and intended to hold a week's supply of clothing; of a type originally made in 18th-century France, Italy, and elsewhere."@en ;
  rdfs:comment "Ladenkasten met zeven laden waarin kleding voor de hele week zit. Dit type werd oorspronkelijk in de 18e eeuw in Frankrijk gemaakt."@nl ;
  rdfs:isDefinedBy <https://w3id.org/con-tax/components/aat-furn> ;
  rdfs:label "semainiers"@en ;
  rdfs:label "semanier"@nl ;
  rdfs:label "semaniers"@nl ;
  rdfs:seeAlso <http://vocab.getty.edu/aat/300039305> ;
  rdfs:subClassOf <https://w3id.org/con-tax/components/aat-furn#300039009> ;
.
<https://w3id.org/con-tax/components/aat-furn#300039306>
  rdf:type owl:Class ;
  rdfs:comment "Brede, meestal lage ladekasten of kastmeubilair op poten, met kastruimte. De kasten worden langs de muur van een eetkamer geplaatst en gebruikt als bewaarplaats en voor het opdienen van voedsel, alsmede voor het uitstallen van borden en ander kostbaar tafelgerei. Vroege exemplaren bestonden vaak slechts uit een plank die bij de eettafel werd geplaatst, en kwamen uitsluitend voor in ruimten waar werd gegeten. Gedurende de middeleeuwen vervulde de kast dezelfde functie. Vroege Europese dressoirs waren vaak etagegewijs opgebouwd, met schappen waarop koppen en schotels konden worden uitgestald. In de 17de eeuw werden de dressoirs ontworpen met een kast of een aantal laden onder een vlak tafelblad. De bovenzijde was hoger dan bij een gewone tafel, waardoor de borden beter zichtbaar waren en het voedsel eenvoudiger bereikbaar was voor een staand persoon. Soms gebruikte men ook dressoirtafels of zijtafels waarop al het voedsel werd uitgestald, en dienden de kostbaarder uitgevoerde dressoirs uitsluitend voor het uitstallen van servieswaar. 'Keukenkasten (wandkasten)' kunnen ongeveer dezelfde vorm en functie hebben, maar kwamen meestal in keukens voor en niet in eetkamers. Gebruik 'dressoirtafels' voor wandtafels die langs de wand van eetkamers worden gebruikt."@nl ;
  rdfs:comment "In modern usage, a general term for case furniture of various designs, sometimes on legs, with cupboard space beneath and placed along the wall of a dining room for serving, storage, and displaying plate and other precious tableware. However, in early usage may refer to a table, as the term derives from pieces that were often simply a board on legs placed near the dining table. By the 17th century sideboards were being designed with a cupboard or drawers beneath a flat table surface. The top was higher than a standard table, allowing the plate on display to be seen easily, as well as making the food more conveniently accessible to a standing person. Victorian sideboards often had levels or shelves above the primary surface, in order to create more space for displaying tableware. \"Dressers (cupboards)\" may be similar in design and function, but were typically found in kitchens rather than dining rooms. In modern usage, for side tables used along the walls of dining rooms, use \"sideboard tables\" or the broader term \"serving tables.\""@en ;
  rdfs:isDefinedBy <https://w3id.org/con-tax/components/aat-furn> ;
  rdfs:label "dressoir (meubel)"@nl ;
  rdfs:label "dressoir"@nl ;
  rdfs:label "dressoirs (meubilair)"@nl ;
  rdfs:label "dressoirs"@nl ;
  rdfs:label "sideboards (furniture)"@en ;
  rdfs:seeAlso <http://vocab.getty.edu/aat/300039306> ;
  rdfs:seeAlso wd:Q1762308 ;
  rdfs:subClassOf <https://w3id.org/con-tax/components/aat-furn#300038860> ;
.
<https://w3id.org/con-tax/components/aat-furn#300039318>
  rdf:type owl:Class ;
  rdfs:comment "Dressoirs die aan één kant ruimte voor wijnflessen hebben en aan de andere kant een gewone la of een la die met lood is gevoerd, waarin glazen kunnen worden gewassen."@nl ;
  rdfs:comment "Sideboards with a place at one end to hold bottles of wine and at the other end either a plain drawer or a drawer lined with lead, in which glasses could be washed."@en ;
  rdfs:isDefinedBy <https://w3id.org/con-tax/components/aat-furn> ;
  rdfs:label "cellaret sideboards"@en ;
  rdfs:label "celleret sideboard"@nl ;
  rdfs:label "celleret sideboards"@nl ;
  rdfs:seeAlso <http://vocab.getty.edu/aat/300039318> ;
  rdfs:subClassOf <https://w3id.org/con-tax/components/aat-furn#300039306> ;
.
<https://w3id.org/con-tax/components/aat-furn#300039330>
  rdf:type owl:Class ;
  rdfs:comment "Refers to sideboards with a cupboard. For small, low chests of drawers, use \"chiffonnières (low chests of drawers).\""@en ;
  rdfs:comment "Verengelste naam die uit Frankrijk afkomstig is en wordt gebruikt voor een kleine wandkast waarvan het blad een dressoir vormt. Gebruik 'chiffonnières (ladenkasten)' voor kleine, lage ladenkasten."@nl ;
  rdfs:isDefinedBy <https://w3id.org/con-tax/components/aat-furn> ;
  rdfs:label "chiffoniers (sideboards)"@en ;
  rdfs:label "chiffonnière (zijtafel)"@nl ;
  rdfs:label "chiffonnière"@nl ;
  rdfs:label "chiffonnières (zijtafels)"@nl ;
  rdfs:label "chiffonnières"@nl ;
  rdfs:seeAlso <http://vocab.getty.edu/aat/300039330> ;
  rdfs:subClassOf <https://w3id.org/con-tax/components/aat-furn#300039306> ;
.
<https://w3id.org/con-tax/components/aat-furn#300039331>
  rdf:type owl:Class ;
  rdfs:comment "Franse dressoirs met één of meerdere laden onder het blad en een plank tussen de poten. Ze hebben meestal de vorm van een D maar zijn soms rechthoekig. Ze worden gebruikt om voedsel te serveren."@nl ;
  rdfs:comment "Sideboards of French design, used for the serving of food. They are characterized by having a design more like a large table than case furniture, with a shelf below and often one or more drawers."@en ;
  rdfs:isDefinedBy <https://w3id.org/con-tax/components/aat-furn> ;
  rdfs:label "console desserte"@nl ;
  rdfs:label "console dessertes"@en ;
  rdfs:label "console dessertes"@nl ;
  rdfs:seeAlso <http://vocab.getty.edu/aat/300039331> ;
  rdfs:subClassOf <https://w3id.org/con-tax/components/aat-furn#300039306> ;
  rdfs:subClassOf <https://w3id.org/con-tax/components/aat-furn#300403907> ;
.
<https://w3id.org/con-tax/components/aat-furn#300039333>
  rdf:type owl:Class ;
  rdfs:comment "Dressoirs met een la in het midden en een groot, doosachtig onderstel aan elke kant. Deze onderstellen worden vaak in compartimenten verdeeld en kunnen laden of planken hebben."@nl ;
  rdfs:comment "Sideboards having a center drawer and a large boxlike support on either end; often these supports are partitioned into divisions, or they may have drawers or shelves."@en ;
  rdfs:isDefinedBy <https://w3id.org/con-tax/components/aat-furn> ;
  rdfs:label "pedestal end sideboard"@nl ;
  rdfs:label "pedestal end sideboards"@en ;
  rdfs:label "pedestal end sideboards"@nl ;
  rdfs:seeAlso <http://vocab.getty.edu/aat/300039333> ;
  rdfs:seeAlso wd:Q21550868 ;
  rdfs:subClassOf <https://w3id.org/con-tax/components/aat-furn#300039306> ;
.
<https://w3id.org/con-tax/components/aat-furn#300039337>
  rdf:type owl:Class ;
  rdfs:comment "Furniture used to hold or support other materials."@en ;
  rdfs:isDefinedBy <https://w3id.org/con-tax/components/aat-furn> ;
  rdfs:label "ondersteunend meubilair"@nl ;
  rdfs:label "support furniture"@en ;
  rdfs:seeAlso <http://vocab.getty.edu/aat/300039337> ;
  rdfs:subClassOf <https://w3id.org/con-tax/components/aat-furn#300037680> ;
  contax:containsGuideTerm <https://w3id.org/con-tax/components/aat-furn#300435640> ;
.
<https://w3id.org/con-tax/components/aat-furn#300039338>
  rdf:type owl:Class ;
  rdfs:comment "Various forms of furniture for readers or writers, generally having a flat writing surface and often drawers and other compartments."@en ;
  rdfs:comment "Verschillende soorten meubels voor lezers of schrijvers die meestal een vlak schrijfblad, laden en andere ruimten hebben."@nl ;
  rdfs:isDefinedBy <https://w3id.org/con-tax/components/aat-furn> ;
  rdfs:label "bureau (meubilair)"@nl ;
  rdfs:label "bureau"@nl ;
  rdfs:label "bureaus (meubilair)"@nl ;
  rdfs:label "bureaus"@nl ;
  rdfs:label "desks"@en ;
  rdfs:label "schrijfmeubel"@nl ;
  rdfs:label "schrijfmeubels"@nl ;
  rdfs:seeAlso <http://vocab.getty.edu/aat/300039338> ;
  rdfs:seeAlso wd:Q1064858 ;
  rdfs:subClassOf <https://w3id.org/con-tax/components/aat-furn#300038860> ;
.
<https://w3id.org/con-tax/components/aat-furn#300039343>
  rdf:type owl:Class ;
  rdfs:comment "Benaming uit de 18e eeuw voor bureaus waarvan het onderstel op hoge poten staat."@nl ;
  rdfs:comment "Desks on frames set on high legs, of the type generally used in mercantile establishments in the early 19th century."@en ;
  rdfs:isDefinedBy <https://w3id.org/con-tax/components/aat-furn> ;
  rdfs:label "boekhoudtafel"@nl ;
  rdfs:label "boekhoudtafels"@nl ;
  rdfs:label "counting-house desks"@en ;
  rdfs:seeAlso <http://vocab.getty.edu/aat/300039343> ;
  rdfs:subClassOf <https://w3id.org/con-tax/components/aat-furn#300039338> ;
.
<https://w3id.org/con-tax/components/aat-furn#300039347>
  rdf:type owl:Class ;
  rdfs:comment "Bureaus waar een boekenkast op staat waarvan de deuren zijn beglaasd of met panelen zijn bekleed. Gebruik 'bureau-bookcases' voor soortgelijke Engelse vormen met een schuingeplaatst schrijfblad."@nl ;
  rdfs:comment "Refers to desks surmounted by a bookcase with glazed or paneled doors. For similar English forms which have a steeply sloping lid, use \"bureau-bookcases.\""@en ;
  rdfs:isDefinedBy <https://w3id.org/con-tax/components/aat-furn> ;
  rdfs:label "desk and bookcase"@nl ;
  rdfs:label "desks and bookcases"@en ;
  rdfs:label "desks and bookcases"@nl ;
  rdfs:seeAlso <http://vocab.getty.edu/aat/300039347> ;
  rdfs:subClassOf <https://w3id.org/con-tax/components/aat-furn#300039338> ;
.
<https://w3id.org/con-tax/components/aat-furn#300039355>
  rdf:type owl:Class ;
  rdfs:comment "Bureaus en boekenkasten met een scharnierend, rond deksel of bedekking die op een gedeelte van een cilinder lijkt en in de schrijftafel kan worden gerold. Ze werden voornamelijk aan het eind van de 18e en het begin van de 19e eeuw gemaakt. Gebruik 'cylinder fall desks' voor soortgelijke bureaus zonder boekenkast."@nl ;
  rdfs:comment "Desks and bookcases with a hinged one-piece round lid or cover that resembles a section of a cylinder and which rolls up into the desk top; chiefly made in the late 18th and early 19th centuries. For similar desks without a bookcase use \"cylinder fall desks.\""@en ;
  rdfs:isDefinedBy <https://w3id.org/con-tax/components/aat-furn> ;
  rdfs:label "cilinderbureau en boekenkast"@nl ;
  rdfs:label "cilinderbureaus en boekenkasten"@nl ;
  rdfs:label "cylinder desks and bookcases"@en ;
  rdfs:seeAlso <http://vocab.getty.edu/aat/300039355> ;
  rdfs:subClassOf <https://w3id.org/con-tax/components/aat-furn#300039347> ;
.
<https://w3id.org/con-tax/components/aat-furn#300039360>
  rdf:type owl:Class ;
  rdfs:comment "Verwijst naar schrijftafels, meestal met laden onder en een boekenkast boven, en vaak met een klep die als schrijfblad fungeert. De term verwees oorspronkelijk naar een kleine, draagbare schrijftafel, vaak voorzien van laden, die boven op een tafel was geplaatst of zelf op dunne poten stond. In het moderne taalgebruik worden deze kleine draagbare schrijftafels meestal aangeduid als 'escritoires', terwijl de term 'secretaires' verwijst naar grotere meubelstukken die bedoeld zijn om tegen een muur te worden geplaatst."@nl ;
  rdfs:comment "Writing desks, generally fall-front desks sitting on top of a chest of drawers, having compartments, slots, and cubbyholes above. For secretaries surmounted by a bookcase, use \"secretaries-bookcases.\" The term \"secretary\" originally referred to a small, portable writing desk, often with drawers, that was placed on top of a table. In modern usage, these small portable desks are generally called \"escritoires,\" and the term \"secretaries\" refers to larger pieces meant to be placed against a wall."@en ;
  rdfs:isDefinedBy <https://w3id.org/con-tax/components/aat-furn> ;
  rdfs:label "secretaire (meubilair)"@nl ;
  rdfs:label "secretaire"@nl ;
  rdfs:label "secretaires (meubilair)"@nl ;
  rdfs:label "secretaires"@nl ;
  rdfs:label "secretaries (furniture)"@en ;
  rdfs:seeAlso <http://vocab.getty.edu/aat/300039360> ;
  rdfs:subClassOf <https://w3id.org/con-tax/components/aat-furn#300039338> ;
.
<https://w3id.org/con-tax/components/aat-furn#300039407>
  rdf:type owl:Class ;
  rdfs:comment "Bureaus met een schuin geplaatst schrijfblad en een laag, afneembaar onderstel, die in de Queen Anne-periode  populair waren."@nl ;
  rdfs:comment "Slant-front desks supported on low removable frames, popular in the Queen Anne period."@en ;
  rdfs:isDefinedBy <https://w3id.org/con-tax/components/aat-furn> ;
  rdfs:label "desks-on-frame"@nl ;
  rdfs:label "desks-on-frames"@en ;
  rdfs:label "desks-on-frames"@nl ;
  rdfs:seeAlso <http://vocab.getty.edu/aat/300039407> ;
  rdfs:subClassOf <https://w3id.org/con-tax/components/aat-furn#300039338> ;
.
<https://w3id.org/con-tax/components/aat-furn#300039411>
  rdf:type owl:Class ;
  rdfs:comment "Benaming die meestal van toepassing is op verschillende kleine bureaus die voor vrouwen zijn ontworpen. Dit type werd populair in de 18e eeuw."@nl ;
  rdfs:comment "Term generally applied to a variety of small-scale desks designed for women; of a type popular in the 18th century."@en ;
  rdfs:isDefinedBy <https://w3id.org/con-tax/components/aat-furn> ;
  rdfs:label "damesbureau"@nl ;
  rdfs:label "damesbureaus"@nl ;
  rdfs:label "ladies' desks"@en ;
  rdfs:seeAlso <http://vocab.getty.edu/aat/300039411> ;
  rdfs:subClassOf <https://w3id.org/con-tax/components/aat-furn#300039338> ;
.
<https://w3id.org/con-tax/components/aat-furn#300039413>
  rdf:type owl:Class ;
  rdfs:comment "Bureaus met een vlak bovenblad en twee kistachtige onderstellen waarin kastjes of laden zitten."@nl ;
  rdfs:comment "Desks having a flat top and two boxlike supports either containing cupboards or drawers."@en ;
  rdfs:isDefinedBy <https://w3id.org/con-tax/components/aat-furn> ;
  rdfs:label "pedestal desks"@en ;
  rdfs:label "piëdestal schrijfmeubel"@nl ;
  rdfs:label "piëdestal schrijfmeubels"@nl ;
  rdfs:seeAlso <http://vocab.getty.edu/aat/300039413> ;
  rdfs:seeAlso wd:Q14946468 ;
  rdfs:subClassOf <https://w3id.org/con-tax/components/aat-furn#300039338> ;
.
<https://w3id.org/con-tax/components/aat-furn#300039414>
  rdf:type owl:Class ;
  rdfs:comment "Desks or stands designed with a slanted front and ledge for the positioning of an open book for comfortable reading. Desks or stands designed with a slanted front and ledge for the positioning of an open book for comfortable reading."@en ;
  rdfs:isDefinedBy <https://w3id.org/con-tax/components/aat-furn> ;
  rdfs:label "leesbureau"@nl ;
  rdfs:label "leesbureaus"@nl ;
  rdfs:label "reading desks"@en ;
  rdfs:seeAlso <http://vocab.getty.edu/aat/300039414> ;
  rdfs:seeAlso wd:Q390539 ;
  rdfs:subClassOf <https://w3id.org/con-tax/components/aat-furn#300039338> ;
.
<https://w3id.org/con-tax/components/aat-furn#300039424>
  rdf:type owl:Class ;
  rdfs:comment "Small, portable desks, designed to be sutiable for use while traveling; typically equipped with a wrting surface and containers for pens, ink, and paper."@en ;
  rdfs:isDefinedBy <https://w3id.org/con-tax/components/aat-furn> ;
  rdfs:label "reisbureau (object)"@nl ;
  rdfs:label "reisbureau"@nl ;
  rdfs:label "reisbureaus (objecten)"@nl ;
  rdfs:label "reisbureaus"@nl ;
  rdfs:label "traveling desks"@en ;
  rdfs:seeAlso <http://vocab.getty.edu/aat/300039424> ;
  rdfs:subClassOf <https://w3id.org/con-tax/components/aat-furn#300039338> ;
.
<https://w3id.org/con-tax/components/aat-furn#300039426>
  rdf:type owl:Class ;
  rdfs:comment "Benaming die vrij soepel wordt gebruikt voor de Wooton kabinetkantoorsecretaires en de '@rotary desks' die beiden door William S. Wooton zijn uitgevonden. Gebruik waar mogelijk een meer specifieke benaming."@nl ;
  rdfs:comment "Term used loosely to describe Wooton cabinet office secretaries and rotary desks, each invented by William S. Wooton. Whenever possible use more specific term."@en ;
  rdfs:isDefinedBy <https://w3id.org/con-tax/components/aat-furn> ;
  rdfs:label "Wooton desks"@en ;
  rdfs:label "Wootonbureau"@nl ;
  rdfs:label "Wootonbureaus"@nl ;
  rdfs:seeAlso <http://vocab.getty.edu/aat/300039426> ;
  rdfs:seeAlso wd:Q8034074 ;
  rdfs:subClassOf <https://w3id.org/con-tax/components/aat-furn#300039338> ;
.
<https://w3id.org/con-tax/components/aat-furn#300039427>
  rdf:type owl:Class ;
  rdfs:comment "Boxlike nests of drawers enclosed in the front by a flap that drops down to form a writing surface. For flat-top desks on long legs, generally taking the form of a table with one long drawer in the apron, use \"writing tables.\""@en ;
  rdfs:comment "Een stel laden die aan de voorkant worden afgesloten door een blad dat als het wordt neergelaten een schrijfblad vormt. Gebruik 'schrijftafels' voor vlakke bureaus op hoge poten die meestal de vorm van een tafel hebben met een lange la onder het blad."@nl ;
  rdfs:isDefinedBy <https://w3id.org/con-tax/components/aat-furn> ;
  rdfs:label "schrijfbureau"@nl ;
  rdfs:label "schrijfbureaus"@nl ;
  rdfs:label "writing desks"@en ;
  rdfs:seeAlso <http://vocab.getty.edu/aat/300039427> ;
  rdfs:seeAlso wd:Q3512772 ;
  rdfs:subClassOf <https://w3id.org/con-tax/components/aat-furn#300039338> ;
.
<https://w3id.org/con-tax/components/aat-furn#300039436>
  rdf:type owl:Class ;
  rdfs:comment "Flat-top desks on long legs, generally taking the form of a table with one long drawer in the apron. Use \"writing desks\" for similar forms having a superstructure with pigeonholes for writing materials."@en ;
  rdfs:comment "Wordt gebruikt voor vlakke bureaus op lange poten die meestal de vorm aannemen van een tafel met een lange la onder het blad. Gebruik 'schrijfbureaus' voor gelijksoortige stukken die  een opbouw hebben met vakjes voor schrijfbenodigdheden."@nl ;
  rdfs:isDefinedBy <https://w3id.org/con-tax/components/aat-furn> ;
  rdfs:label "schrijftafel"@nl ;
  rdfs:label "schrijftafels"@nl ;
  rdfs:label "writing tables"@en ;
  rdfs:seeAlso <http://vocab.getty.edu/aat/300039436> ;
  rdfs:seeAlso wd:Q8038544 ;
  rdfs:subClassOf <https://w3id.org/con-tax/components/aat-furn#300039338> ;
.
<https://w3id.org/con-tax/components/aat-furn#300039449>
  rdf:type owl:Class ;
  rdfs:comment "'Bureax plats' met een reeks laden of vakjes langs één zijde van het blad."@nl ;
  rdfs:comment "Bureaux plats with a set of drawers or pigeonholes along one side of the top."@en ;
  rdfs:isDefinedBy <https://w3id.org/con-tax/components/aat-furn> ;
  rdfs:label "bureau à gradin"@nl ;
  rdfs:label "bureaux à gradin"@en ;
  rdfs:label "bureaux à gradin"@nl ;
  rdfs:seeAlso <http://vocab.getty.edu/aat/300039449> ;
  rdfs:subClassOf <https://w3id.org/con-tax/components/aat-furn#300039451> ;
.
<https://w3id.org/con-tax/components/aat-furn#300039451>
  rdf:type owl:Class ;
  rdfs:comment "Grote, vlakke schrijftafels die meestal zijn voorzien van laden in het fries."@nl ;
  rdfs:comment "Large flat-top writing tables, usually with drawers in the frieze."@en ;
  rdfs:isDefinedBy <https://w3id.org/con-tax/components/aat-furn> ;
  rdfs:label "bureau plats"@nl ;
  rdfs:label "bureaux plats"@en ;
  rdfs:label "bureaux plats"@nl ;
  rdfs:seeAlso <http://vocab.getty.edu/aat/300039451> ;
  rdfs:subClassOf <https://w3id.org/con-tax/components/aat-furn#300039436> ;
.
<https://w3id.org/con-tax/components/aat-furn#300039452>
  rdf:type owl:Class ;
  rdfs:comment "Schrijftafels met een lage opbouw, bestaande uit twee of drie rijen kleine laden die uit de achterkant oprijzen en rond de zijdes lopen. Waarschijnlijk zijn ze genoemd naar het Prince Regent's Carlton House aan het eind van de 18e eeuw."@nl ;
  rdfs:comment "Writing tables with a low superstructure consisting of two or three tiers of small drawers rising from the back and curving around the sides. Presumably named in the late 18th century after the Prince Regent's Carlton House."@en ;
  rdfs:isDefinedBy <https://w3id.org/con-tax/components/aat-furn> ;
  rdfs:label "Carlton House tables"@en ;
  rdfs:label "Carlton Housetafel"@nl ;
  rdfs:label "Carlton Housetafels"@nl ;
  rdfs:seeAlso <http://vocab.getty.edu/aat/300039452> ;
  rdfs:seeAlso wd:Q5043024 ;
  rdfs:subClassOf <https://w3id.org/con-tax/components/aat-furn#300039436> ;
.
<https://w3id.org/con-tax/components/aat-furn#300039457>
  rdf:type owl:Class ;
  rdfs:comment "Kleine schrijfkasten op tafelhoogte met laden in het onderstuk en een opklapbaar tafelblad met inlegstukken. Dit type werd aan het eind van de 18e eeuw in Engeland uitgevonden door Herbert Croft."@nl ;
  rdfs:comment "Small writing cabinets of table height with drawers in the support and a flap top with drop leaves; of a type invented in late 18th-century England by the Reverend Sir Herbert Croft."@en ;
  rdfs:isDefinedBy <https://w3id.org/con-tax/components/aat-furn> ;
  rdfs:label "croft"@nl ;
  rdfs:label "crofts (writing tables)"@en ;
  rdfs:label "crofts"@nl ;
  rdfs:seeAlso <http://vocab.getty.edu/aat/300039457> ;
  rdfs:subClassOf <https://w3id.org/con-tax/components/aat-furn#300039436> ;
.
<https://w3id.org/con-tax/components/aat-furn#300039458>
  rdf:type owl:Class ;
  rdfs:comment "Compact writing tables fitted with drawers."@en ;
  rdfs:isDefinedBy <https://w3id.org/con-tax/components/aat-furn> ;
  rdfs:label "davenport (bureau)"@nl ;
  rdfs:label "davenport"@nl ;
  rdfs:label "davenports (bureaus)"@nl ;
  rdfs:label "davenports (desks)"@en ;
  rdfs:label "davenports"@nl ;
  rdfs:seeAlso <http://vocab.getty.edu/aat/300039458> ;
  rdfs:subClassOf <https://w3id.org/con-tax/components/aat-furn#300039338> ;
.
<https://w3id.org/con-tax/components/aat-furn#300039460>
  rdf:type owl:Class ;
  rdfs:comment "Desks constructed so that two people may work face-to-face; generally taking the form of a large writing table or desk with drawers on both sides."@en ;
  rdfs:comment "Wordt gebruikt voor bureaus waaraan twee mensen met hun gezicht naar elkaar toe kunnen werken. Ze hebben meestal een grote schrijftafel of bureau met laden aan beide zijden."@nl ;
  rdfs:isDefinedBy <https://w3id.org/con-tax/components/aat-furn> ;
  rdfs:label "partner bureau"@nl ;
  rdfs:label "partner bureaus"@nl ;
  rdfs:label "partners' desks"@en ;
  rdfs:seeAlso <http://vocab.getty.edu/aat/300039460> ;
  rdfs:subClassOf <https://w3id.org/con-tax/components/aat-furn#300039338> ;
.
<https://w3id.org/con-tax/components/aat-furn#300039470>
  rdf:type owl:Class ;
  rdfs:comment "Kleine schrijftafels die voor vrouwen zijn ontworpen."@nl ;
  rdfs:comment "Small writing tables of various forms, designed for women. They may have a relatively delicate form and distinctive features, such as a wide opening to accommodate ladies' skirts when seated."@en ;
  rdfs:isDefinedBy <https://w3id.org/con-tax/components/aat-furn> ;
  rdfs:label "damesschrijftafel"@nl ;
  rdfs:label "damesschrijftafels"@nl ;
  rdfs:label "ladies' secretaries"@nl ;
  rdfs:label "ladies' writing tables"@en ;
  rdfs:seeAlso <http://vocab.getty.edu/aat/300039470> ;
  rdfs:subClassOf <https://w3id.org/con-tax/components/aat-furn#300039436> ;
.
<https://w3id.org/con-tax/components/aat-furn#300039475>
  rdf:type owl:Class ;
  rdfs:comment "Kleine schrijftafels voor vrouwen met een gradine (kast) aan de achterkant. Ze zijn vaak uitvoerig versierd en kunnen als schrijftafel en soms als toilettafel worden gebruikt."@nl ;
  rdfs:comment "Women's small writing tables with a cabinet at the back; often elaborately decorated and occasionally fitted for toilet purposes as well as writing."@en ;
  rdfs:isDefinedBy <https://w3id.org/con-tax/components/aat-furn> ;
  rdfs:label "bonheur-du-jour"@nl ;
  rdfs:label "bonheurs-du-jour"@en ;
  rdfs:label "bonheurs-du-jour"@nl ;
  rdfs:label "damessecretaire"@nl ;
  rdfs:label "damessecretaires"@nl ;
  rdfs:seeAlso <http://vocab.getty.edu/aat/300039475> ;
  rdfs:subClassOf <https://w3id.org/con-tax/components/aat-furn#300039470> ;
.
<https://w3id.org/con-tax/components/aat-furn#300039487>
  rdf:type owl:Class ;
  rdfs:comment "Oblong tables of sturdy construction for use in libraries both public and private, for writing and the inspection of books or other materials."@en ;
  rdfs:isDefinedBy <https://w3id.org/con-tax/components/aat-furn> ;
  rdfs:label "bibliotheektafel"@nl ;
  rdfs:label "bibliotheektafels"@nl ;
  rdfs:label "library tables (writing tables)"@en ;
  rdfs:seeAlso <http://vocab.getty.edu/aat/300039487> ;
  rdfs:subClassOf <https://w3id.org/con-tax/components/aat-furn#300039436> ;
.
<https://w3id.org/con-tax/components/aat-furn#300039490>
  rdf:type owl:Class ;
  rdfs:comment "Small tables designed at such a height to be used for writing while sitting on a sofa."@en ;
  rdfs:isDefinedBy <https://w3id.org/con-tax/components/aat-furn> ;
  rdfs:label "sofa writing tables"@en ;
  rdfs:label "sofaschrijftafel"@nl ;
  rdfs:label "sofaschrijftafels"@nl ;
  rdfs:seeAlso <http://vocab.getty.edu/aat/300039490> ;
  rdfs:subClassOf <https://w3id.org/con-tax/components/aat-furn#300039436> ;
.
<https://w3id.org/con-tax/components/aat-furn#300039495>
  rdf:type owl:Class ;
  rdfs:comment "English desks which are a modification of the cylinder desk, having tambour shutters instead of a curved cylinder. Distinct from the American \"tambour desk,\" which has upright reeded or slatted shutters that cover up the rest of the drawers and pigeonholes."@en ;
  rdfs:comment "Wordt gebruikt voor Engelse bureaus die een variatie op het cilinderbureau zijn, met een tambourdeksel in plaats van een gebogen cilinder. Ze verschillen van het Amerikaanse 'tambourbureau' dat een rechtopstaande deksel van riet of latten heeft waarachter de laden en de vakjes zitten."@nl ;
  rdfs:isDefinedBy <https://w3id.org/con-tax/components/aat-furn> ;
  rdfs:label "tambour writing tables"@en ;
  rdfs:label "tambourschrijftafel"@nl ;
  rdfs:label "tambourschrijftafels"@nl ;
  rdfs:seeAlso <http://vocab.getty.edu/aat/300039495> ;
  rdfs:seeAlso wd:Q7681069 ;
  rdfs:subClassOf <https://w3id.org/con-tax/components/aat-furn#300039338> ;
.
<https://w3id.org/con-tax/components/aat-furn#300039519>
  rdf:type owl:Class ;
  rdfs:comment "Grote Franse bureaus die populair waren aan het eind van de periode van Lodewijk XV en Lodewijk de XVI. Het kwartronde deksel kan over de schrijftafel worden getrokken. Dit type werd soms nagemaakt in andere landen, waaronder Frankrijk, vooral Duitsland en Scandinavië in het laatste decennium van de 18e eeuw en bijna in elk westers land tijdens de 19e en 20e eeuw."@nl ;
  rdfs:comment "Large French desks popular in the late Louis XV and the Louis XVI periods with a roll top in the shape of a quarter cylinder. This type was occasionally imitated in other countries, besides France, particularly in Germany and Scandinavia in the last decade of the 18th century and virtually every western country during the 19th and 20th centuries."@en ;
  rdfs:isDefinedBy <https://w3id.org/con-tax/components/aat-furn> ;
  rdfs:label "bureaux à cylindre"@en ;
  rdfs:label "cilinderbureau"@nl ;
  rdfs:label "cilinderbureaus"@nl ;
  rdfs:label "trommelbureau"@nl ;
  rdfs:label "trommelbureaus"@nl ;
  rdfs:seeAlso <http://vocab.getty.edu/aat/300039519> ;
  rdfs:subClassOf <https://w3id.org/con-tax/components/aat-furn#300146667> ;
.
<https://w3id.org/con-tax/components/aat-furn#300039521>
  rdf:type owl:Class ;
  rdfs:comment "Bureaus met een scharnierende sluiting die omlaag kan worden getrokken om als schrijftafel te dienen."@nl ;
  rdfs:comment "Desks with a hinged cover that may be lowered to form the writing surface or table."@en ;
  rdfs:isDefinedBy <https://w3id.org/con-tax/components/aat-furn> ;
  rdfs:label "fall-front desks"@en ;
  rdfs:label "uitklapbureau"@nl ;
  rdfs:label "uitklapbureaus"@nl ;
  rdfs:seeAlso <http://vocab.getty.edu/aat/300039521> ;
  rdfs:seeAlso wd:Q3477318 ;
  rdfs:subClassOf <https://w3id.org/con-tax/components/aat-furn#300039338> ;
.
<https://w3id.org/con-tax/components/aat-furn#300039526>
  rdf:type owl:Class ;
  rdfs:comment "Fall-front desks having a writing surface that, when closed, folds upward and inward, forming an angle with the carcass."@en ;
  rdfs:comment "Wordt gebruikt voor uitklapbureaus waarvan het schrijfblad sluit door het omhoog en naar binnen te klappen zodat het een hoek met het geraamte maakt."@nl ;
  rdfs:isDefinedBy <https://w3id.org/con-tax/components/aat-furn> ;
  rdfs:label "schrijfcommode"@nl ;
  rdfs:label "schrijfcommodes"@nl ;
  rdfs:label "slant-front desks"@en ;
  rdfs:seeAlso <http://vocab.getty.edu/aat/300039526> ;
  rdfs:subClassOf <https://w3id.org/con-tax/components/aat-furn#300039521> ;
.
<https://w3id.org/con-tax/components/aat-furn#300039545>
  rdf:type owl:Class ;
  rdfs:comment "American desks with upright reeded or slatted shutters that cover up the nest of drawers and pigeonholes. Distinct from English \"tambour writing tables\", which are a modification of the cylinder desk with tambour shutters instead of a curved solid cylinder. Distinct from \"rolltop desks\" which close by means of a flexible shutter of convex shape composed of horizontal slats of wood."@en ;
  rdfs:comment "Wordt gebruikt voor Amerikaanse bureaus met een rechtopstaande deksel van riet of latten die de rij laden en vakjes bedekt. Ze verschillen van de Engelse 'tambourschrijftafels' die een variatie op het cilinderbureau zijn met een tambourdeksel in plaats van een massieve, gebogen cilinder. Ze zijn ook anders dan '@rolltop desks' die worden gesloten met een flexibele, bolvormige deksel die houten, horizontale latten heeft."@nl ;
  rdfs:isDefinedBy <https://w3id.org/con-tax/components/aat-furn> ;
  rdfs:label "tambour desks"@en ;
  rdfs:label "tambourbureau"@nl ;
  rdfs:label "tambourbureaus"@nl ;
  rdfs:seeAlso <http://vocab.getty.edu/aat/300039545> ;
  rdfs:subClassOf <https://w3id.org/con-tax/components/aat-furn#300039338> ;
.
<https://w3id.org/con-tax/components/aat-furn#300039548>
  rdf:type owl:Class ;
  rdfs:comment "Articles of furniture consisting of a flat, slablike top supported on one or more legs or supports."@en ;
  rdfs:comment "Meubelstukken met een vlakke, plaatachtige bovenkant die op één of meer poten of dragers steunt."@nl ;
  rdfs:isDefinedBy <https://w3id.org/con-tax/components/aat-furn> ;
  rdfs:label "tables (support furniture)"@en ;
  rdfs:label "tafel (dragend meubilair)"@nl ;
  rdfs:label "tafel"@nl ;
  rdfs:label "tafels (dragend meubilair)"@nl ;
  rdfs:label "tafels"@nl ;
  rdfs:seeAlso <http://vocab.getty.edu/aat/300039548> ;
  rdfs:subClassOf <https://w3id.org/con-tax/components/aat-furn#300039337> ;
  contax:containsGuideTerm <https://w3id.org/con-tax/components/aat-furn#300039620> ;
  contax:containsGuideTerm <https://w3id.org/con-tax/components/aat-furn#300039928> ;
  contax:containsGuideTerm <https://w3id.org/con-tax/components/aat-furn#300165791> ;
  contax:containsGuideTerm <https://w3id.org/con-tax/components/aat-furn#300165794> ;
.
<https://w3id.org/con-tax/components/aat-furn#300039554>
  rdf:type owl:Class ;
  rdfs:comment "Late 18th- and early 19th-century circular or octagonal pedestal tables which have a deep top with numerous drawers in the frieze. Often the drawers are marked with days of the week or dates, as such tables were used by landlords for filing collected rents."@en ;
  rdfs:comment "Ronde of achthoekige tafels uit het eind van de 18e en het begin van de 19e eeuw, met een voetstuk en een diep tafelblad met talloze laden in het fries. De laden zijn vaak gemerkt met de dagen van de week of met data, omdat ze door pachtheren werden gebruikt om de verzamelde huur in op te bergen."@nl ;
  rdfs:isDefinedBy <https://w3id.org/con-tax/components/aat-furn> ;
  rdfs:label "huurtafel"@nl ;
  rdfs:label "huurtafels"@nl ;
  rdfs:label "rent tables (pedestal tables)"@en ;
  rdfs:seeAlso <http://vocab.getty.edu/aat/300039554> ;
  rdfs:subClassOf <https://w3id.org/con-tax/components/aat-furn#300039548> ;
.
<https://w3id.org/con-tax/components/aat-furn#300039574>
  rdf:type owl:Class ;
  rdfs:comment "Benaming voor Franse tafels met een diepe rand of strook rondom het tafelblad."@nl ;
  rdfs:comment "Term for French tables with a deep rim or gallery around the top."@en ;
  rdfs:isDefinedBy <https://w3id.org/con-tax/components/aat-furn> ;
  rdfs:label "table en crachoir"@nl ;
  rdfs:label "tables en crachoir"@en ;
  rdfs:label "tables en crachoir"@nl ;
  rdfs:seeAlso <http://vocab.getty.edu/aat/300039574> ;
  rdfs:subClassOf <https://w3id.org/con-tax/components/aat-furn#300039548> ;
.
<https://w3id.org/con-tax/components/aat-furn#300039578>
  rdf:type gvp:GuideTerm ;
  rdfs:isDefinedBy <https://w3id.org/con-tax/components/aat-furn> ;
  rdfs:label "<tables by form: base form>"@en ;
  rdfs:label "<tafel naar vorm: basisvorm>"@nl ;
  rdfs:label "<tafels naar vorm: basisvorm>"@nl ;
  rdfs:label "tafel naar vorm: basisvorm"@nl ;
  rdfs:label "tafels naar vorm: basisvorm"@nl ;
  rdfs:seeAlso <http://vocab.getty.edu/aat/300039578> ;
  contax:containsConcept <https://w3id.org/con-tax/components/aat-furn#300039580> ;
  contax:containsConcept <https://w3id.org/con-tax/components/aat-furn#300039587> ;
  contax:containsConcept <https://w3id.org/con-tax/components/aat-furn#300039596> ;
  contax:containsConcept <https://w3id.org/con-tax/components/aat-furn#300039602> ;
  contax:containsConcept <https://w3id.org/con-tax/components/aat-furn#300039612> ;
  contax:containsConcept <https://w3id.org/con-tax/components/aat-furn#300039619> ;
  contax:containsConcept <https://w3id.org/con-tax/components/aat-furn#300164519> ;
.
<https://w3id.org/con-tax/components/aat-furn#300039580>
  rdf:type owl:Class ;
  rdfs:comment "Tables supported by a fixed bracket (console) against a wall, or supported by a substructure consisting of two or more legs of console form. The term may be used for similar tables having other forms of supporting legs. May have marble tops and heavily carved substructures."@en ;
  rdfs:comment "Zijtafels waarvan het blad wordt gesteund door een samenstel van twee of meer poten in consolevorm; ze hebben soms een marmeren tafelblad en zwaar bewerkte draagconstructies."@nl ;
  rdfs:isDefinedBy <https://w3id.org/con-tax/components/aat-furn> ;
  rdfs:label "console tables"@en ;
  rdfs:label "consoletafel"@nl ;
  rdfs:label "consoletafels"@nl ;
  rdfs:seeAlso <http://vocab.getty.edu/aat/300039580> ;
  rdfs:subClassOf <https://w3id.org/con-tax/components/aat-furn#300039548> ;
  rdfs:subClassOf <https://w3id.org/con-tax/components/aat-furn#300039999> ;
.
<https://w3id.org/con-tax/components/aat-furn#300039583>
  rdf:type owl:Class ;
  rdfs:comment "Console tables supported by an eagle bracket."@en ;
  rdfs:comment "Consoletafels die door een adelaarsconsole worden ondersteund."@nl ;
  rdfs:isDefinedBy <https://w3id.org/con-tax/components/aat-furn> ;
  rdfs:label "adelaarsconsoletafel"@nl ;
  rdfs:label "adelaarsconsoletafels"@nl ;
  rdfs:label "eagle console tables"@en ;
  rdfs:seeAlso <http://vocab.getty.edu/aat/300039583> ;
  rdfs:subClassOf <https://w3id.org/con-tax/components/aat-furn#300039580> ;
.
<https://w3id.org/con-tax/components/aat-furn#300039584>
  rdf:type owl:Class ;
  rdfs:comment "Tables whose flaps are supported by jointed gates which swing out from the central section."@en ;
  rdfs:comment "Tafels waarvan de bladen worden ondersteund door gelede poten, die vanuit het middengedeelte uitklappen."@nl ;
  rdfs:isDefinedBy <https://w3id.org/con-tax/components/aat-furn> ;
  rdfs:label "gate leg tafels"@nl ;
  rdfs:label "gate-leg tables"@en ;
  rdfs:label "gate-leg tafel"@nl ;
  rdfs:label "gate-leg tafels"@nl ;
  rdfs:seeAlso <http://vocab.getty.edu/aat/300039584> ;
  rdfs:subClassOf <https://w3id.org/con-tax/components/aat-furn#300039933> ;
.
<https://w3id.org/con-tax/components/aat-furn#300039587>
  rdf:type owl:Class ;
  rdfs:comment "Tables with a single columnar support."@en ;
  rdfs:comment "Tafels met een enkele stijl als steun."@nl ;
  rdfs:isDefinedBy <https://w3id.org/con-tax/components/aat-furn> ;
  rdfs:label "kolomtafel"@nl ;
  rdfs:label "kolomtafels"@nl ;
  rdfs:label "pedestal tables"@en ;
  rdfs:seeAlso <http://vocab.getty.edu/aat/300039587> ;
  rdfs:subClassOf <https://w3id.org/con-tax/components/aat-furn#300039548> ;
.
<https://w3id.org/con-tax/components/aat-furn#300039591>
  rdf:type owl:Class ;
  rdfs:comment "Grote ovale of ronde kaarttafels met een middensteun en een schuingeplaatst blad."@nl ;
  rdfs:comment "Large oval or circular card tables with a central support and tilt top."@en ;
  rdfs:isDefinedBy <https://w3id.org/con-tax/components/aat-furn> ;
  rdfs:label "loo tables"@en ;
  rdfs:label "loo tafel"@nl ;
  rdfs:label "loo tafels"@nl ;
  rdfs:seeAlso <http://vocab.getty.edu/aat/300039591> ;
  rdfs:seeAlso wd:Q16931203 ;
  rdfs:subClassOf <https://w3id.org/con-tax/components/aat-furn#300039702> ;
.
<https://w3id.org/con-tax/components/aat-furn#300039596>
  rdf:type owl:Class ;
  rdfs:comment "Benaming die van toepassing is op tafels met poten die uit een pilaar steken, ongeacht hun vorm,  en waarvan de voeten in klauwen uitlopen."@nl ;
  rdfs:comment "Term applied to tables with legs jutting from a pillar, regardless of their form, and with feet terminating into claws."@en ;
  rdfs:isDefinedBy <https://w3id.org/con-tax/components/aat-furn> ;
  rdfs:label "pilaar en voeklauwtafel"@nl ;
  rdfs:label "pilaar en voeklauwtafels"@nl ;
  rdfs:label "pillar and claw tables"@en ;
  rdfs:seeAlso <http://vocab.getty.edu/aat/300039596> ;
  rdfs:subClassOf <https://w3id.org/con-tax/components/aat-furn#300039548> ;
.
<https://w3id.org/con-tax/components/aat-furn#300039602>
  rdf:type owl:Class ;
  rdfs:comment "A variant form of trestle table with an X-shaped trestle at either end."@en ;
  rdfs:comment "Een variant op de 'schraagtafels' met een X-vormig onderstel aan beide uiteinden."@nl ;
  rdfs:isDefinedBy <https://w3id.org/con-tax/components/aat-furn> ;
  rdfs:label "sawbuck tables"@en ;
  rdfs:label "zaagtafel"@nl ;
  rdfs:label "zaagtafels"@nl ;
  rdfs:seeAlso <http://vocab.getty.edu/aat/300039602> ;
  rdfs:subClassOf <https://w3id.org/con-tax/components/aat-furn#300039548> ;
  rdfs:subClassOf <https://w3id.org/con-tax/components/aat-furn#300039612> ;
.
<https://w3id.org/con-tax/components/aat-furn#300039605>
  rdf:type owl:Class ;
  rdfs:comment "Joined tables with three legs; of a type made in 17th-century England."@en ;
  rdfs:comment "Schrijnwerk tafels met drie poten die in de 17e eeuw in Engeland werden gemaakt."@nl ;
  rdfs:isDefinedBy <https://w3id.org/con-tax/components/aat-furn> ;
  rdfs:label "cricket tables"@en ;
  rdfs:label "crickettafel"@nl ;
  rdfs:label "crickettafels"@nl ;
  rdfs:seeAlso <http://vocab.getty.edu/aat/300039605> ;
  rdfs:subClassOf <https://w3id.org/con-tax/components/aat-furn#300039548> ;
.
<https://w3id.org/con-tax/components/aat-furn#300039612>
  rdf:type owl:Class ;
  rdfs:comment "Tables with a removable board top resting on two or three trestle supports connected by a longitudinal bar instead of legs. For tables with X-shaped trestle supports, use \"sawbuck tables.\""@en ;
  rdfs:comment "Wordt gebruikt voor tafels met een afneembaar tafelblad dat niet op poten maar op twee of drie schragen steunt, die met een overlangse balk zijn verbonden. Gebruik 'zaagtafels' voor tafels met X-vormige schragen als onderstel."@nl ;
  rdfs:isDefinedBy <https://w3id.org/con-tax/components/aat-furn> ;
  rdfs:label "schraagtafel"@nl ;
  rdfs:label "schraagtafels"@nl ;
  rdfs:label "trestle tables"@en ;
  rdfs:seeAlso <http://vocab.getty.edu/aat/300039612> ;
  rdfs:seeAlso wd:Q7838852 ;
  rdfs:subClassOf <https://w3id.org/con-tax/components/aat-furn#300039548> ;
.
<https://w3id.org/con-tax/components/aat-furn#300039619>
  rdf:type owl:Class ;
  rdfs:comment "Tables with a pedestal base supported by three legs."@en ;
  rdfs:comment "Tafels met een voetstuk dat door drie poten wordt ondersteund."@nl ;
  rdfs:isDefinedBy <https://w3id.org/con-tax/components/aat-furn> ;
  rdfs:label "driepoottafel"@nl ;
  rdfs:label "driepoottafels"@nl ;
  rdfs:label "tripod tables"@en ;
  rdfs:seeAlso <http://vocab.getty.edu/aat/300039619> ;
  rdfs:subClassOf <https://w3id.org/con-tax/components/aat-furn#300039548> ;
.
<https://w3id.org/con-tax/components/aat-furn#300039620>
  rdf:type gvp:GuideTerm ;
  rdfs:isDefinedBy <https://w3id.org/con-tax/components/aat-furn> ;
  rdfs:label "<tables by function>"@en ;
  rdfs:label "<tafel naar functie>"@nl ;
  rdfs:label "<tafels naar functie>"@nl ;
  rdfs:label "tafel naar functie"@nl ;
  rdfs:label "tafels naar functie"@nl ;
  rdfs:seeAlso <http://vocab.getty.edu/aat/300039620> ;
  contax:containsConcept <https://w3id.org/con-tax/components/aat-furn#300038148> ;
  contax:containsConcept <https://w3id.org/con-tax/components/aat-furn#300039554> ;
  contax:containsConcept <https://w3id.org/con-tax/components/aat-furn#300039627> ;
  contax:containsConcept <https://w3id.org/con-tax/components/aat-furn#300039633> ;
  contax:containsConcept <https://w3id.org/con-tax/components/aat-furn#300039640> ;
  contax:containsConcept <https://w3id.org/con-tax/components/aat-furn#300039646> ;
  contax:containsConcept <https://w3id.org/con-tax/components/aat-furn#300039648> ;
  contax:containsConcept <https://w3id.org/con-tax/components/aat-furn#300039667> ;
  contax:containsConcept <https://w3id.org/con-tax/components/aat-furn#300039668> ;
  contax:containsConcept <https://w3id.org/con-tax/components/aat-furn#300039694> ;
  contax:containsConcept <https://w3id.org/con-tax/components/aat-furn#300039702> ;
  contax:containsConcept <https://w3id.org/con-tax/components/aat-furn#300039734> ;
  contax:containsConcept <https://w3id.org/con-tax/components/aat-furn#300039741> ;
  contax:containsConcept <https://w3id.org/con-tax/components/aat-furn#300039745> ;
  contax:containsConcept <https://w3id.org/con-tax/components/aat-furn#300039755> ;
  contax:containsConcept <https://w3id.org/con-tax/components/aat-furn#300039756> ;
  contax:containsConcept <https://w3id.org/con-tax/components/aat-furn#300039886> ;
  contax:containsConcept <https://w3id.org/con-tax/components/aat-furn#300039894> ;
  contax:containsConcept <https://w3id.org/con-tax/components/aat-furn#300039896> ;
  contax:containsConcept <https://w3id.org/con-tax/components/aat-furn#300039897> ;
  contax:containsConcept <https://w3id.org/con-tax/components/aat-furn#300039900> ;
  contax:containsConcept <https://w3id.org/con-tax/components/aat-furn#300135321> ;
  contax:containsConcept <https://w3id.org/con-tax/components/aat-furn#300141687> ;
  contax:containsConcept <https://w3id.org/con-tax/components/aat-furn#300161823> ;
  contax:containsConcept <https://w3id.org/con-tax/components/aat-furn#300164317> ;
  contax:containsConcept <https://w3id.org/con-tax/components/aat-furn#300164406> ;
  contax:containsConcept <https://w3id.org/con-tax/components/aat-furn#300164547> ;
  contax:containsConcept <https://w3id.org/con-tax/components/aat-furn#300164593> ;
  contax:containsConcept <https://w3id.org/con-tax/components/aat-furn#300170858> ;
  contax:containsConcept <https://w3id.org/con-tax/components/aat-furn#300170905> ;
  contax:containsConcept <https://w3id.org/con-tax/components/aat-furn#300250397> ;
  contax:containsConcept <https://w3id.org/con-tax/components/aat-furn#300251534> ;
  contax:containsConcept <https://w3id.org/con-tax/components/aat-furn#300265762> ;
  contax:containsConcept <https://w3id.org/con-tax/components/aat-furn#300311855> ;
  contax:containsConcept <https://w3id.org/con-tax/components/aat-furn#300375208> ;
  contax:containsConcept <https://w3id.org/con-tax/components/aat-furn#300375689> ;
  contax:containsConcept <https://w3id.org/con-tax/components/aat-furn#300391111> ;
  contax:containsConcept <https://w3id.org/con-tax/components/aat-furn#300391286> ;
  contax:containsConcept <https://w3id.org/con-tax/components/aat-furn#300400635> ;
  contax:containsConcept <https://w3id.org/con-tax/components/aat-furn#300403907> ;
  contax:containsConcept <https://w3id.org/con-tax/components/aat-furn#300404365> ;
  contax:containsConcept <https://w3id.org/con-tax/components/aat-furn#300419378> ;
  contax:containsConcept <https://w3id.org/con-tax/components/aat-furn#300421866> ;
  contax:containsConcept <https://w3id.org/con-tax/components/aat-furn#300438650> ;
  contax:containsConcept <https://w3id.org/con-tax/components/aat-furn#300438693> ;
  contax:containsConcept <https://w3id.org/con-tax/components/aat-furn#300438694> ;
.
<https://w3id.org/con-tax/components/aat-furn#300039627>
  rdf:type owl:Class ;
  rdfs:comment "Tables with a slate surface covered with cloth and surrounded by cushioned rails, on which the game of billiards is played. Distinct from \"pool tables\" which are similar in form but have six pockets."@en ;
  rdfs:comment "Tafels waarop het biljartspel wordt gespeeld en waarvan het oppervlak bestaat uit met stof beklede leistenen platen, omringd door een stootrand. Te onderscheiden van 'pooltafels' die qua vorm hetzelfde zijn maar zes zakken hebben."@nl ;
  rdfs:isDefinedBy <https://w3id.org/con-tax/components/aat-furn> ;
  rdfs:label "biljarttafel"@nl ;
  rdfs:label "biljarttafels"@nl ;
  rdfs:label "billiard tables"@en ;
  rdfs:seeAlso <http://vocab.getty.edu/aat/300039627> ;
  rdfs:seeAlso wd:Q3500725 ;
  rdfs:subClassOf <https://w3id.org/con-tax/components/aat-furn#300039548> ;
.
<https://w3id.org/con-tax/components/aat-furn#300039633>
  rdf:type owl:Class ;
  rdfs:comment "Middelmatig grote tafels zonder de verhoogde rand van een theetafel en kleiner dan een eettafel. Ze hebben een opklapbaar tafelblad, soms met één of twee kleine laatjes in het onderstel."@nl ;
  rdfs:comment "Moderate-sized tables lacking the raised edge of a tea table or the scale of a dining table and having drop leaves and sometimes a small drawer or two in the apron."@en ;
  rdfs:isDefinedBy <https://w3id.org/con-tax/components/aat-furn> ;
  rdfs:label "breakfast tables"@en ;
  rdfs:label "ontbijttafel"@nl ;
  rdfs:label "ontbijttafels"@nl ;
  rdfs:seeAlso <http://vocab.getty.edu/aat/300039633> ;
  rdfs:subClassOf <https://w3id.org/con-tax/components/aat-furn#300039548> ;
.
<https://w3id.org/con-tax/components/aat-furn#300039640>
  rdf:type owl:Class ;
  rdfs:comment "Occasional tables, often placed in front of a sofa in a living room. A coffee table is relatively low, of a convenient height for access while seated at the sofa. It is used for serving coffee, tea, cocktails, displaying large books or magazines, or various other purposes."@en ;
  rdfs:isDefinedBy <https://w3id.org/con-tax/components/aat-furn> ;
  rdfs:label "coffee tables"@en ;
  rdfs:label "koffietafel"@nl ;
  rdfs:label "koffietafels"@nl ;
  rdfs:seeAlso <http://vocab.getty.edu/aat/300039640> ;
  rdfs:subClassOf <https://w3id.org/con-tax/components/aat-furn#300039548> ;
  rdfs:subClassOf <https://w3id.org/con-tax/components/aat-furn#300039752> ;
.
<https://w3id.org/con-tax/components/aat-furn#300039646>
  rdf:type owl:Class ;
  rdfs:comment "Tables used for the distribution of communion during the Eucharist in Christian churches."@en ;
  rdfs:isDefinedBy <https://w3id.org/con-tax/components/aat-furn> ;
  rdfs:label "avondmaalstafel"@nl ;
  rdfs:label "avondmaalstafels"@nl ;
  rdfs:label "communion tables"@en ;
  rdfs:seeAlso <http://vocab.getty.edu/aat/300039646> ;
  rdfs:seeAlso wd:Q318958 ;
  rdfs:subClassOf <https://w3id.org/con-tax/components/aat-furn#300039548> ;
.
<https://w3id.org/con-tax/components/aat-furn#300039648>
  rdf:type owl:Class ;
  rdfs:comment "Tables designed for and used while eating meals in a dining room. Distinguished from kitchen tables, which are intended for less formal meals in a kitchen."@en ;
  rdfs:isDefinedBy <https://w3id.org/con-tax/components/aat-furn> ;
  rdfs:label "dinertafel"@nl ;
  rdfs:label "dinertafels"@nl ;
  rdfs:label "dining tables"@en ;
  rdfs:label "eettafel"@nl ;
  rdfs:label "eettafels"@nl ;
  rdfs:seeAlso <http://vocab.getty.edu/aat/300039648> ;
  rdfs:seeAlso wd:Q10578291 ;
  rdfs:subClassOf <https://w3id.org/con-tax/components/aat-furn#300039548> ;
.
<https://w3id.org/con-tax/components/aat-furn#300039653>
  rdf:type owl:Class ;
  rdfs:comment "Dining tables with extending frames whose tops can be lengthened by inserting loose leaves."@en ;
  rdfs:comment "Dining tables with extending frames whose tops can be lengthened by inserting loose leaves."@nl ;
  rdfs:isDefinedBy <https://w3id.org/con-tax/components/aat-furn> ;
  rdfs:label "extension dining tables"@en ;
  rdfs:label "uitschuifbare eettafel"@nl ;
  rdfs:label "uitschuifbare eettafels"@nl ;
  rdfs:label "uittrektafels"@nl ;
  rdfs:seeAlso <http://vocab.getty.edu/aat/300039653> ;
  rdfs:subClassOf <https://w3id.org/con-tax/components/aat-furn#300039648> ;
.
<https://w3id.org/con-tax/components/aat-furn#300039659>
  rdf:type owl:Class ;
  rdfs:comment "Extension dining tables invented during the Victorian period, which received their name from the slide action by which their length is varied."@en ;
  rdfs:comment "Uitschuifbare eettafels die in de Victoriaanse periode werden uitgevonden. De naam verwijst naar de manier van uitschuiven."@nl ;
  rdfs:isDefinedBy <https://w3id.org/con-tax/components/aat-furn> ;
  rdfs:label "telescooptafel"@nl ;
  rdfs:label "telescooptafels"@nl ;
  rdfs:label "telescope tables"@en ;
  rdfs:seeAlso <http://vocab.getty.edu/aat/300039659> ;
  rdfs:subClassOf <https://w3id.org/con-tax/components/aat-furn#300039653> ;
.
<https://w3id.org/con-tax/components/aat-furn#300039661>
  rdf:type owl:Class ;
  rdfs:comment "Tables common in the American Federal period that consist of two semicircular end parts and a rectangular middle section. The middle section often incorporates drop leaves that serve to extend the length of the table."@en ;
  rdfs:isDefinedBy <https://w3id.org/con-tax/components/aat-furn> ;
  rdfs:label "driedelige dinertafel"@nl ;
  rdfs:label "driedelige dinertafels"@nl ;
  rdfs:label "three-part dining tables"@en ;
  rdfs:seeAlso <http://vocab.getty.edu/aat/300039661> ;
  rdfs:subClassOf <https://w3id.org/con-tax/components/aat-furn#300039648> ;
.
<https://w3id.org/con-tax/components/aat-furn#300039667>
  rdf:type owl:Class ;
  rdfs:comment "Tables with surfaces adjustable for elevation and angles of incline."@en ;
  rdfs:comment "Tafels met een oppervlak dat op verschillende hoogten en onder verschillende hoeken kan worden ingesteld."@nl ;
  rdfs:isDefinedBy <https://w3id.org/con-tax/components/aat-furn> ;
  rdfs:label "drawing tables (artists' tables)"@en ;
  rdfs:label "tekentafel"@nl ;
  rdfs:label "tekentafels"@nl ;
  rdfs:seeAlso <http://vocab.getty.edu/aat/300039667> ;
  rdfs:subClassOf <https://w3id.org/con-tax/components/aat-furn#300039548> ;
.
<https://w3id.org/con-tax/components/aat-furn#300039668>
  rdf:type owl:Class ;
  rdfs:comment "Benaming die van toepassing is op verschillende tafels waaraan toilet kan worden gemaakt, meestal met een spiegel en laden waarin toiletartikelen liggen zoals borstels en kammen."@nl ;
  rdfs:comment "Generally applied to a variety of tables used for dressing and conducting one's toilet; they may be fitted with a mirror and drawers to hold toilet articles such as brushes and combs."@en ;
  rdfs:isDefinedBy <https://w3id.org/con-tax/components/aat-furn> ;
  rdfs:label "dressing tables"@en ;
  rdfs:label "kaptafel"@nl ;
  rdfs:label "kaptafels"@nl ;
  rdfs:label "toilettafel"@nl ;
  rdfs:label "toilettafels"@nl ;
  rdfs:seeAlso <http://vocab.getty.edu/aat/300039668> ;
  rdfs:subClassOf <https://w3id.org/con-tax/components/aat-furn#300039548> ;
.
<https://w3id.org/con-tax/components/aat-furn#300039670>
  rdf:type owl:Class ;
  rdfs:comment "Engelse en Amerikaanse tafels die in de 18e eeuw werden gemaakt om de faciliteiten van een moderne badkamer te bieden, met voorzieningen voor een waskom, kannen, bidet en andere toiletbenodigdheden."@nl ;
  rdfs:comment "English and American 18th-century tables made to provide the facilities of the modern bathroom, with provisions for a basin, bottles, bidet, and other toilet equipment."@en ;
  rdfs:isDefinedBy <https://w3id.org/con-tax/components/aat-furn> ;
  rdfs:label "gentlemen's dressing tables"@en ;
  rdfs:label "herenkaptafel"@nl ;
  rdfs:label "herenkaptafels"@nl ;
  rdfs:seeAlso <http://vocab.getty.edu/aat/300039670> ;
  rdfs:subClassOf <https://w3id.org/con-tax/components/aat-furn#300039668> ;
.
<https://w3id.org/con-tax/components/aat-furn#300039672>
  rdf:type owl:Class ;
  rdfs:comment "Heren- of dameskapdozen op een hoog onderstel, met een deksel waaronder een compleet ingerichte binnenkant zit,  meestal met laden eronder. Ze verschillen van andere kaptafels omdat ze op hogere poten staan en geen volledige ladenkast onder hebben."@nl ;
  rdfs:comment "Men's or ladies' dressing boxes on a tall stand with a lid that opens to reveal a fitted interior, usually with drawers beneath. Unlike other dressing tables, it has taller legs and lacks a full case of drawers beneath."@en ;
  rdfs:isDefinedBy <https://w3id.org/con-tax/components/aat-furn> ;
  rdfs:label "Beau-Brummel dressing tables"@en ;
  rdfs:label "Beau-Brummelkaptafel"@nl ;
  rdfs:label "Beau-Brummelkaptafels"@nl ;
  rdfs:seeAlso <http://vocab.getty.edu/aat/300039672> ;
  rdfs:subClassOf <https://w3id.org/con-tax/components/aat-furn#300039670> ;
.
<https://w3id.org/con-tax/components/aat-furn#300039674>
  rdf:type owl:Class ;
  rdfs:comment "Benaming die meestal wordt gebruikt voor verschillende soorten kaptafels met een spiegel en lades voor toiletartikelen. Gebruik 'Rudd-tafels' voor dameskaptafels waarbij de laden aan de zijkant uitklappen met een driedelige toiletspiegel erop. Gebruik 'toilettafels' voor Franse kaptafels die voor vrouwen zijn ontworpen."@nl ;
  rdfs:comment "Term generally applied to a variety of dressing tables which are fitted with a mirror and have drawers to hold toilet articles. For ladies' dressing tables having drawers on the side which swing out and provide mirrors on a quadrant, use \"Rudd tables.\" Use \"toilettes\" with reference to French dressing tables designed for women."@en ;
  rdfs:isDefinedBy <https://w3id.org/con-tax/components/aat-furn> ;
  rdfs:label "dameskaptafel"@nl ;
  rdfs:label "dameskaptafels"@nl ;
  rdfs:label "ladies' dressing tables"@en ;
  rdfs:seeAlso <http://vocab.getty.edu/aat/300039674> ;
  rdfs:subClassOf <https://w3id.org/con-tax/components/aat-furn#300039668> ;
.
<https://w3id.org/con-tax/components/aat-furn#300039677>
  rdf:type owl:Class ;
  rdfs:comment "Benaming die van toepassing is op verschillende Franse kaptafels die voor vrouwen zijn ontworpen."@nl ;
  rdfs:comment "Term applied to a variety of French dressing tables designed for women."@en ;
  rdfs:isDefinedBy <https://w3id.org/con-tax/components/aat-furn> ;
  rdfs:label "poudreuse"@nl ;
  rdfs:label "poudreuses"@nl ;
  rdfs:label "spiegeltafel"@nl ;
  rdfs:label "spiegeltafels"@nl ;
  rdfs:label "toilette"@nl ;
  rdfs:label "toilettes (dressing tables)"@en ;
  rdfs:label "toilettes"@nl ;
  rdfs:seeAlso <http://vocab.getty.edu/aat/300039677> ;
  rdfs:subClassOf <https://w3id.org/con-tax/components/aat-furn#300039674> ;
.
<https://w3id.org/con-tax/components/aat-furn#300039685>
  rdf:type owl:Class ;
  rdfs:comment "Hartvormige kaptafels met laden die aan beide zijden uitspringen zodat het geheel enigszins op de vleugels van een vlinder lijkt."@nl ;
  rdfs:comment "Heart-shaped dressing tables with drawers springing out at each side somewhat like butterfly wings."@en ;
  rdfs:isDefinedBy <https://w3id.org/con-tax/components/aat-furn> ;
  rdfs:label "toilet en papillon"@nl ;
  rdfs:label "toilettes en papillon"@en ;
  rdfs:label "toilettes en papillon"@nl ;
  rdfs:seeAlso <http://vocab.getty.edu/aat/300039685> ;
  rdfs:subClassOf <https://w3id.org/con-tax/components/aat-furn#300039677> ;
.
<https://w3id.org/con-tax/components/aat-furn#300039694>
  rdf:type owl:Class ;
  rdfs:comment "Tables of various designs at which cards, dice, and other games are played. They may have tops marked as a game board for playing chess, backgammon, goobun, or other games; they may have tops edged with a railing. Distinct from \"card tables\" which have a smooth, undecorated top."@en ;
  rdfs:comment "Wordt gebruikt voor tafels waarbij op het blad speelborden voor schaken, backgammon of andere spelletjes zijn aangebracht. Te onderscheiden van 'kaarttafels' die een glad, onversierd blad hebben."@nl ;
  rdfs:isDefinedBy <https://w3id.org/con-tax/components/aat-furn> ;
  rdfs:label "gaming tables"@en ;
  rdfs:label "speeltafel"@nl ;
  rdfs:label "speeltafels"@nl ;
  rdfs:seeAlso <http://vocab.getty.edu/aat/300039694> ;
  rdfs:subClassOf <https://w3id.org/con-tax/components/aat-furn#300039548> ;
.
<https://w3id.org/con-tax/components/aat-furn#300039699>
  rdf:type owl:Class ;
  rdfs:comment "Gaming tables with tops marked as boards for playing backgammon. They may be similar to French \"tric-trac tables,\" because the games are similar. Tric-trac was popular in France and elsewhere from 16th through 19th centuries. Both games could be played on either table. Backgammon tables tend to be of more recent origin."@en ;
  rdfs:comment "Speeltafels waarbij op het blad een speelbord voor backgammon is aangebracht."@nl ;
  rdfs:isDefinedBy <https://w3id.org/con-tax/components/aat-furn> ;
  rdfs:label "backgammon tables"@en ;
  rdfs:label "backgammontafel"@nl ;
  rdfs:label "backgammontafels"@nl ;
  rdfs:seeAlso <http://vocab.getty.edu/aat/300039699> ;
  rdfs:subClassOf <https://w3id.org/con-tax/components/aat-furn#300039694> ;
.
<https://w3id.org/con-tax/components/aat-furn#300039700>
  rdf:type owl:Class ;
  rdfs:comment "Tables designed for a game similar to billiards called bagatelle. These tables have a semicircular area at one end in which there are nine numbered holes or cups, each number signifying the points to be scored by pocketing a ball. The table width is usually one-third of its length."@en ;
  rdfs:isDefinedBy <https://w3id.org/con-tax/components/aat-furn> ;
  rdfs:label "bagatelle tables"@en ;
  rdfs:label "bagatelletafel"@nl ;
  rdfs:label "bagatelletafels"@nl ;
  rdfs:seeAlso <http://vocab.getty.edu/aat/300039700> ;
  rdfs:subClassOf <https://w3id.org/con-tax/components/aat-furn#300039627> ;
.
<https://w3id.org/con-tax/components/aat-furn#300039702>
  rdf:type owl:Class ;
  rdfs:comment "Tables with a smooth top, generally intended to be used for playing cards; often having a folding top, may have inset pockets to hold coins or counters. Distinguished from \"gaming tables\" which may have tops marked as game boards for playing chess, backgammon, or other games."@en ;
  rdfs:comment "Tafels met een glad, onversierd blad die meestal worden gebruikt om kaart op te spelen. Ze hebben veelal een inklapbaar blad en kunnen ingezette zakken hebben waarin munten of fiches kunnen worden opgeborgen. Te onderscheiden van 'speeltafels' waarbij op de tafelbladen speelborden voor schaken, backgammon of andere spelletjes zijn aangebracht."@nl ;
  rdfs:isDefinedBy <https://w3id.org/con-tax/components/aat-furn> ;
  rdfs:label "card tables"@en ;
  rdfs:label "kaarttafel"@nl ;
  rdfs:label "kaarttafels"@nl ;
  rdfs:seeAlso <http://vocab.getty.edu/aat/300039702> ;
  rdfs:subClassOf <https://w3id.org/con-tax/components/aat-furn#300039548> ;
.
<https://w3id.org/con-tax/components/aat-furn#300039705>
  rdf:type owl:Class ;
  rdfs:comment "Kleine kaarttafels om basset op te spelen, een kaartspel dat populair was in Italië en Frankrijk aan het eind van de 17e eeuw en in Engeland in het begin van de 18e eeuw."@nl ;
  rdfs:comment "Small card tables for playing bassette, a card game popular in Italy and France in the late 17th century and in England in the early 18th century."@en ;
  rdfs:isDefinedBy <https://w3id.org/con-tax/components/aat-furn> ;
  rdfs:label "basset table"@nl ;
  rdfs:label "basset tables"@en ;
  rdfs:label "basset tables"@nl ;
  rdfs:seeAlso <http://vocab.getty.edu/aat/300039705> ;
  rdfs:subClassOf <https://w3id.org/con-tax/components/aat-furn#300039702> ;
.
<https://w3id.org/con-tax/components/aat-furn#300039714>
  rdf:type owl:Class ;
  rdfs:comment "Tables with round, octagonal, or sometimes rectangular tops supported on columns ending in three flared legs. The tops often include a mechanism that allows it to tilt down for storage."@en ;
  rdfs:isDefinedBy <https://w3id.org/con-tax/components/aat-furn> ;
  rdfs:label "driepotige kaarttafel"@nl ;
  rdfs:label "driepotige kaarttafels"@nl ;
  rdfs:label "tripod card tables"@en ;
  rdfs:seeAlso <http://vocab.getty.edu/aat/300039714> ;
  rdfs:subClassOf <https://w3id.org/con-tax/components/aat-furn#300039702> ;
.
<https://w3id.org/con-tax/components/aat-furn#300039715>
  rdf:type owl:Class ;
  rdfs:comment "Tables with tops marked with a gameboard divided into 64 squares of two alternating colors, for playing chess."@en ;
  rdfs:comment "Tafels waarbij op het blad een speelbord voor schaken of dammen is aangebracht."@nl ;
  rdfs:isDefinedBy <https://w3id.org/con-tax/components/aat-furn> ;
  rdfs:label "chess tables"@en ;
  rdfs:label "damtafel"@nl ;
  rdfs:label "damtafels"@nl ;
  rdfs:label "schaaktafel"@nl ;
  rdfs:label "schaaktafels"@nl ;
  rdfs:seeAlso <http://vocab.getty.edu/aat/300039715> ;
  rdfs:seeAlso wd:Q1321488 ;
  rdfs:subClassOf <https://w3id.org/con-tax/components/aat-furn#300039694> ;
.
<https://w3id.org/con-tax/components/aat-furn#300039717>
  rdf:type owl:Class ;
  rdfs:comment "Kleine, driekantige tafels met kuiltjes in het tafelblad om fiches in op te bergen."@nl ;
  rdfs:comment "Small, three-sided tables, with pits in the top to hold counters."@en ;
  rdfs:isDefinedBy <https://w3id.org/con-tax/components/aat-furn> ;
  rdfs:label "ombre tables"@en ;
  rdfs:label "ombre-tafel"@nl ;
  rdfs:label "ombre-tafels"@nl ;
  rdfs:seeAlso <http://vocab.getty.edu/aat/300039717> ;
  rdfs:subClassOf <https://w3id.org/con-tax/components/aat-furn#300039702> ;
.
<https://w3id.org/con-tax/components/aat-furn#300039718>
  rdf:type owl:Class ;
  rdfs:comment "Circular card tables with a depression in the center for the cards and for a candlestick."@en ;
  rdfs:comment "Ronde kaarttafels met een uitholling in het midden voor de kaarten en een kaars."@nl ;
  rdfs:isDefinedBy <https://w3id.org/con-tax/components/aat-furn> ;
  rdfs:label "table de brelan"@nl ;
  rdfs:label "tables de brelan"@en ;
  rdfs:label "tables de brelan"@nl ;
  rdfs:seeAlso <http://vocab.getty.edu/aat/300039718> ;
  rdfs:subClassOf <https://w3id.org/con-tax/components/aat-furn#300039702> ;
.
<https://w3id.org/con-tax/components/aat-furn#300039719>
  rdf:type owl:Class ;
  rdfs:comment "Franse speeltafels met een triktrakbord (backgammon-speelbord) dat meestal is verzonken onder een afneembaar tafelblad dat aan een zijde is uitgerust met een gevernist schaakbord en aan de andere zijde met laken of leer is bekleed om kaart op te spelen."@nl ;
  rdfs:comment "Gaming tables, often French, incorporating a tric-trac board; the board typically has twelve holes along the base of each side, used for scoring.The table may also include a chess board and surface for the playing of cards. Although similar, \"backgammon tables\" tend to be of more recent origin and different design. Tric-trac was popular in France and elsewhere 16th-19th centuries. Both games could be played on either table. "@en ;
  rdfs:isDefinedBy <https://w3id.org/con-tax/components/aat-furn> ;
  rdfs:label "tric-trac tables"@en ;
  rdfs:label "triktraktafel"@nl ;
  rdfs:label "triktraktafels"@nl ;
  rdfs:seeAlso <http://vocab.getty.edu/aat/300039719> ;
  rdfs:seeAlso wd:Q2452586 ;
  rdfs:subClassOf <https://w3id.org/con-tax/components/aat-furn#300039694> ;
.
<https://w3id.org/con-tax/components/aat-furn#300039734>
  rdf:type owl:Class ;
  rdfs:comment "Flat boards or other surfaces, usually cloth-covered and with one tapered end, on which clothing or similar articles are ironed; may be freestanding and supported with collapsible legs or attached to a vertical surface."@en ;
  rdfs:comment "Te gebruiken voor platte planken of andere oppervlakken, gewoonlijk bedekt met stof en aan één zijde spits toelopend, waarop kleding en dergelijke worden gestreken; kunnen vrijstaand zijn met een inklapbaar onderstel of bevestigd aan een verticaal oppervlak."@nl ;
  rdfs:isDefinedBy <https://w3id.org/con-tax/components/aat-furn> ;
  rdfs:label "ironing boards"@en ;
  rdfs:label "strijkplank"@nl ;
  rdfs:label "strijkplanken"@nl ;
  rdfs:seeAlso <http://vocab.getty.edu/aat/300039734> ;
  rdfs:seeAlso wd:Q2007190 ;
  rdfs:subClassOf <https://w3id.org/con-tax/components/aat-furn#300039548> ;
.
<https://w3id.org/con-tax/components/aat-furn#300039741>
  rdf:type owl:Class ;
  rdfs:comment "Side or serving tables arranged with compartments or drawers for bottles and decanters, and a flat work space for mixing drinks. It may be marble-topped and have a roll top that descends to cover the marble slab when not in use. "@en ;
  rdfs:comment "Tafels met een marmeren tafelblad en een opbouw met laden voor wijnkannen en een tambourdeksel dat omlaag kan rollen om het blad te bedekken als de tafel niet in gebruik is. Gebruik 'slab tables' voor 18e-eeuwse tafels met marmeren tafelblad zonder opbouw."@nl ;
  rdfs:isDefinedBy <https://w3id.org/con-tax/components/aat-furn> ;
  rdfs:label "mengtafel"@nl ;
  rdfs:label "mengtafels"@nl ;
  rdfs:label "mixing tables"@en ;
  rdfs:seeAlso <http://vocab.getty.edu/aat/300039741> ;
  rdfs:subClassOf <https://w3id.org/con-tax/components/aat-furn#300039548> ;
.
<https://w3id.org/con-tax/components/aat-furn#300039743>
  rdf:type owl:Class ;
  rdfs:comment "Kleine tafels met een houten blad die op een driehoekig frame met drie poten steunen."@nl ;
  rdfs:comment "Small plank top tables supported on a triangular frame with three legs."@en ;
  rdfs:isDefinedBy <https://w3id.org/con-tax/components/aat-furn> ;
  rdfs:label "drinking tables (mixing tables)"@en ;
  rdfs:label "drinktafel"@nl ;
  rdfs:label "drinktafels"@nl ;
  rdfs:seeAlso <http://vocab.getty.edu/aat/300039743> ;
  rdfs:subClassOf <https://w3id.org/con-tax/components/aat-furn#300039741> ;
.
<https://w3id.org/con-tax/components/aat-furn#300039745>
  rdf:type owl:Class ;
  rdfs:comment "Kleine tafeltjes die zijn bestemd om naast een bed te staan. Hieronder worden ook de tafeltjes gerekend met een kastje voor een po  of met een stilletje dat uit het onderste gedeelte naar voren schuift."@nl ;
  rdfs:comment "Small tables made to stand beside a bed; includes those having a cupboard to hold a chamber pot and those with a close stool that pulls forward in the lower part."@en ;
  rdfs:isDefinedBy <https://w3id.org/con-tax/components/aat-furn> ;
  rdfs:label "nachttafel"@nl ;
  rdfs:label "nachttafels"@nl ;
  rdfs:label "night tables"@en ;
  rdfs:seeAlso <http://vocab.getty.edu/aat/300039745> ;
  rdfs:seeAlso wd:Q667999 ;
  rdfs:subClassOf <https://w3id.org/con-tax/components/aat-furn#300039548> ;
.
<https://w3id.org/con-tax/components/aat-furn#300039752>
  rdf:type owl:Class ;
  rdfs:comment "Kleine tafels die makkelijk verplaatsbaar zijn."@nl ;
  rdfs:comment "Relatively small, easily movable tables."@en ;
  rdfs:isDefinedBy <https://w3id.org/con-tax/components/aat-furn> ;
  rdfs:label "gelegenheidstafel"@nl ;
  rdfs:label "gelegenheidstafels"@nl ;
  rdfs:label "occasional tables"@en ;
  rdfs:seeAlso <http://vocab.getty.edu/aat/300039752> ;
  rdfs:subClassOf <https://w3id.org/con-tax/components/aat-furn#300039548> ;
.
<https://w3id.org/con-tax/components/aat-furn#300039755>
  rdf:type owl:Class ;
  rdfs:comment "Tables used at a picnic, often collapsible. "@en ;
  rdfs:isDefinedBy <https://w3id.org/con-tax/components/aat-furn> ;
  rdfs:label "picknicktafel"@nl ;
  rdfs:label "picknicktafels"@nl ;
  rdfs:label "picnic tables"@en ;
  rdfs:seeAlso <http://vocab.getty.edu/aat/300039755> ;
  rdfs:seeAlso wd:Q2466395 ;
  rdfs:subClassOf <https://w3id.org/con-tax/components/aat-furn#300039548> ;
  rdfs:subClassOf <https://w3id.org/con-tax/components/aat-furn#300165810> ;
.
<https://w3id.org/con-tax/components/aat-furn#300039756>
  rdf:type owl:Class ;
  rdfs:comment "Tables with slate surfaces covered with cloth, having six pockets and surrounded by cushioned rails. Distinct from \"billiard tables\" which do not have pockets."@en ;
  rdfs:comment "Tafels met een oppervlak van met stof beklede leistenen platen, met zes zakken en een stootrand rondom. Te onderscheiden van 'biljarttafels' die geen zakken hebben."@nl ;
  rdfs:isDefinedBy <https://w3id.org/con-tax/components/aat-furn> ;
  rdfs:label "pool tables"@en ;
  rdfs:label "pooltafel"@nl ;
  rdfs:label "pooltafels"@nl ;
  rdfs:seeAlso <http://vocab.getty.edu/aat/300039756> ;
  rdfs:subClassOf <https://w3id.org/con-tax/components/aat-furn#300039548> ;
.
<https://w3id.org/con-tax/components/aat-furn#300039757>
  rdf:type owl:Class ;
  rdfs:comment "Spaanse en Portugese koloniale, zeer kleine, lage tafels met meestal snijwerk zonder reliëf en zware afhangende randen."@nl ;
  rdfs:comment "Spanish and Portuguese Colonial very small, low tables generally having flat carving and heavy aprons."@en ;
  rdfs:isDefinedBy <https://w3id.org/con-tax/components/aat-furn> ;
  rdfs:label "ratona"@nl ;
  rdfs:label "ratona's"@nl ;
  rdfs:label "ratonas"@en ;
  rdfs:seeAlso <http://vocab.getty.edu/aat/300039757> ;
  rdfs:subClassOf <https://w3id.org/con-tax/components/aat-furn#300039548> ;
.
<https://w3id.org/con-tax/components/aat-furn#300039760>
  rdf:type owl:Class ;
  rdfs:comment "Relatively large side tables, some of which may have tops attached to the wall, which are used in a dining room for serving food or displaying dishes. For case furniture used to serve food and display, use \"sideboards (furniture).\""@en ;
  rdfs:comment "Wandtafels die in de eetkamer worden gebruikt en waarvan sommige tafelbladen aan de wand kunnen zijn bevestigd. Gebruik 'dressoirs (meubelen)' voor lage, brede ladenkasten of  bergmeubels op poten die ook in eetkamers worden gebruikt."@nl ;
  rdfs:isDefinedBy <https://w3id.org/con-tax/components/aat-furn> ;
  rdfs:label "dressoirtafel"@nl ;
  rdfs:label "dressoirtafels"@nl ;
  rdfs:label "sideboard tables"@en ;
  rdfs:seeAlso <http://vocab.getty.edu/aat/300039760> ;
  rdfs:subClassOf <https://w3id.org/con-tax/components/aat-furn#300039999> ;
  rdfs:subClassOf <https://w3id.org/con-tax/components/aat-furn#300403907> ;
.
<https://w3id.org/con-tax/components/aat-furn#300039767>
  rdf:type owl:Class ;
  rdfs:comment "Objecten die ontworpen zijn om andere voorwerpen te ondersteunen en te presenteren. Voorbeelden zijn op tafels gelijkende meubelsstukken om voorwerpen te dragen en ze te tonen. Voor ondersteundende structuren die ontworpen zijn voor, en bevestigd zijn aan, het ondersteunde voorwerp, gebruik dan 'voetstukken'."@nl ;
  rdfs:comment "Objects designed to support or display another object; examples are small tablelike pieces of furniture used for holding or displaying objects. For supporting structures that are designed with and attached to the supported object, use \"bases (object components).\""@en ;
  rdfs:isDefinedBy <https://w3id.org/con-tax/components/aat-furn> ;
  rdfs:label "standaard (ondersteunend meubilair)"@nl ;
  rdfs:label "standaard"@nl ;
  rdfs:label "standaarden (ondersteunend meubilair)"@nl ;
  rdfs:label "standaarden"@nl ;
  rdfs:label "stander"@nl ;
  rdfs:label "standers"@nl ;
  rdfs:label "stands (support objects)"@en ;
  rdfs:seeAlso <http://vocab.getty.edu/aat/300039767> ;
  rdfs:subClassOf <https://w3id.org/con-tax/components/aat-furn#300039337> ;
  contax:containsGuideTerm <https://w3id.org/con-tax/components/aat-furn#300039786> ;
  contax:containsGuideTerm <https://w3id.org/con-tax/components/aat-furn#300165783> ;
.
<https://w3id.org/con-tax/components/aat-furn#300039770>
  rdf:type owl:Class ;
  rdfs:comment "Stands with two or more tiers or stands for maximizing surface area."@en ;
  rdfs:isDefinedBy <https://w3id.org/con-tax/components/aat-furn> ;
  rdfs:label "etagère (standaard)"@nl ;
  rdfs:label "etagère"@nl ;
  rdfs:label "etagères (standaarden)"@nl ;
  rdfs:label "etagères"@nl ;
  rdfs:label "tiered stands"@en ;
  rdfs:seeAlso <http://vocab.getty.edu/aat/300039770> ;
  rdfs:subClassOf <https://w3id.org/con-tax/components/aat-furn#300039767> ;
.
<https://w3id.org/con-tax/components/aat-furn#300039777>
  rdf:type gvp:GuideTerm ;
  rdfs:isDefinedBy <https://w3id.org/con-tax/components/aat-furn> ;
  rdfs:label "<standaard naar vorm: basisvorm>"@nl ;
  rdfs:label "<standaarden naar vorm: basisvorm>"@nl ;
  rdfs:label "<stands by form: base form>"@en ;
  rdfs:label "standaard naar vorm: basisvorm"@nl ;
  rdfs:label "standaarden naar vorm: basisvorm"@nl ;
  rdfs:seeAlso <http://vocab.getty.edu/aat/300039777> ;
  contax:containsConcept <https://w3id.org/con-tax/components/aat-furn#300164679> ;
  contax:containsConcept <https://w3id.org/con-tax/components/aat-furn#300265144> ;
.
<https://w3id.org/con-tax/components/aat-furn#300039786>
  rdf:type gvp:GuideTerm ;
  rdfs:isDefinedBy <https://w3id.org/con-tax/components/aat-furn> ;
  rdfs:label "<standaard naar functie>"@nl ;
  rdfs:label "<standaarden naar functie>"@nl ;
  rdfs:label "<stands by function>"@en ;
  rdfs:label "standaard naar functie"@nl ;
  rdfs:label "standaarden naar functie"@nl ;
  rdfs:seeAlso <http://vocab.getty.edu/aat/300039786> ;
  contax:containsConcept <https://w3id.org/con-tax/components/aat-furn#300022862> ;
  contax:containsConcept <https://w3id.org/con-tax/components/aat-furn#300037709> ;
  contax:containsConcept <https://w3id.org/con-tax/components/aat-furn#300039790> ;
  contax:containsConcept <https://w3id.org/con-tax/components/aat-furn#300039797> ;
  contax:containsConcept <https://w3id.org/con-tax/components/aat-furn#300039810> ;
  contax:containsConcept <https://w3id.org/con-tax/components/aat-furn#300039822> ;
  contax:containsConcept <https://w3id.org/con-tax/components/aat-furn#300039830> ;
  contax:containsConcept <https://w3id.org/con-tax/components/aat-furn#300039835> ;
  contax:containsConcept <https://w3id.org/con-tax/components/aat-furn#300039843> ;
  contax:containsConcept <https://w3id.org/con-tax/components/aat-furn#300039844> ;
  contax:containsConcept <https://w3id.org/con-tax/components/aat-furn#300039846> ;
  contax:containsConcept <https://w3id.org/con-tax/components/aat-furn#300039851> ;
  contax:containsConcept <https://w3id.org/con-tax/components/aat-furn#300039852> ;
  contax:containsConcept <https://w3id.org/con-tax/components/aat-furn#300039857> ;
  contax:containsConcept <https://w3id.org/con-tax/components/aat-furn#300077342> ;
  contax:containsConcept <https://w3id.org/con-tax/components/aat-furn#300079639> ;
  contax:containsConcept <https://w3id.org/con-tax/components/aat-furn#300135332> ;
  contax:containsConcept <https://w3id.org/con-tax/components/aat-furn#300164323> ;
  contax:containsConcept <https://w3id.org/con-tax/components/aat-furn#300164361> ;
  contax:containsConcept <https://w3id.org/con-tax/components/aat-furn#300164367> ;
  contax:containsConcept <https://w3id.org/con-tax/components/aat-furn#300164419> ;
  contax:containsConcept <https://w3id.org/con-tax/components/aat-furn#300164491> ;
  contax:containsConcept <https://w3id.org/con-tax/components/aat-furn#300164508> ;
  contax:containsConcept <https://w3id.org/con-tax/components/aat-furn#300170801> ;
  contax:containsConcept <https://w3id.org/con-tax/components/aat-furn#300174721> ;
  contax:containsConcept <https://w3id.org/con-tax/components/aat-furn#300250899> ;
  contax:containsConcept <https://w3id.org/con-tax/components/aat-furn#300261032> ;
  contax:containsConcept <https://w3id.org/con-tax/components/aat-furn#300262819> ;
  contax:containsConcept <https://w3id.org/con-tax/components/aat-furn#300262826> ;
  contax:containsConcept <https://w3id.org/con-tax/components/aat-furn#300310116> ;
  contax:containsConcept <https://w3id.org/con-tax/components/aat-furn#300311735> ;
  contax:containsConcept <https://w3id.org/con-tax/components/aat-furn#300375207> ;
  contax:containsConcept <https://w3id.org/con-tax/components/aat-furn#300375673> ;
  contax:containsConcept <https://w3id.org/con-tax/components/aat-furn#300375675> ;
  contax:containsConcept <https://w3id.org/con-tax/components/aat-furn#300390973> ;
  contax:containsConcept <https://w3id.org/con-tax/components/aat-furn#300391111> ;
  contax:containsConcept <https://w3id.org/con-tax/components/aat-furn#300395631> ;
  contax:containsConcept <https://w3id.org/con-tax/components/aat-furn#300404220> ;
  contax:containsConcept <https://w3id.org/con-tax/components/aat-furn#300417914> ;
  contax:containsConcept <https://w3id.org/con-tax/components/aat-furn#300424865> ;
.
<https://w3id.org/con-tax/components/aat-furn#300039789>
  rdf:type owl:Class ;
  rdfs:comment "Carved tripod stand that was popular as a type of furniture, particularly in Neoclassical French design. Often used as a washstand. It was based on the style of the metal tripod on the choregic monument of Lysikrates and also found in Herculaneum. The form was reconstructed by James Stuart as a motif at Kedleston Hall, Derbyshire. The form is also depicted in a painting by Joseph-Marie Vien, \"La Vertueuse Athénienne\" (1763), and thus the name is derived."@en ;
  rdfs:comment "Sierlijke, multifunctionele statieven, met name de statieven in de stijl van antieke bronzen voorwerpen uit Herculaneum. Algemeen voorkomend in neoklassiek Frans meubilair."@nl ;
  rdfs:isDefinedBy <https://w3id.org/con-tax/components/aat-furn> ;
  rdfs:label "athénienne"@nl ;
  rdfs:label "athéniennes"@en ;
  rdfs:label "athéniennes"@nl ;
  rdfs:seeAlso <http://vocab.getty.edu/aat/300039789> ;
  rdfs:subClassOf <https://w3id.org/con-tax/components/aat-furn#300164679> ;
.
<https://w3id.org/con-tax/components/aat-furn#300039790>
  rdf:type owl:Class ;
  rdfs:comment "Stands intended to hold books."@en ;
  rdfs:isDefinedBy <https://w3id.org/con-tax/components/aat-furn> ;
  rdfs:label "boekenstandaard (standaard)"@nl ;
  rdfs:label "boekenstandaard"@nl ;
  rdfs:label "boekenstandaarden (standaarden)"@nl ;
  rdfs:label "boekenstandaarden"@nl ;
  rdfs:label "bookstands"@en ;
  rdfs:seeAlso <http://vocab.getty.edu/aat/300039790> ;
  rdfs:subClassOf <https://w3id.org/con-tax/components/aat-furn#300039767> ;
.
<https://w3id.org/con-tax/components/aat-furn#300039794>
  rdf:type owl:Class ;
  rdfs:comment "Stands for supporting the Koran in a position convenient for reading. May resemble a common bookstand or take the form of an X, with the book supported in the upper cradle of the crossing planks. Stands for supporting the Koran in a position convenient for reading. May resemble a common bookstand or take the form of an X, with the book supported in the upper cradle of the crossing planks."@en ;
  rdfs:isDefinedBy <https://w3id.org/con-tax/components/aat-furn> ;
  rdfs:label "Koran stands"@en ;
  rdfs:label "koranstandaarden"@nl ;
  rdfs:label "koranstandaards"@nl ;
  rdfs:seeAlso <http://vocab.getty.edu/aat/300039794> ;
  rdfs:subClassOf <https://w3id.org/con-tax/components/aat-furn#300039790> ;
.
<https://w3id.org/con-tax/components/aat-furn#300039797>
  rdf:type owl:Class ;
  rdfs:comment "Draagbare standaarden met een zeer klein blad waarop een kaars of lamp kan staan. Ze hebben meestal een rond of gevormd blad dat op een middenpilaar steunt met een statief als onderstel."@nl ;
  rdfs:comment "Portable stands with a very small top intended to hold a candle or lamp; usually having a round or shaped top supported on a central pillar and with a tripod base."@en ;
  rdfs:isDefinedBy <https://w3id.org/con-tax/components/aat-furn> ;
  rdfs:label "candlestands (furniture)"@en ;
  rdfs:label "kaarshouder (meubilair)"@nl ;
  rdfs:label "kaarshouder"@nl ;
  rdfs:label "kaarshouders (meubilair)"@nl ;
  rdfs:label "kaarshouders"@nl ;
  rdfs:seeAlso <http://vocab.getty.edu/aat/300039797> ;
  rdfs:subClassOf <https://w3id.org/con-tax/components/aat-furn#300039767> ;
.
<https://w3id.org/con-tax/components/aat-furn#300039805>
  rdf:type owl:Class ;
  rdfs:comment "Candlestands with a notched mechanism for raising or lowering a support for a candle and usually with a trestle base."@en ;
  rdfs:comment "Kaarshouders met een palmechanisme voor het omhoog- en omlaagbrengen van het steuntje van de kaars. Meestal hebben ze een geschraagd onderstel."@nl ;
  rdfs:isDefinedBy <https://w3id.org/con-tax/components/aat-furn> ;
  rdfs:label "ratchet candlestand"@nl ;
  rdfs:label "ratchet candlestands"@en ;
  rdfs:label "ratchet candlestands"@nl ;
  rdfs:seeAlso <http://vocab.getty.edu/aat/300039805> ;
  rdfs:subClassOf <https://w3id.org/con-tax/components/aat-furn#300039797> ;
.
<https://w3id.org/con-tax/components/aat-furn#300039810>
  rdf:type owl:Class ;
  rdfs:comment "Standaarden waarin flessen en glazen passen."@nl ;
  rdfs:comment "Stands or small tables fitted for or of a size and shape appropriate for bottles and glasses, such as the horseshoe-shaped tables popular in the 18th century."@en ;
  rdfs:isDefinedBy <https://w3id.org/con-tax/components/aat-furn> ;
  rdfs:label "drinking stands"@en ;
  rdfs:label "flessenstandaard"@nl ;
  rdfs:label "flessenstandaarden"@nl ;
  rdfs:seeAlso <http://vocab.getty.edu/aat/300039810> ;
  rdfs:subClassOf <https://w3id.org/con-tax/components/aat-furn#300039767> ;
.
<https://w3id.org/con-tax/components/aat-furn#300039813>
  rdf:type owl:Class ;
  rdfs:comment "Articles of dining-room furniture intended to dispense with the services of a waiter at table. It comprises an upright pole bearing one or more trays or shelves, sometimes revolving. On these are placed glasses, dishes, and other table requisites."@en ;
  rdfs:comment "Benaming die door Sheraton wordt gebruikt voor standaarden met drie verdiepeingen, die zijn bestemd om, in de eetkamer, de schone en gebruikte borden en glazen op te zetten."@nl ;
  rdfs:isDefinedBy <https://w3id.org/con-tax/components/aat-furn> ;
  rdfs:label "dumbwaiters (stands)"@en ;
  rdfs:label "serveertafel"@nl ;
  rdfs:label "serveertafels"@nl ;
  rdfs:seeAlso <http://vocab.getty.edu/aat/300039813> ;
  rdfs:subClassOf <https://w3id.org/con-tax/components/aat-furn#300039770> ;
.
<https://w3id.org/con-tax/components/aat-furn#300039822>
  rdf:type owl:Class ;
  rdfs:comment "Standaarden voor wereldbollen en hemelglobes."@nl ;
  rdfs:comment "Stands for terrestrial and celestial globes."@en ;
  rdfs:isDefinedBy <https://w3id.org/con-tax/components/aat-furn> ;
  rdfs:label "globe stands"@en ;
  rdfs:label "globestandaard"@nl ;
  rdfs:label "globestandaarden"@nl ;
  rdfs:seeAlso <http://vocab.getty.edu/aat/300039822> ;
  rdfs:subClassOf <https://w3id.org/con-tax/components/aat-furn#300039767> ;
.
<https://w3id.org/con-tax/components/aat-furn#300039823>
  rdf:type owl:Class ;
  rdfs:comment "Compact, fitted dressing chests intended to hold a lady's jewelry and cosmetics. Compact, fitted dressing chests intended to hold a lady's jewelry and cosmetics."@en ;
  rdfs:isDefinedBy <https://w3id.org/con-tax/components/aat-furn> ;
  rdfs:label "dameskledingstandaard"@nl ;
  rdfs:label "dameskledingstandaarden"@nl ;
  rdfs:label "ladies' dressing stands"@en ;
  rdfs:seeAlso <http://vocab.getty.edu/aat/300039823> ;
  rdfs:subClassOf <https://w3id.org/con-tax/components/aat-furn#300174721> ;
.
<https://w3id.org/con-tax/components/aat-furn#300039830>
  rdf:type owl:Class ;
  rdfs:comment "Furniture in the form of pedestals with an an inclined, sometimes moveable frame; used to hold scores or sheet music in position for reading. "@en ;
  rdfs:comment "Standaarden die zijn ontworpen om partituren of bladmuziek op te zetten zodat ze makkelijk kunnen worden gelezen."@nl ;
  rdfs:isDefinedBy <https://w3id.org/con-tax/components/aat-furn> ;
  rdfs:label "music stands"@en ;
  rdfs:label "muzieklessenaar"@nl ;
  rdfs:label "muzieklessenaars"@nl ;
  rdfs:label "muziekstandaard"@nl ;
  rdfs:label "muziekstandaarden"@nl ;
  rdfs:seeAlso <http://vocab.getty.edu/aat/300039830> ;
  rdfs:seeAlso wd:Q930133 ;
  rdfs:subClassOf <https://w3id.org/con-tax/components/aat-furn#300039767> ;
.
<https://w3id.org/con-tax/components/aat-furn#300039835>
  rdf:type owl:Class ;
  rdfs:comment "Kleine tafelachtige meubelstukken waarop planten of bloemen worden gezet voor vertoning."@nl ;
  rdfs:comment "Relatively small table-like or shelf-like pieces of furniture used to hold or display potted plants, or sometimes containers of cut flowers."@en ;
  rdfs:isDefinedBy <https://w3id.org/con-tax/components/aat-furn> ;
  rdfs:label "plant stands"@en ;
  rdfs:label "plantenbak"@nl ;
  rdfs:label "plantenbakken"@nl ;
  rdfs:seeAlso <http://vocab.getty.edu/aat/300039835> ;
  rdfs:subClassOf <https://w3id.org/con-tax/components/aat-furn#300039767> ;
.
<https://w3id.org/con-tax/components/aat-furn#300039840>
  rdf:type owl:Class ;
  rdfs:comment "Houders waarin planten worden gekweekt, of waarin ze worden geplaatst voor decoratieve doeleinden; bovenkant soms gevoerd met lood; ze komen voor in een grote verscheidenheid aan vormen, maten en decoratie."@nl ;
  rdfs:comment "Ornamental receptacles on an elevated stand, used for growing plants and flowers, sometimes having a lead-lined top. For receptacles not associated with a stand, use \"jardinières (containers).\""@en ;
  rdfs:isDefinedBy <https://w3id.org/con-tax/components/aat-furn> ;
  rdfs:label "jardinière (plantenbak)"@nl ;
  rdfs:label "jardinière"@nl ;
  rdfs:label "jardinières (plant stands)"@en ;
  rdfs:label "jardinières (plantenbakken)"@nl ;
  rdfs:label "jardinières"@nl ;
  rdfs:seeAlso <http://vocab.getty.edu/aat/300039840> ;
  rdfs:subClassOf <https://w3id.org/con-tax/components/aat-furn#300039835> ;
.
<https://w3id.org/con-tax/components/aat-furn#300039843>
  rdf:type owl:Class ;
  rdfs:comment "Standaarden voor grote afdrukken. Ze hebben meestal een uitklapbare voorkant  en vaak een slot."@nl ;
  rdfs:comment "Stands for holding large prints; generally having a front which falls down and often having a lock."@en ;
  rdfs:isDefinedBy <https://w3id.org/con-tax/components/aat-furn> ;
  rdfs:label "portfolio (standaard)"@nl ;
  rdfs:label "portfolio stands"@en ;
  rdfs:label "portfolio"@nl ;
  rdfs:label "portfolio's (standaarden)"@nl ;
  rdfs:label "portfolio's"@nl ;
  rdfs:seeAlso <http://vocab.getty.edu/aat/300039843> ;
  rdfs:subClassOf <https://w3id.org/con-tax/components/aat-furn#300039767> ;
.
<https://w3id.org/con-tax/components/aat-furn#300039844>
  rdf:type owl:Class ;
  rdfs:comment "Periodiek gebruikte term: wordt gebruikt om een verscheidenheid aan 18de - en 19de eeuwse standaarden met verstelbare spiegels aan te duiden; gebruikt door mannen terwijl ze zich scheren of aankleden."@nl ;
  rdfs:comment "Stands with adjustable mirrors and a small table surface at chest-level, used by men to hold the implements required for shaving. The form appears in Europe in the 17th century, and was common in Britain and North America through the early 20th century."@en ;
  rdfs:isDefinedBy <https://w3id.org/con-tax/components/aat-furn> ;
  rdfs:label "scheerstandaard"@nl ;
  rdfs:label "scheerstandaarden"@nl ;
  rdfs:label "shaving stands"@en ;
  rdfs:seeAlso <http://vocab.getty.edu/aat/300039844> ;
  rdfs:subClassOf <https://w3id.org/con-tax/components/aat-furn#300039767> ;
.
<https://w3id.org/con-tax/components/aat-furn#300039846>
  rdf:type owl:Class ;
  rdfs:comment "Asbakken bevestigd op een laag voetstuk, meestal naast een sofa. Te onderscheiden van 'rookgereistandaarden'; kleine standaarden of kabinetten met vakjes die zijn omlijnd met zink, gebruikt om rookwaar in te bewaren."@nl ;
  rdfs:comment "Ashtrays mounted on a low pedestal stand generally used along side of a sofa. Distinct from \"smoking stands\" which are small stands or cabinets with zinc-lined compartments used to store smoking supplies."@en ;
  rdfs:isDefinedBy <https://w3id.org/con-tax/components/aat-furn> ;
  rdfs:label "smokers (ashtrays)"@en ;
  rdfs:label "staande asbak"@nl ;
  rdfs:label "staande asbakken"@nl ;
  rdfs:seeAlso <http://vocab.getty.edu/aat/300039846> ;
  rdfs:subClassOf <https://w3id.org/con-tax/components/aat-furn#300039767> ;
.
<https://w3id.org/con-tax/components/aat-furn#300039851>
  rdf:type owl:Class ;
  rdfs:comment "Stands designed to hold trays, typically for use in food service and display."@en ;
  rdfs:isDefinedBy <https://w3id.org/con-tax/components/aat-furn> ;
  rdfs:label "dienblad standaard"@nl ;
  rdfs:label "dienblad standaards"@nl ;
  rdfs:label "tray stands"@en ;
  rdfs:seeAlso <http://vocab.getty.edu/aat/300039851> ;
  rdfs:subClassOf <https://w3id.org/con-tax/components/aat-furn#300039767> ;
.
<https://w3id.org/con-tax/components/aat-furn#300039852>
  rdf:type owl:Class ;
  rdfs:comment "Stands or receptacles for holding umbrellas, generally located inside a home or other building near an exterior door. The term is used for stands of metal or wood construction as well as for large cylinder-shaped vessels of ceramic, metal, or another material, designed and used for holding umbrellas. Stands or receptacles for holding umbrellas, generally located inside a home or other building near an exterior door. The term is used for stands of metal or wood construction as well as for large cylinder-shaped vessels of ceramic, metal, or another material, designed and used for holding umbrellas."@en ;
  rdfs:isDefinedBy <https://w3id.org/con-tax/components/aat-furn> ;
  rdfs:label "paraplubak"@nl ;
  rdfs:label "paraplubakken"@nl ;
  rdfs:label "paraplustandaard"@nl ;
  rdfs:label "paraplustandaarden"@nl ;
  rdfs:label "umbrella stands"@en ;
  rdfs:seeAlso <http://vocab.getty.edu/aat/300039852> ;
  rdfs:seeAlso wd:Q5361833 ;
  rdfs:subClassOf <https://w3id.org/con-tax/components/aat-furn#300039767> ;
.
<https://w3id.org/con-tax/components/aat-furn#300039857>
  rdf:type owl:Class ;
  rdfs:comment "Furniture combining features of a table and cupboard and used to hold articles (as a pitcher, basin, and towel) for washing the hands and face."@en ;
  rdfs:comment "Meubilair dat een combinatie vormt van een tafel en een kast en wordt gebruikt om attributen voor het wassen van de handen en het gezicht in te bewaren, zoals een kan, schaal en handdoek."@nl ;
  rdfs:isDefinedBy <https://w3id.org/con-tax/components/aat-furn> ;
  rdfs:label "washstands"@en ;
  rdfs:label "wastafel (meubel)"@nl ;
  rdfs:label "wastafel"@nl ;
  rdfs:label "wastafels (meubel)"@nl ;
  rdfs:label "wastafels"@nl ;
  rdfs:seeAlso <http://vocab.getty.edu/aat/300039857> ;
  rdfs:subClassOf <https://w3id.org/con-tax/components/aat-furn#300039767> ;
.
<https://w3id.org/con-tax/components/aat-furn#300039859>
  rdf:type owl:Class ;
  rdfs:comment "Kleine standaarden om op te wassen. Ze hebben vaak een gevormde ring om de wasbak in te hangen, kleine laden onder het fries en een plank aan de onderkant om een kan op te zetten."@nl ;
  rdfs:comment "Small stands for washing, having a shelf or ring to hold the basin, and often shelves for a pitcher and chamber pot beneath. Drawers, towel bars, and ledges for soap and other toiltries may be included."@en ;
  rdfs:isDefinedBy <https://w3id.org/con-tax/components/aat-furn> ;
  rdfs:label "basin stands"@en ;
  rdfs:label "wastafelmeubel"@nl ;
  rdfs:label "wastafelmeubels"@nl ;
  rdfs:seeAlso <http://vocab.getty.edu/aat/300039859> ;
  rdfs:subClassOf <https://w3id.org/con-tax/components/aat-furn#300039857> ;
.
<https://w3id.org/con-tax/components/aat-furn#300039865>
  rdf:type owl:Class ;
  rdfs:comment "Basin stands designed to fit into the corner of a room."@en ;
  rdfs:isDefinedBy <https://w3id.org/con-tax/components/aat-furn> ;
  rdfs:label "corner basin stands"@en ;
  rdfs:label "hoek wastafelmeubel"@nl ;
  rdfs:label "hoek wastafelmeubelen"@nl ;
  rdfs:seeAlso <http://vocab.getty.edu/aat/300039865> ;
  rdfs:subClassOf <https://w3id.org/con-tax/components/aat-furn#300039859> ;
.
<https://w3id.org/con-tax/components/aat-furn#300039879>
  rdf:type owl:Class ;
  rdfs:comment "Tables with adjustable tops which could be raised by means of a ratchet so that they could be used as standing desks."@en ;
  rdfs:comment "Tafels met verstelbaar tafelblad dat omhoog kan worden gebracht met een palmechanisme zodat de tafels als sta-bureaus kunnen dienen."@nl ;
  rdfs:isDefinedBy <https://w3id.org/con-tax/components/aat-furn> ;
  rdfs:label "table à la tronchin"@nl ;
  rdfs:label "tables à la tronchin"@en ;
  rdfs:label "tables à la tronchin"@nl ;
  rdfs:seeAlso <http://vocab.getty.edu/aat/300039879> ;
  rdfs:subClassOf <https://w3id.org/con-tax/components/aat-furn#300039548> ;
  rdfs:subClassOf <https://w3id.org/con-tax/components/aat-furn#300164527> ;
.
<https://w3id.org/con-tax/components/aat-furn#300039880>
  rdf:type owl:Class ;
  rdfs:comment "18th-century French term for any small, easily portable table."@en ;
  rdfs:comment "Franse benaming uit de 18e eeuw  voor kleine, makkelijk draagbare tafels."@nl ;
  rdfs:isDefinedBy <https://w3id.org/con-tax/components/aat-furn> ;
  rdfs:label "table ambulante"@nl ;
  rdfs:label "tables ambulantes (occasional tables)"@en ;
  rdfs:label "tables ambulantes"@nl ;
  rdfs:seeAlso <http://vocab.getty.edu/aat/300039880> ;
  rdfs:seeAlso wd:Q7075679 ;
  rdfs:subClassOf <https://w3id.org/con-tax/components/aat-furn#300039752> ;
.
<https://w3id.org/con-tax/components/aat-furn#300039886>
  rdf:type owl:Class ;
  rdfs:comment "Term applied to a variety of small tables intended to hold a tea service and other articles used for serving tea; may have a top so made that it could be lifted off for separate use as a tray."@nl ;
  rdfs:comment "Term applied to small tables of various designs, intended to hold a tea service, or part of the service, and other articles used for serving tea; may have a top so made that it could be lifted off for separate use as a tray."@en ;
  rdfs:isDefinedBy <https://w3id.org/con-tax/components/aat-furn> ;
  rdfs:label "tea tables (tables)"@en ;
  rdfs:label "theetafel"@nl ;
  rdfs:label "theetafels"@nl ;
  rdfs:seeAlso <http://vocab.getty.edu/aat/300039886> ;
  rdfs:subClassOf <https://w3id.org/con-tax/components/aat-furn#300039548> ;
.
<https://w3id.org/con-tax/components/aat-furn#300039894>
  rdf:type owl:Class ;
  rdfs:comment "Kleine tafeltjes op wieltjes die worden gebruikt om thee en versnaperingen op te serveren."@nl ;
  rdfs:comment "Tables or other platforms on wheels used in serving tea and light refreshments; may have attached platforms or storage attachments."@en ;
  rdfs:isDefinedBy <https://w3id.org/con-tax/components/aat-furn> ;
  rdfs:label "tea wagons"@en ;
  rdfs:label "theewagen"@nl ;
  rdfs:label "theewagens"@nl ;
  rdfs:seeAlso <http://vocab.getty.edu/aat/300039894> ;
  rdfs:subClassOf <https://w3id.org/con-tax/components/aat-furn#300039548> ;
.
<https://w3id.org/con-tax/components/aat-furn#300039896>
  rdf:type owl:Class ;
  rdfs:comment "Italiaans soort kleine, spichtige tafeltjes op drie poten, die vooral in de 18e eeuw in Venetië populair waren."@nl ;
  rdfs:comment "Italian type of small, spindly three-legged tables, especially popular in 18th-century Venice."@en ;
  rdfs:isDefinedBy <https://w3id.org/con-tax/components/aat-furn> ;
  rdfs:label "trespoli"@en ;
  rdfs:label "trespoli"@nl ;
  rdfs:seeAlso <http://vocab.getty.edu/aat/300039896> ;
  rdfs:subClassOf <https://w3id.org/con-tax/components/aat-furn#300039548> ;
.
<https://w3id.org/con-tax/components/aat-furn#300039897>
  rdf:type owl:Class ;
  rdfs:comment "Kleine slaapkamertafels, vaak geschraagd, met een tafelblad met brede rand en soms één of meerdere planken, waar een man de inhoud van zijn zakken op kan legen wanneer hij zich uitkleedt. Ze werden voor het eerst gemaakt in Frankrijk, rond 1720, en werden tegen het einde van de 18e eeuw eveneens populair in Frankrijk."@nl ;
  rdfs:comment "Small bedroom tables, often of trestle form, with deeply rimmed tops and sometimes one or more shelves designed to hold the contents of a man's pockets when he undresses. First made in France in the 1720s and popular there and in England in the late 18th century."@en ;
  rdfs:isDefinedBy <https://w3id.org/con-tax/components/aat-furn> ;
  rdfs:label "vide-poche"@nl ;
  rdfs:label "vide-poches"@en ;
  rdfs:label "vide-poches"@nl ;
  rdfs:seeAlso <http://vocab.getty.edu/aat/300039897> ;
  rdfs:subClassOf <https://w3id.org/con-tax/components/aat-furn#300039548> ;
  rdfs:subClassOf <https://w3id.org/con-tax/components/aat-furn#300039612> ;
.
<https://w3id.org/con-tax/components/aat-furn#300039900>
  rdf:type owl:Class ;
  rdfs:comment "Relatively small tables used for sewing and other handiwork, usually having storage areas for working materials and implements."@en ;
  rdfs:comment "Tafels waarin werkmateriaal en gereedschap wordt opgeborgen, met name de kleine tafeltjes met laatjes en vaak een neerhangende stoffen zak voor naaiwerk."@nl ;
  rdfs:isDefinedBy <https://w3id.org/con-tax/components/aat-furn> ;
  rdfs:label "handiwork tables"@en ;
  rdfs:label "handwerktafel"@nl ;
  rdfs:label "handwerktafels"@nl ;
  rdfs:label "werktafel"@nl ;
  rdfs:label "werktafels"@nl ;
  rdfs:seeAlso <http://vocab.getty.edu/aat/300039900> ;
  rdfs:subClassOf <https://w3id.org/con-tax/components/aat-furn#300039548> ;
.
<https://w3id.org/con-tax/components/aat-furn#300039920>
  rdf:type owl:Class ;
  rdfs:comment "Dameswerktafels met een blad met verhoogde rand, soms ook met planken. De naam komt van tricoter, breien, maar de tafel wordt gebruikt voor verschillende soorten naaiwerk. Een 19e-eeuwse term die voornamelijk voor 18e-eeuwse meubels wordt gebruikt."@nl ;
  rdfs:comment "Ladies' work tables with tray tops and sometimes shelves; from \"tricoter,\" meaning to knit, but used for a variety of needlework forms. A 19th-century term used mainly for 18th-century pieces."@en ;
  rdfs:isDefinedBy <https://w3id.org/con-tax/components/aat-furn> ;
  rdfs:label "tricoteuses"@en ;
  rdfs:label "tricoteuses"@nl ;
  rdfs:seeAlso <http://vocab.getty.edu/aat/300039920> ;
  rdfs:seeAlso wd:Q21551068 ;
  rdfs:subClassOf <https://w3id.org/con-tax/components/aat-furn#300039900> ;
.
<https://w3id.org/con-tax/components/aat-furn#300039921>
  rdf:type owl:Class ;
  rdfs:comment "Franse benaming uit de 18e eeuw voor kleine, gelaagde tafeltjes, meestal met drie poten en beweegbare steuntjes voor kaarsen. Ze werden meestal gebruikt door vrouwen om aan te werken of te lezen."@nl ;
  rdfs:comment "French 18th-century term for small tiered tables, usually of tripod form, with movable arms to support candlesticks; generally used by women both for work and for reading."@en ;
  rdfs:isDefinedBy <https://w3id.org/con-tax/components/aat-furn> ;
  rdfs:label "serviteur fidèle"@nl ;
  rdfs:label "serviteurs fidèle"@nl ;
  rdfs:label "serviteurs-fidèle"@en ;
  rdfs:seeAlso <http://vocab.getty.edu/aat/300039921> ;
  rdfs:subClassOf <https://w3id.org/con-tax/components/aat-furn#300039619> ;
  rdfs:subClassOf <https://w3id.org/con-tax/components/aat-furn#300039900> ;
.
<https://w3id.org/con-tax/components/aat-furn#300039922>
  rdf:type owl:Class ;
  rdfs:comment "Kleine dameswerktafels in de klassieke uitvoering, met randen rondom het tafelblad en rondom de plank die de poten verbindt, zodat hier ondiepe 'bakjes' ontstonden waar chiffons (reepjes lint en stof) en ander naaiwerk kon worden bewaard. Ze waren vierkant of rond en hadden meestal drie laden, waarvan de bovenste soms met schrijfgerei was uitgerust."@nl ;
  rdfs:comment "Small ladies' work tables. In their classic form, may have galleries around its top and the shelf joining its legs to provide shallow receptacles into which one could place chiffons (scraps of ribbon and cloth) and other needlework materials; either square or circular in form and generally having three drawers, the uppermost sometimes fitted with writing equipment."@en ;
  rdfs:isDefinedBy <https://w3id.org/con-tax/components/aat-furn> ;
  rdfs:label "table en chiffonière"@nl ;
  rdfs:label "tables en chiffonière"@nl ;
  rdfs:label "tables en chiffonnière"@en ;
  rdfs:seeAlso <http://vocab.getty.edu/aat/300039922> ;
  rdfs:subClassOf <https://w3id.org/con-tax/components/aat-furn#300039900> ;
.
<https://w3id.org/con-tax/components/aat-furn#300039928>
  rdf:type gvp:GuideTerm ;
  rdfs:isDefinedBy <https://w3id.org/con-tax/components/aat-furn> ;
  rdfs:label "<tables by form>"@en ;
  rdfs:label "<tafel naar vorm>"@nl ;
  rdfs:label "<tafels naar vorm>"@nl ;
  rdfs:label "tafel naar vorm"@nl ;
  rdfs:label "tafels naar vorm"@nl ;
  rdfs:seeAlso <http://vocab.getty.edu/aat/300039928> ;
  contax:containsConcept <https://w3id.org/con-tax/components/aat-furn#300039605> ;
  contax:containsConcept <https://w3id.org/con-tax/components/aat-furn#300039752> ;
  contax:containsConcept <https://w3id.org/con-tax/components/aat-furn#300039757> ;
  contax:containsConcept <https://w3id.org/con-tax/components/aat-furn#300039879> ;
  contax:containsConcept <https://w3id.org/con-tax/components/aat-furn#300039929> ;
  contax:containsConcept <https://w3id.org/con-tax/components/aat-furn#300039933> ;
  contax:containsConcept <https://w3id.org/con-tax/components/aat-furn#300039951> ;
  contax:containsConcept <https://w3id.org/con-tax/components/aat-furn#300039963> ;
  contax:containsConcept <https://w3id.org/con-tax/components/aat-furn#300077320> ;
  contax:containsConcept <https://w3id.org/con-tax/components/aat-furn#300134019> ;
  contax:containsConcept <https://w3id.org/con-tax/components/aat-furn#300134034> ;
  contax:containsConcept <https://w3id.org/con-tax/components/aat-furn#300138411> ;
  contax:containsConcept <https://w3id.org/con-tax/components/aat-furn#300139992> ;
  contax:containsConcept <https://w3id.org/con-tax/components/aat-furn#300143751> ;
  contax:containsConcept <https://w3id.org/con-tax/components/aat-furn#300164357> ;
  contax:containsConcept <https://w3id.org/con-tax/components/aat-furn#300170140> ;
  contax:containsConcept <https://w3id.org/con-tax/components/aat-furn#300172364> ;
  contax:containsConcept <https://w3id.org/con-tax/components/aat-furn#300301349> ;
  contax:containsConcept <https://w3id.org/con-tax/components/aat-furn#300375699> ;
  contax:containsConcept <https://w3id.org/con-tax/components/aat-furn#300438673> ;
  contax:containsConcept <https://w3id.org/con-tax/components/aat-furn#300438695> ;
  contax:containsGuideTerm <https://w3id.org/con-tax/components/aat-furn#300039578> ;
  contax:containsGuideTerm <https://w3id.org/con-tax/components/aat-furn#300165790> ;
.
<https://w3id.org/con-tax/components/aat-furn#300039929>
  rdf:type owl:Class ;
  rdfs:comment "Tables with flaps which may be drawn out from beneath the top to extend the length. Late 16th-century and early 17th-century hall tables are often of this type."@en ;
  rdfs:comment "Tafels met zijstukken die vanonder het tafelblad kunnen worden getrokken om hem langer te maken. Haltafels uit het eind van de 16e en begin van de 17e eeuw zijn vaak van dit type."@nl ;
  rdfs:isDefinedBy <https://w3id.org/con-tax/components/aat-furn> ;
  rdfs:label "draw tables"@en ;
  rdfs:label "trektafel"@nl ;
  rdfs:label "trektafels"@nl ;
  rdfs:seeAlso <http://vocab.getty.edu/aat/300039929> ;
  rdfs:subClassOf <https://w3id.org/con-tax/components/aat-furn#300039548> ;
.
<https://w3id.org/con-tax/components/aat-furn#300039933>
  rdf:type owl:Class ;
  rdfs:comment "Algemene naam voor verschillende soorten ruimtebesparende tafels met bladen die met scharnieren aan het tafelblad zijn bevestigd, zodat ze omhoog kunnen worden geklapt om het oppervlak te vergroten."@nl ;
  rdfs:comment "Generic term for various types of space-saving tables with leaves hinged to the top so that they can be raised to extend the surface."@en ;
  rdfs:isDefinedBy <https://w3id.org/con-tax/components/aat-furn> ;
  rdfs:label "dropleaf tables"@en ;
  rdfs:label "opklapbare tafel"@nl ;
  rdfs:label "opklapbare tafels"@nl ;
  rdfs:seeAlso <http://vocab.getty.edu/aat/300039933> ;
  rdfs:seeAlso wd:Q5308374 ;
  rdfs:subClassOf <https://w3id.org/con-tax/components/aat-furn#300039548> ;
  rdfs:subClassOf <https://w3id.org/con-tax/components/aat-furn#300425808> ;
.
<https://w3id.org/con-tax/components/aat-furn#300039937>
  rdf:type owl:Class ;
  rdfs:comment "Drop leaf tables having a pear-shaped surface, that when the leaf is dropped, resemble butterfly wings; named after a table first designed by Finn Juhl in 1949."@en ;
  rdfs:isDefinedBy <https://w3id.org/con-tax/components/aat-furn> ;
  rdfs:label "butterfly tables"@en ;
  rdfs:label "hangoortafel"@nl ;
  rdfs:label "hangoortafels"@nl ;
  rdfs:label "valtafel"@nl ;
  rdfs:label "valtafels"@nl ;
  rdfs:seeAlso <http://vocab.getty.edu/aat/300039937> ;
  rdfs:subClassOf <https://w3id.org/con-tax/components/aat-furn#300039933> ;
.
<https://w3id.org/con-tax/components/aat-furn#300039939>
  rdf:type owl:Class ;
  rdfs:comment "Tables with a triangular top and one triangular folding leaf that, when raised, converts it to a square-top table; intended to stand in corners."@en ;
  rdfs:comment "Tafels met een driehoekig tafelblad en een eveneens driehoekig opklapblad, zodanig ontworpen dat de tafel vierkant wordt als het blad is opgeklapt. Hij is bedoeld om in een hoek te staan."@nl ;
  rdfs:isDefinedBy <https://w3id.org/con-tax/components/aat-furn> ;
  rdfs:label "handkerchief table"@nl ;
  rdfs:label "handkerchief tables"@en ;
  rdfs:label "handkerchief tables"@nl ;
  rdfs:seeAlso <http://vocab.getty.edu/aat/300039939> ;
  rdfs:subClassOf <https://w3id.org/con-tax/components/aat-furn#300039933> ;
.
<https://w3id.org/con-tax/components/aat-furn#300039941>
  rdf:type owl:Class ;
  rdfs:comment "Klaptafels met één of meerdere laden onder het tafelblad aan beide zijden. Ze werden tijdens de Chippendale-periode geïntroduceerd als geschikt voor vele doeleinden."@nl ;
  rdfs:comment "Relatively small, rectangular dropleaf tables with a drawer or drawers below. The leaves are supported by brackets. The form was introduced during the Chippendale period and intended to serve many purposes. The name refers to the Earl of Pembroke."@en ;
  rdfs:isDefinedBy <https://w3id.org/con-tax/components/aat-furn> ;
  rdfs:label "Pembroke tables"@en ;
  rdfs:label "Pembroketafel"@nl ;
  rdfs:label "Pembroketafels"@nl ;
  rdfs:seeAlso <http://vocab.getty.edu/aat/300039941> ;
  rdfs:subClassOf <https://w3id.org/con-tax/components/aat-furn#300039933> ;
.
<https://w3id.org/con-tax/components/aat-furn#300039944>
  rdf:type owl:Class ;
  rdfs:comment "A more elaborate version of the Pembroke table, with a small nest of drawers which is concealed in the body and may be made to rise from the top by means of weights; of a type made in late 18th-century England."@en ;
  rdfs:comment "Een  uitgebreidere versie van de Pembroketafel, met een kleine stapel laden die in het centrale deel zijn verborgen en met behulp van gewichten boven het blad kunnen worden gebracht. Dit type werd aan het eind van de 18e eeuw in Engeland gemaakt."@nl ;
  rdfs:isDefinedBy <https://w3id.org/con-tax/components/aat-furn> ;
  rdfs:label "harlequin table"@nl ;
  rdfs:label "harlequin tables"@en ;
  rdfs:label "harlequin tables"@nl ;
  rdfs:seeAlso <http://vocab.getty.edu/aat/300039944> ;
  rdfs:seeAlso wd:Q21972910 ;
  rdfs:subClassOf <https://w3id.org/con-tax/components/aat-furn#300039941> ;
.
<https://w3id.org/con-tax/components/aat-furn#300039951>
  rdf:type owl:Class ;
  rdfs:comment "Double-top card or dining tables that unfold like a book, supported by pivoting about to the opposite axis, by a swing leg, or by a runner."@en ;
  rdfs:comment "Eet- of kaarttafels met een dubbel tafelblad dat net zoals een boek openslaat en wordt ondersteund door een draaipoot of een rail, of door om een draaipunt te kantelen. ."@nl ;
  rdfs:isDefinedBy <https://w3id.org/con-tax/components/aat-furn> ;
  rdfs:label "flip-top tables"@en ;
  rdfs:label "tafel met omkeerbaar blad"@nl ;
  rdfs:label "tafels met omkeerbaar blad"@nl ;
  rdfs:seeAlso <http://vocab.getty.edu/aat/300039951> ;
  rdfs:subClassOf <https://w3id.org/con-tax/components/aat-furn#300039548> ;
  rdfs:subClassOf <https://w3id.org/con-tax/components/aat-furn#300425808> ;
.
<https://w3id.org/con-tax/components/aat-furn#300039958>
  rdf:type owl:Class ;
  rdfs:comment "A set of several tables, graduated in size so as to fit one over another."@en ;
  rdfs:comment "Een reeks tafels, oplopend in grootte zodat ze over elkaar heen passen."@nl ;
  rdfs:isDefinedBy <https://w3id.org/con-tax/components/aat-furn> ;
  rdfs:label "in elkaar passende tafel"@nl ;
  rdfs:label "in elkaar passende tafels"@nl ;
  rdfs:label "nesting tables"@en ;
  rdfs:seeAlso <http://vocab.getty.edu/aat/300039958> ;
  rdfs:subClassOf <https://w3id.org/con-tax/components/aat-furn#300039548> ;
.
<https://w3id.org/con-tax/components/aat-furn#300039962>
  rdf:type owl:Class ;
  rdfs:comment "Benaming die door Sheraton werd gebruikt voor een reeks van vier kleine tafels."@nl ;
  rdfs:comment "Term used by Sheraton to describe a nest of four small tables."@en ;
  rdfs:isDefinedBy <https://w3id.org/con-tax/components/aat-furn> ;
  rdfs:label "quartetto tables"@en ;
  rdfs:label "quartettotafel"@nl ;
  rdfs:label "quartettotafels"@nl ;
  rdfs:seeAlso <http://vocab.getty.edu/aat/300039962> ;
  rdfs:subClassOf <https://w3id.org/con-tax/components/aat-furn#300039958> ;
.
<https://w3id.org/con-tax/components/aat-furn#300039963>
  rdf:type owl:Class ;
  rdfs:comment "Driepotige tafels, veelal met een rond, scharnierend tafelblad dat tot een verticale positie gekanteld kan worden."@nl ;
  rdfs:comment "Tables whose tops are hinged to tilt to a vertical position."@en ;
  rdfs:isDefinedBy <https://w3id.org/con-tax/components/aat-furn> ;
  rdfs:label "opklaptafel"@nl ;
  rdfs:label "opklaptafels"@nl ;
  rdfs:label "tilt-top tables"@en ;
  rdfs:seeAlso <http://vocab.getty.edu/aat/300039963> ;
  rdfs:subClassOf <https://w3id.org/con-tax/components/aat-furn#300039548> ;
.
<https://w3id.org/con-tax/components/aat-furn#300039995>
  rdf:type owl:Class ;
  rdfs:comment "Tables that are usually rectangular, but may be round or oval; finished on all sides, and intended for use in the center of a parlor or other room. They are not necessarily of a design and height to accommodate seating in chairs. They are often made en suite with various forms of parlor furniture. For smaller, oval-shaped ornamental tables meant to be used as an accent piece and accommodating chairs for one or two people, especially in 19th-century parlors, use \"parlor tables.\" "@en ;
  rdfs:comment "Tafels met verschillende vormen, die aan alle kanten zijn afgewerkt en bedoeld om in het midden van een kamer te worden gezet.  Ze worden vaak in dezelfde stijl als andere woonkamermeubels gemaakt. Gebruik 'woonkamertafels' voor versierde tafels die, vooral in woonkamers, als pronkstuk dienen."@nl ;
  rdfs:isDefinedBy <https://w3id.org/con-tax/components/aat-furn> ;
  rdfs:label "center tables"@en-us ;
  rdfs:label "huiskamertafel"@nl ;
  rdfs:label "huiskamertafels"@nl ;
  rdfs:seeAlso <http://vocab.getty.edu/aat/300039995> ;
  rdfs:subClassOf <https://w3id.org/con-tax/components/aat-furn#300039548> ;
.
<https://w3id.org/con-tax/components/aat-furn#300039998>
  rdf:type owl:Class ;
  rdfs:comment "Any small tables used in relation to a couch or chair."@en ;
  rdfs:comment "Kleine tafeltjes die in bij een bank of stoel worden gebruikt."@nl ;
  rdfs:isDefinedBy <https://w3id.org/con-tax/components/aat-furn> ;
  rdfs:label "bijzettafeltje"@nl ;
  rdfs:label "bijzettafeltjes"@nl ;
  rdfs:label "end tables"@en ;
  rdfs:seeAlso <http://vocab.getty.edu/aat/300039998> ;
  rdfs:subClassOf <https://w3id.org/con-tax/components/aat-furn#300039548> ;
.
<https://w3id.org/con-tax/components/aat-furn#300039999>
  rdf:type owl:Class ;
  rdfs:comment "Tables designed to stand against the wall, generally with one side undecorated."@en ;
  rdfs:comment "Tafels om tegen een muur aan te zetten, meestal is één zijde onversierd."@nl ;
  rdfs:isDefinedBy <https://w3id.org/con-tax/components/aat-furn> ;
  rdfs:label "side tables"@en ;
  rdfs:label "zijtafel"@nl ;
  rdfs:label "zijtafels"@nl ;
  rdfs:seeAlso <http://vocab.getty.edu/aat/300039999> ;
  rdfs:subClassOf <https://w3id.org/con-tax/components/aat-furn#300039548> ;
.
<https://w3id.org/con-tax/components/aat-furn#300040000>
  rdf:type owl:Class ;
  rdfs:comment "Side tables of a size and design to stand in front of the pier or wall between two windows; sometimes surmounted by a pier glass."@en ;
  rdfs:comment "Zijtafels die tussen twee ramen staan; soms met een penantspiegel erboven."@nl ;
  rdfs:isDefinedBy <https://w3id.org/con-tax/components/aat-furn> ;
  rdfs:label "penanttafel"@nl ;
  rdfs:label "penanttafels"@nl ;
  rdfs:label "pier tables (side tables)"@en ;
  rdfs:seeAlso <http://vocab.getty.edu/aat/300040000> ;
  rdfs:subClassOf <https://w3id.org/con-tax/components/aat-furn#300039999> ;
.
<https://w3id.org/con-tax/components/aat-furn#300040014>
  rdf:type owl:Class ;
  rdfs:comment "Long, narrow tables having drop leaves and usually drawers, popular in the 18th and 19th centuries. The sofa table was usually placed in front of a sofa, but could be placed behind it. Modern versions typically have no drop leaves and are placed behind the sofa. For smaller drop leaf tables often placed near sofas or other seats, see \"Pembroke tables.\" For shorter tables without drop leaves that are placed in front of sofas, see \"coffee tables.\""@en ;
  rdfs:comment "Oorspronkelijk gebruikt als historische benaming voor tafels uit het eind van de 18e en het begin van de 19e eeuw, die leken op Pembroketafels, met scharnierende bladen aan elk uiteinde. Ze waren bestemd om voor een sofa te worden gezet. De benaming wordt tegenwoordig meer algemeen gebruikt voor elke tafel die bestemd is om voor of achter een sofa te staan."@nl ;
  rdfs:isDefinedBy <https://w3id.org/con-tax/components/aat-furn> ;
  rdfs:label "sofa tables"@en ;
  rdfs:label "sofa-tafel"@nl ;
  rdfs:label "sofa-tafels"@nl ;
  rdfs:seeAlso <http://vocab.getty.edu/aat/300040014> ;
  rdfs:subClassOf <https://w3id.org/con-tax/components/aat-furn#300039548> ;
  rdfs:subClassOf <https://w3id.org/con-tax/components/aat-furn#300039752> ;
.
<https://w3id.org/con-tax/components/aat-furn#300040026>
  rdf:type gvp:GuideTerm ;
  rdfs:isDefinedBy <https://w3id.org/con-tax/components/aat-furn> ;
  rdfs:label "<furniture by design>"@en ;
  rdfs:label "<meubilair naar ontwerp>"@nl ;
  rdfs:label "meubilair naar ontwerp"@nl ;
  rdfs:seeAlso <http://vocab.getty.edu/aat/300040026> ;
  contax:containsConcept <https://w3id.org/con-tax/components/aat-furn#300040029> ;
  contax:containsConcept <https://w3id.org/con-tax/components/aat-furn#300040033> ;
  contax:containsConcept <https://w3id.org/con-tax/components/aat-furn#300040036> ;
  contax:containsConcept <https://w3id.org/con-tax/components/aat-furn#300040039> ;
  contax:containsConcept <https://w3id.org/con-tax/components/aat-furn#300040041> ;
  contax:containsConcept <https://w3id.org/con-tax/components/aat-furn#300040157> ;
  contax:containsConcept <https://w3id.org/con-tax/components/aat-furn#300040163> ;
  contax:containsConcept <https://w3id.org/con-tax/components/aat-furn#300164268> ;
  contax:containsConcept <https://w3id.org/con-tax/components/aat-furn#300256336> ;
.
<https://w3id.org/con-tax/components/aat-furn#300040029>
  rdf:type owl:Class ;
  rdfs:comment "Furniture designed by architects or to match or accord with the architectural features of the rooms for which it is intended."@en ;
  rdfs:comment "Wordt gebruikt voor meubels die door architecten zijn ontworpen, of zo zijn gemaakt dat ze passen bij de architectonische kenmerken van de ruimte waarvoor ze zijn ontworpen."@nl ;
  rdfs:isDefinedBy <https://w3id.org/con-tax/components/aat-furn> ;
  rdfs:label "architectonisch meubilair"@nl ;
  rdfs:label "architectural furniture"@en ;
  rdfs:seeAlso <http://vocab.getty.edu/aat/300040029> ;
  rdfs:subClassOf <https://w3id.org/con-tax/components/aat-furn#300037680> ;
.
<https://w3id.org/con-tax/components/aat-furn#300040033>
  rdf:type owl:Class ;
  rdfs:comment "Furniture, typically made of flexible, airtight material such as plastic or vinyl, designed to be inflated by air. Inflatable furniture can be uninflated when not in use and stored conveniently stored in small spaces."@en ;
  rdfs:isDefinedBy <https://w3id.org/con-tax/components/aat-furn> ;
  rdfs:label "inflatable furniture"@en ;
  rdfs:label "opblaasbaar meubilair"@nl ;
  rdfs:seeAlso <http://vocab.getty.edu/aat/300040033> ;
  rdfs:subClassOf <https://w3id.org/con-tax/components/aat-furn#300037680> ;
.
<https://w3id.org/con-tax/components/aat-furn#300040036>
  rdf:type owl:Class ;
  rdfs:comment "Refers to a great variety of furniture including barbers' chairs, wheelchairs, and space-saving office furniture; designed to solve a particular problem."@en ;
  rdfs:comment "Verwijst naar allerlei soorten meubilair, waaronder kappersstoelen, rolstoelen en ruimtebesparend kantoormubilair, dat is ontworpen om een bepaald probleem op te lossen."@nl ;
  rdfs:isDefinedBy <https://w3id.org/con-tax/components/aat-furn> ;
  rdfs:label "mechanical furniture"@en ;
  rdfs:label "mechanisch meubilair"@nl ;
  rdfs:seeAlso <http://vocab.getty.edu/aat/300040036> ;
  rdfs:subClassOf <https://w3id.org/con-tax/components/aat-furn#300037680> ;
.
<https://w3id.org/con-tax/components/aat-furn#300040038>
  rdf:type owl:Class ;
  rdfs:comment "Variety of innovative furniture forms covered wholly or in part by a registered patent."@en ;
  rdfs:comment "Wordt gebruikt voor allerlei soorten vernieuwend meubilair waar geheel of gedeeltelijk patent op rust."@nl ;
  rdfs:isDefinedBy <https://w3id.org/con-tax/components/aat-furn> ;
  rdfs:label "gepatenteerd meubilair"@nl ;
  rdfs:label "patent furniture"@en ;
  rdfs:seeAlso <http://vocab.getty.edu/aat/300040038> ;
  rdfs:subClassOf <https://w3id.org/con-tax/components/aat-furn#300040036> ;
.
<https://w3id.org/con-tax/components/aat-furn#300040039>
  rdf:type owl:Class ;
  rdfs:comment "Aanduiding voor meubilair dat uit samenhangende eenheden bestaat, zodat meubelstukken als kleerkasten, wandkasten, boekenkasten of schrijfbureaus, die allemaal in standaardmaten worden gemaakt, gemakkelijk toegevoegd of opnieuw gerangschikt kunnen worden."@nl ;
  rdfs:comment "Describes furniture made in related units, so that pieces such as wardrobes, chests, cupboards, bookcases, or writing desks, made in standard sizes, may be conveniently added to and rearranged."@en ;
  rdfs:isDefinedBy <https://w3id.org/con-tax/components/aat-furn> ;
  rdfs:label "unit furniture"@en ;
  rdfs:label "unit furniture"@nl ;
  rdfs:seeAlso <http://vocab.getty.edu/aat/300040039> ;
  rdfs:subClassOf <https://w3id.org/con-tax/components/aat-furn#300037680> ;
.
<https://w3id.org/con-tax/components/aat-furn#300040041>
  rdf:type owl:Class ;
  rdfs:comment "Furniture designed to be used for a number of functions, such as writing, reading, needlework, or games, as well as larger pieces with ingeniously fitted interiors."@en ;
  rdfs:comment "Meubilair dat is ontworpen om voor meerdere doeleinden te worden gebruikt, zoals schrijven, lezen, naaiwerk of spelletjes, maar ook  grotere meubelstukken met een ingenieus ingebouwde binnenkant."@nl ;
  rdfs:isDefinedBy <https://w3id.org/con-tax/components/aat-furn> ;
  rdfs:label "multifunctioneel meubilair"@nl ;
  rdfs:label "multipurpose furniture"@en ;
  rdfs:seeAlso <http://vocab.getty.edu/aat/300040041> ;
  rdfs:subClassOf <https://w3id.org/con-tax/components/aat-furn#300037680> ;
.
<https://w3id.org/con-tax/components/aat-furn#300040045>
  rdf:type owl:Class ;
  rdfs:comment "Draagbaar meubilair voor gebruik buitenshuis."@nl ;
  rdfs:comment "Portable furniture intended for use outdoors."@en ;
  rdfs:isDefinedBy <https://w3id.org/con-tax/components/aat-furn> ;
  rdfs:label "camp furniture"@en ;
  rdfs:label "kampeermeubilair"@nl ;
  rdfs:seeAlso <http://vocab.getty.edu/aat/300040045> ;
  rdfs:subClassOf <https://w3id.org/con-tax/components/aat-furn#300256336> ;
.
<https://w3id.org/con-tax/components/aat-furn#300040046>
  rdf:type owl:Class ;
  rdfs:comment "Furniture designed to be erected and dissasembled easily and quickly, produced for officers to be taken on military campaign.  Despite these requirements, campaign furniture is typically luxurious and crafted from quality materials."@en ;
  rdfs:isDefinedBy <https://w3id.org/con-tax/components/aat-furn> ;
  rdfs:label "campagnemeubilair"@nl ;
  rdfs:label "campaign furniture"@en ;
  rdfs:seeAlso <http://vocab.getty.edu/aat/300040046> ;
  rdfs:seeAlso wd:Q5027833 ;
  rdfs:subClassOf <https://w3id.org/con-tax/components/aat-furn#300256336> ;
.
<https://w3id.org/con-tax/components/aat-furn#300040048>
  rdf:type owl:Class ;
  rdfs:comment "Furniture sold in units which can be packed flat and easily assembled with a screwdriver."@en ;
  rdfs:comment "Meubels die in onderdelen worden verkocht, zodat ze plat kunnen worden verpakt, en die makkelijk met een schroevendraaier in elkaar kunnen worden gezet."@nl ;
  rdfs:isDefinedBy <https://w3id.org/con-tax/components/aat-furn> ;
  rdfs:label "bouwpakketmeubilair"@nl ;
  rdfs:label "knock-down furniture"@en ;
  rdfs:seeAlso <http://vocab.getty.edu/aat/300040048> ;
  rdfs:seeAlso wd:Q1092595 ;
  rdfs:subClassOf <https://w3id.org/con-tax/components/aat-furn#300256336> ;
.
<https://w3id.org/con-tax/components/aat-furn#300040132>
  rdf:type gvp:GuideTerm ;
  rdfs:isDefinedBy <https://w3id.org/con-tax/components/aat-furn> ;
  rdfs:label "<furniture by location or context>"@en ;
  rdfs:label "<meubilair naar locatie of context>"@nl ;
  rdfs:label "meubilair naar locatie of context"@nl ;
  rdfs:seeAlso <http://vocab.getty.edu/aat/300040132> ;
  contax:containsConcept <https://w3id.org/con-tax/components/aat-furn#300165810> ;
  contax:containsConcept <https://w3id.org/con-tax/components/aat-furn#300266715> ;
.
<https://w3id.org/con-tax/components/aat-furn#300040157>
  rdf:type owl:Class ;
  rdfs:comment "Furniture built into the walls or overall structure of a building. This can include, chests, cabinets, corner cupboards, bookcases, beds, and seating."@en ;
  rdfs:isDefinedBy <https://w3id.org/con-tax/components/aat-furn> ;
  rdfs:label "built-in furniture"@en ;
  rdfs:label "ingebouwd meubilair"@nl ;
  rdfs:seeAlso <http://vocab.getty.edu/aat/300040157> ;
  rdfs:subClassOf <https://w3id.org/con-tax/components/aat-furn#300037680> ;
.
<https://w3id.org/con-tax/components/aat-furn#300040163>
  rdf:type owl:Class ;
  rdfs:comment "Furniture of simple design which makes the most economical use of materials and labor; generally austere, well-proportioned, and unornamented."@en ;
  rdfs:comment "Meubilair met een eenvoudig ontwerp waarbij zo efficiënt mogelijk gebruik wordt gemaakt van materiaal en arbeid; meestal sober, goed geproportioneerd en onversierd."@nl ;
  rdfs:isDefinedBy <https://w3id.org/con-tax/components/aat-furn> ;
  rdfs:label "praktisch meubilair"@nl ;
  rdfs:label "utility furniture"@en ;
  rdfs:seeAlso <http://vocab.getty.edu/aat/300040163> ;
  rdfs:seeAlso wd:Q7902843 ;
  rdfs:subClassOf <https://w3id.org/con-tax/components/aat-furn#300037680> ;
.
<https://w3id.org/con-tax/components/aat-furn#300040206>
  rdf:type owl:Class ;
  rdfs:comment "Ladders die worden gebruikt om mee in bed te klimmen."@nl ;
  rdfs:comment "Steps used to climb into a bed."@en ;
  rdfs:isDefinedBy <https://w3id.org/con-tax/components/aat-furn> ;
  rdfs:label "bed steps"@en ;
  rdfs:label "bedladder"@nl ;
  rdfs:label "bedladders"@nl ;
  rdfs:seeAlso <http://vocab.getty.edu/aat/300040206> ;
  rdfs:subClassOf <https://w3id.org/con-tax/components/aat-furn#300165788> ;
.
<https://w3id.org/con-tax/components/aat-furn#300040210>
  rdf:type owl:Class ;
  rdfs:comment "Ladders from which the upper shelves of a bookcase may be reached, often fitted into a chair, stool, table, or other piece of furniture."@en ;
  rdfs:comment "Ladders waarmee de bovenste planken van een boekenkast kunnen worden bereikt. Ze zijn vaak in een stoel, kruk, tafel of ander soort meubel verwerkt."@nl ;
  rdfs:isDefinedBy <https://w3id.org/con-tax/components/aat-furn> ;
  rdfs:label "bibliotheekladder"@nl ;
  rdfs:label "bibliotheekladders"@nl ;
  rdfs:label "library steps"@en ;
  rdfs:seeAlso <http://vocab.getty.edu/aat/300040210> ;
  rdfs:subClassOf <https://w3id.org/con-tax/components/aat-furn#300165788> ;
.
<https://w3id.org/con-tax/components/aat-furn#300048628>
  rdf:type gvp:GuideTerm ;
  rdfs:isDefinedBy <https://w3id.org/con-tax/components/aat-furn> ;
  rdfs:label "<furniture by form or function>"@en ;
  rdfs:label "<meubilair naar vorm of functie>"@nl ;
  rdfs:label "meubilair naar vorm of functie"@nl ;
  rdfs:seeAlso <http://vocab.getty.edu/aat/300048628> ;
  contax:containsConcept <https://w3id.org/con-tax/components/aat-furn#300037737> ;
  contax:containsConcept <https://w3id.org/con-tax/components/aat-furn#300037769> ;
  contax:containsConcept <https://w3id.org/con-tax/components/aat-furn#300039337> ;
  contax:containsGuideTerm <https://w3id.org/con-tax/components/aat-furn#300038696> ;
  contax:containsGuideTerm <https://w3id.org/con-tax/components/aat-furn#300164528> ;
.
<https://w3id.org/con-tax/components/aat-furn#300065017>
  rdf:type owl:Class ;
  rdfs:comment "Screens that separate the altar area from the space behind it. Distinct from \"reredoses,\" which relate visually to the altar and may form part of the inner side of an altar screen."@en ;
  rdfs:comment "Wordt gebruikt voor de hekken die de altaarruimte van de ruimte erachter scheiden. Te onderscheiden van 'reredoses' die visueel met het altaar verbonden zijn en een onderdeel kunnen zijn van de binnenkant van het altaarscherm."@nl ;
  rdfs:isDefinedBy <https://w3id.org/con-tax/components/aat-furn> ;
  rdfs:label "altaarscherm"@nl ;
  rdfs:label "altaarschermen"@nl ;
  rdfs:label "altar screens"@en ;
  rdfs:seeAlso <http://vocab.getty.edu/aat/300065017> ;
  rdfs:subClassOf <https://w3id.org/con-tax/components/aat-furn#300037737> ;
.
<https://w3id.org/con-tax/components/aat-furn#300065029>
  rdf:type owl:Class ;
  rdfs:comment "Hekwerk of traliewerk in een kerk, ontworpen om ongelovigen buiten een kapel of altaar te houden."@nl ;
  rdfs:comment "Screens, partitions, or railings serving to enclose or shut off a space in a building, particularly such structures located in a church, where they are designed to exclude nonworshippers from a chapel or shrine."@en ;
  rdfs:isDefinedBy <https://w3id.org/con-tax/components/aat-furn> ;
  rdfs:label "parcloses"@en ;
  rdfs:label "traliewerk (religieuze gebouwen)"@nl ;
  rdfs:label "traliewerk"@nl ;
  rdfs:label "traliewerken (religieuze gebouwen)"@nl ;
  rdfs:label "traliewerken"@nl ;
  rdfs:seeAlso <http://vocab.getty.edu/aat/300065029> ;
  rdfs:subClassOf <https://w3id.org/con-tax/components/aat-furn#300037737> ;
.
<https://w3id.org/con-tax/components/aat-furn#300065033>
  rdf:type owl:Class ;
  rdfs:comment "Distinctive rood screens found in Italian churches, often deep free-standing structures found particularly in mendicant churches and in many other monastic churches in Italy."@en ;
  rdfs:comment "Verwijst naar een Italiaans type koorhek."@nl ;
  rdfs:isDefinedBy <https://w3id.org/con-tax/components/aat-furn> ;
  rdfs:label "koorhek"@nl ;
  rdfs:label "tramezzi"@en ;
  rdfs:label "tramezzi"@nl ;
  rdfs:seeAlso <http://vocab.getty.edu/aat/300065033> ;
  rdfs:seeAlso wd:Q837995 ;
  rdfs:subClassOf <https://w3id.org/con-tax/components/aat-furn#300265155> ;
.
<https://w3id.org/con-tax/components/aat-furn#300075947>
  rdf:type owl:Class ;
  rdfs:comment "Refers to relatively large ornamented walls, screens, or other structures located above and behind the high altar of a Christian church, often holding the sacred tabernacle. A reredos may be placed against the apse wall, directly behind the altar, or may form part an altar screen. Its form evolved from the dossal, a tapestry or painting on the wall behind the altar. In church design, It may serve as a screen between celebrant and the congregation or between the choir and the retrochoir. In Spanish churches the reredos grew to be as wide as the nave and reaching to the vaulting of the roof. The reredos may be made of precious materials and heavily decorated, often with carvings, niches, sculptures, paintings and tapestries. It is distinct from a 'retable'; while the reredos typically rises from ground level behind the altar, the retable is smaller, standing either on the back of the altar itself or on a pedestal behind it. Many altars have both a reredos and a retable."@en ;
  rdfs:comment "Verwijst naar relatief grote versierde muren, schermen of andere constructies boven en achter het hoogaltaar van een christelijke kerk. Een reredos kan tegen de apsismuur of direct achter het altaar zijn geplaatst. Ook kan een reredos deel uitmaken van een altaarscherm. De term is afgeleid van een Anglo-Frans woord dat 'achter' of 'achterkant' betekende en raakte ingeburgerd in de 15de eeuw. De reredos ontstond uit de dorsaal, een tapisserie of schildering op de muur achter het altaar. In het kerkinterieur werden vanaf de late 11de eeuw de zetel van de bisschop en het koorgestoelte naar voren gebracht ten opzichte van de altaarmuur, en kwam de reredos als een scherm tussen hen en de congregatie in te staan. In bepaalde Engelse kerken diende de reredos als afscheiding tussen het koor en het achterkoor. In de loop van de tijd ging men voor het maken van de reredos kostbare materialen gebruiken en werd deze overdadig gedecoreerd, vaak met beeldsnijwerken, nissen, beeldhouwwerken, schilderingen en tapisserieën. De reredoses in Spaanse kerken werden in de loop der tijd zo breed als het schip en zo hoog als het dakgewelf. Een 'retabel' is iets anders. Dit is kleiner en staat achter op het altaar zelf of op een sokkel achter het altaar. Dit in tegenstelling tot reredoses die meestal vanaf de grond verrijzen achter het altaar. Veel altaren hebben zowel een reredos als een retabel. In de architectuur kan de term 'reredos' ook verwijzen naar een scherm of scheidingswand in een andere context, bijvoorbeeld naar de muur die de achterkant vormt van een open haard in een oude zaal."@nl ;
  rdfs:isDefinedBy <https://w3id.org/con-tax/components/aat-furn> ;
  rdfs:label "reredos"@nl ;
  rdfs:label "reredoses (screens)"@en ;
  rdfs:label "reredoses"@nl ;
  rdfs:seeAlso <http://vocab.getty.edu/aat/300075947> ;
  rdfs:seeAlso wd:Q46686 ;
  rdfs:subClassOf <https://w3id.org/con-tax/components/aat-furn#300037737> ;
.
<https://w3id.org/con-tax/components/aat-furn#300076039>
  rdf:type owl:Class ;
  rdfs:comment "Kerkbanken die afgeschermd zijn en omgeven door hoge achter- en zijkanten die meestal met deurtjes zijn afgesloten. Ze zijn bestemd voor specifieke groep kerkgangers, die een bepaald aanzien binnen of buiten de kerk hebben, zoals voorname families en andere notabelen."@nl ;
  rdfs:comment "Pews screened and enclosed by high backs and sides."@en ;
  rdfs:isDefinedBy <https://w3id.org/con-tax/components/aat-furn> ;
  rdfs:label "box pews"@en ;
  rdfs:label "gesloten kerkbank"@nl ;
  rdfs:label "gesloten kerkbanken"@nl ;
  rdfs:label "kerkgestoelten"@nl ;
  rdfs:label "kerkmeestersbanken"@nl ;
  rdfs:seeAlso <http://vocab.getty.edu/aat/300076039> ;
  rdfs:subClassOf <https://w3id.org/con-tax/components/aat-furn#300038521> ;
.
<https://w3id.org/con-tax/components/aat-furn#300076058>
  rdf:type owl:Class ;
  rdfs:comment "In het algemeen te gebruiken voor tussenwanden in religieuze en Romeinse keizerlijke gebouwen en openluchtlocaties tussen gewijde en wereldse ruimten of tussen bepaalde keizerlijke en openbare ruimten. In joodse context specifiek te gebruiken voor tussenwanden voor Torah-altaars, voornamelijk tijdens of voor de Byzantijnse tijd, en in christelijke kerken voor tussenwanden die het koor scheiden van het schip van de kerk, vooral als het koor geen zangkoor bevat. Gebruik 'koorafsluitingen' voor de schermen om het zangkoor als de koristen in het koor zitten. Gebruik 'iconostasen' voor de schermen in oosters-orthodoxe kerken die het heiligdom van het schip scheiden."@nl ;
  rdfs:comment "Use generally for partitions set up in religious and Roman Imperial buildings or outdoor areas between sacred and profane spaces or between certain Imperial and public spaces; use specifically in Jewish contexts for partitions in front of Torah shrines, especially in Byzantine and earlier periods, and in Christian churches for partitions separating the chancel from the body of the church, particularly when the chancel does not also include a choir. Use \"choir screens\" for the screens around the choir when the choristers are seated in the chancel area. For screens separating the sanctuary from the nave in Orthodox Eastern churches, use \"iconostases.\""@en ;
  rdfs:isDefinedBy <https://w3id.org/con-tax/components/aat-furn> ;
  rdfs:label "chancel screens"@en ;
  rdfs:label "koorscherm"@nl ;
  rdfs:label "koorschermen"@nl ;
  rdfs:seeAlso <http://vocab.getty.edu/aat/300076058> ;
  rdfs:seeAlso wd:Q837995 ;
  rdfs:subClassOf <https://w3id.org/con-tax/components/aat-furn#300037737> ;
.
<https://w3id.org/con-tax/components/aat-furn#300077236>
  rdf:type owl:Class ;
  rdfs:comment "Hedendaagse naam voor een bepaald soort elizabethaanse stoel  met een brede maar niet erg diepe zitting, een lage rugleuning en geen armleuningen. De onjuiste veronderstelling bestond dat ze werden gemaakt ten behoeve van de modieuze wijde hoepeljurken die crinolines werden genoemd."@nl ;
  rdfs:comment "Term of convenience for a type of chair with a wide but not very deep seat, low back, and no arms, originating in England in Elizabethan times. Term may have been coined under the assumption that the chairs were designed to accommodate the wide, hooped dresses called farthingales."@en ;
  rdfs:isDefinedBy <https://w3id.org/con-tax/components/aat-furn> ;
  rdfs:label "crinolinestoel"@nl ;
  rdfs:label "crinolinestoelen"@nl ;
  rdfs:label "farthingale chairs"@en ;
  rdfs:seeAlso <http://vocab.getty.edu/aat/300077236> ;
  rdfs:subClassOf <https://w3id.org/con-tax/components/aat-furn#300037789> ;
.
<https://w3id.org/con-tax/components/aat-furn#300077244>
  rdf:type owl:Class ;
  rdfs:comment "Medieval Spanish type of X-chairs, often with inlaid decoration."@en ;
  rdfs:comment "Spaanse X-framestoelen uit de Middeleeuwen, vaak versierd met inlegwerk."@nl ;
  rdfs:isDefinedBy <https://w3id.org/con-tax/components/aat-furn> ;
  rdfs:label "sillones de cadera"@en ;
  rdfs:label "sillóns de cadera"@nl ;
  rdfs:seeAlso <http://vocab.getty.edu/aat/300077244> ;
  rdfs:subClassOf <https://w3id.org/con-tax/components/aat-furn#300037904> ;
.
<https://w3id.org/con-tax/components/aat-furn#300077250>
  rdf:type owl:Class ;
  rdfs:comment "Term die werd gebruikt door Sheraton voor leunstoelen met een halfronde achterkant en verlengde zitting, waarvan de vorm aan een open rijtuig doet denken."@nl ;
  rdfs:comment "Term first used by Sheraton to describe armchairs having a semicircular back and elongated seat, the shape suggesting an open carriage."@en ;
  rdfs:isDefinedBy <https://w3id.org/con-tax/components/aat-furn> ;
  rdfs:label "curricle (stoelen)"@nl ;
  rdfs:label "curricle"@nl ;
  rdfs:label "curricles (chairs)"@en ;
  rdfs:label "curricles (stoelen)"@nl ;
  rdfs:label "curricles"@nl ;
  rdfs:seeAlso <http://vocab.getty.edu/aat/300077250> ;
  rdfs:subClassOf <https://w3id.org/con-tax/components/aat-furn#300037772> ;
  rdfs:subClassOf <https://w3id.org/con-tax/components/aat-furn#300037776> ;
.
<https://w3id.org/con-tax/components/aat-furn#300077252>
  rdf:type owl:Class ;
  rdfs:comment "American adaptations of late Sheraton-Style, open-backed side chairs. These are usually painted black with stencilled decoration that emulated gilt and lacquered furniture imported from Europe, and were developed and sold by Lambert Hitchcock in Connecticut in the mid-nineteenth century."@en ;
  rdfs:isDefinedBy <https://w3id.org/con-tax/components/aat-furn> ;
  rdfs:label "Hitchcock chairs"@en ;
  rdfs:label "Hitchcock-stoel"@nl ;
  rdfs:label "Hitchcock-stoelen"@nl ;
  rdfs:seeAlso <http://vocab.getty.edu/aat/300077252> ;
  rdfs:subClassOf <https://w3id.org/con-tax/components/aat-furn#300037772> ;
.
<https://w3id.org/con-tax/components/aat-furn#300077258>
  rdf:type owl:Class ;
  rdfs:comment "Franse stoelen uit de 18e eeuw die in het midden van een kamer stonden en verplaatsbaar waren. Ze verschillen van 'sièges courants' die grotendeels decoratief waren en tegen de muur werden gezet."@nl ;
  rdfs:comment "French 18th-century chairs that stood in the center of a room and could be moved. Distinct from \"sièges meublants\" which were largely decorative and were positioned against the wall."@en ;
  rdfs:isDefinedBy <https://w3id.org/con-tax/components/aat-furn> ;
  rdfs:label "sièges courants"@en ;
  rdfs:label "sièges courants"@nl ;
  rdfs:seeAlso <http://vocab.getty.edu/aat/300077258> ;
  rdfs:subClassOf <https://w3id.org/con-tax/components/aat-furn#300037772> ;
.
<https://w3id.org/con-tax/components/aat-furn#300077260>
  rdf:type owl:Class ;
  rdfs:comment "Franse stoelen uit de 18e eeuw die tegen de muur werden gezet. Het in gebruik nemen van deze stoelen werd strikt volgens de etiquette bepaald; sièges meublants werden meestal niet gebruikt om op te zitten maar maakten deel uit van de architektonische decoratie van een kamer. Ze zijn verschillend van 'sièges courants' die in het midden van een kamer stonden en verplaatsbaar waren."@nl ;
  rdfs:comment "French 18th-century chairs that were positioned against the wall. Their use was governed by strict protocol and sièges meublants were usually not sat on, but rather meant to be a part of the architectural decoration of a room. Distinct from \"sièges courants\" which stood in the center of a room and could be moved."@en ;
  rdfs:isDefinedBy <https://w3id.org/con-tax/components/aat-furn> ;
  rdfs:label "sièges meublant"@nl ;
  rdfs:label "sièges meublants"@en ;
  rdfs:seeAlso <http://vocab.getty.edu/aat/300077260> ;
  rdfs:subClassOf <https://w3id.org/con-tax/components/aat-furn#300037772> ;
.
<https://w3id.org/con-tax/components/aat-furn#300077268>
  rdf:type owl:Class ;
  rdfs:comment "19th-century sofas with a central backrest on either side of which people can sit."@en ;
  rdfs:comment "Negentiende-eeuwse sofa's met een rugleuning in het midden zodat mensen aan beide zijdes van de rugleuning kunnen zitten."@nl ;
  rdfs:isDefinedBy <https://w3id.org/con-tax/components/aat-furn> ;
  rdfs:label "boudeusse"@nl ;
  rdfs:label "boudeusses"@en ;
  rdfs:label "boudeusses"@nl ;
  rdfs:seeAlso <http://vocab.getty.edu/aat/300077268> ;
  rdfs:subClassOf <https://w3id.org/con-tax/components/aat-furn#300038634> ;
.
<https://w3id.org/con-tax/components/aat-furn#300077277>
  rdf:type owl:Class ;
  rdfs:comment "Ladenkasten of kasten op stoelhoogte die voor het vertonen en opbergen van voorwerpen worden gebruikt en vaak zeer uitvoerig zijn versierd. De benaming wordt vooral gebruikt voor Franse vormen of voor Engelse, Amerikaanse en andere stijlen om naar de Franse invloed op hun stijl te verwijzen."@nl ;
  rdfs:comment "Refers to chests of drawers or cabinets of chair-rail height, made for display as well as storage and often quite elaborately decorated. Term is applied especially to French forms, and to English, American, and other styles to indicate a form inspired by French taste."@en ;
  rdfs:isDefinedBy <https://w3id.org/con-tax/components/aat-furn> ;
  rdfs:label "commode (ladenkast)"@nl ;
  rdfs:label "commode"@nl ;
  rdfs:label "commodes (French chests of drawers)"@en ;
  rdfs:label "commodes (ladenkasten)"@nl ;
  rdfs:label "commodes"@nl ;
  rdfs:label "kommode"@nl ;
  rdfs:label "kommodes"@nl ;
  rdfs:seeAlso <http://vocab.getty.edu/aat/300077277> ;
  rdfs:subClassOf <https://w3id.org/con-tax/components/aat-furn#300039009> ;
.
<https://w3id.org/con-tax/components/aat-furn#300077279>
  rdf:type owl:Class ;
  rdfs:comment "Populaire benaming voor een bepaald soort Amerikaanse kaptafel uit de 18e eeuw, met laden en hoge poten. De kaptafel had dezelfde vorm als het onderste gedeelte van een hoge ladenkist, waar ze vaak aan werden aangepast."@nl ;
  rdfs:comment "Popular name for a type of 18th-century American dressing table with drawers, set on high legs, and similar in form to the lower section of a high chest of drawers, which it was often made to match."@en ;
  rdfs:isDefinedBy <https://w3id.org/con-tax/components/aat-furn> ;
  rdfs:label "lage kist"@nl ;
  rdfs:label "lage kisten"@nl ;
  rdfs:label "low chests"@en ;
  rdfs:seeAlso <http://vocab.getty.edu/aat/300077279> ;
  rdfs:subClassOf <https://w3id.org/con-tax/components/aat-furn#300039668> ;
.
<https://w3id.org/con-tax/components/aat-furn#300077291>
  rdf:type owl:Class ;
  rdfs:comment "Cupboards for the storage of linen items, including undergarments, shirts, bed linens, or table linens."@en ;
  rdfs:comment "Wandkasten waarin linnengoed wordt opgeborgen."@nl ;
  rdfs:isDefinedBy <https://w3id.org/con-tax/components/aat-furn> ;
  rdfs:label "linen presses"@en ;
  rdfs:label "linnen muurkast"@nl ;
  rdfs:label "linnen muurkasten"@nl ;
  rdfs:seeAlso <http://vocab.getty.edu/aat/300077291> ;
  rdfs:subClassOf <https://w3id.org/con-tax/components/aat-furn#300039252> ;
.
<https://w3id.org/con-tax/components/aat-furn#300077292>
  rdf:type owl:Class ;
  rdfs:comment "Kleine, driehoekige wandkasten die zijn bestemd om in een hoek te staan. Ze worden meestal per paar gemaakt en passen vaak bij een commode."@nl ;
  rdfs:comment "Small triangular cupboards made to fit into a corner; usually made in pairs, often to match a commode; often of ornamantal design."@en ;
  rdfs:isDefinedBy <https://w3id.org/con-tax/components/aat-furn> ;
  rdfs:label "encoignure"@nl ;
  rdfs:label "encoignures"@en ;
  rdfs:label "encoignures"@nl ;
  rdfs:seeAlso <http://vocab.getty.edu/aat/300077292> ;
  rdfs:seeAlso wd:Q3053821 ;
  rdfs:subClassOf <https://w3id.org/con-tax/components/aat-furn#300039285> ;
.
<https://w3id.org/con-tax/components/aat-furn#300077298>
  rdf:type owl:Class ;
  rdfs:comment "Franse bureaus met een verticaal uitklapblad waarachter laden en vakjes zitten. Ze hebben meestal een kastje aan de onderkant maar soms staan ze op hoge poten."@nl ;
  rdfs:comment "French desks with a vertical fall front enclosing drawers and pigeonholes; usually with a cupboard below, but sometimes raised up on tall legs."@en ;
  rdfs:isDefinedBy <https://w3id.org/con-tax/components/aat-furn> ;
  rdfs:label "secretaire à abattant"@nl ;
  rdfs:label "secretaires à abattant"@nl ;
  rdfs:label "secrétaires à abattant"@en ;
  rdfs:seeAlso <http://vocab.getty.edu/aat/300077298> ;
  rdfs:seeAlso wd:Q21550964 ;
  rdfs:subClassOf <https://w3id.org/con-tax/components/aat-furn#300039521> ;
.
<https://w3id.org/con-tax/components/aat-furn#300077310>
  rdf:type owl:Class ;
  rdfs:comment "Bureaus met een schuine voorkant, die meestal door vrouwen worden gebruikt."@nl ;
  rdfs:comment "Slant-front desks generally intended for a woman's use."@en ;
  rdfs:isDefinedBy <https://w3id.org/con-tax/components/aat-furn> ;
  rdfs:label "bureau en pente"@nl ;
  rdfs:label "bureaus en pente"@nl ;
  rdfs:label "bureaux en pente"@en ;
  rdfs:seeAlso <http://vocab.getty.edu/aat/300077310> ;
  rdfs:subClassOf <https://w3id.org/con-tax/components/aat-furn#300039526> ;
.
<https://w3id.org/con-tax/components/aat-furn#300077320>
  rdf:type owl:Class ;
  rdfs:comment "Kidney-shaped tables, generally used as writing or dressing tables, which were first made in France during the Louis XV period and later introduced in England and America."@en ;
  rdfs:comment "Wordt gebruikt voor niervormige tafels die meestal als schrijf- of toilettafel dienen. Ze werden eerst in Frankrijk gemaakt tijdens de periode van Louis XV, later zijn ze in Engeland en Amerika geïntroduceerd."@nl ;
  rdfs:isDefinedBy <https://w3id.org/con-tax/components/aat-furn> ;
  rdfs:label "kidney tables"@en ;
  rdfs:label "niervormige tafel"@nl ;
  rdfs:label "niervormige tafels"@nl ;
  rdfs:seeAlso <http://vocab.getty.edu/aat/300077320> ;
  rdfs:subClassOf <https://w3id.org/con-tax/components/aat-furn#300039436> ;
  rdfs:subClassOf <https://w3id.org/con-tax/components/aat-furn#300039548> ;
  rdfs:subClassOf <https://w3id.org/con-tax/components/aat-furn#300039668> ;
.
<https://w3id.org/con-tax/components/aat-furn#300077332>
  rdf:type owl:Class ;
  rdfs:comment "18th-century English writing tables with oblong tops, shallow drawers below, and four slender tapering legs joined with a shelf; often made in satinwood."@en ;
  rdfs:comment "Engelse schrijftafels uit de 18e eeuw met rechthoekig tafelblad waaronder ondiepe laden zitten en vier slanke, taps toelopende poten die zijn verbonden met een plank. Ze zijn vaak van satijnhout gemaakt."@nl ;
  rdfs:isDefinedBy <https://w3id.org/con-tax/components/aat-furn> ;
  rdfs:label "cheveret"@nl ;
  rdfs:label "cheverets"@en ;
  rdfs:label "cheverets"@nl ;
  rdfs:seeAlso <http://vocab.getty.edu/aat/300077332> ;
  rdfs:subClassOf <https://w3id.org/con-tax/components/aat-furn#300039436> ;
.
<https://w3id.org/con-tax/components/aat-furn#300077342>
  rdf:type owl:Class ;
  rdfs:comment "Standaarden waar theeketels of waterketels op kunnen staan. Gebruik ' theeketels met houders' voor theeketels met bijpassende ketelhouder."@nl ;
  rdfs:comment "Stands made to support hot water urns or teakettles. May be short-legged stands that are set upon a table, or taller stands with legs that reach the floor. For tables that support a tea service, use \"tea tables.\" Use \"teakettles-on-stands\" for teakettles made en suite with a stand."@en ;
  rdfs:isDefinedBy <https://w3id.org/con-tax/components/aat-furn> ;
  rdfs:label "ketelhouder"@nl ;
  rdfs:label "ketelhouders"@nl ;
  rdfs:label "kettle stands"@en ;
  rdfs:seeAlso <http://vocab.getty.edu/aat/300077342> ;
  rdfs:subClassOf <https://w3id.org/con-tax/components/aat-furn#300039767> ;
.
<https://w3id.org/con-tax/components/aat-furn#300077356>
  rdf:type owl:Class ;
  rdfs:comment "Cases of any size, usually made of glass, designed to display books, museum objects, or other objects and protect them from dust and insects; often having controlled humidity."@en ;
  rdfs:comment "Kasten van elke omvang, meestal gemaakt van glas, ontworpen om te boeken, museale voorwerpen, of andere objecten tentoon te stellen en hen te beschermen tegen stof en insecten; ze hebben vaak een gecontroleerde luchtvochtigheid."@nl ;
  rdfs:isDefinedBy <https://w3id.org/con-tax/components/aat-furn> ;
  rdfs:label "exhibit cases"@en ;
  rdfs:label "tentoonstellingskast"@nl ;
  rdfs:label "tentoonstellingskasten"@nl ;
  rdfs:label "uitstalkast"@nl ;
  rdfs:label "uitstalkasten"@nl ;
  rdfs:seeAlso <http://vocab.getty.edu/aat/300077356> ;
  rdfs:subClassOf <https://w3id.org/con-tax/components/aat-furn#300038860> ;
.
<https://w3id.org/con-tax/components/aat-furn#300078129>
  rdf:type owl:Class ;
  rdfs:comment "Refers to screens in Christian churches that separate the choir from the nave and aisles of a church. For partitions that separate the chancel from the nave of the church, use \"chancel screens.\" For partitions that separate the altar from the choir, use \"reredos.\""@en ;
  rdfs:comment "Verwijst naar afsluitingen in christelijke kerken waarmee het koor wordt afgescheiden van het schip en de zijbeuken van een kerk. Gebruik 'koorschermen' voor afsluitingen waarmee het koor wordt gescheiden van het schip van de kerk. Gebruik 'reredoses' voor afsluitingen waarmee het altaar wordt gescheiden van het koor."@nl ;
  rdfs:isDefinedBy <https://w3id.org/con-tax/components/aat-furn> ;
  rdfs:label "choir screens"@en ;
  rdfs:label "koorafsluiting"@nl ;
  rdfs:label "koorafsluitingen"@nl ;
  rdfs:seeAlso <http://vocab.getty.edu/aat/300078129> ;
  rdfs:seeAlso wd:Q837995 ;
  rdfs:subClassOf <https://w3id.org/con-tax/components/aat-furn#300037737> ;
.
<https://w3id.org/con-tax/components/aat-furn#300079633>
  rdf:type owl:Class ;
  rdfs:comment "Kleine kasten met glazen deuren en meestal glazen planken om miniaturen of kunstvoorwerpen te vertonen. Ze zijn in Frankrijk ontwikkeld en elders overgenomen. De benaming geldt ook  voor kleine tafels met een glazen bovenkant die voor hetzelfde doel worden gebruikt."@nl ;
  rdfs:comment "Small cabinets with glass doors and generally glass shelves for the display of miniatures or art objects; developed in France and adopted elsewhere. Also, small tables with glass tops used for the same purpose."@en ;
  rdfs:isDefinedBy <https://w3id.org/con-tax/components/aat-furn> ;
  rdfs:label "tentoonstellingsvitrine"@nl ;
  rdfs:label "tentoonstellingsvitrines"@nl ;
  rdfs:label "vitrine"@nl ;
  rdfs:label "vitrines (cabinets)"@en ;
  rdfs:label "vitrines"@nl ;
  rdfs:seeAlso <http://vocab.getty.edu/aat/300079633> ;
  rdfs:subClassOf <https://w3id.org/con-tax/components/aat-furn#300038888> ;
.
<https://w3id.org/con-tax/components/aat-furn#300079638>
  rdf:type owl:Class ;
  rdfs:comment "Standaarden of raamwerken die schuin staan en als onderstel of uitstalling van een schildersdoek, een schoolbord, een porseleinen bord of een ander voorwerp dienen."@nl ;
  rdfs:comment "Stands or frames for supporting or displaying at an angle an artist's canvas, a blackboard, china plate, or other object."@en ;
  rdfs:isDefinedBy <https://w3id.org/con-tax/components/aat-furn> ;
  rdfs:label "easels"@en ;
  rdfs:label "ezel (standaard)"@nl ;
  rdfs:label "ezel"@nl ;
  rdfs:label "ezels (standaarden)"@nl ;
  rdfs:label "ezels"@nl ;
  rdfs:label "schildersezel"@nl ;
  rdfs:label "schildersezels"@nl ;
  rdfs:seeAlso <http://vocab.getty.edu/aat/300079638> ;
  rdfs:seeAlso wd:Q939611 ;
  rdfs:subClassOf <https://w3id.org/con-tax/components/aat-furn#300039337> ;
.
<https://w3id.org/con-tax/components/aat-furn#300079639>
  rdf:type owl:Class ;
  rdfs:comment "Pieces of furniture having hooks, used to receive  hats, coats, umbrellas, and scarves, and often having shelves, a seat, and mirror. Usually situated near the front door in the hall of the house. For upright postlike stands with pegs or hooks around the top, use \"coat trees.\""@en ;
  rdfs:isDefinedBy <https://w3id.org/con-tax/components/aat-furn> ;
  rdfs:label "hall stands"@en ;
  rdfs:label "kapstok"@nl ;
  rdfs:label "kapstokken"@nl ;
  rdfs:label "klerenstandaard"@nl ;
  rdfs:label "klerenstandaarden"@nl ;
  rdfs:seeAlso <http://vocab.getty.edu/aat/300079639> ;
  rdfs:subClassOf <https://w3id.org/con-tax/components/aat-furn#300039767> ;
.
<https://w3id.org/con-tax/components/aat-furn#300109707>
  rdf:type owl:Class ;
  rdfs:comment "Ornamental screens in churches which either support an organ, or separate an organ chamber from the main space of the church."@en ;
  rdfs:comment "Wordt gebruikt voor de versierde hekken in een kerk die ofwel een orgel ondersteunen, ofwel een aparte orgelkamer scheiden van de hoofdruimte van de kerk."@nl ;
  rdfs:isDefinedBy <https://w3id.org/con-tax/components/aat-furn> ;
  rdfs:label "organ screens"@en ;
  rdfs:label "orgelscherm"@nl ;
  rdfs:label "orgelschermen"@nl ;
  rdfs:seeAlso <http://vocab.getty.edu/aat/300109707> ;
  rdfs:subClassOf <https://w3id.org/con-tax/components/aat-furn#300037737> ;
.
<https://w3id.org/con-tax/components/aat-furn#300121145>
  rdf:type owl:Class ;
  rdfs:comment "Gevlochten stoelen met armleuningen die een voorwaardse voortzetting van de achterkant zijn en meestal een rietvormige voet hebben in plaats van poten."@nl ;
  rdfs:comment "Wicker chairs with arms that are a forward continuation of the back, usually with a cane-shaped base in lieu of legs."@en ;
  rdfs:isDefinedBy <https://w3id.org/con-tax/components/aat-furn> ;
  rdfs:label "basket chairs"@en ;
  rdfs:label "korfstoel"@nl ;
  rdfs:label "korfstoelen"@nl ;
  rdfs:seeAlso <http://vocab.getty.edu/aat/300121145> ;
  rdfs:subClassOf <https://w3id.org/con-tax/components/aat-furn#300037772> ;
.
<https://w3id.org/con-tax/components/aat-furn#300121151>
  rdf:type owl:Class ;
  rdfs:comment "Benaming die wordt gebruikt voor het eerste type bentwoodstoelen. Gepatenteerd door  Samuel Gragg in 1808."@nl ;
  rdfs:comment "Term for the earliest type of bentwood chairs; patented by Samuel Gragg in 1808."@en ;
  rdfs:isDefinedBy <https://w3id.org/con-tax/components/aat-furn> ;
  rdfs:label "elastic chair"@nl ;
  rdfs:label "elastic chairs"@en ;
  rdfs:label "elastic chairs"@nl ;
  rdfs:seeAlso <http://vocab.getty.edu/aat/300121151> ;
  rdfs:subClassOf <https://w3id.org/con-tax/components/aat-furn#300037772> ;
.
<https://w3id.org/con-tax/components/aat-furn#300121177>
  rdf:type owl:Class ;
  rdfs:comment "Easy chairs with exaggerated wingbacks that protect the sitter from noise or drafts."@en ;
  rdfs:isDefinedBy <https://w3id.org/con-tax/components/aat-furn> ;
  rdfs:label "fauteuil à orieilles"@nl ;
  rdfs:label "fauteuils à oreilles"@en ;
  rdfs:label "fauteuils à oreilles"@nl ;
  rdfs:seeAlso <http://vocab.getty.edu/aat/300121177> ;
  rdfs:subClassOf <https://w3id.org/con-tax/components/aat-furn#300037838> ;
  rdfs:subClassOf <https://w3id.org/con-tax/components/aat-furn#300037856> ;
.
<https://w3id.org/con-tax/components/aat-furn#300121196>
  rdf:type owl:Class ;
  rdfs:comment "Refers to a variety of 19th-century chairs with nautical motifs and often a tablet top and a backrail incorporating cable molding. Made after the Battle of Trafalgar in 1805."@en ;
  rdfs:comment "Wordt gebruikt voor verschillende soorten stoelen uit de 19e eeuw met zeevaartmotieven, meestal een plaat als bovenkant en een bovenregel bewerkt met kabelpatronen. Ze werden gemaakt na de Zeeslag bij Trafalgar in 1805."@nl ;
  rdfs:isDefinedBy <https://w3id.org/con-tax/components/aat-furn> ;
  rdfs:label "Trafalgar chairs"@en ;
  rdfs:label "Trafalgar stoel"@nl ;
  rdfs:label "Trafalgar stoelen"@nl ;
  rdfs:seeAlso <http://vocab.getty.edu/aat/300121196> ;
  rdfs:subClassOf <https://w3id.org/con-tax/components/aat-furn#300037772> ;
.
<https://w3id.org/con-tax/components/aat-furn#300121231>
  rdf:type owl:Class ;
  rdfs:comment "Franse stoelen met een rugleuning in de vorm van een ellips of medallion waarbij het frame in het midden van de bovenkant is versierd met houtsnijwerk in de vorm van een gestrikt lint."@nl ;
  rdfs:comment "French chairs with oval or medallion-shaped backs, the frames being carved in the center of the top with a ribbon bow."@en ;
  rdfs:isDefinedBy <https://w3id.org/con-tax/components/aat-furn> ;
  rdfs:label "chaise à la d'artois"@nl ;
  rdfs:label "chaises à la d'artois"@en ;
  rdfs:label "chaises à la d'artois"@nl ;
  rdfs:seeAlso <http://vocab.getty.edu/aat/300121231> ;
  rdfs:subClassOf <https://w3id.org/con-tax/components/aat-furn#300037977> ;
.
<https://w3id.org/con-tax/components/aat-furn#300121246>
  rdf:type owl:Class ;
  rdfs:comment "Bureaustoelen met een diep gewelfde rugleuning en meestal een uitstekende poot middenvoor. Ze kunnen vier of vijf poten hebben en zijn vaak met houtsnijwerk versierd."@nl ;
  rdfs:comment "Desk chairs with deeply coved backs and usually, but not always, with a projecting central front leg; may have four or five legs. Very often carved."@en ;
  rdfs:isDefinedBy <https://w3id.org/con-tax/components/aat-furn> ;
  rdfs:label "bureaufauteuil"@nl ;
  rdfs:label "bureaufauteuils"@nl ;
  rdfs:label "fauteuils de bureau"@en ;
  rdfs:seeAlso <http://vocab.getty.edu/aat/300121246> ;
  rdfs:subClassOf <https://w3id.org/con-tax/components/aat-furn#300037856> ;
  rdfs:subClassOf <https://w3id.org/con-tax/components/aat-furn#300038165> ;
.
<https://w3id.org/con-tax/components/aat-furn#300121255>
  rdf:type owl:Class ;
  rdfs:comment "Ancient Greek folding stools without a back and having crossed legs."@en ;
  rdfs:comment "Oud-Griekse opvouwbare krukken zonder rugleuning en met gekruiste poten."@nl ;
  rdfs:isDefinedBy <https://w3id.org/con-tax/components/aat-furn> ;
  rdfs:label "diphroi okladias"@en ;
  rdfs:label "diphroi okladias"@nl ;
  rdfs:label "diphros okladias"@nl ;
  rdfs:seeAlso <http://vocab.getty.edu/aat/300121255> ;
  rdfs:subClassOf <https://w3id.org/con-tax/components/aat-furn#300244761> ;
.
<https://w3id.org/con-tax/components/aat-furn#300121308>
  rdf:type owl:Class ;
  rdfs:comment "Popular American term for mid-19th-century benches on rockers, with detachable fences two thirds of their length so that a baby could lie on the seat without rolling off, while the mother sat beside it."@en ;
  rdfs:comment "Veel voorkomende Amerikaanse benaming voor schommelbanken uit het midden van de 19e eeuw, met afneembare hekjes over tweederde van de lengte, zodat de moeder naast de baby op de bank kon zitten zonder dat het kind van de bank rolde."@nl ;
  rdfs:isDefinedBy <https://w3id.org/con-tax/components/aat-furn> ;
  rdfs:label "cradle benches"@en ;
  rdfs:label "wiegebank"@nl ;
  rdfs:label "wiegebanken"@nl ;
  rdfs:seeAlso <http://vocab.getty.edu/aat/300121308> ;
  rdfs:subClassOf <https://w3id.org/con-tax/components/aat-furn#300038494> ;
.
<https://w3id.org/con-tax/components/aat-furn#300121326>
  rdf:type owl:Class ;
  rdfs:comment "Refers to S-shaped sofas with ends curving inward so two people could sit face to face. For straight-fronted sofas with small triangular seats (sometimes detachable) set outside the arms at either end, use \"confidantes.\""@en ;
  rdfs:comment "Wordt gebruikt voor sofa's met een S-vorm waarbij de uiteinden naar binnen zijn gebogen zodat twee mensen met hun gezicht naar elkaar toe kunnen zitten. Gebruik 'confidentes' voor sofa's met een rechte voorkant en kleine, driehoekige zittingen die soms afneembaar zijn en aan de buitenzijden van de armleuningen zitten."@nl ;
  rdfs:isDefinedBy <https://w3id.org/con-tax/components/aat-furn> ;
  rdfs:label "canapé à confident"@nl ;
  rdfs:label "canapés à confident"@en ;
  rdfs:label "canapés à confident"@nl ;
  rdfs:seeAlso <http://vocab.getty.edu/aat/300121326> ;
  rdfs:subClassOf <https://w3id.org/con-tax/components/aat-furn#300038636> ;
.
<https://w3id.org/con-tax/components/aat-furn#300121340>
  rdf:type owl:Class ;
  rdfs:comment "Lange, lage, gestoffeerde stoelen van Turkse afkomst, meestal zonder rug- of armleuningen."@nl ;
  rdfs:comment "Long, low, upholstered seats of Turkish origin usually without backs or arms."@en ;
  rdfs:isDefinedBy <https://w3id.org/con-tax/components/aat-furn> ;
  rdfs:label "divan"@nl ;
  rdfs:label "divans"@en ;
  rdfs:label "divans"@nl ;
  rdfs:seeAlso <http://vocab.getty.edu/aat/300121340> ;
  rdfs:subClassOf <https://w3id.org/con-tax/components/aat-furn#300038493> ;
.
<https://w3id.org/con-tax/components/aat-furn#300121345>
  rdf:type owl:Class ;
  rdfs:comment "Beds, particularly those created in Europe prior to the 16th century, of various designs having a high wooden frame suspended over the head half of the bed, from which curtains may be hung in a tent-like fashion. Sparver beds typically do not have bedposts, but the frame may be attached to the wall or ceiling."@en ;
  rdfs:comment "Middeleeuwse bedden met een kom- of tentvormig gordijn dat over het hoofdeinde van het bed naar beneden hangt."@nl ;
  rdfs:isDefinedBy <https://w3id.org/con-tax/components/aat-furn> ;
  rdfs:label "sparver bed"@nl ;
  rdfs:label "sparver beds"@en ;
  rdfs:label "sparver beds"@nl ;
  rdfs:seeAlso <http://vocab.getty.edu/aat/300121345> ;
  rdfs:subClassOf <https://w3id.org/con-tax/components/aat-furn#300142742> ;
.
<https://w3id.org/con-tax/components/aat-furn#300121352>
  rdf:type owl:Class ;
  rdfs:comment "Cupboards containing bookshelves and closed with doors usually of glass or sometimes fitted with grilles."@en ;
  rdfs:comment "Kasten die boekenplanken bevatten en worden gesloten met deuren, gewoonlijk van glas, en soms voorzien van traliewerk."@nl ;
  rdfs:isDefinedBy <https://w3id.org/con-tax/components/aat-furn> ;
  rdfs:label "bibliotheek (kast)"@nl ;
  rdfs:label "bibliotheek"@nl ;
  rdfs:label "bibliotheken (kasten)"@nl ;
  rdfs:label "bibliotheken"@nl ;
  rdfs:label "bibliothèques (bookcases)"@en ;
  rdfs:seeAlso <http://vocab.getty.edu/aat/300121352> ;
  rdfs:subClassOf <https://w3id.org/con-tax/components/aat-furn#300143716> ;
.
<https://w3id.org/con-tax/components/aat-furn#300121376>
  rdf:type owl:Class ;
  rdfs:comment "Chests made from a hollowed log or tree trunk, and used primarily in the Middle Ages. Frequently used as safes."@en ;
  rdfs:isDefinedBy <https://w3id.org/con-tax/components/aat-furn> ;
  rdfs:label "dug-out chest"@nl ;
  rdfs:label "dug-out chests"@en ;
  rdfs:label "dug-out chests"@nl ;
  rdfs:seeAlso <http://vocab.getty.edu/aat/300121376> ;
  rdfs:subClassOf <https://w3id.org/con-tax/components/aat-furn#300038992> ;
.
<https://w3id.org/con-tax/components/aat-furn#300121378>
  rdf:type owl:Class ;
  rdfs:comment "Benaming die oorspronkelijk werd gebruikt voor kleine tafels en kisten met een bovenkant die is bedoeld om geld te tellen, soms met een kastje eronder. De benaming werd later gebruikt voor kasten of plankachtige oppervlakken die meestal op een zodanige hoogte zitten dat de persoon die ervoor staat, zoals in een keuken of winkel, of op een kruk ervoor zit, zoals in een restaurant of bar, er gemakkelijk bij kan."@nl ;
  rdfs:comment "Cases or shelflike surfaces, usually of a height convenient for a person standing before them, as in a kitchen or store, or sitting on stools in front of them, as in a restaurant or bar. For small tables or chests with the top marked for counting money, sometimes with a cupboard below, use the more specific \"counter tables.\""@en ;
  rdfs:isDefinedBy <https://w3id.org/con-tax/components/aat-furn> ;
  rdfs:label "counters (furniture)"@en ;
  rdfs:label "counters"@nl ;
  rdfs:label "toonbank"@nl ;
  rdfs:label "toonbanken"@nl ;
  rdfs:seeAlso <http://vocab.getty.edu/aat/300121378> ;
  rdfs:seeAlso wd:Q1420266 ;
  rdfs:subClassOf <https://w3id.org/con-tax/components/aat-furn#300038860> ;
  rdfs:subClassOf <https://w3id.org/con-tax/components/aat-furn#300040157> ;
.
<https://w3id.org/con-tax/components/aat-furn#300121380>
  rdf:type owl:Class ;
  rdfs:comment "Ancient Roman cupboards, generally having a rectangular case, mounted on feet, with doors reaching approximately from top to bottom, a gabled or flat top, and interior shelving."@en ;
  rdfs:comment "Oud-Romeinse wandkasten die meestal bestaan uit een rechthoekige kast op poten, deuren die min of meer van boven tot onder reiken, een puntige of platte bovenkant en planken aan de binnenkant."@nl ;
  rdfs:isDefinedBy <https://w3id.org/con-tax/components/aat-furn> ;
  rdfs:label "armaria"@en ;
  rdfs:label "armaria"@nl ;
  rdfs:label "armarium"@nl ;
  rdfs:seeAlso <http://vocab.getty.edu/aat/300121380> ;
  rdfs:seeAlso wd:Q679077 ;
  rdfs:subClassOf <https://w3id.org/con-tax/components/aat-furn#300039183> ;
.
<https://w3id.org/con-tax/components/aat-furn#300121381>
  rdf:type owl:Class ;
  rdfs:comment "Houten keukengootstenen, met name uit de 19e eeuw, die niet met een externe wateraanvoer zijn verbonden. Ze hebben boven een ondiepe zinken of tinnen bak waarin een afwasteil kan worden geplaatst en eronder meestal een kastje."@nl ;
  rdfs:comment "Wooden kitchen sinks, especially of the 19th century, that are counter height, not connected to an external drain, often with a shallow zinc or tin-lined well on top in which a dishpan or basin can be placed, and usually a cupboard below. A dry sink is often not connected to an external water supply, however, some are mounted with a hand pump. For similar pieces of furniture located in bathrooms or bedrooms, intended for personal hygiene rather than washing dishes, use \"washstands.\""@en ;
  rdfs:isDefinedBy <https://w3id.org/con-tax/components/aat-furn> ;
  rdfs:label "dry sink"@nl ;
  rdfs:label "dry sinks"@en ;
  rdfs:label "dry sinks"@nl ;
  rdfs:seeAlso <http://vocab.getty.edu/aat/300121381> ;
  rdfs:seeAlso wd:Q21550565 ;
  rdfs:subClassOf <https://w3id.org/con-tax/components/aat-furn#300039183> ;
.
<https://w3id.org/con-tax/components/aat-furn#300121481>
  rdf:type owl:Class ;
  rdfs:comment "Ancient Roman sideboards, generally having a tablelike lower member and an upper member with shelving; used to display highly prized ornaments."@en ;
  rdfs:comment "Oud-Romeinse zijrafels of dressoirs die meestal een tafelachtig onderstuk en een bovenstuk met planken hebben. Ze worden gebruikt om kostbaarheden te vertonen."@nl ;
  rdfs:isDefinedBy <https://w3id.org/con-tax/components/aat-furn> ;
  rdfs:label "abaci (sideboards)"@en ;
  rdfs:label "abaci (zijtafels)"@nl ;
  rdfs:label "abaci"@nl ;
  rdfs:label "abacus (zijtafel)"@nl ;
  rdfs:label "abacus"@nl ;
  rdfs:seeAlso <http://vocab.getty.edu/aat/300121481> ;
  rdfs:subClassOf <https://w3id.org/con-tax/components/aat-furn#300039306> ;
.
<https://w3id.org/con-tax/components/aat-furn#300121482>
  rdf:type owl:Class ;
  rdfs:comment "Dressoirs, met name Italiaanse of in Italiaanse stijl gemaakte dressoirs, die meestal twee of drie kastdeuren hebben met laden in het fries. Het onderstuk wordt vaak gemodelleerd en rust direct op de vloer of op leeuwenpoten."@nl ;
  rdfs:comment "Sideboards usually for use in the dining room and typically of Italian or Italian-styled designs, generally having two or three cupboard doors and drawers in the frieze area; the bases are often molded and rest directly on the floor or on short feet. "@en ;
  rdfs:isDefinedBy <https://w3id.org/con-tax/components/aat-furn> ;
  rdfs:label "credenza (dressoir)"@nl ;
  rdfs:label "credenza"@nl ;
  rdfs:label "credenzas (dressoirs)"@nl ;
  rdfs:label "credenzas (sideboards)"@en ;
  rdfs:label "credenzas"@nl ;
  rdfs:seeAlso <http://vocab.getty.edu/aat/300121482> ;
  rdfs:seeAlso wd:Q16676881 ;
  rdfs:subClassOf <https://w3id.org/con-tax/components/aat-furn#300039306> ;
.
<https://w3id.org/con-tax/components/aat-furn#300121499>
  rdf:type owl:Class ;
  rdfs:comment "Desks that close by means of a flexible shutter of convex shape and composed of horizontal slats of wood. Distinguished from \"tambour desks\" which close by means of upright reeded or slatted shutters."@en ;
  rdfs:comment "Wordt gebruikt voor bureaus die afsluiten met een flexibel, bolvormig deksel dat uit horizontale houen latjes bestaat. Ze verschillen van 'tambourbureaus' die worden afgesloten door een rechtopstaand deksel van riet of latjes."@nl ;
  rdfs:isDefinedBy <https://w3id.org/con-tax/components/aat-furn> ;
  rdfs:label "rolltop desks"@en ;
  rdfs:label "rolluikbureau"@nl ;
  rdfs:label "rolluikbureaus"@nl ;
  rdfs:seeAlso <http://vocab.getty.edu/aat/300121499> ;
  rdfs:seeAlso wd:Q7361371 ;
  rdfs:subClassOf <https://w3id.org/con-tax/components/aat-furn#300039338> ;
.
<https://w3id.org/con-tax/components/aat-furn#300121537>
  rdf:type owl:Class ;
  rdfs:comment "Tea tables of various designs, having a raised edge or gallery to protect china against slipping off or other damage."@en ;
  rdfs:comment "Wordt gebruikt voor theetafels met een opgehoogde rand of strook zodat het porselein wordt beschermd tegen beschadiging."@nl ;
  rdfs:isDefinedBy <https://w3id.org/con-tax/components/aat-furn> ;
  rdfs:label "china tables"@en ;
  rdfs:label "porseleintafel"@nl ;
  rdfs:label "porseleintafels"@nl ;
  rdfs:seeAlso <http://vocab.getty.edu/aat/300121537> ;
  rdfs:subClassOf <https://w3id.org/con-tax/components/aat-furn#300039886> ;
.
<https://w3id.org/con-tax/components/aat-furn#300124818>
  rdf:type owl:Class ;
  rdfs:comment "Series of seats, usually three in number, or a bench, and rarely only one seat, either movable or recessed in the wall and crowned with canopies, pinnacles, and other enrichments, usually placed on the south side of the choir near the altar for the officiating clergy: celebrant, deacon, and sub-deacon."@en ;
  rdfs:comment "Wordt gebruikt voor rijen zitplaatsen voor de dienstdoende geestelijken, meestal van steen en telkens drie, over het algemeen gesitueerd aan de zuidkant van het altaar."@nl ;
  rdfs:isDefinedBy <https://w3id.org/con-tax/components/aat-furn> ;
  rdfs:label "altaarbank"@nl ;
  rdfs:label "altaarbanken"@nl ;
  rdfs:label "sedilia"@en ;
  rdfs:label "sedilia"@nl ;
  rdfs:label "sedilium"@nl ;
  rdfs:seeAlso <http://vocab.getty.edu/aat/300124818> ;
  rdfs:seeAlso wd:Q1467789 ;
  rdfs:subClassOf <https://w3id.org/con-tax/components/aat-furn#300038494> ;
  rdfs:subClassOf <https://w3id.org/con-tax/components/aat-furn#300133851> ;
.
<https://w3id.org/con-tax/components/aat-furn#300125933>
  rdf:type owl:Class ;
  rdfs:comment "Chairs or thrones of a bishop in his cathedral church, in which he presides at solemn functions. The form is based on the ancient Roman cathedra. Originally the bishop's cathedra stood in the center of the apse, flanked at a lower level on either side by the benches where the assisting priests sat."@en ;
  rdfs:comment "Romeinse stoelen met een ronde rugleuning op verticale staanders en met gebogen poten. Tevens de zetel of troon van een bisschop in zijn kerk."@nl ;
  rdfs:isDefinedBy <https://w3id.org/con-tax/components/aat-furn> ;
  rdfs:label "bisschopszetel"@nl ;
  rdfs:label "bisschopszetels"@nl ;
  rdfs:label "cathedrae (bishop's chairs)"@en ;
  rdfs:label "katheder (bisschopszetel)"@nl ;
  rdfs:label "katheder"@nl ;
  rdfs:label "katheders (bisschopszetels)"@nl ;
  rdfs:label "katheders"@nl ;
  rdfs:seeAlso <http://vocab.getty.edu/aat/300125933> ;
  rdfs:seeAlso wd:Q1138500 ;
  rdfs:subClassOf <https://w3id.org/con-tax/components/aat-furn#300133851> ;
.
<https://w3id.org/con-tax/components/aat-furn#300133002>
  rdf:type owl:Class ;
  rdfs:comment "Chairs with back splats in the form of a lyre, a Regency period motif popularized by Adam, Hepplewhite, Sheraton, and Duncan Phyfe."@en ;
  rdfs:comment "Wordt gebruikt voor stoelen met een rugleuning in de vorm van een lier, een motief uit de Regency-periode dat bekendheid kreeg door  Adam, Hepplewhite, Sheraton en Duncan Phyfe."@nl ;
  rdfs:isDefinedBy <https://w3id.org/con-tax/components/aat-furn> ;
  rdfs:label "lyre-back chairs"@en ;
  rdfs:label "lyre-backstoel"@nl ;
  rdfs:label "lyre-backstoelen"@nl ;
  rdfs:seeAlso <http://vocab.getty.edu/aat/300133002> ;
  rdfs:subClassOf <https://w3id.org/con-tax/components/aat-furn#300133839> ;
.
<https://w3id.org/con-tax/components/aat-furn#300133763>
  rdf:type owl:Class ;
  rdfs:comment "High-back chairs with broad central splats, generally having leather-upholstered backs and seats; popular in 18th-century America."@en ;
  rdfs:comment "Stoelen met hoge rugleuning en brede rugspijlen in het midden, die meestal een rugleuning en zitting hebben die met leer is bekleed. Ze kwamen veel voor in Amerika in de 18e eeuw."@nl ;
  rdfs:isDefinedBy <https://w3id.org/con-tax/components/aat-furn> ;
  rdfs:label "Boston chairs"@en ;
  rdfs:label "Bostonstoel"@nl ;
  rdfs:label "Bostonstoelen"@nl ;
  rdfs:seeAlso <http://vocab.getty.edu/aat/300133763> ;
  rdfs:subClassOf <https://w3id.org/con-tax/components/aat-furn#300037772> ;
.
<https://w3id.org/con-tax/components/aat-furn#300133771>
  rdf:type owl:Class ;
  rdfs:comment "Lichte, opklapbare stoelen met een zitting en rugleuning die meestal van canvas zijn."@nl ;
  rdfs:comment "Light folding chairs, usually with canvas seats and backs."@en ;
  rdfs:isDefinedBy <https://w3id.org/con-tax/components/aat-furn> ;
  rdfs:label "camp chairs"@en ;
  rdfs:label "kampeerstoel"@nl ;
  rdfs:label "kampeerstoelen"@nl ;
  rdfs:seeAlso <http://vocab.getty.edu/aat/300133771> ;
  rdfs:subClassOf <https://w3id.org/con-tax/components/aat-furn#300040045> ;
  rdfs:subClassOf <https://w3id.org/con-tax/components/aat-furn#300244770> ;
.
<https://w3id.org/con-tax/components/aat-furn#300133811>
  rdf:type owl:Class ;
  rdfs:comment "Angular lawn chairs, similar in form to Adirondack chairs, but constructed of boards rather than slats and heavier and more amply proportioned; older than the classic Adirondack chairs, patented by Harry C. Brunnell, and manufactured between 1904 and 1930."@en ;
  rdfs:comment "Hoekige tuinstoelen die lijken op Adirondackstoelen maar van planken in plaats van latten zijn gemaakt en zwaarder en ruimer van proporties zijn. Ze werden gefabriceerd tussen 1904 en 1930 en zijn ouder dan de klassieke  Adirondackstoelen. Gepatenteerd door Harry C. Brunnell."@nl ;
  rdfs:isDefinedBy <https://w3id.org/con-tax/components/aat-furn> ;
  rdfs:label "Westport chairs"@en ;
  rdfs:label "Westportstoel"@nl ;
  rdfs:label "Westportstoelen"@nl ;
  rdfs:seeAlso <http://vocab.getty.edu/aat/300133811> ;
  rdfs:subClassOf <https://w3id.org/con-tax/components/aat-furn#300037772> ;
  rdfs:subClassOf <https://w3id.org/con-tax/components/aat-furn#300165810> ;
.
<https://w3id.org/con-tax/components/aat-furn#300133822>
  rdf:type owl:Class ;
  rdfs:comment "Chairs with flat backs. "@en ;
  rdfs:isDefinedBy <https://w3id.org/con-tax/components/aat-furn> ;
  rdfs:label "flat-back chairs"@en ;
  rdfs:label "flat-back stoelen"@nl ;
  rdfs:seeAlso <http://vocab.getty.edu/aat/300133822> ;
  rdfs:subClassOf <https://w3id.org/con-tax/components/aat-furn#300037772> ;
.
<https://w3id.org/con-tax/components/aat-furn#300133839>
  rdf:type owl:Class ;
  rdfs:comment "Chairs which have splats on their chair-backs, which are pierced. "@en ;
  rdfs:isDefinedBy <https://w3id.org/con-tax/components/aat-furn> ;
  rdfs:label "pierced splat-back chairs"@en ;
  rdfs:label "pierced splat-back chairs"@nl ;
  rdfs:seeAlso <http://vocab.getty.edu/aat/300133839> ;
  rdfs:subClassOf <https://w3id.org/con-tax/components/aat-furn#300037772> ;
.
<https://w3id.org/con-tax/components/aat-furn#300133850>
  rdf:type owl:Class ;
  rdfs:comment "Ancient Greek throne-like chairs, usually ornamented, having an elevated seat, often a high back and arms and either legs ending in animal feet, turned or rectangular legs, or with solid sides. Used by people of wealth or prominence and seen in depictions of the Greek gods."@en ;
  rdfs:comment "Te gebruiken voor oud-Griekse tronen, gewoonlijk versierd, met een verhoogde zetel en vaak met een hoge rug en armleuningen. Ze hebben soms poten in de vorm van dierenpoten, gedraaid of rechthoekig, en soms zijkanten uit één stuk. Gebruikt door rijke of belangrijke personen en te zien op afbeeldingen van de Griekse goden."@nl ;
  rdfs:isDefinedBy <https://w3id.org/con-tax/components/aat-furn> ;
  rdfs:label "thronoi"@en ;
  rdfs:label "thronoi"@nl ;
  rdfs:seeAlso <http://vocab.getty.edu/aat/300133850> ;
  rdfs:subClassOf <https://w3id.org/con-tax/components/aat-furn#300038141> ;
.
<https://w3id.org/con-tax/components/aat-furn#300133851>
  rdf:type owl:Class ;
  rdfs:comment "Chairs having a primarily ceremonial or ritual purpose."@en ;
  rdfs:isDefinedBy <https://w3id.org/con-tax/components/aat-furn> ;
  rdfs:label "ceremonial chairs"@en ;
  rdfs:label "ceremoniële stoelen"@nl ;
  rdfs:seeAlso <http://vocab.getty.edu/aat/300133851> ;
  rdfs:subClassOf <https://w3id.org/con-tax/components/aat-furn#300037772> ;
.
<https://w3id.org/con-tax/components/aat-furn#300133860>
  rdf:type owl:Class ;
  rdfs:comment "English type of upholstered armchair with wings and an arched top making a niche to screen the occupant from drafts; made from the mid-18th century onwards."@en ;
  rdfs:comment "Gestoffeerde leunstoelen van een Engels type met oren en een gewelfde bovenkant  zodat er een nis ontstaat die de zittende persoon tegen tocht beschermt. Ze werden gemaakt vanaf het midden van de 18e eeuw."@nl ;
  rdfs:isDefinedBy <https://w3id.org/con-tax/components/aat-furn> ;
  rdfs:label "porters' chair"@nl ;
  rdfs:label "porters' chairs"@en ;
  rdfs:label "porters' chairs"@nl ;
  rdfs:seeAlso <http://vocab.getty.edu/aat/300133860> ;
  rdfs:seeAlso wd:Q7231575 ;
  rdfs:subClassOf <https://w3id.org/con-tax/components/aat-furn#300037772> ;
  rdfs:subClassOf <https://w3id.org/con-tax/components/aat-furn#300037776> ;
.
<https://w3id.org/con-tax/components/aat-furn#300133868>
  rdf:type owl:Class ;
  rdfs:comment "Ligstoelen met een veer onder de zitting, zodat de stoel na het achteroverbuigen weer terugklapt. Toegeschreven aan de American Chair Company in Troy in New York, rond 1850."@nl ;
  rdfs:comment "Reclining chairs with a spring concealed under the seat which allows the chairs to recline and then snap into place; attributed to the American Chair Company, Troy, NY, about 1850."@en ;
  rdfs:isDefinedBy <https://w3id.org/con-tax/components/aat-furn> ;
  rdfs:label "centripetal spring chair"@nl ;
  rdfs:label "centripetal spring chairs"@en ;
  rdfs:label "centripetal spring chairs"@nl ;
  rdfs:seeAlso <http://vocab.getty.edu/aat/300133868> ;
  rdfs:seeAlso wd:Q5062760 ;
  rdfs:subClassOf <https://w3id.org/con-tax/components/aat-furn#300038272> ;
  rdfs:subClassOf <https://w3id.org/con-tax/components/aat-furn#300040038> ;
.
<https://w3id.org/con-tax/components/aat-furn#300133874>
  rdf:type owl:Class ;
  rdfs:comment "16th-century English and early 17th-century American stools, usually upholstered and covered with sumptuous fabric and fringe. Term also applied to a variety of small, low stools generally with socketed legs."@en ;
  rdfs:comment "Engelse en Amerikaanse krukken, respectievelijk uit de 16e en het begin van de 17e eeuw, die meestal waren gestoffeerd en bedekt met weelderige stoffen en franjes. De benaming wordt ook gebruikt voor verschillende kleine, lage krukken, meestal met gekraagde poten."@nl ;
  rdfs:isDefinedBy <https://w3id.org/con-tax/components/aat-furn> ;
  rdfs:label "buffet stool"@nl ;
  rdfs:label "buffet stools"@en ;
  rdfs:label "buffet stools"@nl ;
  rdfs:seeAlso <http://vocab.getty.edu/aat/300133874> ;
  rdfs:subClassOf <https://w3id.org/con-tax/components/aat-furn#300038418> ;
.
<https://w3id.org/con-tax/components/aat-furn#300133884>
  rdf:type owl:Class ;
  rdfs:comment "Settles with boards across the tops of the side boards."@en ;
  rdfs:comment "Zittekisten met platen over de bovenkant van de zijplanken."@nl ;
  rdfs:isDefinedBy <https://w3id.org/con-tax/components/aat-furn> ;
  rdfs:label "hooded settles"@en ;
  rdfs:label "overkapte zittekist"@nl ;
  rdfs:label "overkapte zittekisten"@nl ;
  rdfs:seeAlso <http://vocab.getty.edu/aat/300133884> ;
  rdfs:subClassOf <https://w3id.org/con-tax/components/aat-furn#300038532> ;
.
<https://w3id.org/con-tax/components/aat-furn#300133894>
  rdf:type owl:Class ;
  rdfs:comment "A French type of small canape or large chair for two people."@en ;
  rdfs:comment "Een Frans soort kleine canapé of grote stoel  waarop twee mensen kunnen zitten."@nl ;
  rdfs:isDefinedBy <https://w3id.org/con-tax/components/aat-furn> ;
  rdfs:label "marquise (settee)"@nl ;
  rdfs:label "marquise"@nl ;
  rdfs:label "marquises (settees)"@en ;
  rdfs:label "marquises (settees)"@nl ;
  rdfs:label "marquises"@nl ;
  rdfs:seeAlso <http://vocab.getty.edu/aat/300133894> ;
  rdfs:subClassOf <https://w3id.org/con-tax/components/aat-furn#300038595> ;
  rdfs:subClassOf <https://w3id.org/con-tax/components/aat-furn#300038636> ;
.
<https://w3id.org/con-tax/components/aat-furn#300133901>
  rdf:type owl:Class ;
  rdfs:comment "Rustbanken met een hoge rugleuning en scharnierende armleuningen die verticaal staan of schuin oplopen vanuit de zitting. Ze zijn genoemd naar het unieke eerste exemlaar uit Knole Park in Kent en waren populair bij de rijke provincialen van Engeland in de jaren twintig en dertig van deze eeuw."@nl ;
  rdfs:comment "Settees with high backs and hinged arms that may be upright or sloped out from the seat, named after the unique early specimen at Knole Park, Kent; popular for rich suburban furnishings in England in the 1920s and 1930s."@en ;
  rdfs:isDefinedBy <https://w3id.org/con-tax/components/aat-furn> ;
  rdfs:label "Knole settee"@nl ;
  rdfs:label "Knole settees"@en ;
  rdfs:label "Knole settees"@nl ;
  rdfs:seeAlso <http://vocab.getty.edu/aat/300133901> ;
  rdfs:subClassOf <https://w3id.org/con-tax/components/aat-furn#300038595> ;
.
<https://w3id.org/con-tax/components/aat-furn#300133904>
  rdf:type owl:Class ;
  rdfs:comment "Asymmetrical seating forms with gently curved backs and having one arm higher than the other; made especially during the French Empire period."@en ;
  rdfs:comment "Asymmetrisch zitmeubel met een licht gewelfde rugleuning en armleuningen van verschillende hoogtes. Ze werden vooral tijdens de Franse Empire-periode gemaakt."@nl ;
  rdfs:isDefinedBy <https://w3id.org/con-tax/components/aat-furn> ;
  rdfs:label "meridienne"@nl ;
  rdfs:label "meridiennes"@nl ;
  rdfs:label "méridiennes"@en ;
  rdfs:seeAlso <http://vocab.getty.edu/aat/300133904> ;
  rdfs:subClassOf <https://w3id.org/con-tax/components/aat-furn#300038493> ;
.
<https://w3id.org/con-tax/components/aat-furn#300133909>
  rdf:type owl:Class ;
  rdfs:comment "Algemene naam voor lage kisten met laden die aan elke kant handvatten hebben om ze aan op te tillen."@nl ;
  rdfs:comment "Popular name for low chests of drawers having handles on each end for lifting."@en ;
  rdfs:isDefinedBy <https://w3id.org/con-tax/components/aat-furn> ;
  rdfs:label "campagnekist"@nl ;
  rdfs:label "campagnekisten"@nl ;
  rdfs:label "campaign chests"@en ;
  rdfs:seeAlso <http://vocab.getty.edu/aat/300133909> ;
  rdfs:subClassOf <https://w3id.org/con-tax/components/aat-furn#300038992> ;
.
<https://w3id.org/con-tax/components/aat-furn#300134005>
  rdf:type owl:Class ;
  rdfs:comment "Boxy tables or case pieces on tall legs, used for serving food. Characterized by having no lower shelf, and occasionally drawers. Originally used outdoors for serving hunting parties."@en ;
  rdfs:comment "Dressoirtafels zonder laden of met een enkele rij laden onder het blad. Dit type wordt gemaakt in de zuidelijke staten van Noord-Amerika."@nl ;
  rdfs:isDefinedBy <https://w3id.org/con-tax/components/aat-furn> ;
  rdfs:label "huntboard"@nl ;
  rdfs:label "huntboards"@en ;
  rdfs:label "huntboards"@nl ;
  rdfs:seeAlso <http://vocab.getty.edu/aat/300134005> ;
  rdfs:subClassOf <https://w3id.org/con-tax/components/aat-furn#300039306> ;
.
<https://w3id.org/con-tax/components/aat-furn#300134010>
  rdf:type owl:Class ;
  rdfs:comment "Schrijftafels die vaak een verschuifbaar, met leer bedekt blad hebben en soms een verstelbaar, scharnierend paneel om op te lezen. Te onderscheiden van 'bureaux plats' doordat ze kleiner zijn."@nl ;
  rdfs:comment "Writing tables often with a leather-covered slide and sometimes with an adjustable hinged panel for reading. Distinguished from \"bureaux plats\" by their much smaller size."@en ;
  rdfs:isDefinedBy <https://w3id.org/con-tax/components/aat-furn> ;
  rdfs:label "table à écrire"@nl ;
  rdfs:label "tables à écrire (leather-covered writing tables)"@en ;
  rdfs:label "tables à écrire"@nl ;
  rdfs:seeAlso <http://vocab.getty.edu/aat/300134010> ;
  rdfs:subClassOf <https://w3id.org/con-tax/components/aat-furn#300039436> ;
.
<https://w3id.org/con-tax/components/aat-furn#300134019>
  rdf:type owl:Class ;
  rdfs:comment "Long dining tables popular 16th-17th centuries, so-called because they resemble tables used in a refectory, although they were not necessarily actually used in a refectory. Typical examples are oblong tables with four or six turned legs that may be expanded by leaves."@en ;
  rdfs:isDefinedBy <https://w3id.org/con-tax/components/aat-furn> ;
  rdfs:label "refectory tables"@en ;
  rdfs:label "reftertafel"@nl ;
  rdfs:label "reftertafels"@nl ;
  rdfs:seeAlso <http://vocab.getty.edu/aat/300134019> ;
  rdfs:seeAlso wd:Q7307089 ;
  rdfs:subClassOf <https://w3id.org/con-tax/components/aat-furn#300039548> ;
.
<https://w3id.org/con-tax/components/aat-furn#300134034>
  rdf:type owl:Class ;
  rdfs:comment "Kleine, lage tafels met box stretchers en meestal gedraaide poten en overhangende tafelbladen. Ze zijn ontworpen voor algemeen huishoudelijk gebruik en niet noodzakelijk voor kroegen."@nl ;
  rdfs:comment "Small, low tables with box stretchers and, generally, turned legs and overhanging tops; designed for a variety of domestic uses, not necessarily exclusively for taverns."@en ;
  rdfs:isDefinedBy <https://w3id.org/con-tax/components/aat-furn> ;
  rdfs:label "tavern table"@nl ;
  rdfs:label "tavern tables"@en ;
  rdfs:label "tavern tables"@nl ;
  rdfs:seeAlso <http://vocab.getty.edu/aat/300134034> ;
  rdfs:subClassOf <https://w3id.org/con-tax/components/aat-furn#300039548> ;
.
<https://w3id.org/con-tax/components/aat-furn#300134053>
  rdf:type owl:Class ;
  rdfs:comment "Historische benaming voor 18e-eeuwse tafels met een marmeren tafelblad. Gebruik 'mengtafels' voor tafels met een marmeren tafelblad met een opbouw waarin laden zitten voor wijnkaraffen en een tambourdeksel dat neergerold kan worden om de marmeren plaat te bedekken als de tafel niet wordt gebruikt."@nl ;
  rdfs:comment "Tables having single slab of marble as a top surface. The form was particularly popular in the 18th century."@en ;
  rdfs:isDefinedBy <https://w3id.org/con-tax/components/aat-furn> ;
  rdfs:label "marble slab tables"@en ;
  rdfs:label "slab table"@nl ;
  rdfs:label "slab tables"@nl ;
  rdfs:seeAlso <http://vocab.getty.edu/aat/300134053> ;
  rdfs:subClassOf <https://w3id.org/con-tax/components/aat-furn#300375699> ;
.
<https://w3id.org/con-tax/components/aat-furn#300134066>
  rdf:type owl:Class ;
  rdfs:comment "Precut furniture parts, made of wood generally used for crates, sold in kits to be assembled by the purchaser into tables, chairs, and bookcases at low cost. Designed by Gerrit Rietveld in 1934."@en ;
  rdfs:comment "Van tevoren op maat gemaakte meubelonderdelen, van een houtsoort die meestal werd gebruikt om kratten van te maken.  Ze werden als goedkoop bouwpakket verkocht en door de koper zelf in elkaar gezet tot tafels, stoelen en boekenkasten. Ze zijn ontworpen door Gerrit Rietveld in 1934."@nl ;
  rdfs:isDefinedBy <https://w3id.org/con-tax/components/aat-furn> ;
  rdfs:label "crate furniture"@en ;
  rdfs:label "kratmeubelen"@nl ;
  rdfs:seeAlso <http://vocab.getty.edu/aat/300134066> ;
  rdfs:subClassOf <https://w3id.org/con-tax/components/aat-furn#300040048> ;
.
<https://w3id.org/con-tax/components/aat-furn#300134616>
  rdf:type owl:Class ;
  rdfs:comment "Hangbanken of -bedden die meestal van netwerk of canvas zijn. Ze hangen aan koorden die aan de beide uiteinden zijn bevestigd."@nl ;
  rdfs:comment "Swinging couches or beds usually made of netting or canvas and slung by cords from supports at each end."@en ;
  rdfs:isDefinedBy <https://w3id.org/con-tax/components/aat-furn> ;
  rdfs:label "hammocks"@en ;
  rdfs:label "hangmat"@nl ;
  rdfs:label "hangmatten"@nl ;
  rdfs:seeAlso <http://vocab.getty.edu/aat/300134616> ;
  rdfs:seeAlso wd:Q193823 ;
  rdfs:subClassOf <https://w3id.org/con-tax/components/aat-furn#300037680> ;
.
<https://w3id.org/con-tax/components/aat-furn#300134802>
  rdf:type owl:Class ;
  rdfs:comment "Grote vouwschermen die bescherming tegen tocht bieden."@nl ;
  rdfs:comment "Large folding screens to provide protection against drafts."@en ;
  rdfs:isDefinedBy <https://w3id.org/con-tax/components/aat-furn> ;
  rdfs:label "paravent"@nl ;
  rdfs:label "paravents"@en ;
  rdfs:label "paravents"@nl ;
  rdfs:seeAlso <http://vocab.getty.edu/aat/300134802> ;
  rdfs:subClassOf <https://w3id.org/con-tax/components/aat-furn#300037737> ;
  rdfs:subClassOf <https://w3id.org/con-tax/components/aat-furn#300265156> ;
.
<https://w3id.org/con-tax/components/aat-furn#300134826>
  rdf:type owl:Class ;
  rdfs:comment "Ronde, driepotige tafels met veelal een schuingeplaatst blad met een gevormde schulprand die op de rand van een pastei lijkt."@nl ;
  rdfs:comment "Tripod, often tilt-top, circular tables whose top has a scalloped, molded rim resembling the edges of a pie."@en ;
  rdfs:isDefinedBy <https://w3id.org/con-tax/components/aat-furn> ;
  rdfs:label "piecrust tables"@en ;
  rdfs:label "ronde Chippendale tafel"@nl ;
  rdfs:label "ronde Chippendale tafels"@nl ;
  rdfs:seeAlso <http://vocab.getty.edu/aat/300134826> ;
  rdfs:subClassOf <https://w3id.org/con-tax/components/aat-furn#300039548> ;
.
<https://w3id.org/con-tax/components/aat-furn#300135321>
  rdf:type owl:Class ;
  rdfs:comment "Benaming die meestal wordt gebruikt voor kleine, draagbare tafels waarop eten of drinken voor één persoon kan staan."@nl ;
  rdfs:comment "Term generally applied to small, portable tables designed to hold food or drink for one person."@en ;
  rdfs:isDefinedBy <https://w3id.org/con-tax/components/aat-furn> ;
  rdfs:label "snack tables"@en ;
  rdfs:label "snacktafel"@nl ;
  rdfs:label "snacktafels"@nl ;
  rdfs:seeAlso <http://vocab.getty.edu/aat/300135321> ;
  rdfs:subClassOf <https://w3id.org/con-tax/components/aat-furn#300039548> ;
.
<https://w3id.org/con-tax/components/aat-furn#300135332>
  rdf:type owl:Class ;
  rdfs:comment "Refers to very tall stands, generally carved and gilt, intended to hold candelabras."@en ;
  rdfs:comment "Wordt gebruikt voor zeer hoge standaarden waarop kandelabers staan. Ze zijn meestal met snijwerk versierd en verguld."@nl ;
  rdfs:isDefinedBy <https://w3id.org/con-tax/components/aat-furn> ;
  rdfs:label "torchère (standaard)"@nl ;
  rdfs:label "torchère"@nl ;
  rdfs:label "torchères (standaarden)"@nl ;
  rdfs:label "torchères (stands)"@en ;
  rdfs:label "torchères"@nl ;
  rdfs:seeAlso <http://vocab.getty.edu/aat/300135332> ;
  rdfs:subClassOf <https://w3id.org/con-tax/components/aat-furn#300039767> ;
.
<https://w3id.org/con-tax/components/aat-furn#300136031>
  rdf:type owl:Class ;
  rdfs:comment "Chests of drawers with a secretary drawer at the top."@en ;
  rdfs:comment "Ladenkasten met een laadje voor schrijfbenodigdheden aan de bovenkant."@nl ;
  rdfs:isDefinedBy <https://w3id.org/con-tax/components/aat-furn> ;
  rdfs:label "butlers' desk"@nl ;
  rdfs:label "butlers' desks"@en ;
  rdfs:label "butlers' desks"@nl ;
  rdfs:seeAlso <http://vocab.getty.edu/aat/300136031> ;
  rdfs:subClassOf <https://w3id.org/con-tax/components/aat-furn#300039009> ;
.
<https://w3id.org/con-tax/components/aat-furn#300136379>
  rdf:type owl:Class ;
  rdfs:comment "Bureaus of kisten met een uitsparing in het middenstuk dat meestal door een rij laden aan elke kant wordt geflankeerd."@nl ;
  rdfs:comment "Desks or chests with a recessed center front which is usually flanked on each side by a set of drawers."@en ;
  rdfs:isDefinedBy <https://w3id.org/con-tax/components/aat-furn> ;
  rdfs:label "kneehole bureau"@nl ;
  rdfs:label "kneehole bureaus"@nl ;
  rdfs:label "kneehole desks (recessed center desks)"@en ;
  rdfs:seeAlso <http://vocab.getty.edu/aat/300136379> ;
  rdfs:subClassOf <https://w3id.org/con-tax/components/aat-furn#300039338> ;
.
<https://w3id.org/con-tax/components/aat-furn#300136596>
  rdf:type owl:Class ;
  rdfs:comment "Grote kasten die meestal zeven of meer laden hebben en door een kroonlijst in twee secties zijn verdeeld, waarbij het onderste gedeelte op verhoogde poten staat. Gebruik 'hoge ladenkasten'  voor soortgelijke (minder specifieke) Amerikaanse meubels."@nl ;
  rdfs:comment "Tall case pieces generally having seven or more drawers divided by a cornice into two sections with the lower section supported on raised legs. For the equivalent American pieces, use \"high chests of drawers.\""@en ;
  rdfs:isDefinedBy <https://w3id.org/con-tax/components/aat-furn> ;
  rdfs:label "tallboys (furniture)"@en ;
  rdfs:label "tallboys (meubilair)"@nl ;
  rdfs:label "tallboys"@nl ;
  rdfs:seeAlso <http://vocab.getty.edu/aat/300136596> ;
  rdfs:seeAlso wd:Q7680090 ;
  rdfs:subClassOf <https://w3id.org/con-tax/components/aat-furn#300039009> ;
.
<https://w3id.org/con-tax/components/aat-furn#300136630>
  rdf:type owl:Class ;
  rdfs:comment "Small racks with partitions intended to hold sheet music, books, or loose papers."@en ;
  rdfs:comment "Wordt gebruikt voor kleine rekjes met vakken voor bladmuziek, boeken of losse paperassen."@nl ;
  rdfs:isDefinedBy <https://w3id.org/con-tax/components/aat-furn> ;
  rdfs:label "canterburie (opslagmeubel)"@nl ;
  rdfs:label "canterburie"@nl ;
  rdfs:label "canterburies (opslagmeubels)"@nl ;
  rdfs:label "canterburies (storage furniture)"@en ;
  rdfs:label "canterburies"@nl ;
  rdfs:seeAlso <http://vocab.getty.edu/aat/300136630> ;
  rdfs:subClassOf <https://w3id.org/con-tax/components/aat-furn#300037680> ;
.
<https://w3id.org/con-tax/components/aat-furn#300136635>
  rdf:type owl:Class ;
  rdfs:comment "18th-century term for English stands in the form of a deep partitioned tray on legs intended to be placed near a table to hold plates and cutlery."@en ;
  rdfs:comment "Blad op poten, om naast een tafel te zetten om borden en bestek op te bergen, Engels, 18e eeuw."@nl ;
  rdfs:isDefinedBy <https://w3id.org/con-tax/components/aat-furn> ;
  rdfs:label "canterburies (standaarden)"@nl ;
  rdfs:label "canterburies (stands)"@en ;
  rdfs:label "canterburies"@nl ;
  rdfs:label "canterbury (standaard)"@nl ;
  rdfs:label "canterbury"@nl ;
  rdfs:seeAlso <http://vocab.getty.edu/aat/300136635> ;
  rdfs:subClassOf <https://w3id.org/con-tax/components/aat-furn#300039767> ;
.
<https://w3id.org/con-tax/components/aat-furn#300136637>
  rdf:type owl:Class ;
  rdfs:comment "Kneehole writing or dressing tables."@en ;
  rdfs:comment "Schrijf- of toilettafels met beenruimte."@nl ;
  rdfs:isDefinedBy <https://w3id.org/con-tax/components/aat-furn> ;
  rdfs:label "bureau tables"@en ;
  rdfs:label "bureautafel"@nl ;
  rdfs:label "bureautafels"@nl ;
  rdfs:seeAlso <http://vocab.getty.edu/aat/300136637> ;
  rdfs:subClassOf <https://w3id.org/con-tax/components/aat-furn#300039338> ;
  rdfs:subClassOf <https://w3id.org/con-tax/components/aat-furn#300039436> ;
  rdfs:subClassOf <https://w3id.org/con-tax/components/aat-furn#300039668> ;
.
<https://w3id.org/con-tax/components/aat-furn#300136953>
  rdf:type gvp:GuideTerm ;
  rdfs:isDefinedBy <https://w3id.org/con-tax/components/aat-furn> ;
  rdfs:label "<meubelvorm>"@nl ;
  rdfs:label "<meubilairvorm>"@nl ;
  rdfs:label "<shape for furniture>"@en ;
  rdfs:label "<vorm: meubilair>"@nl ;
  rdfs:label "meubelvorm"@nl ;
  rdfs:label "meubilairvorm"@nl ;
  rdfs:label "vorm: meubilair"@nl ;
  rdfs:seeAlso <http://vocab.getty.edu/aat/300136953> ;
  contax:containsConcept <https://w3id.org/con-tax/components/aat-furn#300136954> ;
  contax:containsConcept <https://w3id.org/con-tax/components/aat-furn#300136959> ;
  contax:containsConcept <https://w3id.org/con-tax/components/aat-furn#300136972> ;
  contax:containsConcept <https://w3id.org/con-tax/components/aat-furn#300136975> ;
  contax:containsConcept <https://w3id.org/con-tax/components/aat-furn#300136977> ;
  contax:containsConcept <https://w3id.org/con-tax/components/aat-furn#300136979> ;
  contax:containsConcept <https://w3id.org/con-tax/components/aat-furn#300136982> ;
  contax:containsConcept <https://w3id.org/con-tax/components/aat-furn#300136990> ;
  contax:containsConcept <https://w3id.org/con-tax/components/aat-furn#300165349> ;
  contax:containsConcept <https://w3id.org/con-tax/components/aat-furn#300264314> ;
.
<https://w3id.org/con-tax/components/aat-furn#300136954>
  rdf:type owl:Class ;
  rdfs:comment "Shape having a flattened curve between convex sections of similar flattened curves, particularly in reference to furniture pieces."@en ;
  rdfs:comment "Te gebruiken om te verwijzen naar meubelstukken met een voorkant waarvan het midden terugwijkt in een afgeplatte ronding tussen convexe delen van soortgelijke afgeplatte rondingen."@nl ;
  rdfs:isDefinedBy <https://w3id.org/con-tax/components/aat-furn> ;
  rdfs:label "blockfront (shape)"@en ;
  rdfs:label "blockfront"@nl ;
  rdfs:seeAlso <http://vocab.getty.edu/aat/300136954> ;
  rdfs:subClassOf <https://w3id.org/con-tax/components/aat-furn#300037680> ;
.
<https://w3id.org/con-tax/components/aat-furn#300136959>
  rdf:type owl:Class ;
  rdfs:comment "Having a rounded, outward bulging, or swelling curved form, particularly referring to furniture having sides and front of this form."@en ;
  rdfs:comment "Voorzien van geronde, naar buiten bollende of zwellende zij- en voorkanten, te gebruiken met betrekking tot meubilair."@nl ;
  rdfs:isDefinedBy <https://w3id.org/con-tax/components/aat-furn> ;
  rdfs:label "bombé"@en ;
  rdfs:label "gerond"@nl ;
  rdfs:seeAlso <http://vocab.getty.edu/aat/300136959> ;
  rdfs:subClassOf <https://w3id.org/con-tax/components/aat-furn#300037680> ;
.
<https://w3id.org/con-tax/components/aat-furn#300136972>
  rdf:type owl:Class ;
  rdfs:comment "Having a central section that projects in front of the side sections, especially used in reference to 18th-century bookcases or cabinets."@en ;
  rdfs:comment "Voorzien van een enigzins vooruitspringend middenstuk; wordt gebruikt met betrekking tot kastmeubilair."@nl ;
  rdfs:isDefinedBy <https://w3id.org/con-tax/components/aat-furn> ;
  rdfs:label "breakfront (shape)"@en ;
  rdfs:label "breakfront"@nl ;
  rdfs:seeAlso <http://vocab.getty.edu/aat/300136972> ;
  rdfs:subClassOf <https://w3id.org/con-tax/components/aat-furn#300037680> ;
.
<https://w3id.org/con-tax/components/aat-furn#300136975>
  rdf:type owl:Class ;
  rdfs:comment "Having an arch in the middle, particularly with reference to desks and tables, where the arch is located over the space where the lap and knees of the seated person; also used with reference to other furniture, coach design, jewelry, architectural elements (such as porches and window design), and other works."@en ;
  rdfs:comment "Met betrekking tot bureaus en tafels: met een boog in het midden, boven de ruimte waar zich de schoot en knieën bevinden van iemand die aan het bureau of de tafel zit."@nl ;
  rdfs:isDefinedBy <https://w3id.org/con-tax/components/aat-furn> ;
  rdfs:label "circular front (shape)"@en ;
  rdfs:label "rondgevormde façade"@nl ;
  rdfs:seeAlso <http://vocab.getty.edu/aat/300136975> ;
  rdfs:subClassOf <https://w3id.org/con-tax/components/aat-furn#300037680> ;
.
<https://w3id.org/con-tax/components/aat-furn#300136977>
  rdf:type owl:Class ;
  rdfs:comment "Having the shape of a semicircle or crescent, particularly as used with reference to furniture, battlements, and other works. Name refers to half-moon."@en ;
  rdfs:comment "Met betrekking tot meubilair: met de vorm van een halve maan."@nl ;
  rdfs:isDefinedBy <https://w3id.org/con-tax/components/aat-furn> ;
  rdfs:label "demi-lune (shape)"@en ;
  rdfs:label "halvemaanvormig"@nl ;
  rdfs:seeAlso <http://vocab.getty.edu/aat/300136977> ;
  rdfs:subClassOf <https://w3id.org/con-tax/components/aat-furn#300037680> ;
.
<https://w3id.org/con-tax/components/aat-furn#300136979>
  rdf:type owl:Class ;
  rdfs:comment "Having one convex and one concave curve, particularly with reference to furniture edges and sides."@en ;
  rdfs:comment "Met betrekking tot randen en zijkanten van meubilair: met één bolle en één holle kromming."@nl ;
  rdfs:isDefinedBy <https://w3id.org/con-tax/components/aat-furn> ;
  rdfs:label "half-serpentine (shape)"@en ;
  rdfs:label "half-serpentine"@nl ;
  rdfs:label "half-serpentinevormig"@nl ;
  rdfs:label "halfkronkelend"@nl ;
  rdfs:label "halfkronkelig"@nl ;
  rdfs:seeAlso <http://vocab.getty.edu/aat/300136979> ;
  rdfs:subClassOf <https://w3id.org/con-tax/components/aat-furn#300037680> ;
.
<https://w3id.org/con-tax/components/aat-furn#300136982>
  rdf:type owl:Class ;
  rdfs:comment "A shape composed of two convex sections and a central concave section, for example with furniture pieces the fronts of which curve inward between outcurved ends and the center. Named for its resemblance to the bow-shaped piece of wood forming a collar for a yoked ox, with the upper ends fastened to the yoke."@en ;
  rdfs:comment "Te gebruiken om meubelstukken te beschrijven waarvan de voorkanten naar binnen buigen tussen naar buiten gebogen einden en het midden."@nl ;
  rdfs:isDefinedBy <https://w3id.org/con-tax/components/aat-furn> ;
  rdfs:label "meander (vorm)"@nl ;
  rdfs:label "meander"@nl ;
  rdfs:label "oxbow (shape)"@en ;
  rdfs:seeAlso <http://vocab.getty.edu/aat/300136982> ;
  rdfs:seeAlso wd:Q209333 ;
  rdfs:subClassOf <https://w3id.org/con-tax/components/aat-furn#300037680> ;
.
<https://w3id.org/con-tax/components/aat-furn#300136990>
  rdf:type owl:Class ;
  rdfs:comment "Having a straight, uncurved and unbent front, particularly as used in reference to the fronts of case furniture, legs of furniture, and architecture."@en ;
  rdfs:comment "Met betrekking tot kastmeubilair: met een rechte, ongebogen voorkant."@nl ;
  rdfs:isDefinedBy <https://w3id.org/con-tax/components/aat-furn> ;
  rdfs:label "straight-front (shape)"@en ;
  rdfs:label "straight-front"@nl ;
  rdfs:seeAlso <http://vocab.getty.edu/aat/300136990> ;
  rdfs:subClassOf <https://w3id.org/con-tax/components/aat-furn#300037680> ;
.
<https://w3id.org/con-tax/components/aat-furn#300137711>
  rdf:type gvp:GuideTerm ;
  rdf:type skos:OrderedCollection ;
  rdfs:isDefinedBy <https://w3id.org/con-tax/components/aat-furn> ;
  rdfs:label "<chairs by location or context>"@en ;
  rdfs:label "<stoel naar locatie of context>"@nl ;
  rdfs:label "<stoelen naar locatie of context>"@nl ;
  rdfs:label "stoel naar locatie of context"@nl ;
  rdfs:label "stoelen naar locatie of context"@nl ;
  rdfs:seeAlso <http://vocab.getty.edu/aat/300137711> ;
  contax:containsConcept <https://w3id.org/con-tax/components/aat-furn#300037837> ;
  contax:containsConcept <https://w3id.org/con-tax/components/aat-furn#300164274> ;
  contax:containsConcept <https://w3id.org/con-tax/components/aat-furn#300435628> ;
  contax:containsGuideTerm <https://w3id.org/con-tax/components/aat-furn#300165327> ;
  contax:containsGuideTerm <https://w3id.org/con-tax/components/aat-furn#300165534> ;
.
<https://w3id.org/con-tax/components/aat-furn#300137869>
  rdf:type owl:Class ;
  rdfs:comment "Kussens, krukjes of plankjes om op te knielen, die vaak vastzitten aan de kerkbanken."@nl ;
  rdfs:comment "Raised cushions, stools, or boards for kneeling, often attached to pews or having an elbow rest or desk attached. Kneelers are found in churches, but also in private chambers, including chapels, bedrooms, and studies."@en ;
  rdfs:isDefinedBy <https://w3id.org/con-tax/components/aat-furn> ;
  rdfs:label "bidbank"@nl ;
  rdfs:label "bidbanken"@nl ;
  rdfs:label "bidbankje"@nl ;
  rdfs:label "bidbankjes"@nl ;
  rdfs:label "kneelers (furniture)"@en ;
  rdfs:seeAlso <http://vocab.getty.edu/aat/300137869> ;
  rdfs:subClassOf <https://w3id.org/con-tax/components/aat-furn#300037680> ;
.
<https://w3id.org/con-tax/components/aat-furn#300138112>
  rdf:type owl:Class ;
  rdfs:comment "Commode-achtige bureaus die voor meerdere doeleinden geschikt zijn, met een reeks laden die mechanisch  vanuit de achterkant omhoog konden worden gebracht."@nl ;
  rdfs:comment "Multipurpose commodelike desks containing a set of drawers which could be mechanically raised from the back section of the piece."@en ;
  rdfs:isDefinedBy <https://w3id.org/con-tax/components/aat-furn> ;
  rdfs:label "secrétaire à la Bourgogne"@nl ;
  rdfs:label "secrétaires à la Bourgogne"@en ;
  rdfs:label "secrétaires à la Bourgogne"@nl ;
  rdfs:seeAlso <http://vocab.getty.edu/aat/300138112> ;
  rdfs:subClassOf <https://w3id.org/con-tax/components/aat-furn#300039338> ;
  rdfs:subClassOf <https://w3id.org/con-tax/components/aat-furn#300265064> ;
.
<https://w3id.org/con-tax/components/aat-furn#300138142>
  rdf:type owl:Class ;
  rdfs:comment "Gestoffeerde stoelen met een lage zitting en zeer hoge rugleuning die naast of voor het haardvuur worden geplaatst"@nl ;
  rdfs:comment "Upholstered chairs with low seats and very high backs placed either beside or in front of the fire."@en ;
  rdfs:isDefinedBy <https://w3id.org/con-tax/components/aat-furn> ;
  rdfs:label "chauffeuse"@nl ;
  rdfs:label "chauffeuses"@en ;
  rdfs:label "chauffeuses"@nl ;
  rdfs:seeAlso <http://vocab.getty.edu/aat/300138142> ;
  rdfs:subClassOf <https://w3id.org/con-tax/components/aat-furn#300037772> ;
.
<https://w3id.org/con-tax/components/aat-furn#300138244>
  rdf:type owl:Class ;
  rdfs:comment "Bedden die overdwars tegen de muur staan en een koepelvormig baldakijn hebben dat wordt ondersteund door ijzeren roedes die vanaf de hoeken van het hoofdeinde omhoog buigen. De roedes zijn niet zichtbaar door de bedbekleding."@nl ;
  rdfs:comment "Beds having dome-shaped testers supported by rods, often of iron, curving up from the corners of the head boards, with the rods being hidden by the bed hangings. Developed in the 18th century, such beds were often meant to stand in a deep niche in the bedroom of the main apartment of a palace or mansion. In other installations, the bed are often placed with one side lengthwise flush against a wall."@en ;
  rdfs:isDefinedBy <https://w3id.org/con-tax/components/aat-furn> ;
  rdfs:label "lit à la polonaise"@nl ;
  rdfs:label "lits à la polonaise"@en ;
  rdfs:label "lits à la polonaise"@nl ;
  rdfs:seeAlso <http://vocab.getty.edu/aat/300138244> ;
  rdfs:subClassOf <https://w3id.org/con-tax/components/aat-furn#300038737> ;
.
<https://w3id.org/con-tax/components/aat-furn#300138247>
  rdf:type owl:Class ;
  rdfs:comment "Franse benaming uit de 18e eeuw die wordt gebruikt voor indrukwekkende staatsbedden in ceremoniële slaapkamers van koninklijke verblijfplaatsen; niet bedoeld om in te slapen."@nl ;
  rdfs:comment "Magnificent state beds used in the ceremonial bedrooms of a noble or royal residence, coined in 18th-century French usage. Such beds were not intended to be used for routine sleeping, but for example, for the display of a royal newborn with his mother, of the sick or dying monarch, etc."@en ;
  rdfs:isDefinedBy <https://w3id.org/con-tax/components/aat-furn> ;
  rdfs:label "lit de parade"@nl ;
  rdfs:label "lits de parade"@en ;
  rdfs:label "lits de parade"@nl ;
  rdfs:seeAlso <http://vocab.getty.edu/aat/300138247> ;
  rdfs:subClassOf <https://w3id.org/con-tax/components/aat-furn#300038771> ;
.
<https://w3id.org/con-tax/components/aat-furn#300138251>
  rdf:type owl:Class ;
  rdfs:comment "Bedden met twee uiteindes van gelijke hoogte waarbij ieder eind is afgewerkt met krullen."@nl ;
  rdfs:comment "Beds with two ends of equal height, with each end overscrolled."@en ;
  rdfs:isDefinedBy <https://w3id.org/con-tax/components/aat-furn> ;
  rdfs:label "lit en bateau"@nl ;
  rdfs:label "lits en bateau"@en ;
  rdfs:label "lits en bateau"@nl ;
  rdfs:seeAlso <http://vocab.getty.edu/aat/300138251> ;
  rdfs:subClassOf <https://w3id.org/con-tax/components/aat-furn#300038758> ;
.
<https://w3id.org/con-tax/components/aat-furn#300138256>
  rdf:type owl:Class ;
  rdfs:comment "Kleine tafels die verschillende rijen laden boven elkaar hebben en meestal op hoge poten staan."@nl ;
  rdfs:comment "Small tables containing several tiers of drawers and generally set on tall legs."@en ;
  rdfs:isDefinedBy <https://w3id.org/con-tax/components/aat-furn> ;
  rdfs:label "petites commode"@nl ;
  rdfs:label "petites commodes"@en ;
  rdfs:label "petites commodes"@nl ;
  rdfs:seeAlso <http://vocab.getty.edu/aat/300138256> ;
  rdfs:subClassOf <https://w3id.org/con-tax/components/aat-furn#300077277> ;
.
<https://w3id.org/con-tax/components/aat-furn#300138411>
  rdf:type owl:Class ;
  rdfs:comment "Elaborate mechanical tables that could sink or rise through the floor to be replenished with food."@en ;
  rdfs:comment "Ingenieuze tafels die mechanisch door de vloer omhoog en omlaag gebracht konden worden om het voedsel aan te vullen."@nl ;
  rdfs:isDefinedBy <https://w3id.org/con-tax/components/aat-furn> ;
  rdfs:label "tables volante"@nl ;
  rdfs:label "tables volantes"@en ;
  rdfs:label "tables volantes"@nl ;
  rdfs:seeAlso <http://vocab.getty.edu/aat/300138411> ;
  rdfs:subClassOf <https://w3id.org/con-tax/components/aat-furn#300039548> ;
  rdfs:subClassOf <https://w3id.org/con-tax/components/aat-furn#300040036> ;
.
<https://w3id.org/con-tax/components/aat-furn#300139388>
  rdf:type owl:Class ;
  rdfs:comment "Refers to English and European desks with a steeply sloping lid (usually a 45-degree angle) surmounted by a bookcase. For similar American examples use \"desks and bookcases.\" The furniture type developed from the bureau. In the early 18th century one form of bureau comrpised drawers below a sloping writing flap, resting on cabriole legs. Many bureaus of this period and earlier were surmounted by a bookcase, often enclosed by glazed or unglazed doors. Dutch furniture makers developed the form, creating the \"bureau-bookcase,\" which was often fitted with an ingenious combination of drawers and compartments. It became very popular, and spread to other parts of Europe. "@en ;
  rdfs:comment "Verwijst naar Engelse en andere Europese bureaus met een zeer schuin geplaatst schrijfblad (meestal onder een hoek van 45 graden) met daarboven een boekenkast. Gebruik 'desks and bookcases' voor soortgelijke Amerikaanse voorbeelden. Dit meubeltype heeft zich ontwikkeld uit het bureau. Aan het begin van de 18de eeuw bestond er een type bureau dat bestond uit laden onder een schuin aflopend schrijfblad, geplaatst op cabriolepoten. Op veel bureaus uit deze periode en eerder was een boekenkast geplaatst, vaak met al dan niet beglaasde deuren. Hollandse meubelmakers werkten de vorm verder uit en creëerden zo de 'bureau-boekenkast', die vaak is voorzien van een vernuftige combinatie van laden en vakken. Dit type bureau werd zeer populair en verspreidde zich ook naar andere delen van Europa."@nl ;
  rdfs:isDefinedBy <https://w3id.org/con-tax/components/aat-furn> ;
  rdfs:label "bureau-boekenkasten"@nl ;
  rdfs:label "bureau-bookcase"@nl ;
  rdfs:label "bureau-bookcases"@en ;
  rdfs:seeAlso <http://vocab.getty.edu/aat/300139388> ;
  rdfs:subClassOf <https://w3id.org/con-tax/components/aat-furn#300039347> ;
.
<https://w3id.org/con-tax/components/aat-furn#300139419>
  rdf:type owl:Class ;
  rdfs:comment "Ancient Roman couches, of a variety of forms, but generally having turned legs and often having both head and foot boards."@en ;
  rdfs:comment "Oud-Romeinse rustbanken die in verschillende vormen voorkomen maar meestal gedraaide poten en vaak zowel een plank aan het hoofd- als aan het voeteneinde hebben."@nl ;
  rdfs:isDefinedBy <https://w3id.org/con-tax/components/aat-furn> ;
  rdfs:label "lecti"@en ;
  rdfs:label "lecti"@nl ;
  rdfs:label "lectus"@nl ;
  rdfs:seeAlso <http://vocab.getty.edu/aat/300139419> ;
  rdfs:subClassOf <https://w3id.org/con-tax/components/aat-furn#300038583> ;
.
<https://w3id.org/con-tax/components/aat-furn#300139435>
  rdf:type owl:Class ;
  rdfs:comment "Folding stools having curved legs forming a wide X, no back, and low arms. They were originally easily transportable chairs for magisterial commanders in the field; over time, the seat developed a hieratic significance;  Ancient Roman folding curule stools were used by senators and magistrates. Although often of luxurious construction, the Roman curule was meant to be uncomfortable, symbolizing that the official should carry out his duties in an efficient and timely manner."@en ;
  rdfs:comment "Oud-Romeinse opklapbare krukken die door senatoren en magistraten werden gebruikt."@nl ;
  rdfs:isDefinedBy <https://w3id.org/con-tax/components/aat-furn> ;
  rdfs:label "curule chairs"@en ;
  rdfs:label "sellae curulis"@nl ;
  rdfs:seeAlso <http://vocab.getty.edu/aat/300139435> ;
  rdfs:seeAlso wd:Q1064051 ;
  rdfs:subClassOf <https://w3id.org/con-tax/components/aat-furn#300244761> ;
.
<https://w3id.org/con-tax/components/aat-furn#300139525>
  rdf:type owl:Class ;
  rdfs:comment "15th- and 16th-century groom's chests with a single large compartment; made only in the Catalana region of Spain."@en ;
  rdfs:comment "Kist voor een bruidegom die één grote ruimte bevat. Ze werden alleen in de 15e en 16e eeuw in Catalonië in Spanje gemaakt."@nl ;
  rdfs:isDefinedBy <https://w3id.org/con-tax/components/aat-furn> ;
  rdfs:label "macho"@nl ;
  rdfs:label "macho's"@nl ;
  rdfs:label "machos"@en ;
  rdfs:seeAlso <http://vocab.getty.edu/aat/300139525> ;
  rdfs:subClassOf <https://w3id.org/con-tax/components/aat-furn#300039125> ;
.
<https://w3id.org/con-tax/components/aat-furn#300139530>
  rdf:type owl:Class ;
  rdfs:comment "15th- and 16th-century brides' chests constructed in the Catalonia region of Spain. At one side of its face is a door which conceals a set of drawers to hold small articles. Both inner and outer sides of the lid are decorated."@en ;
  rdfs:comment "Bruidskisten die in de 16e en 17e eeuw werden gemaakt in Catalonië in Spanje. Aan de voorkant van de kist zit links of rechts een deur met een aantal laden erachter, waarin kleine spulletjes worden opgeborgen. Zowel de binnen- als de buitenkant van het deksel zijn versierd."@nl ;
  rdfs:isDefinedBy <https://w3id.org/con-tax/components/aat-furn> ;
  rdfs:label "hembra"@nl ;
  rdfs:label "hembra's"@nl ;
  rdfs:label "hembras"@en ;
  rdfs:seeAlso <http://vocab.getty.edu/aat/300139530> ;
  rdfs:subClassOf <https://w3id.org/con-tax/components/aat-furn#300039125> ;
.
<https://w3id.org/con-tax/components/aat-furn#300139541>
  rdf:type owl:Class ;
  rdfs:comment "Grote kasten met drie verdiepingen die met inlegwerk zijn versierd, waarbij een blad tussen twee wandkasten inzit. Ze zijn tijdens de 17e eeuw in Spanje gebouwd. De bovenste laag heeft spijlen ter ventilatie en vormt zo een kast voor fruit, kaas en brood."@nl ;
  rdfs:comment "Tall, three-storied cabinets consisting of a desk between two cupboards and typically decorated with inlay, built in Spain during the 17th century. The name refers to the spindled top story, which form a ventilated food cupboard for fruit, cheese, and bread."@en ;
  rdfs:isDefinedBy <https://w3id.org/con-tax/components/aat-furn> ;
  rdfs:label "fresquera"@nl ;
  rdfs:label "fresqueras"@en ;
  rdfs:label "fresqueras"@nl ;
  rdfs:seeAlso <http://vocab.getty.edu/aat/300139541> ;
  rdfs:subClassOf <https://w3id.org/con-tax/components/aat-furn#300039218> ;
.
<https://w3id.org/con-tax/components/aat-furn#300139717>
  rdf:type owl:Class ;
  rdfs:comment "Strong chests, coffers, bins, boxes, close baskets, or similar tightly covered receptacles, generally made of wood and distinguished by having particularly strong, durable, and often water-tight construction. Used to store food or articles of great value."@en ;
  rdfs:comment "Verschillende kasten, koffers en andere bedekte vergaarplaatsen die meestal sterk en duurzaam zijn gemaakt. Ze worden gebruikt om waardevolle artikelen in op te bergen, zoals de Thorarollen in synagoges."@nl ;
  rdfs:isDefinedBy <https://w3id.org/con-tax/components/aat-furn> ;
  rdfs:label "ark (kastmeubilair)"@nl ;
  rdfs:label "ark"@nl ;
  rdfs:label "arken (kastmeubilair)"@nl ;
  rdfs:label "arken"@nl ;
  rdfs:label "arks (case furniture)"@en ;
  rdfs:seeAlso <http://vocab.getty.edu/aat/300139717> ;
  rdfs:subClassOf <https://w3id.org/con-tax/components/aat-furn#300038860> ;
  rdfs:subClassOf <https://w3id.org/con-tax/components/aat-furn#300038992> ;
  rdfs:subClassOf <https://w3id.org/con-tax/components/aat-furn#300039119> ;
.
<https://w3id.org/con-tax/components/aat-furn#300139728>
  rdf:type owl:Class ;
  rdfs:comment "Eenvoudige kisten uit zes platen die samen zijn gevoegd, gelapt, gespijkerd en van scharnieren voorzien. Ze vormen een goedkoop alternatief voor kisten van schrijnwerk."@nl ;
  rdfs:comment "Simple chests constructed of six boards butted, lapped, nailed, and hinged together; an economical alternative to joined chests."@en ;
  rdfs:isDefinedBy <https://w3id.org/con-tax/components/aat-furn> ;
  rdfs:label "board chests"@en ;
  rdfs:label "planken kist"@nl ;
  rdfs:label "planken kisten"@nl ;
  rdfs:seeAlso <http://vocab.getty.edu/aat/300139728> ;
  rdfs:subClassOf <https://w3id.org/con-tax/components/aat-furn#300038992> ;
.
<https://w3id.org/con-tax/components/aat-furn#300139745>
  rdf:type owl:Class ;
  rdfs:comment "Lage tafels, vaak met een opzetje langs de rand, die een kast, kist of ander meubelstuk horen te ondersteunen. Ze zijn bestemd om tegen een wand aan te staan en zijn daarom meestal aan één kant onversierd."@nl ;
  rdfs:comment "Low tables, often with a raised rim around the edge, intended to support a cabinet, chest, or other piece of case furniture. Intended to stand against a wall, and thus usually undecorated on one side."@en ;
  rdfs:isDefinedBy <https://w3id.org/con-tax/components/aat-furn> ;
  rdfs:label "cabinet stands"@en ;
  rdfs:label "kabinetstandaard"@nl ;
  rdfs:label "kabinetstandaarden"@nl ;
  rdfs:seeAlso <http://vocab.getty.edu/aat/300139745> ;
  rdfs:subClassOf <https://w3id.org/con-tax/components/aat-furn#300039767> ;
.
<https://w3id.org/con-tax/components/aat-furn#300139992>
  rdf:type owl:Class ;
  rdfs:comment "Design which originally appeared in Chippendale's Director for garden tables with a top carved in the form of an open scallop shell; often silver gilt or painted to look like mother of pearl."@en ;
  rdfs:comment "Ontwerp dat oorspronkelijk in Chippendale's Director verscheen. De tuintafels hebben een tafelblad in de vorm van een open sint-jacobsschelp. Vaak zijn ze verzilverd of beschilderd zodat ze op parelmoer lijken"@nl ;
  rdfs:isDefinedBy <https://w3id.org/con-tax/components/aat-furn> ;
  rdfs:label "grotto tables"@en ;
  rdfs:label "grottotafel"@nl ;
  rdfs:label "grottotafels"@nl ;
  rdfs:seeAlso <http://vocab.getty.edu/aat/300139992> ;
  rdfs:subClassOf <https://w3id.org/con-tax/components/aat-furn#300039548> ;
.
<https://w3id.org/con-tax/components/aat-furn#300139997>
  rdf:type owl:Class ;
  rdfs:comment "Design which originally appeared in Chippendale's Director for chairs with a back in the form of an open scallop shell; often decorated in silver gilt or painted to look like mother of pearl."@en ;
  rdfs:comment "Ontwerp dat oorspronkelijk in Chippendale's gids voor stoelen verscheen, met een rugleuning in de vorm van een open kamschelp. Ze worden vaak met zilververguldsel versierd of zo geschilderd dat ze op parelmoer lijken."@nl ;
  rdfs:isDefinedBy <https://w3id.org/con-tax/components/aat-furn> ;
  rdfs:label "grotto chairs"@en ;
  rdfs:label "grottostoel"@nl ;
  rdfs:label "grottostoelen"@nl ;
  rdfs:seeAlso <http://vocab.getty.edu/aat/300139997> ;
  rdfs:subClassOf <https://w3id.org/con-tax/components/aat-furn#300037772> ;
.
<https://w3id.org/con-tax/components/aat-furn#300140010>
  rdf:type owl:Class ;
  rdfs:comment "Eenvoudige stoelen die bestaan uit een platte, rechthoekige zitting, vier dunne rechte poten en een rugleuning die bestaat uit een plank die in een gleuf in de zitting wordt gevoegd."@nl ;
  rdfs:comment "Simple chairs consisting of a slab seat, four stick legs, and a plank back inserted into a slot in the seat."@en ;
  rdfs:isDefinedBy <https://w3id.org/con-tax/components/aat-furn> ;
  rdfs:label "board chairs"@en ;
  rdfs:label "plankenstoel"@nl ;
  rdfs:label "plankenstoelen"@nl ;
  rdfs:seeAlso <http://vocab.getty.edu/aat/300140010> ;
  rdfs:subClassOf <https://w3id.org/con-tax/components/aat-furn#300037772> ;
.
<https://w3id.org/con-tax/components/aat-furn#300140021>
  rdf:type owl:Class ;
  rdfs:comment "Kisten met panelen bekleed die vaak als voetstuk voor kasten worden gebruikt."@nl ;
  rdfs:comment "Paneled chests often used as cabinet stands."@en ;
  rdfs:isDefinedBy <https://w3id.org/con-tax/components/aat-furn> ;
  rdfs:label "taquillóne"@nl ;
  rdfs:label "taquillónes"@en ;
  rdfs:label "taquillónes"@nl ;
  rdfs:seeAlso <http://vocab.getty.edu/aat/300140021> ;
  rdfs:subClassOf <https://w3id.org/con-tax/components/aat-furn#300038992> ;
.
<https://w3id.org/con-tax/components/aat-furn#300140023>
  rdf:type owl:Class ;
  rdfs:comment "Small ladies writing desks with cabriole legs, mounted with drawers or compartments, and with a pull-out writing surface."@en ;
  rdfs:isDefinedBy <https://w3id.org/con-tax/components/aat-furn> ;
  rdfs:label "bureau de dame"@nl ;
  rdfs:label "bureaux de dame"@en ;
  rdfs:label "bureaux de dame"@nl ;
  rdfs:seeAlso <http://vocab.getty.edu/aat/300140023> ;
  rdfs:subClassOf <https://w3id.org/con-tax/components/aat-furn#300039470> ;
.
<https://w3id.org/con-tax/components/aat-furn#300140027>
  rdf:type owl:Class ;
  rdfs:comment "Pliants die een rugleuning met uitsteeksels hadden die vaak naar voren waren gebogen zodat ze op parkieten leken. Ze kwamen in het begin van de 17e eeuw in Frankrijk in de mode en werden voornamelijk gebruikt bij eettafels."@nl ;
  rdfs:comment "Pliants having a back with finials, which were often hooked forward and made to resemble parakeets (thus the name). Came into fashion in France in the early 17th century; principally used at dining tables."@en ;
  rdfs:isDefinedBy <https://w3id.org/con-tax/components/aat-furn> ;
  rdfs:label "perroquet"@nl ;
  rdfs:label "perroquets"@en ;
  rdfs:label "perroquets"@nl ;
  rdfs:seeAlso <http://vocab.getty.edu/aat/300140027> ;
  rdfs:subClassOf <https://w3id.org/con-tax/components/aat-furn#300038478> ;
  rdfs:subClassOf <https://w3id.org/con-tax/components/aat-furn#300039648> ;
.
<https://w3id.org/con-tax/components/aat-furn#300140114>
  rdf:type owl:Class ;
  rdfs:comment "Duitse variant op de plankenstoel."@nl ;
  rdfs:comment "German variety of the board chair."@en ;
  rdfs:isDefinedBy <https://w3id.org/con-tax/components/aat-furn> ;
  rdfs:label "Brettstuhle"@nl ;
  rdfs:label "Brettstuhls"@en ;
  rdfs:seeAlso <http://vocab.getty.edu/aat/300140114> ;
  rdfs:subClassOf <https://w3id.org/con-tax/components/aat-furn#300140010> ;
.
<https://w3id.org/con-tax/components/aat-furn#300140253>
  rdf:type owl:Class ;
  rdfs:comment "Franse benaming, waarvan de herkomst niet vast staat, voor decoratieve kaarshouders. Het oorspronkelijke type had een rond blad met een standaard in het midden. Ze hadden vaak de vorm van een Moor of, naarmate de interesse in exotica toenam, een negerin of Indiaan. In de periode van Louis XV en Louis XVI werden guéridons  kleine, verplaatsbare tafels."@nl ;
  rdfs:comment "French term of uncertain derivation denoting decorative candlestands; original type had a circular top and a central standard, often in the form of a Moor, or, as the taste for exoticism increased, of a negress or Indian. In Louis XV and Louis XVI periods guéridons became small movable tables."@en ;
  rdfs:isDefinedBy <https://w3id.org/con-tax/components/aat-furn> ;
  rdfs:label "guéridon"@nl ;
  rdfs:label "guéridons"@en ;
  rdfs:label "guéridons"@nl ;
  rdfs:seeAlso <http://vocab.getty.edu/aat/300140253> ;
  rdfs:seeAlso wd:Q1557709 ;
  rdfs:subClassOf <https://w3id.org/con-tax/components/aat-furn#300039587> ;
  rdfs:subClassOf <https://w3id.org/con-tax/components/aat-furn#300039752> ;
  rdfs:subClassOf <https://w3id.org/con-tax/components/aat-furn#300039797> ;
.
<https://w3id.org/con-tax/components/aat-furn#300140296>
  rdf:type owl:Class ;
  rdfs:comment "Compleet uitgeruste kaptafels. De meest kenmerkende 18e-eeuwse versie heeft drie opslaande bladen, waarvan de middelste is uitgerust met een spiegel."@nl ;
  rdfs:comment "Fitted dressing tables. The most typical 18th-century form has three rising flaps, the center one being fitted with a mirror."@en ;
  rdfs:isDefinedBy <https://w3id.org/con-tax/components/aat-furn> ;
  rdfs:label "coiffeuse (tafel)"@nl ;
  rdfs:label "coiffeuse"@nl ;
  rdfs:label "coiffeuses (tables)"@en ;
  rdfs:label "coiffeuses (tafels)"@nl ;
  rdfs:label "coiffeuses"@nl ;
  rdfs:seeAlso <http://vocab.getty.edu/aat/300140296> ;
  rdfs:seeAlso wd:Q2106696 ;
  rdfs:subClassOf <https://w3id.org/con-tax/components/aat-furn#300039677> ;
.
<https://w3id.org/con-tax/components/aat-furn#300141151>
  rdf:type owl:Class ;
  rdfs:comment "Benaming die meestal van toepassing is op verschillende soorten stoelen met een lage zitting."@nl ;
  rdfs:comment "Term generally applied to a variety of different chairs with low seats."@en ;
  rdfs:isDefinedBy <https://w3id.org/con-tax/components/aat-furn> ;
  rdfs:label "damesfauteuil"@nl ;
  rdfs:label "damesfauteuils"@nl ;
  rdfs:label "ladies' chairs"@en ;
  rdfs:seeAlso <http://vocab.getty.edu/aat/300141151> ;
  rdfs:subClassOf <https://w3id.org/con-tax/components/aat-furn#300037772> ;
.
<https://w3id.org/con-tax/components/aat-furn#300141674>
  rdf:type owl:Class ;
  rdfs:comment "Portugese kabinetten die met panelen zijn bekleed en op een voetstuk staan."@nl ;
  rdfs:comment "Portuguese paneled cabinets on stands."@en ;
  rdfs:isDefinedBy <https://w3id.org/con-tax/components/aat-furn> ;
  rdfs:label "contadore"@nl ;
  rdfs:label "contadores"@en ;
  rdfs:label "contadores"@nl ;
  rdfs:seeAlso <http://vocab.getty.edu/aat/300141674> ;
  rdfs:subClassOf <https://w3id.org/con-tax/components/aat-furn#300038896> ;
.
<https://w3id.org/con-tax/components/aat-furn#300141677>
  rdf:type owl:Class ;
  rdfs:comment "Portugese baldakijnbedden met gedraaide onderdelen en houtsnijwerk op het hoofdeinde. Ze hebben meestal gedraaide posten en een rechte of pagodevormige overkapping. Dit type werd in de 16e eeuw gemaakt."@nl ;
  rdfs:comment "Portuguese tester beds with turned elements and carvings on the headboard; generally having turned posts and either a plain or pagoda-shaped tester. Of a type made in the 16th century."@en ;
  rdfs:isDefinedBy <https://w3id.org/con-tax/components/aat-furn> ;
  rdfs:label "cama de bilros"@nl ;
  rdfs:label "camas de bilros"@en ;
  rdfs:label "camas de bilros"@nl ;
  rdfs:seeAlso <http://vocab.getty.edu/aat/300141677> ;
  rdfs:subClassOf <https://w3id.org/con-tax/components/aat-furn#300038737> ;
.
<https://w3id.org/con-tax/components/aat-furn#300141681>
  rdf:type owl:Class ;
  rdfs:comment "Castilian name for small writing tables with hidden places for jewels and other valuables."@en ;
  rdfs:comment "Spaanse naam voor kleine schrijftafels met verborgen ruimten voor juwelen en andere kostbaarheden."@nl ;
  rdfs:isDefinedBy <https://w3id.org/con-tax/components/aat-furn> ;
  rdfs:label "bufetillo"@nl ;
  rdfs:label "bufetillos"@en ;
  rdfs:label "bufetillos"@nl ;
  rdfs:seeAlso <http://vocab.getty.edu/aat/300141681> ;
  rdfs:subClassOf <https://w3id.org/con-tax/components/aat-furn#300039436> ;
.
<https://w3id.org/con-tax/components/aat-furn#300141687>
  rdf:type owl:Class ;
  rdfs:comment "Kleine keukentafeltjes voor het zouten van varkensvlees en het maken van worstjes."@nl ;
  rdfs:comment "Small tables or supported planks dedicated to pork-salting or producing other pork products."@en ;
  rdfs:isDefinedBy <https://w3id.org/con-tax/components/aat-furn> ;
  rdfs:label "tocinera"@nl ;
  rdfs:label "tocinera's"@nl ;
  rdfs:label "tocineras"@en ;
  rdfs:seeAlso <http://vocab.getty.edu/aat/300141687> ;
  rdfs:subClassOf <https://w3id.org/con-tax/components/aat-furn#300039548> ;
.
<https://w3id.org/con-tax/components/aat-furn#300142154>
  rdf:type owl:Class ;
  rdfs:comment "Kleine, Spaanse tafels die meestal in de kamer van een vrouw staan."@nl ;
  rdfs:comment "Small Spanish tables, usually in a woman's room."@en ;
  rdfs:isDefinedBy <https://w3id.org/con-tax/components/aat-furn> ;
  rdfs:label "bufete"@nl ;
  rdfs:label "bufetes"@en ;
  rdfs:label "bufetes"@nl ;
  rdfs:seeAlso <http://vocab.getty.edu/aat/300142154> ;
  rdfs:subClassOf <https://w3id.org/con-tax/components/aat-furn#300039674> ;
.
<https://w3id.org/con-tax/components/aat-furn#300142552>
  rdf:type owl:Class ;
  rdfs:comment "Ancient Roman couches, used for dining and therefore generally lacking head and foot boards."@en ;
  rdfs:comment "Oud-Romeinse rustbanken die worden gebruikt bij het diner en zodoende meestal geen plank aan het hoofd- en voeteneinde hebben."@nl ;
  rdfs:isDefinedBy <https://w3id.org/con-tax/components/aat-furn> ;
  rdfs:label "aanligbed"@nl ;
  rdfs:label "aanligbedden"@nl ;
  rdfs:label "triclinia (banken)"@nl ;
  rdfs:label "triclinia (couches)"@en ;
  rdfs:label "triclinia"@nl ;
  rdfs:label "triclinium (bank)"@nl ;
  rdfs:label "triclinium"@nl ;
  rdfs:seeAlso <http://vocab.getty.edu/aat/300142552> ;
  rdfs:subClassOf <https://w3id.org/con-tax/components/aat-furn#300139419> ;
.
<https://w3id.org/con-tax/components/aat-furn#300142594>
  rdf:type owl:Class ;
  rdfs:comment "Franse bedden die bedoeld zijn om een afzonderlijk baldakijn erboven te hebben. Dit type werd aan het eind van de 17e eeuw gemaakt."@nl ;
  rdfs:comment "French beds meant to have a separate canopy overhead; of a type made in the late 17th century."@en ;
  rdfs:isDefinedBy <https://w3id.org/con-tax/components/aat-furn> ;
  rdfs:label "lit à la romaine"@nl ;
  rdfs:label "lits à la romaine"@en ;
  rdfs:label "lits à la romaine"@nl ;
  rdfs:seeAlso <http://vocab.getty.edu/aat/300142594> ;
  rdfs:subClassOf <https://w3id.org/con-tax/components/aat-furn#300038697> ;
.
<https://w3id.org/con-tax/components/aat-furn#300142721>
  rdf:type owl:Class ;
  rdfs:comment "Kleine tafels met  uitstekende bladen die op slanke poten of beugels met scharnieren steunen."@nl ;
  rdfs:comment "Small tables with extending flaps supported on slender legs, or hinged brackets."@en ;
  rdfs:isDefinedBy <https://w3id.org/con-tax/components/aat-furn> ;
  rdfs:label "fly tables"@en ;
  rdfs:label "uitklaptafel"@nl ;
  rdfs:label "uitklaptafels"@nl ;
  rdfs:seeAlso <http://vocab.getty.edu/aat/300142721> ;
  rdfs:subClassOf <https://w3id.org/con-tax/components/aat-furn#300039933> ;
.
<https://w3id.org/con-tax/components/aat-furn#300142732>
  rdf:type owl:Class ;
  rdfs:comment "Klaptafels met inklapbare poten en een zeer smal middengedeelte. Dit type werd vanaf het begin van de 19e eeuw in Engeland gemaakt."@nl ;
  rdfs:comment "Swing-leg, dropleaf tables with a very narrow central portion; of a type made in England from the early 19th century."@en ;
  rdfs:isDefinedBy <https://w3id.org/con-tax/components/aat-furn> ;
  rdfs:label "Sutherland tables"@en ;
  rdfs:label "Sutherlandtafel"@nl ;
  rdfs:label "Sutherlandtafels"@nl ;
  rdfs:seeAlso <http://vocab.getty.edu/aat/300142732> ;
  rdfs:subClassOf <https://w3id.org/con-tax/components/aat-furn#300039933> ;
.
<https://w3id.org/con-tax/components/aat-furn#300142742>
  rdf:type owl:Class ;
  rdfs:comment "Beds with suspended canopies, rectangular, cone-shaped, or domed, which support curtains that may encompass the head half or the full length of the bed. Use \"tester beds\" for beds having a rooflike component supported on posts."@en ;
  rdfs:comment "Wordt gebruikt voor bedden met een hangende hemel in de vorm van een kegel of koepel met gordijnen die het voeteneind raken en omringen. Gebruik 'baldakijnbedden' voor bedden waarbij een soort dak door posten wordt ondersteund."@nl ;
  rdfs:isDefinedBy <https://w3id.org/con-tax/components/aat-furn> ;
  rdfs:label "canopy beds"@en ;
  rdfs:label "hemelbed"@nl ;
  rdfs:label "hemelbedden"@nl ;
  rdfs:seeAlso <http://vocab.getty.edu/aat/300142742> ;
  rdfs:seeAlso wd:Q3256519 ;
  rdfs:subClassOf <https://w3id.org/con-tax/components/aat-furn#300038697> ;
.
<https://w3id.org/con-tax/components/aat-furn#300142783>
  rdf:type owl:Class ;
  rdfs:comment "Bedden met een eenvoudig, houten raamwerk waaraan de bedbehangsels zijn opgehangen zodat ze een vlakke, rechthoekige 'doos' vormen. De houten onderdelen zijn onzichtbaar, zelfs de posten zijn met stof  bekleed. Gebruik 'sledebedden' voor bedden waarvan de twee uiteindes dezelfde hoogte hebben."@nl ;
  rdfs:comment "Beds with a simple wooden framework, which supports the bed hangings so as to form a plain, rectangular box. No wooden components are visible, even the posts are encased in cloth. Use \"sleigh beds\" for beds with two ends of equal height."@en ;
  rdfs:isDefinedBy <https://w3id.org/con-tax/components/aat-furn> ;
  rdfs:label "Frans bed"@nl ;
  rdfs:label "Franse bedden"@nl ;
  rdfs:label "French beds"@en ;
  rdfs:seeAlso <http://vocab.getty.edu/aat/300142783> ;
  rdfs:subClassOf <https://w3id.org/con-tax/components/aat-furn#300038697> ;
.
<https://w3id.org/con-tax/components/aat-furn#300143690>
  rdf:type owl:Class ;
  rdfs:comment "Lady's writing desks fitted with an adjustable looking glass above."@en ;
  rdfs:comment "Schrijfbureaus voor dames waarboven een verstelbare spiegel zit."@nl ;
  rdfs:isDefinedBy <https://w3id.org/con-tax/components/aat-furn> ;
  rdfs:label "ladies' cabinet dressing table"@nl ;
  rdfs:label "ladies' cabinet dressing tables"@en ;
  rdfs:label "ladies' cabinet dressing tables"@nl ;
  rdfs:seeAlso <http://vocab.getty.edu/aat/300143690> ;
  rdfs:subClassOf <https://w3id.org/con-tax/components/aat-furn#300039411> ;
.
<https://w3id.org/con-tax/components/aat-furn#300143697>
  rdf:type owl:Class ;
  rdfs:comment "Dressing tables with two drawers in the sides which swing out and provide mirrors on a quadrant so that a woman could see herself at any angle."@en ;
  rdfs:comment "Kaptafels met twee laden aan de zijkanten, die uitklappen met een driedelige toiletspiegel erop zodat een vrouw zichzelf van alle kanten kan zien."@nl ;
  rdfs:isDefinedBy <https://w3id.org/con-tax/components/aat-furn> ;
  rdfs:label "Rudd tables"@en ;
  rdfs:label "Rudd-tafel"@nl ;
  rdfs:label "Rudd-tafels"@nl ;
  rdfs:seeAlso <http://vocab.getty.edu/aat/300143697> ;
  rdfs:subClassOf <https://w3id.org/con-tax/components/aat-furn#300039674> ;
.
<https://w3id.org/con-tax/components/aat-furn#300143716>
  rdf:type owl:Class ;
  rdfs:comment "Cases for holding books generally having several shelves enclosed by doors; distinct from \"bookshelves\" which are open shelves for holding books."@en ;
  rdfs:comment "Kasten om boeken in te zetten waarbij meestal meerdere planken door een deur worden ingesloten. Ze verschillen van 'boekenplanken' die een openkast-systeem hebben waar boeken op staan."@nl ;
  rdfs:isDefinedBy <https://w3id.org/con-tax/components/aat-furn> ;
  rdfs:label "boekenkast"@nl ;
  rdfs:label "boekenkasten"@nl ;
  rdfs:label "bookcases"@en ;
  rdfs:seeAlso <http://vocab.getty.edu/aat/300143716> ;
  rdfs:seeAlso wd:Q215857 ;
  rdfs:subClassOf <https://w3id.org/con-tax/components/aat-furn#300038860> ;
.
<https://w3id.org/con-tax/components/aat-furn#300143751>
  rdf:type owl:Class ;
  rdfs:comment "Halfronde tafels die meestal als eettafel worden gebruikt."@nl ;
  rdfs:comment "Semicircular tables, generally used as dining tables."@en ;
  rdfs:isDefinedBy <https://w3id.org/con-tax/components/aat-furn> ;
  rdfs:label "hoefijzervormige tafel"@nl ;
  rdfs:label "hoefijzervormige tafels"@nl ;
  rdfs:label "horseshoe tables"@en ;
  rdfs:seeAlso <http://vocab.getty.edu/aat/300143751> ;
  rdfs:subClassOf <https://w3id.org/con-tax/components/aat-furn#300039548> ;
  rdfs:subClassOf <https://w3id.org/con-tax/components/aat-furn#300039648> ;
.
<https://w3id.org/con-tax/components/aat-furn#300143761>
  rdf:type owl:Class ;
  rdfs:comment "Schrijftafels met vuurscherm om de schrijvende persoon tegen de hitte van het vuur te beschermen."@nl ;
  rdfs:comment "Writing tables with fire screens to protect the writer from the heat of the fire."@en ;
  rdfs:isDefinedBy <https://w3id.org/con-tax/components/aat-furn> ;
  rdfs:label "ladies' screen writing table"@nl ;
  rdfs:label "ladies' screen writing tables"@en ;
  rdfs:label "ladies' screen writing tables"@nl ;
  rdfs:seeAlso <http://vocab.getty.edu/aat/300143761> ;
  rdfs:subClassOf <https://w3id.org/con-tax/components/aat-furn#300039470> ;
.
<https://w3id.org/con-tax/components/aat-furn#300143781>
  rdf:type owl:Class ;
  rdfs:comment "In modern usage, generally refers to small, portable writing desks that first appeared in 16th-century Europe, and were extremely popular in France in the 18th century. They are generally characterized by having a nest of drawers enclosed in a box, often with a sloping front that is hinged along the bottom edge and may be let down to provide a writing platform. An escritoire was placed on top of a table or had its own legs. Formerly, these small portable desks were also called \"secretaries\"; however, in modern usage, the term \"secretaries\" typically refers to larger pieces meant to be placed against a wall."@en ;
  rdfs:comment "Verwijst in het moderne taalgebruik gewoonlijk naar kleine, draagbare schrijfbureaus die voor het eerst in de 16de eeuw verschenen en uiterst populair waren in het Frankrijk van de 18de eeuw. Kenmerkend is met name de aanwezigheid van een stel laden in een kist, meestal met een schuin geplaatst blad dat aan de onderkant met scharnieren vastzit en kan worden neergeklapt om op te schrijven. Vroeger werden deze kleine draagbare schrijfbureaus ook wel aangeduid als 'secretaires', maar in het moderne taalgebruik verwijst 'secretaires' meestal naar grotere meubelstukken die tegen een muur worden geplaatst."@nl ;
  rdfs:isDefinedBy <https://w3id.org/con-tax/components/aat-furn> ;
  rdfs:label "escritoire"@nl ;
  rdfs:label "escritoires (writing desks)"@en ;
  rdfs:label "escritoires"@nl ;
  rdfs:seeAlso <http://vocab.getty.edu/aat/300143781> ;
  rdfs:subClassOf <https://w3id.org/con-tax/components/aat-furn#300039427> ;
.
<https://w3id.org/con-tax/components/aat-furn#300143809>
  rdf:type owl:Class ;
  rdfs:comment "Kleine bureaus met een schuin geplaatst tafelblad om op te schrijven of te lezen. Soms hebben ze een inkpotje of een strooibusje met zand."@nl ;
  rdfs:comment "Small desks generally having a sloping surface for writing or for propping up books for reading; sometimes fitted with an inkwell or pounce box for sand."@en ;
  rdfs:isDefinedBy <https://w3id.org/con-tax/components/aat-furn> ;
  rdfs:label "draagbaar bureau"@nl ;
  rdfs:label "draagbare bureaus"@nl ;
  rdfs:label "portable desks"@en ;
  rdfs:seeAlso <http://vocab.getty.edu/aat/300143809> ;
  rdfs:subClassOf <https://w3id.org/con-tax/components/aat-furn#300039338> ;
.
<https://w3id.org/con-tax/components/aat-furn#300144119>
  rdf:type owl:Class ;
  rdfs:comment "Pivoting fire screens adjusted in position by a thumbscrew on a rod."@en ;
  rdfs:comment "Vuurschermen die om een spil draaien waarbij een duimschroef op een stang de verschillende posities instelt."@nl ;
  rdfs:isDefinedBy <https://w3id.org/con-tax/components/aat-furn> ;
  rdfs:label "écran à pivot"@nl ;
  rdfs:label "écrans à pivot"@en ;
  rdfs:label "écrans à pivot"@nl ;
  rdfs:seeAlso <http://vocab.getty.edu/aat/300144119> ;
  rdfs:subClassOf <https://w3id.org/con-tax/components/aat-furn#300037752> ;
.
<https://w3id.org/con-tax/components/aat-furn#300144135>
  rdf:type owl:Class ;
  rdfs:comment "Late-19th-century, richly upholstered armchairs with little or no frame exposed and usually mounted on a spring platform or having a spring back."@en ;
  rdfs:comment "Wordt gebruikt voor rijk gestoffeerde leunstoelen uit het eind van de 19e eeuw die weinig tot niets van het frame laten zien en meestal op een bodem van springveren zijn gezet of een rugleuning van springveren hebben."@nl ;
  rdfs:isDefinedBy <https://w3id.org/con-tax/components/aat-furn> ;
  rdfs:label "Turkish chairs"@en ;
  rdfs:label "Turkse stoel"@nl ;
  rdfs:label "Turkse stoelen"@nl ;
  rdfs:seeAlso <http://vocab.getty.edu/aat/300144135> ;
  rdfs:subClassOf <https://w3id.org/con-tax/components/aat-furn#300037772> ;
.
<https://w3id.org/con-tax/components/aat-furn#300144145>
  rdf:type owl:Class ;
  rdfs:comment "Ondiepe bureaus met een schuin geplaatst schrijfblad op het onderstel van een boekenkast."@nl ;
  rdfs:comment "Shallow desks with a slant front over a bookcase base."@en ;
  rdfs:isDefinedBy <https://w3id.org/con-tax/components/aat-furn> ;
  rdfs:label "desks-over-bookcase"@nl ;
  rdfs:label "desks-over-bookcases"@en ;
  rdfs:label "desks-over-bookcases"@nl ;
  rdfs:seeAlso <http://vocab.getty.edu/aat/300144145> ;
  rdfs:subClassOf <https://w3id.org/con-tax/components/aat-furn#300039338> ;
.
<https://w3id.org/con-tax/components/aat-furn#300144148>
  rdf:type owl:Class ;
  rdfs:comment "Beglaasde kisten, kasten of kabinetten, waarin de goederen van een winkel worden getoond en beschermd."@nl ;
  rdfs:comment "Glazed boxes, cases, or cabinets, of relatively small size, used for displaying and protecting items in a store, museum, home, or other location. For large, wooden cabinets with drawers, shelves, and doors or a fall front, designed for storing rare collections and popular in the 17th century, use \"display cabinets.\""@en ;
  rdfs:isDefinedBy <https://w3id.org/con-tax/components/aat-furn> ;
  rdfs:label "glazenkast"@nl ;
  rdfs:label "glazenkasten"@nl ;
  rdfs:label "goudkast"@nl ;
  rdfs:label "goudkasten"@nl ;
  rdfs:label "showcases"@en ;
  rdfs:label "tinnekast"@nl ;
  rdfs:label "tinnekasten"@nl ;
  rdfs:label "vitrinekast"@nl ;
  rdfs:label "vitrinekasten"@nl ;
  rdfs:label "zilverkast"@nl ;
  rdfs:label "zilverkasten"@nl ;
  rdfs:seeAlso <http://vocab.getty.edu/aat/300144148> ;
  rdfs:subClassOf <https://w3id.org/con-tax/components/aat-furn#300077356> ;
.
<https://w3id.org/con-tax/components/aat-furn#300144780>
  rdf:type owl:Class ;
  rdfs:comment "Type Franse sofa met een golvende rugleuning die vaak in bij elkaar passende paren wordt gemaakt om aan beide zijden van het haardvuur te plaatsen."@nl ;
  rdfs:comment "Type of French sofa with an undulating back; often made in matching pairs and placed on either side of the fireplace."@en ;
  rdfs:isDefinedBy <https://w3id.org/con-tax/components/aat-furn> ;
  rdfs:label "veilleuse (sofa)"@nl ;
  rdfs:label "veilleuse"@nl ;
  rdfs:label "veilleuses (furniture)"@en ;
  rdfs:label "veilleuses (sofa's)"@nl ;
  rdfs:label "veilleuses"@nl ;
  rdfs:seeAlso <http://vocab.getty.edu/aat/300144780> ;
  rdfs:subClassOf <https://w3id.org/con-tax/components/aat-furn#300038634> ;
.
<https://w3id.org/con-tax/components/aat-furn#300146616>
  rdf:type owl:Class ;
  rdfs:comment "Chairs having interlaced ornamental backs, and that may be perforated or cut in low relief, usually in geometric patterns."@en ;
  rdfs:isDefinedBy <https://w3id.org/con-tax/components/aat-furn> ;
  rdfs:label "fret-back chairs"@en ;
  rdfs:label "fret-backstoel"@nl ;
  rdfs:label "fret-backstoelen"@nl ;
  rdfs:seeAlso <http://vocab.getty.edu/aat/300146616> ;
  rdfs:subClassOf <https://w3id.org/con-tax/components/aat-furn#300037772> ;
.
<https://w3id.org/con-tax/components/aat-furn#300146667>
  rdf:type owl:Class ;
  rdfs:comment "Bureaus met een scharnierend, rond deksel of bedekking, die op een deel van een cilinder lijkt en in de bovenkant van het bureau oprolt. Gebruik 'cilinderbureaus en boekenkasten' voor soortgelijke bureaus waar een boekenkast op staat."@nl ;
  rdfs:comment "Desks with a hinged one-piece round lid or cover that resembles a section of a cylinder and which rolls up into the desk top. For similar desks surmounted by a bookcase use \"cylinder desks and bookcases.\""@en ;
  rdfs:isDefinedBy <https://w3id.org/con-tax/components/aat-furn> ;
  rdfs:label "cylinder fall desk"@nl ;
  rdfs:label "cylinder fall desks"@en ;
  rdfs:label "cylinder fall desks"@nl ;
  rdfs:seeAlso <http://vocab.getty.edu/aat/300146667> ;
  rdfs:subClassOf <https://w3id.org/con-tax/components/aat-furn#300039338> ;
.
<https://w3id.org/con-tax/components/aat-furn#300159126>
  rdf:type owl:Class ;
  rdfs:comment "Office furniture that is a hybrid of cabinet and desk manufactured by Wooton and Company in Indianapolis in the latter part of the 19th century. These are characterized by two locking doors that themselves carry drawers and compartments for storage. When opened, a fall extends to create a writing surface facing an interior of ranged compartments and drawers."@en ;
  rdfs:isDefinedBy <https://w3id.org/con-tax/components/aat-furn> ;
  rdfs:label "Wooton cabinet office secretaries"@en ;
  rdfs:label "Wooton kabinetkantoorsecretaire"@nl ;
  rdfs:label "Wooton kabinetkantoorsecretaires"@nl ;
  rdfs:seeAlso <http://vocab.getty.edu/aat/300159126> ;
  rdfs:subClassOf <https://w3id.org/con-tax/components/aat-furn#300039426> ;
.
<https://w3id.org/con-tax/components/aat-furn#300159130>
  rdf:type owl:Class ;
  rdfs:comment "Desks invented by William S. Wooton in 1875, manufactured by the Wooten Desk Company, and characterized by either a flat or slanted writing surface and a single or double pedestal base; the base contains a hinged or pivoted caselike section which, when opened, reveals dozens of slots, shelves, and pigeonholes."@en ;
  rdfs:comment "Wordt gebruikt voor bureaus die door William S. Wooton in 1875 zijn uitgevonden en door de Wooten Desk Company werden gemaakt. Ze hebben een vlak of schuin geplaatst schrijfblad en een enkel of dubbel onderstel. Het onderstel bevat een scharnierend of draaiend kastachtig gedeelte waarachter tientallen ruimten, planken en vakjes zitten."@nl ;
  rdfs:isDefinedBy <https://w3id.org/con-tax/components/aat-furn> ;
  rdfs:label "rotary desk"@nl ;
  rdfs:label "rotary desks"@en ;
  rdfs:label "rotary desks"@nl ;
  rdfs:seeAlso <http://vocab.getty.edu/aat/300159130> ;
  rdfs:subClassOf <https://w3id.org/con-tax/components/aat-furn#300039426> ;
.
<https://w3id.org/con-tax/components/aat-furn#300161823>
  rdf:type owl:Class ;
  rdfs:comment "Stevige, zware, middelhoge tafels waarop het werk van technici, monteurs of timmerlieden wordt uitgevoerd."@nl ;
  rdfs:comment "Strong heavy waist-high tables on which the work of mechanics, machinists, and carpenters is performed."@en ;
  rdfs:isDefinedBy <https://w3id.org/con-tax/components/aat-furn> ;
  rdfs:label "werkbank"@nl ;
  rdfs:label "werkbanken"@nl ;
  rdfs:label "workbenches"@en ;
  rdfs:seeAlso <http://vocab.getty.edu/aat/300161823> ;
  rdfs:seeAlso wd:Q347690 ;
  rdfs:subClassOf <https://w3id.org/con-tax/components/aat-furn#300039548> ;
.
<https://w3id.org/con-tax/components/aat-furn#300162353>
  rdf:type owl:Class ;
  rdfs:comment "Spaans-renaissancistische variatie op de vargue±os. Papeleras worden gebruikt om paperassen in op te bergen. Ze zijn meestal kleiner dan vargue±os, hebben geen schrijfblad, meestal gedraaide poten en kunnen met ijzer zijn beslagen."@nl ;
  rdfs:comment "Spanish Renaissance variation of vargueños, used for storing papers. They are usually smaller than vargueños and lack a writing lid; generally they have turned feet and may be bound with iron."@en ;
  rdfs:isDefinedBy <https://w3id.org/con-tax/components/aat-furn> ;
  rdfs:label "papelera"@nl ;
  rdfs:label "papeleras"@en ;
  rdfs:label "papeleras"@nl ;
  rdfs:seeAlso <http://vocab.getty.edu/aat/300162353> ;
  rdfs:subClassOf <https://w3id.org/con-tax/components/aat-furn#300038888> ;
.
<https://w3id.org/con-tax/components/aat-furn#300164259>
  rdf:type owl:Class ;
  rdfs:comment "Draagbare krukken met poten die aan elkaar zijn bevestigd met een stevig weefsel dat als zitting dient wanneer de kruk geopend is."@nl ;
  rdfs:comment "Portable stools with joined legs which, when opened, are bound by girth webbing which serves as a seat."@en ;
  rdfs:isDefinedBy <https://w3id.org/con-tax/components/aat-furn> ;
  rdfs:label "fishing stools"@en ;
  rdfs:label "viskruk"@nl ;
  rdfs:label "viskrukken"@nl ;
  rdfs:seeAlso <http://vocab.getty.edu/aat/300164259> ;
  rdfs:seeAlso wd:Q25931055 ;
  rdfs:subClassOf <https://w3id.org/con-tax/components/aat-furn#300244761> ;
.
<https://w3id.org/con-tax/components/aat-furn#300164260>
  rdf:type owl:Class ;
  rdfs:comment "Adjustable highchairs which may be converted into a carriage or walker."@en ;
  rdfs:comment "Verstelbare kinderstoeltjes die tot wagen of loophekje kunnnen worden omgeklapt."@nl ;
  rdfs:isDefinedBy <https://w3id.org/con-tax/components/aat-furn> ;
  rdfs:label "carriage chairs"@en ;
  rdfs:label "klapkinderstoeltje"@nl ;
  rdfs:label "klapkinderstoeltjes"@nl ;
  rdfs:seeAlso <http://vocab.getty.edu/aat/300164260> ;
  rdfs:subClassOf <https://w3id.org/con-tax/components/aat-furn#300038184> ;
.
<https://w3id.org/con-tax/components/aat-furn#300164268>
  rdf:type owl:Class ;
  rdfs:comment "Benaming die in de jaren zestig van de 19e eeuw werd gebruikt voor meubilair dat door bedrijven met toonaangevende ontwerpers en architecten werd gemaakt. De ontwerpen bestonden vooral uit eenvoudige vormen met handgesneden en geschilderde decoraties."@nl ;
  rdfs:comment "Term applied in the 1860s to furniture produced by firms which employed leading designers and architects. Designs tended toward simple forms with hand-carved and painted decoration."@en ;
  rdfs:isDefinedBy <https://w3id.org/con-tax/components/aat-furn> ;
  rdfs:label "art furniture"@en ;
  rdfs:label "kunstmeubilair"@nl ;
  rdfs:seeAlso <http://vocab.getty.edu/aat/300164268> ;
  rdfs:subClassOf <https://w3id.org/con-tax/components/aat-furn#300037680> ;
.
<https://w3id.org/con-tax/components/aat-furn#300164274>
  rdf:type owl:Class ;
  rdfs:comment "Chairs of various form designed to be used in a seaside recreational context. These are often designed to be lightweight, incorporating fabric or wicker, and may have the ability to be broken down and carried."@en ;
  rdfs:isDefinedBy <https://w3id.org/con-tax/components/aat-furn> ;
  rdfs:label "badstoel"@nl ;
  rdfs:label "badstoelen"@nl ;
  rdfs:label "beach chairs"@en ;
  rdfs:label "strandstoel"@nl ;
  rdfs:label "strandstoelen"@nl ;
  rdfs:seeAlso <http://vocab.getty.edu/aat/300164274> ;
  rdfs:seeAlso wd:Q1824203 ;
  rdfs:seeAlso wd:Q766217 ;
  rdfs:subClassOf <https://w3id.org/con-tax/components/aat-furn#300037772> ;
.
<https://w3id.org/con-tax/components/aat-furn#300164278>
  rdf:type owl:Class ;
  rdfs:comment "Seats suspended from a steel framework by links or springs; generally used on porches."@en ;
  rdfs:comment "Stoelen die met schakels of springveren aan een stalen geraamte hangen. Ze worden meestal op veranda's gebruikt."@nl ;
  rdfs:isDefinedBy <https://w3id.org/con-tax/components/aat-furn> ;
  rdfs:label "glider (furniture)"@nl ;
  rdfs:label "glider"@nl ;
  rdfs:label "gliders (furniture)"@en ;
  rdfs:label "gliders (furniture)"@nl ;
  rdfs:label "gliders"@nl ;
  rdfs:seeAlso <http://vocab.getty.edu/aat/300164278> ;
  rdfs:subClassOf <https://w3id.org/con-tax/components/aat-furn#300038493> ;
  rdfs:subClassOf <https://w3id.org/con-tax/components/aat-furn#300165810> ;
.
<https://w3id.org/con-tax/components/aat-furn#300164316>
  rdf:type owl:Class ;
  rdfs:comment "Banken die vaak bijpassend met stoelen of halspiegels worden gemaakt, meestal zonder opvulling en stoffering. Ze zijn bedoeld om in hallen en gallerijen te gebruiken."@nl ;
  rdfs:comment "Benches, generally without padding and upholstery, often made en suite with chairs or hall mirrors and intended for use in halls and galleries."@en ;
  rdfs:isDefinedBy <https://w3id.org/con-tax/components/aat-furn> ;
  rdfs:label "gangbank"@nl ;
  rdfs:label "gangbanken"@nl ;
  rdfs:label "halbank"@nl ;
  rdfs:label "halbanken"@nl ;
  rdfs:label "hall seats"@en ;
  rdfs:seeAlso <http://vocab.getty.edu/aat/300164316> ;
  rdfs:subClassOf <https://w3id.org/con-tax/components/aat-furn#300038494> ;
.
<https://w3id.org/con-tax/components/aat-furn#300164317>
  rdf:type owl:Class ;
  rdfs:comment "Adjustable tables, with ledges at the back and sides, used by persons in bed, usually for eating or writing. Also may refer to tables at the side of a bed. "@en ;
  rdfs:comment "Een klein, veelal niervormig tafeltje, op vier zeer korte pootjes, dat men in bed zittend voor zich kan zetten; het blad kan geheel of gedeeltelijk schuin gezet worden; soms vormt een beddetafel als een los opzetstuk één geheel met een hogere ondertafel met hetzelfde grondplan."@nl ;
  rdfs:isDefinedBy <https://w3id.org/con-tax/components/aat-furn> ;
  rdfs:label "bed tables"@en ;
  rdfs:label "beddetafel"@nl ;
  rdfs:label "beddetafels"@nl ;
  rdfs:label "bedtafel"@nl ;
  rdfs:label "bedtafels"@nl ;
  rdfs:seeAlso <http://vocab.getty.edu/aat/300164317> ;
  rdfs:subClassOf <https://w3id.org/con-tax/components/aat-furn#300039548> ;
.
<https://w3id.org/con-tax/components/aat-furn#300164323>
  rdf:type owl:Class ;
  rdfs:comment "Small stands or cabinets with zinc-lined compartments used to store smoking supplies. Distinct from \"smokers\" which are ashtrays mounted on a low pedestal stand."@en ;
  rdfs:comment "Standaarden of kastjes voor het opbergen van rookgerei. Gebruik 'asbakken' voor rookgerei om as van tabak in op te vangen; ze komen voor in allerlei maten, vormen en uitvoeringen."@nl ;
  rdfs:isDefinedBy <https://w3id.org/con-tax/components/aat-furn> ;
  rdfs:label "rookgereistandaarden"@nl ;
  rdfs:label "rookgereistandaards"@nl ;
  rdfs:label "smoking stands (supply holders)"@en ;
  rdfs:seeAlso <http://vocab.getty.edu/aat/300164323> ;
  rdfs:subClassOf <https://w3id.org/con-tax/components/aat-furn#300039767> ;
.
<https://w3id.org/con-tax/components/aat-furn#300164327>
  rdf:type owl:Class ;
  rdfs:comment "Box stools with a china bowl and cover. Use \"commode chairs\" for chairs having a chamber pot."@en ;
  rdfs:comment "Porseleinen wasstel met deksel. Gebruik 'commodestoelen' voor stoelen met een po."@nl ;
  rdfs:isDefinedBy <https://w3id.org/con-tax/components/aat-furn> ;
  rdfs:label "bidet (draagbaar)"@nl ;
  rdfs:label "bidet"@nl ;
  rdfs:label "bidets (box stools)"@en ;
  rdfs:label "bidets (draagbaar)"@nl ;
  rdfs:label "bidets"@nl ;
  rdfs:seeAlso <http://vocab.getty.edu/aat/300164327> ;
  rdfs:seeAlso wd:Q21550400 ;
  rdfs:subClassOf <https://w3id.org/con-tax/components/aat-furn#300038424> ;
.
<https://w3id.org/con-tax/components/aat-furn#300164329>
  rdf:type owl:Class ;
  rdfs:comment "Deception beds which fold into a dummy bookcase."@en ;
  rdfs:comment "Verborgen bedden die in een schijnboekenkast worden opgeklapt."@nl ;
  rdfs:isDefinedBy <https://w3id.org/con-tax/components/aat-furn> ;
  rdfs:label "boekenkastbed"@nl ;
  rdfs:label "boekenkastbedden"@nl ;
  rdfs:label "bookcase beds"@en ;
  rdfs:seeAlso <http://vocab.getty.edu/aat/300164329> ;
  rdfs:subClassOf <https://w3id.org/con-tax/components/aat-furn#300038803> ;
.
<https://w3id.org/con-tax/components/aat-furn#300164332>
  rdf:type owl:Class ;
  rdfs:comment "Boekenkasten met dichte in plaats van beglaasde deuren."@nl ;
  rdfs:comment "Bookcases having solid, as opposed to glazed, doors."@en ;
  rdfs:isDefinedBy <https://w3id.org/con-tax/components/aat-furn> ;
  rdfs:label "book cupboards"@en ;
  rdfs:label "book cupboards"@nl ;
  rdfs:label "book cupboars"@nl ;
  rdfs:seeAlso <http://vocab.getty.edu/aat/300164332> ;
  rdfs:subClassOf <https://w3id.org/con-tax/components/aat-furn#300143716> ;
.
<https://w3id.org/con-tax/components/aat-furn#300164343>
  rdf:type owl:Class ;
  rdfs:comment "Deception beds that fold into dummy cabinets."@en ;
  rdfs:comment "Verborgen bedden die in schijnkabinetten worden opgeklapt."@nl ;
  rdfs:isDefinedBy <https://w3id.org/con-tax/components/aat-furn> ;
  rdfs:label "cabinet beds"@en ;
  rdfs:label "kabinetbed"@nl ;
  rdfs:label "kabinetbedden"@nl ;
  rdfs:seeAlso <http://vocab.getty.edu/aat/300164343> ;
  rdfs:subClassOf <https://w3id.org/con-tax/components/aat-furn#300038803> ;
.
<https://w3id.org/con-tax/components/aat-furn#300164347>
  rdf:type owl:Class ;
  rdfs:comment "Deception beds that fold into a piece of case furniture that looks like a chiffonier."@en ;
  rdfs:comment "Verborgen bedden die in schijnchiffonnières worden opgeklapt."@nl ;
  rdfs:isDefinedBy <https://w3id.org/con-tax/components/aat-furn> ;
  rdfs:label "chiffonier beds"@en ;
  rdfs:label "chiffonnièrebed"@nl ;
  rdfs:label "chiffonnièrebedden"@nl ;
  rdfs:seeAlso <http://vocab.getty.edu/aat/300164347> ;
  rdfs:seeAlso wd:Q21550465 ;
  rdfs:subClassOf <https://w3id.org/con-tax/components/aat-furn#300038803> ;
.
<https://w3id.org/con-tax/components/aat-furn#300164351>
  rdf:type owl:Class ;
  rdfs:comment "Een soort commodestoel uit het eind van de 19e eeuw die vaak met invaliden wordt geassocieerd en een pot heeft die in een klein kabinet onder de zitting is verborgen. Zulke kabinetten hebben meestal een opening in de rugleuning zodat de pot kan worden verwijderd zonder de patient te storen."@nl ;
  rdfs:comment "Form of late 19th-century commode chair, often associated with invalids, having a chamber pot concealed within a small cabinet under the seat; such cabinets usually have a door in the back so the chamber pot can be removed without disturbing the patient."@en ;
  rdfs:isDefinedBy <https://w3id.org/con-tax/components/aat-furn> ;
  rdfs:label "cabinet chairs"@en ;
  rdfs:label "kabinetstoel"@nl ;
  rdfs:label "kabinetstoelen"@nl ;
  rdfs:seeAlso <http://vocab.getty.edu/aat/300164351> ;
  rdfs:subClassOf <https://w3id.org/con-tax/components/aat-furn#300038155> ;
.
<https://w3id.org/con-tax/components/aat-furn#300164357>
  rdf:type owl:Class ;
  rdfs:comment "Tables with a circular top that expands on an iron frame to allow eight extra leaves to be inserted. It was patented by Robert Jupe in 1835."@en ;
  rdfs:comment "Tafels met een rond blad op een ijzeren raamwerk dat kan worden vergroot om acht extra delen in te voegen. Gepatenteerd in 1835 door Robert Jupe."@nl ;
  rdfs:isDefinedBy <https://w3id.org/con-tax/components/aat-furn> ;
  rdfs:label "capstan table"@nl ;
  rdfs:label "capstan tables"@en ;
  rdfs:label "capstan tables"@nl ;
  rdfs:seeAlso <http://vocab.getty.edu/aat/300164357> ;
  rdfs:subClassOf <https://w3id.org/con-tax/components/aat-furn#300039548> ;
.
<https://w3id.org/con-tax/components/aat-furn#300164361>
  rdf:type owl:Class ;
  rdfs:comment "Kleine standaarden met een schuine bovenkant waarin een naamkaartje kan worden gezet. Dit type werd aan het eind van de 19e eeuw gemaakt."@nl ;
  rdfs:comment "Small stands with a dished top intended to hold calling cards; of a type made in the late 19th century."@en ;
  rdfs:isDefinedBy <https://w3id.org/con-tax/components/aat-furn> ;
  rdfs:label "card stand"@nl ;
  rdfs:label "card stands"@en ;
  rdfs:label "card stands"@nl ;
  rdfs:seeAlso <http://vocab.getty.edu/aat/300164361> ;
  rdfs:subClassOf <https://w3id.org/con-tax/components/aat-furn#300039767> ;
.
<https://w3id.org/con-tax/components/aat-furn#300164365>
  rdf:type owl:Class ;
  rdfs:comment "Cradles with two front wheels for transport."@en ;
  rdfs:comment "Wiegen die twee voorwielen hebben zodat de wieg vervoerbaar is."@nl ;
  rdfs:isDefinedBy <https://w3id.org/con-tax/components/aat-furn> ;
  rdfs:label "carriage cradles"@en ;
  rdfs:label "reiswieg"@nl ;
  rdfs:label "reiswiegen"@nl ;
  rdfs:seeAlso <http://vocab.getty.edu/aat/300164365> ;
  rdfs:subClassOf <https://w3id.org/con-tax/components/aat-furn#300038847> ;
.
<https://w3id.org/con-tax/components/aat-furn#300164367>
  rdf:type owl:Class ;
  rdfs:comment "Standaarden waaraan hoeden kunnen worden gehangen, meestal ook met plaats voor jassen of paraplu's. Over het algemeen zijn ze uitgebreider en vaker vrijstaand dan 'hoedenrekken'."@nl ;
  rdfs:comment "Stands with pegs, hooks, or other devices for hanging hats, often also with places for coats or umbrellas. More elaborate and more likely to be freestanding furniture than \"hat racks.\""@en ;
  rdfs:isDefinedBy <https://w3id.org/con-tax/components/aat-furn> ;
  rdfs:label "hat stands"@en ;
  rdfs:label "hoedenstandaard"@nl ;
  rdfs:label "hoedenstandaarden"@nl ;
  rdfs:seeAlso <http://vocab.getty.edu/aat/300164367> ;
  rdfs:subClassOf <https://w3id.org/con-tax/components/aat-furn#300039767> ;
.
<https://w3id.org/con-tax/components/aat-furn#300164370>
  rdf:type owl:Class ;
  rdfs:comment "Benaming uit de 18e eeuw voor eenvoudige kap- of schrijftafels in de 18e eeuw."@nl ;
  rdfs:comment "Contemporary name for plain dressing or writing tables in the 18th century."@en ;
  rdfs:isDefinedBy <https://w3id.org/con-tax/components/aat-furn> ;
  rdfs:label "chamber tables"@en ;
  rdfs:label "kamertafel"@nl ;
  rdfs:label "kamertafels"@nl ;
  rdfs:seeAlso <http://vocab.getty.edu/aat/300164370> ;
  rdfs:subClassOf <https://w3id.org/con-tax/components/aat-furn#300039436> ;
  rdfs:subClassOf <https://w3id.org/con-tax/components/aat-furn#300039668> ;
.
<https://w3id.org/con-tax/components/aat-furn#300164380>
  rdf:type owl:Class ;
  rdfs:comment "Chests of drawers having a full-length mirror on one side and drawers on the other."@en ;
  rdfs:comment "Ladenkasten met een passpiegel aan de ene kant en laden aan de andere kant."@nl ;
  rdfs:isDefinedBy <https://w3id.org/con-tax/components/aat-furn> ;
  rdfs:label "cheval dresser"@nl ;
  rdfs:label "cheval dressers"@en ;
  rdfs:label "cheval dressers"@nl ;
  rdfs:seeAlso <http://vocab.getty.edu/aat/300164380> ;
  rdfs:subClassOf <https://w3id.org/con-tax/components/aat-furn#300039009> ;
.
<https://w3id.org/con-tax/components/aat-furn#300164386>
  rdf:type owl:Class ;
  rdfs:comment "Een hoog meubelstuk dat meestal aan één zijde is voorzien van laden en aan de andere zijde ruimte bevat voor het ophangen van kleding. De term heeft zijn oorsprong in het zuiden van de Verenigde Staten en is een samenvoeging van 'chiffonier' (chiffonière) en 'wardrobe' (kleerkast)."@nl ;
  rdfs:comment "Tall pieces of furniture typically having drawers on one side and a narrow closet or space for hanging clothes on the other. The term originated in the Southern United States, combining the words \"chiffonier\" and \"wardrobe,\" referring to the two functions of the chifforobe."@en ;
  rdfs:isDefinedBy <https://w3id.org/con-tax/components/aat-furn> ;
  rdfs:label "chifforobe"@nl ;
  rdfs:label "chifforobes"@en ;
  rdfs:label "chifforobes"@nl ;
  rdfs:seeAlso <http://vocab.getty.edu/aat/300164386> ;
  rdfs:seeAlso wd:Q643661 ;
  rdfs:subClassOf <https://w3id.org/con-tax/components/aat-furn#300039009> ;
.
<https://w3id.org/con-tax/components/aat-furn#300164389>
  rdf:type owl:Class ;
  rdfs:comment "Tables having semi-circular or \"U\" shaped surfaces, designed for and used while eating meals in large formal dining rooms."@en ;
  rdfs:isDefinedBy <https://w3id.org/con-tax/components/aat-furn> ;
  rdfs:label "hoefijzervormige dinertafel"@nl ;
  rdfs:label "hoefijzervormige dinertafels"@nl ;
  rdfs:label "horseshoe dining tables"@en ;
  rdfs:seeAlso <http://vocab.getty.edu/aat/300164389> ;
  rdfs:subClassOf <https://w3id.org/con-tax/components/aat-furn#300039648> ;
.
<https://w3id.org/con-tax/components/aat-furn#300164390>
  rdf:type owl:Class ;
  rdfs:comment "Historische benaming die in de 18e eeuw werd gebruikt voor rekken waarop nat wasgoed werd gehangen om te drogen."@nl ;
  rdfs:comment "Racks on which wet laundry is hung for drying or airing, typically an upright wooden frame standing upon legs, with horizontal bars on which clothes are hung."@en ;
  rdfs:isDefinedBy <https://w3id.org/con-tax/components/aat-furn> ;
  rdfs:label "clothes horses"@en ;
  rdfs:label "droogrek"@nl ;
  rdfs:label "droogrekken"@nl ;
  rdfs:seeAlso <http://vocab.getty.edu/aat/300164390> ;
  rdfs:subClassOf <https://w3id.org/con-tax/components/aat-furn#300435395> ;
.
<https://w3id.org/con-tax/components/aat-furn#300164398>
  rdf:type owl:Class ;
  rdfs:comment "Large boxes with hinged lids intended for the storage of clothing, often with built-in or removeable trays used as dividers."@en ;
  rdfs:isDefinedBy <https://w3id.org/con-tax/components/aat-furn> ;
  rdfs:label "clothes chests"@en ;
  rdfs:label "kledingkist"@nl ;
  rdfs:label "kledingkisten"@nl ;
  rdfs:seeAlso <http://vocab.getty.edu/aat/300164398> ;
  rdfs:subClassOf <https://w3id.org/con-tax/components/aat-furn#300038992> ;
.
<https://w3id.org/con-tax/components/aat-furn#300164406>
  rdf:type owl:Class ;
  rdfs:comment "Small low table for resting glasses on in a domestic environment."@en ;
  rdfs:isDefinedBy <https://w3id.org/con-tax/components/aat-furn> ;
  rdfs:label "cocktail tables"@en ;
  rdfs:label "cocktailtafel"@nl ;
  rdfs:label "cocktailtafels"@nl ;
  rdfs:seeAlso <http://vocab.getty.edu/aat/300164406> ;
  rdfs:seeAlso wd:Q2407432 ;
  rdfs:subClassOf <https://w3id.org/con-tax/components/aat-furn#300039548> ;
.
<https://w3id.org/con-tax/components/aat-furn#300164409>
  rdf:type owl:Class ;
  rdfs:comment "Dressing tables fitted with mirrors, compartments for cosmetics, and drawers or cabinets enclosed by doors for the storage of clothing."@en ;
  rdfs:isDefinedBy <https://w3id.org/con-tax/components/aat-furn> ;
  rdfs:label "commode dressing table"@nl ;
  rdfs:label "commode dressing tables"@en ;
  rdfs:label "commode dressing tables"@nl ;
  rdfs:seeAlso <http://vocab.getty.edu/aat/300164409> ;
  rdfs:subClassOf <https://w3id.org/con-tax/components/aat-furn#300039668> ;
.
<https://w3id.org/con-tax/components/aat-furn#300164411>
  rdf:type owl:Class ;
  rdfs:comment "Wash basin stands meant to be situated in spaces where walls meet, and that have closed, rather than open support structures, sometimes fitted with doors for storage."@en ;
  rdfs:isDefinedBy <https://w3id.org/con-tax/components/aat-furn> ;
  rdfs:label "corner enclosed basin stand"@nl ;
  rdfs:label "corner enclosed basin stands"@en ;
  rdfs:label "corner enclosed basin stands"@nl ;
  rdfs:seeAlso <http://vocab.getty.edu/aat/300164411> ;
  rdfs:subClassOf <https://w3id.org/con-tax/components/aat-furn#300039865> ;
.
<https://w3id.org/con-tax/components/aat-furn#300164414>
  rdf:type owl:Class ;
  rdfs:comment "Shelves designed to be mounted in the angle where walls meet. Common types are intended to hold small decorative objects."@en ;
  rdfs:isDefinedBy <https://w3id.org/con-tax/components/aat-furn> ;
  rdfs:label "corner shelves"@en ;
  rdfs:label "hoekplank"@nl ;
  rdfs:label "hoekplanken"@nl ;
  rdfs:seeAlso <http://vocab.getty.edu/aat/300164414> ;
  rdfs:subClassOf <https://w3id.org/con-tax/components/aat-furn#300038860> ;
.
<https://w3id.org/con-tax/components/aat-furn#300164415>
  rdf:type owl:Class ;
  rdfs:comment "Relatively small tables, originally designed to seat customers in ice-cream parlors."@en ;
  rdfs:isDefinedBy <https://w3id.org/con-tax/components/aat-furn> ;
  rdfs:label "ice-cream table"@nl ;
  rdfs:label "ice-cream tables"@en ;
  rdfs:label "ice-cream tables"@nl ;
  rdfs:seeAlso <http://vocab.getty.edu/aat/300164415> ;
  rdfs:subClassOf <https://w3id.org/con-tax/components/aat-furn#300039548> ;
.
<https://w3id.org/con-tax/components/aat-furn#300164419>
  rdf:type owl:Class ;
  rdfs:comment "Upright stands, typically resembling drying racks, with projecting arms or cross bars used to hold clothing in a dressing room or bedroom. The rack is designed so that clothing may be folded across the arms or bars. Pegs may also be included for hanging clothes."@en ;
  rdfs:isDefinedBy <https://w3id.org/con-tax/components/aat-furn> ;
  rdfs:label "costumers (furniture)"@en ;
  rdfs:label "kleedstelling (meubilair)"@nl ;
  rdfs:label "kleedstelling"@nl ;
  rdfs:label "kleedstellingen (meubilair)"@nl ;
  rdfs:label "kleedstellingen"@nl ;
  rdfs:seeAlso <http://vocab.getty.edu/aat/300164419> ;
  rdfs:subClassOf <https://w3id.org/con-tax/components/aat-furn#300039767> ;
.
<https://w3id.org/con-tax/components/aat-furn#300164421>
  rdf:type owl:Class ;
  rdfs:comment "High stools that are usually one of a row of such stools fixed in front of a counter; often backless and having a revolving seat."@en ;
  rdfs:comment "Hoge krukken die meestal deel uitmaken van een reeks dezelfde krukken die voor een toonbank staan. Ze hebben vaak een draaiende zitting en geen rugleuning."@nl ;
  rdfs:isDefinedBy <https://w3id.org/con-tax/components/aat-furn> ;
  rdfs:label "counter stools"@en ;
  rdfs:label "toonbankkruk"@nl ;
  rdfs:label "toonbankkrukken"@nl ;
  rdfs:seeAlso <http://vocab.getty.edu/aat/300164421> ;
  rdfs:subClassOf <https://w3id.org/con-tax/components/aat-furn#300038418> ;
.
<https://w3id.org/con-tax/components/aat-furn#300164425>
  rdf:type owl:Class ;
  rdfs:comment "Wash basin stands that have closed, rather than open support structures, sometimes fitted with doors for storage."@en ;
  rdfs:isDefinedBy <https://w3id.org/con-tax/components/aat-furn> ;
  rdfs:label "enclosed basin stand"@nl ;
  rdfs:label "enclosed basin stands"@en ;
  rdfs:label "enclosed basin stands"@nl ;
  rdfs:seeAlso <http://vocab.getty.edu/aat/300164425> ;
  rdfs:subClassOf <https://w3id.org/con-tax/components/aat-furn#300039859> ;
.
<https://w3id.org/con-tax/components/aat-furn#300164429>
  rdf:type owl:Class ;
  rdfs:comment "Relatively small and narrow bookcases, often approximately 3 feet wide and 3 feet high, of the type used in the 18th and 19th century mercantile establishments for keeping account books."@en ;
  rdfs:comment "Term die wordt gebruikt in de late 18e en vroege 19e eeuw voor relatief kleine en smalle boekenkasten, over het algemeen ongeveer 1 meter (3 voet breed) en 1 meter (3 voet) hoog."@nl ;
  rdfs:isDefinedBy <https://w3id.org/con-tax/components/aat-furn> ;
  rdfs:label "counting-house bookcases"@en ;
  rdfs:label "kantoorkast"@nl ;
  rdfs:label "kantoorkasten"@nl ;
  rdfs:seeAlso <http://vocab.getty.edu/aat/300164429> ;
  rdfs:subClassOf <https://w3id.org/con-tax/components/aat-furn#300143716> ;
.
<https://w3id.org/con-tax/components/aat-furn#300164431>
  rdf:type owl:Class ;
  rdfs:comment "Low tables or shelves meant to stand against a wall in the space between two windows, often surmounted with a mirror, and with a rail or shelf enclosing the surface."@en ;
  rdfs:isDefinedBy <https://w3id.org/con-tax/components/aat-furn> ;
  rdfs:label "enclosed pier tables"@en ;
  rdfs:label "ingesloten penanttafel"@nl ;
  rdfs:label "ingesloten penanttafels"@nl ;
  rdfs:seeAlso <http://vocab.getty.edu/aat/300164431> ;
  rdfs:subClassOf <https://w3id.org/con-tax/components/aat-furn#300040000> ;
.
<https://w3id.org/con-tax/components/aat-furn#300164456>
  rdf:type owl:Class ;
  rdfs:comment "Benaming die meestal van toepassing is op tafels die in de keuken worden gebruikt, met name de tafels met ruim werkoppervlak en laden of bakken als opslagruimte."@nl ;
  rdfs:comment "Term generally applied to tables intended for use in kitchens, especially those having an ample work surface and drawers or bins for storage."@en ;
  rdfs:isDefinedBy <https://w3id.org/con-tax/components/aat-furn> ;
  rdfs:label "keukentafel"@nl ;
  rdfs:label "keukentafels"@nl ;
  rdfs:label "kitchen tables"@en ;
  rdfs:seeAlso <http://vocab.getty.edu/aat/300164456> ;
  rdfs:subClassOf <https://w3id.org/con-tax/components/aat-furn#300039548> ;
.
<https://w3id.org/con-tax/components/aat-furn#300164472>
  rdf:type owl:Class ;
  rdfs:comment "Folding beds built into cabinets that incorporate shelving for books on either side of a mid-section covered by double doors, and which were intended to be used in a dining room to make an occasional extra bedroom."@en ;
  rdfs:isDefinedBy <https://w3id.org/con-tax/components/aat-furn> ;
  rdfs:label "library press bed"@nl ;
  rdfs:label "library press beds"@en ;
  rdfs:label "library press beds"@nl ;
  rdfs:seeAlso <http://vocab.getty.edu/aat/300164472> ;
  rdfs:subClassOf <https://w3id.org/con-tax/components/aat-furn#300038807> ;
.
<https://w3id.org/con-tax/components/aat-furn#300164491>
  rdf:type owl:Class ;
  rdfs:comment "Standaarden met een grote, rechtopstaande post en een verschuifbare dwarsbalk, die op verschillende hoogtes kan worden ingesteld, met pinnen waaraan kaarten kunnen worden opgehangen."@nl ;
  rdfs:comment "Stands with a tall upright post and a sliding cross bar which can be adjusted at different heights and bears pins for suspending maps or charts."@en ;
  rdfs:isDefinedBy <https://w3id.org/con-tax/components/aat-furn> ;
  rdfs:label "kaarthouder"@nl ;
  rdfs:label "kaarthouders"@nl ;
  rdfs:label "map stands"@en ;
  rdfs:seeAlso <http://vocab.getty.edu/aat/300164491> ;
  rdfs:subClassOf <https://w3id.org/con-tax/components/aat-furn#300039767> ;
.
<https://w3id.org/con-tax/components/aat-furn#300164492>
  rdf:type owl:Class ;
  rdfs:isDefinedBy <https://w3id.org/con-tax/components/aat-furn> ;
  rdfs:label "double counting-house desks"@en ;
  rdfs:label "dubbele boekhoudtafel"@nl ;
  rdfs:label "dubbele boekhoudtafels"@nl ;
  rdfs:seeAlso <http://vocab.getty.edu/aat/300164492> ;
  rdfs:subClassOf <https://w3id.org/con-tax/components/aat-furn#300039343> ;
.
<https://w3id.org/con-tax/components/aat-furn#300164496>
  rdf:type owl:Class ;
  rdfs:comment "Lage boekenkasten die zo zijn ontworpen dat de wand erboven vrij is voor schilderijen of hoge spiegels. Ze hebben meestal een openkast-systeem of deuren met open traliewerk in plaats van massieve deuren of deuren bekleed met zijde."@nl ;
  rdfs:comment "Low bookcases deliberately designed so as to leave the wall above free for paintings or pier glasses; generally having open shelves or doors with open grilles, instead of solid or silk-paneled doors."@en ;
  rdfs:isDefinedBy <https://w3id.org/con-tax/components/aat-furn> ;
  rdfs:label "dwarf bookcases"@en ;
  rdfs:label "lage boekenkast"@nl ;
  rdfs:label "lage boekenkasten"@nl ;
  rdfs:seeAlso <http://vocab.getty.edu/aat/300164496> ;
  rdfs:subClassOf <https://w3id.org/con-tax/components/aat-furn#300143716> ;
.
<https://w3id.org/con-tax/components/aat-furn#300164504>
  rdf:type owl:Class ;
  rdfs:comment "Bedside table with a cabinet integrated beneath the table surface."@en ;
  rdfs:isDefinedBy <https://w3id.org/con-tax/components/aat-furn> ;
  rdfs:label "somnoes"@en ;
  rdfs:label "somnoes"@nl ;
  rdfs:seeAlso <http://vocab.getty.edu/aat/300164504> ;
  rdfs:subClassOf <https://w3id.org/con-tax/components/aat-furn#300039745> ;
.
<https://w3id.org/con-tax/components/aat-furn#300164508>
  rdf:type owl:Class ;
  rdfs:comment "Kleine lichtgewicht standaarden met meerdere verdiepingen, die vaak opvouwbaar en draagbaar zijn. Ze worden op een tafel neergezet met licht voedsel erin, zoals muffins."@nl ;
  rdfs:comment "Small lightweight tiered stands, often folding and portable, intended to be used alongside a table for holding such light foods as muffins."@en ;
  rdfs:isDefinedBy <https://w3id.org/con-tax/components/aat-furn> ;
  rdfs:label "muffin stands"@en ;
  rdfs:label "muffinhouder"@nl ;
  rdfs:label "muffinhouders"@nl ;
  rdfs:seeAlso <http://vocab.getty.edu/aat/300164508> ;
  rdfs:subClassOf <https://w3id.org/con-tax/components/aat-furn#300039767> ;
.
<https://w3id.org/con-tax/components/aat-furn#300164509>
  rdf:type owl:Class ;
  rdfs:comment "Desks that resemble spinets, the keyed musical instruments which are closely related to harpsichords. "@en ;
  rdfs:isDefinedBy <https://w3id.org/con-tax/components/aat-furn> ;
  rdfs:label "spinet desks"@en ;
  rdfs:label "spinetbureau"@nl ;
  rdfs:label "spinetbureaus"@nl ;
  rdfs:seeAlso <http://vocab.getty.edu/aat/300164509> ;
  rdfs:subClassOf <https://w3id.org/con-tax/components/aat-furn#300039338> ;
.
<https://w3id.org/con-tax/components/aat-furn#300164515>
  rdf:type owl:Class ;
  rdfs:comment "Chairs with adjustable backs, swivel seats, and commonly mounted with castors, designed to be used in the course of office work."@en ;
  rdfs:isDefinedBy <https://w3id.org/con-tax/components/aat-furn> ;
  rdfs:label "kantoorstoel"@nl ;
  rdfs:label "kantoorstoelen (bureaustoelen)"@nl ;
  rdfs:label "kantoorstoelen"@nl ;
  rdfs:label "office chairs"@en ;
  rdfs:seeAlso <http://vocab.getty.edu/aat/300164515> ;
  rdfs:seeAlso wd:Q1021686 ;
  rdfs:subClassOf <https://w3id.org/con-tax/components/aat-furn#300038165> ;
.
<https://w3id.org/con-tax/components/aat-furn#300164516>
  rdf:type owl:Class ;
  rdfs:comment "Cabinets with the interior divided into nests of small drawers for holding spices."@en ;
  rdfs:comment "Kasten die in kleine laadjes zijn verdeeld waarin kruiden worden bewaard."@nl ;
  rdfs:isDefinedBy <https://w3id.org/con-tax/components/aat-furn> ;
  rdfs:label "kruidenkast"@nl ;
  rdfs:label "kruidenkasten"@nl ;
  rdfs:label "spice cabinets"@en ;
  rdfs:seeAlso <http://vocab.getty.edu/aat/300164516> ;
  rdfs:subClassOf <https://w3id.org/con-tax/components/aat-furn#300038888> ;
.
<https://w3id.org/con-tax/components/aat-furn#300164518>
  rdf:type owl:Class ;
  rdfs:comment "Kleine wandkastjes die meestal hangen en voornamelijk voor kruiden worden gebruikt."@nl ;
  rdfs:comment "Miniature cupboards, usually hanging, primarily intended to hold spices."@en ;
  rdfs:isDefinedBy <https://w3id.org/con-tax/components/aat-furn> ;
  rdfs:label "kruidenrekje"@nl ;
  rdfs:label "kruidenrekjes"@nl ;
  rdfs:label "spice cupboards"@en ;
  rdfs:seeAlso <http://vocab.getty.edu/aat/300164518> ;
  rdfs:subClassOf <https://w3id.org/con-tax/components/aat-furn#300249925> ;
.
<https://w3id.org/con-tax/components/aat-furn#300164519>
  rdf:type owl:Class ;
  rdfs:comment "Tables with very slender supports, sometimes of gate-leg design."@en ;
  rdfs:comment "Tafels met een zeer dun onderstel, soms met inklappoten."@nl ;
  rdfs:isDefinedBy <https://w3id.org/con-tax/components/aat-furn> ;
  rdfs:label "spider-leg tables"@en ;
  rdfs:label "spinnenpoottafel"@nl ;
  rdfs:label "spinnenpoottafels"@nl ;
  rdfs:seeAlso <http://vocab.getty.edu/aat/300164519> ;
  rdfs:subClassOf <https://w3id.org/con-tax/components/aat-furn#300039548> ;
.
<https://w3id.org/con-tax/components/aat-furn#300164527>
  rdf:type owl:Class ;
  rdfs:comment "Historische benaming die in de 19e eeuw werd gebruikt voor schuin geplaatste bureaus met een hoog geplaatst schrijfblad waarachter wordt gestaan."@nl ;
  rdfs:comment "Slant-front desks having a high writing surface, designed at a height to be used while standing; popular in the 19th century."@en ;
  rdfs:isDefinedBy <https://w3id.org/con-tax/components/aat-furn> ;
  rdfs:label "sta-bureau"@nl ;
  rdfs:label "sta-bureaus"@nl ;
  rdfs:label "standing desks"@en ;
  rdfs:seeAlso <http://vocab.getty.edu/aat/300164527> ;
  rdfs:seeAlso wd:Q3416733 ;
  rdfs:subClassOf <https://w3id.org/con-tax/components/aat-furn#300039338> ;
  rdfs:subClassOf <https://w3id.org/con-tax/components/aat-furn#300039526> ;
.
<https://w3id.org/con-tax/components/aat-furn#300164528>
  rdf:type gvp:GuideTerm ;
  rdfs:isDefinedBy <https://w3id.org/con-tax/components/aat-furn> ;
  rdfs:label "<opslag en tentoonstellingsmeubilair>"@nl ;
  rdfs:label "<storage and display furniture>"@en ;
  rdfs:label "opslag en tentoonstellingsmeubilair"@nl ;
  rdfs:seeAlso <http://vocab.getty.edu/aat/300164528> ;
  contax:containsConcept <https://w3id.org/con-tax/components/aat-furn#300038860> ;
  contax:containsConcept <https://w3id.org/con-tax/components/aat-furn#300039300> ;
  contax:containsConcept <https://w3id.org/con-tax/components/aat-furn#300136630> ;
  contax:containsConcept <https://w3id.org/con-tax/components/aat-furn#300165579> ;
  contax:containsConcept <https://w3id.org/con-tax/components/aat-furn#300167586> ;
  contax:containsConcept <https://w3id.org/con-tax/components/aat-furn#300215543> ;
  contax:containsConcept <https://w3id.org/con-tax/components/aat-furn#300249762> ;
  contax:containsConcept <https://w3id.org/con-tax/components/aat-furn#300263101> ;
  contax:containsConcept <https://w3id.org/con-tax/components/aat-furn#300266704> ;
  contax:containsConcept <https://w3id.org/con-tax/components/aat-furn#300310713> ;
  contax:containsConcept <https://w3id.org/con-tax/components/aat-furn#300375198> ;
  contax:containsConcept <https://w3id.org/con-tax/components/aat-furn#300375209> ;
  contax:containsGuideTerm <https://w3id.org/con-tax/components/aat-furn#300435638> ;
.
<https://w3id.org/con-tax/components/aat-furn#300164529>
  rdf:type owl:Class ;
  rdfs:comment "Benaming die aan het eind van de 19e eeuw werd gebruikt voor een soort gestoffeerde leunstoel die bedoeld was om als leesstoel in slaapzalen te gebruiken."@nl ;
  rdfs:comment "Type of upholstered armchair intended to be used as reading chairs in 19th-century dormitories."@en ;
  rdfs:isDefinedBy <https://w3id.org/con-tax/components/aat-furn> ;
  rdfs:label "student chairs"@en ;
  rdfs:label "studentenstoel"@nl ;
  rdfs:label "studentenstoelen"@nl ;
  rdfs:seeAlso <http://vocab.getty.edu/aat/300164529> ;
  rdfs:subClassOf <https://w3id.org/con-tax/components/aat-furn#300037776> ;
  rdfs:subClassOf <https://w3id.org/con-tax/components/aat-furn#300038217> ;
.
<https://w3id.org/con-tax/components/aat-furn#300164535>
  rdf:type owl:Class ;
  rdfs:isDefinedBy <https://w3id.org/con-tax/components/aat-furn> ;
  rdfs:label "schommelwieg"@nl ;
  rdfs:label "schommelwiegen"@nl ;
  rdfs:label "swinging cradles"@en ;
  rdfs:seeAlso <http://vocab.getty.edu/aat/300164535> ;
  rdfs:subClassOf <https://w3id.org/con-tax/components/aat-furn#300038847> ;
.
<https://w3id.org/con-tax/components/aat-furn#300164542>
  rdf:type owl:Class ;
  rdfs:comment "Dual-purpose side tables having a hinged top and a front containing a folding bed."@en ;
  rdfs:comment "Wandtafels die twee doelen dienen. Ze hebben een scharnierend blad en een front waarachter zich een opklapbed bevindt."@nl ;
  rdfs:isDefinedBy <https://w3id.org/con-tax/components/aat-furn> ;
  rdfs:label "table beds"@en ;
  rdfs:label "tafelbed"@nl ;
  rdfs:label "tafelbedden"@nl ;
  rdfs:seeAlso <http://vocab.getty.edu/aat/300164542> ;
  rdfs:subClassOf <https://w3id.org/con-tax/components/aat-furn#300038803> ;
  rdfs:subClassOf <https://w3id.org/con-tax/components/aat-furn#300039999> ;
.
<https://w3id.org/con-tax/components/aat-furn#300164547>
  rdf:type owl:Class ;
  rdfs:comment "Furniture designed specifically to support analog telephone sets. These usually include compartments or drawers for telephone directories, notepads, or writing utensils."@en ;
  rdfs:isDefinedBy <https://w3id.org/con-tax/components/aat-furn> ;
  rdfs:label "telefoontafel"@nl ;
  rdfs:label "telefoontafels"@nl ;
  rdfs:label "telephone tables"@en ;
  rdfs:seeAlso <http://vocab.getty.edu/aat/300164547> ;
  rdfs:subClassOf <https://w3id.org/con-tax/components/aat-furn#300039548> ;
.
<https://w3id.org/con-tax/components/aat-furn#300164562>
  rdf:type owl:Class ;
  rdfs:comment "Grote ladenkasten waarop een spiegel is bevestigd. Ze kwamen veel voor aan het eind van de 19e en het begin van de 20e eeuw."@nl ;
  rdfs:comment "Tall chests of drawers with a mirror on top; common in late 19th and early 20th century."@en ;
  rdfs:isDefinedBy <https://w3id.org/con-tax/components/aat-furn> ;
  rdfs:label "chiffoniers (tall chests of drawers)"@en ;
  rdfs:label "chiffonnière (ladenkast met spiegel)"@nl ;
  rdfs:label "chiffonnière"@nl ;
  rdfs:label "chiffonnières (ladenkasten met spiegel)"@nl ;
  rdfs:label "chiffonnières"@nl ;
  rdfs:seeAlso <http://vocab.getty.edu/aat/300164562> ;
  rdfs:subClassOf <https://w3id.org/con-tax/components/aat-furn#300039009> ;
.
<https://w3id.org/con-tax/components/aat-furn#300164566>
  rdf:type owl:Class ;
  rdfs:comment "Historische benaming die in de 19e eeuw werd gebruikt voor decoratieve tafels, bedoeld om  als pronkstuk te dienen, met name in woonkamers. Gebruik 'huiskamertafels' voor tafels die meestal bijpassend aan het overige meubilair zijn gemaakt en zijn bedoeld om in het midden van een kamer te staan."@nl ;
  rdfs:comment "Ornamental tables meant to be used as accent pieces, especially in 19th-century parlors. They are often of a round or oval shape, are of a size and style allowing one or two people to sit at the table in chairs, and often displayed a lamp, books, framed photographs, and other items of interest. For tables that were made en suite and finished on all sides, intended to be placed in the center of a room, often rectangular but of various shapes, and not necessarily designed for seating with chairs, use \"center tables.\""@en ;
  rdfs:isDefinedBy <https://w3id.org/con-tax/components/aat-furn> ;
  rdfs:label "parlor tables"@en-us ;
  rdfs:label "woonkamertafel"@nl ;
  rdfs:label "woonkamertafels"@nl ;
  rdfs:seeAlso <http://vocab.getty.edu/aat/300164566> ;
  rdfs:subClassOf <https://w3id.org/con-tax/components/aat-furn#300039548> ;
.
<https://w3id.org/con-tax/components/aat-furn#300164567>
  rdf:type owl:Class ;
  rdfs:comment "Chairs which served as models from which to work; frequently with arms or legs showing alternative forms and styles of decoration."@en ;
  rdfs:comment "Stoelen die als werkmodel dienst deden. De armleuningen en poten vertoonden vaak verschillende vormen en decoratiestijlen."@nl ;
  rdfs:isDefinedBy <https://w3id.org/con-tax/components/aat-furn> ;
  rdfs:label "pattern chair"@nl ;
  rdfs:label "pattern chairs"@en ;
  rdfs:label "pattern chairs"@nl ;
  rdfs:seeAlso <http://vocab.getty.edu/aat/300164567> ;
  rdfs:subClassOf <https://w3id.org/con-tax/components/aat-furn#300037772> ;
.
<https://w3id.org/con-tax/components/aat-furn#300164579>
  rdf:type owl:Class ;
  rdfs:comment "Cabinets with narrow shelves for holding piano rolls."@en ;
  rdfs:comment "Kabinetten met smalle planken om pianolarollen op te bergen."@nl ;
  rdfs:isDefinedBy <https://w3id.org/con-tax/components/aat-furn> ;
  rdfs:label "pianola roll cabinets"@en ;
  rdfs:label "pianolarol-kast"@nl ;
  rdfs:label "pianolarol-kasten"@nl ;
  rdfs:seeAlso <http://vocab.getty.edu/aat/300164579> ;
  rdfs:subClassOf <https://w3id.org/con-tax/components/aat-furn#300038950> ;
.
<https://w3id.org/con-tax/components/aat-furn#300164581>
  rdf:type owl:Class ;
  rdfs:comment "Dining tables, or tables used for other purposes, having pillar and claw supports, with legs jutting from a pillar and with feet terminating into a claw."@en ;
  rdfs:comment "Historische benaming die vooral  in het begin van de 19e eeuw werd gebruikt voor eettafels met poten die uit een pilaar steken en eindigen in klauwen."@nl ;
  rdfs:isDefinedBy <https://w3id.org/con-tax/components/aat-furn> ;
  rdfs:label "pilaar en voetklauw dinertafel"@nl ;
  rdfs:label "pilaar en voetklauw dinertafels"@nl ;
  rdfs:label "pillar and claw dining tables"@en ;
  rdfs:seeAlso <http://vocab.getty.edu/aat/300164581> ;
  rdfs:subClassOf <https://w3id.org/con-tax/components/aat-furn#300039596> ;
  rdfs:subClassOf <https://w3id.org/con-tax/components/aat-furn#300039648> ;
.
<https://w3id.org/con-tax/components/aat-furn#300164584>
  rdf:type owl:Class ;
  rdfs:comment "Dropleaf tables of the Pembroke stye, having pillar and claw supports, with legs jutting from a pillar or columns, and with feet terminating into a claw."@en ;
  rdfs:isDefinedBy <https://w3id.org/con-tax/components/aat-furn> ;
  rdfs:label "pilaar-klauw Pembroke tafel"@nl ;
  rdfs:label "pilaar-klauw Pembroke tafels"@nl ;
  rdfs:label "pillar and claw Pembroke tables"@en ;
  rdfs:seeAlso <http://vocab.getty.edu/aat/300164584> ;
  rdfs:subClassOf <https://w3id.org/con-tax/components/aat-furn#300039596> ;
  rdfs:subClassOf <https://w3id.org/con-tax/components/aat-furn#300039941> ;
.
<https://w3id.org/con-tax/components/aat-furn#300164591>
  rdf:type owl:Class ;
  rdfs:comment "Chairs that are designed or used to serve as both a chair and a pulpit or lectern in a relgious setting; found in the context of Buddhism, Islam, Christianity, and other religions. Examples are chairs having a tall back surmounted by a lectern, so that the chair could be used as a pulpit at open-air services or worship conducted at local houses."@en ;
  rdfs:comment "Stoelen die een hoge rugleuning hebben waar een lessenaar bovenop is geplaatst, zodat de stoel als preekstoel kan worden gebruikt bij diensten in de open lucht of in privéhuizen."@nl ;
  rdfs:isDefinedBy <https://w3id.org/con-tax/components/aat-furn> ;
  rdfs:label "preaching chairs"@en ;
  rdfs:label "preekstoel (meubilair)"@nl ;
  rdfs:label "preekstoel"@nl ;
  rdfs:label "preekstoelen (meubilair)"@nl ;
  rdfs:label "preekstoelen"@nl ;
  rdfs:seeAlso <http://vocab.getty.edu/aat/300164591> ;
  rdfs:subClassOf <https://w3id.org/con-tax/components/aat-furn#300037772> ;
  rdfs:subClassOf <https://w3id.org/con-tax/components/aat-furn#300170801> ;
.
<https://w3id.org/con-tax/components/aat-furn#300164593>
  rdf:type owl:Class ;
  rdfs:comment "Furniture consisting of a flat, slablike top mounted on legs, designed specifically to support large radio sets."@en ;
  rdfs:isDefinedBy <https://w3id.org/con-tax/components/aat-furn> ;
  rdfs:label "radio tables"@en ;
  rdfs:label "radiotafel"@nl ;
  rdfs:label "radiotafels"@nl ;
  rdfs:seeAlso <http://vocab.getty.edu/aat/300164593> ;
  rdfs:subClassOf <https://w3id.org/con-tax/components/aat-furn#300039548> ;
.
<https://w3id.org/con-tax/components/aat-furn#300164594>
  rdf:type owl:Class ;
  rdfs:comment "Lightweight chairs, often with upholstered seats, which are meant to be used as informal seating for guests. "@en ;
  rdfs:isDefinedBy <https://w3id.org/con-tax/components/aat-furn> ;
  rdfs:label "receptiestoel"@nl ;
  rdfs:label "receptiestoelen"@nl ;
  rdfs:label "reception chairs"@en ;
  rdfs:seeAlso <http://vocab.getty.edu/aat/300164594> ;
  rdfs:subClassOf <https://w3id.org/con-tax/components/aat-furn#300037772> ;
.
<https://w3id.org/con-tax/components/aat-furn#300164614>
  rdf:type owl:Class ;
  rdfs:comment "Cabinets of varied design intended to store phonograph records. These may incorporate separators or other methods devised to aid organization."@en ;
  rdfs:isDefinedBy <https://w3id.org/con-tax/components/aat-furn> ;
  rdfs:label "platenkast"@nl ;
  rdfs:label "platenkasten"@nl ;
  rdfs:label "record cabinets"@en ;
  rdfs:seeAlso <http://vocab.getty.edu/aat/300164614> ;
  rdfs:subClassOf <https://w3id.org/con-tax/components/aat-furn#300038888> ;
.
<https://w3id.org/con-tax/components/aat-furn#300164628>
  rdf:type owl:Class ;
  rdfs:comment "Desks on long legs, generally taking the form of a table, with a folding top and writing surface that can enclose a drawer or cubbyholes."@en ;
  rdfs:isDefinedBy <https://w3id.org/con-tax/components/aat-furn> ;
  rdfs:label "rising-top writing table"@nl ;
  rdfs:label "rising-top writing tables"@en ;
  rdfs:label "rising-top writing tables"@nl ;
  rdfs:seeAlso <http://vocab.getty.edu/aat/300164628> ;
  rdfs:subClassOf <https://w3id.org/con-tax/components/aat-furn#300039436> ;
.
<https://w3id.org/con-tax/components/aat-furn#300164649>
  rdf:type owl:Class ;
  rdfs:comment "Stevige tafels, soms uitgerust met onderzetters of buidels, meestal met een plank onder het tafelblad om glazen en stenen bierkroezen in te zetten zodat het blad vrij kon blijven voor het kaartspelen."@nl ;
  rdfs:comment "Sturdy tables, sometimes fitted with coasters or pockets, generally having a shelf under the top to hold glasses and steins so the top could remain clear for card playing."@en ;
  rdfs:isDefinedBy <https://w3id.org/con-tax/components/aat-furn> ;
  rdfs:label "saloon tables"@en ;
  rdfs:label "saloontafel"@nl ;
  rdfs:label "saloontafels"@nl ;
  rdfs:seeAlso <http://vocab.getty.edu/aat/300164649> ;
  rdfs:subClassOf <https://w3id.org/con-tax/components/aat-furn#300039548> ;
.
<https://w3id.org/con-tax/components/aat-furn#300164653>
  rdf:type owl:Class ;
  rdfs:comment "Book furniture composed of stackable modules in which the books are housed allowing the user to add more storage as needed. These modules or sections are often fitted with glass doors."@en ;
  rdfs:isDefinedBy <https://w3id.org/con-tax/components/aat-furn> ;
  rdfs:label "boekenkast in secties"@nl ;
  rdfs:label "boekenkasten in secties"@nl ;
  rdfs:label "sectional bookcases"@en ;
  rdfs:seeAlso <http://vocab.getty.edu/aat/300164653> ;
  rdfs:subClassOf <https://w3id.org/con-tax/components/aat-furn#300143716> ;
.
<https://w3id.org/con-tax/components/aat-furn#300164655>
  rdf:type owl:Class ;
  rdfs:comment "Gestoffeerde leunstoelen, vaak met  een sterk hellende 'button-tufted' rugleuning uit een stuk en een concave zitting. Dit type werd in het midden van de 19e en het begin van de 20e eeuw in Amerika gemaakt."@nl ;
  rdfs:comment "Upholstered armchairs, often with a button-tufted back, having a single piece forming a high sloping back and a concave seat; of a type made in America in the mid-19th to early 20th centuries."@en ;
  rdfs:isDefinedBy <https://w3id.org/con-tax/components/aat-furn> ;
  rdfs:label "Sleepy Hollow chair"@nl ;
  rdfs:label "Sleepy Hollow chairs"@en ;
  rdfs:label "Sleepy Hollow chairs"@nl ;
  rdfs:seeAlso <http://vocab.getty.edu/aat/300164655> ;
  rdfs:subClassOf <https://w3id.org/con-tax/components/aat-furn#300037772> ;
  rdfs:subClassOf <https://w3id.org/con-tax/components/aat-furn#300037776> ;
.
<https://w3id.org/con-tax/components/aat-furn#300164657>
  rdf:type owl:Class ;
  rdfs:comment "Chairs with compartments for smoking equipment."@en ;
  rdfs:comment "Stoelen die aparte vakjes hebben om benodigdheden voor het roken te bergen."@nl ;
  rdfs:isDefinedBy <https://w3id.org/con-tax/components/aat-furn> ;
  rdfs:label "fumeuse"@nl ;
  rdfs:label "fumeuses"@nl ;
  rdfs:label "rookstoel"@nl ;
  rdfs:label "rookstoelen"@nl ;
  rdfs:label "smoking chairs (chairs for smoking)"@en ;
  rdfs:seeAlso <http://vocab.getty.edu/aat/300164657> ;
  rdfs:subClassOf <https://w3id.org/con-tax/components/aat-furn#300037772> ;
.
<https://w3id.org/con-tax/components/aat-furn#300164663>
  rdf:type owl:Class ;
  rdfs:isDefinedBy <https://w3id.org/con-tax/components/aat-furn> ;
  rdfs:label "toilet table beds"@en ;
  rdfs:label "toilettafelbed"@nl ;
  rdfs:label "toilettafelbedden"@nl ;
  rdfs:seeAlso <http://vocab.getty.edu/aat/300164663> ;
  rdfs:subClassOf <https://w3id.org/con-tax/components/aat-furn#300164542> ;
.
<https://w3id.org/con-tax/components/aat-furn#300164673>
  rdf:type owl:Class ;
  rdfs:comment "Bidets die uit een kast te voorschijn komen. Gebruik '@portable bidets' voor bidets met afschroefbare poten en afsluitbare bovenkant."@nl ;
  rdfs:comment "Bidets made to rise out a chest. Use \"portable bidets\" for those with legs made to screw off and tops made to lock."@en ;
  rdfs:isDefinedBy <https://w3id.org/con-tax/components/aat-furn> ;
  rdfs:label "reisbidet"@nl ;
  rdfs:label "reisbidets"@nl ;
  rdfs:label "traveling bidets"@en ;
  rdfs:seeAlso <http://vocab.getty.edu/aat/300164673> ;
  rdfs:subClassOf <https://w3id.org/con-tax/components/aat-furn#300164327> ;
.
<https://w3id.org/con-tax/components/aat-furn#300164679>
  rdf:type owl:Class ;
  rdfs:comment "Refers generally to three-legged supports of any kind. The word may be applied variously to objects such as stools, tables, light stands, stands for cameras, or pedestals. Ancient, antique, or classical forms are associated with religious or symbolic altars, or sacrificial vessels. The seat of the Delphic oracle was in the form of a tripod."@en ;
  rdfs:isDefinedBy <https://w3id.org/con-tax/components/aat-furn> ;
  rdfs:label "drievoeten"@nl ;
  rdfs:label "statief (standaarden)"@nl ;
  rdfs:label "statief"@nl ;
  rdfs:label "statieven (standaarden)"@nl ;
  rdfs:label "statieven"@nl ;
  rdfs:label "tripods (stands)"@en ;
  rdfs:seeAlso <http://vocab.getty.edu/aat/300164679> ;
  rdfs:subClassOf <https://w3id.org/con-tax/components/aat-furn#300039767> ;
.
<https://w3id.org/con-tax/components/aat-furn#300164698>
  rdf:type owl:Class ;
  rdfs:comment "Low-back chairs with wide seats; intended to be used in the embrasure of a window."@en ;
  rdfs:comment "Stoelen die een lage rugleuning hebben met een brede zitting. Ze zijn bedoeld om bij een vensteropening te zetten."@nl ;
  rdfs:isDefinedBy <https://w3id.org/con-tax/components/aat-furn> ;
  rdfs:label "raamstoel"@nl ;
  rdfs:label "raamstoelen"@nl ;
  rdfs:label "window chairs"@en ;
  rdfs:seeAlso <http://vocab.getty.edu/aat/300164698> ;
  rdfs:subClassOf <https://w3id.org/con-tax/components/aat-furn#300037772> ;
.
<https://w3id.org/con-tax/components/aat-furn#300164704>
  rdf:type owl:Class ;
  rdfs:comment "Clothes presses flanked with additional drawers and storage areas on either side of the central carcass, coined in the late 18th and early 19th centuries."@en ;
  rdfs:comment "Historische benaming die eind 18e en begin 19e eeuw werd gebruikt voor 'clothes presses' met extra laden en opbergruimtes aan beide zijdes van het middengedeelte."@nl ;
  rdfs:isDefinedBy <https://w3id.org/con-tax/components/aat-furn> ;
  rdfs:label "wing clothes press"@nl ;
  rdfs:label "wing clothes presses"@en ;
  rdfs:label "wing clothes presses"@nl ;
  rdfs:seeAlso <http://vocab.getty.edu/aat/300164704> ;
  rdfs:subClassOf <https://w3id.org/con-tax/components/aat-furn#300039253> ;
.
<https://w3id.org/con-tax/components/aat-furn#300165321>
  rdf:type owl:Class ;
  rdfs:comment "Armchairs having open arms and padded rests."@en ;
  rdfs:comment "Term die wordt gebruikt voor leunstoelen, met name voor de leunstoelen met open armleuningen en opgevulde armsteuntjes."@nl ;
  rdfs:isDefinedBy <https://w3id.org/con-tax/components/aat-furn> ;
  rdfs:label "armstoel"@nl ;
  rdfs:label "armstoelen"@nl ;
  rdfs:label "elbow chairs"@en ;
  rdfs:seeAlso <http://vocab.getty.edu/aat/300165321> ;
  rdfs:subClassOf <https://w3id.org/con-tax/components/aat-furn#300037776> ;
.
<https://w3id.org/con-tax/components/aat-furn#300165324>
  rdf:type owl:Class ;
  rdfs:comment "Folding portable chairs usually with a wood frame and canvas seat and back originally used on the sets of motion pictures as seating for actors or directors."@en ;
  rdfs:isDefinedBy <https://w3id.org/con-tax/components/aat-furn> ;
  rdfs:label "directors' chairs"@en ;
  rdfs:label "regisseursstoel"@nl ;
  rdfs:label "regisseursstoelen"@nl ;
  rdfs:seeAlso <http://vocab.getty.edu/aat/300165324> ;
  rdfs:seeAlso wd:Q5280501 ;
  rdfs:subClassOf <https://w3id.org/con-tax/components/aat-furn#300037772> ;
.
<https://w3id.org/con-tax/components/aat-furn#300165327>
  rdf:type gvp:GuideTerm ;
  rdfs:isDefinedBy <https://w3id.org/con-tax/components/aat-furn> ;
  rdfs:label "<chairs by location or context: rooms or spaces>"@en ;
  rdfs:label "<stoel naar locatie of context: kamer en ruimte>"@nl ;
  rdfs:label "<stoelen naar locatie of context: kamers en ruimten>"@nl ;
  rdfs:label "stoel naar locatie of context: kamer en ruimte"@nl ;
  rdfs:label "stoelen naar locatie of context: kamers en ruimten"@nl ;
  rdfs:seeAlso <http://vocab.getty.edu/aat/300165327> ;
  contax:containsConcept <https://w3id.org/con-tax/components/aat-furn#300037899> ;
  contax:containsConcept <https://w3id.org/con-tax/components/aat-furn#300038379> ;
  contax:containsConcept <https://w3id.org/con-tax/components/aat-furn#300038382> ;
  contax:containsConcept <https://w3id.org/con-tax/components/aat-furn#300038383> ;
  contax:containsConcept <https://w3id.org/con-tax/components/aat-furn#300164698> ;
.
<https://w3id.org/con-tax/components/aat-furn#300165349>
  rdf:type owl:Class ;
  rdfs:comment "Having a front that is convex in the center and concave at both ends, used with reference to case furniture."@en ;
  rdfs:comment "Met betrekking tot kastmeubilair: met een voorkant die bol is in het midden en hol aan beide uiteinden."@nl ;
  rdfs:isDefinedBy <https://w3id.org/con-tax/components/aat-furn> ;
  rdfs:label "dubbelgebogen front"@nl ;
  rdfs:label "serpentine-front (shape)"@en ;
  rdfs:seeAlso <http://vocab.getty.edu/aat/300165349> ;
  rdfs:subClassOf <https://w3id.org/con-tax/components/aat-furn#300037680> ;
.
<https://w3id.org/con-tax/components/aat-furn#300165496>
  rdf:type owl:Class ;
  rdfs:comment "Benaming voor een bepaald soort algemeen voorkomende stoel, waarschijnlijk met een waaiervormig middenblad."@nl ;
  rdfs:comment "Descriptive term for a type of common chair, presumably with a fan-shaped splat."@en ;
  rdfs:isDefinedBy <https://w3id.org/con-tax/components/aat-furn> ;
  rdfs:label "fan-back chairs"@en ;
  rdfs:label "fan-back stoel"@nl ;
  rdfs:label "fan-back stoelen"@nl ;
  rdfs:seeAlso <http://vocab.getty.edu/aat/300165496> ;
  rdfs:subClassOf <https://w3id.org/con-tax/components/aat-furn#300037772> ;
.
<https://w3id.org/con-tax/components/aat-furn#300165523>
  rdf:type owl:Class ;
  rdfs:comment "Franse chaises longues waarvan het voeteneind aan drie kanten wordt omringd door een lage, gebogen rugleuning."@nl ;
  rdfs:comment "French chaise longues characterized by the foot end that is surrounded on three sides by a low curving back."@en ;
  rdfs:isDefinedBy <https://w3id.org/con-tax/components/aat-furn> ;
  rdfs:label "duchesse (chaise longue)"@nl ;
  rdfs:label "duchesse"@nl ;
  rdfs:label "duchesses (chaise longues)"@en ;
  rdfs:label "duchesses (chaises longues)"@nl ;
  rdfs:label "duchesses"@nl ;
  rdfs:seeAlso <http://vocab.getty.edu/aat/300165523> ;
  rdfs:subClassOf <https://w3id.org/con-tax/components/aat-furn#300038151> ;
.
<https://w3id.org/con-tax/components/aat-furn#300165534>
  rdf:type gvp:GuideTerm ;
  rdfs:isDefinedBy <https://w3id.org/con-tax/components/aat-furn> ;
  rdfs:label "<chairs by location or context: position>"@en ;
  rdfs:label "<stoel naar locatie of context: positie>"@nl ;
  rdfs:label "<stoelen naar locatie of context: positie>"@nl ;
  rdfs:label "stoel naar locatie of context: positie"@nl ;
  rdfs:label "stoelen naar locatie of context: positie"@nl ;
  rdfs:seeAlso <http://vocab.getty.edu/aat/300165534> ;
  contax:containsConcept <https://w3id.org/con-tax/components/aat-furn#300077258> ;
  contax:containsConcept <https://w3id.org/con-tax/components/aat-furn#300077260> ;
.
<https://w3id.org/con-tax/components/aat-furn#300165536>
  rdf:type gvp:GuideTerm ;
  rdfs:isDefinedBy <https://w3id.org/con-tax/components/aat-furn> ;
  rdfs:label "<krukken naar functie>"@nl ;
  rdfs:label "<stools by function>"@en ;
  rdfs:label "krukken naar functie"@nl ;
  rdfs:seeAlso <http://vocab.getty.edu/aat/300165536> ;
  contax:containsConcept <https://w3id.org/con-tax/components/aat-furn#300038429> ;
  contax:containsConcept <https://w3id.org/con-tax/components/aat-furn#300038449> ;
  contax:containsConcept <https://w3id.org/con-tax/components/aat-furn#300038454> ;
  contax:containsConcept <https://w3id.org/con-tax/components/aat-furn#300038457> ;
.
<https://w3id.org/con-tax/components/aat-furn#300165537>
  rdf:type gvp:GuideTerm ;
  rdfs:isDefinedBy <https://w3id.org/con-tax/components/aat-furn> ;
  rdfs:label "<krukken naar ontwerp>"@nl ;
  rdfs:label "<stools by design>"@en ;
  rdfs:label "krukken naar ontwerp"@nl ;
  rdfs:seeAlso <http://vocab.getty.edu/aat/300165537> ;
  contax:containsConcept <https://w3id.org/con-tax/components/aat-furn#300038483> ;
  contax:containsConcept <https://w3id.org/con-tax/components/aat-furn#300244761> ;
  contax:containsConcept <https://w3id.org/con-tax/components/aat-furn#300263111> ;
.
<https://w3id.org/con-tax/components/aat-furn#300165539>
  rdf:type gvp:GuideTerm ;
  rdfs:isDefinedBy <https://w3id.org/con-tax/components/aat-furn> ;
  rdfs:label "<krukken naar locatie of context>"@nl ;
  rdfs:label "<stools by location or context>"@en ;
  rdfs:label "krukken naar locatie of context"@nl ;
  rdfs:seeAlso <http://vocab.getty.edu/aat/300165539> ;
  contax:containsConcept <https://w3id.org/con-tax/components/aat-furn#300038422> ;
  contax:containsConcept <https://w3id.org/con-tax/components/aat-furn#300038431> ;
  contax:containsConcept <https://w3id.org/con-tax/components/aat-furn#300164421> ;
.
<https://w3id.org/con-tax/components/aat-furn#300165544>
  rdf:type gvp:GuideTerm ;
  rdf:type skos:OrderedCollection ;
  rdfs:isDefinedBy <https://w3id.org/con-tax/components/aat-furn> ;
  rdfs:label "<banken naar vorm of functie>"@nl ;
  rdfs:label "<benches by form or function>"@en ;
  rdfs:label "banken naar vorm of functie"@nl ;
  rdfs:seeAlso <http://vocab.getty.edu/aat/300165544> ;
  contax:containsConcept <https://w3id.org/con-tax/components/aat-furn#300038498> ;
  contax:containsConcept <https://w3id.org/con-tax/components/aat-furn#300038507> ;
  contax:containsConcept <https://w3id.org/con-tax/components/aat-furn#300038509> ;
  contax:containsConcept <https://w3id.org/con-tax/components/aat-furn#300038514> ;
  contax:containsConcept <https://w3id.org/con-tax/components/aat-furn#300038521> ;
  contax:containsConcept <https://w3id.org/con-tax/components/aat-furn#300038532> ;
  contax:containsConcept <https://w3id.org/con-tax/components/aat-furn#300121308> ;
  contax:containsConcept <https://w3id.org/con-tax/components/aat-furn#300124818> ;
  contax:containsConcept <https://w3id.org/con-tax/components/aat-furn#300259214> ;
  contax:containsConcept <https://w3id.org/con-tax/components/aat-furn#300264555> ;
  contax:containsConcept <https://w3id.org/con-tax/components/aat-furn#300264594> ;
  contax:containsConcept <https://w3id.org/con-tax/components/aat-furn#300298975> ;
  contax:containsConcept <https://w3id.org/con-tax/components/aat-furn#300395530> ;
.
<https://w3id.org/con-tax/components/aat-furn#300165548>
  rdf:type gvp:GuideTerm ;
  rdfs:isDefinedBy <https://w3id.org/con-tax/components/aat-furn> ;
  rdfs:label "<banken naar locatie of context>"@nl ;
  rdfs:label "<benches by location or context>"@en ;
  rdfs:label "banken naar locatie of context"@nl ;
  rdfs:seeAlso <http://vocab.getty.edu/aat/300165548> ;
  contax:containsConcept <https://w3id.org/con-tax/components/aat-furn#300038523> ;
  contax:containsConcept <https://w3id.org/con-tax/components/aat-furn#300038524> ;
  contax:containsConcept <https://w3id.org/con-tax/components/aat-furn#300038552> ;
  contax:containsConcept <https://w3id.org/con-tax/components/aat-furn#300164316> ;
  contax:containsConcept <https://w3id.org/con-tax/components/aat-furn#300172457> ;
  contax:containsConcept <https://w3id.org/con-tax/components/aat-furn#300298974> ;
  contax:containsConcept <https://w3id.org/con-tax/components/aat-furn#300395528> ;
  contax:containsConcept <https://w3id.org/con-tax/components/aat-furn#300411438> ;
.
<https://w3id.org/con-tax/components/aat-furn#300165579>
  rdf:type owl:Class ;
  rdfs:comment "Open shelves for holding books; distinct from \"bookcases\" which generally have several shelves enclosed by doors."@en ;
  rdfs:comment "Openkast-systeem om boeken in te zetten. Ze verschillen van 'boekenkasten met deuren'  waarbij de planken door een deur worden afgesloten."@nl ;
  rdfs:isDefinedBy <https://w3id.org/con-tax/components/aat-furn> ;
  rdfs:label "boekenplank"@nl ;
  rdfs:label "boekenplanken"@nl ;
  rdfs:label "bookshelves"@en ;
  rdfs:seeAlso <http://vocab.getty.edu/aat/300165579> ;
  rdfs:subClassOf <https://w3id.org/con-tax/components/aat-furn#300037680> ;
.
<https://w3id.org/con-tax/components/aat-furn#300165757>
  rdf:type owl:Class ;
  rdfs:comment "Beds designed for children."@en ;
  rdfs:isDefinedBy <https://w3id.org/con-tax/components/aat-furn> ;
  rdfs:label "children's beds"@en ;
  rdfs:label "kinderbedden"@nl ;
  rdfs:seeAlso <http://vocab.getty.edu/aat/300165757> ;
  rdfs:subClassOf <https://w3id.org/con-tax/components/aat-furn#300038697> ;
  rdfs:subClassOf <https://w3id.org/con-tax/components/aat-furn#300266715> ;
.
<https://w3id.org/con-tax/components/aat-furn#300165783>
  rdf:type gvp:GuideTerm ;
  rdf:type skos:OrderedCollection ;
  rdfs:isDefinedBy <https://w3id.org/con-tax/components/aat-furn> ;
  rdfs:label "<standaard naar vorm>"@nl ;
  rdfs:label "<standaarden naar vorm>"@nl ;
  rdfs:label "<stands by form>"@en ;
  rdfs:label "standaard naar vorm"@nl ;
  rdfs:label "standaarden naar vorm"@nl ;
  rdfs:seeAlso <http://vocab.getty.edu/aat/300165783> ;
  contax:containsConcept <https://w3id.org/con-tax/components/aat-furn#300039770> ;
  contax:containsConcept <https://w3id.org/con-tax/components/aat-furn#300136635> ;
  contax:containsConcept <https://w3id.org/con-tax/components/aat-furn#300139745> ;
  contax:containsConcept <https://w3id.org/con-tax/components/aat-furn#300170137> ;
  contax:containsGuideTerm <https://w3id.org/con-tax/components/aat-furn#300039777> ;
.
<https://w3id.org/con-tax/components/aat-furn#300165788>
  rdf:type owl:Class ;
  rdfs:comment "Pieces of furniture consisting of risers and treads, typically used indoors in place of ladders."@en ;
  rdfs:isDefinedBy <https://w3id.org/con-tax/components/aat-furn> ;
  rdfs:label "ladders: meubilair"@nl ;
  rdfs:label "steps (furniture)"@en ;
  rdfs:seeAlso <http://vocab.getty.edu/aat/300165788> ;
  rdfs:subClassOf <https://w3id.org/con-tax/components/aat-furn#300039337> ;
.
<https://w3id.org/con-tax/components/aat-furn#300165790>
  rdf:type gvp:GuideTerm ;
  rdfs:isDefinedBy <https://w3id.org/con-tax/components/aat-furn> ;
  rdfs:label "<tables by form: top form>"@en ;
  rdfs:label "<tafel naar vorm: tafelbladvorm>"@nl ;
  rdfs:label "<tafels naar vorm: tafelbladvorm>"@nl ;
  rdfs:label "tafel naar vorm: tafelbladvorm"@nl ;
  rdfs:label "tafels naar vorm: tafelbladvorm"@nl ;
  rdfs:seeAlso <http://vocab.getty.edu/aat/300165790> ;
  contax:containsConcept <https://w3id.org/con-tax/components/aat-furn#300039574> ;
  contax:containsConcept <https://w3id.org/con-tax/components/aat-furn#300134826> ;
.
<https://w3id.org/con-tax/components/aat-furn#300165791>
  rdf:type gvp:GuideTerm ;
  rdfs:isDefinedBy <https://w3id.org/con-tax/components/aat-furn> ;
  rdfs:label "<tables by location or context>"@en ;
  rdfs:label "<tafel naar locatie of context>"@nl ;
  rdfs:label "<tafels naar locatie of context>"@nl ;
  rdfs:label "tafel naar locatie of context"@nl ;
  rdfs:label "tafels naar locatie of context"@nl ;
  rdfs:seeAlso <http://vocab.getty.edu/aat/300165791> ;
  contax:containsGuideTerm <https://w3id.org/con-tax/components/aat-furn#300165792> ;
  contax:containsGuideTerm <https://w3id.org/con-tax/components/aat-furn#300165793> ;
.
<https://w3id.org/con-tax/components/aat-furn#300165792>
  rdf:type gvp:GuideTerm ;
  rdfs:isDefinedBy <https://w3id.org/con-tax/components/aat-furn> ;
  rdfs:label "<tables by location or context: position>"@en ;
  rdfs:label "<tafel naar locatie of context: positie>"@nl ;
  rdfs:label "<tafels naar locatie of context: positie>"@nl ;
  rdfs:label "tafel naar locatie of context: positie"@nl ;
  rdfs:label "tafels naar locatie of context: positie"@nl ;
  rdfs:seeAlso <http://vocab.getty.edu/aat/300165792> ;
  contax:containsConcept <https://w3id.org/con-tax/components/aat-furn#300039995> ;
  contax:containsConcept <https://w3id.org/con-tax/components/aat-furn#300039998> ;
  contax:containsConcept <https://w3id.org/con-tax/components/aat-furn#300039999> ;
  contax:containsConcept <https://w3id.org/con-tax/components/aat-furn#300040014> ;
.
<https://w3id.org/con-tax/components/aat-furn#300165793>
  rdf:type gvp:GuideTerm ;
  rdfs:isDefinedBy <https://w3id.org/con-tax/components/aat-furn> ;
  rdfs:label "<tables by location or context: rooms or spaces>"@en ;
  rdfs:label "<tafel naar locatie of context: kamer of ruimte>"@nl ;
  rdfs:label "<tafels naar locatie of context: kamers of ruimten>"@nl ;
  rdfs:label "tafel naar locatie of context: kamer of ruimte"@nl ;
  rdfs:label "tafels naar locatie of context: kamers of ruimten"@nl ;
  rdfs:seeAlso <http://vocab.getty.edu/aat/300165793> ;
  contax:containsConcept <https://w3id.org/con-tax/components/aat-furn#300164415> ;
  contax:containsConcept <https://w3id.org/con-tax/components/aat-furn#300164456> ;
  contax:containsConcept <https://w3id.org/con-tax/components/aat-furn#300164566> ;
  contax:containsConcept <https://w3id.org/con-tax/components/aat-furn#300164649> ;
.
<https://w3id.org/con-tax/components/aat-furn#300165794>
  rdf:type gvp:GuideTerm ;
  rdfs:isDefinedBy <https://w3id.org/con-tax/components/aat-furn> ;
  rdfs:label "<tables by design>"@en ;
  rdfs:label "<tafel naar ontwerp>"@nl ;
  rdfs:label "<tafels naar ontwerp>"@nl ;
  rdfs:label "tafel naar ontwerp"@nl ;
  rdfs:label "tafels naar ontwerp"@nl ;
  rdfs:seeAlso <http://vocab.getty.edu/aat/300165794> ;
  contax:containsConcept <https://w3id.org/con-tax/components/aat-furn#300039958> ;
  contax:containsConcept <https://w3id.org/con-tax/components/aat-furn#300265064> ;
  contax:containsConcept <https://w3id.org/con-tax/components/aat-furn#300425808> ;
  contax:containsConcept <https://w3id.org/con-tax/components/aat-furn#300438696> ;
.
<https://w3id.org/con-tax/components/aat-furn#300165810>
  rdf:type owl:Class ;
  rdfs:comment "Benaming die meestal wordt gebruikt voor allerlei soorten meubilair, dat speciaal is ontworpen voor gebruik buitenshuis."@nl ;
  rdfs:comment "Term generally applied to a great variety of furniture specially designed for use outdoors."@en ;
  rdfs:isDefinedBy <https://w3id.org/con-tax/components/aat-furn> ;
  rdfs:label "buitenhuismeubilair"@nl ;
  rdfs:label "outdoor furniture"@en ;
  rdfs:label "tuinmeubilair"@nl ;
  rdfs:seeAlso <http://vocab.getty.edu/aat/300165810> ;
  rdfs:seeAlso wd:Q2744736 ;
  rdfs:subClassOf <https://w3id.org/con-tax/components/aat-furn#300037680> ;
  contax:containsGuideTerm <https://w3id.org/con-tax/components/aat-furn#300266346> ;
  contax:containsGuideTerm <https://w3id.org/con-tax/components/aat-furn#300266347> ;
.
<https://w3id.org/con-tax/components/aat-furn#300165827>
  rdf:type owl:Class ;
  rdfs:comment "Bidets with legs made to screw off and tops made to lock, popular in the 19th century. Use \"traveling bidets\" for those made to rise out of a chest."@en ;
  rdfs:comment "Historische term die vooral in de 19e eeuw werd gebruikt voor bidets met afschroefbare poten en afsluitbare bovenkant. Gebruik 'reisbidets' voor bidets die uit een kast te voorschijn komen."@nl ;
  rdfs:isDefinedBy <https://w3id.org/con-tax/components/aat-furn> ;
  rdfs:label "draagbaar bidet"@nl ;
  rdfs:label "draagbare bidets"@nl ;
  rdfs:label "portable bidets"@en ;
  rdfs:seeAlso <http://vocab.getty.edu/aat/300165827> ;
  rdfs:subClassOf <https://w3id.org/con-tax/components/aat-furn#300164327> ;
.
<https://w3id.org/con-tax/components/aat-furn#300165852>
  rdf:type owl:Class ;
  rdfs:comment "Kleine kistjes die speciaal voor flesjes met medicijnen zijn gemaakt. Dit type werd in de 18e en het begin van de 19e eeuw vervaardigd."@nl ;
  rdfs:comment "Small chests fitted for bottles and intended to hold medical supplies; of a type made in the 18th and early 19th centuries."@en ;
  rdfs:isDefinedBy <https://w3id.org/con-tax/components/aat-furn> ;
  rdfs:label "medicijnkist"@nl ;
  rdfs:label "medicijnkisten"@nl ;
  rdfs:label "medicine chests"@en ;
  rdfs:seeAlso <http://vocab.getty.edu/aat/300165852> ;
  rdfs:seeAlso wd:Q6806761 ;
  rdfs:subClassOf <https://w3id.org/con-tax/components/aat-furn#300038992> ;
.
<https://w3id.org/con-tax/components/aat-furn#300165855>
  rdf:type owl:Class ;
  rdfs:comment "Canvas chairs suspended from a tree limb, roof, or other structure; of a type made in the late 19th and early 20th centuries."@en ;
  rdfs:comment "Canvas stoelen die aan een boomtak, dak of andere constructie hangen, van het soort dat aan het eind van de 19e en het begin van de 20e eeuw werd gemaakt."@nl ;
  rdfs:isDefinedBy <https://w3id.org/con-tax/components/aat-furn> ;
  rdfs:label "hammock chairs"@en ;
  rdfs:label "hangmatstoel"@nl ;
  rdfs:label "hangmatstoelen"@nl ;
  rdfs:seeAlso <http://vocab.getty.edu/aat/300165855> ;
  rdfs:subClassOf <https://w3id.org/con-tax/components/aat-furn#300037772> ;
  rdfs:subClassOf <https://w3id.org/con-tax/components/aat-furn#300134616> ;
.
<https://w3id.org/con-tax/components/aat-furn#300167570>
  rdf:type owl:Class ;
  rdfs:comment "Refers to either a writing table incorporating drawers or a type of case furniture, generally a chest of drawers, with a hinged, fall-front writing surface. The first furniture types to be referred to by this term developed in France in the mid-17th century, the term having evolved from the medieval French word for a coarse linen cloth that was laid on a table to provide a surface for writing.  In modern usage, in Europe a \"bureau\" is a writing desk, usually with a hinged writing flap that rests at a sloping angle when closed and, when opened, reveals a tier of pigeonholes, small drawers, and sometimes a small cupboard.  In the United States, a \"bureau\" is typically synonymous with a \"chest of drawers,\" having lost the surface for writing."@en ;
  rdfs:comment "Verwijst ofwel naar een schrijftafel met laden ofwel naar een soort kastmeubilair, meestal een ladekast, met een scharnierende, naar voren vallende klep die als schrijfblad fungeert. De eerste meubeltypen waarnaar deze term verwijst, kwamen halverwege de 17de eeuw in Frankrijk tot ontwikkeling. De term 'bureau' heeft zijn oorsprong in een middeleeuws Frans woord voor een grof type linnendoek dat op tafel werd gelegd om als schrijfoppervlak te dienen. In het moderne taalgebruik wordt met 'bureau' een schrijftafel bedoeld, meestal voorzien van een scharnierend schrijfblad dat in gesloten stand in een schuine hoek is geplaatst, terwijl na opening een rij vakjes, laatjes en soms ook een klein kastje zichtbaar wordt. In de Verenigde Staten wordt 'bureau' als synoniem gebruikt voor 'ladekast', waarbij het schrijfblad dus is verdwenen."@nl ;
  rdfs:isDefinedBy <https://w3id.org/con-tax/components/aat-furn> ;
  rdfs:label "bureau met schuin schrijfblad"@nl ;
  rdfs:label "bureaus (slant-front desks)"@en ;
  rdfs:label "bureaus met schuine schrijfbladen"@nl ;
  rdfs:seeAlso <http://vocab.getty.edu/aat/300167570> ;
  rdfs:subClassOf <https://w3id.org/con-tax/components/aat-furn#300039526> ;
.
<https://w3id.org/con-tax/components/aat-furn#300167585>
  rdf:type owl:Class ;
  rdfs:comment "Benaming die door Chippendale wordt gebruikt voor rustbanken met twee hoofdeindes en een baldakijn."@nl ;
  rdfs:comment "Term used by Chippendale for double-headed couches with a canopy."@en ;
  rdfs:isDefinedBy <https://w3id.org/con-tax/components/aat-furn> ;
  rdfs:label "couch bed"@nl ;
  rdfs:label "couch beds"@en ;
  rdfs:label "couch beds"@nl ;
  rdfs:seeAlso <http://vocab.getty.edu/aat/300167585> ;
  rdfs:seeAlso wd:Q2894990 ;
  rdfs:subClassOf <https://w3id.org/con-tax/components/aat-furn#300038583> ;
.
<https://w3id.org/con-tax/components/aat-furn#300167586>
  rdf:type owl:Class ;
  rdfs:comment "Hangend openkast-systeem waarop porselein wordt getoond, vaak met latwerk aan de zijdes."@nl ;
  rdfs:comment "Open hanging shelves for displaying china, often with lattice work on the sides."@en ;
  rdfs:isDefinedBy <https://w3id.org/con-tax/components/aat-furn> ;
  rdfs:label "china shelves"@en ;
  rdfs:label "hangende porceleinkast"@nl ;
  rdfs:label "hangende porceleinkasten"@nl ;
  rdfs:seeAlso <http://vocab.getty.edu/aat/300167586> ;
  rdfs:subClassOf <https://w3id.org/con-tax/components/aat-furn#300037680> ;
.
<https://w3id.org/con-tax/components/aat-furn#300167587>
  rdf:type owl:Class ;
  rdfs:comment "Benaming van Chippendale voor luie stoelen met een hoge rugleuning die helemaal zijn opgevuld en gestoffeerd met wol."@nl ;
  rdfs:comment "Chippendale's term for high-backed easy chairs stuffed all over and upholstered in wool fabric."@en ;
  rdfs:isDefinedBy <https://w3id.org/con-tax/components/aat-furn> ;
  rdfs:label "cloath chair"@nl ;
  rdfs:label "cloath chairs"@en ;
  rdfs:label "cloath chairs"@nl ;
  rdfs:seeAlso <http://vocab.getty.edu/aat/300167587> ;
  rdfs:seeAlso wd:Q46641834 ;
  rdfs:subClassOf <https://w3id.org/con-tax/components/aat-furn#300037838> ;
.
<https://w3id.org/con-tax/components/aat-furn#300167588>
  rdf:type owl:Class ;
  rdfs:comment "Fire screens constructed of two folding leaves; many, but not all designs allow sliding of the panels to adjust coverage."@en ;
  rdfs:comment "Vuurschermen die worden gevormd door twee scharnierende bladen met schuifpanelen."@nl ;
  rdfs:isDefinedBy <https://w3id.org/con-tax/components/aat-furn> ;
  rdfs:label "double fire screens (furniture)"@en ;
  rdfs:label "double sliding fire screen"@nl ;
  rdfs:label "double sliding fire screens"@nl ;
  rdfs:seeAlso <http://vocab.getty.edu/aat/300167588> ;
  rdfs:subClassOf <https://w3id.org/con-tax/components/aat-furn#300037745> ;
  rdfs:subClassOf <https://w3id.org/con-tax/components/aat-furn#300265156> ;
.
<https://w3id.org/con-tax/components/aat-furn#300167589>
  rdf:type owl:Class ;
  rdfs:comment "Benaming die wordt gebruikt door Chippendale voor kleine geschilderde stoelen met onbesproken plaatsen die worden gebruikt bij shows."@nl ;
  rdfs:comment "Term used by Chippendale for small painted chairs with rush seats used at general entertainments."@en ;
  rdfs:isDefinedBy <https://w3id.org/con-tax/components/aat-furn> ;
  rdfs:label "rout chair"@nl ;
  rdfs:label "rout chairs"@en ;
  rdfs:label "rout chairs"@nl ;
  rdfs:seeAlso <http://vocab.getty.edu/aat/300167589> ;
  rdfs:subClassOf <https://w3id.org/con-tax/components/aat-furn#300037772> ;
.
<https://w3id.org/con-tax/components/aat-furn#300167590>
  rdf:type owl:Class ;
  rdfs:comment "Benaming die door Chippendale werd gebruikt voor lage bedden zonder enige bovenbouw die meestal door het personeel werden gebruikt."@nl ;
  rdfs:comment "Term used by Chippendale for low beds without any superstructure, generally used by servants."@en ;
  rdfs:isDefinedBy <https://w3id.org/con-tax/components/aat-furn> ;
  rdfs:label "stump bed"@nl ;
  rdfs:label "stump beds"@en ;
  rdfs:label "stump beds"@nl ;
  rdfs:seeAlso <http://vocab.getty.edu/aat/300167590> ;
  rdfs:subClassOf <https://w3id.org/con-tax/components/aat-furn#300038697> ;
.
<https://w3id.org/con-tax/components/aat-furn#300167602>
  rdf:type owl:Class ;
  rdfs:comment "Term die tijdens het midden van de 18e eeuw werd gebruikt voor leunstoelen met een gestoffeerde zitting en rug, een frame met houtsnijwerk en cabrioolpoten."@nl ;
  rdfs:comment "Term used during the mid-18th century for armchairs with upholstered seats and backs, carved frames and cabriole legs."@en ;
  rdfs:isDefinedBy <https://w3id.org/con-tax/components/aat-furn> ;
  rdfs:label "Franse armstoel"@nl ;
  rdfs:label "Franse armstoelen"@nl ;
  rdfs:label "French elbow chairs"@en ;
  rdfs:seeAlso <http://vocab.getty.edu/aat/300167602> ;
  rdfs:subClassOf <https://w3id.org/con-tax/components/aat-furn#300165321> ;
.
<https://w3id.org/con-tax/components/aat-furn#300170026>
  rdf:type owl:Class ;
  rdfs:comment "Windsor chairs with a bowlike back comprised of three sawn pieces of wood containing a central vertical back splat, sometimes spindles; common in the mid-19th century."@en ;
  rdfs:comment "Windsorstoelen met een boogvormige rugleuning die is opgebouwd uit drie uitgezaagde stukken hout met een verticaal middeblad in de rug, eventueel met spijlen. Ze kwamen veel voor in het midden van de 19e eeuw."@nl ;
  rdfs:isDefinedBy <https://w3id.org/con-tax/components/aat-furn> ;
  rdfs:label "balloon-back Windsor chairs"@en ;
  rdfs:label "balloon-back Windsorstoel"@nl ;
  rdfs:label "balloon-back Windsorstoelen"@nl ;
  rdfs:seeAlso <http://vocab.getty.edu/aat/300170026> ;
  rdfs:subClassOf <https://w3id.org/con-tax/components/aat-furn#300266583> ;
.
<https://w3id.org/con-tax/components/aat-furn#300170031>
  rdf:type owl:Class ;
  rdfs:comment "Windsor chairs having a back of medium height consisting of spindles contained within a bent bow that is anchored in the seat; may or may not have arms."@en ;
  rdfs:comment "Windsorstoelen met een middelmatig hoge rugleuning met spijlen, ingesloten door een gebogen regel die in de zitting is verankerd. Ze kunnen met of zonder armleuningen voorkomen."@nl ;
  rdfs:isDefinedBy <https://w3id.org/con-tax/components/aat-furn> ;
  rdfs:label "bow-back Windsor chairs"@en ;
  rdfs:label "bow-back Windsorstoel"@nl ;
  rdfs:label "bow-back Windsorstoelen"@nl ;
  rdfs:seeAlso <http://vocab.getty.edu/aat/300170031> ;
  rdfs:seeAlso wd:Q21550413 ;
  rdfs:subClassOf <https://w3id.org/con-tax/components/aat-furn#300266583> ;
.
<https://w3id.org/con-tax/components/aat-furn#300170039>
  rdf:type owl:Class ;
  rdfs:comment "Windsor armchairs having a back of medium height consisting of back spindles contained within a bent bow that continues forward to form arms; frequently with a back brace."@en ;
  rdfs:comment "Windsor-leunstoelen met een middelmatig hoge rugleuning met spijlen, ingesloten door een gebogen regel die naar voren doorloopt en zo de armleuningen vormt. Ze komen vaak voor met verstevigde rug."@nl ;
  rdfs:isDefinedBy <https://w3id.org/con-tax/components/aat-furn> ;
  rdfs:label "continuous-bow Windsor armchairs"@en ;
  rdfs:label "continuous-bow Windsorleunstoel"@nl ;
  rdfs:label "continuous-bow Windsorleunstoelen"@nl ;
  rdfs:seeAlso <http://vocab.getty.edu/aat/300170039> ;
  rdfs:subClassOf <https://w3id.org/con-tax/components/aat-furn#300266583> ;
.
<https://w3id.org/con-tax/components/aat-furn#300170046>
  rdf:type owl:Class ;
  rdfs:comment "'Windsorstoelen met een geniddeld hoge rugleuning die op een gedeeltelijk geopende waaier lijkt. De spijlen in de rug zijn aan de bovenregel bevestigd die naar de zijkant afbuigt en zo de bocht van de zitting volgt. Aan de uiteinden worden ze ondersteund door sterk gedraaide achterstijlen. Deze vorm heeft soms een verlengde rug- en armleuning die uitlopen in de achterstijl. Zulke stoelen hebben meestal een verstevigde rug."@nl ;
  rdfs:comment "Windsor side chairs having a back of medium height, approximating a partially opened fan, with the back spindles crowned by a crest rail curved laterally to follow the outside curve of the seat back and supported at the ends by heavy turned back posts. The form sometimes has an extended back and arms terminating in the back post. Such chairs usually have a back brace."@en ;
  rdfs:isDefinedBy <https://w3id.org/con-tax/components/aat-furn> ;
  rdfs:label "fan-back Windsor chairs"@en ;
  rdfs:label "fan-back Windsorstoel"@nl ;
  rdfs:label "fan-back Windsorstoelen"@nl ;
  rdfs:seeAlso <http://vocab.getty.edu/aat/300170046> ;
  rdfs:subClassOf <https://w3id.org/con-tax/components/aat-furn#300266583> ;
.
<https://w3id.org/con-tax/components/aat-furn#300170051>
  rdf:type owl:Class ;
  rdfs:comment "Windsor chairs with sawn back posts of gunstock shape; common in the mid-19th century."@en ;
  rdfs:comment "Windsorstoelen met uitgezaagde achterstijlen in de vorm van een geweerkolf. Ze kwamen veel voor in het midden van de 19e eeuw."@nl ;
  rdfs:isDefinedBy <https://w3id.org/con-tax/components/aat-furn> ;
  rdfs:label "gunstock Windsor chairs"@en ;
  rdfs:label "gunstock Windsorstoel"@nl ;
  rdfs:label "gunstock Windsorstoelen"@nl ;
  rdfs:seeAlso <http://vocab.getty.edu/aat/300170051> ;
  rdfs:subClassOf <https://w3id.org/con-tax/components/aat-furn#300266583> ;
.
<https://w3id.org/con-tax/components/aat-furn#300170054>
  rdf:type owl:Class ;
  rdfs:comment "Hoge Windsor-leunstoelen met een horizontale U-vormige armleuning met lange rugspijlen die zijn bevestigd aan de bovenregel die zijwaarts afbuigt en zo de buitenrand van de zitting volgt."@nl ;
  rdfs:comment "Tall Windsor armchairs with a horizontal U-shaped armrail and long back spindles crowned by a crest rail curved laterally to follow the outside curve of the seat back."@en ;
  rdfs:isDefinedBy <https://w3id.org/con-tax/components/aat-furn> ;
  rdfs:label "high-back Windsor chairs"@en ;
  rdfs:label "high-back Windsorstoel"@nl ;
  rdfs:label "high-back Windsorstoelen"@nl ;
  rdfs:seeAlso <http://vocab.getty.edu/aat/300170054> ;
  rdfs:subClassOf <https://w3id.org/con-tax/components/aat-furn#300266583> ;
.
<https://w3id.org/con-tax/components/aat-furn#300170063>
  rdf:type owl:Class ;
  rdfs:comment "Windsor armchairs with a low back that terminates at arm level and usually is comprised of a three-piece sawn arm rail that follows the outside curve of the seat."@en ;
  rdfs:comment "Windsor-leunstoelen met een lage rugleuning op armhoogte die meestal  bestaat uit een uitgezaagde driedelige armleuning die de buitenrand van de zitting volgt."@nl ;
  rdfs:isDefinedBy <https://w3id.org/con-tax/components/aat-furn> ;
  rdfs:label "low-back Windsor chairs"@en ;
  rdfs:label "low-back Windsorstoel"@nl ;
  rdfs:label "low-back Windsorstoelen"@nl ;
  rdfs:seeAlso <http://vocab.getty.edu/aat/300170063> ;
  rdfs:subClassOf <https://w3id.org/con-tax/components/aat-furn#300266583> ;
.
<https://w3id.org/con-tax/components/aat-furn#300170072>
  rdf:type owl:Class ;
  rdfs:comment "Windsor armchairs with a horizontal U-shaped arm rail and back of medium height consisting of spindles contained within a curved bow anchored in the arm rail."@en ;
  rdfs:comment "Windsor-leunstoelen met een U-vormige armleuning en een middelmatig hoge rugleuning, bestaande uit spijlen die worden omsloten door een gebogen rail die in de armleuning is verankerd."@nl ;
  rdfs:isDefinedBy <https://w3id.org/con-tax/components/aat-furn> ;
  rdfs:label "sack-back Windsor chairs"@en ;
  rdfs:label "sack-back Windsorstoel"@nl ;
  rdfs:label "sack-back Windsorstoelen"@nl ;
  rdfs:seeAlso <http://vocab.getty.edu/aat/300170072> ;
  rdfs:subClassOf <https://w3id.org/con-tax/components/aat-furn#300266583> ;
.
<https://w3id.org/con-tax/components/aat-furn#300170079>
  rdf:type owl:Class ;
  rdfs:comment "Benaming die wordt gebruikt voor elke Windsorstoel, met een vierkante of ronde rugleuning, die een verticaal middenblad in de rug heeft."@nl ;
  rdfs:comment "Term generally applied to any Windsor chair, of square or round back, having a central vertical back splat."@en ;
  rdfs:isDefinedBy <https://w3id.org/con-tax/components/aat-furn> ;
  rdfs:label "splat-back Windsor chairs"@en ;
  rdfs:label "splat-back Windsorstoel"@nl ;
  rdfs:label "splat-back Windsorstoelen"@nl ;
  rdfs:seeAlso <http://vocab.getty.edu/aat/300170079> ;
  rdfs:seeAlso wd:Q21551001 ;
  rdfs:subClassOf <https://w3id.org/con-tax/components/aat-furn#300266583> ;
.
<https://w3id.org/con-tax/components/aat-furn#300170083>
  rdf:type owl:Class ;
  rdfs:comment "Benaming die werd geïntroduceerd in de 19e eeuw voor elke Windsorstoel, met of zonder armleuningen, die een vierkante of bijna vierkante rugleuning heeft."@nl ;
  rdfs:comment "Term introduced in the 19th century for any Windsor chair, with or without arms, of a square or nearly square back."@en ;
  rdfs:isDefinedBy <https://w3id.org/con-tax/components/aat-furn> ;
  rdfs:label "square-back Windsor chairs"@en ;
  rdfs:label "square-back Windsorstoel"@nl ;
  rdfs:label "square-back Windsorstoelen"@nl ;
  rdfs:seeAlso <http://vocab.getty.edu/aat/300170083> ;
  rdfs:subClassOf <https://w3id.org/con-tax/components/aat-furn#300266583> ;
.
<https://w3id.org/con-tax/components/aat-furn#300170092>
  rdf:type owl:Class ;
  rdfs:comment "Square-back Windsor chairs with narrow vertical lath instead of round spindles."@en ;
  rdfs:comment "Square-back Windsorstoelen met smalle, verticale latten in plaats van ronde spijlen."@nl ;
  rdfs:isDefinedBy <https://w3id.org/con-tax/components/aat-furn> ;
  rdfs:label "lath-back Windsor chairs"@en ;
  rdfs:label "lath-back Windsorstoel"@nl ;
  rdfs:label "lath-back Windsorstoelen"@nl ;
  rdfs:seeAlso <http://vocab.getty.edu/aat/300170092> ;
  rdfs:subClassOf <https://w3id.org/con-tax/components/aat-furn#300170083> ;
.
<https://w3id.org/con-tax/components/aat-furn#300170097>
  rdf:type owl:Class ;
  rdfs:comment "Elegante Windsorstoelen met een vierkante rugleuning naar de ontwerpen van Sheraton. Ze kwamen in Engeland voor in de omgeving van Mendlesham aan het begin van de 19e eeuw."@nl ;
  rdfs:comment "Fancy Windsor chairs of square-back based on Sheraton's designs, and found in the region of Mendlesham, England in the early 19th century."@en ;
  rdfs:isDefinedBy <https://w3id.org/con-tax/components/aat-furn> ;
  rdfs:label "Mendlesham chairs"@en ;
  rdfs:label "Mendlesham-stoel"@nl ;
  rdfs:label "Mendlesham-stoelen"@nl ;
  rdfs:seeAlso <http://vocab.getty.edu/aat/300170097> ;
  rdfs:subClassOf <https://w3id.org/con-tax/components/aat-furn#300170083> ;
.
<https://w3id.org/con-tax/components/aat-furn#300170103>
  rdf:type owl:Class ;
  rdfs:comment "Square-back Windsor chairs with a turned cross piece framed at the top of the back posts and accompanied by one or two horizontal cross slats at mid-back and sometimes with short spindles between the seat and lower slat."@en ;
  rdfs:comment "Square-back Windsorstoelen met een gedraaide dwarsverbinding  bovenop de achterstijlen en één of twee horizontale dwarslatten midden in de rug. Soms hebben ze korte spijlen tussen de zitting en de onderste dwarslat."@nl ;
  rdfs:isDefinedBy <https://w3id.org/con-tax/components/aat-furn> ;
  rdfs:label "roll-top Windsor chairs"@en ;
  rdfs:label "roll-top Windsorstoel"@nl ;
  rdfs:label "roll-top Windsorstoelen"@nl ;
  rdfs:seeAlso <http://vocab.getty.edu/aat/300170103> ;
  rdfs:subClassOf <https://w3id.org/con-tax/components/aat-furn#300170083> ;
.
<https://w3id.org/con-tax/components/aat-furn#300170108>
  rdf:type owl:Class ;
  rdfs:comment "'@ Square-back Windsor chairs' met een middenblad aan de bovenkant van de rugleuning die tussen de achterstijlen wordt geplaatst."@nl ;
  rdfs:comment "Square-back Windsor chairs with a slat across the upper back framed between the back posts."@en ;
  rdfs:isDefinedBy <https://w3id.org/con-tax/components/aat-furn> ;
  rdfs:label "slat-back Windsor chairs"@en ;
  rdfs:label "slat-back Windsorstoel"@nl ;
  rdfs:label "slat-back Windsorstoelen"@nl ;
  rdfs:seeAlso <http://vocab.getty.edu/aat/300170108> ;
  rdfs:subClassOf <https://w3id.org/con-tax/components/aat-furn#300170083> ;
.
<https://w3id.org/con-tax/components/aat-furn#300170112>
  rdf:type owl:Class ;
  rdfs:comment "Square-back Windsor chairs with a single turned rod across the top usually capping the back posts."@en ;
  rdfs:comment "Square-back Windsorstoelen met een enkele gedraaide staaf aan de bovenkant, die meestal de achterstijlen overdekt."@nl ;
  rdfs:isDefinedBy <https://w3id.org/con-tax/components/aat-furn> ;
  rdfs:label "single rod-back Windsor chairs"@en ;
  rdfs:label "single-rod-back Windsorstoel"@nl ;
  rdfs:label "single-rod-back Windsorstoelen"@nl ;
  rdfs:seeAlso <http://vocab.getty.edu/aat/300170112> ;
  rdfs:subClassOf <https://w3id.org/con-tax/components/aat-furn#300170083> ;
.
<https://w3id.org/con-tax/components/aat-furn#300170116>
  rdf:type owl:Class ;
  rdfs:comment "Square-back Windsor chairs with two turned rods across the top, the upper rod either capping the back posts or framed between them."@en ;
  rdfs:comment "Square-back Windsorstoelen met twee gedraaide staven aan de bovenkant waarbij de bovenste staaf de achterstijlen overdekt of tussen ze in wordt geplaatst."@nl ;
  rdfs:isDefinedBy <https://w3id.org/con-tax/components/aat-furn> ;
  rdfs:label "double rod-back Windsor chairs"@en ;
  rdfs:label "double-rod-back Windsorstoel"@nl ;
  rdfs:label "double-rod-back Windsorstoelen"@nl ;
  rdfs:seeAlso <http://vocab.getty.edu/aat/300170116> ;
  rdfs:subClassOf <https://w3id.org/con-tax/components/aat-furn#300170083> ;
.
<https://w3id.org/con-tax/components/aat-furn#300170125>
  rdf:type owl:Class ;
  rdfs:comment "Square-back Windsor chairs with a cross panel capping and usually extending beyond the top of the back posts. Such chairs can have backs consisting of long spindles, cross slats, one or more cross slats with short spindles, or a vertical back splat."@en ;
  rdfs:comment "Square-back Windsorstoelen met een dwarspaneel op de achterstijlen dat meestal buiten de achterstijlen uitsteekt. Zulke stoelen kunnen een rugleuning hebben die bestaat uit lange spijlen, dwarslatten, één of meer dwarslatten met korte spijlen of een verticaal middenblad in de rug."@nl ;
  rdfs:isDefinedBy <https://w3id.org/con-tax/components/aat-furn> ;
  rdfs:label "tablet-top Windsor chairs"@en ;
  rdfs:label "tablet-top Windsorstoel"@nl ;
  rdfs:label "tablet-top Windsorstoelen"@nl ;
  rdfs:seeAlso <http://vocab.getty.edu/aat/300170125> ;
  rdfs:subClassOf <https://w3id.org/con-tax/components/aat-furn#300170083> ;
.
<https://w3id.org/con-tax/components/aat-furn#300170131>
  rdf:type owl:Class ;
  rdfs:comment "Any Windsor chair having one shaped, flat leaf, in lieu of a standard arm, used as a writing surface."@en ;
  rdfs:comment "Elke Windsorstoel die aan een kant in plaats van een standaard armleuning een gevormd, plat blad heeft dat als schrijfondergrond wordt gebruikt."@nl ;
  rdfs:isDefinedBy <https://w3id.org/con-tax/components/aat-furn> ;
  rdfs:label "writing-arm Windsor chairs"@en ;
  rdfs:label "writing-arm Windsorstoel"@nl ;
  rdfs:label "writing-arm Windsorstoelen"@nl ;
  rdfs:seeAlso <http://vocab.getty.edu/aat/300170131> ;
  rdfs:seeAlso wd:Q21551102 ;
  rdfs:subClassOf <https://w3id.org/con-tax/components/aat-furn#300038252> ;
  rdfs:subClassOf <https://w3id.org/con-tax/components/aat-furn#300266583> ;
.
<https://w3id.org/con-tax/components/aat-furn#300170137>
  rdf:type owl:Class ;
  rdfs:comment "Standaarden met meestal drie poten die zijn verstevigd met dwarsbalken en direct in een klein, meestal rond blad steken."@nl ;
  rdfs:comment "Stands usually having three legs braced with stretchers which socket directly into a small, usually round, top."@en ;
  rdfs:isDefinedBy <https://w3id.org/con-tax/components/aat-furn> ;
  rdfs:label "Windsor stands"@en ;
  rdfs:label "Windsorstandaard"@nl ;
  rdfs:label "Windsorstandaarden"@nl ;
  rdfs:seeAlso <http://vocab.getty.edu/aat/300170137> ;
  rdfs:subClassOf <https://w3id.org/con-tax/components/aat-furn#300039767> ;
.
<https://w3id.org/con-tax/components/aat-furn#300170140>
  rdf:type owl:Class ;
  rdfs:comment "Tables with a top, usually round, supported on legs which socket directly into the top; such tables have three legs braced by stretchers."@en ;
  rdfs:comment "Tafels met een meestal rond blad met poten die direct in het blad steken. Zulke tafels hebben drie poten die met dwarsbalken zijn verstevigd."@nl ;
  rdfs:isDefinedBy <https://w3id.org/con-tax/components/aat-furn> ;
  rdfs:label "Windsor tables"@en ;
  rdfs:label "Windsortafel"@nl ;
  rdfs:label "Windsortafels"@nl ;
  rdfs:seeAlso <http://vocab.getty.edu/aat/300170140> ;
  rdfs:subClassOf <https://w3id.org/con-tax/components/aat-furn#300039548> ;
.
<https://w3id.org/con-tax/components/aat-furn#300170143>
  rdf:type owl:Class ;
  rdfs:comment "Any Windsor chair with the legs supported on bends for rocking."@en ;
  rdfs:comment "Elke  Windsorstoel waarvan de poten op schommelbalken rusten."@nl ;
  rdfs:isDefinedBy <https://w3id.org/con-tax/components/aat-furn> ;
  rdfs:label "Windsor rocking chairs"@en ;
  rdfs:label "Windsor schommelstoel"@nl ;
  rdfs:label "Windsor schommelstoelen"@nl ;
  rdfs:seeAlso <http://vocab.getty.edu/aat/300170143> ;
  rdfs:subClassOf <https://w3id.org/con-tax/components/aat-furn#300038273> ;
  rdfs:subClassOf <https://w3id.org/con-tax/components/aat-furn#300266583> ;
.
<https://w3id.org/con-tax/components/aat-furn#300170149>
  rdf:type owl:Class ;
  rdfs:comment "Krukken van variërende hoogte, bestaande uit een horizontale plank die uiteenlopende vormen kan hebben, met drie of vier gedraaide of geschaafde poten, vaak verstevigd met dwarsbalken, die direkt in de zitting worden bevestigd.."@nl ;
  rdfs:comment "Stools of varied height consisting of a horizontal plank of varied shape supported on three or four turned or shaved legs, frequently braced by stretchers, which socket directly into the plank."@en ;
  rdfs:isDefinedBy <https://w3id.org/con-tax/components/aat-furn> ;
  rdfs:label "Windsor krukje"@nl ;
  rdfs:label "Windsor krukjes"@nl ;
  rdfs:label "Windsor stools"@en ;
  rdfs:seeAlso <http://vocab.getty.edu/aat/300170149> ;
  rdfs:subClassOf <https://w3id.org/con-tax/components/aat-furn#300038418> ;
.
<https://w3id.org/con-tax/components/aat-furn#300170152>
  rdf:type owl:Class ;
  rdfs:comment "Chairs with tall legs and a high seat, such as those used at counters."@en ;
  rdfs:comment "Stoelen met lange poten en een hoge zitting, zoals de stoelen die achter toonbanken worden gebruikt."@nl ;
  rdfs:isDefinedBy <https://w3id.org/con-tax/components/aat-furn> ;
  rdfs:label "hoge stoel"@nl ;
  rdfs:label "hoge stoelen"@nl ;
  rdfs:label "tall chairs"@en ;
  rdfs:seeAlso <http://vocab.getty.edu/aat/300170152> ;
  rdfs:subClassOf <https://w3id.org/con-tax/components/aat-furn#300037772> ;
.
<https://w3id.org/con-tax/components/aat-furn#300170221>
  rdf:type owl:Class ;
  rdfs:comment "Cantilever chairs that are considered a major development in modern furniture. Mart Stam created the first experimental models with gas pipes and flanges and developed the principle of cantilevering chair supports without four legs. Later innovations allowed the use of tubular steel. Others such as Marcel Breuer and Mies van der Rohe designed their own variations on the principle."@en ;
  rdfs:isDefinedBy <https://w3id.org/con-tax/components/aat-furn> ;
  rdfs:label "S chairs (chair forms)"@en ;
  rdfs:label "S-vormige stoel"@nl ;
  rdfs:label "S-vormige stoelen"@nl ;
  rdfs:seeAlso <http://vocab.getty.edu/aat/300170221> ;
  rdfs:subClassOf <https://w3id.org/con-tax/components/aat-furn#300037772> ;
.
<https://w3id.org/con-tax/components/aat-furn#300170227>
  rdf:type owl:Class ;
  rdfs:comment "Chair designed by Ludwig Mies van der Rohe ca. 1929-1930 having a cantilevered construction of chromed steel and leather or parchment upholstery. Prized as an example of Bauhaus design."@en ;
  rdfs:isDefinedBy <https://w3id.org/con-tax/components/aat-furn> ;
  rdfs:label "Brno chairs"@en ;
  rdfs:label "Brno-stoel"@nl ;
  rdfs:label "Brno-stoelen"@nl ;
  rdfs:seeAlso <http://vocab.getty.edu/aat/300170227> ;
  rdfs:seeAlso wd:Q2738352 ;
  rdfs:subClassOf <https://w3id.org/con-tax/components/aat-furn#300037772> ;
.
<https://w3id.org/con-tax/components/aat-furn#300170233>
  rdf:type owl:Class ;
  rdfs:comment "A chair designed by Marcel Breuer ca. 1925 that features a tubular chromed-steel structure and strips of leather used as seat, back, and arm support. This chair is often used as a prime example of the design aesthetic of the Bauhaus during this period, and of mid-20th century modernist design in general, due to the innovation of the use of tubular steel in its construction."@en ;
  rdfs:isDefinedBy <https://w3id.org/con-tax/components/aat-furn> ;
  rdfs:label "Wassily chairs"@en ;
  rdfs:label "Wassilystoel"@nl ;
  rdfs:label "Wassilystoelen"@nl ;
  rdfs:seeAlso <http://vocab.getty.edu/aat/300170233> ;
  rdfs:seeAlso wd:Q2629013 ;
  rdfs:subClassOf <https://w3id.org/con-tax/components/aat-furn#300037772> ;
.
<https://w3id.org/con-tax/components/aat-furn#300170239>
  rdf:type owl:Class ;
  rdfs:comment "Reclining chaise lounges framed in tubular aluminum. They have rocker bases and stretched canvas supports and were intended to be used indoors or outdoors. Designed by Bartolucci and Waldman in 1947, based on a previous lounge by Corbusier."@en ;
  rdfs:isDefinedBy <https://w3id.org/con-tax/components/aat-furn> ;
  rdfs:label "Barwa chairs"@en ;
  rdfs:label "Barwa-stoel"@nl ;
  rdfs:label "Barwa-stoelen"@nl ;
  rdfs:seeAlso <http://vocab.getty.edu/aat/300170239> ;
  rdfs:subClassOf <https://w3id.org/con-tax/components/aat-furn#300037772> ;
.
<https://w3id.org/con-tax/components/aat-furn#300170242>
  rdf:type owl:Class ;
  rdfs:comment "Upholstered fiberglass-shell armchairs designed by Joe Colombo in 1964 and manufactured by Comfort Italy from 1965. The 'Elda 1005' is considered to be the first large armchair made out of fiberglass. A large self-supporting shell rotates on a base, the inside of which is upholstered in leather."@en ;
  rdfs:isDefinedBy <https://w3id.org/con-tax/components/aat-furn> ;
  rdfs:label "Elda 1005 upholstered chair"@nl ;
  rdfs:label "Elda 1005 upholstered chairs"@en ;
  rdfs:label "Elda 1005 upholstered chairs"@nl ;
  rdfs:seeAlso <http://vocab.getty.edu/aat/300170242> ;
  rdfs:subClassOf <https://w3id.org/con-tax/components/aat-furn#300037772> ;
.
<https://w3id.org/con-tax/components/aat-furn#300170245>
  rdf:type owl:Class ;
  rdfs:comment "Chair design by Mies van der Rohe for his German Pavilion at the Barcelona Exposition of 1929. Only two chairs were made for this purpose, but the design proved popular and has been in almost continuous production since 1929."@en ;
  rdfs:isDefinedBy <https://w3id.org/con-tax/components/aat-furn> ;
  rdfs:label "Barcelona chairs"@en ;
  rdfs:label "Barcelonastoel"@nl ;
  rdfs:label "Barcelonastoelen"@nl ;
  rdfs:seeAlso <http://vocab.getty.edu/aat/300170245> ;
  rdfs:seeAlso wd:Q733154 ;
  rdfs:subClassOf <https://w3id.org/con-tax/components/aat-furn#300037772> ;
.
<https://w3id.org/con-tax/components/aat-furn#300170249>
  rdf:type owl:Class ;
  rdfs:comment "Chairs designed in Buenos Aires by Antonio Bonet, Juan Kurchan and Jorge Ferrari Hardoy, having steel frames and slinglike one-piece fabric or leather seats. Though commonly referred to as a butterfly chair because of the distinctive shape of its frame, the official name is the B.K.F. Chair, which credits its three designers. The lightweight and inexpensive chair became hugely popular in the U.S. from the 1950s, particularly on the West Coast, where it was frequently used as outdoor seating. The chair was produced by Artek-Pascoe from 1941 to 1948. Knoll Associates acquired U.S. rights to the design in the late 1940s. Unauthorized copies continue to be made."@en ;
  rdfs:isDefinedBy <https://w3id.org/con-tax/components/aat-furn> ;
  rdfs:label "Hardoy chairs"@en ;
  rdfs:label "Hardoystoel"@nl ;
  rdfs:label "Hardoystoelen"@nl ;
  rdfs:seeAlso <http://vocab.getty.edu/aat/300170249> ;
  rdfs:subClassOf <https://w3id.org/con-tax/components/aat-furn#300038126> ;
.
<https://w3id.org/con-tax/components/aat-furn#300170256>
  rdf:type owl:Class ;
  rdfs:comment "Modernist easy chair design created by Arne Jacobsen in 1958 for the SAS Royal Hotel in Copenhagen. "@en ;
  rdfs:isDefinedBy <https://w3id.org/con-tax/components/aat-furn> ;
  rdfs:label "egg chairs"@en ;
  rdfs:label "eifauteuil"@nl ;
  rdfs:label "eifauteuils"@nl ;
  rdfs:seeAlso <http://vocab.getty.edu/aat/300170256> ;
  rdfs:seeAlso wd:Q1301042 ;
  rdfs:subClassOf <https://w3id.org/con-tax/components/aat-furn#300037772> ;
.
<https://w3id.org/con-tax/components/aat-furn#300170262>
  rdf:type owl:Class ;
  rdfs:comment "Modernist chair designed for Knoll International in 1952 by Harry Bertoia. The basic form of the chair is constructed from wire rods welded together. There are many variations in upholstery and finish."@en ;
  rdfs:isDefinedBy <https://w3id.org/con-tax/components/aat-furn> ;
  rdfs:label "diamond chair"@nl ;
  rdfs:label "diamond chairs"@en ;
  rdfs:label "diamond chairs"@nl ;
  rdfs:seeAlso <http://vocab.getty.edu/aat/300170262> ;
  rdfs:subClassOf <https://w3id.org/con-tax/components/aat-furn#300037772> ;
.
<https://w3id.org/con-tax/components/aat-furn#300170271>
  rdf:type owl:Class ;
  rdfs:comment "Modernist armchair design in beech and teak wood by Peter Hvidt and Orla Molgaard Nielsen, ca. 1947."@en ;
  rdfs:isDefinedBy <https://w3id.org/con-tax/components/aat-furn> ;
  rdfs:label "ax chairs"@en ;
  rdfs:label "ax-stoel"@nl ;
  rdfs:label "ax-stoelen"@nl ;
  rdfs:seeAlso <http://vocab.getty.edu/aat/300170271> ;
  rdfs:subClassOf <https://w3id.org/con-tax/components/aat-furn#300037772> ;
.
<https://w3id.org/con-tax/components/aat-furn#300170274>
  rdf:type owl:Class ;
  rdfs:comment "Refers to a specific design of folding chair first created by Giancarlo Piretti in the 1960s, characterized as a folding chair that could be easily stacked and opened with one hand, composed of a steel or aluminum frame with a press-molded transparent plastic backrest and seat."@en ;
  rdfs:isDefinedBy <https://w3id.org/con-tax/components/aat-furn> ;
  rdfs:label "Plia folding chairs"@en ;
  rdfs:label "Plia vouwstoel"@nl ;
  rdfs:label "Plia vouwstoelen"@nl ;
  rdfs:seeAlso <http://vocab.getty.edu/aat/300170274> ;
  rdfs:subClassOf <https://w3id.org/con-tax/components/aat-furn#300244770> ;
.
<https://w3id.org/con-tax/components/aat-furn#300170280>
  rdf:type owl:Class ;
  rdfs:comment "Modernist folding chair with a polished alumnum structure and leather seat designed by Gian Carlo Piretti for Anonima Castelli ca. 1970."@en ;
  rdfs:isDefinedBy <https://w3id.org/con-tax/components/aat-furn> ;
  rdfs:label "Plona folding armchairs"@en ;
  rdfs:label "Plona vouwleunstoel"@nl ;
  rdfs:label "Plona vouwleunstoelen"@nl ;
  rdfs:seeAlso <http://vocab.getty.edu/aat/300170280> ;
  rdfs:subClassOf <https://w3id.org/con-tax/components/aat-furn#300244770> ;
.
<https://w3id.org/con-tax/components/aat-furn#300170285>
  rdf:type owl:Class ;
  rdfs:comment "Cantilevered chair designed in 1928 by Marcel Breuer at the Bauhaus, Dessau. Constructed of bent chromed tubular steel, wood, and cane, it has proved one of the most popular modernist chair designs and remains in production."@en ;
  rdfs:isDefinedBy <https://w3id.org/con-tax/components/aat-furn> ;
  rdfs:label "Cesca chairs"@en ;
  rdfs:label "Cescastoel"@nl ;
  rdfs:label "Cescastoelen"@nl ;
  rdfs:seeAlso <http://vocab.getty.edu/aat/300170285> ;
  rdfs:subClassOf <https://w3id.org/con-tax/components/aat-furn#300037772> ;
.
<https://w3id.org/con-tax/components/aat-furn#300170291>
  rdf:type owl:Class ;
  rdfs:comment "Refers to a series of cantilevered chair designs by Ludwig Mies van der Rohe first realized ca. 1927. the structure is of tubular steel and is regarded as a prime example of this type of furniture design emerging from the Bauhaus in the 1920s."@en ;
  rdfs:isDefinedBy <https://w3id.org/con-tax/components/aat-furn> ;
  rdfs:label "MR chairs"@en ;
  rdfs:label "MR-stoel"@nl ;
  rdfs:label "MR-stoelen"@nl ;
  rdfs:seeAlso <http://vocab.getty.edu/aat/300170291> ;
  rdfs:subClassOf <https://w3id.org/con-tax/components/aat-furn#300037772> ;
.
<https://w3id.org/con-tax/components/aat-furn#300170297>
  rdf:type owl:Class ;
  rdfs:comment "Brede, ronde stoelen bestaande uit een voorgevormd plastic geraamte, met schuimrubber gevulde bekleding van wollen stof, op een buisvormig frame; ontworpen door Eero Saarinen en geïntroduceerd in het midden van de jaren 40 van de 20ste eeuw; gewoonlijk gecombineerd met een bijpassend gestoffeerd voetenbankje."@nl ;
  rdfs:comment "Wide, contoured chairs consisting of a molded plastic shell covered with foam rubber padding and wool cloth set on a tubular steel frame; designed by Eero Saarinen and introduced in the mid-1940s; usually accompanied by a matching upholstered footstool."@en ;
  rdfs:isDefinedBy <https://w3id.org/con-tax/components/aat-furn> ;
  rdfs:label "womb chair"@nl ;
  rdfs:label "womb chairs"@en ;
  rdfs:label "womb chairs"@nl ;
  rdfs:seeAlso <http://vocab.getty.edu/aat/300170297> ;
  rdfs:subClassOf <https://w3id.org/con-tax/components/aat-furn#300037772> ;
.
<https://w3id.org/con-tax/components/aat-furn#300170301>
  rdf:type owl:Class ;
  rdfs:comment "Modernist chair designed ca. 1958. The chair features a foam and upholstery-covered molded shell of synthetic material on an aluminum swivel base."@en ;
  rdfs:isDefinedBy <https://w3id.org/con-tax/components/aat-furn> ;
  rdfs:label "swan chairs"@en ;
  rdfs:label "zwaanfauteuil"@nl ;
  rdfs:label "zwaanfauteuils"@nl ;
  rdfs:seeAlso <http://vocab.getty.edu/aat/300170301> ;
  rdfs:seeAlso wd:Q1290874 ;
  rdfs:subClassOf <https://w3id.org/con-tax/components/aat-furn#300037772> ;
.
<https://w3id.org/con-tax/components/aat-furn#300170305>
  rdf:type owl:Class ;
  rdfs:comment "Modernist chair designed by Hans J. Wegner ca. 1950, and manufactured by Carl Hansen. The frame is of beech and the seat is constructed of woven paper cord. Part of the backrest is in the form of the letter 'Y,' from which the chair derived its name."@en ;
  rdfs:isDefinedBy <https://w3id.org/con-tax/components/aat-furn> ;
  rdfs:label "Y-chairs"@en ;
  rdfs:label "Y-framestoel"@nl ;
  rdfs:label "Y-framestoelen"@nl ;
  rdfs:seeAlso <http://vocab.getty.edu/aat/300170305> ;
  rdfs:subClassOf <https://w3id.org/con-tax/components/aat-furn#300037772> ;
.
<https://w3id.org/con-tax/components/aat-furn#300170309>
  rdf:type owl:Class ;
  rdfs:comment "Armchairs developed in the mid-twentieth century, with foam rubber upholstery on the back and seat, and a characteristic \"floating\" seat which rests on only the two front legs and a crossbar running between the side slats. The design originated with Danish architect and furniture designer, Finn Juhl (1912-1989)."@en ;
  rdfs:comment "Leunstoelen, ontwikkeld in het midden van de 20ste eeuw, met stoffering van schuimrubber op rug en zitting, en een karakteristieke ‘zwevende’ zitting die slechts rust op twee voorpoten en een dwarsbalk tussen de zijlatten."@nl ;
  rdfs:isDefinedBy <https://w3id.org/con-tax/components/aat-furn> ;
  rdfs:label "136 armchair"@nl ;
  rdfs:label "136 armchairs"@en ;
  rdfs:label "136 armchairs"@nl ;
  rdfs:seeAlso <http://vocab.getty.edu/aat/300170309> ;
  rdfs:subClassOf <https://w3id.org/con-tax/components/aat-furn#300037776> ;
.
<https://w3id.org/con-tax/components/aat-furn#300170371>
  rdf:type owl:Class ;
  rdfs:comment "Roman couch intended to seat six for dining."@en ;
  rdfs:isDefinedBy <https://w3id.org/con-tax/components/aat-furn> ;
  rdfs:label "biclinia"@en ;
  rdfs:label "biclinia"@nl ;
  rdfs:label "biclinium"@nl ;
  rdfs:seeAlso <http://vocab.getty.edu/aat/300170371> ;
  rdfs:subClassOf <https://w3id.org/con-tax/components/aat-furn#300038583> ;
.
<https://w3id.org/con-tax/components/aat-furn#300170373>
  rdf:type owl:Class ;
  rdfs:comment "A Roman seat or bench for two persons, though usually occupied by only one for festivals, etc."@en ;
  rdfs:isDefinedBy <https://w3id.org/con-tax/components/aat-furn> ;
  rdfs:label "bisellia"@en ;
  rdfs:label "bisellia"@nl ;
  rdfs:label "bisellia's"@nl ;
  rdfs:seeAlso <http://vocab.getty.edu/aat/300170373> ;
  rdfs:subClassOf <https://w3id.org/con-tax/components/aat-furn#300038493> ;
.
<https://w3id.org/con-tax/components/aat-furn#300170801>
  rdf:type owl:Class ;
  rdfs:comment "Elevated stands with a sloping top and usually a ledge at the bottom of the slope designed to support a book or script in a convenient position for a reader standing before it. A lectern may be placed on a table or mounted on a pedestal. A lectern In a church is usually situated in the chancel, sometimes inside a rood screen or tribune."@en ;
  rdfs:comment "Standaarden met een schuin blad en meestal een rand aan de onderkant van het blad om een boek of geschrift te ondersteunen zodat de lezer die ervoor staat het makkelijk kan lezen."@nl ;
  rdfs:isDefinedBy <https://w3id.org/con-tax/components/aat-furn> ;
  rdfs:label "lecterns"@en ;
  rdfs:label "lessenaar"@nl ;
  rdfs:label "lessenaars"@nl ;
  rdfs:label "lezenaar"@nl ;
  rdfs:label "lezenaars"@nl ;
  rdfs:seeAlso <http://vocab.getty.edu/aat/300170801> ;
  rdfs:seeAlso wd:Q390539 ;
  rdfs:subClassOf <https://w3id.org/con-tax/components/aat-furn#300039767> ;
.
<https://w3id.org/con-tax/components/aat-furn#300170813>
  rdf:type owl:Class ;
  rdfs:comment "Tall wooden cupboards with holes for ventilation, originally referring to livery cupboards used for storing loaves of bread that were doled out to poor persons, often in churches."@en ;
  rdfs:isDefinedBy <https://w3id.org/con-tax/components/aat-furn> ;
  rdfs:label "dole cupboard"@nl ;
  rdfs:label "dole cupboards"@en ;
  rdfs:label "dole cupboards"@nl ;
  rdfs:seeAlso <http://vocab.getty.edu/aat/300170813> ;
  rdfs:subClassOf <https://w3id.org/con-tax/components/aat-furn#300039183> ;
.
<https://w3id.org/con-tax/components/aat-furn#300170824>
  rdf:type owl:Class ;
  rdfs:comment "Half-chests of drawers, made for use in a small study or lobby."@en ;
  rdfs:isDefinedBy <https://w3id.org/con-tax/components/aat-furn> ;
  rdfs:label "lobby chests"@en ;
  rdfs:label "lobbykist"@nl ;
  rdfs:label "lobbykisten"@nl ;
  rdfs:seeAlso <http://vocab.getty.edu/aat/300170824> ;
  rdfs:subClassOf <https://w3id.org/con-tax/components/aat-furn#300038992> ;
.
<https://w3id.org/con-tax/components/aat-furn#300170829>
  rdf:type owl:Class ;
  rdfs:comment "Early form of footstool that was reproduced in great numbers during the 19th century. Thebes stools generally have concave tops, with flared legs and cross bracing. "@en ;
  rdfs:isDefinedBy <https://w3id.org/con-tax/components/aat-furn> ;
  rdfs:label "Thebe krukje"@nl ;
  rdfs:label "Thebe krukjes"@nl ;
  rdfs:label "Thebes stools"@en ;
  rdfs:seeAlso <http://vocab.getty.edu/aat/300170829> ;
  rdfs:subClassOf <https://w3id.org/con-tax/components/aat-furn#300038418> ;
.
<https://w3id.org/con-tax/components/aat-furn#300170858>
  rdf:type owl:Class ;
  rdfs:comment "Speciale tafel om oesters aan te eten. Ze waren rond, met een gat in het midden waaronder een mandje stond voor de lege schelpen."@nl ;
  rdfs:comment "Specialized form of table at which one ate oysters; circular in form with a hole in the center, under which stood a basket for the empty shells."@en ;
  rdfs:isDefinedBy <https://w3id.org/con-tax/components/aat-furn> ;
  rdfs:label "oestertafel"@nl ;
  rdfs:label "oestertafels"@nl ;
  rdfs:label "oyster tables"@en ;
  rdfs:seeAlso <http://vocab.getty.edu/aat/300170858> ;
  rdfs:subClassOf <https://w3id.org/con-tax/components/aat-furn#300039548> ;
.
<https://w3id.org/con-tax/components/aat-furn#300170864>
  rdf:type owl:Class ;
  rdfs:comment "Desks designed to be mounted on the surface of walls with no secondary support. These usually incorporate a folding or sliding work surface incorporated into a cabinet for storage."@en ;
  rdfs:isDefinedBy <https://w3id.org/con-tax/components/aat-furn> ;
  rdfs:label "muurbureau"@nl ;
  rdfs:label "muurbureaus"@nl ;
  rdfs:label "wall desks"@en ;
  rdfs:seeAlso <http://vocab.getty.edu/aat/300170864> ;
  rdfs:subClassOf <https://w3id.org/con-tax/components/aat-furn#300039338> ;
.
<https://w3id.org/con-tax/components/aat-furn#300170867>
  rdf:type owl:Class ;
  rdfs:comment "Cabinets for dentists, either free standing or fixed to a wall, that are meant for storage of instruments. 19th and early 20th century dental cabinets featured multiple drawers of varied sizes, and articulated or removeable trays for instruments."@en ;
  rdfs:isDefinedBy <https://w3id.org/con-tax/components/aat-furn> ;
  rdfs:label "dental cabinets"@en ;
  rdfs:label "tandkast"@nl ;
  rdfs:label "tandkasten"@nl ;
  rdfs:seeAlso <http://vocab.getty.edu/aat/300170867> ;
  rdfs:subClassOf <https://w3id.org/con-tax/components/aat-furn#300038888> ;
.
<https://w3id.org/con-tax/components/aat-furn#300170870>
  rdf:type owl:Class ;
  rdfs:comment "Cabinets that hold spools of thread on spindles. Holes are drilled in the fronts of the cabinets where thread can be pulled out. "@en ;
  rdfs:isDefinedBy <https://w3id.org/con-tax/components/aat-furn> ;
  rdfs:label "draadkast"@nl ;
  rdfs:label "draadkasten"@nl ;
  rdfs:label "thread cabinets"@en ;
  rdfs:seeAlso <http://vocab.getty.edu/aat/300170870> ;
  rdfs:subClassOf <https://w3id.org/con-tax/components/aat-furn#300038888> ;
.
<https://w3id.org/con-tax/components/aat-furn#300170887>
  rdf:type owl:Class ;
  rdfs:comment "Pieces of furniture used for serving food, often reserved for relatively small or portable sideboards. For tables used to serve food, use \"serving tables.\""@en ;
  rdfs:isDefinedBy <https://w3id.org/con-tax/components/aat-furn> ;
  rdfs:label "server (sideboard)"@nl ;
  rdfs:label "server"@nl ;
  rdfs:label "servers (sideboards)"@en ;
  rdfs:label "servers (sideboards)"@nl ;
  rdfs:label "servers"@nl ;
  rdfs:seeAlso <http://vocab.getty.edu/aat/300170887> ;
  rdfs:subClassOf <https://w3id.org/con-tax/components/aat-furn#300039306> ;
.
<https://w3id.org/con-tax/components/aat-furn#300170905>
  rdf:type owl:Class ;
  rdfs:comment "Marble top tables intended primarily for confectionery work."@en ;
  rdfs:comment "Tafels met een marmeren blad die voornamelijk waren bedoeld voor het maken van zoetigheid."@nl ;
  rdfs:isDefinedBy <https://w3id.org/con-tax/components/aat-furn> ;
  rdfs:label "pasteitafel"@nl ;
  rdfs:label "pasteitafels"@nl ;
  rdfs:label "pastry tables"@en ;
  rdfs:seeAlso <http://vocab.getty.edu/aat/300170905> ;
  rdfs:subClassOf <https://w3id.org/con-tax/components/aat-furn#300039548> ;
.
<https://w3id.org/con-tax/components/aat-furn#300170910>
  rdf:type owl:Class ;
  rdfs:comment "Open-front cupboards on wheels, used in front of a fire to warm plates of food."@en ;
  rdfs:comment "Wandkasten op wieltjes met open voorkant, die voor een haardvuur worden gezet om borden met voedsel op te warmen."@nl ;
  rdfs:isDefinedBy <https://w3id.org/con-tax/components/aat-furn> ;
  rdfs:label "hasters"@en ;
  rdfs:label "hasters"@nl ;
  rdfs:seeAlso <http://vocab.getty.edu/aat/300170910> ;
  rdfs:subClassOf <https://w3id.org/con-tax/components/aat-furn#300039183> ;
.
<https://w3id.org/con-tax/components/aat-furn#300170938>
  rdf:type owl:Class ;
  rdfs:comment "Folding stools used by worshippers to sit or kneel, especially those used by the sovereign during coronation. For chairs used by bishops or other prelates in the chancel of a church, use \"faldistories.\" For the French form of folding stool used at court or domestically after the 17th century, use \"pliants.\""@en ;
  rdfs:comment "Opvouwbare krukken van uiteenlopende aard die door gelovigen worden gebruikt om op te zitten of te knielen, in het bijzonder door het staatshoofd tijdens de kroning. Gebruik ‘faldistoria’ voor stoelen die door bisschoppen of andere prelaten worden gebruikt in het koor van een kerk. Gebruik 'pliants' voor een Frans type vouwkruk dat na de 17de eeuw aan het hof of in woonhuizen werd gebruikt."@nl ;
  rdfs:isDefinedBy <https://w3id.org/con-tax/components/aat-furn> ;
  rdfs:label "bisschopskruk"@nl ;
  rdfs:label "bisschopskrukken"@nl ;
  rdfs:label "faldstools (ecclesiastical furniture)"@en ;
  rdfs:seeAlso <http://vocab.getty.edu/aat/300170938> ;
  rdfs:seeAlso wd:Q2738685 ;
  rdfs:subClassOf <https://w3id.org/con-tax/components/aat-furn#300244761> ;
.
<https://w3id.org/con-tax/components/aat-furn#300171016>
  rdf:type owl:Class ;
  rdfs:comment "Chairs with a low seat and a tall sloping back, used as a prayer seat or stool; the form was seen in the 17th century, but became particularly popular during the Gothic Revival of the 19th century. For kneelers of similar form having a support for elbows and bookshelf, but not in the form of a chair, use \"prie-dieus (benches).\" For chairs with a very similar design, particularly those dating to the 18th century, but intended for use by females watching card games, use \"voyeuses à genoux.\" Prie-dieu chairs may be made of humble materials, such as a wooden frame with a rattan seat-kneeler, or they may be upholstered; they may include a shelf for prayer books. They are found in private chambers and occasionally in churches. If they are part of a set, it is usually a bedroom set. Voyeuses à genoux are always upholstered, and are generally part of a larger set along with voyeuses intended for males to sit astride while watching card games."@en ;
  rdfs:isDefinedBy <https://w3id.org/con-tax/components/aat-furn> ;
  rdfs:label "bidstoelen"@nl ;
  rdfs:label "knielbank (bidstoel)"@nl ;
  rdfs:label "knielbank"@nl ;
  rdfs:label "knielbanken (bidstoelen)"@nl ;
  rdfs:label "knielbanken"@nl ;
  rdfs:label "prie-dieu chairs"@en ;
  rdfs:seeAlso <http://vocab.getty.edu/aat/300171016> ;
  rdfs:subClassOf <https://w3id.org/con-tax/components/aat-furn#300037772> ;
  rdfs:subClassOf <https://w3id.org/con-tax/components/aat-furn#300137869> ;
.
<https://w3id.org/con-tax/components/aat-furn#300171576>
  rdf:type owl:Class ;
  rdfs:isDefinedBy <https://w3id.org/con-tax/components/aat-furn> ;
  rdfs:label "chaise à médaillon"@nl ;
  rdfs:label "chaises à médaillon"@en ;
  rdfs:label "chaises à médaillon"@nl ;
  rdfs:seeAlso <http://vocab.getty.edu/aat/300171576> ;
  rdfs:subClassOf <https://w3id.org/con-tax/components/aat-furn#300037977> ;
.
<https://w3id.org/con-tax/components/aat-furn#300171587>
  rdf:type owl:Class ;
  rdfs:comment "Populaire benaming voor Amerikaanse bureaus met een schuine voorkant."@nl ;
  rdfs:comment "Popular term for American slant-front desks."@en ;
  rdfs:isDefinedBy <https://w3id.org/con-tax/components/aat-furn> ;
  rdfs:label "Governor Winthrop desks"@en ;
  rdfs:label "Governor Winthropbureau"@nl ;
  rdfs:label "Governor Winthropbureaus"@nl ;
  rdfs:seeAlso <http://vocab.getty.edu/aat/300171587> ;
  rdfs:subClassOf <https://w3id.org/con-tax/components/aat-furn#300039526> ;
.
<https://w3id.org/con-tax/components/aat-furn#300171605>
  rdf:type owl:Class ;
  rdfs:comment "Simple, wooden slat-back chairs with a seat usually of woven material, originating in Chiavari, Italy. Mass-produced chairs have been based on this design, including Gio Ponti's 'Superleggera' chair of the 1950s."@en ;
  rdfs:isDefinedBy <https://w3id.org/con-tax/components/aat-furn> ;
  rdfs:label "Chiavari chairs"@en ;
  rdfs:label "Chiavaristoel"@nl ;
  rdfs:label "Chiavaristoelen"@nl ;
  rdfs:seeAlso <http://vocab.getty.edu/aat/300171605> ;
  rdfs:seeAlso wd:Q3954157 ;
  rdfs:subClassOf <https://w3id.org/con-tax/components/aat-furn#300038003> ;
.
<https://w3id.org/con-tax/components/aat-furn#300171674>
  rdf:type owl:Class ;
  rdfs:comment "Refers to a traditional Norwegian chair made from a solid log, produced by hollowing out a tree trunk so that the lower portion retains the cylindrical shape of the trunk. The kubbestol is typically decorated with traditional Norwegian painting and carving."@en ;
  rdfs:comment "Verwijst naar een traditionele Noorse stoel die uit één massief houtblok is gemaakt door een stuk boomstam zodanig uit te hollen dat het onderste deel van de stoel de cilindervorm van de stam behoudt. De kubbestol wordt doorgaans versierd met traditionele Noorse beschilderingen en houtsnijwerken."@nl ;
  rdfs:isDefinedBy <https://w3id.org/con-tax/components/aat-furn> ;
  rdfs:label "Kubbestols"@nl ;
  rdfs:label "kubbestol"@nl ;
  rdfs:label "kubbestols (stoel naar vorm)"@nl ;
  rdfs:label "kubbestols"@en ;
  rdfs:label "kubbestols"@nl ;
  rdfs:seeAlso <http://vocab.getty.edu/aat/300171674> ;
  rdfs:seeAlso wd:Q3378009 ;
  rdfs:subClassOf <https://w3id.org/con-tax/components/aat-furn#300037772> ;
.
<https://w3id.org/con-tax/components/aat-furn#300171702>
  rdf:type owl:Class ;
  rdfs:comment "Angular armchairs with slatted seats and backs; not known to have originated in the Adirondacks. They are generally used outdoors."@en ;
  rdfs:comment "Rechte stoelen waarbij zitting en rugleuning uit latten bestaan. Het is onbekend of ze afkomstig zijn uit het Adirondackgebergte."@nl ;
  rdfs:isDefinedBy <https://w3id.org/con-tax/components/aat-furn> ;
  rdfs:label "Adirondack chairs"@en ;
  rdfs:label "Adirondackstoel"@nl ;
  rdfs:label "Adirondackstoelen"@nl ;
  rdfs:seeAlso <http://vocab.getty.edu/aat/300171702> ;
  rdfs:seeAlso wd:Q357530 ;
  rdfs:subClassOf <https://w3id.org/con-tax/components/aat-furn#300037776> ;
  rdfs:subClassOf <https://w3id.org/con-tax/components/aat-furn#300165810> ;
.
<https://w3id.org/con-tax/components/aat-furn#300172119>
  rdf:type owl:Class ;
  rdfs:comment "Case furniture for a dining room having compartments or shelves for holding articles of table service below, and a surface for serving or preparing food. The term has been in use since the 16th century."@en ;
  rdfs:comment "Verwijst naar meubelstukken voor een eetkamer met vakken of schappen voor het uitstallen van tafelservies alsmede een oppervlak voor het opdienen of bereiden van voedsel. De term is reeds sinds de 16de eeuw in gebruik, en er is sprake van overlap met de betekenis van 'dressoirs (meubilair)' en 'keukenkasten (wandkasten)'."@nl ;
  rdfs:isDefinedBy <https://w3id.org/con-tax/components/aat-furn> ;
  rdfs:label "buffet"@nl ;
  rdfs:label "buffetkast"@nl ;
  rdfs:label "buffetkasten"@nl ;
  rdfs:label "buffets (sideboards)"@en ;
  rdfs:label "buffetten"@nl ;
  rdfs:seeAlso <http://vocab.getty.edu/aat/300172119> ;
  rdfs:subClassOf <https://w3id.org/con-tax/components/aat-furn#300039306> ;
.
<https://w3id.org/con-tax/components/aat-furn#300172131>
  rdf:type owl:Class ;
  rdfs:isDefinedBy <https://w3id.org/con-tax/components/aat-furn> ;
  rdfs:label "dispensaries (furniture)"@en ;
  rdfs:label "dispenser (meubilair)"@nl ;
  rdfs:label "dispenser"@nl ;
  rdfs:label "dispensers (meubilair)"@nl ;
  rdfs:label "dispensers"@nl ;
  rdfs:seeAlso <http://vocab.getty.edu/aat/300172131> ;
  rdfs:subClassOf <https://w3id.org/con-tax/components/aat-furn#300038860> ;
.
<https://w3id.org/con-tax/components/aat-furn#300172137>
  rdf:type owl:Class ;
  rdfs:comment "Eighteenth-century term referring to chairs, particularly those used by women, located in the dressing room. "@en ;
  rdfs:isDefinedBy <https://w3id.org/con-tax/components/aat-furn> ;
  rdfs:label "dressing chair"@nl ;
  rdfs:label "dressing chairs"@en ;
  rdfs:label "dressing chairs"@nl ;
  rdfs:seeAlso <http://vocab.getty.edu/aat/300172137> ;
  rdfs:subClassOf <https://w3id.org/con-tax/components/aat-furn#300037772> ;
.
<https://w3id.org/con-tax/components/aat-furn#300172142>
  rdf:type owl:Class ;
  rdfs:comment "Compact, fitted dressing chests intended to hold a gentleman's fashion accessories. "@en ;
  rdfs:isDefinedBy <https://w3id.org/con-tax/components/aat-furn> ;
  rdfs:label "gentlemen's dressing stands"@en ;
  rdfs:label "herenkledingstandaard"@nl ;
  rdfs:label "herenkledingstandaarden"@nl ;
  rdfs:seeAlso <http://vocab.getty.edu/aat/300172142> ;
  rdfs:subClassOf <https://w3id.org/con-tax/components/aat-furn#300174721> ;
.
<https://w3id.org/con-tax/components/aat-furn#300172148>
  rdf:type owl:Class ;
  rdfs:comment "Screens on a writing or dressing table. Originally intended as a guard against heat from a nearby fireplace, while writing."@en ;
  rdfs:isDefinedBy <https://w3id.org/con-tax/components/aat-furn> ;
  rdfs:label "writing fire screen"@nl ;
  rdfs:label "writing fire screens"@en ;
  rdfs:label "writing fire screens"@nl ;
  rdfs:seeAlso <http://vocab.getty.edu/aat/300172148> ;
  rdfs:subClassOf <https://w3id.org/con-tax/components/aat-furn#300037745> ;
.
<https://w3id.org/con-tax/components/aat-furn#300172154>
  rdf:type owl:Class ;
  rdfs:isDefinedBy <https://w3id.org/con-tax/components/aat-furn> ;
  rdfs:label "gentlemen's writing fire screen"@nl ;
  rdfs:label "gentlemen's writing fire screens"@en ;
  rdfs:label "gentlemen's writing fire screens"@nl ;
  rdfs:seeAlso <http://vocab.getty.edu/aat/300172154> ;
  rdfs:subClassOf <https://w3id.org/con-tax/components/aat-furn#300172148> ;
.
<https://w3id.org/con-tax/components/aat-furn#300172158>
  rdf:type owl:Class ;
  rdfs:isDefinedBy <https://w3id.org/con-tax/components/aat-furn> ;
  rdfs:label "ladies' writing fire screen"@nl ;
  rdfs:label "ladies' writing fire screens"@en ;
  rdfs:label "ladies' writing fire screens"@nl ;
  rdfs:seeAlso <http://vocab.getty.edu/aat/300172158> ;
  rdfs:subClassOf <https://w3id.org/con-tax/components/aat-furn#300172148> ;
.
<https://w3id.org/con-tax/components/aat-furn#300172163>
  rdf:type owl:Class ;
  rdfs:comment "Oblong tables with simple tapered legs, often outfitted with one or more drawers beneath the tabletop and occasionally a leather pad inlaid in the writing surface."@en ;
  rdfs:isDefinedBy <https://w3id.org/con-tax/components/aat-furn> ;
  rdfs:label "gentlemen's writing tables"@en ;
  rdfs:label "herenschrijftafel"@nl ;
  rdfs:label "herenschrijftafels"@nl ;
  rdfs:seeAlso <http://vocab.getty.edu/aat/300172163> ;
  rdfs:subClassOf <https://w3id.org/con-tax/components/aat-furn#300039436> ;
.
<https://w3id.org/con-tax/components/aat-furn#300172167>
  rdf:type owl:Class ;
  rdfs:comment "Cabinets of various form that are designed to be fixed to the surface of a wall, and that have no floor support."@en ;
  rdfs:isDefinedBy <https://w3id.org/con-tax/components/aat-furn> ;
  rdfs:label "hanging cabinets"@en ;
  rdfs:label "hangkabinet"@nl ;
  rdfs:label "hangkabinetten"@nl ;
  rdfs:seeAlso <http://vocab.getty.edu/aat/300172167> ;
  rdfs:subClassOf <https://w3id.org/con-tax/components/aat-furn#300038888> ;
.
<https://w3id.org/con-tax/components/aat-furn#300172172>
  rdf:type owl:Class ;
  rdfs:comment "Fall-front desks that were intended for use by ladies, often of relatively delicate design and sometimes having a wide opening to accommodate ladies' voluminous skirts. "@en ;
  rdfs:isDefinedBy <https://w3id.org/con-tax/components/aat-furn> ;
  rdfs:label "damessecretaire"@nl ;
  rdfs:label "damessecretaires"@nl ;
  rdfs:label "ladies' secretaries"@en ;
  rdfs:seeAlso <http://vocab.getty.edu/aat/300172172> ;
  rdfs:subClassOf <https://w3id.org/con-tax/components/aat-furn#300039360> ;
  rdfs:subClassOf <https://w3id.org/con-tax/components/aat-furn#300039470> ;
.
<https://w3id.org/con-tax/components/aat-furn#300172182>
  rdf:type owl:Class ;
  rdfs:comment "Cupboards for storing clothes that are not as tall as standard clothes presses, often of shoulder height or shorter."@en ;
  rdfs:isDefinedBy <https://w3id.org/con-tax/components/aat-furn> ;
  rdfs:label "low clothes press"@nl ;
  rdfs:label "low clothes presses"@en ;
  rdfs:label "low clothes presses"@nl ;
  rdfs:seeAlso <http://vocab.getty.edu/aat/300172182> ;
  rdfs:subClassOf <https://w3id.org/con-tax/components/aat-furn#300039253> ;
.
<https://w3id.org/con-tax/components/aat-furn#300172207>
  rdf:type owl:Class ;
  rdfs:comment "Fairly small bookcases, generally between three and four feet high, set on castors to facilitate their easy movement, of a style popular in the 18th and 19th centuries."@en ;
  rdfs:comment "Historische benaming die aan het einde van de 18e en het begin van de 19e eeuw werd gebruikt voor vrij kleine boekenkasten die meestal tussen de 90 en 120 cm hoog zijn. Ze staan op zwenkwieltjes zodat ze makkelijk verplaatsbaar zijn."@nl ;
  rdfs:isDefinedBy <https://w3id.org/con-tax/components/aat-furn> ;
  rdfs:label "bewegende bibliotheek"@nl ;
  rdfs:label "bewegende bibliotheken"@nl ;
  rdfs:label "moving libraries"@en ;
  rdfs:seeAlso <http://vocab.getty.edu/aat/300172207> ;
  rdfs:subClassOf <https://w3id.org/con-tax/components/aat-furn#300038867> ;
.
<https://w3id.org/con-tax/components/aat-furn#300172232>
  rdf:type owl:Class ;
  rdfs:comment "Refers to case furniture similar to sideboard or buffet and used for dressing food and for storing and displaying dishes, fine tableware, and eating and serving utensils. The dresser was used in England beginning in the Tudor period, when it developed as a side table that was often fitted with a row of drawers. In the late 17th century, a dresser typically included a low backboard and narrow shelves or drawers, sometimes used to display valuable dishes.  Dressers of this type were very popular in the 19th century. In France and Germany, dressers were more elaborately carved, and often included a cupboard, with or without doors, and a pot board below. In America, the term \"dresser (chest of drawers)\" refers to a piece of bedroom furniture that is similar in form to the European \"dresser (cupboard).\""@en ;
  rdfs:comment "Verwijst naar een dressoir of buffet voor het bereiden van voedsel en het uitstallen van borden, fijn tafelgerei en eet- en drinkgerei. In Engeland was de keukenkast in gebruik sinds de Tudorperiode, waar hij zich ontwikkelde uit een zijtafel met een rij laden. Aan het einde van de 17de eeuw omvatte de keukenkast meestal ook een lage achterplank en smalle schappen of laden, welke soms dienden voor het uitstallen van waardevolle borden. Keukenkasten van dit type waren in de 19de eeuw zeer geliefd. Franse en Engelse keukenkasten waren rijker bewerkt, en bestonden vaak uit een wandkast (met of zonder deuren) met daaronder een pottenkast."@nl ;
  rdfs:isDefinedBy <https://w3id.org/con-tax/components/aat-furn> ;
  rdfs:label "dressers (cupboards)"@en ;
  rdfs:label "keukenkast (wandkast)"@nl ;
  rdfs:label "keukenkast"@nl ;
  rdfs:label "keukenkasten (wandkasten)"@nl ;
  rdfs:label "keukenkasten"@nl ;
  rdfs:seeAlso <http://vocab.getty.edu/aat/300172232> ;
  rdfs:subClassOf <https://w3id.org/con-tax/components/aat-furn#300039183> ;
.
<https://w3id.org/con-tax/components/aat-furn#300172270>
  rdf:type owl:Class ;
  rdfs:isDefinedBy <https://w3id.org/con-tax/components/aat-furn> ;
  rdfs:label "gentlemen's secretaries"@en ;
  rdfs:label "herensecretaire"@nl ;
  rdfs:label "herensecretaires"@nl ;
  rdfs:seeAlso <http://vocab.getty.edu/aat/300172270> ;
  rdfs:subClassOf <https://w3id.org/con-tax/components/aat-furn#300039360> ;
.
<https://w3id.org/con-tax/components/aat-furn#300172285>
  rdf:type owl:Class ;
  rdfs:comment "Chests of drawers having specially designed upper drawers that provide mirrors set on a quadrant, as on Rudd tables. Popular in the late 18th and early 19th centuries."@en ;
  rdfs:comment "Historische benaming die wordt gebruikt voor ladenkasten uit het einde van de 18e en het begin van de 19e eeuw, die speciaal ontworpen laden aan de bovenkant hebben met  toiletspiegels, net zoals bij Rudd-tafels."@nl ;
  rdfs:isDefinedBy <https://w3id.org/con-tax/components/aat-furn> ;
  rdfs:label "Rudd dressing chest"@nl ;
  rdfs:label "Rudd dressing chests"@en ;
  rdfs:label "Rudd dressing chests"@nl ;
  rdfs:seeAlso <http://vocab.getty.edu/aat/300172285> ;
  rdfs:subClassOf <https://w3id.org/con-tax/components/aat-furn#300039009> ;
.
<https://w3id.org/con-tax/components/aat-furn#300172364>
  rdf:type owl:Class ;
  rdfs:comment "Settles having a hinged back so that it can be let down to rest on the arms and thereby forming a table."@en ;
  rdfs:comment "Zittekisten met een scharnierende rugleuning die omlaag kan worden gebracht tot op de armleuningen zodat er een tafel ontstaat."@nl ;
  rdfs:isDefinedBy <https://w3id.org/con-tax/components/aat-furn> ;
  rdfs:label "settle table"@nl ;
  rdfs:label "settle tables"@en ;
  rdfs:label "settle tables"@nl ;
  rdfs:seeAlso <http://vocab.getty.edu/aat/300172364> ;
  rdfs:subClassOf <https://w3id.org/con-tax/components/aat-furn#300038532> ;
  rdfs:subClassOf <https://w3id.org/con-tax/components/aat-furn#300039548> ;
.
<https://w3id.org/con-tax/components/aat-furn#300172436>
  rdf:type owl:Class ;
  rdfs:comment "Chests with continuous, low-relief carvings, often depicting Biblical scenes or the lives of the saints."@en ;
  rdfs:isDefinedBy <https://w3id.org/con-tax/components/aat-furn> ;
  rdfs:label "tilting chest"@nl ;
  rdfs:label "tilting chests"@en ;
  rdfs:label "tilting chests"@nl ;
  rdfs:seeAlso <http://vocab.getty.edu/aat/300172436> ;
  rdfs:subClassOf <https://w3id.org/con-tax/components/aat-furn#300038992> ;
.
<https://w3id.org/con-tax/components/aat-furn#300172449>
  rdf:type owl:Class ;
  rdfs:comment "Onderzetters die zijn ontworpen als een soort kastjes, met tin gevoerd en uitgerust met rekken en een verwarmingselement."@nl ;
  rdfs:comment "Pedestals designed as cupboards lined with tin and fitted with racks and a heater."@en ;
  rdfs:isDefinedBy <https://w3id.org/con-tax/components/aat-furn> ;
  rdfs:label "bordenwarmer"@nl ;
  rdfs:label "bordenwarmers"@nl ;
  rdfs:label "plate warmers"@en ;
  rdfs:seeAlso <http://vocab.getty.edu/aat/300172449> ;
  rdfs:subClassOf <https://w3id.org/con-tax/components/aat-furn#300039337> ;
.
<https://w3id.org/con-tax/components/aat-furn#300172457>
  rdf:type owl:Class ;
  rdfs:comment "Seats, usually made of cast-iron and in period character, located in a garden. "@en ;
  rdfs:isDefinedBy <https://w3id.org/con-tax/components/aat-furn> ;
  rdfs:label "garden seats"@en ;
  rdfs:label "tuinbank"@nl ;
  rdfs:label "tuinbanken"@nl ;
  rdfs:seeAlso <http://vocab.getty.edu/aat/300172457> ;
  rdfs:subClassOf <https://w3id.org/con-tax/components/aat-furn#300038494> ;
.
<https://w3id.org/con-tax/components/aat-furn#300172507>
  rdf:type owl:Class ;
  rdfs:comment "Chests with deep storage space, at least one drawer, and a hinged lid. Frequently used for the storage of blankets."@en ;
  rdfs:comment "Diepe kisten met een grote opslagcapaciteit, ten minste één lade en een deksel met scharnier. Veelvuldig gebruikt voor het bewaren van dekens."@nl ;
  rdfs:isDefinedBy <https://w3id.org/con-tax/components/aat-furn> ;
  rdfs:label "blanket chests"@en ;
  rdfs:label "dekenkist"@nl ;
  rdfs:label "dekenkisten"@nl ;
  rdfs:seeAlso <http://vocab.getty.edu/aat/300172507> ;
  rdfs:subClassOf <https://w3id.org/con-tax/components/aat-furn#300038992> ;
.
<https://w3id.org/con-tax/components/aat-furn#300174209>
  rdf:type owl:Class ;
  rdfs:comment "Bureaus die twee rijen laden hebben met beenruimte ertussen. Sommige vormen worden als schrijfbureaus gebruikt en andere als toilettafels. Dit type was populair in Frankrijk tijdens de tweede helft van de 17e eeuw."@nl ;
  rdfs:comment "Bureaux with two tiers of drawers flanking a kneehole recess, some forms intended to be used as writing desks, others as dressing tables; of a type popular in France during the second half of the 17th century."@en ;
  rdfs:isDefinedBy <https://w3id.org/con-tax/components/aat-furn> ;
  rdfs:label "bureau Mazarin"@nl ;
  rdfs:label "bureaus Mazarins"@nl ;
  rdfs:label "bureaux Mazarins"@en ;
  rdfs:seeAlso <http://vocab.getty.edu/aat/300174209> ;
  rdfs:subClassOf <https://w3id.org/con-tax/components/aat-furn#300039668> ;
  rdfs:subClassOf <https://w3id.org/con-tax/components/aat-furn#300136379> ;
.
<https://w3id.org/con-tax/components/aat-furn#300174232>
  rdf:type owl:Class ;
  rdfs:comment "Franse vorm van een sta-bureau met soms een pupitre."@nl ;
  rdfs:comment "French form of standing desk, sometimes having a pupitre."@en ;
  rdfs:isDefinedBy <https://w3id.org/con-tax/components/aat-furn> ;
  rdfs:label "bureau debout"@nl ;
  rdfs:label "bureaux debout"@en ;
  rdfs:label "bureaux debout"@nl ;
  rdfs:seeAlso <http://vocab.getty.edu/aat/300174232> ;
  rdfs:subClassOf <https://w3id.org/con-tax/components/aat-furn#300164527> ;
.
<https://w3id.org/con-tax/components/aat-furn#300174236>
  rdf:type owl:Class ;
  rdfs:comment "Canapés met een rugleuning die licht naar voren en beneden buigt zodat aan het eind de armleuningen worden gevormd."@nl ;
  rdfs:comment "Canapés whose backs gently curve forward and downward to form the arms."@en ;
  rdfs:isDefinedBy <https://w3id.org/con-tax/components/aat-furn> ;
  rdfs:label "canapé à corbeille"@nl ;
  rdfs:label "canapés à corbeille"@en ;
  rdfs:label "canapés à corbeille"@nl ;
  rdfs:seeAlso <http://vocab.getty.edu/aat/300174236> ;
  rdfs:subClassOf <https://w3id.org/con-tax/components/aat-furn#300038636> ;
.
<https://w3id.org/con-tax/components/aat-furn#300174275>
  rdf:type owl:Class ;
  rdfs:comment "Meubelstukken met vakjes of laadjes waarin paperassen worden gelegd. Ze kunnen op een speciaal gemaakt kastje aan één kant van het bureau staan of bovenop het bureaublad zelf worden geplaatst."@nl ;
  rdfs:comment "Pieces of furniture fitted with pigeonholes or compartments to hold paper; either resting on a specially made cabinet placed at one end of a bureau plat or on the top of the bureau plat itself."@en ;
  rdfs:isDefinedBy <https://w3id.org/con-tax/components/aat-furn> ;
  rdfs:label "serre papier"@nl ;
  rdfs:label "serre papiers (cabinets)"@en ;
  rdfs:label "serre papiers"@nl ;
  rdfs:seeAlso <http://vocab.getty.edu/aat/300174275> ;
  rdfs:subClassOf <https://w3id.org/con-tax/components/aat-furn#300038888> ;
.
<https://w3id.org/con-tax/components/aat-furn#300174509>
  rdf:type owl:Class ;
  rdfs:comment "Kleine, verplaatsbare tafels die soms een porseleinen of marmeren tafelblad hebben."@nl ;
  rdfs:comment "Small movable tables sometimes with a porcelain or marble top."@en ;
  rdfs:isDefinedBy <https://w3id.org/con-tax/components/aat-furn> ;
  rdfs:label "salontafel"@nl ;
  rdfs:label "salontafels"@nl ;
  rdfs:label "tables de salon"@en ;
  rdfs:seeAlso <http://vocab.getty.edu/aat/300174509> ;
  rdfs:subClassOf <https://w3id.org/con-tax/components/aat-furn#300039880> ;
.
<https://w3id.org/con-tax/components/aat-furn#300174701>
  rdf:type owl:Class ;
  rdfs:comment "Chairs that have backs that are rounded inward. "@en ;
  rdfs:isDefinedBy <https://w3id.org/con-tax/components/aat-furn> ;
  rdfs:label "concaaf-rugstoelen"@nl ;
  rdfs:label "concave-back chairs"@en ;
  rdfs:seeAlso <http://vocab.getty.edu/aat/300174701> ;
  rdfs:subClassOf <https://w3id.org/con-tax/components/aat-furn#300037772> ;
.
<https://w3id.org/con-tax/components/aat-furn#300174713>
  rdf:type owl:Class ;
  rdfs:comment "Racks, usually with pegs, knobs, or hooks, from which to hang hats; generally attached to walls or other pieces of furniture. Less elaborate and less likely to be free-standing and furniturelike than \"hat stands.\""@en ;
  rdfs:comment "Rekken, meestal met pennen, knoppen, of haken, waaraan hoeden gehangen kunnen worden, in het algemeen bevestigd aan muren of meubels. Minder afgewerkt en minder als meubelstuk bedoeld dan 'hoedenstandaarden'."@nl ;
  rdfs:isDefinedBy <https://w3id.org/con-tax/components/aat-furn> ;
  rdfs:label "hat racks"@en ;
  rdfs:label "hoedenrek"@nl ;
  rdfs:label "hoedenrekken"@nl ;
  rdfs:seeAlso <http://vocab.getty.edu/aat/300174713> ;
  rdfs:seeAlso wd:Q26267183 ;
  rdfs:subClassOf <https://w3id.org/con-tax/components/aat-furn#300039337> ;
.
<https://w3id.org/con-tax/components/aat-furn#300174721>
  rdf:type owl:Class ;
  rdfs:comment "Compact, fitted dressing chests which stand on four tapering legs, and are intended to hold cosmetics and jewelry. "@en ;
  rdfs:isDefinedBy <https://w3id.org/con-tax/components/aat-furn> ;
  rdfs:label "dressing stands"@en ;
  rdfs:label "kledingstandaard"@nl ;
  rdfs:label "kledingstandaarden"@nl ;
  rdfs:seeAlso <http://vocab.getty.edu/aat/300174721> ;
  rdfs:subClassOf <https://w3id.org/con-tax/components/aat-furn#300039767> ;
.
<https://w3id.org/con-tax/components/aat-furn#300174746>
  rdf:type owl:Class ;
  rdfs:comment "Portable, lightweight beds or cots that can be folded for transport and carried with handles, resembling a suitcase. The beds may include attached light bedding, or may be only the bedframe."@en ;
  rdfs:isDefinedBy <https://w3id.org/con-tax/components/aat-furn> ;
  rdfs:label "kofferbed"@nl ;
  rdfs:label "kofferbedden"@nl ;
  rdfs:label "suitcase beds"@en ;
  rdfs:seeAlso <http://vocab.getty.edu/aat/300174746> ;
  rdfs:subClassOf <https://w3id.org/con-tax/components/aat-furn#300038697> ;
.
<https://w3id.org/con-tax/components/aat-furn#300174750>
  rdf:type owl:Class ;
  rdfs:comment "Cabinets or chests of drawers with triangular bodies that are meant to occupy the juncture of two walls. They are made for display as well as storage and are often elaborately decorated."@en ;
  rdfs:isDefinedBy <https://w3id.org/con-tax/components/aat-furn> ;
  rdfs:label "corner commodes"@en ;
  rdfs:label "hoekcommode"@nl ;
  rdfs:label "hoekcommodes"@nl ;
  rdfs:seeAlso <http://vocab.getty.edu/aat/300174750> ;
  rdfs:subClassOf <https://w3id.org/con-tax/components/aat-furn#300077277> ;
.
<https://w3id.org/con-tax/components/aat-furn#300175575>
  rdf:type owl:Class ;
  rdfs:comment "Schrijftafels met een uitklapbare boekenhouder."@nl ;
  rdfs:comment "Writing tables with a pop-up reading stand."@en ;
  rdfs:isDefinedBy <https://w3id.org/con-tax/components/aat-furn> ;
  rdfs:label "bureau en pupitre"@nl ;
  rdfs:label "bureaux en pupitre"@en ;
  rdfs:label "bureaux en pupitre"@nl ;
  rdfs:seeAlso <http://vocab.getty.edu/aat/300175575> ;
  rdfs:subClassOf <https://w3id.org/con-tax/components/aat-furn#300039436> ;
.
<https://w3id.org/con-tax/components/aat-furn#300176430>
  rdf:type owl:Class ;
  rdfs:comment "Pierced wooden seats with removable containers underneath; used as a commode. "@en ;
  rdfs:isDefinedBy <https://w3id.org/con-tax/components/aat-furn> ;
  rdfs:label "close stool"@nl ;
  rdfs:label "close stools"@nl ;
  rdfs:label "close-stools"@en ;
  rdfs:seeAlso <http://vocab.getty.edu/aat/300176430> ;
  rdfs:seeAlso wd:Q2947723 ;
  rdfs:subClassOf <https://w3id.org/con-tax/components/aat-furn#300038424> ;
.
<https://w3id.org/con-tax/components/aat-furn#300176672>
  rdf:type owl:Class ;
  rdfs:comment "Historische benaming voor kleine ontbijttafels die in het begin van de 19e eeuw werden gemaakt om te gebruiken in boudoirs of eethoeken."@nl ;
  rdfs:comment "Small breakfast tables, made in early 19th century, intended to be used in ladies' boudoirs or morning rooms."@en ;
  rdfs:isDefinedBy <https://w3id.org/con-tax/components/aat-furn> ;
  rdfs:label "déjeuner tables"@en ;
  rdfs:label "déjeunertafel"@nl ;
  rdfs:label "déjeunertafels"@nl ;
  rdfs:seeAlso <http://vocab.getty.edu/aat/300176672> ;
  rdfs:subClassOf <https://w3id.org/con-tax/components/aat-furn#300039633> ;
.
<https://w3id.org/con-tax/components/aat-furn#300176753>
  rdf:type owl:Class ;
  rdfs:comment "Cabinets which stand at elbow height."@en ;
  rdfs:comment "Kabinetten die tot ellebooghoogte reiken."@nl ;
  rdfs:isDefinedBy <https://w3id.org/con-tax/components/aat-furn> ;
  rdfs:label "meuble à hauteur 'appui"@nl ;
  rdfs:label "meubles à hauteur 'appui"@nl ;
  rdfs:label "meubles à hauteur d'appui"@en ;
  rdfs:seeAlso <http://vocab.getty.edu/aat/300176753> ;
  rdfs:subClassOf <https://w3id.org/con-tax/components/aat-furn#300038888> ;
.
<https://w3id.org/con-tax/components/aat-furn#300178785>
  rdf:type owl:Class ;
  rdfs:comment "Rows of columns that serve primarily to separate interior spaces."@en ;
  rdfs:comment "Wordt gebruikt voor rijen zuilen die voornamelijk dienst doen om binnenruimten van elkaar te scheiden."@nl ;
  rdfs:isDefinedBy <https://w3id.org/con-tax/components/aat-furn> ;
  rdfs:label "columnar screens"@en ;
  rdfs:label "zuilenscherm"@nl ;
  rdfs:label "zuilenschermen"@nl ;
  rdfs:seeAlso <http://vocab.getty.edu/aat/300178785> ;
  rdfs:subClassOf <https://w3id.org/con-tax/components/aat-furn#300037737> ;
.
<https://w3id.org/con-tax/components/aat-furn#300215533>
  rdf:type owl:Class ;
  rdfs:comment "Kleine kisten die zijn ontworpen om aan het voeteneinde van een bed te zetten, met name om de persoonlijke bezittingen van soldaten te bewaren."@nl ;
  rdfs:comment "Small trunks designed to be kept at the foot of a bed, especially to contain a soldier's personal effects."@en ;
  rdfs:isDefinedBy <https://w3id.org/con-tax/components/aat-furn> ;
  rdfs:label "footlockers"@en ;
  rdfs:label "opbergkist"@nl ;
  rdfs:label "opbergkisten"@nl ;
  rdfs:seeAlso <http://vocab.getty.edu/aat/300215533> ;
  rdfs:subClassOf <https://w3id.org/con-tax/components/aat-furn#300215543> ;
  rdfs:subClassOf <https://w3id.org/con-tax/components/aat-furn#300249762> ;
.
<https://w3id.org/con-tax/components/aat-furn#300215543>
  rdf:type owl:Class ;
  rdfs:comment "Onbuigzame, doosachtige houders, meestal groot en vaak versterkt, voor het inpakken van kleren en andere persoonlijke bezittingen of artikelen voor op reis of opslag."@nl ;
  rdfs:comment "Rigid, boxlike containers, usually large and often reinforced, for packing clothing and other personal gear or articles for travel or storage."@en ;
  rdfs:isDefinedBy <https://w3id.org/con-tax/components/aat-furn> ;
  rdfs:label "hutkoffer (houder)"@nl ;
  rdfs:label "hutkoffer"@nl ;
  rdfs:label "hutkoffers (houders)"@nl ;
  rdfs:label "hutkoffers"@nl ;
  rdfs:label "trunks (containers)"@en ;
  rdfs:seeAlso <http://vocab.getty.edu/aat/300215543> ;
  rdfs:subClassOf <https://w3id.org/con-tax/components/aat-furn#300037680> ;
.
<https://w3id.org/con-tax/components/aat-furn#300233725>
  rdf:type owl:Class ;
  rdfs:comment "Grote, stevige ezels die in een atelier van een kunstenaar worden gebruikt."@nl ;
  rdfs:comment "Large, sturdy easels for use in artists' studios."@en ;
  rdfs:isDefinedBy <https://w3id.org/con-tax/components/aat-furn> ;
  rdfs:label "atelier-ezel"@nl ;
  rdfs:label "atelier-ezels"@nl ;
  rdfs:label "studio easels"@en ;
  rdfs:seeAlso <http://vocab.getty.edu/aat/300233725> ;
  rdfs:subClassOf <https://w3id.org/con-tax/components/aat-furn#300079638> ;
.
<https://w3id.org/con-tax/components/aat-furn#300233726>
  rdf:type owl:Class ;
  rdfs:comment "Any of variously constructed small easels designed for use on a table, altar, desk, workbench, or the like."@en ;
  rdfs:comment "Verschillende kleine ezels die zijn ontworpen om op een tafel, bureau, werktafel of iets dergelijks te gebruiken."@nl ;
  rdfs:isDefinedBy <https://w3id.org/con-tax/components/aat-furn> ;
  rdfs:label "table easels"@en ;
  rdfs:label "tafel-ezel"@nl ;
  rdfs:label "tafel-ezels"@nl ;
  rdfs:seeAlso <http://vocab.getty.edu/aat/300233726> ;
  rdfs:subClassOf <https://w3id.org/con-tax/components/aat-furn#300079638> ;
.
<https://w3id.org/con-tax/components/aat-furn#300244761>
  rdf:type owl:Class ;
  rdfs:comment "Refers to stools, which are armless and backless seats for one person, characterized by often having a cloth or leather seat and a frame that may be folded or collapsed for transportation or storage."@en ;
  rdfs:isDefinedBy <https://w3id.org/con-tax/components/aat-furn> ;
  rdfs:label "folding stools"@en ;
  rdfs:label "vouwkruk"@nl ;
  rdfs:label "vouwkrukken"@nl ;
  rdfs:seeAlso <http://vocab.getty.edu/aat/300244761> ;
  rdfs:seeAlso wd:Q15479103 ;
  rdfs:subClassOf <https://w3id.org/con-tax/components/aat-furn#300038418> ;
.
<https://w3id.org/con-tax/components/aat-furn#300244770>
  rdf:type owl:Class ;
  rdfs:comment "Chairs that are lightweight, portable, and can be folded flat for storage, typically made of wood, metal, or canvas."@en ;
  rdfs:isDefinedBy <https://w3id.org/con-tax/components/aat-furn> ;
  rdfs:label "folding chairs"@en ;
  rdfs:label "klapstoelen"@nl ;
  rdfs:label "vouwstoelen"@nl ;
  rdfs:seeAlso <http://vocab.getty.edu/aat/300244770> ;
  rdfs:seeAlso wd:Q1744391 ;
  rdfs:subClassOf <https://w3id.org/con-tax/components/aat-furn#300037772> ;
.
<https://w3id.org/con-tax/components/aat-furn#300246035>
  rdf:type owl:Class ;
  rdfs:comment "Seating furniture designed for young people. "@en ;
  rdfs:isDefinedBy <https://w3id.org/con-tax/components/aat-furn> ;
  rdfs:label "children's chairs"@en ;
  rdfs:label "stoel voor kinderen"@nl ;
  rdfs:label "stoelen voor kinderen"@nl ;
  rdfs:seeAlso <http://vocab.getty.edu/aat/300246035> ;
  rdfs:subClassOf <https://w3id.org/con-tax/components/aat-furn#300037772> ;
.
<https://w3id.org/con-tax/components/aat-furn#300248045>
  rdf:type owl:Class ;
  rdfs:comment "General term for racks or stands of various forms for the temporary storage of coats and other garments, having pegs, hooks, bars, or projecting arms on or over which clothing may be hung or folded."@en ;
  rdfs:comment "Rekken of standaarden waarop jassen en andere kledingstukken tijdelijk kunnen worden opgeborgen."@nl ;
  rdfs:isDefinedBy <https://w3id.org/con-tax/components/aat-furn> ;
  rdfs:label "coatracks"@en ;
  rdfs:label "jassenrek"@nl ;
  rdfs:label "jassenrekken"@nl ;
  rdfs:seeAlso <http://vocab.getty.edu/aat/300248045> ;
  rdfs:seeAlso wd:Q15247824 ;
  rdfs:subClassOf <https://w3id.org/con-tax/components/aat-furn#300039337> ;
.
<https://w3id.org/con-tax/components/aat-furn#300249762>
  rdf:type owl:Class ;
  rdfs:comment "Afsluitbare ruimten die worden gebruikt voor het veilig bewaren of opslaan van spullen; zoals gebruikt op scholen en sportscholen voor het bewaren van kleding en andere spullen van waarde."@nl ;
  rdfs:comment "Containers, often set into a wall, used for safekeeping or storage and usually capable of being locked, such as those used in schools and gymnasiums for storing clothing and other valuables."@en ;
  rdfs:isDefinedBy <https://w3id.org/con-tax/components/aat-furn> ;
  rdfs:label "kluisje"@nl ;
  rdfs:label "kluisjes"@nl ;
  rdfs:label "lockers"@en ;
  rdfs:seeAlso <http://vocab.getty.edu/aat/300249762> ;
  rdfs:subClassOf <https://w3id.org/con-tax/components/aat-furn#300037680> ;
.
<https://w3id.org/con-tax/components/aat-furn#300249925>
  rdf:type owl:Class ;
  rdfs:comment "Small rooms or furniture pieces for storing food."@en ;
  rdfs:isDefinedBy <https://w3id.org/con-tax/components/aat-furn> ;
  rdfs:label "food cupboards (general cupboards)"@en ;
  rdfs:label "voedselkast"@nl ;
  rdfs:label "voedselkasten"@nl ;
  rdfs:seeAlso <http://vocab.getty.edu/aat/300249925> ;
  rdfs:subClassOf <https://w3id.org/con-tax/components/aat-furn#300039183> ;
.
<https://w3id.org/con-tax/components/aat-furn#300249926>
  rdf:type owl:Class ;
  rdfs:comment "One piece cupboards, usually with two drawers over one or two doors, used to store foodstuffs, particularly when used to store canned or preserved foods."@en ;
  rdfs:comment "Wandkasten die uit één stuk bestaan en meestal twee laden boven één of twee deuren hebben en waarin voedsel wordt opgeborgen."@nl ;
  rdfs:isDefinedBy <https://w3id.org/con-tax/components/aat-furn> ;
  rdfs:label "jelly cupboard"@nl ;
  rdfs:label "jelly cupboards"@en ;
  rdfs:label "jelly cupboards"@nl ;
  rdfs:seeAlso <http://vocab.getty.edu/aat/300249926> ;
  rdfs:subClassOf <https://w3id.org/con-tax/components/aat-furn#300249925> ;
.
<https://w3id.org/con-tax/components/aat-furn#300250397>
  rdf:type owl:Class ;
  rdfs:comment "Bakken met een deksel, staande op poten of standaarden, waarin deeg werd gemengd om te rijzen en gekneed op de bovenkant."@nl ;
  rdfs:comment "Lidded troughs on legs or stands in which dough was mixed and left to rise and kneaded on top."@en ;
  rdfs:isDefinedBy <https://w3id.org/con-tax/components/aat-furn> ;
  rdfs:label "deegtafel"@nl ;
  rdfs:label "deegtafels"@nl ;
  rdfs:label "dough tray tables"@en ;
  rdfs:seeAlso <http://vocab.getty.edu/aat/300250397> ;
  rdfs:subClassOf <https://w3id.org/con-tax/components/aat-furn#300039548> ;
.
<https://w3id.org/con-tax/components/aat-furn#300250532>
  rdf:type owl:Class ;
  rdfs:comment "Cabinets for radio receivers, often also having places for related audio accessories, such as record players."@en ;
  rdfs:comment "Kasten voor radio-ontvangers,  vaak ook met ruimte voor aanverwante geluidsapparatuur zoals platenspelers."@nl ;
  rdfs:isDefinedBy <https://w3id.org/con-tax/components/aat-furn> ;
  rdfs:label "radio cabinets"@en ;
  rdfs:label "radiokast"@nl ;
  rdfs:label "radiokasten"@nl ;
  rdfs:seeAlso <http://vocab.getty.edu/aat/300250532> ;
  rdfs:subClassOf <https://w3id.org/con-tax/components/aat-furn#300038888> ;
.
<https://w3id.org/con-tax/components/aat-furn#300250899>
  rdf:type owl:Class ;
  rdfs:comment "Compacte vrijstaande dragers, palen of standaarden, versierd met sober of rijk houtsnijwerk met symbolen, gemaakt en gebruikt in Afrika voor het ondersteunen van bogen, met of zonder pijlen. Traditionele symbolen voor stamleiders en eretekens voor grote helden en jagers, maar in sommige regio's zijn ze soms ook in bezit van de gewone man."@nl ;
  rdfs:comment "Small freestanding racks, poles, or stands, either plain or elaborately carved with symbols, made and used in Africa for supporting bows, with or without arrows; traditionally functioning as symbols of office for chieftains and symbols of honor for great heroes and hunters, though in some regions may be owned by any man."@en ;
  rdfs:isDefinedBy <https://w3id.org/con-tax/components/aat-furn> ;
  rdfs:label "boogstandaarden"@nl ;
  rdfs:label "bow stands"@en ;
  rdfs:label "pijldrager"@nl ;
  rdfs:label "pijldragers"@nl ;
  rdfs:seeAlso <http://vocab.getty.edu/aat/300250899> ;
  rdfs:subClassOf <https://w3id.org/con-tax/components/aat-furn#300039767> ;
.
<https://w3id.org/con-tax/components/aat-furn#300251230>
  rdf:type owl:Class ;
  rdfs:comment "Chairs of greater than usual height, often with a front ledge to be used as a foot rest, designed for spectators' use at billiards games."@en ;
  rdfs:comment "Stoelen die hoger dan normaal zijn, vaak met een richel aan de voorkant die als voetensteun dient. Ze zijn speciaal voor toeschouwers van biljart bedoeld."@nl ;
  rdfs:isDefinedBy <https://w3id.org/con-tax/components/aat-furn> ;
  rdfs:label "billiard chair"@nl ;
  rdfs:label "billiard chairs"@en ;
  rdfs:label "billiard chairs"@nl ;
  rdfs:seeAlso <http://vocab.getty.edu/aat/300251230> ;
  rdfs:subClassOf <https://w3id.org/con-tax/components/aat-furn#300037772> ;
.
<https://w3id.org/con-tax/components/aat-furn#300251534>
  rdf:type owl:Class ;
  rdfs:comment "Tables fitted with medical apparatus for doctors' use in examining patients."@en ;
  rdfs:comment "Tafels die zijn uitgerust met medische instrumenten die door dokters worden gebruikt om patiënten te onderzoeken."@nl ;
  rdfs:isDefinedBy <https://w3id.org/con-tax/components/aat-furn> ;
  rdfs:label "examination tables"@en ;
  rdfs:label "onderzoektafel"@nl ;
  rdfs:label "onderzoektafels"@nl ;
  rdfs:seeAlso <http://vocab.getty.edu/aat/300251534> ;
  rdfs:subClassOf <https://w3id.org/con-tax/components/aat-furn#300039548> ;
  rdfs:subClassOf <https://w3id.org/con-tax/components/aat-furn#300040036> ;
.
<https://w3id.org/con-tax/components/aat-furn#300256336>
  rdf:type owl:Class ;
  rdfs:comment "Furnishings designed as movable, temporary, compact, or capable of being dismantled and re-assembled elsewhere. "@en ;
  rdfs:isDefinedBy <https://w3id.org/con-tax/components/aat-furn> ;
  rdfs:label "draagbaar meubilair"@nl ;
  rdfs:label "portable furniture"@en ;
  rdfs:seeAlso <http://vocab.getty.edu/aat/300256336> ;
  rdfs:subClassOf <https://w3id.org/con-tax/components/aat-furn#300037680> ;
.
<https://w3id.org/con-tax/components/aat-furn#300257735>
  rdf:type owl:Class ;
  rdfs:comment "Racks for holding or storing small arms; may be freestanding or attached to something else."@en ;
  rdfs:comment "Rekken voor het opbergen of bewaren van kleine wapens; kan vrijstaand of aan iets vastgemaakt zijn."@nl ;
  rdfs:isDefinedBy <https://w3id.org/con-tax/components/aat-furn> ;
  rdfs:label "geweerrek"@nl ;
  rdfs:label "geweerrekken"@nl ;
  rdfs:label "gun racks"@en ;
  rdfs:seeAlso <http://vocab.getty.edu/aat/300257735> ;
  rdfs:seeAlso wd:Q19563053 ;
  rdfs:subClassOf <https://w3id.org/con-tax/components/aat-furn#300039337> ;
.
<https://w3id.org/con-tax/components/aat-furn#300259214>
  rdf:type owl:Class ;
  rdfs:comment "Arabic benches built of stone or mudbrick; often placed along the front and sometimes sides of traditional houses or in other areas for lodging or socializing."@en ;
  rdfs:comment "Te gebruiken voor Arabische banken, gemaakt van steen of leem; vaak gebouwd langs de voorzijde, soms langs de zijkant van traditionele huizen of op andere plaatsen waar mensen wonen of samenkomen."@nl ;
  rdfs:isDefinedBy <https://w3id.org/con-tax/components/aat-furn> ;
  rdfs:label "mastaba (bank)"@nl ;
  rdfs:label "mastaba"@nl ;
  rdfs:label "mastabas (benches)"@en ;
  rdfs:label "mastaba’s (banken)"@nl ;
  rdfs:label "mastaba’s"@nl ;
  rdfs:seeAlso <http://vocab.getty.edu/aat/300259214> ;
  rdfs:subClassOf <https://w3id.org/con-tax/components/aat-furn#300038494> ;
.
<https://w3id.org/con-tax/components/aat-furn#300261032>
  rdf:type owl:Class ;
  rdfs:comment "Small stands, often ornamental, made to hold a watch upright so that its face may be seen or to secure it during assembly, adjustment, or testing. May also refer to small stands with a base and a glass or plastic dome, dating from the 20th century, and used to display a pocket watch."@en ;
  rdfs:comment "Te gebruiken voor kleine standaarden, vaak versierd, waarin een horloge rechtop kan staan zodat het uurwerk te zien is, of om het horloge vast te zetten tijdens montage, reparatie of testen. Ook te gebruiken voor kleine standaarden met een voet en een ronde glazen of plastic top, sinds de 20ste eeuw in gebruik om zakhorloges tentoon te stellen."@nl ;
  rdfs:isDefinedBy <https://w3id.org/con-tax/components/aat-furn> ;
  rdfs:label "horlogestandaarden"@nl ;
  rdfs:label "horlogestandaards"@nl ;
  rdfs:label "watch stands"@en-us ;
  rdfs:seeAlso <http://vocab.getty.edu/aat/300261032> ;
  rdfs:subClassOf <https://w3id.org/con-tax/components/aat-furn#300039767> ;
.
<https://w3id.org/con-tax/components/aat-furn#300262819>
  rdf:type owl:Class ;
  rdfs:comment "Draagbaren waarop overledenen, al of niet in een doodskist, worden gelegd voor hun begrafenis."@nl ;
  rdfs:comment "Movable stands used to transport a coffin and often upon which corpses or coffins containing corpses may be placed during viewing and religious services before burial. They often have long handles at either end to be carried by or placed on the shoulders of the pall bearers."@en ;
  rdfs:isDefinedBy <https://w3id.org/con-tax/components/aat-furn> ;
  rdfs:label "biers"@en ;
  rdfs:label "doodbaar"@nl ;
  rdfs:label "doodbaren"@nl ;
  rdfs:label "lijkbaar"@nl ;
  rdfs:label "lijkbaren"@nl ;
  rdfs:label "lijkberrie"@nl ;
  rdfs:label "lijkberries"@nl ;
  rdfs:seeAlso <http://vocab.getty.edu/aat/300262819> ;
  rdfs:subClassOf <https://w3id.org/con-tax/components/aat-furn#300039767> ;
.
<https://w3id.org/con-tax/components/aat-furn#300262826>
  rdf:type owl:Class ;
  rdfs:comment "Stands placed on altars or attached to the wall behind an altar, consisting of or featuring a raised platform on which a monstrance is displayed for the adoration of the faithful in the Roman Catholic Church."@en ;
  rdfs:comment "Voetstukken op een altaar of tegen de muur achter het altaar geplaatst, bestaande uit of uitgevoerd met een verhoogd plateau waarop de monstrans wordt uitgestald ter aanbidding door de gelovigen in de rooms-katholieke kerk."@nl ;
  rdfs:isDefinedBy <https://w3id.org/con-tax/components/aat-furn> ;
  rdfs:label "expositietronen"@nl ;
  rdfs:label "expositietroon"@nl ;
  rdfs:label "exposition thrones"@en ;
  rdfs:seeAlso <http://vocab.getty.edu/aat/300262826> ;
  rdfs:subClassOf <https://w3id.org/con-tax/components/aat-furn#300039767> ;
.
<https://w3id.org/con-tax/components/aat-furn#300263098>
  rdf:type owl:Class ;
  rdfs:comment "Easels used primarily or solely for the display or presentation of an object, rather than to support a work as it is created."@en ;
  rdfs:isDefinedBy <https://w3id.org/con-tax/components/aat-furn> ;
  rdfs:label "display easels"@en ;
  rdfs:seeAlso <http://vocab.getty.edu/aat/300263098> ;
  rdfs:subClassOf <https://w3id.org/con-tax/components/aat-furn#300079638> ;
.
<https://w3id.org/con-tax/components/aat-furn#300263101>
  rdf:type owl:Class ;
  rdfs:comment "Tall sets of shelves mounted on low dressers."@en ;
  rdfs:isDefinedBy <https://w3id.org/con-tax/components/aat-furn> ;
  rdfs:label "étagères dressoirs"@en ;
  rdfs:seeAlso <http://vocab.getty.edu/aat/300263101> ;
  rdfs:subClassOf <https://w3id.org/con-tax/components/aat-furn#300037680> ;
.
<https://w3id.org/con-tax/components/aat-furn#300263111>
  rdf:type owl:Class ;
  rdfs:comment "Stools having very tall legs or other supports, designed for sitting at a counter or other high table-like surface."@en ;
  rdfs:isDefinedBy <https://w3id.org/con-tax/components/aat-furn> ;
  rdfs:label "tall stools"@en ;
  rdfs:seeAlso <http://vocab.getty.edu/aat/300263111> ;
  rdfs:subClassOf <https://w3id.org/con-tax/components/aat-furn#300038418> ;
.
<https://w3id.org/con-tax/components/aat-furn#300263125>
  rdf:type owl:Class ;
  rdfs:comment "Cabinets of various designs, intended for the storage and display of medals; popular in 18th-19th centuries."@en ;
  rdfs:isDefinedBy <https://w3id.org/con-tax/components/aat-furn> ;
  rdfs:label "medal cabinets"@en ;
  rdfs:seeAlso <http://vocab.getty.edu/aat/300263125> ;
  rdfs:subClassOf <https://w3id.org/con-tax/components/aat-furn#300038888> ;
.
<https://w3id.org/con-tax/components/aat-furn#300263494>
  rdf:type owl:Class ;
  rdfs:comment "Ancestral screens of the African people of Kalibara, Nigeria, Africa, generally consisting of a screen of bamboo slats in a wooden frame with carved and painted decoration. Lashed to the screen is an image of the ancestor for whom the screen is made, accompanied by two other figures representing attendants. Together with an altar for receiving libations, it constitutes a shrine to the ancestor. The term translates into English as \"foreheads of the dead.\""@en ;
  rdfs:comment "Voorouderschermen van het Kalibaravolk in Nigeria, over het algemeen bestaande uit een reeks bamboelatten in een houten raam, versierd met houtsnij- en schilderwerk. Aan het scherm is een afbeelding vastgebonden van de voorouder voor wie het scherm is gemaakt, vergezeld van twee figuren die bedienden voorstellen. Samen met een altaar voor het ontvangen van plengoffers vormt het scherm een schrijn voor de voorouder. De term betekent letterlijk ‘voorhoofden van de doden’."@nl ;
  rdfs:isDefinedBy <https://w3id.org/con-tax/components/aat-furn> ;
  rdfs:label "duein fubara"@en ;
  rdfs:label "duein fubara"@nl ;
  rdfs:seeAlso <http://vocab.getty.edu/aat/300263494> ;
  rdfs:subClassOf <https://w3id.org/con-tax/components/aat-furn#300037737> ;
.
<https://w3id.org/con-tax/components/aat-furn#300263681>
  rdf:type owl:Class ;
  rdfs:comment "Soort crinolinestoel, ontwikkeld door het Afrikaanse Asantevolk naar het Europees prototype, versierd met koperen kopspijkers, met een lage schuin aflopende rug en meestal een lederen zitting; alleen gebruikt door hooggeplaatste of hooggeëerde personen."@nl ;
  rdfs:comment "Type of farthingale chair developed by the Asante people of Africa after the European prototype, decorated with brass tacks, having a low inclined back, and often with a leather-covered seat, used only by high-ranking or honored persons."@en ;
  rdfs:isDefinedBy <https://w3id.org/con-tax/components/aat-furn> ;
  rdfs:label "asipim"@en ;
  rdfs:label "asipim"@nl ;
  rdfs:seeAlso <http://vocab.getty.edu/aat/300263681> ;
  rdfs:subClassOf <https://w3id.org/con-tax/components/aat-furn#300077236> ;
  rdfs:subClassOf <https://w3id.org/con-tax/components/aat-furn#300133851> ;
.
<https://w3id.org/con-tax/components/aat-furn#300263682>
  rdf:type owl:Class ;
  rdfs:comment "Brass-studded prestige X-chairs of the Asante people of Africa, having arms, openwork backs, and legs that cross diagonally; the leg configuration is based on European folding chairs."@en ;
  rdfs:comment "Met  koper beslagen prestigieuze X-framestoelen van het Afrikaanse Asantevolk, met armleuningen een ajour bewerkte rug en diagonaal gekruiste poten; de vorm van de poten is afgeleid van Europese vouwstoelen."@nl ;
  rdfs:isDefinedBy <https://w3id.org/con-tax/components/aat-furn> ;
  rdfs:label "akonkromfi"@en ;
  rdfs:label "akonkromfi"@nl ;
  rdfs:seeAlso <http://vocab.getty.edu/aat/300263682> ;
  rdfs:subClassOf <https://w3id.org/con-tax/components/aat-furn#300037904> ;
  rdfs:subClassOf <https://w3id.org/con-tax/components/aat-furn#300133851> ;
.
<https://w3id.org/con-tax/components/aat-furn#300263787>
  rdf:type owl:Class ;
  rdfs:comment "Houten koffers waarin de heilige altaartabletten van de Ethiopisch-orthodoxe kerk worden bewaard; ze doen bij tijden ook dienst als altaartafel."@nl ;
  rdfs:comment "Wooden coffers in which are stored the sacred altar tablets of the Ethiopian Orthodox Church; they also at times serve as altar tables."@en ;
  rdfs:isDefinedBy <https://w3id.org/con-tax/components/aat-furn> ;
  rdfs:label "manbara tabots"@en ;
  rdfs:label "manbara tabots"@nl ;
  rdfs:seeAlso <http://vocab.getty.edu/aat/300263787> ;
  rdfs:subClassOf <https://w3id.org/con-tax/components/aat-furn#300039119> ;
.
<https://w3id.org/con-tax/components/aat-furn#300264255>
  rdf:type owl:Class ;
  rdfs:comment "Refers to boxes or chests of pedestal form for the Koran; it can also refer to thrones or preachers' seats in a mosque as well as to large lecterns on which readers of the Koran sit."@en ;
  rdfs:comment "Verwijst naar dozen of kisten als voetstuk voor de Koran; het kan ook verwijzen naar tronen of preekstoelen in een moskee en naar grote katheders waarop lezers van de Koran zitten."@nl ;
  rdfs:isDefinedBy <https://w3id.org/con-tax/components/aat-furn> ;
  rdfs:label "kursi's"@nl ;
  rdfs:label "kursis"@en ;
  rdfs:seeAlso <http://vocab.getty.edu/aat/300264255> ;
  rdfs:subClassOf <https://w3id.org/con-tax/components/aat-furn#300038141> ;
  rdfs:subClassOf <https://w3id.org/con-tax/components/aat-furn#300039794> ;
.
<https://w3id.org/con-tax/components/aat-furn#300264314>
  rdf:type owl:Class ;
  rdfs:comment "Having a convex curved front; the term is used particularly with reference to case furniture and to buildings."@en ;
  rdfs:comment "Met betrekking tot kastmeubilair: met een voorkant die ononderbroken buitenwaarts is gebogen, van de randen naar het midden."@nl ;
  rdfs:isDefinedBy <https://w3id.org/con-tax/components/aat-furn> ;
  rdfs:label "bowfront"@en ;
  rdfs:label "gebogen voorkant"@nl ;
  rdfs:seeAlso <http://vocab.getty.edu/aat/300264314> ;
  rdfs:subClassOf <https://w3id.org/con-tax/components/aat-furn#300037680> ;
.
<https://w3id.org/con-tax/components/aat-furn#300264537>
  rdf:type owl:Class ;
  rdfs:comment "Refers to tables having a set of cabinets above, used for writing. The form was popular in France, England, and America in the early 18th century. In modern usage, it is typically distinguished from an \"escritoire\" or a \"secretary.\""@en ;
  rdfs:comment "Verwijst naar schrijfmeubels die in het algemeen zijn voorzien van een rolluik. Een scrutoire kan ook bestaan uit een groep kastjes op een tafel die wordt gebruikt om op te schrijven. De scrutoire was begin 18de eeuw populair in Frankrijk, Engeland en de Verenigde Staten, maar werd ook later wel gebruikt. Tegenwoordig wordt een scrutoire doorgaans onderscheiden van een 'escritoire' of een 'secretaire' door de aanwezigheid van karakteristieke vakjes en laatjes boven het schrijfblad; de drie termen worden soms echter door elkaar gebruikt."@nl ;
  rdfs:isDefinedBy <https://w3id.org/con-tax/components/aat-furn> ;
  rdfs:label "scrutoires"@en ;
  rdfs:label "scrutoires"@nl ;
  rdfs:seeAlso <http://vocab.getty.edu/aat/300264537> ;
  rdfs:subClassOf <https://w3id.org/con-tax/components/aat-furn#300039338> ;
.
<https://w3id.org/con-tax/components/aat-furn#300264538>
  rdf:type owl:Class ;
  rdfs:comment "Refers to low chests of drawers often surmounted by a mirror and typically used in a bedroom or dressing room as a surface for grooming and to store clothing and toiletries. The term in this context is used primarily in America, and is derived from the European \"dresser (cupboard),\" which contains drawers and is surmounted by shelves, but is used to store kitchen utensils and dishes."@en ;
  rdfs:comment "Verwijst naar lage ladekasten met daarop een spiegel die doorgaans in slaap- of kleedkamers worden gebruikt voor de uiterlijke verzorging en om kledingstukken en toiletartikelen in op te bergen. In deze context wordt de term vooral gebruikt in de Verenigde Staten, en de Engelse term 'dresser' is afgeleid van het Europese begrip 'keukenkast (wandkast)', dat bestaat uit laden met planken daarop, maar wordt gebruikt om keukengerei in op te bergen."@nl ;
  rdfs:isDefinedBy <https://w3id.org/con-tax/components/aat-furn> ;
  rdfs:label "dressers (chests of drawers)"@en ;
  rdfs:label "toilettafels (ladekasten)"@nl ;
  rdfs:label "toilettafels"@nl ;
  rdfs:seeAlso <http://vocab.getty.edu/aat/300264538> ;
  rdfs:seeAlso wd:Q14169227 ;
  rdfs:subClassOf <https://w3id.org/con-tax/components/aat-furn#300039009> ;
.
<https://w3id.org/con-tax/components/aat-furn#300264555>
  rdf:type owl:Class ;
  rdfs:comment "Refers to benches on which stonecutters place blocks of stone in order to dress and prepare them."@en ;
  rdfs:comment "Verwijst naar banken waarop steenhouwers blokken steen plaatsen om deze te bewerken en te prepareren."@nl ;
  rdfs:isDefinedBy <https://w3id.org/con-tax/components/aat-furn> ;
  rdfs:label "bankers (benches)"@en ;
  rdfs:label "werkplanken"@nl ;
  rdfs:seeAlso <http://vocab.getty.edu/aat/300264555> ;
  rdfs:subClassOf <https://w3id.org/con-tax/components/aat-furn#300038494> ;
.
<https://w3id.org/con-tax/components/aat-furn#300264594>
  rdf:type owl:Class ;
  rdfs:comment "High-backed benches with a chest below the seat that doubled as a narrow bed, used primarily in Medieval and later Italian homes."@en ;
  rdfs:comment "Verwijst naar een bank met hoge rugleuning en een kist onder het zitvlak die tevens dienstdeed als een smal bed en voornamelijk werd gebruikt in Italiaanse woonhuizen uit de middeleeuwen en later."@nl ;
  rdfs:isDefinedBy <https://w3id.org/con-tax/components/aat-furn> ;
  rdfs:label "lettucci"@en ;
  rdfs:label "luttuci"@nl ;
  rdfs:seeAlso <http://vocab.getty.edu/aat/300264594> ;
  rdfs:subClassOf <https://w3id.org/con-tax/components/aat-furn#300038494> ;
  rdfs:subClassOf <https://w3id.org/con-tax/components/aat-furn#300038697> ;
.
<https://w3id.org/con-tax/components/aat-furn#300265064>
  rdf:type owl:Class ;
  rdfs:comment "Tables that can perform a variety of functions by rearranging or removing its parts such as the top and drawers, for example, to transform from a dressing table to a writing desk."@en ;
  rdfs:comment "Tafels die diverse functies kunnen vervullen door de onderdelen ervan, zoals het tafelblad en de laden, te herschikken of te verwijderen."@nl ;
  rdfs:isDefinedBy <https://w3id.org/con-tax/components/aat-furn> ;
  rdfs:label "mechanical tables"@en ;
  rdfs:label "mechanische tafels"@nl ;
  rdfs:seeAlso <http://vocab.getty.edu/aat/300265064> ;
  rdfs:subClassOf <https://w3id.org/con-tax/components/aat-furn#300039548> ;
  rdfs:subClassOf <https://w3id.org/con-tax/components/aat-furn#300040036> ;
.
<https://w3id.org/con-tax/components/aat-furn#300265131>
  rdf:type owl:Class ;
  rdfs:comment "Devices for supporting a cross on the altar and by extension, any device for supporting or fixing a cross at or near the altar. As early as the 5th and 6th centuries there is evidence in Byzantine art of partly combined candlesticks and cross, which are the precursors to cross feet as the form developed in the later Middle Ages. There are four main groups of cross feet placed on the altar: four-sided, three-sided, circular, and architectural."@en ;
  rdfs:comment "Middel ter ondersteuning van een kruis op het altaar of, bij uitbreiding, ieder middel ter ondersteuning of bevestiging van een kruis bij of nabij het altaar. Al in de 5de en 6de eeuw zijn er in Byzantijnse kunst aanwijzingen te vinden van gedeeltelijke combinaties van kandelaars en kruizen, die de voorlopers vormen van de kruisvoeten zoals deze in de late middeleeuwen werden ontwikkeld. Er zijn vier hoofdsoorten van op het altaar geplaatste kruisvoeten: vierkantige, driekantige, ronde en architectonische."@nl ;
  rdfs:isDefinedBy <https://w3id.org/con-tax/components/aat-furn> ;
  rdfs:label "cross feet"@en ;
  rdfs:label "kruisvoeten"@nl ;
  rdfs:seeAlso <http://vocab.getty.edu/aat/300265131> ;
  rdfs:subClassOf <https://w3id.org/con-tax/components/aat-furn#300039337> ;
.
<https://w3id.org/con-tax/components/aat-furn#300265144>
  rdf:type owl:Class ;
  rdfs:comment "Schraagstandaarden uit de Spaanse renaissance, die dienden als onderstel voor varguenos. Aan elke kant van de standaard zitten krukken waar de uiklapbare voorkant van het kabinet op kan steunen."@nl ;
  rdfs:comment "Spanish Renaissance trestle stands used to support vargueños; oblong pulls on each side of the stand support the drop-front of the cabinet."@en ;
  rdfs:isDefinedBy <https://w3id.org/con-tax/components/aat-furn> ;
  rdfs:label "pies de puente"@en ;
  rdfs:label "pies de puente"@nl ;
  rdfs:seeAlso <http://vocab.getty.edu/aat/300265144> ;
  rdfs:subClassOf <https://w3id.org/con-tax/components/aat-furn#300039767> ;
.
<https://w3id.org/con-tax/components/aat-furn#300265151>
  rdf:type gvp:GuideTerm ;
  rdfs:comment "Refers to barriers for the subdivision of churches into areas of differing function and liturgical significance."@en ;
  rdfs:comment "Verwijst naar afscheidingen bedoeld om kerken onder te verdelen in ruimten met verschillende functies of van groter of kleiner liturgisch belang."@nl ;
  rdfs:isDefinedBy <https://w3id.org/con-tax/components/aat-furn> ;
  rdfs:label "<scherm of hek in christelijk religieus gebouw>"@nl ;
  rdfs:label "<schermen of hekken in christelijke religieuze gebouwen>"@nl ;
  rdfs:label "<screens in Christian religious buildings>"@en ;
  rdfs:label "scherm of hek in christelijk religieus gebouw"@nl ;
  rdfs:label "schermen of hekken in christelijke religieuze gebouwen"@nl ;
  rdfs:seeAlso <http://vocab.getty.edu/aat/300265151> ;
  contax:containsConcept <https://w3id.org/con-tax/components/aat-furn#300003784> ;
  contax:containsConcept <https://w3id.org/con-tax/components/aat-furn#300065017> ;
  contax:containsConcept <https://w3id.org/con-tax/components/aat-furn#300065029> ;
  contax:containsConcept <https://w3id.org/con-tax/components/aat-furn#300075947> ;
  contax:containsConcept <https://w3id.org/con-tax/components/aat-furn#300076058> ;
  contax:containsConcept <https://w3id.org/con-tax/components/aat-furn#300078129> ;
  contax:containsConcept <https://w3id.org/con-tax/components/aat-furn#300109707> ;
  contax:containsConcept <https://w3id.org/con-tax/components/aat-furn#300265153> ;
  contax:containsConcept <https://w3id.org/con-tax/components/aat-furn#300265155> ;
  contax:containsConcept <https://w3id.org/con-tax/components/aat-furn#300265157> ;
  contax:containsConcept <https://w3id.org/con-tax/components/aat-furn#300404223> ;
.
<https://w3id.org/con-tax/components/aat-furn#300265153>
  rdf:type owl:Class ;
  rdfs:comment "Screens between the choir and body of the church, particularly the low screens that served to separate the chancel from the nave. Cancellos were widespread in the Early Christian period, particularly in Rome, and continued throughout the Middle Ages. This early form of screen was gradually expanded into the higher, deeper, and generally more elaborate rood screen."@en ;
  rdfs:comment "Verwijst naar lage schermen die als scheidingswand tussen het koor en het schip fungeerden. In de vroegchristelijke periode werden ze veelvuldig toegepast, met name in Rome, en ze bleven tot in de Middeleeuwen in gebruik. Dit vroege type koorafsluiting werd geleidelijk uitgebreid tot het hogere, diepere en doorgaans rijker gedecoreerde koorhek."@nl ;
  rdfs:isDefinedBy <https://w3id.org/con-tax/components/aat-furn> ;
  rdfs:label "cancelli"@nl ;
  rdfs:label "cancellos"@en ;
  rdfs:seeAlso <http://vocab.getty.edu/aat/300265153> ;
  rdfs:subClassOf <https://w3id.org/con-tax/components/aat-furn#300037737> ;
  rdfs:subClassOf <https://w3id.org/con-tax/components/aat-furn#300076058> ;
.
<https://w3id.org/con-tax/components/aat-furn#300265155>
  rdf:type owl:Class ;
  rdfs:comment "Chancel screens surmounted by a cross or crucifix, and which evolved from 'rood beams.' Rood screens are often richly adorned and are sometimes double with vaulting between and a rood loft on top. The French term of 'jubé' derives from the Latin phrase Jube domine benedicere (\"Let us bless the Lord\"), which is often said by Catholic priests before the lesson while standing in front of the screen; some jubés have a balcony or platform from which to preach to the laity."@en ;
  rdfs:comment "Te gebruiken voor koorschermen waarop een kruis of crucifix is geplaatst. Koorhekken zijn vaak rijk gedecoreerd en komen soms in een dubbele vorm voor, met gewelfbogen ertussen en een doksaal daarboven. De Franse term 'jubé' is afgeleid van Jube domine benedicere ('Heer, wil mij zegenen'), een Latijnse zin die vaak voor de mis door de katholieke priester wordt uitgesproken terwijl deze voor het scherm staat; sommige jubés zijn voorzien van een balkon of verhoging waarop de priester de gemeente toespreekt."@nl ;
  rdfs:isDefinedBy <https://w3id.org/con-tax/components/aat-furn> ;
  rdfs:label "koorhekken"@nl ;
  rdfs:label "rood screens"@en ;
  rdfs:seeAlso <http://vocab.getty.edu/aat/300265155> ;
  rdfs:seeAlso wd:Q837995 ;
  rdfs:subClassOf <https://w3id.org/con-tax/components/aat-furn#300037737> ;
  rdfs:subClassOf <https://w3id.org/con-tax/components/aat-furn#300076058> ;
.
<https://w3id.org/con-tax/components/aat-furn#300265156>
  rdf:type owl:Class ;
  rdfs:comment "Refers to screens comprising two or more panels in a frame which has hinged sections that can be folded to adjust coverage. They are often decorated. Early examples include the Chinese form, mentioned as early as the 2nd century BCE. The earliest surviving examples date to the Ming dynasty. Folding screens were introduced to Japan from China in the 8th century; such screens were often designed in pairs in Japan. From the early 17th century eastern folding screens were imported to Europe and the form was soon adopted by European craftsmen. "@en ;
  rdfs:comment "Verwijst naar schermen die bestaan uit twee of meer panelen en doorgaans versierd en vaak gelakt zijn. De vorm is uitgevonden door de Chinezen en werd in de 2de eeuw v. Chr. reeds genoemd. De oudste nog bestaande exemplaren dateren van de Ming-dynastie. Vouwschermen werden in de 8ste eeuw vanuit China in Japan geïntroduceerd; deze schermen werden vaak paarsgewijs ontworpen in Japan. Vanaf de 17de eeuw werden oosterse vouwschermen in Europa geïmporteerd en de vorm werd al snel overgenomen door Europese vaklieden. Net als de Japanse bestonden de Europese vouwschermen doorgaans uit zes panelen; ze waren echter vaak hoger en kloeker."@nl ;
  rdfs:isDefinedBy <https://w3id.org/con-tax/components/aat-furn> ;
  rdfs:label "folding screens"@en ;
  rdfs:label "kamerscherm"@nl ;
  rdfs:label "kamerschermen"@nl ;
  rdfs:seeAlso <http://vocab.getty.edu/aat/300265156> ;
  rdfs:subClassOf <https://w3id.org/con-tax/components/aat-furn#300037737> ;
.
<https://w3id.org/con-tax/components/aat-furn#300265157>
  rdf:type owl:Class ;
  rdfs:comment "Refers to screens surrounding or placed in front of confessionals in order to shield penitents from public view."@en ;
  rdfs:comment "Verwijst naar schermen rond of voor een biechtstoel, bedoeld om de biechtelingen aan het zicht te onttrekken."@nl ;
  rdfs:isDefinedBy <https://w3id.org/con-tax/components/aat-furn> ;
  rdfs:label "pardon screens"@en ;
  rdfs:label "pardon screens"@nl ;
  rdfs:seeAlso <http://vocab.getty.edu/aat/300265157> ;
  rdfs:subClassOf <https://w3id.org/con-tax/components/aat-furn#300037737> ;
.
<https://w3id.org/con-tax/components/aat-furn#300265169>
  rdf:type owl:Class ;
  rdfs:comment "Refers to screens consisting of one panel, typically made of wood with low legs. The single-panel screen is generally the smallest of the three types of screens in East Asia. Single-panel screens in China were set in stands and were usually of lacquer; the panels often framed a painted picture, jade panel, or looking glass. In Japan such screens were stationery and used at the entrance of a house to denote status or a ceremony in progress. "@en ;
  rdfs:comment "Verwijst naar schermen die bestaan uit één paneel, doorgaans gemaakt van hout met lage poten. Het enkelvoudige scherm is in het algemeen de kleinste van de drie typen schermen in Oost-Azië. Enkelvoudige schermen uit China werden in standaards geplaatst en doorgaans gelakt; de panelen bevatten vaak een geschilderd tafereel, jadepaneel of spiegel. In Japan werden dergelijke panelen vaak vast gemonteerd en bij de ingang van een huis gebruikt als statussymbool of om aan te geven dat er een ceremonie aan de gang was."@nl ;
  rdfs:isDefinedBy <https://w3id.org/con-tax/components/aat-furn> ;
  rdfs:label "enkelvoudige schermen"@nl ;
  rdfs:label "single-panel screens"@en ;
  rdfs:seeAlso <http://vocab.getty.edu/aat/300265169> ;
  rdfs:subClassOf <https://w3id.org/con-tax/components/aat-furn#300037737> ;
.
<https://w3id.org/con-tax/components/aat-furn#300265170>
  rdf:type owl:Class ;
  rdfs:comment "Refers to semi-permanent screens sliding in tracks that are characteristic features of traditional Japanese architecture. They can be open and closed or removed altogether to alter the dimensions or character of a room. Location determined the materials from which they were made: wood was typically used for screens near the exterior of a building, while screens made of wooden lattices covered with translucent paper, painted or upainted, were more often used for interior rooms."@en ;
  rdfs:comment "Verwijst naar semipermanente, in schuifprofielen geplaatste schermen die een karakteristiek element in traditionele Japanse bouwkunst vormen. Ze kunnen worden geopend en gesloten of helemaal worden verwijderd om aldus de afmetingen of het karakter van een kamer te veranderen. De locatie van de schermen bepaalde het materiaalgebruik: hout werd doorgaans gebruikt voor schermen nabij de buitenkant van een gebouw, terwijl schermen van doorschijnend, beschilderd of onbeschilderd papier op een houten raamwerk meestal werden gebruikt voor binnenkamers."@nl ;
  rdfs:isDefinedBy <https://w3id.org/con-tax/components/aat-furn> ;
  rdfs:label "fusuma"@en ;
  rdfs:label "fusuma"@nl ;
  rdfs:seeAlso <http://vocab.getty.edu/aat/300265170> ;
  rdfs:seeAlso wd:Q1069573 ;
  rdfs:subClassOf <https://w3id.org/con-tax/components/aat-furn#300037737> ;
.
<https://w3id.org/con-tax/components/aat-furn#300265171>
  rdf:type owl:Class ;
  rdfs:comment "Refers to a type of Chinese folding screen that was typically very large, as tall as ten feet in height and twenty in length, with twelve panels of lacquered and gilded wood. Coromandel screens feature incised lacquer decoration and often have wide borders around the main design. The name comes from a part of the southeastern Indian coast near Madras that was a transfer point for Far Eastern goods being shipped to Europe by England's East India Company. Coromandel screens were mainly made in China in the 17th and 18th centuries for the European market."@en ;
  rdfs:comment "Verwijst naar een type Chinese kamerschermen die doorgaans een zeer forse omvang hadden, tot wel drie meter hoog en zes meter breed, met twaalf panelen van gelakt en verguld hout. Coromandel-schermen bevatten ingesneden en gelakte decoraties en hebben vaak een brede rand om het hoofdonderwerp. De naam is afkomstig van een deel van de kust van Zuidoost-India bij Madras, waar goederen uit het Verre Oosten werden overgeslagen om verder door de Engelse East India Company naar Europa te worden vervoerd. Coromandel-schermen werden voornamelijk in de 17de en 18de eeuw in China gemaakt voor de Europese markt."@nl ;
  rdfs:isDefinedBy <https://w3id.org/con-tax/components/aat-furn> ;
  rdfs:label "Chinese Coromandel screens"@en ;
  rdfs:label "Chinese coromandel-schermen"@nl ;
  rdfs:seeAlso <http://vocab.getty.edu/aat/300265171> ;
  rdfs:subClassOf <https://w3id.org/con-tax/components/aat-furn#300265156> ;
.
<https://w3id.org/con-tax/components/aat-furn#300265174>
  rdf:type owl:Class ;
  rdfs:comment "Refers to small decorative screens, usually Chinese or Japanese, made to stand on tables. Table screens can be either single-panel screens or folding screens."@en ;
  rdfs:comment "Verwijst naar kleine decoratieve schermen, meestal van Chinese of Japanse herkomst, die zijn bedoeld om op een tafel te worden gezet. Tafelschermen kunnen uit één of meerdere panelen bestaan."@nl ;
  rdfs:isDefinedBy <https://w3id.org/con-tax/components/aat-furn> ;
  rdfs:label "table screens"@en ;
  rdfs:label "tafelschermen"@nl ;
  rdfs:seeAlso <http://vocab.getty.edu/aat/300265174> ;
  rdfs:subClassOf <https://w3id.org/con-tax/components/aat-furn#300037737> ;
.
<https://w3id.org/con-tax/components/aat-furn#300265196>
  rdf:type owl:Class ;
  rdfs:comment "Refers to a type of French chaise longue featuring a foot surrounded on three sides by a low curving back."@en ;
  rdfs:comment "Verwijst naar een type Franse chaise longue met een poot die aan drie kanten wordt omringd door een lage, gewelfde rugleuning."@nl ;
  rdfs:isDefinedBy <https://w3id.org/con-tax/components/aat-furn> ;
  rdfs:label "duchesses en bateau"@en ;
  rdfs:label "duchesses en bateau"@nl ;
  rdfs:seeAlso <http://vocab.getty.edu/aat/300265196> ;
  rdfs:subClassOf <https://w3id.org/con-tax/components/aat-furn#300165523> ;
.
<https://w3id.org/con-tax/components/aat-furn#300265197>
  rdf:type owl:Class ;
  rdfs:comment "Refers to a simpler type of bed that originated in France in the first half of the 17th century, replacing the massive carved frames of earlier beds. The frame of a lit à housse was a simple cubelike form, broken only by plumed finials at the corners of the tester, and covered entirely in fabric. This type of bed featured a deep valance and four curtains: two wide curtains went from the center of the foot of the bed round the outside of the footposts and to the center of the sides; two narrow curtains went from the bedhead to the center of the sides. Towards the end of the century the lit à housse became more elaborate and taller, although the frame continued to be entirely covered by fabric. Lits à housse are so-called because they resemble a grand state bed with its protective covers."@en ;
  rdfs:comment "Verwijst naar een vereenvoudigd type bed dat dateert uit de eerste helft van de 17de eeuw, waarbij de zware gesneden frames van oude bedden werden vervangen. Het frame van een lit à housse had een eenvoudige kubusachtige vorm die slechts werd onderbroken door prions met veren op de hoeken van het baldakijn, en was volledig overtrokken met textiel. Dit type bed had een hoge val en vier gordijnen: twee brede gordijnen liepen vanaf het midden van het voeteneinde via de buitenkant van de stijlen aan het voeteneinde naar het midden van beide zijkanten; de smalle gordijnen liepen vanaf het hoofdeinde van het bed naar midden van de zijkanten. Rond het eind van de eeuw werden lits à housse verfijnder afgewerkt en hoger, terwijl het frame volledig met textiel overtrokken bleef. Lits à housse worden zo genoemd omdat ze op vanwege de beschermende overtrekken doen denken aan voorname staatsbedden."@nl ;
  rdfs:isDefinedBy <https://w3id.org/con-tax/components/aat-furn> ;
  rdfs:label "lits à housse"@en ;
  rdfs:label "lits à housse"@nl ;
  rdfs:seeAlso <http://vocab.getty.edu/aat/300265197> ;
  rdfs:subClassOf <https://w3id.org/con-tax/components/aat-furn#300038697> ;
.
<https://w3id.org/con-tax/components/aat-furn#300265223>
  rdf:type owl:Class ;
  rdfs:comment "Curule-stoel die is afgeleid van de vouwkrukken met gekruist onderstel uit het oude Egypte. De stoel wordt gekenmerkt door een niet-vouwbare curule-onderstel met daarop een verstelbare rugleuning van reliëfleer of riet. Aangenomen wordt dat ze van Spaanse herkomst zijn en ze zijn genoemd naar de havenstad op het schiereiland Yucatán. Veelvuldig aangetroffen in Louisiana tussen plantagemeubilair uit de 19de eeuw."@nl ;
  rdfs:comment "Curule-type chair that derives from the x-frame folding stools of ancient Egypt. It is characterized by a non-folding curule base supporting an embossed leather or cane sling back and seat. Believed to be of Spanish origin, they are named for the port city on the Yucatán Peninsula. Often found in Louisiana among plantation furniture of the 19th century."@en ;
  rdfs:isDefinedBy <https://w3id.org/con-tax/components/aat-furn> ;
  rdfs:label "campeche chairs"@en ;
  rdfs:label "campeche-stoelen"@nl ;
  rdfs:seeAlso <http://vocab.getty.edu/aat/300265223> ;
  rdfs:subClassOf <https://w3id.org/con-tax/components/aat-furn#300037772> ;
.
<https://w3id.org/con-tax/components/aat-furn#300265230>
  rdf:type owl:Class ;
  rdfs:comment "Refers to beds in the shape of a shallow basket, primarily found during the period of the French Restoration in the early 19th century."@en ;
  rdfs:comment "Verwijst naar bedden in de vorm van een ondiepe mand, vooral aangetroffen tijdens de Franse Restauratie van begin 19de eeuw."@nl ;
  rdfs:isDefinedBy <https://w3id.org/con-tax/components/aat-furn> ;
  rdfs:label "lits en corbeille"@en ;
  rdfs:label "lits en corbeille"@nl ;
  rdfs:seeAlso <http://vocab.getty.edu/aat/300265230> ;
  rdfs:subClassOf <https://w3id.org/con-tax/components/aat-furn#300038697> ;
.
<https://w3id.org/con-tax/components/aat-furn#300265614>
  rdf:type owl:Class ;
  rdfs:comment "Multi-panelled sanctuary screens like those used in the Eastern Orthodox church, but on a small scale. Used in private devotion in a family chapel, in private homes, or for travel. The depiction of saints matched that of the church iconostasis."@en ;
  rdfs:comment "Voor sanctuaria bestemde schermen bestaande uit meerdere panelen zoals die in oosters-orthodoxe kerken voorkomen, maar dan op kleinere schaal uitgevoerd. Gebruikt voor privédevotie in familiekapellen, woonhuizen of op reis. De heiligen werden op dezelfde wijze afgebeeld als op iconostasen in kerken."@nl ;
  rdfs:isDefinedBy <https://w3id.org/con-tax/components/aat-furn> ;
  rdfs:label "portable iconostases"@en ;
  rdfs:label "reisiconostasen"@nl ;
  rdfs:seeAlso <http://vocab.getty.edu/aat/300265614> ;
  rdfs:subClassOf <https://w3id.org/con-tax/components/aat-furn#300003784> ;
.
<https://w3id.org/con-tax/components/aat-furn#300265646>
  rdf:type owl:Class ;
  rdfs:comment "Armless chair used in the chancel by a bishop or prelate while officiating at a church not his own. For ecclesiastical folding stools used by worshippers in various functions, use \"faldstools.\" For French domestic folding stools from the 17th century on, use \"pliants.\""@en ;
  rdfs:comment "Stoel zonder armleuningen die in het koor wordt gebruikt door een bisschop of prelaat als deze de mis opdraagt in een andere kerk dan de zijne. Gebruik 'bisschopskrukken' voor kerkelijke vouwbankjes die voor diverse doeleinden door kerkgangers worden gebruikt. Gebruik 'pliants' voor 17de-eeuwse Franse vouwkrukjes voor huiselijk gebruik."@nl ;
  rdfs:isDefinedBy <https://w3id.org/con-tax/components/aat-furn> ;
  rdfs:label "faldistoria (bisschopsstoelen)"@nl ;
  rdfs:label "faldistoria"@nl ;
  rdfs:label "faldistories (bishops' chairs)"@en ;
  rdfs:seeAlso <http://vocab.getty.edu/aat/300265646> ;
  rdfs:subClassOf <https://w3id.org/con-tax/components/aat-furn#300244761> ;
.
<https://w3id.org/con-tax/components/aat-furn#300265762>
  rdf:type owl:Class ;
  rdfs:comment "Small tables supported on legs, pillar, or tripod, with an adjustable top, hinged to fold flat. GLOAG."@en ;
  rdfs:comment "Tafeltjes ondersteund door één, drie of vier pootjes met een verstelbaar blad en een scharnier om ze in te klappen."@nl ;
  rdfs:isDefinedBy <https://w3id.org/con-tax/components/aat-furn> ;
  rdfs:label "leestafels"@nl ;
  rdfs:label "reading tables"@en ;
  rdfs:seeAlso <http://vocab.getty.edu/aat/300265762> ;
  rdfs:subClassOf <https://w3id.org/con-tax/components/aat-furn#300039548> ;
.
<https://w3id.org/con-tax/components/aat-furn#300266178>
  rdf:type owl:Class ;
  rdfs:comment "Folding screens, originally secular, painted during the late Heian period, and later used in Buddhist ordination ceremonies. "@en ;
  rdfs:comment "Oorspronkelijk niet-religieuze vouwschermen die in de late Heian-periode werden geschilderd en later werden gebruikt in boeddhistische inwijdingsrituelen."@nl ;
  rdfs:isDefinedBy <https://w3id.org/con-tax/components/aat-furn> ;
  rdfs:label "senzui byōbu"@en ;
  rdfs:label "senzui byōbu"@nl ;
  rdfs:seeAlso <http://vocab.getty.edu/aat/300266178> ;
  rdfs:subClassOf <https://w3id.org/con-tax/components/aat-furn#300265156> ;
.
<https://w3id.org/con-tax/components/aat-furn#300266343>
  rdf:type owl:Class ;
  rdfs:comment "Furniture specially designed for or used outdoors in a garden."@en ;
  rdfs:comment "Meubels die speciaal zijn ontworpen om in de openlucht in tuinen te gebruiken."@nl ;
  rdfs:isDefinedBy <https://w3id.org/con-tax/components/aat-furn> ;
  rdfs:label "garden furniture"@en ;
  rdfs:label "tuinmeubel"@nl ;
  rdfs:label "tuinmeubels"@nl ;
  rdfs:seeAlso <http://vocab.getty.edu/aat/300266343> ;
  rdfs:seeAlso wd:Q2744736 ;
  rdfs:subClassOf <https://w3id.org/con-tax/components/aat-furn#300165810> ;
.
<https://w3id.org/con-tax/components/aat-furn#300266344>
  rdf:type owl:Class ;
  rdfs:comment "Furniture specially designed for or used outdoors on a porch."@en ;
  rdfs:comment "Meubels die speciaal zijn bedoeld om in de openlucht op veranda's te gebruiken."@nl ;
  rdfs:isDefinedBy <https://w3id.org/con-tax/components/aat-furn> ;
  rdfs:label "porch furniture"@en ;
  rdfs:label "verandameubel"@nl ;
  rdfs:label "verandameubels"@nl ;
  rdfs:seeAlso <http://vocab.getty.edu/aat/300266344> ;
  rdfs:subClassOf <https://w3id.org/con-tax/components/aat-furn#300165810> ;
.
<https://w3id.org/con-tax/components/aat-furn#300266345>
  rdf:type owl:Class ;
  rdfs:comment "Furniture specially designed for or used outdoors in a patio."@en ;
  rdfs:comment "Meubels die speciaal zijn bedoeld om in de openlucht op patio's te gebruiken."@nl ;
  rdfs:isDefinedBy <https://w3id.org/con-tax/components/aat-furn> ;
  rdfs:label "patio furniture"@en ;
  rdfs:label "patiomeubel"@nl ;
  rdfs:label "patiomeubels"@nl ;
  rdfs:seeAlso <http://vocab.getty.edu/aat/300266345> ;
  rdfs:seeAlso wd:Q2744736 ;
  rdfs:subClassOf <https://w3id.org/con-tax/components/aat-furn#300165810> ;
.
<https://w3id.org/con-tax/components/aat-furn#300266346>
  rdf:type gvp:GuideTerm ;
  rdfs:isDefinedBy <https://w3id.org/con-tax/components/aat-furn> ;
  rdfs:label "<buitenmeubels naar algemeen type>"@nl ;
  rdfs:label "<outdoor furniture by general type>"@en ;
  rdfs:label "buitenmeubels naar algemeen type"@nl ;
  rdfs:seeAlso <http://vocab.getty.edu/aat/300266346> ;
  contax:containsConcept <https://w3id.org/con-tax/components/aat-furn#300266343> ;
  contax:containsConcept <https://w3id.org/con-tax/components/aat-furn#300266344> ;
  contax:containsConcept <https://w3id.org/con-tax/components/aat-furn#300266345> ;
.
<https://w3id.org/con-tax/components/aat-furn#300266347>
  rdf:type gvp:GuideTerm ;
  rdfs:isDefinedBy <https://w3id.org/con-tax/components/aat-furn> ;
  rdfs:label "<buitenmeubels naar specifiek type>"@nl ;
  rdfs:label "<outdoor furniture by specific type>"@en ;
  rdfs:label "buitenmeubels naar specifiek type"@nl ;
  rdfs:seeAlso <http://vocab.getty.edu/aat/300266347> ;
  contax:containsConcept <https://w3id.org/con-tax/components/aat-furn#300037837> ;
  contax:containsConcept <https://w3id.org/con-tax/components/aat-furn#300038524> ;
  contax:containsConcept <https://w3id.org/con-tax/components/aat-furn#300039755> ;
  contax:containsConcept <https://w3id.org/con-tax/components/aat-furn#300133811> ;
  contax:containsConcept <https://w3id.org/con-tax/components/aat-furn#300164278> ;
  contax:containsConcept <https://w3id.org/con-tax/components/aat-furn#300171702> ;
.
<https://w3id.org/con-tax/components/aat-furn#300266583>
  rdf:type owl:Class ;
  rdfs:comment "Chairs having a seat that is a shaped and contoured plank drilled with sockets on the upper and lower surfaces to anchor the back and undercarriage and having the rear legs and a back that are separate rather than continuous members. The elements of the back are vertical, horizontal, or curved, and spindles may or may not be present. Chairs using bentwood back frame and legs pegged directly into the seat instead of being framed with aprons. The style is so named for chairs originating around Windsor Castle in England between 1700 and 1725, and was made by wheelwrights or turners, rather than cabinetmakers."@en ;
  rdfs:comment "Stoelen waarbij de zitting bestaat uit een bewerkte plank waarbij holtes in het bovenste en onderste oppervlak zijn geboord om de achterkant en het onderstel te verankeren. De achterpoten en de rugleuning staan los van elkaar in plaats van dat ze een doorlopend geheel vormen. De elementen van de rugleuning zijn verticaal, horizontaal of gebogen en spijlen kunnen een onderdeel van de stoel vormen."@nl ;
  rdfs:isDefinedBy <https://w3id.org/con-tax/components/aat-furn> ;
  rdfs:label "Windsor chairs"@en ;
  rdfs:label "Windsorstoel"@nl ;
  rdfs:label "Windsorstoelen"@nl ;
  rdfs:seeAlso <http://vocab.getty.edu/aat/300266583> ;
  rdfs:seeAlso wd:Q635443 ;
  rdfs:subClassOf <https://w3id.org/con-tax/components/aat-furn#300037772> ;
.
<https://w3id.org/con-tax/components/aat-furn#300266704>
  rdf:type owl:Class ;
  rdfs:comment "Boards upon which notes, messages, bulletins, and advertisements are posted, often in a public place. Also may refer to an online facility that performs the same function."@en ;
  rdfs:comment "Borden waarop men briefjes, boodschappen, communiqués en advertenties kan ophangen, vaak in een publieke ruimte. Men gebruikt de term ook voor digitale faciliteiten met deze functie."@nl ;
  rdfs:isDefinedBy <https://w3id.org/con-tax/components/aat-furn> ;
  rdfs:label "bulletin boards"@en-us ;
  rdfs:label "mededelingenbord"@nl ;
  rdfs:label "mededelingenborden"@nl ;
  rdfs:label "mededelingenborden; mededelingenbord"@nl ;
  rdfs:seeAlso <http://vocab.getty.edu/aat/300266704> ;
  rdfs:subClassOf <https://w3id.org/con-tax/components/aat-furn#300037680> ;
.
<https://w3id.org/con-tax/components/aat-furn#300266715>
  rdf:type owl:Class ;
  rdfs:comment "Furniture designed for use by children rather than for adults."@en ;
  rdfs:isDefinedBy <https://w3id.org/con-tax/components/aat-furn> ;
  rdfs:label "children's furniture"@en ;
  rdfs:seeAlso <http://vocab.getty.edu/aat/300266715> ;
  rdfs:subClassOf <https://w3id.org/con-tax/components/aat-furn#300037680> ;
.
<https://w3id.org/con-tax/components/aat-furn#300266737>
  rdf:type owl:Class ;
  rdfs:comment "Oorspronkelijk de benaming voor een kist of koffer waarin men objecten bewaarde en ook voor een hok in de vorm van een kist waarin dieren werden opgesloten. Tegenwoordig gebruikt men de term voor een meubel in de eetkamer bestaande uit een blad op een stevige constructie of solide poten en daarop een kast met deuren of open planken."@nl ;
  rdfs:comment "Originally a chest or coffer in which things were stored, including a  box-like pen in which an animal was confined. Today the term typically refers to a dining room case piece with a surface surmounted by an enclosed cupboard or open shelves, generally resting on either a relatively solid base or taller legs."@en ;
  rdfs:isDefinedBy <https://w3id.org/con-tax/components/aat-furn> ;
  rdfs:label "buffetkast"@nl ;
  rdfs:label "buffetkasten"@nl ;
  rdfs:label "hutches"@en ;
  rdfs:seeAlso <http://vocab.getty.edu/aat/300266737> ;
  rdfs:subClassOf <https://w3id.org/con-tax/components/aat-furn#300038860> ;
  rdfs:subClassOf <https://w3id.org/con-tax/components/aat-furn#300040157> ;
.
<https://w3id.org/con-tax/components/aat-furn#300266738>
  rdf:type owl:Class ;
  rdfs:comment "Case furniture on low legs, popular during the Victorian period. It is characterized by being divided in half vertically, with one half comprising shelves enclosed by a wooden or glass-fronted door, for the storage of books, dishes, or curiosities, and the other side often comprising a secretary, cabinet, or some combination of mirror, drawers, and fold-down desk top. Distinguished from a chifforobe, which is case furniture also divided vertically, but typically characterized by placement in a bedroom, having a narrow clothes closet on one side, and a narrow chest of drawers with a mirror on the other side."@en ;
  rdfs:comment "Kasten op lage poten die in het victoriaanse tijdperk populair waren. De kast is verticaal in tweeën gedeeld, waarbij het ene deel bestaat uit planken met een houten of glazen deur ervoor, bedoeld voor boeken, borden of curiosa, en het andere deel uit een secretaire, een kabinet of een combinatie van een spiegel, laden en een neerklapbaar tafelblad. Te onderscheiden van chifforobes: kasten die ook verticaal in tweeën zijn gedeeld, maar die meestal in slaapkamers worden gebruikt, met een smal gedeelte voor kleren aan de ene kant en laden en een spiegel aan de andere kant."@nl ;
  rdfs:isDefinedBy <https://w3id.org/con-tax/components/aat-furn> ;
  rdfs:label "side by sides (case furniture)"@en ;
  rdfs:label "side by sides (kasten)"@nl ;
  rdfs:label "side by sides"@nl ;
  rdfs:seeAlso <http://vocab.getty.edu/aat/300266738> ;
  rdfs:subClassOf <https://w3id.org/con-tax/components/aat-furn#300038860> ;
.
<https://w3id.org/con-tax/components/aat-furn#300266804>
  rdf:type owl:Class ;
  rdfs:comment "Lessenaar voor boeken of ander leesmateriaal voor gebeden, studie of voordrachten. Afkomstig van het Duitse woord ���stehender', dat ���staande' betekent."@nl ;
  rdfs:comment "Reading stands used to support a book or other reading material for prayer, study, or speaking. Ultimately from the German \"stehender,\" meaning \"standing\" or \"upright.\""@en ;
  rdfs:isDefinedBy <https://w3id.org/con-tax/components/aat-furn> ;
  rdfs:label "shtender"@nl ;
  rdfs:label "shtenders"@en ;
  rdfs:label "shtenders"@nl ;
  rdfs:seeAlso <http://vocab.getty.edu/aat/300266804> ;
  rdfs:subClassOf <https://w3id.org/con-tax/components/aat-furn#300170801> ;
.
<https://w3id.org/con-tax/components/aat-furn#300298862>
  rdf:type owl:Class ;
  rdfs:comment "Algemene term voor constructies die bedoeld zijn voor de overblijfselen van overledenen. Met name gebruikt voor Etruskische, oud-Griekse en oud-Egyptische tomben."@nl ;
  rdfs:comment "General term for secure chests or arks intended to contain the remains of the deceased, used particularly for such chests from ancient Greek, Etruscan, and Egyptian cultures."@en ;
  rdfs:isDefinedBy <https://w3id.org/con-tax/components/aat-furn> ;
  rdfs:label "graftombe"@nl ;
  rdfs:label "graftomben"@nl ;
  rdfs:label "sepulchral chests"@en ;
  rdfs:seeAlso <http://vocab.getty.edu/aat/300298862> ;
  rdfs:subClassOf <https://w3id.org/con-tax/components/aat-furn#300139717> ;
.
<https://w3id.org/con-tax/components/aat-furn#300298883>
  rdf:type owl:Class ;
  rdfs:comment "Piece of sacristy furniture in the form of a cupboard, intended to store a variety of liturgical objects, such as robes, apparel, and altar vestments, or used for other liturgy-related functions. It may be either an isolated piece of furniture, built into the wall, or incorporated as an integral part of the sacristy furnishings. It is generally surmounted by a cross or a religious symbol. "@en ;
  rdfs:comment "Sacristiemeubel in de vorm van een kast, bedoeld voor het bewaren van diverse liturgische objecten, zoals priestergewaden en altaargewaden, of voor andere liturgische doeleinden. Ingebouwd in de muur, een los meubelstuk of een integraal onderdeel van het sacristiemeubilair. Gewoonlijk is bovenaan een kruis aangebracht of een ander religieus symbool."@nl ;
  rdfs:isDefinedBy <https://w3id.org/con-tax/components/aat-furn> ;
  rdfs:label "sacristiekast"@nl ;
  rdfs:label "sacristiekasten"@nl ;
  rdfs:label "sacristy cupboards"@en ;
  rdfs:seeAlso <http://vocab.getty.edu/aat/300298883> ;
  rdfs:subClassOf <https://w3id.org/con-tax/components/aat-furn#300039183> ;
.
<https://w3id.org/con-tax/components/aat-furn#300298887>
  rdf:type owl:Class ;
  rdfs:comment "Cupboard in which the archives are kept. An inscription sometimes indicates its function. The term is often used to refer to the archives of a church, confraternity, or a town."@en ;
  rdfs:comment "Kasten waarin men archieven bewaart. Soms geeft een opschrift aan wat de functie is. De term wordt vaak gebruikt met betrekking tot archieven van een kerk, broederschap of gemeente."@nl ;
  rdfs:isDefinedBy <https://w3id.org/con-tax/components/aat-furn> ;
  rdfs:label "archiefkast"@nl ;
  rdfs:label "archiefkasten"@nl ;
  rdfs:label "archives cupboards"@en ;
  rdfs:seeAlso <http://vocab.getty.edu/aat/300298887> ;
  rdfs:subClassOf <https://w3id.org/con-tax/components/aat-furn#300039183> ;
.
<https://w3id.org/con-tax/components/aat-furn#300298924>
  rdf:type owl:Class ;
  rdfs:comment "Arrangements of hooks or pegs attached directly to the wall or to a plank or other piece which is mounted on the wall, for hanging coats, hats, and other clothes."@en ;
  rdfs:comment "Haken die men direct aan de muur bevestigt, of aan een plank of een ander voorwerp aan de muur, om jassen, hoeden of andere kledingstukken op te hangen. "@nl ;
  rdfs:isDefinedBy <https://w3id.org/con-tax/components/aat-furn> ;
  rdfs:label "wall hooks (clothing)"@en ;
  rdfs:label "wandhaak"@nl ;
  rdfs:label "wandhaken (kleding)"@nl ;
  rdfs:label "wandhaken"@nl ;
  rdfs:seeAlso <http://vocab.getty.edu/aat/300298924> ;
  rdfs:subClassOf <https://w3id.org/con-tax/components/aat-furn#300039337> ;
.
<https://w3id.org/con-tax/components/aat-furn#300298926>
  rdf:type owl:Class ;
  rdfs:comment "Planken met een rij haken aan de onderkant waaraan men hoeden, kledingstukken, paraplu's of andere objecten kan ophangen."@nl ;
  rdfs:comment "Shelves designed with a row of hooks or pegs beneath, for the hanging of hats, clothing, umbrellas, or other items."@en ;
  rdfs:isDefinedBy <https://w3id.org/con-tax/components/aat-furn> ;
  rdfs:label "plank met haken"@nl ;
  rdfs:label "planken met haken (kledingrek)"@nl ;
  rdfs:label "planken met haken"@nl ;
  rdfs:label "shelves with hooks (clothing rack)"@en ;
  rdfs:seeAlso <http://vocab.getty.edu/aat/300298926> ;
  rdfs:subClassOf <https://w3id.org/con-tax/components/aat-furn#300039337> ;
.
<https://w3id.org/con-tax/components/aat-furn#300298927>
  rdf:type owl:Class ;
  rdfs:comment "Rods secured horizontally, usually in closets or armoires, for the purpose of hanging clothes on clothes hangers. They may be removable or permanent fixtures."@en ;
  rdfs:comment "Stangen die horizontaal hangen, gewoonlijk in (kleren)kasten, waaraan men klerenhangers met kledingstukken kan ophangen. Ze kunnen vast zitten of verwijderbaar zijn."@nl ;
  rdfs:isDefinedBy <https://w3id.org/con-tax/components/aat-furn> ;
  rdfs:label "clothing rods"@en ;
  rdfs:label "kledingstang"@nl ;
  rdfs:label "kledingstangen"@nl ;
  rdfs:seeAlso <http://vocab.getty.edu/aat/300298927> ;
  rdfs:subClassOf <https://w3id.org/con-tax/components/aat-furn#300039337> ;
.
<https://w3id.org/con-tax/components/aat-furn#300298949>
  rdf:type owl:Class ;
  rdfs:comment """Hoge staande lessenaar 
die werd gebruikt voor monumentale boekwerken. Vaak in de vorm van een vogel met een boekensteun op de rug. De vogels die het meest uitgebeeld worden zijn de adelaar, de pelikaan en de zwaan. In Nederland worden de termen arend-lezenaar en lutrijn ook wel gebruikt voor de oude exemplaren."""@nl ;
  rdfs:comment "Large elevated lecterns that may be pivoted, usually found in the choir of churches."@en ;
  rdfs:isDefinedBy <https://w3id.org/con-tax/components/aat-furn> ;
  rdfs:label "badalones"@en ;
  rdfs:label "koorlessenaar"@nl ;
  rdfs:label "koorlessenaren"@nl ;
  rdfs:seeAlso <http://vocab.getty.edu/aat/300298949> ;
  rdfs:subClassOf <https://w3id.org/con-tax/components/aat-furn#300170801> ;
.
<https://w3id.org/con-tax/components/aat-furn#300298974>
  rdf:type owl:Class ;
  rdfs:comment "Banken die in klaslokalen staan met schrijftafels, die meestal aan de banken vastzitten, bedoeld voor twee of meer leerlingen. "@nl ;
  rdfs:comment "Benches with desks, usually attached, designed for the seating of two or more students in a class room."@en ;
  rdfs:isDefinedBy <https://w3id.org/con-tax/components/aat-furn> ;
  rdfs:label "school benches"@en ;
  rdfs:label "schoolbank"@nl ;
  rdfs:label "schoolbanken"@nl ;
  rdfs:seeAlso <http://vocab.getty.edu/aat/300298974> ;
  rdfs:subClassOf <https://w3id.org/con-tax/components/aat-furn#300038494> ;
.
<https://w3id.org/con-tax/components/aat-furn#300298975>
  rdf:type owl:Class ;
  rdfs:comment "Bank-achtige meubels voor het gebruik door een persoon in gebed, bestaande uit een bidbank met een smalle opstaande voorkant met daarboven een lessenaar voor boeken of om de ellebogen te rusten en vaak een plankje daaronder om boeken te bergen. Voor soortgelijke meubels die in de vorm van een lage stoel, gebruik 'prie-dieu chairs'."@nl ;
  rdfs:comment "Bench-like pieces of furniture for the use of a person at prayer, consisting of a kneeler with a narrow upright front surmounted by a ledge for books or for resting the elbows, and often a shelf below this for storing books. For similar pieces that are in the form of a low chair, use \"prie-dieu chairs.\""@en ;
  rdfs:isDefinedBy <https://w3id.org/con-tax/components/aat-furn> ;
  rdfs:label "knielbank"@nl ;
  rdfs:label "knielbanken"@nl ;
  rdfs:label "prie-dieus (benches)"@en ;
  rdfs:seeAlso <http://vocab.getty.edu/aat/300298975> ;
  rdfs:subClassOf <https://w3id.org/con-tax/components/aat-furn#300038494> ;
  rdfs:subClassOf <https://w3id.org/con-tax/components/aat-furn#300137869> ;
.
<https://w3id.org/con-tax/components/aat-furn#300299277>
  rdf:type owl:Class ;
  rdfs:comment "Cabinets for storing wine, usually located near the dining table, having four or more openings for bottles, often with ice to cool the wine. The type is particularly well known in Tuscany."@en ;
  rdfs:isDefinedBy <https://w3id.org/con-tax/components/aat-furn> ;
  rdfs:label "cantinettas"@en ;
  rdfs:seeAlso <http://vocab.getty.edu/aat/300299277> ;
  rdfs:subClassOf <https://w3id.org/con-tax/components/aat-furn#300391454> ;
  rdfs:subClassOf <https://w3id.org/con-tax/components/aat-furn#300433219> ;
.
<https://w3id.org/con-tax/components/aat-furn#300299344>
  rdf:type owl:Class ;
  rdfs:comment "General term for rectangular chests used in homes, probably one of the earliest types of home furnishings; in the chest could be stored various items, and it could be used for seating or as a bed as well. For relatively ornate versions of chests, particularly as used in Florentine homes, prefer \"cassoni.\""@en ;
  rdfs:isDefinedBy <https://w3id.org/con-tax/components/aat-furn> ;
  rdfs:label "casse (chests)"@it ;
  rdfs:seeAlso <http://vocab.getty.edu/aat/300299344> ;
  rdfs:subClassOf <https://w3id.org/con-tax/components/aat-furn#300038992> ;
.
<https://w3id.org/con-tax/components/aat-furn#300299372>
  rdf:type owl:Class ;
  rdfs:comment "Cassoni that serve as wedding chests, often coming with the bride to her new home and decorated with images related to marriage and fertility."@en ;
  rdfs:isDefinedBy <https://w3id.org/con-tax/components/aat-furn> ;
  rdfs:label "cassoni nuziali"@en ;
  rdfs:seeAlso <http://vocab.getty.edu/aat/300299372> ;
  rdfs:subClassOf <https://w3id.org/con-tax/components/aat-furn#300039007> ;
.
<https://w3id.org/con-tax/components/aat-furn#300300293>
  rdf:type owl:Class ;
  rdfs:comment "Inclined, sometimes foldable supports, made of wood or metal, on which a missal or other liturgical book is placed on the altar. "@en ;
  rdfs:comment "Schuinopstaande, soms vouwbare, boekenstandaard. Bestemd voor op het altaar en gemaakt van hout of metaal, bedoeld voor het missaal of ander liturgisch boek"@nl ;
  rdfs:isDefinedBy <https://w3id.org/con-tax/components/aat-furn> ;
  rdfs:label "altaarlessenaar"@nl ;
  rdfs:label "altaarlessenaars"@nl ;
  rdfs:label "altaarlezenaar"@nl ;
  rdfs:label "altaarlezenaars"@nl ;
  rdfs:label "missal stands"@en ;
  rdfs:seeAlso <http://vocab.getty.edu/aat/300300293> ;
  rdfs:subClassOf <https://w3id.org/con-tax/components/aat-furn#300039790> ;
.
<https://w3id.org/con-tax/components/aat-furn#300301349>
  rdf:type owl:Class ;
  rdfs:comment "General term for tables of small size or certain types of stands."@en ;
  rdfs:isDefinedBy <https://w3id.org/con-tax/components/aat-furn> ;
  rdfs:label "small tables"@en ;
  rdfs:seeAlso <http://vocab.getty.edu/aat/300301349> ;
  rdfs:subClassOf <https://w3id.org/con-tax/components/aat-furn#300039548> ;
.
<https://w3id.org/con-tax/components/aat-furn#300301373>
  rdf:type owl:Class ;
  rdfs:comment "Chests or tables of various designs used in kitchens or bakeries, having storage areas and a working surface. Used for the storage of flour, making of bread on the table top, and often for the storage of bread. For smaller, counter-top containers used to store bread, use \"bread boxes.\""@en ;
  rdfs:isDefinedBy <https://w3id.org/con-tax/components/aat-furn> ;
  rdfs:label "bread chests (working tables)"@en ;
  rdfs:seeAlso <http://vocab.getty.edu/aat/300301373> ;
  rdfs:subClassOf <https://w3id.org/con-tax/components/aat-furn#300438650> ;
.
<https://w3id.org/con-tax/components/aat-furn#300310116>
  rdf:type owl:Class ;
  rdfs:comment "Een standaard voor kommen, bijvoorbeeld voor Romeinse kraters of Chinese kommen van brons die men voor rituelen."@nl ;
  rdfs:comment "Refers generally to objects designed specifically to support vessels such as Roman kraters or Chinese bronze ritual vessels."@en ;
  rdfs:isDefinedBy <https://w3id.org/con-tax/components/aat-furn> ;
  rdfs:label "vessel stands"@en ;
  rdfs:label "vessel stands"@nl ;
  rdfs:seeAlso <http://vocab.getty.edu/aat/300310116> ;
  rdfs:subClassOf <https://w3id.org/con-tax/components/aat-furn#300039767> ;
.
<https://w3id.org/con-tax/components/aat-furn#300310149>
  rdf:type owl:Class ;
  rdfs:comment "Kleine meubels waarin men de heilige oliën bewaart en die in een muur zijn ingebouwd of daaraan zijn bevestigd, dicht bij het altaar, in de doopkapel of in de sacristie. Op de deur, die men op slot moet houden, staan soms de woorden ���Olea Sancta'."@nl ;
  rdfs:comment "Small pieces of storage furniture built into or hung on a wall near the main altar, in the baptistery, or in the sacristy to contain the holy oils. The door, which must be kept locked, sometimes bears the words \"Olea Sancta.\""@en ;
  rdfs:isDefinedBy <https://w3id.org/con-tax/components/aat-furn> ;
  rdfs:label "holy oils aumbries"@en ;
  rdfs:label "holy oils aumbries"@nl ;
  rdfs:seeAlso <http://vocab.getty.edu/aat/300310149> ;
  rdfs:subClassOf <https://w3id.org/con-tax/components/aat-furn#300039221> ;
.
<https://w3id.org/con-tax/components/aat-furn#300310517>
  rdf:type owl:Class ;
  rdfs:comment "Stevige stoelen met een hoge rugleuning en solide armleuningen die in Romeinse huizen en publieke ruimtes werden gebruikt of stoelen met dezelfde vorm. De zitting was verhoogd, waardoor een voetenbank nodig was. Soliums stonden in het atrium en werden gebruikt door de heer des huizes wanneer hij gasten of klanten ontving. Goden en koningen worden in de kunst vaak zittend in dergelijke stoelen afgebeeld."@nl ;
  rdfs:comment "Stiff, straight, high-backed chairs with solid arms used in Roman homes and public spaces; also, any chair that has the same form. The seat was placed high, requiring a footstool. In a Roman home, it was kept in the atrium for the use of the master of the house when he received guests or clients. Gods and kings in art may be represented as seated in such a chair."@en ;
  rdfs:isDefinedBy <https://w3id.org/con-tax/components/aat-furn> ;
  rdfs:label "soliums"@en ;
  rdfs:label "soliums"@nl ;
  rdfs:seeAlso <http://vocab.getty.edu/aat/300310517> ;
  rdfs:subClassOf <https://w3id.org/con-tax/components/aat-furn#300133851> ;
.
<https://w3id.org/con-tax/components/aat-furn#300310519>
  rdf:type owl:Class ;
  rdfs:comment "Dry sinks surmounted by an enclosed cupboard or open shelves."@en ;
  rdfs:comment "Een 'dry sink' met een gesloten kast of open planken erboven."@nl ;
  rdfs:isDefinedBy <https://w3id.org/con-tax/components/aat-furn> ;
  rdfs:label "dry sink hutches"@en ;
  rdfs:label "dry sink hutches"@nl ;
  rdfs:seeAlso <http://vocab.getty.edu/aat/300310519> ;
  rdfs:subClassOf <https://w3id.org/con-tax/components/aat-furn#300121381> ;
  rdfs:subClassOf <https://w3id.org/con-tax/components/aat-furn#300266737> ;
.
<https://w3id.org/con-tax/components/aat-furn#300310713>
  rdf:type owl:Class ;
  rdfs:comment "Built-in staggered, asymmetrical shelves commonly found in shoin style decoration. This style first because popular at the end of the Muromachi period (1392-1573)."@en ;
  rdfs:comment "Ingebouwde asymmetrische en verspringende planken die men vaak tegenkomt in huizen die zijn ingericht in de shoin-stijl. Deze stijl werd populair aan het eind van de Muromachi-periode (1392-1573). "@nl ;
  rdfs:isDefinedBy <https://w3id.org/con-tax/components/aat-furn> ;
  rdfs:label "chigaidana"@en ;
  rdfs:label "chigaidana"@nl ;
  rdfs:seeAlso <http://vocab.getty.edu/aat/300310713> ;
  rdfs:subClassOf <https://w3id.org/con-tax/components/aat-furn#300037680> ;
.
<https://w3id.org/con-tax/components/aat-furn#300311735>
  rdf:type owl:Class ;
  rdfs:comment "Devices used to hold a camera and secure the printed material or other item to be photographed."@en ;
  rdfs:isDefinedBy <https://w3id.org/con-tax/components/aat-furn> ;
  rdfs:label "copy stands"@en ;
  rdfs:label "fotoreproductie-opstelling"@nl ;
  rdfs:label "fotoreproductie-opstellingen"@nl ;
  rdfs:seeAlso <http://vocab.getty.edu/aat/300311735> ;
  rdfs:subClassOf <https://w3id.org/con-tax/components/aat-furn#300039767> ;
.
<https://w3id.org/con-tax/components/aat-furn#300311855>
  rdf:type owl:Class ;
  rdfs:comment "Tables incorporating a translucent screen illuminated from underneath, for tracing, viewing slides, and other activities."@en ;
  rdfs:isDefinedBy <https://w3id.org/con-tax/components/aat-furn> ;
  rdfs:label "lichtbak (tafel naar functie)"@nl ;
  rdfs:label "lichtbak"@nl ;
  rdfs:label "lichtbakken (tafels naar functie)"@nl ;
  rdfs:label "lichtbakken"@nl ;
  rdfs:label "lichttafel (tafel naar functie)"@nl ;
  rdfs:label "lichttafel"@nl ;
  rdfs:label "lichttafels"@nl ;
  rdfs:label "light tables"@en ;
  rdfs:seeAlso <http://vocab.getty.edu/aat/300311855> ;
  rdfs:subClassOf <https://w3id.org/con-tax/components/aat-furn#300039548> ;
.
<https://w3id.org/con-tax/components/aat-furn#300312264>
  rdf:type owl:Class ;
  rdfs:comment "De term stamt af van het Latijnse woord voor ���stoel' of ���zitting' en wordt gebruikt voor zware Romeinse stoelen die waren afgeleid van klismos-stoelen, die door de oude Grieken waren ontwikkeld en lichter en subtieler waren. Gebruik ���katheders (bisschopstronen)' voor stoelen in christelijke kathedralen die bisschoppen gebruikten."@nl ;
  rdfs:comment "From the Latin for \"chairs\" or \"seats,\" refers to ancient Roman chairs of heavy structure that were derived from the klismos, which is a lighter, more delicate chair developed by the ancient Greeks. For chairs used by bishops in Christian cathedrals, use \"cathedrae (bishop's chairs).\""@en ;
  rdfs:isDefinedBy <https://w3id.org/con-tax/components/aat-furn> ;
  rdfs:label "cathedrae (Roman chairs)"@en ;
  rdfs:label "katheder"@nl ;
  rdfs:label "katheders (Romeinse stoelen)"@nl ;
  rdfs:label "katheders"@nl ;
  rdfs:label "katheders; katheder; leerstoelen; leerstoel"@nl ;
  rdfs:seeAlso <http://vocab.getty.edu/aat/300312264> ;
  rdfs:subClassOf <https://w3id.org/con-tax/components/aat-furn#300037772> ;
.
<https://w3id.org/con-tax/components/aat-furn#300375158>
  rdf:type owl:Class ;
  rdfs:comment "Padded tables for massage, chiropractic treatment, or other body work."@en ;
  rdfs:isDefinedBy <https://w3id.org/con-tax/components/aat-furn> ;
  rdfs:label "massage tables"@en ;
  rdfs:seeAlso <http://vocab.getty.edu/aat/300375158> ;
  rdfs:seeAlso wd:Q6784507 ;
  rdfs:subClassOf <https://w3id.org/con-tax/components/aat-furn#300037680> ;
.
<https://w3id.org/con-tax/components/aat-furn#300375159>
  rdf:type owl:Class ;
  rdfs:comment "Cabinets used to house various data storage media formats. May also refer to cabinets that house and sometimes conceal multimedia support equipment."@en ;
  rdfs:isDefinedBy <https://w3id.org/con-tax/components/aat-furn> ;
  rdfs:label "media cabinets"@en ;
  rdfs:seeAlso <http://vocab.getty.edu/aat/300375159> ;
  rdfs:subClassOf <https://w3id.org/con-tax/components/aat-furn#300038888> ;
.
<https://w3id.org/con-tax/components/aat-furn#300375160>
  rdf:type owl:Class ;
  rdfs:comment "Furniture cabinets meant to hold and enclose television sets, presenting aesthetically pleasing screen views while hiding functional componets. For use in the home."@en ;
  rdfs:isDefinedBy <https://w3id.org/con-tax/components/aat-furn> ;
  rdfs:label "television cabinets"@en ;
  rdfs:seeAlso <http://vocab.getty.edu/aat/300375160> ;
  rdfs:subClassOf <https://w3id.org/con-tax/components/aat-furn#300038888> ;
.
<https://w3id.org/con-tax/components/aat-furn#300375198>
  rdf:type owl:Class ;
  rdfs:comment "Raised platforms or similar work surfaces situated in the middle of a room, especially a kitchen, permitting access from all sides."@en ;
  rdfs:isDefinedBy <https://w3id.org/con-tax/components/aat-furn> ;
  rdfs:label "islands (storage furniture)"@en ;
  rdfs:seeAlso <http://vocab.getty.edu/aat/300375198> ;
  rdfs:subClassOf <https://w3id.org/con-tax/components/aat-furn#300037680> ;
.
<https://w3id.org/con-tax/components/aat-furn#300375207>
  rdf:type owl:Class ;
  rdfs:comment "Stands used to hold or support typewriters."@en ;
  rdfs:isDefinedBy <https://w3id.org/con-tax/components/aat-furn> ;
  rdfs:label "typewriter stands"@en ;
  rdfs:seeAlso <http://vocab.getty.edu/aat/300375207> ;
  rdfs:subClassOf <https://w3id.org/con-tax/components/aat-furn#300039767> ;
.
<https://w3id.org/con-tax/components/aat-furn#300375208>
  rdf:type owl:Class ;
  rdfs:comment "Tables used for the activity of knitting, typically outfitted with drawers or cubbyholes to hold wool or other supplies."@en ;
  rdfs:isDefinedBy <https://w3id.org/con-tax/components/aat-furn> ;
  rdfs:label "knitting tables"@en ;
  rdfs:seeAlso <http://vocab.getty.edu/aat/300375208> ;
  rdfs:subClassOf <https://w3id.org/con-tax/components/aat-furn#300039548> ;
.
<https://w3id.org/con-tax/components/aat-furn#300375209>
  rdf:type owl:Class ;
  rdfs:comment "High chests of deep drawers used for keeping priest's vestments, often with a table so that the garments can be laid out, and a mirror so that the priests can see that they are properly attired."@en ;
  rdfs:isDefinedBy <https://w3id.org/con-tax/components/aat-furn> ;
  rdfs:label "vesting tables"@en ;
  rdfs:seeAlso <http://vocab.getty.edu/aat/300375209> ;
  rdfs:subClassOf <https://w3id.org/con-tax/components/aat-furn#300037680> ;
.
<https://w3id.org/con-tax/components/aat-furn#300375220>
  rdf:type owl:Class ;
  rdfs:comment "Portable enclosures in which young children can play safely alone."@en ;
  rdfs:isDefinedBy <https://w3id.org/con-tax/components/aat-furn> ;
  rdfs:label "playpens"@en ;
  rdfs:seeAlso <http://vocab.getty.edu/aat/300375220> ;
  rdfs:subClassOf <https://w3id.org/con-tax/components/aat-furn#300256336> ;
  rdfs:subClassOf <https://w3id.org/con-tax/components/aat-furn#300266715> ;
.
<https://w3id.org/con-tax/components/aat-furn#300375232>
  rdf:type owl:Class ;
  rdfs:comment "Racks for storing and/or displaying magazines. "@en ;
  rdfs:isDefinedBy <https://w3id.org/con-tax/components/aat-furn> ;
  rdfs:label "magazine racks"@en ;
  rdfs:seeAlso <http://vocab.getty.edu/aat/300375232> ;
  rdfs:subClassOf <https://w3id.org/con-tax/components/aat-furn#300039337> ;
.
<https://w3id.org/con-tax/components/aat-furn#300375233>
  rdf:type owl:Class ;
  rdfs:comment "Racks for storing and/or displaying newspapers."@en ;
  rdfs:isDefinedBy <https://w3id.org/con-tax/components/aat-furn> ;
  rdfs:label "newspaper racks"@en ;
  rdfs:seeAlso <http://vocab.getty.edu/aat/300375233> ;
  rdfs:subClassOf <https://w3id.org/con-tax/components/aat-furn#300039337> ;
.
<https://w3id.org/con-tax/components/aat-furn#300375246>
  rdf:type owl:Class ;
  rdfs:comment "Stands or racks for holding boots. Some include a drip tray for drying wet boots."@en ;
  rdfs:isDefinedBy <https://w3id.org/con-tax/components/aat-furn> ;
  rdfs:label "boot racks"@en ;
  rdfs:seeAlso <http://vocab.getty.edu/aat/300375246> ;
  rdfs:subClassOf <https://w3id.org/con-tax/components/aat-furn#300039337> ;
.
<https://w3id.org/con-tax/components/aat-furn#300375247>
  rdf:type owl:Class ;
  rdfs:comment "Wall mounted racks for hanging keys."@en ;
  rdfs:isDefinedBy <https://w3id.org/con-tax/components/aat-furn> ;
  rdfs:label "key racks"@en ;
  rdfs:seeAlso <http://vocab.getty.edu/aat/300375247> ;
  rdfs:subClassOf <https://w3id.org/con-tax/components/aat-furn#300039337> ;
.
<https://w3id.org/con-tax/components/aat-furn#300375544>
  rdf:type owl:Class ;
  rdfs:comment "Banken met een verhoogd hoofdeinde en verschillende soorten poten, in het oude Griekenland voornamelijk gebruikt om op te slapen of te eten, maar ook om doden op te baren in hun tombes of voor rouwrituelen. De vroegste afbeeldingen van klinai vindt men in begrafenistaferelen op geometrische vazen. "@nl ;
  rdfs:comment "Couches having raised head ends and various distinctive styles of legs, used in ancient Greece chiefly for sleeping and dining but also for laying out the dead during ritual mourning and in their tombs. The earliest depictions are in funerary scenes on Geometric vases."@en ;
  rdfs:isDefinedBy <https://w3id.org/con-tax/components/aat-furn> ;
  rdfs:label "klinai"@en ;
  rdfs:label "klinai"@nl ;
  rdfs:seeAlso <http://vocab.getty.edu/aat/300375544> ;
  rdfs:seeAlso wd:Q922892 ;
  rdfs:subClassOf <https://w3id.org/con-tax/components/aat-furn#300038583> ;
.
<https://w3id.org/con-tax/components/aat-furn#300375669>
  rdf:type owl:Class ;
  rdfs:comment "In Jewish tradition, wooden coffers containing the Tables of the Law, kept in the holiest place of the synagogue."@en ;
  rdfs:comment "In de Joodse traditie houten kisten die de tafelen der wet bevatten. Men bewaarde ze op de heiligste plaats van de tabernakel."@nl ;
  rdfs:isDefinedBy <https://w3id.org/con-tax/components/aat-furn> ;
  rdfs:label "Torah shrines"@en ;
  rdfs:label "Torah shrines"@nl ;
  rdfs:seeAlso <http://vocab.getty.edu/aat/300375669> ;
  rdfs:subClassOf <https://w3id.org/con-tax/components/aat-furn#300139717> ;
.
<https://w3id.org/con-tax/components/aat-furn#300375670>
  rdf:type owl:Class ;
  rdfs:comment "Seats for several people, having a storage chest below and a high back and arms. Examples include benches in the sacristy of a church."@en ;
  rdfs:comment "Zitmeubels voor meerdere mensen met een opbergkist eronder en hoge rug- en armleuningen, bijvoorbeeld de banken in de sacristie van een kerk."@nl ;
  rdfs:isDefinedBy <https://w3id.org/con-tax/components/aat-furn> ;
  rdfs:label "arcibanchi"@en ;
  rdfs:label "arcibanchi"@nl ;
  rdfs:seeAlso <http://vocab.getty.edu/aat/300375670> ;
  rdfs:seeAlso wd:Q21550368 ;
  rdfs:subClassOf <https://w3id.org/con-tax/components/aat-furn#300038507> ;
  rdfs:subClassOf <https://w3id.org/con-tax/components/aat-furn#300038521> ;
.
<https://w3id.org/con-tax/components/aat-furn#300375673>
  rdf:type owl:Class ;
  rdfs:comment "Devices incorporating a rack or tray and often a seat and hanger, designed for holding clothing and personal effects. Generally placed in a dressing room or bedroom, and intended for gentlemen's clothing rather than ladies'."@en ;
  rdfs:comment "Meubels met een rek of plateau en vaak een stoel en hanger, bedoeld voor kledingstukken en persoonlijke eigendommen. Gewoonlijk staan ze in kleed- of slaapkamers en gebruikte men ze voor herenkleding."@nl ;
  rdfs:isDefinedBy <https://w3id.org/con-tax/components/aat-furn> ;
  rdfs:label "clothing valets"@en ;
  rdfs:label "dressboy"@nl ;
  rdfs:label "dressboys"@nl ;
  rdfs:seeAlso <http://vocab.getty.edu/aat/300375673> ;
  rdfs:subClassOf <https://w3id.org/con-tax/components/aat-furn#300039767> ;
.
<https://w3id.org/con-tax/components/aat-furn#300375675>
  rdf:type owl:Class ;
  rdfs:comment "Standaards, gewoonlijk van hout of metaal, met haken aan de bovenkant waaraan men jassen, hoeden of andere kledingstukken kan ophangen."@nl ;
  rdfs:comment "Upright postlike stands, usually of wood or metal, having pegs or hooks around the top from which to hang coats, hats, or other clothing."@en ;
  rdfs:isDefinedBy <https://w3id.org/con-tax/components/aat-furn> ;
  rdfs:label "coat trees"@en ;
  rdfs:label "staande kapstok"@nl ;
  rdfs:label "staande kapstokken"@nl ;
  rdfs:seeAlso <http://vocab.getty.edu/aat/300375675> ;
  rdfs:subClassOf <https://w3id.org/con-tax/components/aat-furn#300039767> ;
.
<https://w3id.org/con-tax/components/aat-furn#300375689>
  rdf:type owl:Class ;
  rdfs:comment "Tables on which monetary calculations were made using tokens or counters on a checkered background, similar in usage to an abacus. Often having a compartment beneath for money, tokens, and goods."@en ;
  rdfs:comment "Tafels waarop men financiële berekeningen maakte met behulp van fiches of muntjes op een geblokte ondergrond, in gebruik te vergelijken met een telraam. Vaak voorzien van een gedeelte onder het blad bestemd voor geld, fiches en andere voorwerpen."@nl ;
  rdfs:isDefinedBy <https://w3id.org/con-tax/components/aat-furn> ;
  rdfs:label "counter tables"@en ;
  rdfs:label "counter tables"@nl ;
  rdfs:seeAlso <http://vocab.getty.edu/aat/300375689> ;
  rdfs:seeAlso wd:Q21550499 ;
  rdfs:subClassOf <https://w3id.org/con-tax/components/aat-furn#300039548> ;
.
<https://w3id.org/con-tax/components/aat-furn#300375694>
  rdf:type owl:Class ;
  rdfs:comment "Banken met een plankje waarop men een boek kan leggen, zodat men het kan lezen als men achterover zit."@nl ;
  rdfs:comment "Sofas with an attached platform upon which to rest a book, for the purpose of reading in a reclining position."@en ;
  rdfs:isDefinedBy <https://w3id.org/con-tax/components/aat-furn> ;
  rdfs:label "reading sofas"@en ;
  rdfs:label "reading sofas"@nl ;
  rdfs:seeAlso <http://vocab.getty.edu/aat/300375694> ;
  rdfs:subClassOf <https://w3id.org/con-tax/components/aat-furn#300038634> ;
.
<https://w3id.org/con-tax/components/aat-furn#300375697>
  rdf:type owl:Class ;
  rdfs:comment "Chairs having a triangular seat and three turned legs, popular in 17th-century America and Britain. The seat may be upholstered. The type is heavily inspired by Late Gothic and Early Renaissance three-cornered chairs of continental Europe."@en ;
  rdfs:comment "Stoelen met een driehoekige zitting en drie gedraaide poten, populair in de zeventiende eeuw in Amerika en Groot-Brittannië. De zitting is soms gestoffeerd. Dit type stoel is in hoge mate geïnspireerd op de driehoekige stoelen die in de late gotiek en vroege Renaissance populair waren op het Europese vasteland."@nl ;
  rdfs:isDefinedBy <https://w3id.org/con-tax/components/aat-furn> ;
  rdfs:label "Harvard chairs"@en ;
  rdfs:label "Harvard chairs"@nl ;
  rdfs:seeAlso <http://vocab.getty.edu/aat/300375697> ;
  rdfs:subClassOf <https://w3id.org/con-tax/components/aat-furn#300037776> ;
.
<https://w3id.org/con-tax/components/aat-furn#300375698>
  rdf:type owl:Class ;
  rdfs:comment "Armchairs designed to sit in a corner, having a back continuing around two sides of the seat and over three legs, with the fourth leg placed under the middle front of the seat. The back is typically rounded, and the occupant may sit facing forward, or to either side. The form was popular in 18th-century Britain, Europe, and North America."@en ;
  rdfs:comment "Leunstoelen die zijn bedoeld voor hoeken in kamers, met vier poten en een doorlopende rugleuning aan twee aanliggende zijden. Gewoonlijk heeft de rugleuning een ronde vorm, en de persoon op de stoel kan met het gezicht naar voren of naar een van de twee zijkanten zitten. Dit soort stoelen was in de achttiende eeuw populair in Europa en Noord-Amerika. "@nl ;
  rdfs:isDefinedBy <https://w3id.org/con-tax/components/aat-furn> ;
  rdfs:label "corner chairs"@en ;
  rdfs:label "hoekstoel"@nl ;
  rdfs:label "hoekstoelen"@nl ;
  rdfs:seeAlso <http://vocab.getty.edu/aat/300375698> ;
  rdfs:subClassOf <https://w3id.org/con-tax/components/aat-furn#300037776> ;
.
<https://w3id.org/con-tax/components/aat-furn#300375699>
  rdf:type owl:Class ;
  rdfs:comment "Tables having a single slab as a top surface, usually having a slab of stone, typically marble or slate but also granite or another type of stone, or of concrete or heavy wood. The slab is set upon a plinth or frame, usually of stone, wood, or metal. The slab top is not enclosed or encased in a supporting structure. For 18th-century tables having a marble top, use the more specific \"marble slab tables.\""@en ;
  rdfs:comment "Tafels met één plaat als blad, gewoonlijk van steen, doorgaans marmer of leisteen, maar soms van graniet of een andere steensoort, of van beton of zwaar hout. De plaat steunt op een onderstel, gewoonlijk van steen, hout of metaal, maar vormt daarmee geen onlosmakelijke eenheid. Voor tafels uit de achttiende eeuw met marmeren bladen, gebruikt men de specifiekere term ���marble slab tables'."@nl ;
  rdfs:isDefinedBy <https://w3id.org/con-tax/components/aat-furn> ;
  rdfs:label "slab tables (algemeen)"@nl ;
  rdfs:label "slab tables (general)"@en ;
  rdfs:label "slab tables"@nl ;
  rdfs:seeAlso <http://vocab.getty.edu/aat/300375699> ;
  rdfs:subClassOf <https://w3id.org/con-tax/components/aat-furn#300039548> ;
.
<https://w3id.org/con-tax/components/aat-furn#300375700>
  rdf:type owl:Class ;
  rdfs:comment "Standaard bedoeld voor een zeer groot woordenboek"@nl ;
  rdfs:comment "Stands or bookrests designed to hold a very large dictionary."@en ;
  rdfs:isDefinedBy <https://w3id.org/con-tax/components/aat-furn> ;
  rdfs:label "dictionary stands"@en ;
  rdfs:label "woordenboekenstandaard"@nl ;
  rdfs:label "woordenboekenstandaarden"@nl ;
  rdfs:seeAlso <http://vocab.getty.edu/aat/300375700> ;
  rdfs:subClassOf <https://w3id.org/con-tax/components/aat-furn#300039790> ;
.
<https://w3id.org/con-tax/components/aat-furn#300379857>
  rdf:type owl:Class ;
  rdfs:comment "Lidded boxes, often decorated, that were placed on the dressing table and contained pins, ribbons, feathers, and other adornments for dressing; they may also contain separate lidded cosmetic canisters. Often used for a lady's toilette, although men used them as well. "@en ;
  rdfs:isDefinedBy <https://w3id.org/con-tax/components/aat-furn> ;
  rdfs:label "toilet caskets"@en ;
  rdfs:seeAlso <http://vocab.getty.edu/aat/300379857> ;
  rdfs:subClassOf <https://w3id.org/con-tax/components/aat-furn#300039006> ;
.
<https://w3id.org/con-tax/components/aat-furn#300379868>
  rdf:type owl:Class ;
  rdfs:comment "Large wooden cabinets having subdivisions, drawers, shelves, and usually doors or a fall front, designed particularly for housing rare, precious, or interesting items. For small, private chambers designed for this purpose, use \"cabinets of curiosities.\""@en ;
  rdfs:isDefinedBy <https://w3id.org/con-tax/components/aat-furn> ;
  rdfs:label "display cabinets"@en ;
  rdfs:seeAlso <http://vocab.getty.edu/aat/300379868> ;
  rdfs:seeAlso wd:Q3561331 ;
  rdfs:subClassOf <https://w3id.org/con-tax/components/aat-furn#300038860> ;
  rdfs:subClassOf <https://w3id.org/con-tax/components/aat-furn#300077356> ;
.
<https://w3id.org/con-tax/components/aat-furn#300379887>
  rdf:type owl:Class ;
  rdfs:comment "A surface designed for relining of oil paintings patented by art restorer George T. Oliver in 1937. Instead of ironing a new canvas onto the old one, the most practiced method to date, this technique bonds the two canvases, which have been coated with a molten adhesive, on a hot metal plate. A pump evacuates oxygen between the canvases and adhesion occurs upon cooling."@en ;
  rdfs:isDefinedBy <https://w3id.org/con-tax/components/aat-furn> ;
  rdfs:label "vacuum hot tables"@en ;
  rdfs:seeAlso <http://vocab.getty.edu/aat/300379887> ;
  rdfs:subClassOf <https://w3id.org/con-tax/components/aat-furn#300391286> ;
.
<https://w3id.org/con-tax/components/aat-furn#300390973>
  rdf:type owl:Class ;
  rdfs:comment "Standaarden of rekken om collectezakken of andere houders voor het ophalen van de collecte te bewaren."@nl ;
  rdfs:comment "Stands or racks designed to store collection bags or other receptacles that are used to gather offertory gifts in churches."@en ;
  rdfs:isDefinedBy <https://w3id.org/con-tax/components/aat-furn> ;
  rdfs:label "collectestokkenrekken"@nl ;
  rdfs:label "collectezakkenrek"@nl ;
  rdfs:label "collectezakkenrekken"@nl ;
  rdfs:label "collectezakkenstandaard"@nl ;
  rdfs:label "collectezakkenstandaarden"@nl ;
  rdfs:label "offertory bag stands"@en ;
  rdfs:label "ponkhouders"@nl ;
  rdfs:seeAlso <http://vocab.getty.edu/aat/300390973> ;
  rdfs:subClassOf <https://w3id.org/con-tax/components/aat-furn#300039767> ;
.
<https://w3id.org/con-tax/components/aat-furn#300390991>
  rdf:type owl:Class ;
  rdfs:comment "Cabinets of relics that are divided into days, weeks, and months with relics of a saint, martyr, deity, or other holy person mounted or displayed within."@en ;
  rdfs:comment "Kast met een indeling in dagen, weken en maanden, waarin voor iedere dag van het jaar een theca (reliekoog)"@nl ;
  rdfs:isDefinedBy <https://w3id.org/con-tax/components/aat-furn> ;
  rdfs:label "calendars of relics"@en ;
  rdfs:label "reliekenkalender"@nl ;
  rdfs:label "reliekenkalenders"@nl ;
  rdfs:seeAlso <http://vocab.getty.edu/aat/300390991> ;
  rdfs:subClassOf <https://w3id.org/con-tax/components/aat-furn#300391234> ;
.
<https://w3id.org/con-tax/components/aat-furn#300391093>
  rdf:type owl:Class ;
  rdfs:comment "Distinctive chests, often portable, designed for the altar to be collapsible or otherwise fit into a chest, along with the other essential items required for the liturgy. The term may also apply to chests associated with a separate altar, whether or not they are portable or were intended to be hidden. Well-known examples of collapsible portable altar chests, intended to be hidden, were those used in northern Europe in the 17th-18th centuries, during times of prohibition of the celebration of Catholic Mass."@en ;
  rdfs:comment "Draagbaar altaar met altaarsteen, uitgevoerd als een uitklapbare kist. In de kist zat een volledige uitrusting voor de eucharistieviering. Dit 'onzichtbare' altaar werd gebruikt in tijden van verbod op de viering van de katholieke eredienst in de zeventiende en achttiende eeuw, de schuilkerkperiode."@nl ;
  rdfs:isDefinedBy <https://w3id.org/con-tax/components/aat-furn> ;
  rdfs:label "altaarkist"@nl ;
  rdfs:label "altaarkisten"@nl ;
  rdfs:label "altar chests"@en ;
  rdfs:seeAlso <http://vocab.getty.edu/aat/300391093> ;
  rdfs:subClassOf <https://w3id.org/con-tax/components/aat-furn#300038860> ;
.
<https://w3id.org/con-tax/components/aat-furn#300391094>
  rdf:type owl:Class ;
  rdfs:comment "Cushioned steps or detached cushions for the step located in front of or around an altar, used at a Mass or other Christian service. An example of usage is by kneeling acolytes, deacons, and sub-deacons during solemn segments of the worship."@en ;
  rdfs:comment "Kussen op de altaartrede waarop wordt geknield tijdens plechtige gedeelten van de eredienst. Bestemd voor misdienaars, diakens en subdiakens."@nl ;
  rdfs:isDefinedBy <https://w3id.org/con-tax/components/aat-furn> ;
  rdfs:label "altaarkussen"@nl ;
  rdfs:label "altaarkussens"@nl ;
  rdfs:label "altar kneelers"@en ;
  rdfs:seeAlso <http://vocab.getty.edu/aat/300391094> ;
  rdfs:subClassOf <https://w3id.org/con-tax/components/aat-furn#300137869> ;
.
<https://w3id.org/con-tax/components/aat-furn#300391111>
  rdf:type owl:Class ;
  rdfs:comment "In Christian churches or places of other religious services, stands or tables used for the collection plate or other offertory gifts. "@en ;
  rdfs:comment "Standaard voor collecteschaal."@nl ;
  rdfs:isDefinedBy <https://w3id.org/con-tax/components/aat-furn> ;
  rdfs:label "collectestandaard"@nl ;
  rdfs:label "collectestandaarden"@nl ;
  rdfs:label "offertory tables"@en ;
  rdfs:seeAlso <http://vocab.getty.edu/aat/300391111> ;
  rdfs:subClassOf <https://w3id.org/con-tax/components/aat-furn#300039548> ;
  rdfs:subClassOf <https://w3id.org/con-tax/components/aat-furn#300039767> ;
.
<https://w3id.org/con-tax/components/aat-furn#300391234>
  rdf:type owl:Class ;
  rdfs:comment "Display cabinets having many openings or drawers, that were originally designed to hold and display multiple relics of a saint, martyr, deity, or other holy person. Later the term came to mean similar cabinets intended to hold historical artifacts or curiosities of any kind, usually modest in size and having a common theme."@en ;
  rdfs:isDefinedBy <https://w3id.org/con-tax/components/aat-furn> ;
  rdfs:label "cabinets of relics"@en ;
  rdfs:seeAlso <http://vocab.getty.edu/aat/300391234> ;
  rdfs:subClassOf <https://w3id.org/con-tax/components/aat-furn#300379868> ;
.
<https://w3id.org/con-tax/components/aat-furn#300391286>
  rdf:type owl:Class ;
  rdfs:comment "Refers to any low pressure suction table whether equipped with heating, air circulation, or humidification capabilities. Vacuum tables are used in conservation science to carry out tasks such as relining and relaxing canvases, cleaning paper and textiles, mending tears in various materials."@en ;
  rdfs:isDefinedBy <https://w3id.org/con-tax/components/aat-furn> ;
  rdfs:label "vacuum tables"@en ;
  rdfs:seeAlso <http://vocab.getty.edu/aat/300391286> ;
  rdfs:subClassOf <https://w3id.org/con-tax/components/aat-furn#300039548> ;
.
<https://w3id.org/con-tax/components/aat-furn#300391453>
  rdf:type owl:Class ;
  rdfs:comment "Large liquor cabinets having spaces designed specifically for holding bottles of liquor, wine, glasses, other utensils, ice, and a shelf or surface needed for making and serving drinks. "@en ;
  rdfs:isDefinedBy <https://w3id.org/con-tax/components/aat-furn> ;
  rdfs:label "bar cabinets"@en ;
  rdfs:seeAlso <http://vocab.getty.edu/aat/300391453> ;
  rdfs:subClassOf <https://w3id.org/con-tax/components/aat-furn#300391454> ;
.
<https://w3id.org/con-tax/components/aat-furn#300391454>
  rdf:type owl:Class ;
  rdfs:comment "Cabinets of any size having shelves or horizontal slots designed specifically for holding bottles of liquor and wine, and also glasses. For chests or smaller cabinets for holding liquor or wine bottles, use \"cellerets.\""@en ;
  rdfs:isDefinedBy <https://w3id.org/con-tax/components/aat-furn> ;
  rdfs:label "liquor cabinets"@en ;
  rdfs:seeAlso <http://vocab.getty.edu/aat/300391454> ;
  rdfs:subClassOf <https://w3id.org/con-tax/components/aat-furn#300038888> ;
.
<https://w3id.org/con-tax/components/aat-furn#300391486>
  rdf:type owl:Class ;
  rdfs:comment "Chairs by means of which an electric current can be passed through a person sitting in it, especially those in which convicted criminals are executed by electrocution."@en ;
  rdfs:isDefinedBy <https://w3id.org/con-tax/components/aat-furn> ;
  rdfs:label "electric chairs"@en ;
  rdfs:label "elektrische stoel"@nl ;
  rdfs:label "elektrische stoelen"@nl ;
  rdfs:seeAlso <http://vocab.getty.edu/aat/300391486> ;
  rdfs:seeAlso wd:Q185639 ;
  rdfs:subClassOf <https://w3id.org/con-tax/components/aat-furn#300037772> ;
.
<https://w3id.org/con-tax/components/aat-furn#300395528>
  rdf:type owl:Class ;
  rdfs:comment "Algemene benaming voor het kerkgestoelte voor de armenmeesters van een broederschap. Vanuit deze bank werden levensmiddelen en zaken voor de eerste levensbehoeften uitgedeeld aan armen, ouden van dagen, wezen en gebrekkigen die hiervoor in aanmerking kwamen, veelal op vertoon van een aan hen geschonken armenpenning. Gesneden voorstellingen van de bank kunnen duiden op het gebruik."@nl ;
  rdfs:comment "Benches designating the location where food and other donations for the poor or needy are distributed. Primarily used in historical contexts, for such benches on the premises of churches, hospitals, guilds, private estates, or other establishments that distributed alms."@en ;
  rdfs:isDefinedBy <https://w3id.org/con-tax/components/aat-furn> ;
  rdfs:label "almoners benches"@en ;
  rdfs:label "armenmeestersbanken"@nl ;
  rdfs:seeAlso <http://vocab.getty.edu/aat/300395528> ;
  rdfs:subClassOf <https://w3id.org/con-tax/components/aat-furn#300038494> ;
.
<https://w3id.org/con-tax/components/aat-furn#300395530>
  rdf:type owl:Class ;
  rdfs:comment "Bank voor het vastzetten van gevangenen of anderen. Het doel varieerde door de geschiedenis heen. Soms diende het om personen tijdelijk vast te zetten in afwachting van straf of rechtszaak. Werd ook gebruikt voor gevangenen die een religieuze dienst, of andere gebeurtenis mochten bijwonen."@nl ;
  rdfs:comment "Benches designed to allow the detainment of prisoners or others. The benches may be enclosed or open, and may be designed to allow the attachment of restraints. The purpose of the benches varied in periods of history and various contexts: purposes include as a temporary means of detainment prior to imprisonment or trial, to shame the citizen in a public place, or to allow the detainees to attend a religious service or other event.    "@en ;
  rdfs:isDefinedBy <https://w3id.org/con-tax/components/aat-furn> ;
  rdfs:label "arrestantenbank"@nl ;
  rdfs:label "arrestantenbanken"@nl ;
  rdfs:label "prisoners' benches"@en ;
  rdfs:seeAlso <http://vocab.getty.edu/aat/300395530> ;
  rdfs:subClassOf <https://w3id.org/con-tax/components/aat-furn#300038494> ;
.
<https://w3id.org/con-tax/components/aat-furn#300395619>
  rdf:type owl:Class ;
  rdfs:comment "Chairs designed for the use of the priest or other celebrant presiding at a Christian mass or other service. The chairs are usually of substantial size and having arms, placed in the choir of the church. For a set of three chairs or seats on a recessed bench for the celebrant, deacon, and sub-deacon, use \"sedilia.\" For the chairs of a presiding bishop, use \"cathedrae (bishop's chairs).\" For chairs specifically for a presiding Protestant preacher, use \"preacher's chairs.\""@en ;
  rdfs:comment "in de Roomse- en Oud-Katholieke kerken: stoel met lage rugleuning in het priesterkoor, ter zijde van het altaar, waarop de priester plaats neemt bij de vespers."@nl ;
  rdfs:isDefinedBy <https://w3id.org/con-tax/components/aat-furn> ;
  rdfs:label "presider's chairs"@en ;
  rdfs:label "vesperstoel"@nl ;
  rdfs:label "vesperstoelen"@nl ;
  rdfs:seeAlso <http://vocab.getty.edu/aat/300395619> ;
  rdfs:subClassOf <https://w3id.org/con-tax/components/aat-furn#300133851> ;
.
<https://w3id.org/con-tax/components/aat-furn#300395631>
  rdf:type owl:Class ;
  rdfs:comment "Standaard waaraan het wierookvat hangt en waaraan soms ook een houder voor een wierookscheepje is bevestigd."@nl ;
  rdfs:comment "Stands of varied design that support containers with perforated covers used for burning incense in a ritual context."@en ;
  rdfs:isDefinedBy <https://w3id.org/con-tax/components/aat-furn> ;
  rdfs:label "censer stands"@en ;
  rdfs:label "wierookstandaard"@nl ;
  rdfs:label "wierookstandaarden"@nl ;
  rdfs:seeAlso <http://vocab.getty.edu/aat/300395631> ;
  rdfs:subClassOf <https://w3id.org/con-tax/components/aat-furn#300039767> ;
.
<https://w3id.org/con-tax/components/aat-furn#300400539>
  rdf:type owl:Class ;
  rdfs:comment "Cupboards intended for the storage of food and other donations for the poor or needy. Primarily used in historical contexts, for such cupboards on the premises of churches, hospitals, guilds, private estates, or other establishments that distributed alms."@en ;
  rdfs:isDefinedBy <https://w3id.org/con-tax/components/aat-furn> ;
  rdfs:label "almoners cupboards"@en ;
  rdfs:seeAlso <http://vocab.getty.edu/aat/300400539> ;
  rdfs:subClassOf <https://w3id.org/con-tax/components/aat-furn#300249925> ;
.
<https://w3id.org/con-tax/components/aat-furn#300400635>
  rdf:type owl:Class ;
  rdfs:comment "Altaar gebruikt tijdens religieuze ceremonies om vloeibare offers te brengen, die erover worden gegoten, vaak met rytons. Het altaar helt soms af naar één kant, waar aan het uiteinde een bekken de vloeistof terug opvangt."@nl ;
  rdfs:comment "Altars used at religious sites for liquid offerings, which are poured over it, often through rhytons. These may slope down toward a basin to collect the liquid, or have carved depressions."@en ;
  rdfs:isDefinedBy <https://w3id.org/con-tax/components/aat-furn> ;
  rdfs:label "libatietafel"@nl ;
  rdfs:label "libatietafels"@nl ;
  rdfs:label "libation tables"@en ;
  rdfs:label "plengoffertafel"@nl ;
  rdfs:label "plengoffertafels"@nl ;
  rdfs:seeAlso <http://vocab.getty.edu/aat/300400635> ;
  rdfs:subClassOf <https://w3id.org/con-tax/components/aat-furn#300039548> ;
.
<https://w3id.org/con-tax/components/aat-furn#300403901>
  rdf:type owl:Class ;
  rdfs:comment "Beds of any form, where a person is laid while dying."@en ;
  rdfs:isDefinedBy <https://w3id.org/con-tax/components/aat-furn> ;
  rdfs:label "deathbeds"@en ;
  rdfs:seeAlso <http://vocab.getty.edu/aat/300403901> ;
  rdfs:subClassOf <https://w3id.org/con-tax/components/aat-furn#300038697> ;
.
<https://w3id.org/con-tax/components/aat-furn#300403902>
  rdf:type owl:Class ;
  rdfs:comment "Beds designed with a very high canopy suspended from an ornate horizontal frame, attached to the wall behind the head or to the ceiling, and often supported by columns or posts at the foot of the bed. For beds of similar design, but of lesser height and bulk, without the supporting posts at the foot, use \"lits à la duchesse.\""@en ;
  rdfs:isDefinedBy <https://w3id.org/con-tax/components/aat-furn> ;
  rdfs:label "lits à l'impériale"@en ;
  rdfs:seeAlso <http://vocab.getty.edu/aat/300403902> ;
  rdfs:subClassOf <https://w3id.org/con-tax/components/aat-furn#300142742> ;
.
<https://w3id.org/con-tax/components/aat-furn#300403907>
  rdf:type owl:Class ;
  rdfs:comment "Tables of various designs used for displaying and serving food in a dining room. In modern usage, for case furniture used for serving food and displaying dishes, use \"sideboards (furniture).\""@en ;
  rdfs:isDefinedBy <https://w3id.org/con-tax/components/aat-furn> ;
  rdfs:label "serving tables (tables)"@en ;
  rdfs:seeAlso <http://vocab.getty.edu/aat/300403907> ;
  rdfs:subClassOf <https://w3id.org/con-tax/components/aat-furn#300039548> ;
.
<https://w3id.org/con-tax/components/aat-furn#300404167>
  rdf:type owl:Class ;
  rdfs:comment "Ceremonial stools common to the Taino culture carved out of wood or stone and are typically made with zoomorphic and anthropomorphic design elements. The stools were used by the higher ranking tribe members during community rituals and activities."@en ;
  rdfs:isDefinedBy <https://w3id.org/con-tax/components/aat-furn> ;
  rdfs:label "duhos"@en ;
  rdfs:seeAlso <http://vocab.getty.edu/aat/300404167> ;
  rdfs:subClassOf <https://w3id.org/con-tax/components/aat-furn#300133851> ;
.
<https://w3id.org/con-tax/components/aat-furn#300404188>
  rdf:type owl:Class ;
  rdfs:comment "Case furniture for storing altar frontals and other antependia, usually located in the sacristy of the church."@en ;
  rdfs:comment "Kast voor het opbergen van de antependia."@nl ;
  rdfs:isDefinedBy <https://w3id.org/con-tax/components/aat-furn> ;
  rdfs:label "antependiumkast"@nl ;
  rdfs:label "antependiumkasten"@nl ;
  rdfs:label "frontal cupboards"@en ;
  rdfs:seeAlso <http://vocab.getty.edu/aat/300404188> ;
  rdfs:subClassOf <https://w3id.org/con-tax/components/aat-furn#300298883> ;
.
<https://w3id.org/con-tax/components/aat-furn#300404220>
  rdf:type owl:Class ;
  rdfs:comment "Staander van hout of metaal, waarop het doopbekken rust."@nl ;
  rdfs:comment "Stands of various designs that rest on the floor or ground and support the baptismal font. For tabletop or wall-mounted supports for the baptismal font, use \"baptismal font supports.\""@en ;
  rdfs:isDefinedBy <https://w3id.org/con-tax/components/aat-furn> ;
  rdfs:label "baptismal font stands"@en ;
  rdfs:label "doopbekkenstandaard"@nl ;
  rdfs:label "doopbekkenstandaarden"@nl ;
  rdfs:seeAlso <http://vocab.getty.edu/aat/300404220> ;
  rdfs:subClassOf <https://w3id.org/con-tax/components/aat-furn#300039767> ;
.
<https://w3id.org/con-tax/components/aat-furn#300404223>
  rdf:type owl:Class ;
  rdfs:comment "Metalen of houten hek ter afsluiting van de dooptuin of doopkapel."@nl ;
  rdfs:comment "Screens separating the baptismal font and area from the rest of the church; may comprise a solid screen, open screen work, or a railing. For separate structures or chapels used for baptisms, use \"baptistries.\""@en ;
  rdfs:isDefinedBy <https://w3id.org/con-tax/components/aat-furn> ;
  rdfs:label "baptismal screens"@en ;
  rdfs:label "doophek"@nl ;
  rdfs:label "doophekken"@nl ;
  rdfs:seeAlso <http://vocab.getty.edu/aat/300404223> ;
  rdfs:subClassOf <https://w3id.org/con-tax/components/aat-furn#300037737> ;
.
<https://w3id.org/con-tax/components/aat-furn#300404231>
  rdf:type owl:Class ;
  rdfs:comment "Kerkbank voor de leden van het Hof. De identiteit van de hofleden kan worden afgeleid van het snijwerk en het familiewapen."@nl ;
  rdfs:comment "Pews in a church reserved for the royal family; the pews may be set up on a high platform or otherwise decorated and designated as belonging to the monarch or family."@en ;
  rdfs:isDefinedBy <https://w3id.org/con-tax/components/aat-furn> ;
  rdfs:label "hofbank"@nl ;
  rdfs:label "hofbanken"@nl ;
  rdfs:label "royal pews"@en ;
  rdfs:seeAlso <http://vocab.getty.edu/aat/300404231> ;
  rdfs:subClassOf <https://w3id.org/con-tax/components/aat-furn#300038521> ;
.
<https://w3id.org/con-tax/components/aat-furn#300404251>
  rdf:type owl:Class ;
  rdfs:comment "Racks of various designs used for drying towels; may be attached to a wall or other surface, or standing on the floor."@en ;
  rdfs:comment "Rek waaraan handdoeken worden gehangen. "@nl ;
  rdfs:isDefinedBy <https://w3id.org/con-tax/components/aat-furn> ;
  rdfs:label "handdoekenrek"@nl ;
  rdfs:label "handdoekenrekken"@nl ;
  rdfs:label "towel racks"@en ;
  rdfs:seeAlso <http://vocab.getty.edu/aat/300404251> ;
  rdfs:subClassOf <https://w3id.org/con-tax/components/aat-furn#300039337> ;
.
<https://w3id.org/con-tax/components/aat-furn#300404253>
  rdf:type owl:Class ;
  rdfs:comment "Stools or other types of simple seats in the choir of a church, used by acolytes or other assistants of the celebrant."@en ;
  rdfs:comment "Zetels, soms opvouwbaar, bedoeld voor de misdienaren. De misdienaarskrukken maken soms ook deel uit van de set van kerkgestoelte."@nl ;
  rdfs:isDefinedBy <https://w3id.org/con-tax/components/aat-furn> ;
  rdfs:label "acolyte seats"@en ;
  rdfs:label "misdienaarskruk"@nl ;
  rdfs:label "misdienaarskrukken"@nl ;
  rdfs:seeAlso <http://vocab.getty.edu/aat/300404253> ;
  rdfs:subClassOf <https://w3id.org/con-tax/components/aat-furn#300133851> ;
.
<https://w3id.org/con-tax/components/aat-furn#300404259>
  rdf:type owl:Class ;
  rdfs:comment "Chairs of various designs, positioned at the front of certain Protestant churches and used by the preacher during services. For chairs having a tall back surmounted by a lectern and used as a  pulpit, use \"preaching chairs.\""@en ;
  rdfs:comment "Zetel, veelal in de nabijheid van de liturgische tafel, waarop de predikant plaatsneemt tijdens momenten van rust in de dienst, zoals tijdens het zingen van een lied, tijdens de collectes en wanneer iemand anders dan de predikant een lezing verricht. Vaak wordt ook met een stoel genoegen genomen."@nl ;
  rdfs:isDefinedBy <https://w3id.org/con-tax/components/aat-furn> ;
  rdfs:label "preacher's chairs (presider's chairs)"@en ;
  rdfs:label "predikantenzetel"@nl ;
  rdfs:label "predikantenzetels"@nl ;
  rdfs:seeAlso <http://vocab.getty.edu/aat/300404259> ;
  rdfs:subClassOf <https://w3id.org/con-tax/components/aat-furn#300395619> ;
.
<https://w3id.org/con-tax/components/aat-furn#300404365>
  rdf:type owl:Class ;
  rdfs:comment "Small tables on which vessels and dishes are placed pior to serving in a dining room. They differ from \"credenzas (sideboards)\" in that they are smaller and their form is of a table rather than case furniture. They may be designed so that they back flush against the table or a wall. The term originates in the custom at courts for food to be tasted and proven trustworthy before being served to the monarch. For similar tables used in churches near the altar, prefer \"credence tables (religious building fixtures).\""@en ;
  rdfs:isDefinedBy <https://w3id.org/con-tax/components/aat-furn> ;
  rdfs:label "credences (dining room tables)"@en ;
  rdfs:seeAlso <http://vocab.getty.edu/aat/300404365> ;
  rdfs:subClassOf <https://w3id.org/con-tax/components/aat-furn#300039548> ;
.
<https://w3id.org/con-tax/components/aat-furn#300404744>
  rdf:type owl:Class ;
  rdfs:comment "Thrones depicted in Buddhist art or used in Buddhism that are supported by lions or incorporating lions in the design; most often thrones upon which the Buddha is seated. An example is the seated Buddha in which eight lions positioned at the corners of the base or dais support his lotus throne; another example is the throne of the Dalai Lama of Tibet."@en ;
  rdfs:comment """Tronen zoals afgebeeld in boeddhistische kunst of gebruikt in het boeddhisme, die worden ondersteund door leeuwen of waarin leeuwen in het ontwerp voorkomen. Meestal zit de Boeddha op de troon. Een voorbeeld is de zittende Boeddha, waarbij acht leeuwen bij de hoeken van het voetstuk, of dais, zijn lotustroon ondersteunen. Een ander voorbeeld is de troon van de Dalai Lama van Tibet.
"""@nl ;
  rdfs:isDefinedBy <https://w3id.org/con-tax/components/aat-furn> ;
  rdfs:label "leeuwentronen"@nl ;
  rdfs:label "leeuwentroon"@nl ;
  rdfs:label "lion thrones"@en ;
  rdfs:seeAlso <http://vocab.getty.edu/aat/300404744> ;
  rdfs:subClassOf <https://w3id.org/con-tax/components/aat-furn#300038141> ;
.
<https://w3id.org/con-tax/components/aat-furn#300411438>
  rdf:type owl:Class ;
  rdfs:comment "Benches located on the stoop of a residence or other building in an urban environment; usually of modest size and fixed in place. For benches, swings, chairs, and other furniture on the porch of a residence, use \"porch furniture.\""@en ;
  rdfs:comment "Vaste bank op een (particuliere) stoep, meestal bevestigd tussen de gevel van de woning en een stoepbaluster. Het is geen openbare zitplek."@nl ;
  rdfs:isDefinedBy <https://w3id.org/con-tax/components/aat-furn> ;
  rdfs:label "stoepbank"@nl ;
  rdfs:label "stoepbanken"@nl ;
  rdfs:label "stoop benches"@en ;
  rdfs:seeAlso <http://vocab.getty.edu/aat/300411438> ;
  rdfs:subClassOf <https://w3id.org/con-tax/components/aat-furn#300038494> ;
.
<https://w3id.org/con-tax/components/aat-furn#300411571>
  rdf:type owl:Class ;
  rdfs:comment "Racks used to dry objects on, especially washed kitchenware."@en ;
  rdfs:comment "Rekken waarop men voorwerpen, met name de gewassen vaat, laat afdruipen."@nl ;
  rdfs:isDefinedBy <https://w3id.org/con-tax/components/aat-furn> ;
  rdfs:label "afdruiprek"@nl ;
  rdfs:label "afdruiprekken"@nl ;
  rdfs:label "dish racks"@en ;
  rdfs:seeAlso <http://vocab.getty.edu/aat/300411571> ;
  rdfs:subClassOf <https://w3id.org/con-tax/components/aat-furn#300039337> ;
.
<https://w3id.org/con-tax/components/aat-furn#300411774>
  rdf:type owl:Class ;
  rdfs:comment "Chairs designed for use at the beach, having a hood for protection from the sun and wind. May be made of wicker, wood and cloth, or other materials. Originally made of wicker in the 19th century, based on wicker armchair furniture with covered high rising hoods that had been created by basketmakers for centuries. "@en ;
  rdfs:comment """Stoelen voor op het strand, met een kap voor bescherming tegen zon en wind. Ze kunnen van vlechtwerk, hout en doek, of andere materialen gemaakt zijn. In de 19de eeuw werden ze van vlechtwerk gemaakt, naar het model van gevlochten stoelen met armleuningen met hoge kappen die al eeuwenlang door mandenmakers werden gemaakt. 
"""@nl ;
  rdfs:isDefinedBy <https://w3id.org/con-tax/components/aat-furn> ;
  rdfs:label "strandkorbs"@en ;
  rdfs:label "strandkorf"@nl ;
  rdfs:label "strandkorven"@nl ;
  rdfs:seeAlso <http://vocab.getty.edu/aat/300411774> ;
  rdfs:subClassOf <https://w3id.org/con-tax/components/aat-furn#300164274> ;
.
<https://w3id.org/con-tax/components/aat-furn#300417284>
  rdf:type owl:Class ;
  rdfs:comment "Cabinets of drawers designed to store unbound maps, prints, posters, drawings, or any other large-format flat documents."@en ;
  rdfs:isDefinedBy <https://w3id.org/con-tax/components/aat-furn> ;
  rdfs:label "flat file cabinets"@en ;
  rdfs:seeAlso <http://vocab.getty.edu/aat/300417284> ;
  rdfs:subClassOf <https://w3id.org/con-tax/components/aat-furn#300038936> ;
.
<https://w3id.org/con-tax/components/aat-furn#300417455>
  rdf:type owl:Class ;
  rdfs:comment "Cylinder desks, that is writing desks with a cover that rolls up into the desk top, that are designed for ladies; they are distinguished by often having a relatively delicate design and a wide space to accommodate ladies' skirts."@en ;
  rdfs:isDefinedBy <https://w3id.org/con-tax/components/aat-furn> ;
  rdfs:label "ladies' cylinder writing tables"@en ;
  rdfs:seeAlso <http://vocab.getty.edu/aat/300417455> ;
  rdfs:subClassOf <https://w3id.org/con-tax/components/aat-furn#300039470> ;
  rdfs:subClassOf <https://w3id.org/con-tax/components/aat-furn#300146667> ;
.
<https://w3id.org/con-tax/components/aat-furn#300417914>
  rdf:type owl:Class ;
  rdfs:comment "Skull racks or similar constructions used in Pre-Columbian Mesoamerica to display the heads or skulls of sacrificed human victims, or platforms carved with human skulls to resemble such a rack. Tzompantlis were usually placed near temples or ballcourts. Those displaying real skulls comprised a wooden framework supporting skulls skewered on horizontal poles run through holes drilled through the temples. Tzompantlis took a variety of forms and seem to have served several functions: altars and venues for ritual; displays of Aztec prowess; and to terrorize subjugated populations."@en ;
  rdfs:isDefinedBy <https://w3id.org/con-tax/components/aat-furn> ;
  rdfs:label "tzompantlis"@en ;
  rdfs:seeAlso <http://vocab.getty.edu/aat/300417914> ;
  rdfs:subClassOf <https://w3id.org/con-tax/components/aat-furn#300039767> ;
.
<https://w3id.org/con-tax/components/aat-furn#300419287>
  rdf:type owl:Class ;
  rdfs:comment "Thrones or seats incorporating lotus motifs, found in Hindu, Buddhist, and other traditions."@en ;
  rdfs:isDefinedBy <https://w3id.org/con-tax/components/aat-furn> ;
  rdfs:label "lotus thrones"@en ;
  rdfs:seeAlso <http://vocab.getty.edu/aat/300419287> ;
  rdfs:subClassOf <https://w3id.org/con-tax/components/aat-furn#300038141> ;
.
<https://w3id.org/con-tax/components/aat-furn#300419378>
  rdf:type owl:Class ;
  rdfs:comment "Tables or other platforms in temples and churches upon which offerings to divinities are set. Not specific to geographic location, religious culture, or historical period: there are Ptolemaic, Shinto Buddhist, Vaishnav, Christian and Jewish offering tables. Examples are the blocks of sculpted stone or wood, intended to be placed in front of the false doors or statues of Egyptian tombs. These held food, drink, or other offerings to the dead and deities. For similar objects used specifically for liquid offerings, use 'libation tables.'"@en ;
  rdfs:isDefinedBy <https://w3id.org/con-tax/components/aat-furn> ;
  rdfs:label "offering tables"@en ;
  rdfs:seeAlso <http://vocab.getty.edu/aat/300419378> ;
  rdfs:subClassOf <https://w3id.org/con-tax/components/aat-furn#300039548> ;
.
<https://w3id.org/con-tax/components/aat-furn#300420055>
  rdf:type owl:Class ;
  rdfs:comment "Chairs used in religious settings; examples include chairs built to hold spirit houses and small altars or bishop’s chairs used in Christian churches."@en ;
  rdfs:isDefinedBy <https://w3id.org/con-tax/components/aat-furn> ;
  rdfs:label "altar chairs"@en ;
  rdfs:seeAlso <http://vocab.getty.edu/aat/300420055> ;
  rdfs:subClassOf <https://w3id.org/con-tax/components/aat-furn#300133851> ;
.
<https://w3id.org/con-tax/components/aat-furn#300420253>
  rdf:type owl:Class ;
  rdfs:isDefinedBy <https://w3id.org/con-tax/components/aat-furn> ;
  rdfs:label "apothecary chest"@en ;
  rdfs:seeAlso <http://vocab.getty.edu/aat/300420253> ;
  rdfs:subClassOf <https://w3id.org/con-tax/components/aat-furn#300037680> ;
.
<https://w3id.org/con-tax/components/aat-furn#300420268>
  rdf:type owl:Class ;
  rdfs:isDefinedBy <https://w3id.org/con-tax/components/aat-furn> ;
  rdfs:label "appliance cart"@en ;
  rdfs:seeAlso <http://vocab.getty.edu/aat/300420268> ;
  rdfs:subClassOf <https://w3id.org/con-tax/components/aat-furn#300039337> ;
.
<https://w3id.org/con-tax/components/aat-furn#300420664>
  rdf:type owl:Class ;
  rdfs:isDefinedBy <https://w3id.org/con-tax/components/aat-furn> ;
  rdfs:label "ballroom chair"@en ;
  rdfs:seeAlso <http://vocab.getty.edu/aat/300420664> ;
  rdfs:subClassOf <https://w3id.org/con-tax/components/aat-furn#300037769> ;
.
<https://w3id.org/con-tax/components/aat-furn#300420742>
  rdf:type owl:Class ;
  rdfs:isDefinedBy <https://w3id.org/con-tax/components/aat-furn> ;
  rdfs:label "barber's cabinet"@en ;
  rdfs:seeAlso <http://vocab.getty.edu/aat/300420742> ;
  rdfs:subClassOf <https://w3id.org/con-tax/components/aat-furn#300037680> ;
.
<https://w3id.org/con-tax/components/aat-furn#300420822>
  rdf:type owl:Class ;
  rdfs:isDefinedBy <https://w3id.org/con-tax/components/aat-furn> ;
  rdfs:label "basket stand"@en ;
  rdfs:seeAlso <http://vocab.getty.edu/aat/300420822> ;
  rdfs:subClassOf <https://w3id.org/con-tax/components/aat-furn#300039337> ;
.
<https://w3id.org/con-tax/components/aat-furn#300421184>
  rdf:type owl:Class ;
  rdfs:isDefinedBy <https://w3id.org/con-tax/components/aat-furn> ;
  rdfs:label "bucket bench"@en ;
  rdfs:seeAlso <http://vocab.getty.edu/aat/300421184> ;
  rdfs:subClassOf <https://w3id.org/con-tax/components/aat-furn#300037769> ;
.
<https://w3id.org/con-tax/components/aat-furn#300421391>
  rdf:type owl:Class ;
  rdfs:isDefinedBy <https://w3id.org/con-tax/components/aat-furn> ;
  rdfs:label "café table"@en ;
  rdfs:seeAlso <http://vocab.getty.edu/aat/300421391> ;
  rdfs:subClassOf <https://w3id.org/con-tax/components/aat-furn#300039337> ;
.
<https://w3id.org/con-tax/components/aat-furn#300421477>
  rdf:type owl:Class ;
  rdfs:isDefinedBy <https://w3id.org/con-tax/components/aat-furn> ;
  rdfs:label "campaign desk"@en ;
  rdfs:seeAlso <http://vocab.getty.edu/aat/300421477> ;
  rdfs:subClassOf <https://w3id.org/con-tax/components/aat-furn#300037680> ;
.
<https://w3id.org/con-tax/components/aat-furn#300421866>
  rdf:type owl:Class ;
  rdfs:comment "Tables used in bookbinding."@en ;
  rdfs:isDefinedBy <https://w3id.org/con-tax/components/aat-furn> ;
  rdfs:label "bindery tables"@en ;
  rdfs:seeAlso <http://vocab.getty.edu/aat/300421866> ;
  rdfs:subClassOf <https://w3id.org/con-tax/components/aat-furn#300039548> ;
.
<https://w3id.org/con-tax/components/aat-furn#300421906>
  rdf:type owl:Class ;
  rdfs:isDefinedBy <https://w3id.org/con-tax/components/aat-furn> ;
  rdfs:label "birdcage stand"@en ;
  rdfs:seeAlso <http://vocab.getty.edu/aat/300421906> ;
  rdfs:subClassOf <https://w3id.org/con-tax/components/aat-furn#300039337> ;
.
<https://w3id.org/con-tax/components/aat-furn#300422207>
  rdf:type owl:Class ;
  rdfs:isDefinedBy <https://w3id.org/con-tax/components/aat-furn> ;
  rdfs:label "computer cart"@en ;
  rdfs:seeAlso <http://vocab.getty.edu/aat/300422207> ;
  rdfs:subClassOf <https://w3id.org/con-tax/components/aat-furn#300039337> ;
.
<https://w3id.org/con-tax/components/aat-furn#300422209>
  rdf:type owl:Class ;
  rdfs:isDefinedBy <https://w3id.org/con-tax/components/aat-furn> ;
  rdfs:label "computer desk"@en ;
  rdfs:seeAlso <http://vocab.getty.edu/aat/300422209> ;
  rdfs:subClassOf <https://w3id.org/con-tax/components/aat-furn#300037680> ;
.
<https://w3id.org/con-tax/components/aat-furn#300422652>
  rdf:type owl:Class ;
  rdfs:isDefinedBy <https://w3id.org/con-tax/components/aat-furn> ;
  rdfs:label "card cabinet"@en ;
  rdfs:seeAlso <http://vocab.getty.edu/aat/300422652> ;
  rdfs:subClassOf <https://w3id.org/con-tax/components/aat-furn#300037680> ;
.
<https://w3id.org/con-tax/components/aat-furn#300422732>
  rdf:type owl:Class ;
  rdfs:isDefinedBy <https://w3id.org/con-tax/components/aat-furn> ;
  rdfs:label "cart table"@en ;
  rdfs:seeAlso <http://vocab.getty.edu/aat/300422732> ;
  rdfs:subClassOf <https://w3id.org/con-tax/components/aat-furn#300039337> ;
.
<https://w3id.org/con-tax/components/aat-furn#300422971>
  rdf:type owl:Class ;
  rdfs:isDefinedBy <https://w3id.org/con-tax/components/aat-furn> ;
  rdfs:label "changing table"@en ;
  rdfs:seeAlso <http://vocab.getty.edu/aat/300422971> ;
  rdfs:subClassOf <https://w3id.org/con-tax/components/aat-furn#300037680> ;
.
<https://w3id.org/con-tax/components/aat-furn#300423001>
  rdf:type owl:Class ;
  rdfs:isDefinedBy <https://w3id.org/con-tax/components/aat-furn> ;
  rdfs:label "chart table"@en ;
  rdfs:seeAlso <http://vocab.getty.edu/aat/300423001> ;
  rdfs:subClassOf <https://w3id.org/con-tax/components/aat-furn#300039337> ;
.
<https://w3id.org/con-tax/components/aat-furn#300423082>
  rdf:type owl:Class ;
  rdfs:isDefinedBy <https://w3id.org/con-tax/components/aat-furn> ;
  rdfs:label "child's bed"@en ;
  rdfs:seeAlso <http://vocab.getty.edu/aat/300423082> ;
  rdfs:subClassOf <https://w3id.org/con-tax/components/aat-furn#300037680> ;
.
<https://w3id.org/con-tax/components/aat-furn#300423083>
  rdf:type owl:Class ;
  rdfs:isDefinedBy <https://w3id.org/con-tax/components/aat-furn> ;
  rdfs:label "child's chair"@en ;
  rdfs:seeAlso <http://vocab.getty.edu/aat/300423083> ;
  rdfs:subClassOf <https://w3id.org/con-tax/components/aat-furn#300037769> ;
.
<https://w3id.org/con-tax/components/aat-furn#300423204>
  rdf:type owl:Class ;
  rdfs:isDefinedBy <https://w3id.org/con-tax/components/aat-furn> ;
  rdfs:label "circular bench"@en ;
  rdfs:seeAlso <http://vocab.getty.edu/aat/300423204> ;
  rdfs:subClassOf <https://w3id.org/con-tax/components/aat-furn#300037769> ;
.
<https://w3id.org/con-tax/components/aat-furn#300423429>
  rdf:type owl:Class ;
  rdfs:isDefinedBy <https://w3id.org/con-tax/components/aat-furn> ;
  rdfs:label "coin cabinet"@en ;
  rdfs:seeAlso <http://vocab.getty.edu/aat/300423429> ;
  rdfs:subClassOf <https://w3id.org/con-tax/components/aat-furn#300037680> ;
.
<https://w3id.org/con-tax/components/aat-furn#300424190>
  rdf:type owl:Class ;
  rdfs:isDefinedBy <https://w3id.org/con-tax/components/aat-furn> ;
  rdfs:label "curio cabinet"@en ;
  rdfs:seeAlso <http://vocab.getty.edu/aat/300424190> ;
  rdfs:subClassOf <https://w3id.org/con-tax/components/aat-furn#300037680> ;
.
<https://w3id.org/con-tax/components/aat-furn#300424703>
  rdf:type owl:Class ;
  rdfs:isDefinedBy <https://w3id.org/con-tax/components/aat-furn> ;
  rdfs:label "futon frame"@en ;
  rdfs:seeAlso <http://vocab.getty.edu/aat/300424703> ;
  rdfs:subClassOf <https://w3id.org/con-tax/components/aat-furn#300037680> ;
.
<https://w3id.org/con-tax/components/aat-furn#300424776>
  rdf:type owl:Class ;
  rdfs:isDefinedBy <https://w3id.org/con-tax/components/aat-furn> ;
  rdfs:label "garden bench"@en ;
  rdfs:seeAlso <http://vocab.getty.edu/aat/300424776> ;
  rdfs:subClassOf <https://w3id.org/con-tax/components/aat-furn#300037769> ;
.
<https://w3id.org/con-tax/components/aat-furn#300424798>
  rdf:type owl:Class ;
  rdfs:isDefinedBy <https://w3id.org/con-tax/components/aat-furn> ;
  rdfs:label "garden table"@en ;
  rdfs:seeAlso <http://vocab.getty.edu/aat/300424798> ;
  rdfs:subClassOf <https://w3id.org/con-tax/components/aat-furn#300039337> ;
.
<https://w3id.org/con-tax/components/aat-furn#300424865>
  rdf:type owl:Class ;
  rdfs:comment "Circular, flat-sided bases, often made of wood; used in conjunction with gavels to communicate particular actions or to gather attention; accomplished by striking the gavel block with the mallet. Examples of use include court proceedings or auctions. "@en ;
  rdfs:isDefinedBy <https://w3id.org/con-tax/components/aat-furn> ;
  rdfs:label "gavel blocks"@en ;
  rdfs:seeAlso <http://vocab.getty.edu/aat/300424865> ;
  rdfs:subClassOf <https://w3id.org/con-tax/components/aat-furn#300039767> ;
.
<https://w3id.org/con-tax/components/aat-furn#300425131>
  rdf:type owl:Class ;
  rdfs:isDefinedBy <https://w3id.org/con-tax/components/aat-furn> ;
  rdfs:label "entertainment cabinet"@en ;
  rdfs:seeAlso <http://vocab.getty.edu/aat/300425131> ;
  rdfs:subClassOf <https://w3id.org/con-tax/components/aat-furn#300037680> ;
.
<https://w3id.org/con-tax/components/aat-furn#300425516>
  rdf:type owl:Class ;
  rdfs:isDefinedBy <https://w3id.org/con-tax/components/aat-furn> ;
  rdfs:label "fireplace chair"@en ;
  rdfs:seeAlso <http://vocab.getty.edu/aat/300425516> ;
  rdfs:subClassOf <https://w3id.org/con-tax/components/aat-furn#300037769> ;
.
<https://w3id.org/con-tax/components/aat-furn#300425717>
  rdf:type owl:Class ;
  rdfs:isDefinedBy <https://w3id.org/con-tax/components/aat-furn> ;
  rdfs:label "floor stand"@en ;
  rdfs:seeAlso <http://vocab.getty.edu/aat/300425717> ;
  rdfs:subClassOf <https://w3id.org/con-tax/components/aat-furn#300039337> ;
.
<https://w3id.org/con-tax/components/aat-furn#300425796>
  rdf:type owl:Class ;
  rdfs:isDefinedBy <https://w3id.org/con-tax/components/aat-furn> ;
  rdfs:label "folding bench"@en ;
  rdfs:seeAlso <http://vocab.getty.edu/aat/300425796> ;
  rdfs:subClassOf <https://w3id.org/con-tax/components/aat-furn#300037769> ;
.
<https://w3id.org/con-tax/components/aat-furn#300425808>
  rdf:type owl:Class ;
  rdfs:comment "Tables of various designs whereby the table top may be folded partially or entirely from the support, or where the legs may be folded under the table top; folding is done for ease of storage or otherwise to make the profile smaller."@en ;
  rdfs:isDefinedBy <https://w3id.org/con-tax/components/aat-furn> ;
  rdfs:label "folding tables"@en ;
  rdfs:seeAlso <http://vocab.getty.edu/aat/300425808> ;
  rdfs:subClassOf <https://w3id.org/con-tax/components/aat-furn#300039548> ;
.
<https://w3id.org/con-tax/components/aat-furn#300426144>
  rdf:type owl:Class ;
  rdfs:isDefinedBy <https://w3id.org/con-tax/components/aat-furn> ;
  rdfs:label "hooded bench"@en ;
  rdfs:seeAlso <http://vocab.getty.edu/aat/300426144> ;
  rdfs:subClassOf <https://w3id.org/con-tax/components/aat-furn#300037769> ;
.
<https://w3id.org/con-tax/components/aat-furn#300426554>
  rdf:type owl:Class ;
  rdfs:isDefinedBy <https://w3id.org/con-tax/components/aat-furn> ;
  rdfs:label "invalid chair"@en ;
  rdfs:seeAlso <http://vocab.getty.edu/aat/300426554> ;
  rdfs:subClassOf <https://w3id.org/con-tax/components/aat-furn#300037769> ;
.
<https://w3id.org/con-tax/components/aat-furn#300426805>
  rdf:type owl:Class ;
  rdfs:isDefinedBy <https://w3id.org/con-tax/components/aat-furn> ;
  rdfs:label "gun safe"@en ;
  rdfs:seeAlso <http://vocab.getty.edu/aat/300426805> ;
  rdfs:subClassOf <https://w3id.org/con-tax/components/aat-furn#300037680> ;
.
<https://w3id.org/con-tax/components/aat-furn#300427302>
  rdf:type owl:Class ;
  rdfs:isDefinedBy <https://w3id.org/con-tax/components/aat-furn> ;
  rdfs:label "media cart"@en ;
  rdfs:seeAlso <http://vocab.getty.edu/aat/300427302> ;
  rdfs:subClassOf <https://w3id.org/con-tax/components/aat-furn#300039337> ;
.
<https://w3id.org/con-tax/components/aat-furn#300427338>
  rdf:type owl:Class ;
  rdfs:isDefinedBy <https://w3id.org/con-tax/components/aat-furn> ;
  rdfs:label "medicine cabinet"@en ;
  rdfs:seeAlso <http://vocab.getty.edu/aat/300427338> ;
  rdfs:subClassOf <https://w3id.org/con-tax/components/aat-furn#300037680> ;
.
<https://w3id.org/con-tax/components/aat-furn#300427398>
  rdf:type owl:Class ;
  rdfs:isDefinedBy <https://w3id.org/con-tax/components/aat-furn> ;
  rdfs:label "mess table"@en ;
  rdfs:seeAlso <http://vocab.getty.edu/aat/300427398> ;
  rdfs:subClassOf <https://w3id.org/con-tax/components/aat-furn#300039337> ;
.
<https://w3id.org/con-tax/components/aat-furn#300427644>
  rdf:type owl:Class ;
  rdfs:isDefinedBy <https://w3id.org/con-tax/components/aat-furn> ;
  rdfs:label "jewelry cabinet"@en ;
  rdfs:seeAlso <http://vocab.getty.edu/aat/300427644> ;
  rdfs:subClassOf <https://w3id.org/con-tax/components/aat-furn#300037680> ;
.
<https://w3id.org/con-tax/components/aat-furn#300427666>
  rdf:type owl:Class ;
  rdfs:isDefinedBy <https://w3id.org/con-tax/components/aat-furn> ;
  rdfs:label "joggling board"@en ;
  rdfs:seeAlso <http://vocab.getty.edu/aat/300427666> ;
  rdfs:subClassOf <https://w3id.org/con-tax/components/aat-furn#300037769> ;
.
<https://w3id.org/con-tax/components/aat-furn#300427741>
  rdf:type owl:Class ;
  rdfs:isDefinedBy <https://w3id.org/con-tax/components/aat-furn> ;
  rdfs:label "key cabinet"@en ;
  rdfs:seeAlso <http://vocab.getty.edu/aat/300427741> ;
  rdfs:subClassOf <https://w3id.org/con-tax/components/aat-furn#300037680> ;
.
<https://w3id.org/con-tax/components/aat-furn#300427791>
  rdf:type owl:Class ;
  rdfs:isDefinedBy <https://w3id.org/con-tax/components/aat-furn> ;
  rdfs:label "kitchen cabinet"@en ;
  rdfs:seeAlso <http://vocab.getty.edu/aat/300427791> ;
  rdfs:subClassOf <https://w3id.org/con-tax/components/aat-furn#300037680> ;
.
<https://w3id.org/con-tax/components/aat-furn#300427793>
  rdf:type owl:Class ;
  rdfs:isDefinedBy <https://w3id.org/con-tax/components/aat-furn> ;
  rdfs:label "kitchen dresser"@en ;
  rdfs:seeAlso <http://vocab.getty.edu/aat/300427793> ;
  rdfs:subClassOf <https://w3id.org/con-tax/components/aat-furn#300037680> ;
.
<https://w3id.org/con-tax/components/aat-furn#300427805>
  rdf:type owl:Class ;
  rdfs:isDefinedBy <https://w3id.org/con-tax/components/aat-furn> ;
  rdfs:label "kitchen stool"@en ;
  rdfs:seeAlso <http://vocab.getty.edu/aat/300427805> ;
  rdfs:subClassOf <https://w3id.org/con-tax/components/aat-furn#300037769> ;
.
<https://w3id.org/con-tax/components/aat-furn#300428484>
  rdf:type owl:Class ;
  rdfs:isDefinedBy <https://w3id.org/con-tax/components/aat-furn> ;
  rdfs:label "mail sorting cabinet"@en ;
  rdfs:seeAlso <http://vocab.getty.edu/aat/300428484> ;
  rdfs:subClassOf <https://w3id.org/con-tax/components/aat-furn#300037680> ;
.
<https://w3id.org/con-tax/components/aat-furn#300428518>
  rdf:type owl:Class ;
  rdfs:isDefinedBy <https://w3id.org/con-tax/components/aat-furn> ;
  rdfs:label "manicure table"@en ;
  rdfs:seeAlso <http://vocab.getty.edu/aat/300428518> ;
  rdfs:subClassOf <https://w3id.org/con-tax/components/aat-furn#300039337> ;
.
<https://w3id.org/con-tax/components/aat-furn#300428622>
  rdf:type owl:Class ;
  rdfs:isDefinedBy <https://w3id.org/con-tax/components/aat-furn> ;
  rdfs:label "massage chair"@en ;
  rdfs:seeAlso <http://vocab.getty.edu/aat/300428622> ;
  rdfs:subClassOf <https://w3id.org/con-tax/components/aat-furn#300037769> ;
.
<https://w3id.org/con-tax/components/aat-furn#300428893>
  rdf:type owl:Class ;
  rdfs:isDefinedBy <https://w3id.org/con-tax/components/aat-furn> ;
  rdfs:label "park bench"@en ;
  rdfs:seeAlso <http://vocab.getty.edu/aat/300428893> ;
  rdfs:subClassOf <https://w3id.org/con-tax/components/aat-furn#300037769> ;
.
<https://w3id.org/con-tax/components/aat-furn#300428904>
  rdf:type owl:Class ;
  rdfs:isDefinedBy <https://w3id.org/con-tax/components/aat-furn> ;
  rdfs:label "parsons table"@en ;
  rdfs:seeAlso <http://vocab.getty.edu/aat/300428904> ;
  rdfs:subClassOf <https://w3id.org/con-tax/components/aat-furn#300039337> ;
.
<https://w3id.org/con-tax/components/aat-furn#300428946>
  rdf:type owl:Class ;
  rdfs:isDefinedBy <https://w3id.org/con-tax/components/aat-furn> ;
  rdfs:label "patio chair"@en ;
  rdfs:seeAlso <http://vocab.getty.edu/aat/300428946> ;
  rdfs:subClassOf <https://w3id.org/con-tax/components/aat-furn#300037769> ;
.
<https://w3id.org/con-tax/components/aat-furn#300428947>
  rdf:type owl:Class ;
  rdfs:isDefinedBy <https://w3id.org/con-tax/components/aat-furn> ;
  rdfs:label "patio table"@en ;
  rdfs:seeAlso <http://vocab.getty.edu/aat/300428947> ;
  rdfs:subClassOf <https://w3id.org/con-tax/components/aat-furn#300039337> ;
.
<https://w3id.org/con-tax/components/aat-furn#300428993>
  rdf:type owl:Class ;
  rdfs:isDefinedBy <https://w3id.org/con-tax/components/aat-furn> ;
  rdfs:label "pedestal stands"@en ;
  rdfs:seeAlso <http://vocab.getty.edu/aat/300428993> ;
  rdfs:subClassOf <https://w3id.org/con-tax/components/aat-furn#300039337> ;
.
<https://w3id.org/con-tax/components/aat-furn#300429683>
  rdf:type owl:Class ;
  rdfs:isDefinedBy <https://w3id.org/con-tax/components/aat-furn> ;
  rdfs:label "office cabinet"@en ;
  rdfs:seeAlso <http://vocab.getty.edu/aat/300429683> ;
  rdfs:subClassOf <https://w3id.org/con-tax/components/aat-furn#300037680> ;
.
<https://w3id.org/con-tax/components/aat-furn#300429935>
  rdf:type owl:Class ;
  rdfs:isDefinedBy <https://w3id.org/con-tax/components/aat-furn> ;
  rdfs:label "restaurant booth"@en ;
  rdfs:seeAlso <http://vocab.getty.edu/aat/300429935> ;
  rdfs:subClassOf <https://w3id.org/con-tax/components/aat-furn#300037769> ;
.
<https://w3id.org/con-tax/components/aat-furn#300429936>
  rdf:type owl:Class ;
  rdfs:isDefinedBy <https://w3id.org/con-tax/components/aat-furn> ;
  rdfs:label "restaurant table"@en ;
  rdfs:seeAlso <http://vocab.getty.edu/aat/300429936> ;
  rdfs:subClassOf <https://w3id.org/con-tax/components/aat-furn#300039337> ;
.
<https://w3id.org/con-tax/components/aat-furn#300430180>
  rdf:type owl:Class ;
  rdfs:isDefinedBy <https://w3id.org/con-tax/components/aat-furn> ;
  rdfs:label "phonograph cabinet"@en ;
  rdfs:seeAlso <http://vocab.getty.edu/aat/300430180> ;
  rdfs:subClassOf <https://w3id.org/con-tax/components/aat-furn#300037680> ;
.
<https://w3id.org/con-tax/components/aat-furn#300430240>
  rdf:type owl:Class ;
  rdfs:comment "Stools for a pianist to sit on, usually adjustable and often with a space inside for storing music"@en ;
  rdfs:isDefinedBy <https://w3id.org/con-tax/components/aat-furn> ;
  rdfs:label "piano stools"@en ;
  rdfs:seeAlso <http://vocab.getty.edu/aat/300430240> ;
  rdfs:subClassOf <https://w3id.org/con-tax/components/aat-furn#300038450> ;
.
<https://w3id.org/con-tax/components/aat-furn#300430533>
  rdf:type owl:Class ;
  rdfs:isDefinedBy <https://w3id.org/con-tax/components/aat-furn> ;
  rdfs:label "podium"@en ;
  rdfs:seeAlso <http://vocab.getty.edu/aat/300430533> ;
  rdfs:subClassOf <https://w3id.org/con-tax/components/aat-furn#300039337> ;
.
<https://w3id.org/con-tax/components/aat-furn#300430618>
  rdf:type owl:Class ;
  rdfs:isDefinedBy <https://w3id.org/con-tax/components/aat-furn> ;
  rdfs:label "porch glider"@en ;
  rdfs:seeAlso <http://vocab.getty.edu/aat/300430618> ;
  rdfs:subClassOf <https://w3id.org/con-tax/components/aat-furn#300037769> ;
.
<https://w3id.org/con-tax/components/aat-furn#300430619>
  rdf:type owl:Class ;
  rdfs:isDefinedBy <https://w3id.org/con-tax/components/aat-furn> ;
  rdfs:label "porch swing"@en ;
  rdfs:seeAlso <http://vocab.getty.edu/aat/300430619> ;
  rdfs:subClassOf <https://w3id.org/con-tax/components/aat-furn#300037769> ;
.
<https://w3id.org/con-tax/components/aat-furn#300430709>
  rdf:type owl:Class ;
  rdfs:isDefinedBy <https://w3id.org/con-tax/components/aat-furn> ;
  rdfs:label "potty chair"@en ;
  rdfs:seeAlso <http://vocab.getty.edu/aat/300430709> ;
  rdfs:subClassOf <https://w3id.org/con-tax/components/aat-furn#300037769> ;
.
<https://w3id.org/con-tax/components/aat-furn#300430821>
  rdf:type owl:Class ;
  rdfs:isDefinedBy <https://w3id.org/con-tax/components/aat-furn> ;
  rdfs:label "printer stand"@en ;
  rdfs:seeAlso <http://vocab.getty.edu/aat/300430821> ;
  rdfs:subClassOf <https://w3id.org/con-tax/components/aat-furn#300039337> ;
.
<https://w3id.org/con-tax/components/aat-furn#300431242>
  rdf:type owl:Class ;
  rdfs:isDefinedBy <https://w3id.org/con-tax/components/aat-furn> ;
  rdfs:label "towel stand"@en ;
  rdfs:seeAlso <http://vocab.getty.edu/aat/300431242> ;
  rdfs:subClassOf <https://w3id.org/con-tax/components/aat-furn#300039337> ;
.
<https://w3id.org/con-tax/components/aat-furn#300431491>
  rdf:type owl:Class ;
  rdfs:isDefinedBy <https://w3id.org/con-tax/components/aat-furn> ;
  rdfs:label "school desk"@en ;
  rdfs:seeAlso <http://vocab.getty.edu/aat/300431491> ;
  rdfs:subClassOf <https://w3id.org/con-tax/components/aat-furn#300037680> ;
.
<https://w3id.org/con-tax/components/aat-furn#300431770>
  rdf:type owl:Class ;
  rdfs:isDefinedBy <https://w3id.org/con-tax/components/aat-furn> ;
  rdfs:label "sectional sofa"@en ;
  rdfs:seeAlso <http://vocab.getty.edu/aat/300431770> ;
  rdfs:subClassOf <https://w3id.org/con-tax/components/aat-furn#300037769> ;
.
<https://w3id.org/con-tax/components/aat-furn#300431844>
  rdf:type owl:Class ;
  rdfs:isDefinedBy <https://w3id.org/con-tax/components/aat-furn> ;
  rdfs:label "serving bar"@en ;
  rdfs:seeAlso <http://vocab.getty.edu/aat/300431844> ;
  rdfs:subClassOf <https://w3id.org/con-tax/components/aat-furn#300037680> ;
.
<https://w3id.org/con-tax/components/aat-furn#300431885>
  rdf:type owl:Class ;
  rdfs:isDefinedBy <https://w3id.org/con-tax/components/aat-furn> ;
  rdfs:label "sewing chest"@en ;
  rdfs:seeAlso <http://vocab.getty.edu/aat/300431885> ;
  rdfs:subClassOf <https://w3id.org/con-tax/components/aat-furn#300037680> ;
.
<https://w3id.org/con-tax/components/aat-furn#300431893>
  rdf:type owl:Class ;
  rdfs:comment "Work tables specifically used for sewing."@en ;
  rdfs:isDefinedBy <https://w3id.org/con-tax/components/aat-furn> ;
  rdfs:label "sewing tables"@en ;
  rdfs:seeAlso <http://vocab.getty.edu/aat/300431893> ;
  rdfs:subClassOf <https://w3id.org/con-tax/components/aat-furn#300039900> ;
.
<https://w3id.org/con-tax/components/aat-furn#300431945>
  rdf:type owl:Class ;
  rdfs:isDefinedBy <https://w3id.org/con-tax/components/aat-furn> ;
  rdfs:label "typing chair"@en ;
  rdfs:seeAlso <http://vocab.getty.edu/aat/300431945> ;
  rdfs:subClassOf <https://w3id.org/con-tax/components/aat-furn#300037769> ;
.
<https://w3id.org/con-tax/components/aat-furn#300432396>
  rdf:type owl:Class ;
  rdfs:isDefinedBy <https://w3id.org/con-tax/components/aat-furn> ;
  rdfs:label "shoeshine chair"@en ;
  rdfs:seeAlso <http://vocab.getty.edu/aat/300432396> ;
  rdfs:subClassOf <https://w3id.org/con-tax/components/aat-furn#300037769> ;
.
<https://w3id.org/con-tax/components/aat-furn#300432716>
  rdf:type owl:Class ;
  rdfs:isDefinedBy <https://w3id.org/con-tax/components/aat-furn> ;
  rdfs:label "weapon cabinet"@en ;
  rdfs:seeAlso <http://vocab.getty.edu/aat/300432716> ;
  rdfs:subClassOf <https://w3id.org/con-tax/components/aat-furn#300037680> ;
.
<https://w3id.org/con-tax/components/aat-furn#300433038>
  rdf:type owl:Class ;
  rdfs:isDefinedBy <https://w3id.org/con-tax/components/aat-furn> ;
  rdfs:label "window bench"@en ;
  rdfs:seeAlso <http://vocab.getty.edu/aat/300433038> ;
  rdfs:subClassOf <https://w3id.org/con-tax/components/aat-furn#300037769> ;
.
<https://w3id.org/con-tax/components/aat-furn#300433074>
  rdf:type owl:Class ;
  rdfs:isDefinedBy <https://w3id.org/con-tax/components/aat-furn> ;
  rdfs:label "smoking cabinet"@en ;
  rdfs:seeAlso <http://vocab.getty.edu/aat/300433074> ;
  rdfs:subClassOf <https://w3id.org/con-tax/components/aat-furn#300037680> ;
.
<https://w3id.org/con-tax/components/aat-furn#300433219>
  rdf:type owl:Class ;
  rdfs:comment "Racks comprising a frame with compartments for holding bottles of wine."@en ;
  rdfs:isDefinedBy <https://w3id.org/con-tax/components/aat-furn> ;
  rdfs:label "wine racks"@en ;
  rdfs:seeAlso <http://vocab.getty.edu/aat/300433219> ;
  rdfs:subClassOf <https://w3id.org/con-tax/components/aat-furn#300039337> ;
.
<https://w3id.org/con-tax/components/aat-furn#300434514>
  rdf:type owl:Class ;
  rdfs:isDefinedBy <https://w3id.org/con-tax/components/aat-furn> ;
  rdfs:label "television stand"@en ;
  rdfs:seeAlso <http://vocab.getty.edu/aat/300434514> ;
  rdfs:subClassOf <https://w3id.org/con-tax/components/aat-furn#300039337> ;
.
<https://w3id.org/con-tax/components/aat-furn#300434611>
  rdf:type owl:Class ;
  rdfs:isDefinedBy <https://w3id.org/con-tax/components/aat-furn> ;
  rdfs:label "theater seat"@en ;
  rdfs:seeAlso <http://vocab.getty.edu/aat/300434611> ;
  rdfs:subClassOf <https://w3id.org/con-tax/components/aat-furn#300037769> ;
.
<https://w3id.org/con-tax/components/aat-furn#300435389>
  rdf:type owl:Class ;
  rdfs:comment "Racks for holding or storing sheet music."@en ;
  rdfs:isDefinedBy <https://w3id.org/con-tax/components/aat-furn> ;
  rdfs:label "music racks"@en ;
  rdfs:seeAlso <http://vocab.getty.edu/aat/300435389> ;
  rdfs:subClassOf <https://w3id.org/con-tax/components/aat-furn#300039337> ;
.
<https://w3id.org/con-tax/components/aat-furn#300435395>
  rdf:type owl:Class ;
  rdfs:comment "Racks of various designs used to hang clothing, linen, or other household fabrics for drying or airing."@en ;
  rdfs:isDefinedBy <https://w3id.org/con-tax/components/aat-furn> ;
  rdfs:label "drying racks (support furniture, laundry )"@en ;
  rdfs:seeAlso <http://vocab.getty.edu/aat/300435395> ;
  rdfs:subClassOf <https://w3id.org/con-tax/components/aat-furn#300039337> ;
.
<https://w3id.org/con-tax/components/aat-furn#300435514>
  rdf:type owl:Class ;
  rdfs:comment "Earlier iterations of ironing boards that existed in table form, originally patented in 1858. Improved design occurred in the 1890s. "@en ;
  rdfs:isDefinedBy <https://w3id.org/con-tax/components/aat-furn> ;
  rdfs:label "ironing tables"@en ;
  rdfs:seeAlso <http://vocab.getty.edu/aat/300435514> ;
  rdfs:subClassOf <https://w3id.org/con-tax/components/aat-furn#300039734> ;
.
<https://w3id.org/con-tax/components/aat-furn#300435628>
  rdf:type owl:Class ;
  rdfs:comment "Chairs, often reclining, for use outdoors in garden areas or on lawns. "@en ;
  rdfs:isDefinedBy <https://w3id.org/con-tax/components/aat-furn> ;
  rdfs:label "lawn chairs"@en ;
  rdfs:seeAlso <http://vocab.getty.edu/aat/300435628> ;
  rdfs:subClassOf <https://w3id.org/con-tax/components/aat-furn#300037772> ;
.
<https://w3id.org/con-tax/components/aat-furn#300435629>
  rdf:type gvp:GuideTerm ;
  rdfs:isDefinedBy <https://w3id.org/con-tax/components/aat-furn> ;
  rdfs:label "<temporary alphabetical list: seating furniture>"@en ;
  rdfs:seeAlso <http://vocab.getty.edu/aat/300435629> ;
  contax:containsConcept <https://w3id.org/con-tax/components/aat-furn#300420664> ;
  contax:containsConcept <https://w3id.org/con-tax/components/aat-furn#300421184> ;
  contax:containsConcept <https://w3id.org/con-tax/components/aat-furn#300423083> ;
  contax:containsConcept <https://w3id.org/con-tax/components/aat-furn#300423204> ;
  contax:containsConcept <https://w3id.org/con-tax/components/aat-furn#300424776> ;
  contax:containsConcept <https://w3id.org/con-tax/components/aat-furn#300425516> ;
  contax:containsConcept <https://w3id.org/con-tax/components/aat-furn#300425796> ;
  contax:containsConcept <https://w3id.org/con-tax/components/aat-furn#300426144> ;
  contax:containsConcept <https://w3id.org/con-tax/components/aat-furn#300426554> ;
  contax:containsConcept <https://w3id.org/con-tax/components/aat-furn#300427666> ;
  contax:containsConcept <https://w3id.org/con-tax/components/aat-furn#300427805> ;
  contax:containsConcept <https://w3id.org/con-tax/components/aat-furn#300428622> ;
  contax:containsConcept <https://w3id.org/con-tax/components/aat-furn#300428893> ;
  contax:containsConcept <https://w3id.org/con-tax/components/aat-furn#300428946> ;
  contax:containsConcept <https://w3id.org/con-tax/components/aat-furn#300429935> ;
  contax:containsConcept <https://w3id.org/con-tax/components/aat-furn#300430618> ;
  contax:containsConcept <https://w3id.org/con-tax/components/aat-furn#300430619> ;
  contax:containsConcept <https://w3id.org/con-tax/components/aat-furn#300430709> ;
  contax:containsConcept <https://w3id.org/con-tax/components/aat-furn#300431770> ;
  contax:containsConcept <https://w3id.org/con-tax/components/aat-furn#300431945> ;
  contax:containsConcept <https://w3id.org/con-tax/components/aat-furn#300432396> ;
  contax:containsConcept <https://w3id.org/con-tax/components/aat-furn#300433038> ;
  contax:containsConcept <https://w3id.org/con-tax/components/aat-furn#300434611> ;
.
<https://w3id.org/con-tax/components/aat-furn#300435632>
  rdf:type gvp:GuideTerm ;
  rdfs:isDefinedBy <https://w3id.org/con-tax/components/aat-furn> ;
  rdfs:label "<temporary alphabetical list: sleeping and reclining furniture>"@en ;
  rdfs:seeAlso <http://vocab.getty.edu/aat/300435632> ;
  contax:containsConcept <https://w3id.org/con-tax/components/aat-furn#300422971> ;
  contax:containsConcept <https://w3id.org/con-tax/components/aat-furn#300423082> ;
  contax:containsConcept <https://w3id.org/con-tax/components/aat-furn#300424703> ;
.
<https://w3id.org/con-tax/components/aat-furn#300435638>
  rdf:type gvp:GuideTerm ;
  rdfs:isDefinedBy <https://w3id.org/con-tax/components/aat-furn> ;
  rdfs:label "<temporary alphabetical list: storage and display furniture>"@en ;
  rdfs:seeAlso <http://vocab.getty.edu/aat/300435638> ;
  contax:containsConcept <https://w3id.org/con-tax/components/aat-furn#300420253> ;
  contax:containsConcept <https://w3id.org/con-tax/components/aat-furn#300420742> ;
  contax:containsConcept <https://w3id.org/con-tax/components/aat-furn#300421477> ;
  contax:containsConcept <https://w3id.org/con-tax/components/aat-furn#300422209> ;
  contax:containsConcept <https://w3id.org/con-tax/components/aat-furn#300422652> ;
  contax:containsConcept <https://w3id.org/con-tax/components/aat-furn#300423429> ;
  contax:containsConcept <https://w3id.org/con-tax/components/aat-furn#300424190> ;
  contax:containsConcept <https://w3id.org/con-tax/components/aat-furn#300425131> ;
  contax:containsConcept <https://w3id.org/con-tax/components/aat-furn#300426805> ;
  contax:containsConcept <https://w3id.org/con-tax/components/aat-furn#300427338> ;
  contax:containsConcept <https://w3id.org/con-tax/components/aat-furn#300427644> ;
  contax:containsConcept <https://w3id.org/con-tax/components/aat-furn#300427741> ;
  contax:containsConcept <https://w3id.org/con-tax/components/aat-furn#300427791> ;
  contax:containsConcept <https://w3id.org/con-tax/components/aat-furn#300427793> ;
  contax:containsConcept <https://w3id.org/con-tax/components/aat-furn#300428484> ;
  contax:containsConcept <https://w3id.org/con-tax/components/aat-furn#300429683> ;
  contax:containsConcept <https://w3id.org/con-tax/components/aat-furn#300430180> ;
  contax:containsConcept <https://w3id.org/con-tax/components/aat-furn#300431491> ;
  contax:containsConcept <https://w3id.org/con-tax/components/aat-furn#300431844> ;
  contax:containsConcept <https://w3id.org/con-tax/components/aat-furn#300431885> ;
  contax:containsConcept <https://w3id.org/con-tax/components/aat-furn#300432716> ;
  contax:containsConcept <https://w3id.org/con-tax/components/aat-furn#300433074> ;
.
<https://w3id.org/con-tax/components/aat-furn#300435640>
  rdf:type gvp:GuideTerm ;
  rdfs:isDefinedBy <https://w3id.org/con-tax/components/aat-furn> ;
  rdfs:label "<temporary alphabetical list: support furniture>"@en ;
  rdfs:seeAlso <http://vocab.getty.edu/aat/300435640> ;
  contax:containsConcept <https://w3id.org/con-tax/components/aat-furn#300420268> ;
  contax:containsConcept <https://w3id.org/con-tax/components/aat-furn#300420822> ;
  contax:containsConcept <https://w3id.org/con-tax/components/aat-furn#300421391> ;
  contax:containsConcept <https://w3id.org/con-tax/components/aat-furn#300421906> ;
  contax:containsConcept <https://w3id.org/con-tax/components/aat-furn#300422207> ;
  contax:containsConcept <https://w3id.org/con-tax/components/aat-furn#300422732> ;
  contax:containsConcept <https://w3id.org/con-tax/components/aat-furn#300423001> ;
  contax:containsConcept <https://w3id.org/con-tax/components/aat-furn#300424798> ;
  contax:containsConcept <https://w3id.org/con-tax/components/aat-furn#300425717> ;
  contax:containsConcept <https://w3id.org/con-tax/components/aat-furn#300427302> ;
  contax:containsConcept <https://w3id.org/con-tax/components/aat-furn#300427398> ;
  contax:containsConcept <https://w3id.org/con-tax/components/aat-furn#300428518> ;
  contax:containsConcept <https://w3id.org/con-tax/components/aat-furn#300428904> ;
  contax:containsConcept <https://w3id.org/con-tax/components/aat-furn#300428947> ;
  contax:containsConcept <https://w3id.org/con-tax/components/aat-furn#300428993> ;
  contax:containsConcept <https://w3id.org/con-tax/components/aat-furn#300429936> ;
  contax:containsConcept <https://w3id.org/con-tax/components/aat-furn#300430533> ;
  contax:containsConcept <https://w3id.org/con-tax/components/aat-furn#300430821> ;
  contax:containsConcept <https://w3id.org/con-tax/components/aat-furn#300431242> ;
  contax:containsConcept <https://w3id.org/con-tax/components/aat-furn#300434514> ;
.
<https://w3id.org/con-tax/components/aat-furn#300438648>
  rdf:type owl:Class ;
  rdfs:comment "Handiwork table of a distinctive style, having four slender legs and a deep body set with several drawers; typically used for sewing."@en ;
  rdfs:isDefinedBy <https://w3id.org/con-tax/components/aat-furn> ;
  rdfs:label "Martha Washington tables"@en ;
  rdfs:seeAlso <http://vocab.getty.edu/aat/300438648> ;
  rdfs:subClassOf <https://w3id.org/con-tax/components/aat-furn#300431893> ;
.
<https://w3id.org/con-tax/components/aat-furn#300438649>
  rdf:type owl:Class ;
  rdfs:comment "Small, light work tables with one or two drawers, the lower of which forms a frame from which is suspended a bag for needlework."@en ;
  rdfs:isDefinedBy <https://w3id.org/con-tax/components/aat-furn> ;
  rdfs:label "bag tables"@en ;
  rdfs:seeAlso <http://vocab.getty.edu/aat/300438649> ;
  rdfs:subClassOf <https://w3id.org/con-tax/components/aat-furn#300431893> ;
.
<https://w3id.org/con-tax/components/aat-furn#300438650>
  rdf:type owl:Class ;
  rdfs:comment "Sturdy tables of relatively substantial size, used for various tasks, from kitchen work to carpentry or other heavy work. For table-like structures of waist height, typically used for heavy work while standing, prefer \"work benches.\""@en ;
  rdfs:isDefinedBy <https://w3id.org/con-tax/components/aat-furn> ;
  rdfs:label "work tables (larger tables)"@en ;
  rdfs:seeAlso <http://vocab.getty.edu/aat/300438650> ;
  rdfs:subClassOf <https://w3id.org/con-tax/components/aat-furn#300039548> ;
.
<https://w3id.org/con-tax/components/aat-furn#300438673>
  rdf:type owl:Class ;
  rdfs:comment "Small three-legged tables or stands; also, table-like stands for tea caddies. The term is of Anglo-Indian origin, originally from the Hindu word \"tepai\" for tripod. From ca. 1810, the term was used specifically for small tables used to support tea caddies or tea chests, whether or not the table had three legs. Teapoys were often fitted with various compartments for storing tea. The stand may be one with, or dettachable from, the tea chest or caddy."@en ;
  rdfs:isDefinedBy <https://w3id.org/con-tax/components/aat-furn> ;
  rdfs:label "teapoys"@en ;
  rdfs:seeAlso <http://vocab.getty.edu/aat/300438673> ;
  rdfs:subClassOf <https://w3id.org/con-tax/components/aat-furn#300039548> ;
  rdfs:subClassOf <https://w3id.org/con-tax/components/aat-furn#300039886> ;
.
<https://w3id.org/con-tax/components/aat-furn#300438674>
  rdf:type owl:Class ;
  rdfs:comment "Tables having an ornamental parapet or railing running along the edge."@en ;
  rdfs:isDefinedBy <https://w3id.org/con-tax/components/aat-furn> ;
  rdfs:label "galleried tables"@en ;
  rdfs:seeAlso <http://vocab.getty.edu/aat/300438674> ;
  rdfs:subClassOf <https://w3id.org/con-tax/components/aat-furn#300121537> ;
.
<https://w3id.org/con-tax/components/aat-furn#300438676>
  rdf:type owl:Class ;
  rdfs:comment "Tables intended for use in dining at special occasions; may be large and elaborate in design."@en ;
  rdfs:isDefinedBy <https://w3id.org/con-tax/components/aat-furn> ;
  rdfs:label "banquet tables"@en ;
  rdfs:seeAlso <http://vocab.getty.edu/aat/300438676> ;
  rdfs:subClassOf <https://w3id.org/con-tax/components/aat-furn#300039648> ;
.
<https://w3id.org/con-tax/components/aat-furn#300438677>
  rdf:type owl:Class ;
  rdfs:comment "Relatively small cases of cabinet-work made to hold wine bottles. They may be lined with lead or another water-impervious material, in order to hold cold water or ice. For larger pieces of case furniture used to hold wine or other alcohol, prefer \"cellaret sideboards.\""@en ;
  rdfs:isDefinedBy <https://w3id.org/con-tax/components/aat-furn> ;
  rdfs:label "wine cellarets (wine chests)"@en ;
  rdfs:seeAlso <http://vocab.getty.edu/aat/300438677> ;
  rdfs:subClassOf <https://w3id.org/con-tax/components/aat-furn#300038978> ;
.
<https://w3id.org/con-tax/components/aat-furn#300438680>
  rdf:type owl:Class ;
  rdfs:comment "Étagères and similar shelved stands intended to hold potted flowers, sometimes other small plants."@en ;
  rdfs:isDefinedBy <https://w3id.org/con-tax/components/aat-furn> ;
  rdfs:label "flower étagères"@en ;
  rdfs:seeAlso <http://vocab.getty.edu/aat/300438680> ;
  rdfs:subClassOf <https://w3id.org/con-tax/components/aat-furn#300039300> ;
  rdfs:subClassOf <https://w3id.org/con-tax/components/aat-furn#300039835> ;
.
<https://w3id.org/con-tax/components/aat-furn#300438681>
  rdf:type owl:Class ;
  rdfs:comment "Stands intended specfically to hold flowers, usually cut flowers. May be small table-top items or larger stands, used for decoration or for selling flowers."@en ;
  rdfs:isDefinedBy <https://w3id.org/con-tax/components/aat-furn> ;
  rdfs:label "flower stands"@en ;
  rdfs:seeAlso <http://vocab.getty.edu/aat/300438681> ;
  rdfs:subClassOf <https://w3id.org/con-tax/components/aat-furn#300039835> ;
.
<https://w3id.org/con-tax/components/aat-furn#300438682>
  rdf:type owl:Class ;
  rdfs:comment "Small tables or tall stands intended to hold bouquets of flowers in decorative vessels."@en ;
  rdfs:isDefinedBy <https://w3id.org/con-tax/components/aat-furn> ;
  rdfs:label "flower tables"@en ;
  rdfs:seeAlso <http://vocab.getty.edu/aat/300438682> ;
  rdfs:subClassOf <https://w3id.org/con-tax/components/aat-furn#300039835> ;
.
<https://w3id.org/con-tax/components/aat-furn#300438683>
  rdf:type owl:Class ;
  rdfs:comment "Dressing tables, usually relatively small, having an attached mirror and usually a matching seat."@en ;
  rdfs:isDefinedBy <https://w3id.org/con-tax/components/aat-furn> ;
  rdfs:label "vanities"@en ;
  rdfs:seeAlso <http://vocab.getty.edu/aat/300438683> ;
  rdfs:subClassOf <https://w3id.org/con-tax/components/aat-furn#300039668> ;
.
<https://w3id.org/con-tax/components/aat-furn#300438690>
  rdf:type owl:Class ;
  rdfs:comment "Tables having tops marked with a checkerboard pattern of 64 squares for the purpose of playing the game of checkers. Chess may also be played on the same board. Traditionally, checkerboards will comprise alternating black and red squares, although any contrasting colors may be used."@en ;
  rdfs:isDefinedBy <https://w3id.org/con-tax/components/aat-furn> ;
  rdfs:label "checker tables"@en ;
  rdfs:seeAlso <http://vocab.getty.edu/aat/300438690> ;
  rdfs:subClassOf <https://w3id.org/con-tax/components/aat-furn#300039694> ;
.
<https://w3id.org/con-tax/components/aat-furn#300438693>
  rdf:type owl:Class ;
  rdfs:comment "Narrow tables, often with a mirror, generally situated near the front door of a home; may be in a hallway or vestibule, may be adjacent to a hat rack or coat rack."@en ;
  rdfs:isDefinedBy <https://w3id.org/con-tax/components/aat-furn> ;
  rdfs:label "hall tables (entryway tables)"@en ;
  rdfs:seeAlso <http://vocab.getty.edu/aat/300438693> ;
  rdfs:subClassOf <https://w3id.org/con-tax/components/aat-furn#300039548> ;
.
<https://w3id.org/con-tax/components/aat-furn#300438694>
  rdf:type owl:Class ;
  rdfs:comment "Large tables situated in the main room or great hall of a manor house or other large, stately home."@en ;
  rdfs:isDefinedBy <https://w3id.org/con-tax/components/aat-furn> ;
  rdfs:label "great tables"@en ;
  rdfs:seeAlso <http://vocab.getty.edu/aat/300438694> ;
  rdfs:subClassOf <https://w3id.org/con-tax/components/aat-furn#300039548> ;
.
<https://w3id.org/con-tax/components/aat-furn#300438695>
  rdf:type owl:Class ;
  rdfs:comment "Unusally long tables used in larger homes, particularly in historical England and colonial America, for large dinner gatherings or other purposes. Typical examples were around three feet wide and 10 or 12 feet long."@en ;
  rdfs:isDefinedBy <https://w3id.org/con-tax/components/aat-furn> ;
  rdfs:label "long tables"@en ;
  rdfs:seeAlso <http://vocab.getty.edu/aat/300438695> ;
  rdfs:subClassOf <https://w3id.org/con-tax/components/aat-furn#300039548> ;
.
<https://w3id.org/con-tax/components/aat-furn#300438696>
  rdf:type owl:Class ;
  rdfs:comment "Tables constructed so that the tabletop is set upon a base or stand constructed using mortise-and-tenon joints."@en ;
  rdfs:isDefinedBy <https://w3id.org/con-tax/components/aat-furn> ;
  rdfs:label "joined tables"@en ;
  rdfs:seeAlso <http://vocab.getty.edu/aat/300438696> ;
  rdfs:subClassOf <https://w3id.org/con-tax/components/aat-furn#300039548> ;
.
